PREFIX : <https://www.ica.org/standards/RiC/ontology#>
PREFIX cc: <http://creativecommons.org/ns#>
PREFIX dc: <http://purl.org/dc/elements/1.1/>
PREFIX dcterms: <http://purl.org/dc/terms/>
PREFIX owl: <http://www.w3.org/2002/07/owl#>
PREFIX rdf: <http://www.w3.org/1999/02/22-rdf-syntax-ns#>
PREFIX rdfs: <http://www.w3.org/2000/01/rdf-schema#>
PREFIX ric-dft: <https://www.ica.org/standards/RiC/vocabularies/documentaryFormTypes#>
PREFIX ric-rst: <https://www.ica.org/standards/RiC/vocabularies/recordSetTypes#>
PREFIX skos: <http://www.w3.org/2004/02/skos/core#>
PREFIX vann: <http://purl.org/vocab/vann/>
PREFIX voaf: <http://purl.org/vocommons/voaf#>
PREFIX xsd: <http://www.w3.org/2001/XMLSchema#>

cc:license
    rdfs:isDefinedBy cc: ;
.

dc:contributor
    rdfs:isDefinedBy dc: ;
.

dc:creator
    rdfs:isDefinedBy dc: ;
.

dc:date
    rdfs:isDefinedBy dc: ;
.

dc:language
    rdfs:isDefinedBy dc: ;
.

dc:publisher
    rdfs:isDefinedBy dc: ;
.

dc:rights
    rdfs:isDefinedBy dc: ;
.

dc:title
    rdfs:isDefinedBy dc: ;
.

dcterms:abstract
    rdfs:isDefinedBy dcterms: ;
.

dcterms:contributor
    rdfs:isDefinedBy dcterms: ;
.

dcterms:creator
    rdfs:isDefinedBy dcterms: ;
.

dcterms:description
    rdfs:isDefinedBy dcterms: ;
.

dcterms:publisher
    rdfs:isDefinedBy dcterms: ;
.

dcterms:rights
    rdfs:isDefinedBy dcterms: ;
.

dcterms:title
    rdfs:isDefinedBy dcterms: ;
.

vann:preferredNamespacePrefix
    a owl:AnnotationProperty ;
    rdfs:isDefinedBy vann: ;
.

vann:preferredNamespaceUri
    a owl:AnnotationProperty ;
    rdfs:isDefinedBy vann: ;
.

rdf:value
    rdfs:isDefinedBy rdf: ;
.

skos:changeNote
    a owl:AnnotationProperty ;
    rdfs:isDefinedBy <http://www.w3.org/2004/02/skos/core> ;
    rdfs:subPropertyOf skos:note ;
.

skos:definition
    a owl:AnnotationProperty ;
    rdfs:isDefinedBy <http://www.w3.org/2004/02/skos/core> ;
    rdfs:subPropertyOf skos:note ;
.

skos:example
    a owl:AnnotationProperty ;
    rdfs:isDefinedBy <http://www.w3.org/2004/02/skos/core> ;
    rdfs:subPropertyOf skos:note ;
.

skos:historyNote
    a owl:AnnotationProperty ;
    rdfs:isDefinedBy <http://www.w3.org/2004/02/skos/core> ;
    rdfs:subPropertyOf skos:note ;
.

skos:inScheme
    a owl:ObjectProperty ;
    rdfs:isDefinedBy <http://www.w3.org/2004/02/skos/core> ;
.

skos:scopeNote
    a owl:AnnotationProperty ;
    rdfs:isDefinedBy <http://www.w3.org/2004/02/skos/core> ;
    rdfs:subPropertyOf skos:note ;
.

:CarrierExtent
    a owl:Class ;
    rdfs:label
        "Carrier Extent"@en ,
        "Extensión del soporte"@es ,
        "Mesure d’un support"@fr ;
    rdfs:comment """Number of physical units and/or physical dimensions of the carrier
         of an Instantiation."""@en ;
    rdfs:isDefinedBy <https://www.ica.org/standards/RiC/ontology> ;
    rdfs:subClassOf :Extent ;
    skos:changeNote
        [
            dc:date "2023-08-25" ;
            rdf:value "Added a new rdfs:label in French."@en ;
        ] ,
        [
            dc:date "2020-11-21" ;
            rdf:value """Changed a bit the definition and added change
               notes."""@en ;
        ] ,
        [
            dc:date "2023-11-02" ;
            rdf:value "Added a new rdfs:label in Spanish."@en ;
        ] ,
        [
            dc:date "2023-11-12" ;
            rdf:value """Aligned with RiC-CM 1.0: updated the description
               (rdfs:comment), skos:scopeNote."""@en ;
        ] ,
        [
            dc:date "2020-10-28" ;
            rdf:value """Class added in order to handle an accurate description of a
               carrier extent"""@en ;
        ] ;
    skos:scopeNote """In order to manage an instantiation of a record resource it is
         necessary to note the extent of the carrier as well as that of the instantiation itself.
         Whether it is necessary to note dimensions, the number of relevant units or both depends on
         the nature of the carrier and particular business needs."""@en ;
    :RiCCMCorrespondingComponent """Class implementation of RiC-A04 (Carrier Extent)
         attribute"""@en ;
.

:InstantiationExtent
    a owl:Class ;
    rdfs:label
        "Instantiation Extent"@en ,
        "Extensión de la instanciación"@es ,
        "Mesure d’une instanciation"@fr ;
    rdfs:comment """Countable characteristics of an Instantiation expressed as a
         quantity."""@en ;
    rdfs:isDefinedBy <https://www.ica.org/standards/RiC/ontology> ;
    rdfs:subClassOf :Extent ;
    skos:changeNote
        [
            dc:date "2020-11-21" ;
            rdf:value """Changed a bit the definition and added change
               notes."""@en ;
        ] ,
        [
            dc:date "2023-08-25" ;
            rdf:value "Added a new rdfs:label in French."@en ;
        ] ,
        [
            dc:date "2023-11-12" ;
            rdf:value """Aligned with RiC-CM 1.0: updated the description
               (rdfs:comment)."""@en ;
        ] ,
        [
            dc:date "2023-11-02" ;
            rdf:value "Added a new rdfs:label in Spanish."@en ;
        ] ,
        [
            dc:date "2020-10-28" ;
            rdf:value """Class added in order to handle an accurate description of an
               instantiation extent"""@en ;
        ] ;
    :RiCCMCorrespondingComponent """Class implementation of RiC-A23 (Instantiation
         Extent attribute)"""@en ;
.

:RecordResourceExtent
    a owl:Class ;
    rdfs:label
        "Record Resource Extent"@en ,
        "Extensión de recurso documental"@es ,
        "Mesure d’une ressource archivistique"@fr ;
    rdfs:comment """The quantity of information content, as human experienced,
         contained in a Record Resource."""@en ;
    rdfs:isDefinedBy <https://www.ica.org/standards/RiC/ontology> ;
    rdfs:subClassOf :Extent ;
    skos:changeNote
        [
            dc:date "2020-10-28" ;
            rdf:value """Class added in order to handle an accurate description of a
               record resource extent"""@en ;
        ] ,
        [
            dc:date "2023-08-25" ;
            rdf:value "Added a new rdfs:label in French."@en ;
        ] ,
        [
            dc:date "2020-11-21" ;
            rdf:value """Changed a bit the definition and added change
               notes."""@en ;
        ] ,
        [
            dc:date "2023-11-02" ;
            rdf:value "Added a new rdfs:label in Spanish."@en ;
        ] ,
        [
            dc:date "2023-11-12" ;
            rdf:value """Aligned with RiC-CM 1.0: updated the description
               (rdfs:comment), skos:scopeNote."""@en ;
        ] ;
    skos:scopeNote """The method and precision of expressing the quantity of
         information represented in a Record Resource will vary according to the kind of record
         resource being described, processing economy constraints, etc. For Record Sets, quantity
         may be expressed as number of records, or, for analogue records in particular, by the
         physical storage dimensions of the members of the Record Set. For individual Records or
         Record Parts, quantity may be expressed in more precise terms."""@en ;
    :RiCCMCorrespondingComponent """Class implementation of RiC-A35 (Record Resource
         extent attribute)"""@en ;
.

:RiCCMCorrespondingComponent
    a owl:AnnotationProperty ;
    rdfs:label
        "RiC-CM corresponding component"@en ,
        "componente correspondiente en RiC-CM"@es ,
        "composant correspondant dans RiC-CM"@fr ;
    rdfs:comment """When it exists, specifies the identifier and name of RiC-CM
         component that corresponds to the annotated class or property."""@en ;
    rdfs:isDefinedBy <https://www.ica.org/standards/RiC/ontology> ;
    rdfs:subPropertyOf rdfs:comment ;
    skos:changeNote
        [
            dc:date "2023-11-25" ;
            rdf:value "Added a new rdfs:label in Spanish."@en ;
        ] ,
        [
            dc:date "2023-08-28" ;
            rdf:value "Added a new rdfs:label in French."@en ;
        ] ;
.

:accruals
    a owl:DatatypeProperty ;
    rdfs:label
        "accruals"@en ,
        "ingresos"@es ,
        "accroissements"@fr ;
    rdfs:comment """Information on the anticipated accession(s) to the Record
         Set."""@en ;
    rdfs:domain :RecordSet ;
    rdfs:isDefinedBy <https://www.ica.org/standards/RiC/ontology> ;
    rdfs:range rdfs:Literal ;
    skos:changeNote
        [
            dc:date "2023-11-02" ;
            rdf:value "Added a new rdfs:label in Spanish."@en ;
        ] ,
        [
            dc:date "2023-08-25" ;
            rdf:value "Added a new rdfs:label in French."@en ;
        ] ,
        [
            dc:date "2023-11-11" ;
            rdf:value """Aligned with RiC-CM 1.0: updated the IRI, mapping to RiC-CM
               (rico:RiCCMCorrespondingComponent), labels, skos:scopeNote, examples
               (skos:example)."""@en ;
        ] ;
    skos:example
        """Accruing - there is an agreement with the creator that additional
         snapshots of their email directory will be accessioned at yearly intervals"""@en ,
        "Non-accruing"@en ,
        "Unknown"@en ;
    skos:scopeNote "See also accrualsStatus"@en ;
    :RiCCMCorrespondingComponent """corresponds to RiC-A01 (Accruals
         attribute)"""@en ;
.

:accrualsStatus
    a owl:DatatypeProperty ;
    rdfs:label
        "accruals status"@en ,
        "estado de los ingresos"@es ,
        "statut des accroissements"@fr ;
    rdfs:comment "Information on the status of possible accruals"@en ;
    rdfs:domain :RecordSet ;
    rdfs:isDefinedBy <https://www.ica.org/standards/RiC/ontology> ;
    rdfs:range rdfs:Literal ;
    skos:changeNote
        [
            dc:date "2023-08-25" ;
            rdf:value "Added a new rdfs:label in French."@en ;
        ] ,
        [
            dc:date "2023-11-02" ;
            rdf:value "Added a new rdfs:label in Spanish."@en ;
        ] ,
        [
            dc:date "2020-11-01" ;
            rdf:value """scope note : updated. Objective: to make RiC-O compliant with
               RiC-CM v0.2."""@en ;
        ] ,
        [
            dc:date "2023-11-11" ;
            rdf:value """Aligned with RiC-CM 1.0: updated the IRI, mapping to RiC-CM
               (rico:RiCCMCorrespondingComponent), labels, description (rdfs:comment),
               skos:scopeNote."""@en ;
        ] ;
    skos:scopeNote """A text statement or single words such as “Closed” to indicate
         that no additional Record Resource will (or is anticipated to) be added to the Record Set;
         “Open” to indicate that additional records or record sets will (or are expected to) be
         added to the Record Set; or “Unknown” to indicate that this information is not available,
         for example. See also accruals"""@en ;
    :RiCCMCorrespondingComponent """specialization of RiC-A01 (Accruals
         attribute)"""@en ;
.

:altimetricSystem
    a owl:DatatypeProperty ;
    rdfs:label
        "altimetric system"@en ,
        "sistema altimétrico"@es ,
        "système altimétrique"@fr ;
    rdfs:comment "Reference system used for altitude"@en ;
    rdfs:domain :Coordinates ;
    rdfs:isDefinedBy <https://www.ica.org/standards/RiC/ontology> ;
    rdfs:range rdfs:Literal ;
    rdfs:subPropertyOf :referenceSystem ;
    skos:changeNote
        [
            dc:date "2023-08-25" ;
            rdf:value "Added a new rdfs:label in French."@en ;
        ] ,
        [
            dc:date "2023-11-02" ;
            rdf:value "Added a new rdfs:label in Spanish."@en ;
        ] ;
.

:altitude
    a owl:DatatypeProperty ;
    rdfs:label
        "altitude"@en ,
        "altitud"@es ,
        "altitude"@fr ;
    rdfs:comment """The height of a Place above a reference level, especially above
         sea level."""@en ;
    rdfs:domain :Coordinates ;
    rdfs:isDefinedBy <https://www.ica.org/standards/RiC/ontology> ;
    rdfs:range rdfs:Literal ;
    rdfs:subPropertyOf :measure ;
    skos:changeNote
        [
            dc:date "2023-08-25" ;
            rdf:value "Added a new rdfs:label in French."@en ;
        ] ,
        [
            dc:date "2023-11-02" ;
            rdf:value "Added a new rdfs:label in Spanish."@en ;
        ] ;
    skos:scopeNote """Property of the Coordinates class. If you don't use this class,
         use geographicalCoordinates property, a property of Place class."""@en ;
.

:authenticityNote
    a owl:DatatypeProperty ;
    rdfs:label
        "authenticity note"@en ,
        "nota de autenticidad"@es ,
        "note sur l’authenticité"@fr ;
    rdfs:comment """Description of the evidence that a Record Resource or
         Instantiation is what it purports to be, was created or sent by the said Agent at the said
         time, and has not been tampered with, corrupted, or forged. """@en ;
    rdfs:domain
        [
            a owl:Class ;
            owl:unionOf (
                :Instantiation
                :RecordResource
            ) ;
        ] ;
    rdfs:isDefinedBy <https://www.ica.org/standards/RiC/ontology> ;
    rdfs:range rdfs:Literal ;
    skos:changeNote
        [
            dc:date "2023-08-25" ;
            rdf:value "Added a new rdfs:label in French."@en ;
        ] ,
        [
            dc:date "2023-11-02" ;
            rdf:value "Added a new rdfs:label in Spanish."@en ;
        ] ,
        [
            dc:date "2020-11-01" ;
            rdf:value """examples added. Objective: to make RiC-O compliant with RiC-CM
               v0.2."""@en ;
        ] ,
        [
            dc:date "2023-11-11" ;
            rdf:value """Aligned with RiC-CM 1.0: updated the description
               (rdfs:comment), skos:scopeNote, examples (skos:example)."""@en ;
        ] ;
    skos:example
        """The deed is digitally signed by the Notary. The electronic
         signature validity cannot be assessed, but the content was not modified from the moment of
         signing."""@en ,
        "The letter is unsigned."@en ,
        "The record bears signatures."@en ,
        "The timestamp exists but cannot be verified."@en ;
    skos:scopeNote """May be used in a Record Set description when its value is shared
         by some or all members of the Record Set. For digital records, it may include results from
         automated means of checking the validity of signatures and timestamp. In particular cases
         it may be contextually related to the state attribute, for example, a document can be an
         original or a copy, either of which can be authentic or a forgery. """@en ;
    :RiCCMCorrespondingComponent """Corresponds to RiC-A03 (Authenticity Note
         attribute)"""@en ;
.

:authorizingMandate
    a owl:DatatypeProperty ;
    rdfs:label
        "authorizing mandate"@en ,
        "norma de control"@es ,
        "mandat"@fr ;
    rdfs:comment """Information on a Mandate that authorizes an Agent to perform an
         Activity."""@en ;
    rdfs:domain :Agent ;
    rdfs:isDefinedBy <https://www.ica.org/standards/RiC/ontology> ;
    rdfs:range rdfs:Literal ;
    rdfs:subPropertyOf :ruleFollowed ;
    skos:changeNote
        [
            dc:date "2023-11-02" ;
            rdf:value "Added a new rdfs:label in Spanish."@en ;
        ] ,
        [
            dc:date "2023-08-25" ;
            rdf:value "Added a new rdfs:label in French."@en ;
        ] ;
    skos:scopeNote """Provided for usability reasons. May be deprecated and removed
         later on. Use only if you don't use the Mandate class for handling
         mandates."""@en ;
.

:birthDate
    a owl:DatatypeProperty ;
    rdfs:label
        "birth date"@en ,
        "fecha de nacimiento"@es ,
        "date de naissance"@fr ;
    rdfs:comment "Date at which a Person was born."@en ;
    rdfs:domain :Person ;
    rdfs:isDefinedBy <https://www.ica.org/standards/RiC/ontology> ;
    rdfs:range rdfs:Literal ;
    rdfs:subPropertyOf :beginningDate ;
    skos:changeNote
        [
            dc:date "2023-08-25" ;
            rdf:value "Added a new rdfs:label in French."@en ;
        ] ,
        [
            dc:date "2023-11-02" ;
            rdf:value "Added a new rdfs:label in Spanish."@en ;
        ] ;
    skos:scopeNote """Provided for usability reasons. May be deprecated and removed
         later on. Use only if you don't use Date classes for handling dates."""@en ;
    :RiCCMCorrespondingComponent """Datatype property specialized implementation of
         RiC-E18 (Date entity)"""@en ;
.

:carrierExtent
    a owl:DatatypeProperty ;
    rdfs:label
        "carrier extent"@en ,
        "extensión del soporte"@es ,
        "mesure du support"@fr ;
    rdfs:comment """Number of physical units and/or physical dimensions of the carrier
         of an Instantiation. In order to manage an Instantiation of a record resource it is
         necessary to note the extent of the carrier as well as that of the Instantiation itself.
         Whether it is necessary to note dimensions, the number of relevant units, or both, depends
         on the nature of the carrier and particular business needs."""@en ;
    rdfs:domain :Instantiation ;
    rdfs:isDefinedBy <https://www.ica.org/standards/RiC/ontology> ;
    rdfs:range rdfs:Literal ;
    rdfs:subPropertyOf :physicalOrLogicalExtent ;
    skos:changeNote
        [
            dc:date "2023-11-02" ;
            rdf:value "Added a new rdfs:label in Spanish."@en ;
        ] ,
        [
            dc:date "2023-08-25" ;
            rdf:value "Added a new rdfs:label in French."@en ;
        ] ,
        [
            dc:date "2020-11-01" ;
            rdf:value """Text definition and scope note updated. Examples added.
               Objective: to make RiC-O compliant with RiC-CM v0.2."""@en ;
        ] ,
        [
            dc:date "2023-11-11" ;
            rdf:value """Aligned with RiC-CM 1.0: updated the description
               (rdfs:comment), skos:scopeNote, examples (skos:example)."""@en ;
        ] ;
    skos:example
        "1 page"@en ,
        "3 GB (1 USB key)"@en ,
        "32.5 x 49 cm (piece of parchment)"@en ;
    skos:scopeNote """For digital resources, it may be used to indicate the size of
         storage capacity (disk, tape, film, etc.). Carrier extent should not be confused with
         instantiation extent or record resource extent. For a given Record Resource, the
         instantiation extent may vary, based on format, density of information on the carrier, etc.
         For example, a CD with a storage capacity of 700 MB (carrier extent) might hold a record of
         1500 words (record resource extent) represented in two versions, one a Word document with
         an instantiation extent of 3 KB and the other a PDF file with an instantiation extent of 5
         KB. """@en ;
    :RiCCMCorrespondingComponent """Corresponds to RiC-A04 (Carrier Extent
         attribute)"""@en ;
.

:classification
    a owl:DatatypeProperty ;
    rdfs:label
        "classification"@en ,
        "clasificación"@es ,
        "classification"@fr ;
    rdfs:comment """A term, number or alphanumeric string that is usually taken from
         an external classification vocabulary or scheme that qualifies a Record Resource. """@en ;
    rdfs:domain :RecordResource ;
    rdfs:isDefinedBy <https://www.ica.org/standards/RiC/ontology> ;
    rdfs:range rdfs:Literal ;
    skos:changeNote
        [
            dc:date "2023-11-11" ;
            rdf:value """Aligned with RiC-CM 1.0: updated the description
               (rdfs:comment), skos:scopeNote, examples (skos:example)."""@en ;
        ] ,
        [
            dc:date "2023-08-25" ;
            rdf:value "Added a new rdfs:label in French."@en ;
        ] ,
        [
            dc:date "2023-11-02" ;
            rdf:value "Added a new rdfs:label in Spanish."@en ;
        ] ,
        [
            dc:date "2020-11-01" ;
            rdf:value """Text definition and scope note updated. Examples added.
               Objective: to make RiC-O compliant with RiC-CM v0.2."""@en ;
        ] ;
    skos:example
        """BUD-01-F002 (classification number from a corporate file
         plan)"""@en ,
        "digitized items"@en ,
        "financial affairs"@en ,
        "human resource management"@en ,
        "student registration"@en ;
    skos:scopeNote """May be used in a Record Set description when its value is shared
         by some or all members of the record set. This datatype property is not to be confused with
         Identifier although, in some cases, the information may be the same."""@en ;
    :RiCCMCorrespondingComponent """Corresponds to RiC-A07 (Classification
         attribute)"""@en ;
.

:closeTo
    a owl:AnnotationProperty ;
    rdfs:label
        "close to"@en ,
        "cerca de"@es ,
        "proche de"@fr ;
    rdfs:comment """An annotation property for recording a possible mapping to a
         component in another model or ontology"""@en ;
    rdfs:isDefinedBy <https://www.ica.org/standards/RiC/ontology> ;
    rdfs:subPropertyOf rdfs:comment ;
    skos:changeNote
        [
            dc:date "2023-08-28" ;
            rdf:value "Added a new rdfs:label in French."@en ;
        ] ,
        [
            dc:date "2023-11-25" ;
            rdf:value "Added a new rdfs:label in Spanish."@en ;
        ] ;
.

:conditionsOfAccess
    a owl:DatatypeProperty ;
    rdfs:label
        "conditions of access"@en ,
        "condiciones de acceso"@es ,
        "conditions d’accès"@fr ;
    rdfs:comment """Terms and circumstances affecting the availability of a Record
         Resource or an Instantiation for consultation."""@en ;
    rdfs:domain
        [
            a owl:Class ;
            owl:unionOf (
                :Instantiation
                :RecordResource
            ) ;
        ] ;
    rdfs:isDefinedBy <https://www.ica.org/standards/RiC/ontology> ;
    rdfs:range rdfs:Literal ;
    skos:changeNote
        [
            dc:date "2023-11-11" ;
            rdf:value """Aligned with RiC-CM 1.0: updated the description
               (rdfs:comment), skos:scopeNote, examples (skos:example)."""@en ;
        ] ,
        [
            dc:date "2020-11-01" ;
            rdf:value """Text definition and scope note updated. Examples added.
               Objective: to make RiC-O compliant with RiC-CM v0.2."""@en ;
        ] ,
        [
            dc:date "2023-08-25" ;
            rdf:value "Added a new rdfs:label in French."@en ;
        ] ,
        [
            dc:date "2023-11-02" ;
            rdf:value "Added a new rdfs:label in Spanish."@en ;
        ] ;
    skos:example
        "Closed as awaiting conservation treatment"@en ,
        "Closed for 30 years"@en ,
        "Closed under data protection legislation"@en ,
        "Open"@en ,
        """Recognita software, min. version 3.0, is needed in order to open
         the file"""@en ,
        """The Archives cannot provide VHS reader to access the content of
         the tape"""@en ,
        "Acceso libre a través de los terminales de consulta"@es ;
    skos:scopeNote """May be used in a Record Set description when its value is shared
         by some or all members of the Record Set. The attribute provides information about the
         accessibility of a Record Resource, as well as the physical, technical or legal limitations
         that exist for providing access to it."""@en ;
    :RiCCMCorrespondingComponent """Corresponds to RiC-A08 (Conditions of Access
         attribute)"""@en ;
.

:conditionsOfUse
    a owl:DatatypeProperty ;
    rdfs:label
        "conditions of use"@en ,
        "condiciones de uso"@es ,
        "conditions d’utilisation"@fr ;
    rdfs:comment """Terms and circumstances affecting the use of a Record Resource or
         an Instantiation after access has been provided. Includes conditions governing reproduction
         of the Record Resource under applicable copyright (intellectual property) and/or property
         legislation or due to conservation status."""@en ;
    rdfs:domain
        [
            a owl:Class ;
            owl:unionOf (
                :Instantiation
                :RecordResource
            ) ;
        ] ;
    rdfs:isDefinedBy <https://www.ica.org/standards/RiC/ontology> ;
    rdfs:range rdfs:Literal ;
    skos:changeNote
        [
            dc:date "2023-11-02" ;
            rdf:value "Added a new rdfs:label in Spanish."@en ;
        ] ,
        [
            dc:date "2023-08-25" ;
            rdf:value "Added a new rdfs:label in French."@en ;
        ] ,
        [
            dc:date "2023-11-11" ;
            rdf:value """Aligned with RiC-CM 1.0: updated the description
               (rdfs:comment), skos:scopeNote, examples (skos:example)."""@en ;
        ] ,
        [
            dc:date "2020-11-01" ;
            rdf:value """Text definition updated. Examples added. Objective: to make
               RiC-O compliant with RiC-CM v0.2."""@en ;
        ] ;
    skos:example
        """Cannot be copied using warm light copying machines or photographed
         using flashlight"""@en ,
        """Permission of the copyright owner must be obtained before
         use"""@en ;
    skos:scopeNote """May be used in a Record Set description when its value is shared
         by some or all members of the Record Set."""@en ;
    :RiCCMCorrespondingComponent """Corresponds to RiC-A09 (Conditions of Use
         attribute)"""@en ;
.

:creationDate
    a owl:DatatypeProperty ;
    rdfs:label
        "creation date"@en ,
        "fecha de creación"@es ,
        "date de création"@fr ;
    rdfs:comment "Date at which an entity was created."@en ;
    rdfs:domain :Thing ;
    rdfs:isDefinedBy <https://www.ica.org/standards/RiC/ontology> ;
    rdfs:range rdfs:Literal ;
    rdfs:subPropertyOf :beginningDate ;
    skos:changeNote
        [
            dc:date "2023-08-25" ;
            rdf:value "Added a new rdfs:label in French."@en ;
        ] ,
        [
            dc:date "2023-11-02" ;
            rdf:value "Added a new rdfs:label in Spanish."@en ;
        ] ;
    skos:scopeNote """Provided for usability reasons. May be deprecated and removed
         later on. Use only if you don't use Date classes for handling dates."""@en ;
    :RiCCMCorrespondingComponent """Datatype property specialized implementation of
         RiC-E18 (Date entity)"""@en ;
.

:dateQualifier
    a owl:DatatypeProperty ;
    rdfs:label
        "date qualifier"@en ,
        "calificador de fecha"@es ,
        "qualificatif de la date"@fr ;
    rdfs:comment """A human readable qualification of a Date to indicate the level of
         precision or certainty."""@en ;
    rdfs:domain :Date ;
    rdfs:isDefinedBy <https://www.ica.org/standards/RiC/ontology> ;
    rdfs:range rdfs:Literal ;
    skos:changeNote
        [
            dc:date "2023-08-25" ;
            rdf:value "Added a new rdfs:label in French."@en ;
        ] ,
        [
            dc:date "2023-11-11" ;
            rdf:value """Aligned with RiC-CM 1.0: updated the description
               (rdfs:comment), skos:scopeNote."""@en ;
        ] ,
        [
            dc:date "2020-11-01" ;
            rdf:value """examples added. Objective: to make RiC-O compliant with RiC-CM
               v0.2."""@en ;
        ] ,
        [
            dc:date "2023-10-10" ;
            rdf:value """Updated the rdfs:comment, skos:scopeNote and examples, in order
               to make this datatype property fully compliant with RiC-CM 1.0"""@en ;
        ] ,
        [
            dc:date "2023-11-02" ;
            rdf:value "Added a new rdfs:label in Spanish."@en ;
        ] ;
    skos:example
        "approximate"@en ,
        "circa"@en ,
        "end unknown"@en ;
    skos:scopeNote """Most often, this human readable expression of the accuracy of
         the date is used along with an ISO 8601 representation of the date. The qualifier can also
         be expressed as a machine-readable value, using the EDTF standard (thus, a specialization
         of the normalizedDateValue datatype property)."""@en ;
    :RiCCMCorrespondingComponent """Corresponds to RiC-A13 (Date Qualifier
         attribute)"""@en ;
.

:deathDate
    a owl:DatatypeProperty ;
    rdfs:label
        "death date"@en ,
        "fecha de muerte"@es ,
        "date de décès"@fr ;
    rdfs:comment "Date at which a Person died."@en ;
    rdfs:domain :Person ;
    rdfs:isDefinedBy <https://www.ica.org/standards/RiC/ontology> ;
    rdfs:range rdfs:Literal ;
    rdfs:subPropertyOf :endDate ;
    skos:changeNote
        [
            dc:date "2023-08-25" ;
            rdf:value "Added a new rdfs:label in French."@en ;
        ] ,
        [
            dc:date "2023-11-02" ;
            rdf:value "Added a new rdfs:label in Spanish."@en ;
        ] ;
    skos:scopeNote """Provided for usability reasons. May be deprecated and removed
         later on. Use only if you don't use Date classes for handling dates."""@en ;
    :RiCCMCorrespondingComponent """Datatype property specialized implementation of
         RiC-E18 (Date entity)"""@en ;
.

:destructionDate
    a owl:DatatypeProperty ;
    rdfs:label
        "destruction date"@en ,
        "fecha de destrucción"@es ,
        "date de destruction"@fr ;
    rdfs:comment "Date at which an entity was deleted."@en ;
    rdfs:domain :Thing ;
    rdfs:isDefinedBy <https://www.ica.org/standards/RiC/ontology> ;
    rdfs:range rdfs:Literal ;
    rdfs:subPropertyOf :endDate ;
    skos:changeNote
        [
            dc:date "2023-11-12" ;
            rdf:value "Added a new rdfs:label in Spanish."@en ;
        ] ,
        [
            dc:date "2023-08-25" ;
            rdf:value "Added a new rdfs:label in French."@en ;
        ] ,
        [
            dc:date "2023-10-12" ;
            rdf:value "Renamed deletion into destruction."@en ;
        ] ;
    skos:scopeNote """Provided for usability reasons. May be deprecated and removed
         later on. Use only if you don't use Date classes for handling dates."""@en ;
    :RiCCMCorrespondingComponent """Datatype property specialized implementation of
         RiC-E18 (Date entity)"""@en ;
.

:expressedDate
    a owl:DatatypeProperty ;
    rdfs:label
        "expressed date"@en ,
        "fecha expresada"@es ,
        "date en langage naturel"@fr ;
    rdfs:comment """Natural language expression of a date. This property is a
         specialization of the name property. In order that the precise meaning of the date can be
         understood, information such as the calendar used or other specific context should be
         included."""@en ;
    rdfs:domain :Date ;
    rdfs:isDefinedBy <https://www.ica.org/standards/RiC/ontology> ;
    rdfs:range rdfs:Literal ;
    rdfs:subPropertyOf
        :name ,
        :textualValue ;
    skos:changeNote
        [
            dc:date "2023-08-25" ;
            rdf:value "Added a new rdfs:label in French."@en ;
        ] ,
        [
            dc:date "2023-11-11" ;
            rdf:value """Aligned with RiC-CM 1.0: updated the description
               (rdfs:comment), examples (skos:example)."""@en ;
        ] ,
        [
            dc:date "2023-10-10" ;
            rdf:value """Updated the rdfs:comment and skos:examples in order to make
               this property fully compliant with RiC-CM 1.0. Made it a subproperty of
               rico:name."""@en ;
        ] ,
        [
            dc:date "2020-11-01" ;
            rdf:value """examples added. Objective: to make RiC-O compliant with RiC-CM
               v0.2."""@en ;
        ] ,
        [
            dc:date "2023-11-02" ;
            rdf:value "Added a new rdfs:label in Spanish."@en ;
        ] ;
    skos:example
        "1550-1553, 1555 (date range)"@en ,
        "1925-1966 (date range)"@en ,
        "All of the years 1550, 1551, 1553, 1555"@en ,
        "October 24, 1999 (month day, year)"@en ,
        "One of the years 1550, 1551, 1553, 1555"@en ,
        "The Middle Ages"@en ,
        """The second semester of 1951 to 1952 (academic reference
         system)"""@en ,
        """15 thermidor an IV (calendrier révolutionnaire
         français)"""@fr ,
        "8 avril 1258 (a. st., style de Pâques)"@fr ,
        "XVIIe siècle"@fr ,
        """Die jovis ultima mensis martii anno domini millesimo quingentesimo
         quadragesimo ante Pascha"""@la ;
    :RiCCMCorrespondingComponent """Corresponds to RiC-A19 (Expressed Date
         attribute)"""@en ;
.

:geodesicSystem
    a owl:DatatypeProperty ;
    rdfs:label
        "geodesic system"@en ,
        "sistema geodésico"@es ,
        "système géodésique"@fr ;
    rdfs:comment "Reference system used for geographical coordinates."@en ;
    rdfs:domain :Coordinates ;
    rdfs:isDefinedBy <https://www.ica.org/standards/RiC/ontology> ;
    rdfs:range rdfs:Literal ;
    rdfs:subPropertyOf :referenceSystem ;
    skos:changeNote
        [
            dc:date "2023-08-25" ;
            rdf:value "Added a new rdfs:label in French."@en ;
        ] ,
        [
            dc:date "2023-11-02" ;
            rdf:value "Added a new rdfs:label in Spanish."@en ;
        ] ;
.

:geographicalCoordinates
    a owl:DatatypeProperty ;
    rdfs:label
        "geographical coordinates"@en ,
        "coordenadas geográficas"@es ,
        "coordonnées géographiques"@fr ;
    rdfs:comment "Longitudinal and latitudinal information about a Place. "@en ;
    rdfs:domain :Place ;
    rdfs:isDefinedBy <https://www.ica.org/standards/RiC/ontology> ;
    rdfs:range rdfs:Literal ;
    skos:changeNote
        [
            dc:date "2023-08-25" ;
            rdf:value "Added a new rdfs:label in French."@en ;
        ] ,
        [
            dc:date "2020-11-01" ;
            rdf:value """Text definition and scope note updated. Examples added.
               Objective: to make RiC-O compliant with RiC-CM v0.2."""@en ;
        ] ,
        [
            dc:date "2023-11-11" ;
            rdf:value """Aligned with RiC-CM 1.0: updated the description
               (rdfs:comment), examples (skos:example)."""@en ;
        ] ,
        [
            dc:date "2023-08-25" ;
            rdf:value "Added a new rdfs:label in French."@en ;
        ] ,
        [
            dc:date "2023-11-02" ;
            rdf:value "Added a new rdfs:label in Spanish."@en ;
        ] ;
    skos:example
        """Latitude 35.89421911, Longitude 139.94637467 (ISO
         6709/F)"""@en ,
        """Latitude 50°40′46,461″N, Longitude 95°48′26,533″W, Height 123,45m
         (ISO 6709/D)"""@en ;
    skos:scopeNote """Provided for usability reasons. May be deprecated and removed
         later on. Use only if you don't use PhysicalLocation and Coordinates classes with Place.
         Coordinates may be based on ISO 6709 Standard representation of geographic point location
         by coordinates."""@en ;
    :RiCCMCorrespondingComponent """Corresponds to RiC-A11 (Coordinates
         attribute)"""@en ;
.

:hasOrHadCorrespondent
    a
        owl:ObjectProperty ,
        owl:SymmetricProperty ;
    rdfs:label
        "has or had correspondent"@en ,
        "tiene o tenía como correspondiente"@es ,
        "a ou a eu pour correspondant"@fr ;
    rdfs:comment """Connects two Persons that correspond or have corresponded with
         each other. This relation is symmetric."""@en ;
    rdfs:domain :Person ;
    rdfs:isDefinedBy <https://www.ica.org/standards/RiC/ontology> ;
    rdfs:range :Person ;
    rdfs:subPropertyOf :knows ;
    owl:propertyChainAxiom (
        :thingIsConnectedToRelation
        :correspondenceRelation_role
        :relationConnects
    ) ;
    skos:changeNote
        [
            dc:date "2023-08-28" ;
            rdf:value "Added a new rdfs:label in French."@en ;
        ] ,
        [
            dc:date "2021-01-22" ;
            rdf:value """changed the IRI, label, textual definition (changed made in
               order to make RiC-O compliant with RiC-CM 0.2; the name of this property in RiC-O 0.1
               was "hasCorrespondent")."""@en ;
        ] ,
        [
            dc:date "2023-11-02" ;
            rdf:value "Added a new rdfs:label in Spanish."@en ;
        ] ,
        [
            dc:date "2023-11-08" ;
            rdf:value """In order to get a system of rolified Relation classes: modified
               the property chain axiom so that it now involves the new correspondenceRelation_role
               object property."""@en ;
        ] ;
    :RiCCMCorrespondingComponent """RiC-R052 ('has or had correspondent'
         relation)"""@en ;
.

:hasOrHadSpouse
    a
        owl:ObjectProperty ,
        owl:SymmetricProperty ;
    rdfs:label
        "has or had spouse"@en ,
        "tiene o tenía como cónyuge a"@es ,
        "a ou a eu pour conjoint"@fr ;
    rdfs:comment """Connects two Persons who are or were married. This relation is
         symmetric."""@en ;
    rdfs:domain :Person ;
    rdfs:isDefinedBy <https://www.ica.org/standards/RiC/ontology> ;
    rdfs:range :Person ;
    rdfs:subPropertyOf :hasFamilyAssociationWith ;
    owl:propertyChainAxiom (
        :thingIsConnectedToRelation
        :spouseRelation_role
        :relationConnects
    ) ;
    skos:changeNote
        [
            dc:date "2023-11-02" ;
            rdf:value "Added a new rdfs:label in Spanish."@en ;
        ] ,
        [
            dc:date "2023-11-08" ;
            rdf:value """In order to get a system of rolified Relation classes: modified
               the property chain axiom so that it now involves the new spouseRelation_role object
               property."""@en ;
        ] ,
        [
            dc:date "2021-01-22" ;
            rdf:value """changed the IRI, label, inverse property IRI, text definition,
               super property IRI (changed made in order to make RiC-O compliant with RiC-CM 0.2;
               the name of this property in RiC-O 0.1 was "hasSpouse")."""@en ;
        ] ,
        [
            dc:date "2023-11-12" ;
            rdf:value """Aligned with RiC-CM 1.0: updated the description
               (rdfs:comment)."""@en ;
        ] ,
        [
            dc:date "2023-08-28" ;
            rdf:value "Added a new rdfs:label in French."@en ;
        ] ;
    :RiCCMCorrespondingComponent """RiC-R049 ('has or had spouse'
         relation)"""@en ;
.

:hasOrHadWorkRelationWith
    a
        owl:ObjectProperty ,
        owl:SymmetricProperty ;
    rdfs:label
        "has or had work relation with"@en ,
        "tiene o tenía relación profesional con"@es ,
        "a ou a eu une relation professionnelle avec"@fr ;
    rdfs:comment """Connects two Agents that have or had some type of work relation in
         the course of their activities. This relation is symmetric."""@en ;
    rdfs:domain :Agent ;
    rdfs:isDefinedBy <https://www.ica.org/standards/RiC/ontology> ;
    rdfs:range :Agent ;
    rdfs:subPropertyOf :isAgentAssociatedWithAgent ;
    owl:propertyChainAxiom (
        :thingIsConnectedToRelation
        :workRelation_role
        :relationConnects
    ) ;
    skos:changeNote
        [
            dc:date "2023-08-28" ;
            rdf:value "Added a new rdfs:label in French."@en ;
        ] ,
        [
            dc:date "2023-11-07" ;
            rdf:value """Added the property chain axiom so that this property is
               formally defined as a shortcut."""@en ;
        ] ,
        [
            dc:date "2023-11-08" ;
            rdf:value """In order to get a system of rolified Relation classes: modified
               the property chain axiom so that it now involves the new workRelation_role object
               property."""@en ;
        ] ,
        [
            dc:date "2023-11-02" ;
            rdf:value "Added a new rdfs:label in Spanish."@en ;
        ] ,
        [
            dc:date "2021-01-22" ;
            rdf:value """changed the IRI, label, text definition (changed made in order
               to make RiC-O compliant with RiC-CM 0.2; the name of this property in RiC-O 0.1 was
               "hasWorkRelationWith")."""@en ;
        ] ;
    :RiCCMCorrespondingComponent """RiC-R046 ('has or had work relation with'
         relation)"""@en ;
.

:hasSibling
    a
        owl:ObjectProperty ,
        owl:SymmetricProperty ;
    rdfs:label
        "has sibling"@en ,
        "tiene como hermano o hermana a"@es ,
        "a pour frère ou sœur"@fr ;
    rdfs:comment """Connects two Persons who are siblings. This relation is
         symmetric."""@en ;
    rdfs:domain :Person ;
    rdfs:isDefinedBy <https://www.ica.org/standards/RiC/ontology> ;
    rdfs:range :Person ;
    rdfs:subPropertyOf :hasFamilyAssociationWith ;
    owl:propertyChainAxiom (
        :thingIsConnectedToRelation
        :siblingRelation_role
        :relationConnects
    ) ;
    skos:changeNote
        [
            dc:date "2023-11-12" ;
            rdf:value """Aligned with RiC-CM 1.0: updated the description
               (rdfs:comment)."""@en ;
        ] ,
        [
            dc:date "2023-08-28" ;
            rdf:value "Added a new rdfs:label in French."@en ;
        ] ,
        [
            dc:date "2021-01-22" ;
            rdf:value "changed the super property IRI."@en ;
        ] ,
        [
            dc:date "2023-11-02" ;
            rdf:value "Added a new rdfs:label in Spanish."@en ;
        ] ,
        [
            dc:date "2023-11-08" ;
            rdf:value """In order to get a system of rolified Relation classes: modified
               the property chain axiom so that it now involves the new siblingRelation_role object
               property."""@en ;
        ] ;
    :RiCCMCorrespondingComponent """RiC-R048 ('has sibling'
         relation)"""@en ;
.

:height
    a owl:DatatypeProperty ;
    rdfs:label
        "height"@en ,
        "altura"@es ,
        "hauteur"@fr ;
    rdfs:comment "Vertical dimension of an entity."@en ;
    rdfs:domain :Thing ;
    rdfs:isDefinedBy <https://www.ica.org/standards/RiC/ontology> ;
    rdfs:range rdfs:Literal ;
    rdfs:subPropertyOf :measure ;
    skos:changeNote
        [
            dc:date "2023-08-25" ;
            rdf:value "Added a new rdfs:label in French."@en ;
        ] ,
        [
            dc:date "2023-11-02" ;
            rdf:value "Added a new rdfs:label in Spanish."@en ;
        ] ;
.

:history
    a owl:DatatypeProperty ;
    rdfs:label
        "history"@en ,
        "historia"@es ,
        "histoire"@fr ;
    rdfs:comment """Summary of the development of an entity throughout its
         existence."""@en ;
    rdfs:domain
        [
            a owl:Class ;
            owl:unionOf (
                :RecordResource
                :Instantiation
                :Agent
                :Event
                :Rule
                :Place
            ) ;
        ] ;
    rdfs:isDefinedBy <https://www.ica.org/standards/RiC/ontology> ;
    rdfs:range rdfs:Literal ;
    skos:changeNote
        [
            dc:date "2020-11-01" ;
            rdf:value """Domains updated. Examples added. Objective: to make RiC-O
               compliant with RiC-CM v0.2."""@en ;
        ] ,
        [
            dc:date "2023-08-25" ;
            rdf:value "Added a new rdfs:label in French."@en ;
        ] ,
        [
            dc:date "2023-11-11" ;
            rdf:value """Aligned with RiC-CM 1.0: updated the description
               (rdfs:comment), skos:scopeNote, domain, examples (skos:example)."""@en ;
        ] ,
        [
            dc:date "2023-11-02" ;
            rdf:value "Added a new rdfs:label in Spanish."@en ;
        ] ;
    skos:example
        """The manuscripts are part of the collections of Robert Harley (d
         1724) and Edward Harley (d 1741), 1st and 2nd Earls of Oxford, that were brought by
         Parliament and transferred to the British Museum in 1753. Those materials were then
         separated into this collection and those for Harley Charters and Harley Rolls and became
         part of the collections of the British Library in 1972. (about a Record Set)"""@en ,
        """El primer sorteo de lotería se celebró el 13 de mayo de 1771,
         siendo desarrollado por la Real Lotería General de Nueva España… (sobre una
         actividad)"""@es ,
        """Nacido en Barbastro en 1892, donde realizó sus primeros estudios
         con los escolapios. Licenciado en Derecho por la Universidad de Zaragoza, aprobó las
         oposiciones al cuerpo nacional de notarios… (sobre una persona)"""@es ;
    skos:scopeNote """For a record set, may be used to summarize the history of the
         Record Set itself, or additionally to summarize the history of some or all members of the
         Record Set. Should not be confused with the scope and content property."""@en ;
    :RiCCMCorrespondingComponent """Corresponds to RiC-A21 (History
         attribute)"""@en ;
.

:identifier
    a owl:DatatypeProperty ;
    rdfs:label
        "identifier"@en ,
        "identificador"@es ,
        "identifiant"@fr ;
    rdfs:comment """A word, number, letter, symbol, or any combination of these used
         to uniquely identify or reference an individual instance of an entity within a specific
         information domain. Can include Global Persistent Identifiers (globally unique and
         persistently resolvable identifier for the entity) and/or Local Identifiers. Both the
         domain within which the identifier is unique, and the rules used in forming the identifier
         value should be provided with the identifier value."""@en ;
    rdfs:domain :Thing ;
    rdfs:isDefinedBy <https://www.ica.org/standards/RiC/ontology> ;
    rdfs:range rdfs:Literal ;
    skos:changeNote
        [
            dc:date "2023-08-25" ;
            rdf:value "Added a new rdfs:label in French."@en ;
        ] ,
        [
            dc:date "2023-11-02" ;
            rdf:value "Added a new rdfs:label in Spanish."@en ;
        ] ,
        [
            dc:date "2023-11-11" ;
            rdf:value """Aligned with RiC-CM 1.0: updated the description
               (rdfs:comment), skos:scopeNote, examples (skos:example)."""@en ;
        ] ,
        [
            dc:date "2020-11-01" ;
            rdf:value """Text definition and scope note updated. Examples added.
               Objective: to make RiC-O compliant with RiC-CM v0.2."""@en ;
        ] ;
    skos:example
        """B-000091 (example of a unique identifier for an instantiation
         assigned by a repository)"""@en ,
        """BUD-01-F002 (example of a classification number from a corporate
         file plan)"""@en ,
        """F 1204 (example of a local identifier for a record set assigned by
         a repository)"""@en ,
        """NAS1/A/1.1 (example of a local identifier for a
         record)"""@en ,
        """http://isni.org/0000000073572182 (example of a persistent
         International Standard Name Identifier for a person)"""@en ,
        """http://n2t.net/ark:/99166/w6tz44ht (example of an Archival
         Resource Key for a person)"""@en ,
        """http://n2t.net/ark:/99166/w6v1266v (example of an Archival
         Resource Key for a record)"""@en ;
    skos:scopeNote """Use only if you don't use Identifier class for handling
         identifiers. Within a given domain (a closed system), identifiers are used to uniquely
         reference instances of an entity. Identifiers are instruments of control that facilitate
         management of the entities within the domain. The formulation of identifiers commonly is
         based on rules. In addition to an identifier needing to be unique within a domain, it is
         also highly desirable that it be persistent, that is, that the identifier uniquely
         identifies the entity over time. A variety of organizations provide rules for the formation
         of identifiers, and services designed to facilitate the persistence of identifiers. Such
         identifiers are commonly referred to as Persistent Identifiers (or PIDs). PIDs conform to
         RFC 3986, but impose additional rules. Common examples are Archival Resource Keys (ARKs)
         and Digital Object Identifiers (DOIs). Within the global environment of the Internet, there
         are special rules for the formation of identifiers to ensure that they are unique within
         the domain of the Internet. Such identifiers must conform to the Internet Engineering Task
         Force (IETF) Uniform Resource Identifier rules (RFC 3986)."""@en ;
    :RiCCMCorrespondingComponent """Corresponds to RiC-A22 (Identifier
         attribute)"""@en ;
.

:instantiationExtent
    a owl:DatatypeProperty ;
    rdfs:label
        "Instantiation extent"@en ,
        "soporte de instanciación"@es ,
        "mesure de l’instanciation"@fr ;
    rdfs:comment """Countable characteristics of an Instantiation expressed as a
         quantity."""@en ;
    rdfs:domain :Instantiation ;
    rdfs:isDefinedBy <https://www.ica.org/standards/RiC/ontology> ;
    rdfs:range rdfs:Literal ;
    rdfs:subPropertyOf :physicalOrLogicalExtent ;
    skos:changeNote
        [
            dc:date "2023-11-11" ;
            rdf:value """Aligned with RiC-CM 1.0: updated the description
               (rdfs:comment), skos:scopeNote, examples (skos:example)."""@en ;
        ] ,
        [
            dc:date "2023-11-02" ;
            rdf:value "Added a new rdfs:label in Spanish."@en ;
        ] ,
        [
            dc:date "2023-08-25" ;
            rdf:value "Added a new rdfs:label in French."@en ;
        ] ,
        [
            dc:date "2020-11-01" ;
            rdf:value """Scope note updated. Examples added. Objective: to make RiC-O
               compliant with RiC-CM v0.2."""@en ;
        ] ;
    skos:example
        "234 linear metres"@en ,
        "Size of PDF file: 1.5 MB"@en ,
        "The register has 345 written folios"@en ;
    skos:scopeNote """Instantiation extent should not be confused with record resource
         extent or carrier extent. For a given Record Resource, the instantiation extent may vary,
         based on format, density of information on the carrier, etc. For example, a CD with a
         storage capacity of 700 MB (carrier extent) might hold a record of 1500 words (record
         resource extent) represented in two versions, one a Word document with an instantiation
         extent of 3 KB and the other a PDF file with an instantiation extent of 5
         KB."""@en ;
    :RiCCMCorrespondingComponent """Corresponds to RiC-A23 (Instantiation Extent
         attribute)"""@en ;
.

:instantiationStructure
    a owl:DatatypeProperty ;
    rdfs:label
        "Instantiation structure"@en ,
        "estructura de la instanciación"@es ,
        "structure de l’instanciation"@fr ;
    rdfs:comment """Information about the physical arrangement and composition of an
         Instantiation."""@en ;
    rdfs:domain :Instantiation ;
    rdfs:isDefinedBy <https://www.ica.org/standards/RiC/ontology> ;
    rdfs:range rdfs:Literal ;
    rdfs:subPropertyOf :structure ;
    skos:changeNote
        [
            dc:date "2023-11-02" ;
            rdf:value "Added a new rdfs:label in Spanish."@en ;
        ] ,
        [
            dc:date "2023-08-25" ;
            rdf:value "Added a new rdfs:label in French."@en ;
        ] ,
        [
            dc:date "2020-11-01" ;
            rdf:value """Text definition fixed. Objective: to make RiC-O compliant with
               RiC-CM v0.2."""@en ;
        ] ;
    :RiCCMCorrespondingComponent """Specialization of RiC-A40 (Structure
         attribute)"""@en ;
.

:integrityNote
    a owl:DatatypeProperty ;
    rdfs:label
        "integrity note"@en ,
        "nota de integridad"@es ,
        "note sur l'intégrité"@fr ;
    rdfs:comment """Information about the known intellectual completeness of a Record
         Resource."""@en ;
    rdfs:domain :RecordResource ;
    rdfs:isDefinedBy <https://www.ica.org/standards/RiC/ontology> ;
    rdfs:range rdfs:Literal ;
    skos:changeNote
        [
            dc:date "2023-11-11" ;
            rdf:value """Aligned with RiC-CM 1.0: updated the IRI, mapping to RiC-CM
               (rico:RiCCMCorrespondingComponent), labels, description (rdfs:comment),
               skos:scopeNote, domain, examples (skos:example)."""@en ;
        ] ,
        [
            dc:date "2023-11-02" ;
            rdf:value "Added a new rdfs:label in Spanish."@en ;
        ] ,
        [
            dc:date "2023-08-25" ;
            rdf:value "Added a new rdfs:label in French."@en ;
        ] ,
        [
            dc:date "2020-11-01" ;
            rdf:value """Scope note and examples added. Objective: to make RiC-O
               compliant with RiC-CM v0.2."""@en ;
        ] ;
    skos:example
        """A web page (HTML, 15 images, 2 CSS, 1 javascript), with 5 images
         missing."""@en ,
        """For record set: series of letters, one is missing so the integrity
         is compromised."""@en ,
        """Line three of a hand-written letter was cut out and a replacement
         text was inserted by an unknown person."""@en ,
        """Part of the text is missing (because a corner on the instantiation
         was cut out, which is a physical characteristic). See also the examples of
         physicalCharacteristics."""@en ;
    skos:scopeNote """May be used in a Record Set description when its value is shared
         by some or all members of the Record Set. The information about integrity may be generated
         manually or automatically. Not to be confused with the physical completeness of the
         instantiation, which is covered by the physical characteristics note attribute. The
         integrity of a Record Resource and the physical characteristics note of an Instantiation
         may be complementary. This attribute also covers any additions to or removal of original
         information."""@en ;
    :RiCCMCorrespondingComponent """Corresponds to RiC-A24 (Integrity Note
         attribute)"""@en ;
.

:intersects
    a
        owl:ObjectProperty ,
        owl:SymmetricProperty ;
    rdfs:label
        "intersects"@en ,
        "cruza"@es ,
        "intersecte"@fr ;
    rdfs:comment """Connects two Dates that overlap. This relation is
         symmetric."""@en ;
    rdfs:domain :Date ;
    rdfs:isDefinedBy <https://www.ica.org/standards/RiC/ontology> ;
    rdfs:range :Date ;
    rdfs:subPropertyOf
        :isAssociatedWithDate ,
        :isDateAssociatedWith ;
    skos:changeNote
        [
            dc:date "2023-10-12" ;
            rdf:value "Added the property"@en ;
        ] ,
        [
            dc:date "2023-11-27" ;
            rdf:value "Added a new rdfs:label in Spanish."@en ;
        ] ,
        [
            dc:date "2023-10-13" ;
            rdf:value """made this property a subproperty of
               isAssociatedWithdate."""@en ;
        ] ;
    :RiCCMCorrespondingComponent """RiC-R086 ('intersects'
         relation)"""@en ;
.

:isFunctionallyEquivalentTo
    a
        owl:ObjectProperty ,
        owl:SymmetricProperty ;
    rdfs:label
        "is functionally equivalent to"@en ,
        "equivale funcionalmente a"@es ,
        "est fonctionnellement équivalente à"@fr ;
    rdfs:comment """Connects two Instantiations which may be considered as equivalent.
         This relation is symmetric."""@en ;
    rdfs:domain :Instantiation ;
    rdfs:isDefinedBy <https://www.ica.org/standards/RiC/ontology> ;
    rdfs:range :Instantiation ;
    rdfs:subPropertyOf
        :isEquivalentTo ,
        :isInstantiationAssociatedWithInstantiation ;
    owl:propertyChainAxiom (
        :thingIsConnectedToRelation
        :functionalEquivalenceRelation_role
        :relationConnects
    ) ;
    skos:changeNote
        [
            dc:date "2021-01-22" ;
            rdf:value "changed the scope note."@en ;
        ] ,
        [
            dc:date "2023-08-28" ;
            rdf:value "Added a new rdfs:label in French."@en ;
        ] ,
        [
            dc:date "2023-11-02" ;
            rdf:value "Added a new rdfs:label in Spanish."@en ;
        ] ,
        [
            dc:date "2023-11-08" ;
            rdf:value """In order to get a system of rolified Relation classes: modified
               the property chain axiom so that it now involves the new
               functionalEquivalenceRelation_role object property."""@en ;
        ] ;
    skos:scopeNote """Two Instantiations, from some point of view, may be considered
         as equivalent. This equivalence is usually based upon the fact that the Instantiations have
         at least the same intellectual content (they instantiate the same Record
         Resource)."""@en ;
    :RiCCMCorrespondingComponent """RiC-R035 ('is functionally equivalent to'
         relation)"""@en ;
.

:isOrWasAdjacentTo
    a
        owl:ObjectProperty ,
        owl:SymmetricProperty ;
    rdfs:label
        "is or was adjacent to"@en ,
        "es o era un lugar contiguo a"@es ,
        "est ou a été adjacent à"@fr ;
    rdfs:comment """Connects two Places that are or were geographically adjacent. This
         relation is symmetric."""@en ;
    rdfs:domain :Place ;
    rdfs:isDefinedBy <https://www.ica.org/standards/RiC/ontology> ;
    rdfs:range :Place ;
    rdfs:subPropertyOf
        :isAssociatedWithPlace ,
        :isPlaceAssociatedWith ;
    skos:changeNote
        [
            dc:date "2023-11-02" ;
            rdf:value "Added a new rdfs:label in Spanish."@en ;
        ] ,
        [
            dc:date "2021-01-22" ;
            rdf:value """changed the IRI, label, textual definition (changed made in
               order to make RiC-O compliant with RiC-CM 0.2; the name of this property in RiC-O 0.1
               was "isAdjacentTo")."""@en ;
        ] ,
        [
            dc:date "2023-11-12" ;
            rdf:value """Aligned with RiC-CM 1.0: updated the description
               (rdfs:comment), skos:scopeNote."""@en ;
        ] ,
        [
            dc:date "2023-08-28" ;
            rdf:value "Added a new rdfs:label in French."@en ;
        ] ;
    skos:scopeNote """Use for connecting two adjacent geographical or administrative
         regions."""@en ;
    :RiCCMCorrespondingComponent """RiC-R077 ('is or was adjacent to'
         relation)"""@en ;
.

:lastModificationDate
    a owl:DatatypeProperty ;
    rdfs:label
        "last modification date"@en ,
        "fecha de última modificación"@es ,
        "date de dernière modification"@fr ;
    rdfs:comment "Date at which an entity was last updated."@en ;
    rdfs:domain :Thing ;
    rdfs:isDefinedBy <https://www.ica.org/standards/RiC/ontology> ;
    rdfs:range rdfs:Literal ;
    rdfs:subPropertyOf :modificationDate ;
    skos:changeNote
        [
            dc:date "2023-11-02" ;
            rdf:value "Added a new rdfs:label in Spanish."@en ;
        ] ,
        [
            dc:date "2023-08-25" ;
            rdf:value "Added a new rdfs:label in French."@en ;
        ] ;
    skos:scopeNote """Provided for usability reasons. May be deprecated and removed
         later on. Use only if you don't use Date classes for handling dates."""@en ;
    :RiCCMCorrespondingComponent """Datatype property specialized implementation of
         RiC-E18 (Date entity)"""@en ;
.

:latitude
    a owl:DatatypeProperty ;
    rdfs:label
        "latitude"@en ,
        "latitud"@es ,
        "latitude"@fr ;
    rdfs:comment "Distance in degrees north or south of the equator."@en ;
    rdfs:domain :Coordinates ;
    rdfs:isDefinedBy <https://www.ica.org/standards/RiC/ontology> ;
    rdfs:range rdfs:Literal ;
    rdfs:subPropertyOf :measure ;
    skos:changeNote
        [
            dc:date "2023-11-02" ;
            rdf:value "Added a new rdfs:label in Spanish."@en ;
        ] ,
        [
            dc:date "2023-08-25" ;
            rdf:value "Added a new rdfs:label in French."@en ;
        ] ;
    skos:scopeNote """Property of the Coordinates class. If you don't use this class,
         use geographicalCoordinates property, a property of Place class."""@en ;
.

:length
    a owl:DatatypeProperty ;
    rdfs:label
        "length"@en ,
        "longitud"@es ,
        "longueur"@fr ;
    rdfs:comment "Length of an entity."@en ;
    rdfs:domain :Thing ;
    rdfs:isDefinedBy <https://www.ica.org/standards/RiC/ontology> ;
    rdfs:range rdfs:Literal ;
    rdfs:subPropertyOf :measure ;
    skos:changeNote
        [
            dc:date "2023-08-28" ;
            rdf:value """Added for enabling to describe entities that have such a
               dimension."""@en ;
        ] ,
        [
            dc:date "2023-11-12" ;
            rdf:value "Added a new rdfs:label in Spanish."@en ;
        ] ;
    skos:scopeNote """May be used, among other cases, for storing the length of some
         places like streets."""@en ;
.

:location
    a owl:DatatypeProperty ;
    rdfs:label
        "location"@en ,
        "localización"@es ,
        "localisation"@fr ;
    rdfs:comment """A delimitation of the physical territory of a Place. Used to
         describe basic human-readable text such as an address, a cadastral reference, or less
         precise information found in a Record."""@en ;
    rdfs:domain :Place ;
    rdfs:isDefinedBy <https://www.ica.org/standards/RiC/ontology> ;
    rdfs:range rdfs:Literal ;
    skos:changeNote
        [
            dc:date "2020-11-01" ;
            rdf:value """Text definition and scope note updated. Examples added.
               Objective: to make RiC-O compliant with RiC-CM v0.2."""@en ;
        ] ,
        [
            dc:date "2023-11-11" ;
            rdf:value """Aligned with RiC-CM 1.0: updated the description
               (rdfs:comment), skos:scopeNote, examples (skos:example)."""@en ;
        ] ,
        [
            dc:date "2023-11-02" ;
            rdf:value "Added a new rdfs:label in Spanish."@en ;
        ] ,
        [
            dc:date "2023-08-25" ;
            rdf:value "Added a new rdfs:label in French."@en ;
        ] ;
    skos:example
        "Montreal (city in Canada)"@en ,
        "25 rue Saint-Denis à Paris"@fr ;
    skos:scopeNote """Use only if you don't use PhysicalLocation class with Place. Use
         the geographicalCoordinates property, or the Coordinates class, to record the geographical
         coordinates of the Place. Use the spatial relations (particularly 'has or had location') to
         capture a relation between two places."""@en ;
    :RiCCMCorrespondingComponent """Corresponds to RiC-A27 (Location
         attribute)"""@en ;
.

:longitude
    a owl:DatatypeProperty ;
    rdfs:label
        "longitude"@en ,
        "longitud"@es ,
        "longitude"@fr ;
    rdfs:comment """Distance in degrees east or west of a prime
         meridian."""@en ;
    rdfs:domain :Coordinates ;
    rdfs:isDefinedBy <https://www.ica.org/standards/RiC/ontology> ;
    rdfs:range rdfs:Literal ;
    rdfs:subPropertyOf :measure ;
    skos:changeNote
        [
            dc:date "2023-08-25" ;
            rdf:value "Added a new rdfs:label in French."@en ;
        ] ,
        [
            dc:date "2023-11-02" ;
            rdf:value "Added a new rdfs:label in Spanish."@en ;
        ] ;
    skos:scopeNote """Property of the Coordinates class. If you don't use this class,
         use geographicalCoordinates property, a property of Place class."""@en ;
.

:normalizedDateValue
    a owl:DatatypeProperty ;
    rdfs:label
        "normalized date value"@en ,
        "valor normalizado de fecha"@es ,
        "valeur normalisée de la date"@fr ;
    rdfs:comment """Machine readable representation of the date based on a public
         technical standard."""@en ;
    rdfs:domain :Date ;
    rdfs:isDefinedBy <https://www.ica.org/standards/RiC/ontology> ;
    rdfs:range rdfs:Literal ;
    rdfs:subPropertyOf :normalizedValue ;
    skos:changeNote
        [
            dc:date "2020-11-01" ;
            rdf:value """Examples added. Objective: to make RiC-O compliant with RiC-CM
               v0.2."""@en ;
        ] ,
        [
            dc:date "2023-11-02" ;
            rdf:value "Added a new rdfs:label in Spanish."@en ;
        ] ,
        [
            dc:date "2023-08-25" ;
            rdf:value "Added a new rdfs:label in French."@en ;
        ] ,
        [
            dc:date "2023-10-10" ;
            rdf:value """Updated the rdfs:comment and examples, and added a scopeNote,
               in order to make this property fully compliant with RiC-CM 1.0."""@en ;
        ] ,
        [
            dc:date "2023-11-11" ;
            rdf:value """Aligned with RiC-CM 1.0: updated the examples
               (skos:example)."""@en ;
        ] ;
    skos:example
        """1550,1551,1553,1555 (a date set in EDTF, meaning one of the years
         1550, 1151, 1553, 1555)"""@en ,
        "1948-03 (an ISO 8601 form of a single date)"@en ,
        "1948-03-08 (an ISO 8601 form of a single date)"@en ,
        """1948-03~ (a single date in ETDF, meaning March 1948
         approximately)"""@en ,
        """1948/ (a date range in EDTF, starting in 1948, end
         unknown)"""@en ,
        """1948/.. (an open date range in EDTF, starting in
         1948)"""@en ,
        """2012-02-14/2015-03-08 (an ISO 8601 form of a date
         range)"""@en ,
        "2012/2015-03 (an ISO 8601 form of a date range)"@en ,
        """{1550,1151,1553,1555} (a date set in EDTF, meaning all of the
         years 1550, 1151, 1553, 1555)"""@en ,
        """{1805,1815..1820} (a date set in EDTF, meaning all of the years
         1805, 1815, 1816, 1817, 1818, 1819, 1820)"""@en ;
    skos:scopeNote """Used to represent the date in a standardized format that can be
         processed programmatically. The main standard used today is ISO 8601, which is based on the
         Gregorian calendar. See also the Extended Date Time Format (EDTF), which is an extension of
         ISO 8601, and enables, among other features, to represent a date set, and to indicate the
         date is approximate."""@en ;
    :RiCCMCorrespondingComponent """Corresponds to RiC-A29 (Normalized Date
         attribute)"""@en ;
.

:overlapsOrOverlapped
    a
        owl:ObjectProperty ,
        owl:SymmetricProperty ;
    rdfs:label
        "overlaps or overlapped"@en ,
        "se superpone o superponía con"@es ,
        "chevauche ou a chevauché"@fr ;
    rdfs:comment """Connects two Places that geographically overlap or overlapped.
         This relation is symmetric."""@en ;
    rdfs:domain :Place ;
    rdfs:isDefinedBy <https://www.ica.org/standards/RiC/ontology> ;
    rdfs:range :Place ;
    rdfs:subPropertyOf
        :isAssociatedWithPlace ,
        :isPlaceAssociatedWith ;
    skos:changeNote
        [
            dc:date "2023-11-02" ;
            rdf:value "Added a new rdfs:label in Spanish."@en ;
        ] ,
        [
            dc:date "2023-11-12" ;
            rdf:value """Aligned with RiC-CM 1.0: updated the description
               (rdfs:comment)."""@en ;
        ] ,
        [
            dc:date "2021-01-22" ;
            rdf:value """changed the IRI, label, text definition (changed made in order
               to make RiC-O compliant with RiC-CM 0.2; the name of this property in RiC-O 0.1 was
               "overlaps")."""@en ;
        ] ,
        [
            dc:date "2023-08-28" ;
            rdf:value "Added a new rdfs:label in French."@en ;
        ] ;
    :RiCCMCorrespondingComponent """RiC-R078 ('overlaps or overlapped'
         relation)"""@en ;
.

:productionTechnique
    a owl:DatatypeProperty ;
    rdfs:label
        "production technique"@en ,
        "técnica de produccióon"@es ,
        "technique de production"@fr ;
    rdfs:comment """The method used in the representation of information on an
         Instantiation."""@en ;
    rdfs:domain :Instantiation ;
    rdfs:isDefinedBy <https://www.ica.org/standards/RiC/ontology> ;
    rdfs:range rdfs:Literal ;
    skos:changeNote
        [
            dc:date "2023-11-02" ;
            rdf:value "Added a new rdfs:label in Spanish."@en ;
        ] ,
        [
            dc:date "2023-08-25" ;
            rdf:value "Added a new rdfs:label in French."@en ;
        ] ,
        [
            dc:date "2020-11-01" ;
            rdf:value """Examples added. Objective: to make RiC-O compliant with RiC-CM
               v0.2."""@en ;
        ] ,
        [
            dc:date "2023-11-11" ;
            rdf:value """Aligned with RiC-CM 1.0: updated the description
               (rdfs:comment)."""@en ;
        ] ;
    skos:example
        "engraving"@en ,
        "handwriting"@en ,
        "magnetic recording"@en ,
        "optical recording"@en ;
    skos:scopeNote """Use only if you have free text or don't have a controlled
         vocabulary for production techniques (in this case, use the ProductionTechniqueType
         class)"""@en ;
    :RiCCMCorrespondingComponent """Corresponds to RiC-A33 (Production Technique
         attribute)"""@en ;
.

:publicationDate
    a owl:DatatypeProperty ;
    rdfs:label
        "publication date"@en ,
        "fecha de publicación"@es ,
        "date de publication"@fr ;
    rdfs:comment "Date of the publication of a Record Resource."@en ;
    rdfs:domain :RecordResource ;
    rdfs:isDefinedBy <https://www.ica.org/standards/RiC/ontology> ;
    rdfs:range rdfs:Literal ;
    rdfs:subPropertyOf :date ;
    skos:changeNote
        [
            dc:date "2023-11-02" ;
            rdf:value "Added a new rdfs:label in Spanish."@en ;
        ] ,
        [
            dc:date "2023-08-25" ;
            rdf:value "Added a new rdfs:label in French."@en ;
        ] ;
    skos:scopeNote """Provided for usability reasons. May be deprecated and removed
         later on. Use only if you don't use Date classes for handling dates."""@en ;
    :RiCCMCorrespondingComponent """Datatype property specialized implementation of
         RiC-E18 (Date entity)"""@en ;
.

:qualityOfRepresentationNote
    a owl:DatatypeProperty ;
    rdfs:label
        "quality of representation note"@en ,
        "nota sobre la calidad de representación"@es ,
        "note sur la qualité de la représentation"@fr ;
    rdfs:comment """Characteristics of an Instantiation that affect the ability to
         recover the intellectual content. Such characteristics may be related to the methods used
         in creating the Instantiation or introduced subsequent to the creation through
         accident."""@en ;
    rdfs:domain :Instantiation ;
    rdfs:isDefinedBy <https://www.ica.org/standards/RiC/ontology> ;
    rdfs:range rdfs:Literal ;
    rdfs:subPropertyOf :physicalCharacteristicsNote ;
    skos:changeNote
        [
            dc:date "2023-11-02" ;
            rdf:value "Added a new rdfs:label in Spanish."@en ;
        ] ,
        [
            dc:date "2020-11-01" ;
            rdf:value """Text definition updated. Examples added. Objective: to make
               RiC-O compliant with RiC-CM v0.2."""@en ;
        ] ,
        [
            dc:date "2023-08-25" ;
            rdf:value "Added a new rdfs:label in French."@en ;
        ] ,
        [
            dc:date "2023-11-11" ;
            rdf:value """Aligned with RiC-CM 1.0: updated the IRI, mapping to RiC-CM
               (rico:RiCCMCorrespondingComponent), labels, description (rdfs:comment),
               skos:scopeNote, rdfs:subpropertyOf."""@en ;
        ] ;
    skos:example
        """Black and white digitization may have led to loss of some
         information."""@en ,
        """some loss of information due to poor quality of image
         capture"""@en ,
        "some loss of text due to rodent damage"@en ;
    skos:scopeNote """Quality of representation note is a specialization of physical
         characteristics note. Quality of representation note should be used in conjunction with
         physical characteristics note when the physical characteristics impact the ability to
         recover the intellectual content."""@en ;
    :RiCCMCorrespondingComponent """Corresponds to RiC-A34 (Quality of
         Representation Note attribute)"""@en ;
.

:quantity
    a owl:DatatypeProperty ;
    rdfs:label
        "quantity"@en ,
        "cantidad"@es ,
        "quantité"@fr ;
    rdfs:comment "Machine-readable quantity."@en ;
    rdfs:domain :Extent ;
    rdfs:isDefinedBy <https://www.ica.org/standards/RiC/ontology> ;
    rdfs:range xsd:decimal ;
    rdfs:subPropertyOf :textualValue ;
    skos:changeNote
        [
            dc:date "2023-11-02" ;
            rdf:value "Added a new rdfs:label in Spanish."@en ;
        ] ,
        [
            dc:date "2020-11-21" ;
            rdf:value "Added a scope note."@en ;
        ] ,
        [
            dc:date "2023-08-28" ;
            rdf:value "Added an xml:lang attribute to the rdfs:comment."@en ;
        ] ,
        [
            dc:date "2023-08-25" ;
            rdf:value "Added a new rdfs:label in French."@en ;
        ] ,
        [
            dc:date "2020-10-28" ;
            rdf:value """Datatype property created along with unitOfMeasurement, Extent
               and UnitOfMeasurement classes, in order to provide methods for handling extent
               accurately."""@en ;
        ] ;
    skos:scopeNote """Use if you use the Extent class and its properties for handling
         an accurate description of the extent of a resource."""@en ;
.

:recordResourceExtent
    a owl:DatatypeProperty ;
    rdfs:label
        "Record Resource Extent"@en ,
        "soporte de recurso documental"@es ,
        "mesure de la ressource archivistique"@fr ;
    rdfs:comment """The quantity of information content, as human experienced,
         contained in a Record Resource. The method and precision of expressing the quantity of
         information represented in a Record Resource will vary according to the kind of Record
         Resource being described, processing economy constraints, etc. For record sets, quantity
         may be expressed as number of records, or, for analogue records in particular, by the
         physical storage dimensions of the members of the Record Set. For individual records or
         record parts, quantity may be expressed in more precise terms. """@en ;
    rdfs:domain :RecordResource ;
    rdfs:isDefinedBy <https://www.ica.org/standards/RiC/ontology> ;
    rdfs:range rdfs:Literal ;
    rdfs:subPropertyOf :physicalOrLogicalExtent ;
    skos:changeNote
        [
            dc:date "2020-11-01" ;
            rdf:value """Text definition and scope note updated. Examples added.
               Objective: to make RiC-O compliant with RiC-CM v0.2."""@en ;
        ] ,
        [
            dc:date "2023-11-11" ;
            rdf:value """Aligned with RiC-CM 1.0: updated the description
               (rdfs:comment), skos:scopeNote, examples (skos:example)."""@en ;
        ] ,
        [
            dc:date "2023-08-25" ;
            rdf:value "Added a new rdfs:label in French."@en ;
        ] ,
        [
            dc:date "2024-03-15" ;
            rdf:value "Fix capitalisation in English label."@en ;
        ] ,
        [
            dc:date "2020-11-21" ;
            rdf:value """Updated the scope note, as a RecordResourceExtent class has
               been created."""@en ;
        ] ,
        [
            dc:date "2023-11-02" ;
            rdf:value "Added a new rdfs:label in Spanish."@en ;
        ] ;
    skos:example
        "1,500 words"@en ,
        "2 films"@en ,
        "2.065.735 characters"@en ,
        "3 minutes and 24 seconds"@en ,
        "6 maps"@en ,
        "6 photographs"@en ;
    skos:scopeNote """Use if you don't use RecordResourceExtent class and its
         properties for handling such information. Record resource extent should not be confused
         with instantiation extent or carrier extent. The number, size or duration of the
         information content unit(s) remains the same even if the information is instantiated in
         various carriers. For example, a CD with a storage capacity of 700 MB (carrier extent)
         might hold a record of 1,500 words (record resource extent) represented in two versions,
         one a Word document with an instantiation extent of 3 KB and the other a PDF file with an
         instantiation extent of 5 KB."""@en ;
    :RiCCMCorrespondingComponent """Corresponds to RiC-A35 (Record Resource Extent
         attribute)"""@en ;
.

:recordResourceStructure
    a owl:DatatypeProperty ;
    rdfs:label
        "Record Resource structure"@en ,
        "estructura de recurso documental"@es ,
        "structure de la ressource archivistique"@fr ;
    rdfs:comment """Information about the intellectual arrangement and composition of
         a Record Resource. For Record and Record Part, it encompasses information about the
         intellectual composition of the record, the presence of record parts and their functions.
         For Record Set, it encompasses information about the methodology or criteria used for
         arranging the Record Set members or Record members within the containing Record
         Set"""@en ;
    rdfs:domain :RecordResource ;
    rdfs:isDefinedBy <https://www.ica.org/standards/RiC/ontology> ;
    rdfs:range rdfs:Literal ;
    rdfs:subPropertyOf :structure ;
    skos:changeNote
        [
            dc:date "2023-08-25" ;
            rdf:value "Added a new rdfs:label in French."@en ;
        ] ,
        [
            dc:date "2023-11-02" ;
            rdf:value "Added a new rdfs:label in Spanish."@en ;
        ] ,
        [
            dc:date "2020-11-01" ;
            rdf:value """Text definition updated. Examples added. Objective: to make
               RiC-O compliant with RiC-CM v0.2."""@en ;
        ] ;
    skos:example
        """Inside each file, the records are arranged
         chronologically."""@en ,
        """The database has 3 related tables: names, addresses, and passport
         numbers."""@en ,
        """The record has 2 appendixes, comprising a full account of the
         income from car taxes and real estate taxes."""@en ,
        """The series have the files arranged according to the alphabetical
         order of the places concerned."""@en ;
    :RiCCMCorrespondingComponent """Specialization of RiC-A40 (Structure
         attribute)"""@en ;
.

:relationCertainty
    a owl:DatatypeProperty ;
    rdfs:label
        "relation certainty "@en ,
        "certeza de la relación"@es ,
        "degré de certitude de la relation"@fr ;
    rdfs:comment """Qualifies the level of certitude of the accuracy of a
         Relation."""@en ;
    rdfs:domain :Relation ;
    rdfs:isDefinedBy <https://www.ica.org/standards/RiC/ontology> ;
    rdfs:range rdfs:Literal ;
    skos:changeNote
        [
            dc:date "2023-11-02" ;
            rdf:value "Added a new rdfs:label in Spanish."@en ;
        ] ,
        [
            dc:date "2023-10-14" ;
            rdf:value """Reintroduced this datatype property, with the definition
               assigned to it in RiC-CM 1.0, apart from its domain that also includes
               Event."""@en ;
        ] ,
        [
            dc:date "2023-12-27" ;
            rdf:value """Renamed the datatype property (was 'certainty') and reduced its
               domain to Relation (the dmain was the union of Event and Relation). Consequently
               updated the labels."""@en ;
        ] ;
    skos:example
        "certain"@en ,
        "uncertain"@en ,
        "unknown"@en ;
    :RiCCMCorrespondingComponent """Corresponds to RiC-RA01 (Certainty of Relation
         attribute)"""@en ;
.

:relationSource
    a owl:DatatypeProperty ;
    rdfs:label
        "relation source"@en ,
        "fuente de la relación"@es ,
        "source de la relation"@fr ;
    rdfs:comment """A source of information used for identifying and describing a
         Relation."""@en ;
    rdfs:domain :Relation ;
    rdfs:isDefinedBy <https://www.ica.org/standards/RiC/ontology> ;
    rdfs:range rdfs:Literal ;
    skos:changeNote
        [
            dc:date "2023-08-25" ;
            rdf:value "Added a new rdfs:label in French."@en ;
        ] ,
        [
            dc:date "2023-12-27" ;
            rdf:value """Renamed the datatype property (was 'source') and reduced its
               domain to Relation (the domain was the union of Record Resource and Relation).
               Consequently updated the rdfs:comment, labels and scope note. Added a
               rico:RiCCMCorrespondingComponent annotation."""@en ;
        ] ,
        [
            dc:date "2023-11-02" ;
            rdf:value "Added a new rdfs:label in Spanish."@en ;
        ] ;
    skos:scopeNote """Use only if you don't use the 'isEvidencedBy' object
         property."""@en ;
    :RiCCMCorrespondingComponent """Corresponds to RiC-RA05 (Source of Relation
         attribute)."""@en ;
.

:relationState
    a owl:DatatypeProperty ;
    rdfs:label
        "relation state"@en ,
        "estado de la relación"@es ,
        "statut de la relation"@fr ;
    rdfs:comment """Used to qualify the state of a Relation (e. g. present, past,
         ongoing, unknown)."""@en ;
    rdfs:domain :Relation ;
    rdfs:isDefinedBy <https://www.ica.org/standards/RiC/ontology> ;
    rdfs:range rdfs:Literal ;
    skos:changeNote
        [
            dc:date "2023-08-25" ;
            rdf:value "Added a new rdfs:label in French."@en ;
        ] ,
        [
            dc:date "2023-11-02" ;
            rdf:value "Added a new rdfs:label in Spanish."@en ;
        ] ;
.

:scopeAndContent
    a owl:DatatypeProperty ;
    rdfs:label
        "scope and content"@en ,
        "alcance y contenido"@es ,
        "portée et contenu"@fr ;
    rdfs:comment """Summary of the scope (such as time periods, geography) and content
         (such as subject matter, administrative processes) of a Record Resource. Provides a more
         complete summary of the informational content of the Record Resource highlighting the
         information conveyed in the Record Resource, why it was created, received, and/or
         maintained, and the agents connected to it. It may include description of relations with
         agents, activities, dates and places, or with other record resources."""@en ;
    rdfs:domain :RecordResource ;
    rdfs:isDefinedBy <https://www.ica.org/standards/RiC/ontology> ;
    rdfs:range rdfs:Literal ;
    rdfs:subPropertyOf :generalDescription ;
    skos:changeNote
        [
            dc:date "2020-11-01" ;
            rdf:value """Text definition updated. Examples added. Objective: to make
               RiC-O compliant with RiC-CM v0.2."""@en ;
        ] ,
        [
            dc:date "2023-08-25" ;
            rdf:value "Added a new rdfs:label in French."@en ;
        ] ,
        [
            dc:date "2023-08-25" ;
            rdf:value "Added a new rdfs:label in French."@en ;
        ] ,
        [
            dc:date "2023-11-11" ;
            rdf:value """Aligned with RiC-CM 1.0: updated the description
               (rdfs:comment), skos:scopeNote, rdfs:subpropertyOf, examples
               (skos:example)."""@en ;
        ] ,
        [
            dc:date "2023-11-02" ;
            rdf:value "Added a new rdfs:label in Spanish."@en ;
        ] ;
    skos:example
        "Among the witnesses, the Duke of Normandy."@en ,
        """Includes a detailed list of the lands and villages given by the
         King to the Abbey."""@en ,
        """Letter from Vlad the Impaler (Dracula) to the Council of Kronstadt
         asking them to send military support against the Ottomans, within the framework of their
         alliance treaty."""@en ,
        """The author explains why he does not agree with the decision made
         and adds that it cannot be applied."""@en ,
        """Se hace referencia a construcción del Gran Hotel, iniciada en 1899
         bajo el nombre de Casa Celestino. Tras su interrupción en 1902, continuó la obra ya con su
         nombre actual."""@es ;
    skos:scopeNote """Scope and content is a specialization of general description.
         For a Record Set, may be used to summarize the scope and content of the Record Set itself,
         or additionally to summarize the scope and content of some or all members of the Record
         Set. It is not to be confused with the history dataytpe property which focuses on the
         origination and subsequent changes to a Record Resource. """@en ;
    :RiCCMCorrespondingComponent """Corresponds to RiC-A38 (Scope and Content
         attribute)"""@en ;
.

:technicalCharacteristics
    a owl:DatatypeProperty ;
    rdfs:label
        "technical characteristics"@en ,
        "características técnicas"@es ,
        "caractéristiques techniques"@fr ;
    rdfs:comment """Describes any relevant physical or software feature of any device
         involved in the creation or management of a Record Resource."""@en ;
    rdfs:domain :Mechanism ;
    rdfs:isDefinedBy <https://www.ica.org/standards/RiC/ontology> ;
    rdfs:range rdfs:Literal ;
    skos:changeNote
        [
            dc:date "2023-08-25" ;
            rdf:value "Added a new rdfs:label in French."@en ;
        ] ,
        [
            dc:date "2020-11-01" ;
            rdf:value """Scope note and examples added. Objective: to make RiC-O
               compliant with RiC-CM v0.2."""@en ;
        ] ,
        [
            dc:date "2023-11-11" ;
            rdf:value """Aligned with RiC-CM 1.0: updated the description
               (rdfs:comment), skos:scopeNote."""@en ;
        ] ,
        [
            dc:date "2023-11-02" ;
            rdf:value "Added a new rdfs:label in Spanish."@en ;
        ] ;
    skos:example """Hubble Space Telescope had until 2002 a flawed mirror that
         introduced severe spherical aberration for the images."""@en ;
    skos:scopeNote """Does not include references to the workflow that the Mechanism
         is involved in, which is described under the Activity entity. It emphasizes those features
         that provide a better understanding of the impact of the Mechanism on the
         records."""@en ;
    :RiCCMCorrespondingComponent """Corresponds to RiC-A41 (Technical Characteristics
         attribute)"""@en ;
.

:title
    a owl:DatatypeProperty ;
    rdfs:label
        "title"@en ,
        "título"@es ,
        "intitulé"@fr ;
    rdfs:comment """An identifying name of a Record Resource, Instantiation or
         Rule."""@en ;
    rdfs:domain
        [
            a owl:Class ;
            owl:unionOf (
                :Instantiation
                :RecordResource
                :Rule
            ) ;
        ] ;
    rdfs:isDefinedBy <https://www.ica.org/standards/RiC/ontology> ;
    rdfs:range rdfs:Literal ;
    rdfs:subPropertyOf :name ;
    skos:changeNote
        [
            dc:date "2023-11-02" ;
            rdf:value "Added a new rdfs:label in Spanish."@en ;
        ] ,
        [
            dc:date "2023-08-25" ;
            rdf:value "Added a new rdfs:label in French."@en ;
        ] ;
    skos:scopeNote """Use only if you don't use Title class for handling
         titles."""@en ;
    :RiCCMCorrespondingComponent """Specialization of RiC-A28 (Name
         attribute)"""@en ;
.

:type
    a owl:DatatypeProperty ;
    rdfs:label
        "type"@en ,
        "tipo"@es ,
        "type"@fr ;
    rdfs:comment "A term used to characterize an entity."@en ;
    rdfs:domain :Thing ;
    rdfs:isDefinedBy <https://www.ica.org/standards/RiC/ontology> ;
    rdfs:range rdfs:Literal ;
    skos:changeNote
        [
            dc:date "2023-11-02" ;
            rdf:value "Added a new rdfs:label in Spanish."@en ;
        ] ,
        [
            dc:date "2023-08-25" ;
            rdf:value "Added a new rdfs:label in French."@en ;
        ] ;
    skos:scopeNote """Provided for usability reasons. May be deprecated and removed
         later on. Use only if you don't use Type subclasses for handling
         categories."""@en ;
.

:unitOfMeasurement
    a owl:DatatypeProperty ;
    rdfs:label
        "unit of measurement"@en ,
        "unidad de medida"@es ,
        "unité de mesure"@fr ;
    rdfs:comment """A definite magnitude of a quantity, defined and adopted by
         convention or by law, that is used as a standard for measurement of the same kind of
         quantity. Can be spacial units (cm, m), weight (g, kg), time (s, h), storage (MB, TB) or
         more informal units used in the archival context like number of boxes, pages or
         words."""@en ;
    rdfs:domain :Extent ;
    rdfs:isDefinedBy <https://www.ica.org/standards/RiC/ontology> ;
    rdfs:range rdfs:Literal ;
    skos:changeNote
        [
            dc:date "2023-11-02" ;
            rdf:value "Added a new rdfs:label in Spanish."@en ;
        ] ,
        [
            dc:date "2020-11-21" ;
            rdf:value "Added a scope note."@en ;
        ] ,
        [
            dc:date "2023-08-25" ;
            rdf:value "Added a new rdfs:label in French."@en ;
        ] ,
        [
            dc:date "2023-08-28" ;
            rdf:value "Added an xml:lang attribute to the rdfs:comment."@en ;
        ] ,
        [
            dc:date "2020-10-28" ;
            rdf:value """Datatype property created along with quantity, Extent and
               UnitOfMeasurement classes, in order to provide methods for handling extent
               accurately."""@en ;
        ] ;
    skos:scopeNote """Use if you do not use the UnitOfMeasurement class for handling
         units of measurement along with Extent."""@en ;
.

:usedFromDate
    a owl:DatatypeProperty ;
    rdfs:label
        "used from date"@en ,
        "usado desde la fecha"@es ,
        "utilisé à partir de"@fr ;
    rdfs:comment "Date at which an Appellation was first used."@en ;
    rdfs:domain :Appellation ;
    rdfs:isDefinedBy <https://www.ica.org/standards/RiC/ontology> ;
    rdfs:range rdfs:Literal ;
    rdfs:subPropertyOf :beginningDate ;
    skos:changeNote
        [
            dc:date "2023-11-02" ;
            rdf:value "Added a new rdfs:label in Spanish."@en ;
        ] ,
        [
            dc:date "2023-11-12" ;
            rdf:value "Made this property a subproperty of beginningDate."@en ;
        ] ,
        [
            dc:date "2023-08-25" ;
            rdf:value "Added a new rdfs:label in French."@en ;
        ] ;
    skos:scopeNote """Provided for usability reasons. May be deprecated and removed
         later on. Use only if you don't use Date classes for handling dates."""@en ;
    :RiCCMCorrespondingComponent """Datatype property specialized implementation of
         RiC-E18 (Date entity)"""@en ;
.

:usedToDate
    a owl:DatatypeProperty ;
    rdfs:label
        "used to date"@en ,
        "usado hasta la fecha"@es ,
        "utilisé jusqu’à"@fr ;
    rdfs:comment "Date until an Appellation was used."@en ;
    rdfs:domain :Appellation ;
    rdfs:isDefinedBy <https://www.ica.org/standards/RiC/ontology> ;
    rdfs:range rdfs:Literal ;
    rdfs:subPropertyOf :endDate ;
    skos:changeNote
        [
            dc:date "2023-08-25" ;
            rdf:value "Added a new rdfs:label in French."@en ;
        ] ,
        [
            dc:date "2023-11-02" ;
            rdf:value "Added a new rdfs:label in Spanish."@en ;
        ] ,
        [
            dc:date "2023-11-12" ;
            rdf:value "Made this property a subproperty of endDate."@en ;
        ] ;
    skos:scopeNote """Provided for usability reasons. May be deprecated and removed
         later on. Use only if you don't use Date classes for handling dates."""@en ;
    :RiCCMCorrespondingComponent """Datatype property specialized implementation of
         RiC-E18 (Date entity)"""@en ;
.

:width
    a owl:DatatypeProperty ;
    rdfs:label
        "width"@en ,
        "anchura"@es ,
        "largeur"@fr ;
    rdfs:comment "Horizontal dimension of an entity."@en ;
    rdfs:domain :Thing ;
    rdfs:isDefinedBy <https://www.ica.org/standards/RiC/ontology> ;
    rdfs:range rdfs:Literal ;
    rdfs:subPropertyOf :measure ;
    skos:changeNote
        [
            dc:date "2023-08-25" ;
            rdf:value "Added a new rdfs:label in French."@en ;
        ] ,
        [
            dc:date "2023-11-02" ;
            rdf:value "Added a new rdfs:label in Spanish."@en ;
        ] ;
.

voaf:Vocabulary
    a owl:Class ;
    rdfs:isDefinedBy <http://purl.org/vocommons/voaf> ;
.

skos:hasTopConcept
    a owl:ObjectProperty ;
    rdfs:isDefinedBy <http://www.w3.org/2004/02/skos/core> ;
    owl:inverseOf skos:topConceptOf ;
.

skos:topConceptOf
    a owl:ObjectProperty ;
    rdfs:isDefinedBy <http://www.w3.org/2004/02/skos/core> ;
    owl:inverseOf skos:hasTopConcept ;
.

:activityIsContextOfRelation
    a owl:ObjectProperty ;
    rdfs:label
        "activity is context of relation"@en ,
        "actividad es contexto de relación"@es ,
        "activité est le contexte de la relation"@fr ;
    rdfs:comment """Connects an Activity to an Agent Temporal Relation (when the
         Activity is transferred from an Agent to another one) or a Mandate Relation (the Mandate
         assigns the Activity to the Agent or defines it)."""@en ;
    rdfs:domain :Activity ;
    rdfs:isDefinedBy <https://www.ica.org/standards/RiC/ontology> ;
    rdfs:range
        [
            a owl:Class ;
            owl:unionOf (
                :AgentTemporalRelation
                :MandateRelation
            ) ;
        ] ;
    rdfs:subPropertyOf :thingIsContextOfRelation ;
    owl:inverseOf :asConcernsActivity ;
    skos:changeNote
        [
            dc:date "2023-11-02" ;
            rdf:value "Added a new rdfs:label in Spanish."@en ;
        ] ,
        [
            dc:date "2023-08-28" ;
            rdf:value "Added a new rdfs:label in French."@en ;
        ] ;
.

:affectsOrAffected
    a owl:ObjectProperty ;
    rdfs:label
        "affects or affected"@en ,
        "afecta o afectaba a"@es ,
        "affecte ou a affecté"@fr ;
    rdfs:comment """Connects an Event to a Thing on which the Event has or had some
         significant impact."""@en ;
    rdfs:domain :Event ;
    rdfs:isDefinedBy <https://www.ica.org/standards/RiC/ontology> ;
    rdfs:range :Thing ;
    rdfs:subPropertyOf :hasOrHadParticipant ;
    owl:inverseOf :isOrWasAffectedBy ;
    skos:changeNote
        [
            dc:date "2021-01-22" ;
            rdf:value """changed the IRI, label, inverse property IRI, text definition
               and corresponding CM component (changed made in order to make RiC-O compliant with
               RiC-CM 0.2; the name of this property in RiC-O 0.1 was "affects")."""@en ;
        ] ,
        [
            dc:date "2023-08-28" ;
            rdf:value "Added a new rdfs:label in French."@en ;
        ] ,
        [
            dc:date "2023-11-02" ;
            rdf:value "Added a new rdfs:label in Spanish."@en ;
        ] ;
    :RiCCMCorrespondingComponent """RiC-R059 ('affects or affected'
         relation)"""@en ;
.

:agentHasOrHadLocation
    a owl:ObjectProperty ;
    rdfs:label
        "agent has or had location"@en ,
        "agente tiene o tenía como localización"@es ,
        "agent a ou a eu pour localisation"@fr ;
    rdfs:comment """Inverse of 'is or was location of agent' object
         property."""@en ;
    rdfs:domain :Agent ;
    rdfs:isDefinedBy <https://www.ica.org/standards/RiC/ontology> ;
    rdfs:range :Place ;
    rdfs:subPropertyOf
        :hasOrHadLocation ,
        :isAgentAssociatedWithPlace ;
    owl:inverseOf :isOrWasLocationOfAgent ;
    skos:changeNote
        [
            dc:date "2023-11-27" ;
            rdf:value "Added a new rdfs:label in Spanish."@en ;
        ] ,
        [
            dc:date "2023-10-26" ;
            rdf:value "Added a rdfs:comment."@en ;
        ] ,
        [
            dc:date "2023-10-20" ;
            rdf:value "Property created for RiC-0 1.0."@en ;
        ] ;
.

:authorizedBy
    a owl:ObjectProperty ;
    rdfs:label
        "authorized by"@en ,
        "controlado por"@es ,
        "autorisé par"@fr ;
    rdfs:comment "Inverse of 'authorizes' object property"@en ;
    rdfs:domain :Agent ;
    rdfs:isDefinedBy <https://www.ica.org/standards/RiC/ontology> ;
    rdfs:range :Mandate ;
    rdfs:subPropertyOf :isAssociatedWithRule ;
    owl:inverseOf :authorizes ;
    owl:propertyChainAxiom (
        :thingIsTargetOfRelation
        :mandateRelation_role
        :relationHasSource
    ) ;
    skos:changeNote
        [
            dc:date "2023-11-02" ;
            rdf:value "Added a new rdfs:label in Spanish."@en ;
        ] ,
        [
            dc:date "2023-08-28" ;
            rdf:value "Added a new rdfs:label in French."@en ;
        ] ,
        [
            dc:date "2023-11-08" ;
            rdf:value """In order to get a system of rolified Relation classes: modified
               the property chain axiom so that it now involves the new mandateRelation_role object
               property."""@en ;
        ] ;
    :RiCCMCorrespondingComponent """RiC-R067i ('authorizedBy'
         relation)"""@en ;
.

:authorizes
    a owl:ObjectProperty ;
    rdfs:label
        "authorizes"@en ,
        "controla"@es ,
        "autorise"@fr ;
    rdfs:comment """Connects a Mandate to the Agent that the Mandate gives the
         authority or competencies to act."""@en ;
    rdfs:domain :Mandate ;
    rdfs:isDefinedBy <https://www.ica.org/standards/RiC/ontology> ;
    rdfs:range :Agent ;
    rdfs:subPropertyOf :isRuleAssociatedWith ;
    owl:inverseOf :authorizedBy ;
    owl:propertyChainAxiom (
        :thingIsSourceOfRelation
        :mandateRelation_role
        :relationHasTarget
    ) ;
    skos:changeNote
        [
            dc:date "2023-11-08" ;
            rdf:value """In order to get a system of rolified Relation classes: modified
               the property chain axiom so that it now involves the new mandateRelation_role object
               property."""@en ;
        ] ,
        [
            dc:date "2021-01-22" ;
            rdf:value "fixed the CM corresponding component name."@en ;
        ] ,
        [
            dc:date "2023-11-02" ;
            rdf:value "Added a new rdfs:label in Spanish."@en ;
        ] ,
        [
            dc:date "2023-08-28" ;
            rdf:value "Added a new rdfs:label in French."@en ;
        ] ;
    :RiCCMCorrespondingComponent """RiC-R067 ('authorizes'
         relation)"""@en ;
.

:authorizingAgent
    a owl:ObjectProperty ;
    rdfs:label
        "authorizing agent"@en ,
        "autorización dada por el agente"@es ,
        "autorisation donnée par l’agent"@fr ;
    rdfs:comment """Connects a Mandate Relation to an Agent that assigns the
         Mandate."""@en ;
    rdfs:domain :MandateRelation ;
    rdfs:isDefinedBy <https://www.ica.org/standards/RiC/ontology> ;
    rdfs:range :Agent ;
    rdfs:subPropertyOf :relationHasContext ;
    owl:inverseOf :isAuthorizingAgentInMandateRelation ;
    skos:changeNote
        [
            dc:date "2023-11-02" ;
            rdf:value "Added a new rdfs:label in Spanish."@en ;
        ] ,
        [
            dc:date "2023-11-13" ;
            rdf:value "Fixed the rdfs:label in Spanish."@en ;
        ] ,
        [
            dc:date "2023-08-28" ;
            rdf:value "Added a new rdfs:label in French."@en ;
        ] ;
.

:contained
    a owl:ObjectProperty ;
    rdfs:label
        "contained"@en ,
        "contenía"@es ,
        "a contenu"@fr ;
    rdfs:comment """Connects a Place to a Place that it contained in the
         past."""@en ;
    rdfs:domain :Place ;
    rdfs:isDefinedBy <https://www.ica.org/standards/RiC/ontology> ;
    rdfs:range :Place ;
    rdfs:subPropertyOf
        :containsOrContained ,
        :hadPart ;
    owl:inverseOf :wasContainedBy ;
    skos:changeNote
        [
            dc:date "2023-09-05" ;
            rdf:value """Object property added, along with its inverse property, in order to enable to
               express past partitive relations between places (the current partitive relations
               being also added, including a transitive one).""" ;
        ] ,
        [
            dc:date "2023-11-12" ;
            rdf:value "Updated the labels, description (rdfs:comment)."@en ;
        ] ,
        [
            dc:date "2023-11-27" ;
            rdf:value "Added a new rdfs:label in Spanish."@en ;
        ] ;
.

:creationWithRole
    a owl:ObjectProperty ;
    rdfs:label
        "creation with role"@en ,
        "creación con el rol de"@es ,
        "création avec pour rôle"@fr ;
    rdfs:comment """Connects a Creation Relation to the Role Type that the creator
         Agent(s) has in the creation process"""@en ;
    rdfs:domain :CreationRelation ;
    rdfs:isDefinedBy <https://www.ica.org/standards/RiC/ontology> ;
    rdfs:range :RoleType ;
    rdfs:subPropertyOf :relationHasContext ;
    owl:inverseOf :roleIsContextOfCreationRelation ;
    skos:changeNote
        [
            dc:date "2023-11-02" ;
            rdf:value "Added a new rdfs:label in Spanish."@en ;
        ] ,
        [
            dc:date "2023-08-28" ;
            rdf:value "Added a new rdfs:label in French."@en ;
        ] ;
.

:describesOrDescribed
    a owl:ObjectProperty ;
    rdfs:label
        "describes or described"@en ,
        "describe o describía"@es ,
        "décrit ou a décrit"@fr ;
    rdfs:comment """Connects a Record Resource to a Thing that it describes or
         described."""@en ;
    rdfs:domain :RecordResource ;
    rdfs:isDefinedBy <https://www.ica.org/standards/RiC/ontology> ;
    rdfs:range :Thing ;
    rdfs:subPropertyOf :hasOrHadSubject ;
    owl:inverseOf :isOrWasDescribedBy ;
    skos:changeNote
        [
            dc:date "2021-01-22" ;
            rdf:value """changed the IRI, label, inverse property IRI, text definition,
               corresponding CM component name (changed made in order to make RiC-O compliant with
               RiC-CM 0.2; the name of this property in RiC-O 0.1 was "describes")."""@en ;
        ] ,
        [
            dc:date "2023-11-02" ;
            rdf:value "Added a new rdfs:label in Spanish."@en ;
        ] ,
        [
            dc:date "2023-11-12" ;
            rdf:value """Aligned with RiC-CM 1.0: updated the description
               (rdfs:comment)."""@en ;
        ] ,
        [
            dc:date "2023-08-28" ;
            rdf:value "Added a new rdfs:label in French."@en ;
        ] ;
    skos:scopeNote """Can be used, among other situations, for specifying that some
         finding aid (a Record that has Documentary Form Type Finding Aid) describes some Record
         Set."""@en ;
    :RiCCMCorrespondingComponent """RiC-R021 ('describes or described'
         relation)"""@en ;
.

:directlyContains
    a owl:ObjectProperty ;
    rdfs:label
        "contains directly"@en ,
        "contiene directamente"@es ,
        "contient directement"@fr ;
    rdfs:comment "Connects a Place to another Place that it directly contains." ;
    rdfs:domain :Place ;
    rdfs:isDefinedBy <https://www.ica.org/standards/RiC/ontology> ;
    rdfs:range :Place ;
    rdfs:subPropertyOf
        :containsTransitive ,
        :hasDirectPart ;
    owl:inverseOf :isDirectlyContainedBy ;
    skos:changeNote
        [
            dc:date "2023-09-05" ;
            rdf:value """Object property added, along with its inverse property, in order to enable to
               express current, direct, partitive relations between places (the possibly indirect,
               transitive relation, superproperty of this one, being also added).""" ;
        ] ,
        [
            dc:date "2023-11-27" ;
            rdf:value "Added a new rdfs:label in Spanish."@en ;
        ] ,
        [
            dc:date "2023-11-12" ;
            rdf:value "Updated the description (rdfs:comment) and labels."@en ;
        ] ;
.

:directlyFollowsInSequence
    a owl:ObjectProperty ;
    rdfs:label
        "directly follows in sequence"@en ,
        "sigue directamente en la secuencia"@es ,
        "suit directement dans la séquence"@fr ;
    rdfs:comment """Connects a Thing to a Thing that it follows directly in some non
         chronological sequence."""@en ;
    rdfs:domain :Thing ;
    rdfs:isDefinedBy <https://www.ica.org/standards/RiC/ontology> ;
    rdfs:range :Thing ;
    rdfs:subPropertyOf :followsInSequenceTransitive ;
    owl:inverseOf :directlyPrecedesInSequence ;
    skos:changeNote
        [
            dc:date "2023-11-27" ;
            rdf:value "Added a new rdfs:label in Spanish."@en ;
        ] ,
        [
            dc:date "2023-09-22" ;
            rdf:value """Renamed the property and modified its definition (rdfs:comment)
               in order to better distinguish it from followsInTime."""@en ;
        ] ,
        [
            dc:date "2023-09-08" ;
            rdf:value """Added transitive super-property and both present direct and
               past sequential relations as well as their respective inverse relations."""@en ;
        ] ,
        [
            dc:date "2023-11-12" ;
            rdf:value "Updated the description (rdfs:comment) and labels."@en ;
        ] ;
.

:directlyIncludes
    a owl:ObjectProperty ;
    rdfs:label
        "directly includes"@en ,
        "incluye directamente"@es ,
        "inclut directement"@fr ;
    rdfs:comment """Connects a Record Set to a Record or Record Set which it includes
         directly."""@en ;
    rdfs:domain :RecordSet ;
    rdfs:isDefinedBy <https://www.ica.org/standards/RiC/ontology> ;
    rdfs:range
        [
            a owl:Class ;
            owl:unionOf (
                :Record
                :RecordSet
            ) ;
        ] ;
    rdfs:subPropertyOf
        :hasDirectPart ,
        :includesTransitive ;
    owl:inverseOf :isDirectlyIncludedIn ;
    skos:changeNote
        [
            dc:date "2023-11-27" ;
            rdf:value "Added a new rdfs:label in Spanish."@en ;
        ] ,
        [
            dc:date "2023-11-12" ;
            rdf:value "Updated the labels, description (rdfs:comment)."@en ;
        ] ,
        [
            dc:date "2023-09-08" ;
            rdf:value """Object property added, along with its inverse property, in
               order to enable to express current, direct, partitive relations between Record Sets
               and their members (the possibly indirect, transitive relation, superproperty of this
               one, being also added)."""@en ;
        ] ;
.

:directlyPrecedesInSequence
    a owl:ObjectProperty ;
    rdfs:label
        "directly precedes in sequence"@en ,
        "precede directamente en la secuencia"@es ,
        "précède directement dans la séquence"@fr ;
    rdfs:comment """Connects a Thing to a Thing that it precedes directly in some non
         chronological sequence."""@en ;
    rdfs:domain :Thing ;
    rdfs:isDefinedBy <https://www.ica.org/standards/RiC/ontology> ;
    rdfs:range :Thing ;
    rdfs:subPropertyOf :precedesInSequenceTransitive ;
    owl:inverseOf :directlyFollowsInSequence ;
    skos:changeNote
        [
            dc:date "2023-11-12" ;
            rdf:value "Updated the description (rdfs:comment) and labels."@en ;
        ] ,
        [
            dc:date "2023-11-27" ;
            rdf:value "Added a new rdfs:label in Spanish."@en ;
        ] ,
        [
            dc:date "2023-09-22" ;
            rdf:value """Renamed the property and modified its definition (rdfs:comment)
               in order to better distinguish it from precedesInTime."""@en ;
        ] ,
        [
            dc:date "2023-09-08"@en ;
            rdf:value """Object property added, along with its inverse property, in
               order to enable to express current, direct, sequential relations between things (the
               possibly indirect, transitive relation, superproperty of this one, being also
               added)."""@en ;
        ] ;
.

:documentedBy
    a owl:ObjectProperty ;
    rdfs:label
        "documented by"@en ,
        "se documenta en"@es ,
        "est documenté par"@fr ;
    rdfs:comment "Inverse of 'documents' object property."@en ;
    rdfs:domain :Activity ;
    rdfs:isDefinedBy <https://www.ica.org/standards/RiC/ontology> ;
    rdfs:range
        [
            a owl:Class ;
            owl:unionOf (
                :Instantiation
                :RecordResource
            ) ;
        ] ;
    rdfs:subPropertyOf
        :isOrganicOrFunctionalProvenanceOf ,
        :resultsOrResultedIn ;
    owl:inverseOf :documents ;
    owl:propertyChainAxiom (
        :thingIsTargetOfRelation
        :activityDocumentationRelation_role
        :relationHasSource
    ) ;
    skos:changeNote
        [
            dc:date "2021-01-22" ;
            rdf:value """changed the inverse property IRI, the superproperty IRI and the
               corresponding CML component name"""@en ;
        ] ,
        [
            dc:date "2023-11-02" ;
            rdf:value "Added a new rdfs:label in Spanish."@en ;
        ] ,
        [
            dc:date "2023-08-28" ;
            rdf:value "Added a new rdfs:label in French."@en ;
        ] ,
        [
            dc:date "2023-11-07" ;
            rdf:value """Made this property a subproperty of the new
               isOrganicOrFunctionalProvenanceOf property."""@en ;
        ] ,
        [
            dc:date "2023-11-08" ;
            rdf:value """In order to get a system of rolified Relation classes: modified
               the property chain axiom so that it now involves the new
               activityDocumentationRelation_role object property."""@en ;
        ] ;
    :RiCCMCorrespondingComponent """RiC-R033i ('documented by'
         relation)"""@en ;
.

:documents
    a owl:ObjectProperty ;
    rdfs:label
        "documents"@en ,
        "documenta"@es ,
        "documente"@fr ;
    rdfs:comment """Connects a Record Resource or an Instantiation to the Activity
         that generates the Record Resource or Instantiation."""@en ;
    rdfs:domain
        [
            a owl:Class ;
            owl:unionOf (
                :Instantiation
                :RecordResource
            ) ;
        ] ;
    rdfs:isDefinedBy <https://www.ica.org/standards/RiC/ontology> ;
    rdfs:range :Activity ;
    rdfs:subPropertyOf
        :hasOrganicOrFunctionalProvenance ,
        :resultsOrResultedFrom ;
    owl:inverseOf :documentedBy ;
    owl:propertyChainAxiom (
        :thingIsSourceOfRelation
        :activityDocumentationRelation_role
        :relationHasTarget
    ) ;
    skos:changeNote
        [
            dc:date "2023-11-12" ;
            rdf:value """Aligned with RiC-CM 1.0: updated the
               skos:scopeNote."""@en ;
        ] ,
        [
            dc:date "2021-01-22" ;
            rdf:value """changed the IRI, label, superproperty IRI, corresponding CM
               component name (changed made in order to make RiC-O compliant with RiC-CM 0.2; the
               name of this property in RiC-O 0.1 was "isDocumentationOf")."""@en ;
        ] ,
        [
            dc:date "2023-11-02" ;
            rdf:value "Added a new rdfs:label in Spanish."@en ;
        ] ,
        [
            dc:date "2023-11-07" ;
            rdf:value """Made this property a subproperty of the new
               hasOrganicOrFunctionalProvenance property."""@en ;
        ] ,
        [
            dc:date "2023-11-08" ;
            rdf:value """In order to get a system of rolified Relation classes: modified
               the property chain axiom so that it now involves the new
               activityDocumentationRelation_role object property."""@en ;
        ] ,
        [
            dc:date "2023-08-28" ;
            rdf:value "Added a new rdfs:label in French."@en ;
        ] ;
    skos:scopeNote """To be used to describe the functional provenance of a Record
         Resource or Instantiation."""@en ;
    :RiCCMCorrespondingComponent """RiC-R033 ('documents'
         relation)"""@en ;
.

:evidences
    a owl:ObjectProperty ;
    rdfs:label
        "evidences"@en ,
        "evidencia"@es ,
        "atteste de"@fr ;
    rdfs:comment """Connects a Record Resource to a Relation, when the first is used
         for proving the existence of the second one, or for describing it."""@en ;
    rdfs:domain :RecordResource ;
    rdfs:isDefinedBy <https://www.ica.org/standards/RiC/ontology> ;
    rdfs:range :Relation ;
    rdfs:subPropertyOf :thingIsConnectedToRelation ;
    owl:inverseOf :isEvidencedBy ;
    skos:changeNote
        [
            dc:date "2023-11-02" ;
            rdf:value "Added a new rdfs:label in Spanish."@en ;
        ] ,
        [
            dc:date "2023-08-28" ;
            rdf:value "Added a new rdfs:label in French."@en ;
        ] ,
        [
            dc:date "2023-12-27" ;
            rdf:value """Renamed the object property (was 'is source of') and reduced
               its domain to Record Resource (the domain was the union of Record Resource and Agent)
               and its range to Relation (the range was the union of Record Resource and Relation).
               Consequently updated the superproperty, the labels, and added a
               rico:RiCCMCorrespondingComponent. Same for the inverse object property."""@en ;
        ] ;
    :RiCCMCorrespondingComponent """Inverse of 'is evidenced by' object
         property."""@en ;
.

:existsOrExistedIn
    a owl:ObjectProperty ;
    rdfs:label
        "exists or existed in"@en ,
        "existe o existía en"@es ,
        "existe ou a existé dans"@fr ;
    rdfs:comment """Connects a Position to a Group in which that Position exists or
         existed, or that is defined by that Group's organizational structure."""@en ;
    rdfs:domain :Position ;
    rdfs:isDefinedBy <https://www.ica.org/standards/RiC/ontology> ;
    rdfs:range :Group ;
    rdfs:subPropertyOf :isAgentAssociatedWithAgent ;
    owl:inverseOf :hasOrHadPosition ;
    owl:propertyChainAxiom (
        :thingIsSourceOfRelation
        :positionToGroupRelation_role
        :relationHasTarget
    ) ;
    skos:changeNote
        [
            dc:date "2024-03-15" ;
            rdf:value "Corrected unparseable symbol in rdfs:comment"@en ;
        ] ,
        [
            dc:date "2023-08-28" ;
            rdf:value "Added a new rdfs:label in French."@en ;
        ] ,
        [
            dc:date "2023-11-02" ;
            rdf:value "Added a new rdfs:label in Spanish."@en ;
        ] ,
        [
            dc:date "2023-11-08" ;
            rdf:value """In order to get a system of rolified Relation classes: modified
               the property chain axiom so that it now involves the new positionToGroupRelation_role
               object property."""@en ;
        ] ,
        [
            dc:date "2021-01-22" ;
            rdf:value """changed the IRI, label, inverse property IRI, text definition,
               corresponding CM component name (changed made in order to make RiC-O compliant with
               RiC-CM 0.2; the name of this property in RiC-O 0.1 was "existsIn")."""@en ;
        ] ;
    :RiCCMCorrespondingComponent """RiC-R056 ('exists or existed in'
         relation)"""@en ;
.

:expressesOrExpressed
    a owl:ObjectProperty ;
    rdfs:label
        "expresses or expressed"@en ,
        "expresa o expresaba"@es ,
        "exprime ou a exprimé"@fr ;
    rdfs:comment """Inverse of 'is or was expressed by' object
         property."""@en ;
    rdfs:domain :RecordResource ;
    rdfs:isDefinedBy <https://www.ica.org/standards/RiC/ontology> ;
    rdfs:range :Rule ;
    rdfs:subPropertyOf :isAssociatedWithRule ;
    owl:inverseOf :isOrWasExpressedBy ;
    skos:changeNote
        [
            dc:date "2023-11-02" ;
            rdf:value "Added a new rdfs:label in Spanish."@en ;
        ] ,
        [
            dc:date "2021-01-22" ;
            rdf:value """changed the IRI, label, inverse property IRI, text definition,
               corresponding CM component name (changed made in order to make RiC-O compliant with
               RiC-CM 0.2; the name of this property in RiC-O 0.1 was "expresses")."""@en ;
        ] ,
        [
            dc:date "2023-08-28" ;
            rdf:value "Added a new rdfs:label in French."@en ;
        ] ;
    :RiCCMCorrespondingComponent """RiC-R064i ('expresses or expressed'
         relation)"""@en ;
.

:followedInSequence
    a owl:ObjectProperty ;
    rdfs:label
        "followed in sequence"@en ,
        "seguía en la secuencia transitivo"@es ,
        "a suivi dans la séquence"@fr ;
    rdfs:comment """Connects a Thing to a Thing that it followed in some non
         chronological sequence in the past."""@en ;
    rdfs:domain :Thing ;
    rdfs:isDefinedBy <https://www.ica.org/standards/RiC/ontology> ;
    rdfs:range :Thing ;
    rdfs:subPropertyOf :followsOrFollowed ;
    owl:inverseOf :precededInSequence ;
    skos:changeNote
        [
            dc:date "2023-09-22" ;
            rdf:value """Renamed the property and modified its definition (rdfs:comment)
               in order to better distinguish it from followsInTime."""@en ;
        ] ,
        [
            dc:date "2023-11-27" ;
            rdf:value "Added a new rdfs:label in Spanish."@en ;
        ] ,
        [
            dc:date "2023-11-12" ;
            rdf:value "Updated the description (rdfs:comment) and labels."@en ;
        ] ,
        [
            dc:date "2023-09-08" ;
            rdf:value """Added transitive super-property and both present direct and
               past sequential relations as well as their respective inverse relations."""@en ;
        ] ;
.

:generalDescription
    a owl:DatatypeProperty ;
    rdfs:label
        "general description"@en ,
        "descripción general"@es ,
        "description générale"@fr ;
    rdfs:comment """General information about an entity. General description may be
         used to describe any entity. There are different appropriate uses for general description.
         First, while it is recommended that more specific properties be used in describing an
         entity, it may be desirable, for economic or other reasons, to describe two or more
         specific properties together. Second, general description may be used to describe one or
         more characteristics that are not otherwise accommodated in RiC-O. Third, it may be used to
         provide a succinct summary or abstract description in addition to more detailed specific
         description."""@en ;
    rdfs:domain :Thing ;
    rdfs:isDefinedBy <https://www.ica.org/standards/RiC/ontology> ;
    rdfs:range rdfs:Literal ;
    skos:changeNote
        [
            dc:date "2023-11-11" ;
            rdf:value """Aligned with RiC-CM 1.0: updated the IRI, mapping to RiC-CM
               (rico:RiCCMCorrespondingComponent), labels, description (rdfs:comment), examples
               (skos:example)."""@en ;
        ] ,
        [
            dc:date "2023-08-25" ;
            rdf:value "Added a new rdfs:label in French."@en ;
        ] ,
        [
            dc:date "2023-11-02" ;
            rdf:value "Added a new rdfs:label in Spanish."@en ;
        ] ;
    skos:example
        """The Senate is the academic governing body of the University of
         Strathclyde and is responsible for all academic matters including academic standards and
         quality. Meetings of the Senate are chaired by the Principal and the membership is drawn
         entirely from within the University, comprising academic and research staff. (about a
         corporate body, University of Strathclyde Senate)"""@en ,
        """This activity involves regulating the nursing profession by
         conducting examinations and on-going education for nurses, maintaining rolls of those
         qualified as enrolled or registered nurses, midwives, psychiatric, and other specialised
         nurses. It also covers hearing disciplinary charges against nurses (and where necessary,
         removing them temporarily or permanently from the registers), as well as promoting the
         nursing profession. (about an activity, Nursing Profession Regulation)"""@en ,
        """Le massif du Mont-Blanc est un massif des Alpes partagé entre la
         France, l'Italie et la Suisse. Il abrite le mont Blanc, plus haut sommet d'Europe
         occidentale qui culmine à 4 809 mètres (altitude relevée en 2015). Il est traversé par le
         tunnel du Mont-Blanc, entre Chamonix dans la vallée de l'Arve et Courmayeur dans la vallée
         d'Aoste."""@fr ,
        """Thomas Blaikie (1750-1838) est un botaniste et jardinier écossais.
         Il a dessiné notamment les jardins de Malmaison et Bagatelle."""@fr ;
    :RiCCMCorrespondingComponent """Corresponds to RiC-A43 (General Description
         attribute)"""@en ;
.

:hadComponent
    a owl:ObjectProperty ;
    rdfs:label
        "had component"@en ,
        "tenía como componente"@es ,
        "a eu pour composant"@fr ;
    rdfs:comment """Connects an Instantiation to another Instantiation that was its
         component in the past."""@en ;
    rdfs:domain :Instantiation ;
    rdfs:isDefinedBy <https://www.ica.org/standards/RiC/ontology> ;
    rdfs:range :Instantiation ;
    rdfs:subPropertyOf
        :hadPart ,
        :hasOrHadComponent ;
    owl:inverseOf :wasComponentOf ;
    skos:changeNote
        [
            dc:date "2023-11-12" ;
            rdf:value "Updated the description (rdfs:comment) and labels."@en ;
        ] ,
        [
            dc:date "2023-09-08" ;
            rdf:value """Object property added, along with its inverse property, in
               order to enable to express past partitive relations between instantiations (the
               current partitive relations being also added, including a transitive
               one)."""@en ;
        ] ,
        [
            dc:date "2023-11-27" ;
            rdf:value "Added a new rdfs:label in Spanish."@en ;
        ] ;
.

:hadConstituent
    a owl:ObjectProperty ;
    rdfs:label
        "had constituent"@en ,
        "tenía como elemento constitutivo"@es ,
        "a eu pour constituant"@fr ;
    rdfs:comment """Connects a Record or Record Part to another Record or Record Part
         that was its constituent in the past."""@en ;
    rdfs:domain
        [
            a owl:Class ;
            owl:unionOf (
                :Record
                :RecordPart
            ) ;
        ] ;
    rdfs:isDefinedBy <https://www.ica.org/standards/RiC/ontology> ;
    rdfs:range
        [
            a owl:Class ;
            owl:unionOf (
                :Record
                :RecordPart
            ) ;
        ] ;
    rdfs:subPropertyOf
        :hadPart ,
        :hasOrHadConstituent ;
    owl:inverseOf :wasConstituentOf ;
    skos:changeNote
        [
            dc:date "2023-11-27" ;
            rdf:value "Added a new rdfs:label in Spanish."@en ;
        ] ,
        [
            dc:date "2023-11-12" ;
            rdf:value "Updated the labels."@en ;
        ] ,
        [
            dc:date "2023-10-26" ;
            rdf:value "Added RecordPart to the domain."@en ;
        ] ,
        [
            dc:date "2023-09-08" ;
            rdf:value """Object property added, along with its inverse property, in
               order to enable to express past partitive relations between Record and Record or
               Record Part (the current partitive relations being also added, including a transitive
               one)."""@en ;
        ] ;
.

:hadSubdivision
    a owl:ObjectProperty ;
    rdfs:label
        "had subdivision"@en ,
        "tenía como subdivisión"@es ,
        "a eu pour subdivision"@fr ;
    rdfs:comment "Connects a Group to one of its past subdivisions."@en ;
    rdfs:domain :Group ;
    rdfs:isDefinedBy <https://www.ica.org/standards/RiC/ontology> ;
    rdfs:range :Group ;
    rdfs:subPropertyOf
        :hadPart ,
        :hadSubordinate ,
        :hasOrHadSubdivision ;
    owl:inverseOf :wasSubdivisionOf ;
    skos:changeNote
        [
            dc:date "2023-11-27" ;
            rdf:value "Added a new rdfs:label in Spanish."@en ;
        ] ,
        [
            dc:date "2023-09-08" ;
            rdf:value """Object property added, along with its inverse property, in
               order to enable to express past partitive relations between groups (the current
               partitive relations being also added, including a transitive one)."""@en ;
        ] ,
        [
            dc:date "2023-11-12" ;
            rdf:value "Updated the labels."@en ;
        ] ;
.

:hadSubevent
    a owl:ObjectProperty ;
    rdfs:label
        "had subevent"@en ,
        "tenía como parte de evento"@es ,
        "a été constitué de l’événement"@fr ;
    rdfs:comment """Connects a past Event to one of a series of past Events that
         constituted that original, broader, past Event."""@en ;
    rdfs:domain :Event ;
    rdfs:isDefinedBy <https://www.ica.org/standards/RiC/ontology> ;
    rdfs:range :Event ;
    rdfs:subPropertyOf
        :hadPart ,
        :hasOrHadSubevent ;
    owl:inverseOf :wasSubeventOf ;
    skos:changeNote
        [
            dc:date "2023-11-27" ;
            rdf:value "Added a new rdfs:label in Spanish."@en ;
        ] ,
        [
            dc:date "2023-11-12" ;
            rdf:value "Updated the labels."@en ;
        ] ,
        [
            dc:date "2023-09-08"@en ;
            rdf:value """Object property added, along with its inverse property, in
               order to enable to express partitive relations between past Events (the partitive
               relations between ongoing events being also added, including a transitive
               one)."""@en ;
        ] ;
.

:hasActivityType
    a owl:ObjectProperty ;
    rdfs:label
        "has activity type"@en ,
        "tiene como tipo de actividad a"@es ,
        "a pour type d’activité"@fr ;
    rdfs:comment """Connects an Activity to an Activity Type that categorizes
         it."""@en ;
    rdfs:domain :Activity ;
    rdfs:isDefinedBy <https://www.ica.org/standards/RiC/ontology> ;
    rdfs:range :ActivityType ;
    rdfs:subPropertyOf :hasOrHadCategory ;
    owl:inverseOf :isActivityTypeOf ;
    skos:changeNote
        [
            dc:date "2023-08-28" ;
            rdf:value "Added a new rdfs:label in French."@en ;
        ] ,
        [
            dc:date "2023-11-02" ;
            rdf:value "Added a new rdfs:label in Spanish."@en ;
        ] ,
        [
            dc:date "2021-01-22" ;
            rdf:value "changed the superproperty IRI."@en ;
        ] ;
.

:hasAddressee
    a owl:ObjectProperty ;
    rdfs:label
        "has addressee"@en ,
        "se dirige a"@es ,
        "a pour destinataire"@fr ;
    rdfs:comment """Connects a Record Resource or an Instantiation to the Agent that
         it is addressed to."""@en ;
    rdfs:domain
        [
            a owl:Class ;
            owl:unionOf (
                :Instantiation
                :RecordResource
            ) ;
        ] ;
    rdfs:isDefinedBy <https://www.ica.org/standards/RiC/ontology> ;
    rdfs:range :Agent ;
    rdfs:subPropertyOf :hasOrganicProvenance ;
    owl:inverseOf :isAddresseeOf ;
    skos:changeNote
        [
            dc:date "2021-01-22" ;
            rdf:value "added a scope note"@en ;
        ] ,
        [
            dc:date "2023-08-28" ;
            rdf:value "Added a new rdfs:label in French."@en ;
        ] ,
        [
            dc:date "2023-11-02" ;
            rdf:value "Added a new rdfs:label in Spanish."@en ;
        ] ;
    skos:scopeNote """The identity of the addressee is (usually) evidenced by the
         Record Resource or Instantiation itself."""@en ;
    :RiCCMCorrespondingComponent """RiC-R032 ('has addressee'
         relation)"""@en ;
.

:hasAuthor
    a owl:ObjectProperty ;
    rdfs:label
        "has author"@en ,
        "tiene como autor a"@es ,
        "a pour responsable intellectuel"@fr ;
    rdfs:comment """Connects a Record to the Group, Person or Position that is
         responsible for conceiving and formulating the information contained in the
         Record."""@en ;
    rdfs:domain :Record ;
    rdfs:isDefinedBy <https://www.ica.org/standards/RiC/ontology> ;
    rdfs:range
        [
            a owl:Class ;
            owl:unionOf (
                :Group
                :Person
                :Position
            ) ;
        ] ;
    rdfs:subPropertyOf :hasCreator ;
    owl:inverseOf :isAuthorOf ;
    owl:propertyChainAxiom (
        :thingIsSourceOfRelation
        :authorshipRelation_role
        :relationHasTarget
    ) ;
    skos:changeNote
        [
            dc:date "2023-08-28" ;
            rdf:value "Added a new rdfs:label in French."@en ;
        ] ,
        [
            dc:date "2020-12-29" ;
            rdf:value """Created following the addition of RiC-R079 relation in RiC-CM
               0.2"""@en ;
        ] ,
        [
            dc:date "2023-11-08" ;
            rdf:value """In order to get a system of rolified Relation classes: modified
               the property chain axiom so that it now involves the new authorshipRelation_role
               object property."""@en ;
        ] ,
        [
            dc:date "2023-11-02" ;
            rdf:value "Added a new rdfs:label in Spanish."@en ;
        ] ,
        [
            dc:date "2023-11-12" ;
            rdf:value """Aligned with RiC-CM 1.0: updated the
               skos:scopeNote."""@en ;
        ] ;
    skos:scopeNote """To be used for a Person, Group or Position that makes any
         contribution to the content of a record. Includes the Person, Group or Position in whose
         name or by whose command the content may have been formulated and first instantiated (for
         example the Person who signed the Record)."""@en ;
    :RiCCMCorrespondingComponent """RiC-R079 ('has author'
         relation)"""@en ;
.

:hasBirthDate
    a owl:ObjectProperty ;
    rdfs:label
        "has birth date"@en ,
        "tiene como fecha de nacimiento"@es ,
        "a pour date de naissance"@fr ;
    rdfs:comment "Inverse of 'is birth date of' object property"@en ;
    rdfs:domain :Person ;
    rdfs:isDefinedBy <https://www.ica.org/standards/RiC/ontology> ;
    rdfs:range :Date ;
    rdfs:subPropertyOf :hasBeginningDate ;
    owl:inverseOf :isBirthDateOf ;
    skos:changeNote
        [
            dc:date "2023-11-02" ;
            rdf:value "Added a new rdfs:label in Spanish."@en ;
        ] ,
        [
            dc:date "2023-08-28" ;
            rdf:value "Added a new rdfs:label in French."@en ;
        ] ;
    :RiCCMCorrespondingComponent """RiC-R070i ('has birth date'
         relation)"""@en ;
.

:hasBirthPlace
    a owl:ObjectProperty ;
    rdfs:label
        "has birth place"@en ,
        "tiene como lugar de nacimiento"@es ,
        "a pour lieu de naissance"@fr ;
    rdfs:comment "Inverse of 'is birth place of' object property"@en ;
    rdfs:domain :Person ;
    rdfs:isDefinedBy <https://www.ica.org/standards/RiC/ontology> ;
    rdfs:range :Place ;
    rdfs:subPropertyOf :isAgentAssociatedWithPlace ;
    owl:inverseOf :isBirthPlaceOf ;
    skos:changeNote
        [
            dc:date "2023-10-19" ;
            rdf:value "Added for RiC-O 1.0."@en ;
        ] ,
        [
            dc:date "2023-10-26" ;
            rdf:value "Fixed the domain of the property."@en ;
        ] ,
        [
            dc:date "2023-11-27" ;
            rdf:value "Added a new rdfs:label in Spanish."@en ;
        ] ,
        [
            dc:date "2023-11-12" ;
            rdf:value "Updated the description (rdfs:comment)."@en ;
        ] ;
.

:hasCarrierType
    a owl:ObjectProperty ;
    rdfs:label
        "has carrier type"@en ,
        "tiene como tipo de soporte"@es ,
        "a pour type de support"@fr ;
    rdfs:comment """Connects an Instantiation to a Carrier Type which categorizes its
         carrier."""@en ;
    rdfs:domain :Instantiation ;
    rdfs:isDefinedBy <https://www.ica.org/standards/RiC/ontology> ;
    rdfs:range :CarrierType ;
    rdfs:subPropertyOf :hasOrHadCategory ;
    owl:inverseOf :isCarrierTypeOf ;
    skos:changeNote
        [
            dc:date "2023-08-28" ;
            rdf:value "Added a new rdfs:label in French."@en ;
        ] ,
        [
            dc:date "2021-01-22" ;
            rdf:value "changed the superproperty IRI."@en ;
        ] ,
        [
            dc:date "2023-11-02" ;
            rdf:value "Added a new rdfs:label in Spanish."@en ;
        ] ;
.

:hasChild
    a owl:ObjectProperty ;
    rdfs:label
        "has child"@en ,
        "tiene como hijo o hija a"@es ,
        "a pour enfant"@fr ;
    rdfs:comment "Connects a Person to one of their children."@en ;
    rdfs:domain :Person ;
    rdfs:isDefinedBy <https://www.ica.org/standards/RiC/ontology> ;
    rdfs:range :Person ;
    rdfs:subPropertyOf :hasDescendant ;
    owl:inverseOf :isChildOf ;
    owl:propertyChainAxiom (
        :thingIsSourceOfRelation
        :childRelation_role
        :relationHasTarget
    ) ;
    skos:changeNote
        [
            dc:date "2021-01-22" ;
            rdf:value "changed the inverse property IRI."@en ;
        ] ,
        [
            dc:date "2023-11-02" ;
            rdf:value "Added a new rdfs:label in Spanish."@en ;
        ] ,
        [
            dc:date "2023-11-08" ;
            rdf:value """In order to get a system of rolified Relation classes: modified
               the property chain axiom so that it now involves the new childRelation_role object
               property."""@en ;
        ] ,
        [
            dc:date "2023-08-28" ;
            rdf:value "Added a new rdfs:label in French."@en ;
        ] ;
    :RiCCMCorrespondingComponent """RiC-R018 ('has child'
         relation)"""@en ;
.

:hasCollector
    a owl:ObjectProperty ;
    rdfs:label
        "has collector"@en ,
        "tiene como coleccionista a"@es ,
        "est collecté par"@fr ;
    rdfs:comment """Connects a Record Resource or an Instantiation to the Agent that
         collects it intentionally, i.e., the Agent is a collector."""@en ;
    rdfs:domain
        [
            a owl:Class ;
            owl:unionOf (
                :Instantiation
                :RecordResource
            ) ;
        ] ;
    rdfs:isDefinedBy <https://www.ica.org/standards/RiC/ontology> ;
    rdfs:range :Agent ;
    rdfs:subPropertyOf :hasAccumulator ;
    owl:inverseOf :isCollectorOf ;
    skos:changeNote
        [
            dc:date "2023-08-28" ;
            rdf:value "Added a new rdfs:label in French."@en ;
        ] ,
        [
            dc:date "2023-11-12" ;
            rdf:value """Aligned with RiC-CM 1.0: updated the description
               (rdfs:comment)."""@en ;
        ] ,
        [
            dc:date "2021-01-22" ;
            rdf:value """changed the IRI, label, inverse property and super property
               IRI, text definition, domain (changed made in order to make RiC-O compliant with
               RiC-CM 0.2; the name of this property in RiC-O 0.1 was "collectedBy")."""@en ;
        ] ,
        [
            dc:date "2023-11-02" ;
            rdf:value "Added a new rdfs:label in Spanish."@en ;
        ] ;
    :RiCCMCorrespondingComponent """RiC-R030 ('has collector'
         relation)"""@en ;
.

:hasContentOfType
    a owl:ObjectProperty ;
    rdfs:label
        "has content of type"@en ,
        "tiene como tipo de contenido"@es ,
        "a pour type de contenu"@fr ;
    rdfs:comment """Connects a Record or a Record Part to a Content Type which
         categorizes its content."""@en ;
    rdfs:domain
        [
            a owl:Class ;
            owl:unionOf (
                :Record
                :RecordPart
            ) ;
        ] ;
    rdfs:isDefinedBy <https://www.ica.org/standards/RiC/ontology> ;
    rdfs:range :ContentType ;
    rdfs:subPropertyOf :hasOrHadCategory ;
    owl:inverseOf :isContentTypeOf ;
    skos:changeNote
        [
            dc:date "2021-01-22" ;
            rdf:value "changed the text definition and superproperty IRI."@en ;
        ] ,
        [
            dc:date "2023-08-28" ;
            rdf:value "Added a new rdfs:label in French."@en ;
        ] ,
        [
            dc:date "2023-11-02" ;
            rdf:value "Added a new rdfs:label in Spanish."@en ;
        ] ;
.

:hasCopy
    a owl:ObjectProperty ;
    rdfs:label
        "has copy"@en ,
        "tiene como copia"@es ,
        "a pour copie"@fr ;
    rdfs:comment """Connects a Record Resource to a copy of that Record
         Resource."""@en ;
    rdfs:domain :RecordResource ;
    rdfs:isDefinedBy <https://www.ica.org/standards/RiC/ontology> ;
    rdfs:range :RecordResource ;
    rdfs:subPropertyOf
        :hasGeneticLinkToRecordResource ,
        :precedesInTime ;
    owl:inverseOf :isCopyOf ;
    skos:changeNote
        [
            dc:date "2023-11-12" ;
            rdf:value """Aligned with RiC-CM 1.0: updated the
               skos:scopeNote."""@en ;
        ] ,
        [
            dc:date "2023-08-28" ;
            rdf:value "Added a new rdfs:label in French."@en ;
        ] ,
        [
            dc:date "2023-11-02" ;
            rdf:value "Added a new rdfs:label in Spanish."@en ;
        ] ;
    skos:scopeNote """Is both a temporal and genetic relation between the two Record
         Resources."""@en ;
    :RiCCMCorrespondingComponent """RiC-R012 ('has copy'
         relation)"""@en ;
.

:hasCreationDate
    a owl:ObjectProperty ;
    rdfs:label
        "has creation date"@en ,
        "tiene como fecha de creación"@es ,
        "a pour date de création"@fr ;
    rdfs:comment "Inverse of 'is creation date of' object property"@en ;
    rdfs:domain
        [
            a owl:Class ;
            owl:unionOf (
                :Instantiation
                :RecordResource
            ) ;
        ] ;
    rdfs:isDefinedBy <https://www.ica.org/standards/RiC/ontology> ;
    rdfs:range :Date ;
    rdfs:subPropertyOf :hasBeginningDate ;
    owl:inverseOf :isCreationDateOf ;
    skos:changeNote
        [
            dc:date "2023-11-27" ;
            rdf:value "Added a new rdfs:label in Spanish."@en ;
        ] ,
        [
            dc:date "2023-09-22" ;
            rdf:value "Added in RiC-O 1.0."@en ;
        ] ;
    :RiCCMCorrespondingComponent """RiC-R080i ('has creation date'
         relation)"""@en ;
.

:hasDateType
    a owl:ObjectProperty ;
    rdfs:label
        "has date type"@en ,
        "tiene como tipo de fecha"@es ,
        "a pour type de date"@fr ;
    rdfs:comment "Connects a Date to its Date Type."@en ;
    rdfs:domain :Date ;
    rdfs:isDefinedBy <https://www.ica.org/standards/RiC/ontology> ;
    rdfs:range :DateType ;
    rdfs:subPropertyOf :hasOrHadCategory ;
    owl:inverseOf :isDateTypeOf ;
    skos:changeNote
        [
            dc:date "2023-09-22" ;
            rdf:value "Added in RiC-O 1.0."@en ;
        ] ,
        [
            dc:date "2023-10-10" ;
            rdf:value "Added a rdfs:comment and a French rdfs:label."@en ;
        ] ,
        [
            dc:date "2023-11-27" ;
            rdf:value "Added a new rdfs:label in Spanish."@en ;
        ] ;
.

:hasDeathDate
    a owl:ObjectProperty ;
    rdfs:label
        "has death date"@en ,
        "tiene como fecha de muerte"@es ,
        "a pour date de décès"@fr ;
    rdfs:comment "Inverse of 'is death date of' object property"@en ;
    rdfs:domain :Person ;
    rdfs:isDefinedBy <https://www.ica.org/standards/RiC/ontology> ;
    rdfs:range :Date ;
    rdfs:subPropertyOf :hasEndDate ;
    owl:inverseOf :isDeathDateOf ;
    skos:changeNote
        [
            dc:date "2023-08-28" ;
            rdf:value "Added a new rdfs:label in French."@en ;
        ] ,
        [
            dc:date "2023-11-02" ;
            rdf:value "Added a new rdfs:label in Spanish."@en ;
        ] ;
    :RiCCMCorrespondingComponent """RiC-R072i ('has death date'
         relation)"""@en ;
.

:hasDeathPlace
    a owl:ObjectProperty ;
    rdfs:label
        "has death place"@en ,
        "tiene como lugar de muerte"@es ,
        "a pour lieu de décès"@fr ;
    rdfs:comment "Inverse of 'is death place of' object property"@en ;
    rdfs:domain :Person ;
    rdfs:isDefinedBy <https://www.ica.org/standards/RiC/ontology> ;
    rdfs:range :Place ;
    rdfs:subPropertyOf :isAgentAssociatedWithPlace ;
    owl:inverseOf :isDeathPlaceOf ;
    skos:changeNote
        [
            dc:date "2023-10-26" ;
            rdf:value "Fixed the domain of the property."@en ;
        ] ,
        [
            dc:date "2023-10-19" ;
            rdf:value "Added for RiC-O v1.0."@en ;
        ] ,
        [
            dc:date "2023-11-13" ;
            rdf:value "Added a rdfs:comment."@en ;
        ] ,
        [
            dc:date "2023-11-27" ;
            rdf:value "Added a new rdfs:label in Spanish."@en ;
        ] ;
.

:hasDestructionDate
    a owl:ObjectProperty ;
    rdfs:label
        "has destruction date"@en ,
        "tiene como fecha de destrucción"@es ,
        "a pour date de destruction"@fr ;
    rdfs:comment """Inverse of 'is destruction date of' object
         property."""@en ;
    rdfs:domain :Thing ;
    rdfs:isDefinedBy <https://www.ica.org/standards/RiC/ontology> ;
    rdfs:range :Date ;
    rdfs:subPropertyOf :hasEndDate ;
    owl:inverseOf :isDestructionDateOf ;
    skos:changeNote
        [
            dc:date "2023-09-22" ;
            rdf:value "Added in RiC-O 1.0."@en ;
        ] ,
        [
            dc:date "2023-10-12" ;
            rdf:value "Renamed deletion into destruction"@en ;
        ] ,
        [
            dc:date "2023-11-27" ;
            rdf:value "Added a new rdfs:label in Spanish."@en ;
        ] ,
        [
            dc:date "2023-10-14" ;
            rdf:value "Added a rdfs:comment; same to the inverse property."@en ;
        ] ;
.

:hasDirectComponent
    a owl:ObjectProperty ;
    rdfs:label
        "has direct component"@en ,
        "tiene directamente como componente"@es ,
        "a directement pour composant"@fr ;
    rdfs:comment """Connects an Instantiation to another Instantiation that is its
         direct component."""@en ;
    rdfs:domain :Instantiation ;
    rdfs:isDefinedBy <https://www.ica.org/standards/RiC/ontology> ;
    rdfs:range :Instantiation ;
    rdfs:subPropertyOf
        :hasComponentTransitive ,
        :hasDirectPart ;
    owl:inverseOf :isDirectComponentOf ;
    skos:changeNote
        [
            dc:date "2023-11-27" ;
            rdf:value "Added a new rdfs:label in Spanish."@en ;
        ] ,
        [
            dc:date "2023-11-12" ;
            rdf:value "Updated the labels."@en ;
        ] ,
        [
            dc:date "2023-09-08" ;
            rdf:value """Object property added, along with its inverse property, in
               order to enable to express current, direct, partitive relations between
               instantiations (the possibly indirect, transitive relation, superproperty of this
               one, being also added)."""@en ;
        ] ;
.

:hasDirectConstituent
    a owl:ObjectProperty ;
    rdfs:label
        "has direct constituent"@en ,
        "tiene directamente como elemento constitutivo"@es ,
        "a directement pour constituant"@fr ;
    rdfs:comment """Connects a Record to another Record or Record Part that is its
         direct constituent."""@en ;
    rdfs:domain
        [
            a owl:Class ;
            owl:unionOf (
                :Record
                :RecordPart
            ) ;
        ] ;
    rdfs:isDefinedBy <https://www.ica.org/standards/RiC/ontology> ;
    rdfs:range
        [
            a owl:Class ;
            owl:unionOf (
                :Record
                :RecordPart
            ) ;
        ] ;
    rdfs:subPropertyOf
        :hasConstituentTransitive ,
        :hasDirectPart ;
    owl:inverseOf :isDirectConstituentOf ;
    skos:changeNote
        [
            dc:date "2023-11-12" ;
            rdf:value "Updated the labels."@en ;
        ] ,
        [
            dc:date "2023-11-27" ;
            rdf:value "Added a new rdfs:label in Spanish."@en ;
        ] ,
        [
            dc:date "2023-09-08" ;
            rdf:value """Object property added, along with its inverse property, in
               order to enable to express current, direct, partitive relations between records and
               other records or record parts (the possibly indirect, transitive relation,
               superproperty of this one, being also added)."""@en ;
        ] ,
        [
            dc:date "2023-10-26" ;
            rdf:value "Added RecordPart to the domain."@en ;
        ] ;
.

:hasDirectSubdivision
    a owl:ObjectProperty ;
    rdfs:label
        "has direct subdivision"@en ,
        "tiene directamente como subdivisión"@es ,
        "a directement pour subdivision"@fr ;
    rdfs:comment "Connects a Group to one of its direct subdivisions."@en ;
    rdfs:domain :Group ;
    rdfs:isDefinedBy <https://www.ica.org/standards/RiC/ontology> ;
    rdfs:range :Group ;
    rdfs:subPropertyOf
        :hasDirectPart ,
        :hasDirectSubordinate ,
        :hasSubdivisionTransitive ;
    owl:inverseOf :isDirectSubdivisionOf ;
    skos:changeNote
        [
            dc:date "2023-11-27" ;
            rdf:value "Added a new rdfs:label in Spanish."@en ;
        ] ,
        [
            dc:date "2023-11-12" ;
            rdf:value "Updated the labels."@en ;
        ] ,
        [
            dc:date "2023-09-08" ;
            rdf:value """Object property added, along with its inverse property, in
               order to enable to express current, direct, partitive relations between groups (the
               possibly indirect, transitive relation, superproperty of this one, being also
               added)."""@en ;
        ] ;
.

:hasDirectSubevent
    a owl:ObjectProperty ;
    rdfs:label
        "has direct subevent"@en ,
        "tiene directamente como parte de evento"@es ,
        "est directement constitué de l’événement"@fr ;
    rdfs:comment """Connects an ongoing Event to one of a series of Events that
         directly constitute that broader, ongoing Event."""@en ;
    rdfs:domain :Event ;
    rdfs:isDefinedBy <https://www.ica.org/standards/RiC/ontology> ;
    rdfs:range :Event ;
    rdfs:subPropertyOf
        :hasDirectPart ,
        :hasSubeventTransitive ;
    owl:inverseOf :isDirectSubeventOf ;
    skos:changeNote
        [
            dc:date "2023-11-12" ;
            rdf:value "Updated the labels."@en ;
        ] ,
        [
            dc:date "2023-09-08" ;
            rdf:value """Object property added, along with its inverse property, in
               order to enable to express current, direct, partitive relations between ongoing
               events (the possibly indirect, transitive relation, superproperty of this one, being
               also added)."""@en ;
        ] ,
        [
            dc:date "2023-11-27" ;
            rdf:value "Added a new rdfs:label in Spanish."@en ;
        ] ;
.

:hasDocumentaryFormType
    a owl:ObjectProperty ;
    rdfs:label
        "has documentary form type"@en ,
        "tiene como tipo documental"@es ,
        "a pour type d’objet informationnel"@fr ;
    rdfs:comment """Connects a Record or Record Part to its Documentary Form
         Type."""@en ;
    rdfs:domain
        [
            a owl:Class ;
            owl:unionOf (
                :Record
                :RecordPart
            ) ;
        ] ;
    rdfs:isDefinedBy <https://www.ica.org/standards/RiC/ontology> ;
    rdfs:range :DocumentaryFormType ;
    rdfs:subPropertyOf :hasOrHadCategory ;
    owl:inverseOf :isDocumentaryFormTypeOf ;
    skos:changeNote
        [
            dc:date "2023-11-02" ;
            rdf:value "Added a new rdfs:label in Spanish."@en ;
        ] ,
        [
            dc:date "2021-01-22" ;
            rdf:value "changed the superproperty IRI."@en ;
        ] ,
        [
            dc:date "2023-12-30" ;
            rdf:value "Fixed a typo in the French label."@en ;
        ] ,
        [
            dc:date "2023-08-28" ;
            rdf:value "Added a new rdfs:label in French."@en ;
        ] ;
.

:hasDraft
    a owl:ObjectProperty ;
    rdfs:label
        "has draft"@en ,
        "tiene como borrador"@es ,
        "a pour ébauche"@fr ;
    rdfs:comment "Inverse of 'is draft of' object property."@en ;
    rdfs:domain
        [
            a owl:Class ;
            owl:unionOf (
                :Record
                :RecordPart
            ) ;
        ] ;
    rdfs:isDefinedBy <https://www.ica.org/standards/RiC/ontology> ;
    rdfs:range
        [
            a owl:Class ;
            owl:unionOf (
                :Record
                :RecordPart
            ) ;
        ] ;
    rdfs:subPropertyOf
        :followsInTime ,
        :hasGeneticLinkToRecordResource ;
    owl:inverseOf :isDraftOf ;
    skos:changeNote
        [
            dc:date "2023-11-02" ;
            rdf:value "Added a new rdfs:label in Spanish."@en ;
        ] ,
        [
            dc:date "2023-08-28" ;
            rdf:value "Added a new rdfs:label in French."@en ;
        ] ;
    :RiCCMCorrespondingComponent """RiC-011i ('has draft'
         relation)"""@en ;
.

:hasEventType
    a owl:ObjectProperty ;
    rdfs:label
        "has event type"@en ,
        "tiene como tipo de evento"@es ,
        "a pour type d’événement"@fr ;
    rdfs:comment """Connects an Event to an Event Type which categorizes
         it."""@en ;
    rdfs:domain :Event ;
    rdfs:isDefinedBy <https://www.ica.org/standards/RiC/ontology> ;
    rdfs:range :EventType ;
    rdfs:subPropertyOf :hasOrHadCategory ;
    owl:inverseOf :isEventTypeOf ;
    skos:changeNote
        [
            dc:date "2023-11-02" ;
            rdf:value "Added a new rdfs:label in Spanish."@en ;
        ] ,
        [
            dc:date "2023-08-28" ;
            rdf:value "Added a new rdfs:label in French."@en ;
        ] ,
        [
            dc:date "2021-01-22" ;
            rdf:value "changed the superproperty IRI."@en ;
        ] ;
.

:hasExtent
    a owl:ObjectProperty ;
    rdfs:label
        "has extent"@en ,
        "tiene como extensión"@es ,
        "a pour mesure"@fr ;
    rdfs:comment """Connects a Record Resource or Instantiation to an
         Extent"""@en ;
    rdfs:domain :Thing ;
    rdfs:isDefinedBy <https://www.ica.org/standards/RiC/ontology> ;
    rdfs:range :Extent ;
    rdfs:subPropertyOf :isRelatedTo ;
    owl:inverseOf :isExtentOf ;
    skos:changeNote
        [
            dc:date "2023-08-28" ;
            rdf:value """Added a new rdfs:label in French; added an xml:lang attribute
               to the rdfs:comment."""@en ;
        ] ,
        [
            dc:date "2020-10-28" ;
            rdf:value """Object property created along with the Extent class and its
               subclasses, in order to provide methods for handling extent accurately."""@en ;
        ] ,
        [
            dc:date "2023-08-28" ;
            rdf:value """Changed the domain (was Instantiation or RecordResource) to
               Thing; changed the definition accordingly."""@en ;
        ] ,
        [
            dc:date "2023-11-02" ;
            rdf:value "Added a new rdfs:label in Spanish."@en ;
        ] ;
.

:hasExtentType
    a owl:ObjectProperty ;
    rdfs:label
        "has extent type"@en ,
        "tiene como tipo de extensión"@es ,
        "a pour type de mesure"@fr ;
    rdfs:comment """Connects an Extent to an Extent Type that categorizes what is
         being measured."""@en ;
    rdfs:domain :Extent ;
    rdfs:isDefinedBy <https://www.ica.org/standards/RiC/ontology> ;
    rdfs:range :ExtentType ;
    rdfs:subPropertyOf :hasOrHadCategory ;
    owl:inverseOf :isExtentTypeOf ;
    skos:changeNote
        [
            dc:date "2023-08-28" ;
            rdf:value """Added a new rdfs:label in French; added an xml:lang attribute
               to the rdfs:comment."""@en ;
        ] ,
        [
            dc:date "2023-11-02" ;
            rdf:value "Added a new rdfs:label in Spanish."@en ;
        ] ,
        [
            dc:date "2020-11-01" ;
            rdf:value """Object property added along with the Extent Type
               class."""@en ;
        ] ;
.

:hasFamilyType
    a owl:ObjectProperty ;
    rdfs:label
        "has family type"@en ,
        "tiene como tipo de familia"@es ,
        "a pour type de famille"@fr ;
    rdfs:comment """Connects a Family to a Family Type that categorizes
         it."""@en ;
    rdfs:domain :Family ;
    rdfs:isDefinedBy <https://www.ica.org/standards/RiC/ontology> ;
    rdfs:range :FamilyType ;
    rdfs:subPropertyOf :hasOrHadCategory ;
    owl:inverseOf :isFamilyTypeOf ;
    skos:changeNote
        [
            dc:date "2021-01-22" ;
            rdf:value "changed the superproperty IRI."@en ;
        ] ,
        [
            dc:date "2023-08-28" ;
            rdf:value "Added a new rdfs:label in French."@en ;
        ] ,
        [
            dc:date "2023-11-02" ;
            rdf:value "Added a new rdfs:label in Spanish."@en ;
        ] ;
.

:hasIdentifierType
    a owl:ObjectProperty ;
    rdfs:label
        "has identifier type"@en ,
        "tiene como tipo de identificador"@es ,
        "a pour type d’identifiant"@fr ;
    rdfs:comment """Connects an Identifier and an Identifier Type that categorizes
         it."""@en ;
    rdfs:domain :Identifier ;
    rdfs:isDefinedBy <https://www.ica.org/standards/RiC/ontology> ;
    rdfs:range :IdentifierType ;
    rdfs:subPropertyOf :hasOrHadCategory ;
    owl:inverseOf :isIdentifierTypeOf ;
    skos:changeNote
        [
            dc:date "2021-01-22" ;
            rdf:value "changed the superproperty IRI."@en ;
        ] ,
        [
            dc:date "2023-11-02" ;
            rdf:value "Added a new rdfs:label in Spanish."@en ;
        ] ,
        [
            dc:date "2020-10-19" ;
            rdf:value """Object property added along with IdentifierType class and
               isIdentifierTypeOf object property. """@en ;
        ] ,
        [
            dc:date "2023-08-28" ;
            rdf:value "Added a new rdfs:label in French."@en ;
        ] ;
.

:hasOrHadAgentName
    a owl:ObjectProperty ;
    rdfs:label
        "has or had agent name"@en ,
        "tiene o tenía como nombre de agente"@es ,
        "a ou a eu pour nom d’agent"@fr ;
    rdfs:comment """Connects an Agent and (one of) its present or past Agent
         Name."""@en ;
    rdfs:domain :Agent ;
    rdfs:isDefinedBy <https://www.ica.org/standards/RiC/ontology> ;
    rdfs:range :AgentName ;
    rdfs:subPropertyOf :hasOrHadName ;
    owl:inverseOf :isOrWasAgentNameOf ;
    skos:changeNote
        [
            dc:date "2021-01-22" ;
            rdf:value """changed the IRI, label, inverse property IRI, textual
               definition (the name of this property in RiC-O 0.1 was "hasAgentName")."""@en ;
        ] ,
        [
            dc:date "2023-08-28" ;
            rdf:value "Added a new rdfs:label in French."@en ;
        ] ,
        [
            dc:date "2023-11-02" ;
            rdf:value "Added a new rdfs:label in Spanish."@en ;
        ] ;
.

:hasOrHadAllMembersWithContentType
    a owl:ObjectProperty ;
    rdfs:label
        "has or had all members with content type"@en ,
        """tienen o tenían todos sus miembros como tipo de
         contenido"""@es ,
        """inclut ou a inclus des membres ayant tous pour type de
         contenu"""@fr ;
    rdfs:comment """Connects a Record Set and a Content Type that categorizes all the
         Records or Record Parts that are or were included in the Record Set."""@en ;
    rdfs:domain :RecordSet ;
    rdfs:isDefinedBy <https://www.ica.org/standards/RiC/ontology> ;
    rdfs:range :ContentType ;
    rdfs:subPropertyOf :hasOrHadAllMembersWithCategory ;
    owl:inverseOf :isOrWasContentTypeOfAllMembersOf ;
    skos:changeNote
        [
            dc:date "2023-08-28" ;
            rdf:value "Added a new rdfs:label in French."@en ;
        ] ,
        [
            dc:date "2020-12-28" ;
            rdf:value """Object property added for handling the case where a Record Set
               is described as having all or some members that belong to some category (see RiC-CM
               0.2 attributes section, #4.4 on Record Set, Record and Record Part
               attributes)."""@en ;
        ] ,
        [
            dc:date "2023-11-02" ;
            rdf:value "Added a new rdfs:label in Spanish."@en ;
        ] ;
.

:hasOrHadAllMembersWithCreationDate
    a owl:ObjectProperty ;
    rdfs:label
        "has or had all members with creation date"@en ,
        """tienen o tenían todos sus miembros como fecha de
         creación"""@es ,
        """inclut ou a inclus des membres ayant tous pour date de
         création"""@fr ;
    rdfs:comment """Inverse of 'is or was creation date of all members of' object
         property"""@en ;
    rdfs:domain :RecordSet ;
    rdfs:isDefinedBy <https://www.ica.org/standards/RiC/ontology> ;
    rdfs:range :Date ;
    rdfs:subPropertyOf :hasBeginningDate ;
    owl:inverseOf :isOrWasCreationDateOfAllMembersOf ;
    skos:changeNote
        [
            dc:date "2023-10-12" ;
            rdf:value "Added the French label"@en ;
        ] ,
        [
            dc:date "2023-10-13" ;
            rdf:value """Renamed the property in order to take the past members of the
               record set into account. Adjusted the annotations accordingly."""@en ;
        ] ,
        [
            dc:date "2023-09-22" ;
            rdf:value "Added in RiC-O 1.0."@en ;
        ] ,
        [
            dc:date "2023-11-27" ;
            rdf:value "Added a new rdfs:label in Spanish."@en ;
        ] ;
    :RiCCMCorrespondingComponent """RiC-R081i ('has or had all members with creation
         date' relation)"""@en ;
.

:hasOrHadAllMembersWithDocumentaryFormType
    a owl:ObjectProperty ;
    rdfs:label
        "has or had all members with documentary form type"@en ,
        "tienen o tenían todos sus miembros como tipo documental"@es ,
        "inclut ou a inclus des membres ayant tous pour type"@fr ;
    rdfs:comment """Connects a Record Set and a Documentary Form Type that categorizes
         all the Records or Record Parts that are or were included in the Record Set."""@en ;
    rdfs:domain :RecordSet ;
    rdfs:isDefinedBy <https://www.ica.org/standards/RiC/ontology> ;
    rdfs:range :DocumentaryFormType ;
    rdfs:subPropertyOf :hasOrHadAllMembersWithCategory ;
    owl:inverseOf :isOrWasDocumentaryFormTypeOfAllMembersOf ;
    skos:changeNote
        [
            dc:date "2023-08-28" ;
            rdf:value "Added a new rdfs:label in French."@en ;
        ] ,
        [
            dc:date "2020-12-28" ;
            rdf:value """Object property added for handling the case where a Record Set
               is described as having all or some members that belong to some category (see RiC-CM
               0.2 attributes section, #4.4 on Record Set, Record and Record Part
               attributes)."""@en ;
        ] ,
        [
            dc:date "2023-11-02" ;
            rdf:value "Added a new rdfs:label in Spanish."@en ;
        ] ;
.

:hasOrHadAllMembersWithLanguage
    a owl:ObjectProperty ;
    rdfs:label
        "has or had all members with language"@en ,
        "tienen o tenían todos sus miembros como lengua"@es ,
        "inclut ou a inclus des membres ayant tous pour langue"@fr ;
    rdfs:comment """Connects a Record Set and a Language used by all the Records or
         Record Parts that are or were included in the Record Set."""@en ;
    rdfs:domain :RecordSet ;
    rdfs:isDefinedBy <https://www.ica.org/standards/RiC/ontology> ;
    rdfs:range :Language ;
    rdfs:subPropertyOf :isRelatedTo ;
    owl:inverseOf :isOrWasLanguageOfAllMembersOf ;
    skos:changeNote
        [
            dc:date "2023-08-28" ;
            rdf:value "Added a new rdfs:label in French."@en ;
        ] ,
        [
            dc:date "2023-11-02" ;
            rdf:value "Added a new rdfs:label in Spanish."@en ;
        ] ,
        [
            dc:date "2020-12-28" ;
            rdf:value """Object property added for handling the case where a Record Set
               is described as having all or some members that belong to some category (see RiC-CM
               0.2 attributes section, #4.4 on Record Set, Record and Record Part
               attributes)."""@en ;
        ] ;
.

:hasOrHadAllMembersWithLegalStatus
    a owl:ObjectProperty ;
    rdfs:label
        "has or had all members with legal status"@en ,
        "tienen o tenían todos sus miembros como status jurídico"@es ,
        """inclut ou a inclus des membres ayant tous pour statut
         légal"""@fr ;
    rdfs:comment """Connects a Record Set and a Legal Status that categorizes all the
         Records or Record Parts that are or were included in the Record Set."""@en ;
    rdfs:domain :RecordSet ;
    rdfs:isDefinedBy <https://www.ica.org/standards/RiC/ontology> ;
    rdfs:range :LegalStatus ;
    rdfs:subPropertyOf :hasOrHadAllMembersWithCategory ;
    owl:inverseOf :isOrWasLegalStatusOfAllMembersOf ;
    skos:changeNote
        [
            dc:date "2023-11-02" ;
            rdf:value "Added a new rdfs:label in Spanish."@en ;
        ] ,
        [
            dc:date "2023-08-28" ;
            rdf:value "Added a new rdfs:label in French."@en ;
        ] ,
        [
            dc:date "2020-12-28" ;
            rdf:value """Object property added for handling the case where a Record Set
               is described as having all or some members that belong to some category (see RiC-CM
               0.2 attributes section, #4.4 on Record Set, Record and Record Part
               attributes)."""@en ;
        ] ;
.

:hasOrHadAllMembersWithRecordState
    a owl:ObjectProperty ;
    rdfs:label
        "has or had all members with record state"@en ,
        """tiene o tenían todos sus miembros como estado de
         documento"""@es ,
        "inclut ou a inclus des membres ayant tous pour état"@fr ;
    rdfs:comment """Connects a Record Set and a Record State that categorizes all the
         Records or Record Parts that are or were included in the Record Set."""@en ;
    rdfs:domain :RecordSet ;
    rdfs:isDefinedBy <https://www.ica.org/standards/RiC/ontology> ;
    rdfs:range :RecordState ;
    rdfs:subPropertyOf :hasOrHadAllMembersWithCategory ;
    owl:inverseOf :isOrWasRecordStateOfAllMembersOf ;
    skos:changeNote
        [
            dc:date "2023-11-02" ;
            rdf:value "Added a new rdfs:label in Spanish."@en ;
        ] ,
        [
            dc:date "2020-12-28" ;
            rdf:value """Object property added for handling the case where a Record Set
               is described as having all or some members that belong to some category (see RiC-CM
               0.2 attributes section, #4.4 on Record Set, Record and Record Part
               attributes)."""@en ;
        ] ,
        [
            dc:date "2023-08-28" ;
            rdf:value "Added a new rdfs:label in French."@en ;
        ] ;
.

:hasOrHadAnalogueInstantiation
    a owl:ObjectProperty ;
    rdfs:label
        "has or had analogue instantiation"@en ,
        "tiene o tenía como instanciación analogica"@es ,
        "a ou a eu pour instanciation analogique"@fr ;
    rdfs:comment """Connects a record resource to one of its analogue instantiations,
         whether it exists or has been lost or destroyed."""@en ;
    rdfs:domain :RecordResource ;
    rdfs:isDefinedBy <https://www.ica.org/standards/RiC/ontology> ;
    rdfs:range :Instantiation ;
    rdfs:subPropertyOf :hasOrHadInstantiation ;
    owl:inverseOf :isOrWasAnalogueInstantiationOf ;
    skos:changeNote
        [
            dc:date "2023-08-29" ;
            rdf:value "Added the property."@en ;
        ] ,
        [
            dc:date "2023-11-27" ;
            rdf:value "Added a new rdfs:label in Spanish."@en ;
        ] ;
    skos:scopeNote """In some situations, it may be useful or necessary to connect a
         record resource to an analogue instantiation that no longer exists or has been
         lost."""@en ;
.

:hasOrHadCoordinates
    a owl:ObjectProperty ;
    rdfs:label
        "has or had coordinates"@en ,
        "tiene como coordenadas de lugar"@es ,
        "a ou a eu pour coordonnées"@fr ;
    rdfs:comment """Connects a Physical Location to its past or present coordinates in
         a reference system."""@en ;
    rdfs:domain :PhysicalLocation ;
    rdfs:isDefinedBy <https://www.ica.org/standards/RiC/ontology> ;
    rdfs:range :Coordinates ;
    rdfs:subPropertyOf :isRelatedTo ;
    owl:inverseOf :isOrWasCoordinatesOf ;
    skos:changeNote
        [
            dc:date "2023-08-28" ;
            rdf:value "Added a new rdfs:label in French."@en ;
        ] ,
        [
            dc:date "2021-01-22" ;
            rdf:value """changed the IRI, label, inverse property IRI, textual
               definition (the name of this property in RiC-O 0.1 was "hasCoordinates")."""@en ;
        ] ,
        [
            dc:date "2023-11-02" ;
            rdf:value "Added a new rdfs:label in Spanish."@en ;
        ] ,
        [
            dc:date "2023-08-29" ;
            rdf:value "fixed the English label (added the past tense.)"@en ;
        ] ;
.

:hasOrHadCorporateBodyType
    a owl:ObjectProperty ;
    rdfs:label
        "has or had corporate body type"@en ,
        "tiene o tenía como tipo de institucion"@es ,
        "a ou a eu pour type de collectivité"@fr ;
    rdfs:comment """Connects a Corporate Body to a Corporate Body Type which
         categorizes or categorized it."""@en ;
    rdfs:domain :CorporateBody ;
    rdfs:isDefinedBy <https://www.ica.org/standards/RiC/ontology> ;
    rdfs:range :CorporateBodyType ;
    rdfs:subPropertyOf :hasOrHadCategory ;
    owl:inverseOf :isOrWasCorporateBodyTypeOf ;
    skos:changeNote
        [
            dc:date "2021-01-22" ;
            rdf:value """changed the IRI, label, inverse property IRI, textual
               definition (the name of this property in RiC-O 0.1 was
               "hasCorporateBodyType")."""@en ;
        ] ,
        [
            dc:date "2023-11-02" ;
            rdf:value "Added a new rdfs:label in Spanish."@en ;
        ] ,
        [
            dc:date "2023-08-28" ;
            rdf:value "Added a new rdfs:label in French."@en ;
        ] ;
.

:hasOrHadDigitalInstantiation
    a owl:ObjectProperty ;
    rdfs:label
        "has or had digital instantiation"@en ,
        "tiene o tenía como instanciación digital"@es ,
        "a ou a eu pour instanciation numérique"@fr ;
    rdfs:comment """Connects a record resource to one of its digital instantiations,
         whether it exists or has been lost or destroyed."""@en ;
    rdfs:domain :RecordResource ;
    rdfs:isDefinedBy <https://www.ica.org/standards/RiC/ontology> ;
    rdfs:range :Instantiation ;
    rdfs:subPropertyOf :hasOrHadInstantiation ;
    owl:inverseOf :isOrWasDigitalInstantiationOf ;
    skos:changeNote
        [
            dc:date "2023-08-29" ;
            rdf:value "Added the property."@en ;
        ] ,
        [
            dc:date "2023-11-27" ;
            rdf:value "Added a new rdfs:label in Spanish."@en ;
        ] ;
    skos:scopeNote """This property can be used, among other cases, when you want to
         convert findings aids encoded in EAD/XML and need a simple and accurate migration path to
         process dao or daogrp EAD elements. Also, in some situations, it may be useful or necessary
         to connect a record resource to a digital instantiation that no longer exists or or has
         been lost."""@en ;
.

:hasOrHadEmployer
    a owl:ObjectProperty ;
    rdfs:label
        "has or had employer"@en ,
        "tiene o tenía como empleador"@es ,
        "a ou a eu pour employeur"@fr ;
    rdfs:comment "Inverse of 'is or was employer of' object property."@en ;
    rdfs:domain :Person ;
    rdfs:isDefinedBy <https://www.ica.org/standards/RiC/ontology> ;
    rdfs:range
        [
            a owl:Class ;
            owl:unionOf (
                :CorporateBody
                :Person
            ) ;
        ] ;
    rdfs:subPropertyOf :hasOrHadController ;
    owl:inverseOf :isOrWasEmployerOf ;
    skos:changeNote
        [
            dc:date "2023-10-13" ;
            rdf:value "Fixed the lang of the French label."@en ;
        ] ,
        [
            dc:date "2023-10-19" ;
            rdf:value "Added for RiC-O 1.0."@en ;
        ] ,
        [
            dc:date "2023-11-27" ;
            rdf:value "Added a new rdfs:label in Spanish."@en ;
        ] ,
        [
            dc:date "2023-10-26" ;
            rdf:value """Changed the domain and range of the property. Added a
               rdfs:comment. Removed the isOrWasMemberOf super-property."""@en ;
        ] ;
.

:hasOrHadHolder
    a owl:ObjectProperty ;
    rdfs:label
        "has or had holder"@en ,
        "tiene o tenía como conservador a"@es ,
        "est ou a été détenu par"@fr ;
    rdfs:comment "Inverse of 'is or was holder of' object property."@en ;
    rdfs:domain
        [
            a owl:Class ;
            owl:unionOf (
                :Instantiation
                :RecordResource
            ) ;
        ] ;
    rdfs:isDefinedBy <https://www.ica.org/standards/RiC/ontology> ;
    rdfs:range :Agent ;
    rdfs:subPropertyOf :hasOrHadManager ;
    owl:inverseOf :isOrWasHolderOf ;
    owl:propertyChainAxiom (
        :thingIsTargetOfRelation
        :recordResourceHoldingRelation_role
        :relationHasSource
    ) ;
    skos:changeNote
        [
            dc:date "2021-01-22" ;
            rdf:value """changed the IRI, label, inverse property IRI, text definition,
               super property IRI (changed made in order to make RiC-O compliant with RiC-CM 0.2;
               the name of this property in RiC-O 0.1 was "heldBy")."""@en ;
        ] ,
        [
            dc:date "2023-11-02" ;
            rdf:value "Added a new rdfs:label in Spanish."@en ;
        ] ,
        [
            dc:date "2023-08-28" ;
            rdf:value "Added a new rdfs:label in French."@en ;
        ] ,
        [
            dc:date "2023-11-08" ;
            rdf:value """In order to get a system of rolified Relation classes: modified
               the property chain axiom so that it now involves the new
               recordResourceHoldingRelation_role object property."""@en ;
        ] ;
    :RiCCMCorrespondingComponent """RiC-R039i ('has or had holder'
         relation)"""@en ;
.

:hasOrHadIdentifier
    a owl:ObjectProperty ;
    rdfs:label
        "has or had identifier"@en ,
        "tiene o tenía como identificador"@es ,
        "a ou a eu pour identifiant"@fr ;
    rdfs:comment """Connects a Thing to one of its past or present
         Identifiers."""@en ;
    rdfs:domain :Thing ;
    rdfs:isDefinedBy <https://www.ica.org/standards/RiC/ontology> ;
    rdfs:range :Identifier ;
    rdfs:subPropertyOf :hasOrHadAppellation ;
    owl:inverseOf :isOrWasIdentifierOf ;
    skos:changeNote
        [
            dc:date "2023-11-02" ;
            rdf:value "Added a new rdfs:label in Spanish."@en ;
        ] ,
        [
            dc:date "2023-08-28" ;
            rdf:value "Added a new rdfs:label in French."@en ;
        ] ,
        [
            dc:date "2021-01-22" ;
            rdf:value """changed the IRI, label, inverse property IRI, text definition,
               super property IRI (the name of this property in RiC-O 0.1 was
               "identifiedBy")."""@en ;
        ] ;
.

:hasOrHadIntellectualPropertyRightsHolder
    a owl:ObjectProperty ;
    rdfs:label
        "has or had intellectual property rights holder"@en ,
        """tiene o tenía como titular de derechos de propiedad intelectual
         a"""@es ,
        """a ou a détenu les droits de propriété intellectuelle
         sur"""@fr ;
    rdfs:comment """Inverse of 'is or was holder of intellectual property rights of'
         object property."""@en ;
    rdfs:domain
        [
            a owl:Class ;
            owl:unionOf (
                :Instantiation
                :RecordResource
            ) ;
        ] ;
    rdfs:isDefinedBy <https://www.ica.org/standards/RiC/ontology> ;
    rdfs:range
        [
            a owl:Class ;
            owl:unionOf (
                :Group
                :Person
                :Position
            ) ;
        ] ;
    rdfs:subPropertyOf :isOrWasUnderAuthorityOf ;
    owl:inverseOf :isOrWasHolderOfIntellectualPropertyRightsOf ;
    owl:propertyChainAxiom (
        :thingIsTargetOfRelation
        :intellectualPropertyRightsRelation_role
        :relationHasSource
    ) ;
    skos:changeNote
        [
            dc:date "2021-01-22" ;
            rdf:value """changed the IRI, label, inverse property IRI, textual
               definition (changed made in order to make RiC-O compliant with RiC-CM 0.2; the name
               of this property in RiC-O 0.1 was "intellectualPropertyRightsHeldBy")."""@en ;
        ] ,
        [
            dc:date "2023-11-02" ;
            rdf:value "Added a new rdfs:label in Spanish."@en ;
        ] ,
        [
            dc:date "2023-08-28" ;
            rdf:value "Added a new rdfs:label in French."@en ;
        ] ,
        [
            dc:date "2023-11-08" ;
            rdf:value """In order to get a system of rolified Relation classes: modified
               the property chain axiom so that it now involves the new
               intellectualPropertyRightsRelation_role object property."""@en ;
        ] ;
    :RiCCMCorrespondingComponent """RiC-R040i ('has or had intellectual property rights
         holder ' relation)"""@en ;
.

:hasOrHadJurisdiction
    a owl:ObjectProperty ;
    rdfs:label
        "has or had jurisdiction"@en ,
        "tiene o tenía como jurisdicción"@es ,
        "a ou a eu pour ressort"@fr ;
    rdfs:comment """Inverse of 'is or was jurisdiction of' object
         property."""@en ;
    rdfs:domain :Agent ;
    rdfs:isDefinedBy <https://www.ica.org/standards/RiC/ontology> ;
    rdfs:range :Place ;
    rdfs:subPropertyOf :isAgentAssociatedWithPlace ;
    owl:inverseOf :isOrWasJurisdictionOf ;
    skos:changeNote
        [
            dc:date "2023-08-28" ;
            rdf:value "Added a new rdfs:label in French."@en ;
        ] ,
        [
            dc:date "2021-01-22" ;
            rdf:value """changed the IRI, label, inverse property IRI and textual
               definition (changed made in order to make RiC-O compliant with RiC-CM 0.2; the name
               of this property in RiC-O 0.1 was "hasJurisdiction")."""@en ;
        ] ,
        [
            dc:date "2023-10-19" ;
            rdf:value """Made subproperty of new property isAgentAssociatedWithPlace
               instead of its parent isAssociatedWithPlace."""@en ;
        ] ,
        [
            dc:date "2023-11-02" ;
            rdf:value "Added a new rdfs:label in Spanish."@en ;
        ] ;
    :RiCCMCorrespondingComponent """RiC-R076i ('has or had jurisdiction'
         relation)"""@en ;
.

:hasOrHadLanguage
    a owl:ObjectProperty ;
    rdfs:label
        "has or had language"@en ,
        "tiene o tenía como lengua"@es ,
        "a ou a eu pour langue"@fr ;
    rdfs:comment """Connects an Agent, Record or Record Part to a Language that uses
         or used it."""@en ;
    rdfs:domain
        [
            a owl:Class ;
            owl:unionOf (
                :Agent
                :Record
                :RecordPart
            ) ;
        ] ;
    rdfs:isDefinedBy <https://www.ica.org/standards/RiC/ontology> ;
    rdfs:range :Language ;
    rdfs:subPropertyOf :isRelatedTo ;
    owl:inverseOf :isOrWasLanguageOf ;
    skos:changeNote
        [
            dc:date "2021-01-22" ;
            rdf:value """changed the IRI, label, inverse property IRI and textual
               definition (the name of this property in RiC-O 0.1 was "hasLanguage")."""@en ;
        ] ,
        [
            dc:date "2023-07-25" ;
            rdf:value """changed the definition to be consistent with the inverse
               relation."""@en ;
        ] ,
        [
            dc:date "2023-11-02" ;
            rdf:value "Added a new rdfs:label in Spanish."@en ;
        ] ,
        [
            dc:date "2023-08-28" ;
            rdf:value "Added a new rdfs:label in French."@en ;
        ] ;
.

:hasOrHadLeader
    a owl:ObjectProperty ;
    rdfs:label
        "has or had leader"@en ,
        "tiene o tenía como líder a"@es ,
        "a ou a eu pour dirigeant"@fr ;
    rdfs:comment "Inverse of 'is or was leader of' object property."@en ;
    rdfs:domain :Group ;
    rdfs:isDefinedBy <https://www.ica.org/standards/RiC/ontology> ;
    rdfs:range :Person ;
    rdfs:subPropertyOf :hasOrHadController ;
    owl:inverseOf :isOrWasLeaderOf ;
    owl:propertyChainAxiom (
        :thingIsTargetOfRelation
        :leadershipRelation_role
        :relationHasSource
    ) ;
    skos:changeNote
        [
            dc:date "2023-11-08" ;
            rdf:value """In order to get a system of rolified Relation classes: modified
               the property chain axiom so that it now involves the new leadershipRelation_role
               object property."""@en ;
        ] ,
        [
            dc:date "2023-11-02" ;
            rdf:value "Added a new rdfs:label in Spanish."@en ;
        ] ,
        [
            dc:date "2023-08-28" ;
            rdf:value "Added a new rdfs:label in French."@en ;
        ] ,
        [
            dc:date "2021-01-22" ;
            rdf:value """changed the IRI, label, inverse property IRI, text definition,
               super property IRI (changed made in order to make RiC-O compliant with RiC-CM 0.2;
               the name of this property in RiC-O 0.1 was "ledBy")."""@en ;
        ] ;
    :RiCCMCorrespondingComponent """RiC-R042i ('has or had leader'
         relation)"""@en ;
.

:hasOrHadLegalStatus
    a owl:ObjectProperty ;
    rdfs:label
        "has or had legal status"@en ,
        "tiene o tenía como status jurídico"@es ,
        "a ou a eu pour statut légal"@fr ;
    rdfs:comment """Connects an Agent or Record Resource to a Legal Status which
         categorized or categorizes it."""@en ;
    rdfs:domain
        [
            a owl:Class ;
            owl:unionOf (
                :Agent
                :Record
                :RecordPart
            ) ;
        ] ;
    rdfs:isDefinedBy <https://www.ica.org/standards/RiC/ontology> ;
    rdfs:range :LegalStatus ;
    rdfs:subPropertyOf :hasOrHadCategory ;
    owl:inverseOf :isOrWasLegalStatusOf ;
    skos:changeNote
        [
            dc:date "2021-01-22" ;
            rdf:value """changed the IRI, label, inverse property IRI and textual
               definition (the name of this property in RiC-O 0.1 was "hasLegalStatus")."""@en ;
        ] ,
        [
            dc:date "2023-08-28" ;
            rdf:value "Added a new rdfs:label in French."@en ;
        ] ,
        [
            dc:date "2023-11-02" ;
            rdf:value "Added a new rdfs:label in Spanish."@en ;
        ] ;
.

:hasOrHadMainSubject
    a owl:ObjectProperty ;
    rdfs:label
        "has or had main subject"@en ,
        "tiene o tenía como matería principal"@es ,
        "a ou a eu pour sujet principal"@fr ;
    rdfs:comment """Connects a Record Resource to a Thing that is or was its main
         subject."""@en ;
    rdfs:domain :RecordResource ;
    rdfs:isDefinedBy <https://www.ica.org/standards/RiC/ontology> ;
    rdfs:range :Thing ;
    rdfs:subPropertyOf :hasOrHadSubject ;
    owl:inverseOf :isOrWasMainSubjectOf ;
    skos:changeNote
        [
            dc:date "2023-08-28" ;
            rdf:value "Added a new rdfs:label in French."@en ;
        ] ,
        [
            dc:date "2023-11-02" ;
            rdf:value "Added a new rdfs:label in Spanish."@en ;
        ] ,
        [
            dc:date "2021-01-22" ;
            rdf:value """changed the IRI, label, inverse property IRI and textual
               definition (changed made in order to make RiC-O compliant with RiC-CM 0.2; the name
               of this property in RiC-O 0.1 was "hasMainSubject")."""@en ;
        ] ;
    skos:scopeNote """Use for specifying, for example, that a Record Set of type
         personal file has main subject some person, which would help end users to retrieve the main
         archival resources about this person."""@en ;
    :RiCCMCorrespondingComponent """RiC-R020 ('has or had main subject'
         relation)"""@en ;
.

:hasOrHadMandateType
    a owl:ObjectProperty ;
    rdfs:label
        "has or had mandate type"@en ,
        "tiene o tenía como tipo de norma"@es ,
        "a ou a eu pour type de mandat"@fr ;
    rdfs:comment """Connects a Mandate to a Mandate Type that categorized or
         categorizes it."""@en ;
    rdfs:domain :Mandate ;
    rdfs:isDefinedBy <https://www.ica.org/standards/RiC/ontology> ;
    rdfs:range :MandateType ;
    rdfs:subPropertyOf :hasOrHadRuleType ;
    owl:inverseOf :isOrWasMandateTypeOf ;
    skos:changeNote
        [
            dc:date "2023-11-13" ;
            rdf:value """Added the property, and its inverse one, following the creation
               of the MandateType class, that corresponds to the new Mandate Type attribute in
               RiC-CM 1.0."""@en ;
        ] ;
.

:hasOrHadMember
    a owl:ObjectProperty ;
    rdfs:label
        "has or had member"@en ,
        "tiene o tenía como miembro a"@es ,
        "a ou a eu pour membre"@fr ;
    rdfs:comment """Connects a Group to a Person that is or was a member of that
         Group."""@en ;
    rdfs:domain :Group ;
    rdfs:isDefinedBy <https://www.ica.org/standards/RiC/ontology> ;
    rdfs:range :Person ;
    rdfs:subPropertyOf :isAgentAssociatedWithAgent ;
    owl:inverseOf :isOrWasMemberOf ;
    owl:propertyChainAxiom (
        :thingIsSourceOfRelation
        :membershipRelation_role
        :relationHasTarget
    ) ;
    skos:changeNote
        [
            dc:date "2023-11-08" ;
            rdf:value """In order to get a system of rolified Relation classes: modified
               the property chain axiom so that it now involves the new membershipRelation_role
               object property."""@en ;
        ] ,
        [
            dc:date "2023-11-02" ;
            rdf:value "Added a new rdfs:label in Spanish."@en ;
        ] ,
        [
            dc:date "2023-08-28" ;
            rdf:value "Added a new rdfs:label in French."@en ;
        ] ,
        [
            dc:date "2021-01-22" ;
            rdf:value """changed the IRI, label, inverse property IRI and textual
               definition (changed made in order to make RiC-O compliant with RiC-CM 0.2; the name
               of this property in RiC-O 0.1 was "hasMember")."""@en ;
        ] ;
    :RiCCMCorrespondingComponent """RiC-R055 ('has or had member'
         relation)"""@en ;
.

:hasOrHadMostMembersWithCreationDate
    a owl:ObjectProperty ;
    rdfs:label
        "has or had most members with creation date"@en ,
        """tienen o tenían la mayoría de sus miembros como fecha de
         creación"""@es ,
        """inclut ou a inclus des membres dont la plupart ont pour date de
         création"""@fr ;
    rdfs:comment """Inverse of 'is or was creation date of most members of' object
         property"""@en ;
    rdfs:domain :RecordSet ;
    rdfs:isDefinedBy <https://www.ica.org/standards/RiC/ontology> ;
    rdfs:range :Date ;
    rdfs:subPropertyOf :hasOrHadSomeMembersWithCreationDate ;
    owl:inverseOf :isOrWasCreationDateOfMostMembersOf ;
    skos:changeNote
        [
            dc:date "2023-09-22" ;
            rdf:value "Added in RiC-O 1.0."@en ;
        ] ,
        [
            dc:date "2023-10-10" ;
            rdf:value """Made this property a subproperty of
               hasSomeMembersWithCreationDate."""@en ;
        ] ,
        [
            dc:date "2023-10-13" ;
            rdf:value """Renamed the property in order to take the past members of the
               record set into account. Adjusted the annotations accordingly."""@en ;
        ] ,
        [
            dc:date "2023-11-27" ;
            rdf:value "Added a new rdfs:label in Spanish."@en ;
        ] ,
        [
            dc:date "2023-10-12" ;
            rdf:value "Added the French label"@en ;
        ] ;
    :RiCCMCorrespondingComponent """RiC-R083i ('has or had most members with creation
         date' relation)"""@en ;
.

:hasOrHadOccupationOfType
    a owl:ObjectProperty ;
    rdfs:label
        "has or had occupation of type"@en ,
        "tiene o tenía como tipo de ocupación"@es ,
        "a ou a eu pour type d’occupation"@fr ;
    rdfs:comment """Connects a Person to an Occupation Type that categorized or
         categorizes his/her occupation (profession, trade or craft)."""@en ;
    rdfs:domain :Person ;
    rdfs:isDefinedBy <https://www.ica.org/standards/RiC/ontology> ;
    rdfs:range :OccupationType ;
    rdfs:subPropertyOf :hasOrHadDemographicGroup ;
    owl:inverseOf :isOrWasOccupationTypeOf ;
    skos:changeNote
        [
            dc:date "2023-08-28" ;
            rdf:value "Added a new rdfs:label in French."@en ;
        ] ,
        [
            dc:date "2021-01-22" ;
            rdf:value """changed the IRI, label, inverse property IRI, textual
               definition, super property IRI (the name of this property in RiC-O 0.1 was
               "hasOccupationOfType")."""@en ;
        ] ,
        [
            dc:date "2023-11-02" ;
            rdf:value "Added a new rdfs:label in Spanish."@en ;
        ] ;
.

:hasOrHadOwner
    a owl:ObjectProperty ;
    rdfs:label
        "has or had owner"@en ,
        "tiene o tenía como poseedor a"@es ,
        "a ou a eu pour propriétaire"@fr ;
    rdfs:comment "Inverse of 'is or was owner of' object property."@en ;
    rdfs:domain :Thing ;
    rdfs:isDefinedBy <https://www.ica.org/standards/RiC/ontology> ;
    rdfs:range
        [
            a owl:Class ;
            owl:unionOf (
                :Group
                :Person
                :Position
            ) ;
        ] ;
    rdfs:subPropertyOf :isOrWasUnderAuthorityOf ;
    owl:inverseOf :isOrWasOwnerOf ;
    owl:propertyChainAxiom (
        :thingIsTargetOfRelation
        :ownershipRelation_role
        :relationHasSource
    ) ;
    skos:changeNote
        [
            dc:date "2023-08-28" ;
            rdf:value "Added a new rdfs:label in French."@en ;
        ] ,
        [
            dc:date "2023-11-08" ;
            rdf:value """In order to get a system of rolified Relation classes: modified
               the property chain axiom so that it now involves the new ownershipRelation_role
               object property."""@en ;
        ] ,
        [
            dc:date "2023-11-02" ;
            rdf:value "Added a new rdfs:label in Spanish."@en ;
        ] ,
        [
            dc:date "2021-01-22" ;
            rdf:value """changed the IRI, label, inverse property IRI, text definition,
               super property IRI (changed made in order to make RiC-O compliant with RiC-CM 0.2;
               the name of this property in RiC-O 0.1 was "ownedBy")."""@en ;
        ] ;
    :RiCCMCorrespondingComponent """RiC-R037i ('has or had owner'
         relation)"""@en ;
.

:hasOrHadPhysicalLocation
    a owl:ObjectProperty ;
    rdfs:label
        "has or had physical location"@en ,
        "tiene o tenía como localización física"@es ,
        "a ou a eu pour localisation physique"@fr ;
    rdfs:comment """Connects a Place to one of its past or present Physical
         Location."""@en ;
    rdfs:domain :Place ;
    rdfs:isDefinedBy <https://www.ica.org/standards/RiC/ontology> ;
    rdfs:range :PhysicalLocation ;
    rdfs:subPropertyOf :isPlaceAssociatedWith ;
    owl:inverseOf :isOrWasPhysicalLocationOf ;
    skos:changeNote
        [
            dc:date "2021-02-01" ;
            rdf:value """Property made a subproperty of
               'isPlaceAssociatedWith"."""@en ;
        ] ,
        [
            dc:date "2021-01-22" ;
            rdf:value """changed the IRI, label, inverse property IRI, textual
               definition (the name of this property in RiC-O 0.1 was
               "hasPhysicalLocation")."""@en ;
        ] ,
        [
            dc:date "2023-08-28" ;
            rdf:value "Added a new rdfs:label in French."@en ;
        ] ,
        [
            dc:date "2023-11-02" ;
            rdf:value "Added a new rdfs:label in Spanish."@en ;
        ] ;
.

:hasOrHadPlaceName
    a owl:ObjectProperty ;
    rdfs:label
        "has or had place name"@en ,
        "tiene o tenía como nombre de lugar"@es ,
        "a ou a eu pour nom de lieu"@fr ;
    rdfs:comment """Connects a Place to one of its past or present
         names."""@en ;
    rdfs:domain :Place ;
    rdfs:isDefinedBy <https://www.ica.org/standards/RiC/ontology> ;
    rdfs:range :PlaceName ;
    rdfs:subPropertyOf :hasOrHadName ;
    owl:inverseOf :isOrWasPlaceNameOf ;
    skos:changeNote
        [
            dc:date "2023-08-28" ;
            rdf:value "Added a new rdfs:label in French."@en ;
        ] ,
        [
            dc:date "2021-01-22" ;
            rdf:value """changed the IRI, label, inverse property IRI, text definition,
               super property IRI (the name of this property in RiC-O 0.1 was
               "hasPlaceName")."""@en ;
        ] ,
        [
            dc:date "2023-11-02" ;
            rdf:value "Added a new rdfs:label in Spanish."@en ;
        ] ;
.

:hasOrHadPlaceType
    a owl:ObjectProperty ;
    rdfs:label
        "has or had place type"@en ,
        "tiene o tenía como tipo de lugar"@es ,
        "a ou a eu pour type de lieu"@fr ;
    rdfs:comment """Connects a Place to a Place Type that categorized or categorizes
         it."""@en ;
    rdfs:domain :Place ;
    rdfs:isDefinedBy <https://www.ica.org/standards/RiC/ontology> ;
    rdfs:range :PlaceType ;
    rdfs:subPropertyOf :hasOrHadCategory ;
    owl:inverseOf :isOrWasPlaceTypeOf ;
    skos:changeNote
        [
            dc:date "2021-01-22" ;
            rdf:value """changed the IRI, label, inverse property IRI, text definition,
               super property IRI (the name of this property in RiC-O 0.1 was
               "hasPlaceType")."""@en ;
        ] ,
        [
            dc:date "2023-11-02" ;
            rdf:value "Added a new rdfs:label in Spanish."@en ;
        ] ,
        [
            dc:date "2023-08-28" ;
            rdf:value "Added a new rdfs:label in French."@en ;
        ] ;
.

:hasOrHadPosition
    a owl:ObjectProperty ;
    rdfs:label
        "has or had position"@en ,
        "tiene o tenía como puesto"@es ,
        "occupe ou a occupé le poste"@fr ;
    rdfs:comment "Inverse of 'exists or existed in' object property."@en ;
    rdfs:domain :Group ;
    rdfs:isDefinedBy <https://www.ica.org/standards/RiC/ontology> ;
    rdfs:range :Position ;
    rdfs:subPropertyOf :isAgentAssociatedWithAgent ;
    owl:inverseOf :existsOrExistedIn ;
    owl:propertyChainAxiom (
        :thingIsTargetOfRelation
        :positionToGroupRelation_role
        :relationHasSource
    ) ;
    skos:changeNote
        [
            dc:date "2023-11-02" ;
            rdf:value "Added a new rdfs:label in Spanish."@en ;
        ] ,
        [
            dc:date "2023-11-08" ;
            rdf:value """In order to get a system of rolified Relation classes: modified
               the property chain axiom so that it now involves the new positionToGroupRelation_role
               object property."""@en ;
        ] ,
        [
            dc:date "2023-08-28" ;
            rdf:value "Added a new rdfs:label in French."@en ;
        ] ,
        [
            dc:date "2021-01-22" ;
            rdf:value """changed the IRI, label, inverse property IRI, text definition,
               corresponding CM component name (changed made in order to make RiC-O compliant with
               RiC-CM 0.2; the name of this property in RiC-O 0.1 was "hasPosition")."""@en ;
        ] ,
        [
            dc:date "2023-11-07" ;
            rdf:value """Added the property chain axiom so that this property is
               formally defined as a shortcut (the inverse property already was)."""@en ;
        ] ;
    :RiCCMCorrespondingComponent """RiC-R056i ('has or had position'
         relation)"""@en ;
.

:hasOrHadSomeMembersWithContentType
    a owl:ObjectProperty ;
    rdfs:label
        "has or had some members with content type"@en ,
        """tienen o tenían algunos de sus miembros como tipo de
         contenido"""@es ,
        """inclut ou a inclus des membres ayant pour type de
         contenu"""@fr ;
    rdfs:comment """Connects a Record Set and a Content Type that categorizes some of
         the Records or Record Parts that are or were included in the Record Set."""@en ;
    rdfs:domain :RecordSet ;
    rdfs:isDefinedBy <https://www.ica.org/standards/RiC/ontology> ;
    rdfs:range :ContentType ;
    rdfs:subPropertyOf :hasOrHadSomeMembersWithCategory ;
    owl:inverseOf :isOrWasContentTypeOfSomeMembersOf ;
    skos:changeNote
        [
            dc:date "2023-08-28" ;
            rdf:value "Added a new rdfs:label in French."@en ;
        ] ,
        [
            dc:date "2020-12-28" ;
            rdf:value """Object property added for handling the case where a Record Set
               is described as having all or some members that belong to some category (see RiC-CM
               0.2 attributes section, #4.4 on Record Set, Record and Record Part
               attributes)."""@en ;
        ] ,
        [
            dc:date "2023-11-02" ;
            rdf:value "Added a new rdfs:label in Spanish."@en ;
        ] ;
.

:hasOrHadSomeMembersWithDocumentaryFormType
    a owl:ObjectProperty ;
    rdfs:label
        "has or had some members with documentary form type"@en ,
        """tienen o tenía algunos de sus miembros como tipo
         documental"""@es ,
        """inclut ou a inclus des membres ayant pour type de
         document"""@fr ;
    rdfs:comment """Connects a Record Set and a Documentary Form Type that categorizes
         some of the Records or Record Parts that are or were included in the Record
         Set."""@en ;
    rdfs:domain :RecordSet ;
    rdfs:isDefinedBy <https://www.ica.org/standards/RiC/ontology> ;
    rdfs:range :DocumentaryFormType ;
    rdfs:subPropertyOf :hasOrHadSomeMembersWithCategory ;
    owl:inverseOf :isOrWasDocumentaryFormTypeOfSomeMembersOf ;
    skos:changeNote
        [
            dc:date "2023-11-02" ;
            rdf:value "Added a new rdfs:label in Spanish."@en ;
        ] ,
        [
            dc:date "2024-03-15" ;
            rdf:value "Fixed a typo in IRI: changed 'with' to 'With'."@en ;
        ] ,
        [
            dc:date "2020-12-28" ;
            rdf:value """Object property added for handling the case where a Record Set
               is described as having all or some members that belong to some category (see RiC-CM
               0.2 attributes section, #4.4 on Record Set, Record and Record Part
               attributes)."""@en ;
        ] ,
        [
            dc:date "2023-08-28" ;
            rdf:value "Added a new rdfs:label in French."@en ;
        ] ;
.

:hasOrHadSomeMembersWithLanguage
    a owl:ObjectProperty ;
    rdfs:label
        "has or had some members with language"@en ,
        "tienen o tenían algunos de sus miembros como lengua"@es ,
        "inclut ou a inclus des membres ayant pour langue"@fr ;
    rdfs:comment """Connects a Record Set and a Language used by some of the Records
         or Record Parts that are or were included in the Record Set."""@en ;
    rdfs:domain :RecordSet ;
    rdfs:isDefinedBy <https://www.ica.org/standards/RiC/ontology> ;
    rdfs:range :Language ;
    rdfs:subPropertyOf :isRelatedTo ;
    owl:inverseOf :isOrWasLanguageOfSomeMembersOf ;
    skos:changeNote
        [
            dc:date "2023-11-02" ;
            rdf:value "Added a new rdfs:label in Spanish."@en ;
        ] ,
        [
            dc:date "2020-12-28" ;
            rdf:value """Object property added for handling the case where a Record Set
               is described as having all or some members that belong to some category (see RiC-CM
               0.2 attributes section, #4.4 on Record Set, Record and Record Part
               attributes)."""@en ;
        ] ,
        [
            dc:date "2023-08-28" ;
            rdf:value "Added a new rdfs:label in French."@en ;
        ] ;
.

:hasOrHadSomeMembersWithLegalStatus
    a owl:ObjectProperty ;
    rdfs:label
        "has or had some members with legal status"@en ,
        """tienen o tenían algunos de sus miembros como status
         jurídico"""@es ,
        "inclut ou a inclus des membres ayant pour statut légal"@fr ;
    rdfs:comment """Connects a Record Set and a Legal Status that categorizes some of
         the Records or Record Parts that are or were included in the Record Set."""@en ;
    rdfs:domain :RecordSet ;
    rdfs:isDefinedBy <https://www.ica.org/standards/RiC/ontology> ;
    rdfs:range :LegalStatus ;
    rdfs:subPropertyOf :hasOrHadSomeMembersWithCategory ;
    owl:inverseOf :isOrWasLegalStatusOfSomeMembersOf ;
    skos:changeNote
        [
            dc:date "2020-12-28" ;
            rdf:value """Object property added for handling the case where a Record Set
               is described as having all or some members that belong to some category (see RiC-CM
               0.2 attributes section, #4.4 on Record Set, Record and Record Part
               attributes)."""@en ;
        ] ,
        [
            dc:date "2023-11-02" ;
            rdf:value "Added a new rdfs:label in Spanish."@en ;
        ] ,
        [
            dc:date "2023-08-28" ;
            rdf:value "Added a new rdfs:label in French."@en ;
        ] ;
.

:hasOrHadSomeMembersWithRecordState
    a owl:ObjectProperty ;
    rdfs:label
        "has or had some members with record state"@en ,
        """tienen o tenía algunos de sus miembros como estado de
         documento"""@es ,
        "inclut ou a inclus des membres ayant pour état"@fr ;
    rdfs:comment """Connects a Record Set and a Record State that categorizes some of
         the Records or Record Parts that are or were included in the Record Set."""@en ;
    rdfs:domain :RecordSet ;
    rdfs:isDefinedBy <https://www.ica.org/standards/RiC/ontology> ;
    rdfs:range :RecordState ;
    rdfs:subPropertyOf :hasOrHadSomeMembersWithCategory ;
    owl:inverseOf :isOrWasRecordStateOfSomeMembersOf ;
    skos:changeNote
        [
            dc:date "2023-11-02" ;
            rdf:value "Added a new rdfs:label in Spanish."@en ;
        ] ,
        [
            dc:date "2023-08-28" ;
            rdf:value "Added a new rdfs:label in French."@en ;
        ] ,
        [
            dc:date "2020-12-28" ;
            rdf:value """Object property added for handling the case where a Record Set
               is described as having all or some members that belong to some category (see RiC-CM
               0.2 attributes section, #4.4 on Record Set, Record and Record Part
               attributes)."""@en ;
        ] ;
.

:hasOrHadStudent
    a owl:ObjectProperty ;
    rdfs:label
        "has or had student"@en ,
        "tiene o tenía como estudiante a"@es ,
        "a ou a eu pour étudiant"@fr ;
    rdfs:comment "Inverse of 'has or had teacher' object property."@en ;
    rdfs:domain :Person ;
    rdfs:isDefinedBy <https://www.ica.org/standards/RiC/ontology> ;
    rdfs:range :Person ;
    rdfs:subPropertyOf :knows ;
    owl:inverseOf :hasOrHadTeacher ;
    owl:propertyChainAxiom (
        :thingIsSourceOfRelation
        :teachingRelation_role
        :relationHasTarget
    ) ;
    skos:changeNote
        [
            dc:date "2021-01-22" ;
            rdf:value """changed the IRI, label, inverse property IRI, text definition
               (changed made in order to make RiC-O compliant with RiC-CM 0.2; the name of this
               property in RiC-O 0.1 was "hasStudent")."""@en ;
        ] ,
        [
            dc:date "2023-11-02" ;
            rdf:value "Added a new rdfs:label in Spanish."@en ;
        ] ,
        [
            dc:date "2023-11-08" ;
            rdf:value """In order to get a system of rolified Relation classes: modified
               the property chain axiom so that it now involves the new teachingRelation_role object
               property."""@en ;
        ] ,
        [
            dc:date "2023-08-28" ;
            rdf:value "Added a new rdfs:label in French."@en ;
        ] ;
    :RiCCMCorrespondingComponent """RiC-R053i ('has or had student'
         relation)"""@en ;
.

:hasOrHadTeacher
    a owl:ObjectProperty ;
    rdfs:label
        "has or had teacher"@en ,
        "tiene o tenía como profesor(a) a"@es ,
        "a ou a eu pour enseignant"@fr ;
    rdfs:comment """Connects a Person to another Person who is or was their
         teacher."""@en ;
    rdfs:domain :Person ;
    rdfs:isDefinedBy <https://www.ica.org/standards/RiC/ontology> ;
    rdfs:range :Person ;
    rdfs:subPropertyOf :knows ;
    owl:inverseOf :hasOrHadStudent ;
    owl:propertyChainAxiom (
        :thingIsTargetOfRelation
        :teachingRelation_role
        :relationHasSource
    ) ;
    skos:changeNote
        [
            dc:date "2023-11-12" ;
            rdf:value """Aligned with RiC-CM 1.0: updated the description
               (rdfs:comment)."""@en ;
        ] ,
        [
            dc:date "2021-01-22" ;
            rdf:value """changed the IRI, label, inverse property IRI, text definition
               (changed made in order to make RiC-O compliant with RiC-CM 0.2; the name of this
               property in RiC-O 0.1 was "hasTeacher")."""@en ;
        ] ,
        [
            dc:date "2023-08-28" ;
            rdf:value "Added a new rdfs:label in French."@en ;
        ] ,
        [
            dc:date "2023-11-08" ;
            rdf:value """In order to get a system of rolified Relation classes: modified
               the property chain axiom so that it now involves the new teachingRelation_role object
               property."""@en ;
        ] ,
        [
            dc:date "2023-11-02" ;
            rdf:value "Added a new rdfs:label in Spanish."@en ;
        ] ;
    :RiCCMCorrespondingComponent """RiC-R053 ('has or had teacher'
         relation)"""@en ;
.

:hasOrHadTitle
    a owl:ObjectProperty ;
    rdfs:label
        "has or had title"@en ,
        "tiene o tenía como título"@es ,
        "a ou a eu pour intitulé"@fr ;
    rdfs:comment """Connects a Record Resource, Instantiation or Rule to a title that
         is or was used for designating it."""@en ;
    rdfs:domain
        [
            a owl:Class ;
            owl:unionOf (
                :Instantiation
                :RecordResource
                :Rule
            ) ;
        ] ;
    rdfs:isDefinedBy <https://www.ica.org/standards/RiC/ontology> ;
    rdfs:range :Title ;
    rdfs:subPropertyOf :hasOrHadName ;
    owl:inverseOf :isOrWasTitleOf ;
    skos:changeNote
        [
            dc:date "2021-01-22" ;
            rdf:value """changed the IRI, label, inverse property IRI, text definition,
               super property IRI (the name of this property in RiC-O 0.1 was
               "hasTitle")."""@en ;
        ] ,
        [
            dc:date "2023-11-02" ;
            rdf:value "Added a new rdfs:label in Spanish."@en ;
        ] ,
        [
            dc:date "2023-08-28" ;
            rdf:value "Added a new rdfs:label in French."@en ;
        ] ;
.

:hasOriginal
    a owl:ObjectProperty ;
    rdfs:label
        "has original"@en ,
        "tiene como original"@es ,
        "a pour original"@fr ;
    rdfs:comment "Inverse of 'is original of' object property."@en ;
    rdfs:domain
        [
            a owl:Class ;
            owl:unionOf (
                :Record
                :RecordPart
            ) ;
        ] ;
    rdfs:isDefinedBy <https://www.ica.org/standards/RiC/ontology> ;
    rdfs:range
        [
            a owl:Class ;
            owl:unionOf (
                :Record
                :RecordPart
            ) ;
        ] ;
    rdfs:subPropertyOf
        :followsInTime ,
        :hasGeneticLinkToRecordResource ;
    owl:inverseOf :isOriginalOf ;
    skos:changeNote
        [
            dc:date "2023-08-28" ;
            rdf:value "Added a new rdfs:label in French."@en ;
        ] ,
        [
            dc:date "2023-11-02" ;
            rdf:value "Added a new rdfs:label in Spanish."@en ;
        ] ;
    :RiCCMCorrespondingComponent """RiC-R010i ('is original of'
         relation)"""@en ;
.

:hasProductionTechniqueType
    a owl:ObjectProperty ;
    rdfs:label
        "has production technique type"@en ,
        "tiene como técnica de producción"@es ,
        "a pour type de technique de production"@fr ;
    rdfs:comment """Connects an Instantiation to a Production Technique Type that
         categorizes its production technique."""@en ;
    rdfs:domain :Instantiation ;
    rdfs:isDefinedBy <https://www.ica.org/standards/RiC/ontology> ;
    rdfs:range :ProductionTechniqueType ;
    rdfs:subPropertyOf :hasOrHadCategory ;
    owl:inverseOf :isProductionTechniqueTypeOf ;
    skos:changeNote
        [
            dc:date "2023-08-28" ;
            rdf:value "Added a new rdfs:label in French."@en ;
        ] ,
        [
            dc:date "2021-01-22" ;
            rdf:value "changed the super property IRI."@en ;
        ] ,
        [
            dc:date "2023-11-02" ;
            rdf:value "Added a new rdfs:label in Spanish."@en ;
        ] ;
.

:hasPublicationDate
    a owl:ObjectProperty ;
    rdfs:label
        "has publication date"@en ,
        "tiene como fecha de publicación"@es ,
        "a pour date de publication"@fr ;
    rdfs:comment "Inverse of 'is publication date of' object property"@en ;
    rdfs:domain :RecordResource ;
    rdfs:isDefinedBy <https://www.ica.org/standards/RiC/ontology> ;
    rdfs:range :Date ;
    rdfs:subPropertyOf :isAssociatedWithDate ;
    owl:inverseOf :isPublicationDateOf ;
    skos:changeNote
        [
            dc:date "2023-10-12" ;
            rdf:value "Added the French label"@en ;
        ] ,
        [
            dc:date "2023-09-22" ;
            rdf:value "Added in RiC-O 1.0."@en ;
        ] ,
        [
            dc:date "2023-11-27" ;
            rdf:value "Added a new rdfs:label in Spanish."@en ;
        ] ;
.

:hasPublisher
    a owl:ObjectProperty ;
    rdfs:label
        "has publisher"@en ,
        "tiene como editor(a) a"@es ,
        "a pour éditeur"@fr ;
    rdfs:comment """Connects a Record resource to an Agent who published
         it."""@en ;
    rdfs:domain :RecordResource ;
    rdfs:isDefinedBy <https://www.ica.org/standards/RiC/ontology> ;
    rdfs:range :Agent ;
    rdfs:subPropertyOf :isRelatedTo ;
    owl:inverseOf :isPublisherOf ;
    skos:changeNote
        [
            dc:date "2021-01-22" ;
            rdf:value """changed the IRI, label, inverse property IRI (the name of this
               property in RiC-O 0.1 was "publishedBy")."""@en ;
        ] ,
        [
            dc:date "2023-08-28" ;
            rdf:value "Added a new rdfs:label in French."@en ;
        ] ,
        [
            dc:date "2023-11-02" ;
            rdf:value "Added a new rdfs:label in Spanish."@en ;
        ] ;
.

:hasReceiver
    a owl:ObjectProperty ;
    rdfs:label
        "has receiver"@en ,
        "tiene como receptor(a) a"@es ,
        "est reçu par"@fr ;
    rdfs:comment """Connects a Record Resource or an Instantiation to the Agent that
         receives it in the course of the Agent's activities."""@en ;
    rdfs:domain
        [
            a owl:Class ;
            owl:unionOf (
                :Instantiation
                :RecordResource
            ) ;
        ] ;
    rdfs:isDefinedBy <https://www.ica.org/standards/RiC/ontology> ;
    rdfs:range :Agent ;
    rdfs:subPropertyOf :hasAccumulator ;
    owl:inverseOf :isReceiverOf ;
    skos:changeNote
        [
            dc:date "2023-08-28" ;
            rdf:value "Added a new rdfs:label in French."@en ;
        ] ,
        [
            dc:date "2021-01-22" ;
            rdf:value """changed the IRI, label, inverse property IRI, super property
               IRI (changed made in order to make RiC-O compliant with RiC-CM 0.2; the name of this
               property in RiC-O 0.1 was "receivedBy")."""@en ;
        ] ,
        [
            dc:date "2023-11-02" ;
            rdf:value "Added a new rdfs:label in Spanish."@en ;
        ] ,
        [
            dc:date "2023-08-28" ;
            rdf:value "Added a new rdfs:label in French."@en ;
        ] ,
        [
            dc:date "2023-11-12" ;
            rdf:value """Aligned with RiC-CM 1.0: updated the description
               (rdfs:comment)."""@en ;
        ] ;
    :RiCCMCorrespondingComponent """RiC-R029 ('has receiver'
         relation)"""@en ;
.

:hasRecordSetType
    a owl:ObjectProperty ;
    rdfs:label
        "has record set type"@en ,
        "tiene como tipo de agrupación documental"@es ,
        "a pour type d’ensemble d’objets informationnels"@fr ;
    rdfs:comment """Connects a Record Set to a Record Set Type that categorizes
         it."""@en ;
    rdfs:domain :RecordSet ;
    rdfs:isDefinedBy <https://www.ica.org/standards/RiC/ontology> ;
    rdfs:range :RecordSetType ;
    rdfs:subPropertyOf :hasOrHadCategory ;
    owl:inverseOf :isRecordSetTypeOf ;
    skos:changeNote
        [
            dc:date "2023-08-28" ;
            rdf:value "Added a new rdfs:label in French."@en ;
        ] ,
        [
            dc:date "2021-01-22" ;
            rdf:value "changed the super property IRI."@en ;
        ] ,
        [
            dc:date "2023-11-02" ;
            rdf:value "Added a new rdfs:label in Spanish."@en ;
        ] ;
.

:hasRecordState
    a owl:ObjectProperty ;
    rdfs:label
        "has record state"@en ,
        "tiene como estado de documento"@es ,
        "a pour état"@fr ;
    rdfs:comment """Connects a Record or Record Part to a Record State that
         categorizes its state."""@en ;
    rdfs:domain
        [
            a owl:Class ;
            owl:unionOf (
                :Record
                :RecordPart
            ) ;
        ] ;
    rdfs:isDefinedBy <https://www.ica.org/standards/RiC/ontology> ;
    rdfs:range :RecordState ;
    rdfs:subPropertyOf :hasOrHadCategory ;
    owl:inverseOf :isRecordStateOf ;
    skos:changeNote
        [
            dc:date "2020-12-28" ;
            rdf:value """Changed the IRI (hasRecordResourceState changed to
               hasRecordState), label, textual definition and domain (RecordResource replaced by
               Record or Record Part)."""@en ;
        ] ,
        [
            dc:date "2023-11-02" ;
            rdf:value "Added a new rdfs:label in Spanish."@en ;
        ] ,
        [
            dc:date "2023-08-28" ;
            rdf:value "Added a new rdfs:label in French."@en ;
        ] ;
.

:hasReply
    a owl:ObjectProperty ;
    rdfs:label
        "has reply"@en ,
        "tiene como contestación"@es ,
        "a pour réponse"@fr ;
    rdfs:comment """Connects a Record Resource to a reply, usually in the form of
         correspondence."""@en ;
    rdfs:domain :RecordResource ;
    rdfs:isDefinedBy <https://www.ica.org/standards/RiC/ontology> ;
    rdfs:range :RecordResource ;
    rdfs:subPropertyOf
        :isRecordResourceAssociatedWithRecordResource ,
        :precedesInTime ;
    owl:inverseOf :isReplyTo ;
    skos:changeNote
        [
            dc:date "2023-11-02" ;
            rdf:value "Added a new rdfs:label in Spanish."@en ;
        ] ,
        [
            dc:date "2021-01-22" ;
            rdf:value """changed the IRI, label, inverse property IRI, text definition
               (changed made in order to make RiC-O compliant with RiC-CM 0.2; the name of this
               property in RiC-O 0.1 was "isRepliedToBy")."""@en ;
        ] ,
        [
            dc:date "2023-08-28" ;
            rdf:value "Added a new rdfs:label in French."@en ;
        ] ;
    :RiCCMCorrespondingComponent """RiC-R013 ('has reply'
         relation)"""@en ;
.

:hasRepresentationType
    a owl:ObjectProperty ;
    rdfs:label
        "has representation type"@en ,
        "tiene como tipo de grabación"@es ,
        "a pour type de représentation"@fr ;
    rdfs:comment """Connects an Instantiation to a Representation Type that
         categorizes its representation type."""@en ;
    rdfs:domain :Instantiation ;
    rdfs:isDefinedBy <https://www.ica.org/standards/RiC/ontology> ;
    rdfs:range :RepresentationType ;
    rdfs:subPropertyOf :hasOrHadCategory ;
    owl:inverseOf :isRepresentationTypeOf ;
    skos:changeNote
        [
            dc:date "2021-01-22" ;
            rdf:value "changed the super property IRI."@en ;
        ] ,
        [
            dc:date "2023-11-02" ;
            rdf:value "Added a new rdfs:label in Spanish."@en ;
        ] ,
        [
            dc:date "2023-08-28" ;
            rdf:value "Added a new rdfs:label in French."@en ;
        ] ;
.

:hasSender
    a owl:ObjectProperty ;
    rdfs:label
        "has sender"@en ,
        "tiene como remitente a"@es ,
        "a pour expéditeur"@fr ;
    rdfs:comment """Connects a Record Resource or an Instantiation to the Agent that
         sends it"""@en ;
    rdfs:domain
        [
            a owl:Class ;
            owl:unionOf (
                :Instantiation
                :RecordResource
            ) ;
        ] ;
    rdfs:isDefinedBy <https://www.ica.org/standards/RiC/ontology> ;
    rdfs:range :Agent ;
    rdfs:subPropertyOf :hasOrganicProvenance ;
    owl:inverseOf :isSenderOf ;
    skos:changeNote
        [
            dc:date "2023-11-12" ;
            rdf:value """Aligned with RiC-CM 1.0: updated the
               skos:scopeNote."""@en ;
        ] ,
        [
            dc:date "2023-11-02" ;
            rdf:value "Added a new rdfs:label in Spanish."@en ;
        ] ,
        [
            dc:date "2023-08-28" ;
            rdf:value "Added a new rdfs:label in French."@en ;
        ] ;
    skos:scopeNote """The identity of the sender is (usually) evidenced by the Record
         Resource or Instantiation itself."""@en ;
    :RiCCMCorrespondingComponent """RiC-R031 ('has sender'
         relation)"""@en ;
.

:hasUnitOfMeasurement
    a owl:ObjectProperty ;
    rdfs:label
        "has unit of measurement"@en ,
        "tiene como unidad de medida"@es ,
        "a pour unité de mesure"@fr ;
    rdfs:comment "Connects an Extent to a Unit Of Measurement"@en ;
    rdfs:domain :Extent ;
    rdfs:isDefinedBy <https://www.ica.org/standards/RiC/ontology> ;
    rdfs:range :UnitOfMeasurement ;
    rdfs:subPropertyOf :isRelatedTo ;
    owl:inverseOf :isUnitOfMeasurementOf ;
    skos:changeNote
        [
            dc:date "2023-08-28" ;
            rdf:value """Added a new rdfs:label in French; added an xml:lang attribute
               to the rdfs:comment."""@en ;
        ] ,
        [
            dc:date "2020-10-28" ;
            rdf:value """Object property created along with Extent and UnitOfMeasurement
               classes, in order to provide methods for handling extent accurately."""@en ;
        ] ,
        [
            dc:date "2023-11-02" ;
            rdf:value "Added a new rdfs:label in Spanish."@en ;
        ] ;
.

:hasWithin
    a owl:ObjectProperty ;
    rdfs:label
        "has within"@en ,
        "tiene dentro"@es ,
        "contient"@fr ;
    rdfs:comment "Inverse of 'is within' object property"@en ;
    rdfs:domain :Date ;
    rdfs:isDefinedBy <https://www.ica.org/standards/RiC/ontology> ;
    rdfs:range :Date ;
    rdfs:subPropertyOf
        :hasOrHadPart ,
        :isAssociatedWithDate ,
        :isDateAssociatedWith ;
    owl:inverseOf :isWithin ;
    skos:changeNote
        [
            dc:date "2023-11-27" ;
            rdf:value "Added a new rdfs:label in Spanish."@en ;
        ] ,
        [
            dc:date "2023-10-12" ;
            rdf:value "Added the property"@en ;
        ] ,
        [
            dc:date "2023-10-13" ;
            rdf:value """made this property a subproperty of both isDateAssociatedWith
               and isAssociatedWithdate, and of hasOrHadPart."""@en ;
        ] ;
    :RiCCMCorrespondingComponent """RiC-R085i ('has within'
         relation)"""@en ;
.

:included
    a owl:ObjectProperty ;
    rdfs:label
        "included"@en ,
        "incluía"@es ,
        "a inclus"@fr ;
    rdfs:comment """Connects a Record Set to a Record or Record Set which it included
         in the past."""@en ;
    rdfs:domain :RecordSet ;
    rdfs:isDefinedBy <https://www.ica.org/standards/RiC/ontology> ;
    rdfs:range
        [
            a owl:Class ;
            owl:unionOf (
                :Record
                :RecordSet
            ) ;
        ] ;
    rdfs:subPropertyOf
        :hadPart ,
        :includesOrIncluded ;
    owl:inverseOf :wasIncludedIn ;
    skos:changeNote
        [
            dc:date "2023-11-13" ;
            rdf:value "Added a French label."@en ;
        ] ,
        [
            dc:date "2023-11-27" ;
            rdf:value "Added a new rdfs:label in Spanish."@en ;
        ] ,
        [
            dc:date "2023-09-08" ;
            rdf:value """Object property added, along with its inverse property, in
               order to enable to express past partitive relations between Record Sets and their
               members (the current partitive relations being also added, including a transitive
               one)."""@en ;
        ] ;
.

:isActivityTypeOf
    a owl:ObjectProperty ;
    rdfs:label
        "is activity type of"@en ,
        "es tipo de actividad de"@es ,
        "est le type d’activité de"@fr ;
    rdfs:comment """Connects an Activity Type to an Activity that it
         categorizes."""@en ;
    rdfs:domain :ActivityType ;
    rdfs:isDefinedBy <https://www.ica.org/standards/RiC/ontology> ;
    rdfs:range :Activity ;
    rdfs:subPropertyOf :isOrWasCategoryOf ;
    owl:inverseOf :hasActivityType ;
    skos:changeNote
        [
            dc:date "2023-11-02" ;
            rdf:value "Added a new rdfs:label in Spanish."@en ;
        ] ,
        [
            dc:date "2021-01-22" ;
            rdf:value "changed the super property IRI."@en ;
        ] ,
        [
            dc:date "2023-08-28" ;
            rdf:value "Added a new rdfs:label in French."@en ;
        ] ;
.

:isAddresseeOf
    a owl:ObjectProperty ;
    rdfs:label
        "is addressee of"@en ,
        "es destino de"@es ,
        "est le destinataire de"@fr ;
    rdfs:comment "Inverse of 'has addressee' object property."@en ;
    rdfs:domain :Agent ;
    rdfs:isDefinedBy <https://www.ica.org/standards/RiC/ontology> ;
    rdfs:range
        [
            a owl:Class ;
            owl:unionOf (
                :Instantiation
                :RecordResource
            ) ;
        ] ;
    rdfs:subPropertyOf :isOrganicProvenanceOf ;
    owl:inverseOf :hasAddressee ;
    skos:changeNote
        [
            dc:date "2023-08-28" ;
            rdf:value "Added a new rdfs:label in French."@en ;
        ] ,
        [
            dc:date "2023-11-02" ;
            rdf:value "Added a new rdfs:label in Spanish."@en ;
        ] ;
    :RiCCMCorrespondingComponent """RiC-032i ('is addressee of'
         relation)"""@en ;
.

:isAuthorOf
    a owl:ObjectProperty ;
    rdfs:label
        "is author of"@en ,
        "es autor(a) de"@es ,
        "est le responsable intellectuel de"@fr ;
    rdfs:comment "Inverse of 'has author' object property."@en ;
    rdfs:domain
        [
            a owl:Class ;
            owl:unionOf (
                :Group
                :Person
                :Position
            ) ;
        ] ;
    rdfs:isDefinedBy <https://www.ica.org/standards/RiC/ontology> ;
    rdfs:range :Record ;
    rdfs:subPropertyOf :isCreatorOf ;
    owl:inverseOf :hasAuthor ;
    owl:propertyChainAxiom (
        :thingIsTargetOfRelation
        :authorshipRelation_role
        :relationHasSource
    ) ;
    skos:changeNote
        [
            dc:date "2023-08-28" ;
            rdf:value "Added a new rdfs:label in French."@en ;
        ] ,
        [
            dc:date "2020-12-29" ;
            rdf:value """Created following the addition of RiC-R079 relation in RiC-CM
               0.2"""@en ;
        ] ,
        [
            dc:date "2023-11-02" ;
            rdf:value "Added a new rdfs:label in Spanish."@en ;
        ] ,
        [
            dc:date "2023-11-08" ;
            rdf:value """In order to get a system of rolified Relation classes: modified
               the property chain axiom so that it now involves the new authorshipRelation_role
               object property."""@en ;
        ] ;
    :RiCCMCorrespondingComponent """RiC-R079i ('is author of'
         relation)"""@en ;
.

:isAuthorizingAgentInMandateRelation
    a owl:ObjectProperty ;
    rdfs:label
        "is authorizing agent in mandate relation"@en ,
        "es el agente autorizador en la relación normativa"@es ,
        """est l’agent donnant l’autorisation dans la relation impliquant un
         mandat"""@fr ;
    rdfs:comment """Connects an Agent that assigns the Mandate, to a Mandate
         Relation."""@en ;
    rdfs:domain :Agent ;
    rdfs:isDefinedBy <https://www.ica.org/standards/RiC/ontology> ;
    rdfs:range :MandateRelation ;
    rdfs:subPropertyOf :thingIsContextOfRelation ;
    owl:inverseOf :authorizingAgent ;
    skos:changeNote
        [
            dc:date "2023-11-02" ;
            rdf:value "Added a new rdfs:label in Spanish."@en ;
        ] ,
        [
            dc:date "2023-11-13" ;
            rdf:value """Added a new rdfs:label in French and fixed the Spanish
               label."""@en ;
        ] ;
.

:isBirthDateOf
    a owl:ObjectProperty ;
    rdfs:label
        "is birth date of"@en ,
        "es fecha de nacimiento de"@es ,
        "est la date de naissance de"@fr ;
    rdfs:comment """Connects a Date to a Person that was born on that
         Date."""@en ;
    rdfs:domain :Date ;
    rdfs:isDefinedBy <https://www.ica.org/standards/RiC/ontology> ;
    rdfs:range :Person ;
    rdfs:subPropertyOf :isBeginningDateOf ;
    owl:inverseOf :hasBirthDate ;
    skos:changeNote
        [
            dc:date "2023-08-28" ;
            rdf:value "Added a new rdfs:label in French."@en ;
        ] ,
        [
            dc:date "2023-11-02" ;
            rdf:value "Added a new rdfs:label in Spanish."@en ;
        ] ;
    :RiCCMCorrespondingComponent """RiC-R070 ('is birth date of'
         relation)"""@en ;
.

:isBirthPlaceOf
    a owl:ObjectProperty ;
    rdfs:label
        "is birth place of"@en ,
        "es lugar de nacimiento de"@es ,
        "est le lieu de naissance de"@fr ;
    rdfs:comment """Connects a Place to a Person who was born in that
         Place."""@en ;
    rdfs:domain :Place ;
    rdfs:isDefinedBy <https://www.ica.org/standards/RiC/ontology> ;
    rdfs:range :Person ;
    rdfs:subPropertyOf :isPlaceAssociatedWithAgent ;
    owl:inverseOf :hasBirthPlace ;
    skos:changeNote
        [
            dc:date "2023-11-12" ;
            rdf:value "Updated the description (rdfs:comment)."@en ;
        ] ,
        [
            dc:date "2023-10-19" ;
            rdf:value "Added for RiC-O v1.0."@en ;
        ] ,
        [
            dc:date "2023-10-26" ;
            rdf:value "Fixed the range."@en ;
        ] ,
        [
            dc:date "2023-11-27" ;
            rdf:value "Added a new rdfs:label in Spanish."@en ;
        ] ;
.

:isCarrierTypeOf
    a owl:ObjectProperty ;
    rdfs:label
        "is carrier type of"@en ,
        "es tipo de soporte de"@es ,
        "est le type de support de"@fr ;
    rdfs:comment """Connects a Carrier Type to an Instantiation whose carrier it
         categorizes."""@en ;
    rdfs:domain :CarrierType ;
    rdfs:isDefinedBy <https://www.ica.org/standards/RiC/ontology> ;
    rdfs:range :Instantiation ;
    rdfs:subPropertyOf :isOrWasCategoryOf ;
    owl:inverseOf :hasCarrierType ;
    skos:changeNote
        [
            dc:date "2023-08-28" ;
            rdf:value "Added a new rdfs:label in French."@en ;
        ] ,
        [
            dc:date "2023-11-02" ;
            rdf:value "Added a new rdfs:label in Spanish."@en ;
        ] ,
        [
            dc:date "2021-01-22" ;
            rdf:value "Changed the super property IRI."@en ;
        ] ;
.

:isChildOf
    a owl:ObjectProperty ;
    rdfs:label
        "is child of"@en ,
        "es hijo o hija de"@es ,
        "est l’enfant de"@fr ;
    rdfs:comment "Inverse of 'has child' object property."@en ;
    rdfs:domain :Person ;
    rdfs:isDefinedBy <https://www.ica.org/standards/RiC/ontology> ;
    rdfs:range :Person ;
    rdfs:subPropertyOf :hasAncestor ;
    owl:inverseOf :hasChild ;
    owl:propertyChainAxiom (
        :thingIsTargetOfRelation
        :childRelation_role
        :relationHasSource
    ) ;
    skos:changeNote
        [
            dc:date "2023-11-07" ;
            rdf:value """Added the property chain axiom so that this property is
               formally defined as a shortcut (the inverse property already was)."""@en ;
        ] ,
        [
            dc:date "2023-11-08" ;
            rdf:value """In order to get a system of rolified Relation classes: modified
               the property chain axiom so that it now involves the new childRelation_role object
               property."""@en ;
        ] ,
        [
            dc:date "2021-01-22" ;
            rdf:value """changed the IRI and label (changed made in order to make RiC-O
               compliant with RiC-CM 0.2; the name of this property in RiC-O 0.1 was
               "hasParent")."""@en ;
        ] ,
        [
            dc:date "2023-11-02" ;
            rdf:value "Added a new rdfs:label in Spanish."@en ;
        ] ,
        [
            dc:date "2023-08-28" ;
            rdf:value "Added a new rdfs:label in French."@en ;
        ] ;
    :RiCCMCorrespondingComponent """RiC-R018i ('is child of'
         relation)"""@en ;
.

:isCollectorOf
    a owl:ObjectProperty ;
    rdfs:label
        "is collector of"@en ,
        "es coleccionista de"@es ,
        "collecte"@fr ;
    rdfs:comment "Inverse of 'has collector' object property."@en ;
    rdfs:domain :Agent ;
    rdfs:isDefinedBy <https://www.ica.org/standards/RiC/ontology> ;
    rdfs:range
        [
            a owl:Class ;
            owl:unionOf (
                :Instantiation
                :RecordResource
            ) ;
        ] ;
    rdfs:subPropertyOf :isAccumulatorOf ;
    owl:inverseOf :hasCollector ;
    skos:changeNote
        [
            dc:date "2023-08-28" ;
            rdf:value "Added a new rdfs:label in French."@en ;
        ] ,
        [
            dc:date "2021-01-22" ;
            rdf:value """changed the IRI, label, inverse property and super property
               IRI, text definition, domain (changed made in order to make RiC-O compliant with
               RiC-CM 0.2; the name of this property in RiC-O 0.1 was "collects")."""@en ;
        ] ,
        [
            dc:date "2023-11-02" ;
            rdf:value "Added a new rdfs:label in Spanish."@en ;
        ] ;
    :RiCCMCorrespondingComponent """RiC-R030i ('is collector of'
         relation)"""@en ;
.

:isContentTypeOf
    a owl:ObjectProperty ;
    rdfs:label
        "is content type of"@en ,
        "es tipo de contenido de"@es ,
        "est le type de contenu de"@fr ;
    rdfs:comment """Connects a Content Type to a Record or Record Part whose content
         it categorizes."""@en ;
    rdfs:domain :ContentType ;
    rdfs:isDefinedBy <https://www.ica.org/standards/RiC/ontology> ;
    rdfs:range
        [
            a owl:Class ;
            owl:unionOf (
                :Record
                :RecordPart
            ) ;
        ] ;
    rdfs:subPropertyOf :isOrWasCategoryOf ;
    owl:inverseOf :hasContentOfType ;
    skos:changeNote
        [
            dc:date "2021-01-22" ;
            rdf:value "changed the text definition and super property IRI."@en ;
        ] ,
        [
            dc:date "2023-11-02" ;
            rdf:value "Added a new rdfs:label in Spanish."@en ;
        ] ,
        [
            dc:date "2023-08-28" ;
            rdf:value "Added a new rdfs:label in French."@en ;
        ] ;
.

:isCopyOf
    a owl:ObjectProperty ;
    rdfs:label
        "is copy of"@en ,
        "es copia de"@es ,
        "est la copie de"@fr ;
    rdfs:comment "Inverse of 'has copy' object property."@en ;
    rdfs:domain :RecordResource ;
    rdfs:isDefinedBy <https://www.ica.org/standards/RiC/ontology> ;
    rdfs:range :RecordResource ;
    rdfs:subPropertyOf
        :followsInTime ,
        :hasGeneticLinkToRecordResource ;
    owl:inverseOf :hasCopy ;
    skos:changeNote
        [
            dc:date "2023-11-02" ;
            rdf:value "Added a new rdfs:label in Spanish."@en ;
        ] ,
        [
            dc:date "2023-08-28" ;
            rdf:value "Added a new rdfs:label in French."@en ;
        ] ;
    :RiCCMCorrespondingComponent """RiC-R012i ('is copy of'
         relation)"""@en ;
.

:isCreationDateOf
    a owl:ObjectProperty ;
    rdfs:label
        "is creation date of"@en ,
        "es fecha de creación de"@es ,
        "est la date de création de"@fr ;
    rdfs:comment """Connects a Date to a Record Resource or Instantiation that was
         created at this Date."""@en ;
    rdfs:domain :Date ;
    rdfs:isDefinedBy <https://www.ica.org/standards/RiC/ontology> ;
    rdfs:range
        [
            a owl:Class ;
            owl:unionOf (
                :Instantiation
                :RecordResource
            ) ;
        ] ;
    rdfs:subPropertyOf :isBeginningDateOf ;
    owl:inverseOf :hasCreationDate ;
    skos:changeNote
        [
            dc:date "2023-10-12" ;
            rdf:value "Added the French label" ;
        ] ,
        [
            dc:date "2023-11-12" ;
            rdf:value """Aligned with RiC-CM 1.0: updated the
               skos:scopeNote."""@en ;
        ] ,
        [
            dc:date "2023-11-27" ;
            rdf:value "Added a new rdfs:label in Spanish."@en ;
        ] ,
        [
            dc:date "2023-09-22" ;
            rdf:value "Added in RiC-O 1.0."@en ;
        ] ;
    skos:scopeNote """When used for a Record Set (e.g. a file), it is the creation
         date of the Record Set itself rather than the creation date of the members of the Record
         Set. To record the creation date of members of the Record Set, use 'is or was creation date
         of all members of', 'is or was creation date of most members of’ or 'is or was creation
         date of some members of’."""@en ;
    :RiCCMCorrespondingComponent """RiC-R080 ('is creation date of'
         relation)"""@en ;
.

:isDateOfOccurrenceOf
    a owl:ObjectProperty ;
    rdfs:label
        "is date of occurrence of"@en ,
        "es fecha de ocurrencia de"@es ,
        "est la date d'occurrence de"@fr ;
    rdfs:comment """Connects a Date to an Event that occurred at this Date. An event
         or activity can be recurrent, which implies that one single event can be related to several
         dates."""@en ;
    rdfs:domain :Date ;
    rdfs:isDefinedBy <https://www.ica.org/standards/RiC/ontology> ;
    rdfs:range :Event ;
    rdfs:subPropertyOf
        :isAssociatedWithEvent ,
        :isDateAssociatedWith ;
    owl:inverseOf :occurredAtDate ;
    skos:changeNote
        [
            dc:date "2023-11-27" ;
            rdf:value "Added a new rdfs:label in Spanish."@en ;
        ] ,
        [
            dc:date "2023-10-13" ;
            rdf:value """Renamed the property to correct a spelling mistake. Also
               corrected the annotations when necessary."""@en ;
        ] ,
        [
            dc:date "2023-10-12" ;
            rdf:value "Added the property"@en ;
        ] ,
        [
            dc:date "2023-10-17" ;
            rdf:value """Made this property a subproperty of
               isAssociatedWithEvent"""@en ;
        ] ;
    :RiCCMCorrespondingComponent """RiC-R084 ('is date of occurrence of'
         relation)"""@en ;
.

:isDateTypeOf
    a owl:ObjectProperty ;
    rdfs:label
        "is date type of"@en ,
        "es tipo de fecha de"@es ,
        "est le type de date de"@fr ;
    rdfs:comment "Connects a Date Type to a Date that it categorizes."@en ;
    rdfs:domain :DateType ;
    rdfs:isDefinedBy <https://www.ica.org/standards/RiC/ontology> ;
    rdfs:range :Date ;
    rdfs:subPropertyOf :isOrWasCategoryOf ;
    owl:inverseOf :hasDateType ;
    skos:changeNote
        [
            dc:date "2023-10-10" ;
            rdf:value "Added a rdfs:comment and a French rdfs:label."@en ;
        ] ,
        [
            dc:date "2023-09-22" ;
            rdf:value "Added in RiC-O 1.0."@en ;
        ] ,
        [
            dc:date "2023-11-27" ;
            rdf:value "Added a new rdfs:label in Spanish."@en ;
        ] ;
.

:isDeathDateOf
    a owl:ObjectProperty ;
    rdfs:label
        "is death date of"@en ,
        "es fecha de muerte de"@es ,
        "est la date de décès de"@fr ;
    rdfs:comment "Connects a Date to a Person who died on that Date."@en ;
    rdfs:domain :Date ;
    rdfs:isDefinedBy <https://www.ica.org/standards/RiC/ontology> ;
    rdfs:range :Person ;
    rdfs:subPropertyOf :isEndDateOf ;
    owl:inverseOf :hasDeathDate ;
    skos:changeNote
        [
            dc:date "2023-08-28" ;
            rdf:value "Added a new rdfs:label in French."@en ;
        ] ,
        [
            dc:date "2023-11-02" ;
            rdf:value "Added a new rdfs:label in Spanish."@en ;
        ] ;
    :RiCCMCorrespondingComponent """RiC-R072 ('is death date of'
         relation)"""@en ;
.

:isDeathPlaceOf
    a owl:ObjectProperty ;
    rdfs:label
        "is death place of"@en ,
        "es lugar de muerte de"@es ,
        "est le lieu de décès de"@fr ;
    rdfs:comment """Connects a Place to a Person who died in that
         Place."""@en ;
    rdfs:domain :Place ;
    rdfs:isDefinedBy <https://www.ica.org/standards/RiC/ontology> ;
    rdfs:range :Person ;
    rdfs:subPropertyOf :isPlaceAssociatedWithAgent ;
    owl:inverseOf :hasDeathPlace ;
    skos:changeNote
        [
            dc:date "2023-10-26" ;
            rdf:value """Fixed the range and the French label of the
               property."""@en ;
        ] ,
        [
            dc:date "2023-11-12" ;
            rdf:value "Updated the description (rdfs:comment)."@en ;
        ] ,
        [
            dc:date "2023-10-19" ;
            rdf:value "Property added to RiC-0 1.0"@en ;
        ] ,
        [
            dc:date "2023-11-27" ;
            rdf:value "Added a new rdfs:label in Spanish."@en ;
        ] ;
.

:isDestructionDateOf
    a owl:ObjectProperty ;
    rdfs:label
        "is destruction date of"@en ,
        "es fecha de destrucción de"@es ,
        "est la date de destruction de"@fr ;
    rdfs:comment """Connects a Date to a Thing that was destructed at that
         Date."""@en ;
    rdfs:domain :Date ;
    rdfs:isDefinedBy <https://www.ica.org/standards/RiC/ontology> ;
    rdfs:range :Thing ;
    rdfs:subPropertyOf :isEndDateOf ;
    owl:inverseOf :hasDestructionDate ;
    skos:changeNote
        [
            dc:date "2023-10-12" ;
            rdf:value "Renamed deletion into destruction."@en ;
        ] ,
        [
            dc:date "2023-11-27" ;
            rdf:value "Added a new rdfs:label in Spanish."@en ;
        ] ,
        [
            dc:date "2023-09-22" ;
            rdf:value "Added in RiC-O 1.0."@en ;
        ] ,
        [
            dc:date "2023-10-14" ;
            rdf:value "Added a rdfs:comment; same to the inverse property."@en ;
        ] ;
.

:isDirectComponentOf
    a owl:ObjectProperty ;
    rdfs:label
        "is direct component of"@en ,
        "es componente directo de"@es ,
        "est le composant direct de"@fr ;
    rdfs:comment """Connects an Instantiation to another Instantiation of which it is
         a direct component."""@en ;
    rdfs:domain :Instantiation ;
    rdfs:isDefinedBy <https://www.ica.org/standards/RiC/ontology> ;
    rdfs:range :Instantiation ;
    rdfs:subPropertyOf
        :isComponentOfTransitive ,
        :isDirectPartOf ;
    owl:inverseOf :hasDirectComponent ;
    skos:changeNote
        [
            dc:date "2023-09-08" ;
            skos:changeNote """Object property added, along with its inverse property,
               in order to enable to express current, direct, partitive relations between
               instantiations (the possibly indirect, transitive relation, superproperty of this
               one, being also added)."""@en ;
        ] ,
        [
            dc:date "2023-11-27" ;
            rdf:value "Added a new rdfs:label in Spanish."@en ;
        ] ,
        [
            dc:date "2023-11-12" ;
            rdf:value "Updated the labels."@en ;
        ] ;
.

:isDirectConstituentOf
    a owl:ObjectProperty ;
    rdfs:label
        "is direct constituent of"@en ,
        "es elemento constitutivo directo de"@es ,
        "est un constituant direct de"@fr ;
    rdfs:comment """Connects a Record or Record Part to another Record or Record Part
         of which it is a direct constituent."""@en ;
    rdfs:domain
        [
            a owl:Class ;
            owl:unionOf (
                :Record
                :RecordPart
            ) ;
        ] ;
    rdfs:isDefinedBy <https://www.ica.org/standards/RiC/ontology> ;
    rdfs:range
        [
            a owl:Class ;
            owl:unionOf (
                :Record
                :RecordPart
            ) ;
        ] ;
    rdfs:subPropertyOf
        :isConstituentOfTransitive ,
        :isDirectPartOf ;
    owl:inverseOf :hasDirectConstituent ;
    skos:changeNote
        [
            dc:date "2023-11-12" ;
            rdf:value "Updated the labels."@en ;
        ] ,
        [
            dc:date "2023-09-08" ;
            rdf:value """Object property added, along with its inverse property, in
               order to enable to express current, direct, partitive relations between records and
               other records or record parts (the possibly indirect, transitive relation,
               superproperty of this one, being also added)."""@en ;
        ] ,
        [
            dc:date "2023-10-26" ;
            rdf:value "Added RecordPart to the range."@en ;
        ] ,
        [
            dc:date "2023-11-27" ;
            rdf:value "Added a new rdfs:label in Spanish."@en ;
        ] ;
.

:isDirectSubdivisionOf
    a owl:ObjectProperty ;
    rdfs:label
        "is direct subdivision of"@en ,
        "es subdivisión directa de"@es ,
        "est la subdivision directe de"@fr ;
    rdfs:comment """Connects a Group to the Group it is a direct subdivision
         of."""@en ;
    rdfs:domain :Group ;
    rdfs:isDefinedBy <https://www.ica.org/standards/RiC/ontology> ;
    rdfs:range :Group ;
    rdfs:subPropertyOf
        :isDirectPartOf ,
        :isDirectSubordinateTo ,
        :isSubdivisionOfTransitive ;
    owl:inverseOf :hasDirectSubdivision ;
    skos:changeNote
        [
            dc:date "2023-11-27" ;
            rdf:value "Added a new rdfs:label in Spanish."@en ;
        ] ,
        [
            dc:date "2023-11-12" ;
            rdf:value "Updated the labels."@en ;
        ] ,
        [
            dc:date "2023-09-08" ;
            rdf:value """Object property added, along with its inverse property, in
               order to enable to express current, direct, partitive relations between groups (the
               possibly indirect, transitive relation, superproperty of this one, being also
               added)."""@en ;
        ] ;
.

:isDirectSubeventOf
    a owl:ObjectProperty ;
    rdfs:label
        "is direct subevent of"@en ,
        "es parte directa de evento de"@es ,
        "est un événement constituant directement l’événement"@fr ;
    rdfs:comment """Connects an ongoing Event to the Event it is a direct part
         of."""@en ;
    rdfs:domain :Event ;
    rdfs:isDefinedBy <https://www.ica.org/standards/RiC/ontology> ;
    rdfs:range :Event ;
    rdfs:subPropertyOf
        :isDirectPartOf ,
        :isSubeventOfTransitive ;
    owl:inverseOf :hasDirectSubevent ;
    skos:changeNote
        [
            dc:date "2023-09-08" ;
            rdf:value """Object property added, along with its inverse property, in
               order to enable to express current, direct, partitive relations between ongoing
               events (the possibly indirect, transitive relation, superproperty of this one, being
               also added)."""@en ;
        ] ,
        [
            dc:date "2023-11-12" ;
            rdf:value "Updated the labels."@en ;
        ] ,
        [
            dc:date "2023-11-27" ;
            rdf:value "Added a new rdfs:label in Spanish."@en ;
        ] ;
.

:isDirectlyContainedBy
    a owl:ObjectProperty ;
    rdfs:label
        "is directly contained by"@en ,
        "está directamente contenido en"@es ,
        "est directement contenu par"@fr ;
    rdfs:comment """Connects a Place to a Place that directly contains
         it."""@en ;
    rdfs:domain :Place ;
    rdfs:isDefinedBy <https://www.ica.org/standards/RiC/ontology> ;
    rdfs:range :Place ;
    rdfs:subPropertyOf
        :isContainedByTransitive ,
        :isDirectPartOf ;
    owl:inverseOf :directlyContains ;
    skos:changeNote
        [
            dc:date "2023-11-12" ;
            rdf:value "Updated the labels."@en ;
        ] ,
        [
            dc:date "2023-09-08" ;
            rdf:value """Object property added, along with its inverse property, in
               order to enable to express current, direct, partitive relations between places (the
               possibly indirect, transitive relation, superproperty of this one, being also
               added)."""@en ;
        ] ,
        [
            dc:date "2023-11-27" ;
            rdf:value "Added a new rdfs:label in Spanish."@en ;
        ] ;
.

:isDirectlyIncludedIn
    a owl:ObjectProperty ;
    rdfs:label
        "is directly included in"@en ,
        "está directamente incluido en"@es ,
        "est directement inclus dans"@fr ;
    rdfs:comment """Connects a Record to a Record or Record Set in which it is
         directly included."""@en ;
    rdfs:domain
        [
            a owl:Class ;
            owl:unionOf (
                :Record
                :RecordSet
            ) ;
        ] ;
    rdfs:isDefinedBy <https://www.ica.org/standards/RiC/ontology> ;
    rdfs:range :RecordSet ;
    rdfs:subPropertyOf
        :isDirectPartOf ,
        :isIncludedInTransitive ;
    owl:inverseOf :directlyIncludes ;
    skos:changeNote
        [
            dc:date "2023-11-27" ;
            rdf:value "Added a new rdfs:label in Spanish."@en ;
        ] ,
        [
            dc:date "2023-11-12" ;
            rdf:value "Updated the labels."@en ;
        ] ,
        [
            dc:date "2023-09-08" ;
            rdf:value """Object property added, along with its inverse property, in
               order to enable to express current, direct, partitive relations between Record Sets
               and their members (the possibly indirect, transitive relation, superproperty of this
               one, being also added)."""@en ;
        ] ;
.

:isDocumentaryFormTypeOf
    a owl:ObjectProperty ;
    rdfs:label
        "is documentary form type of"@en ,
        "es tipo documental de"@es ,
        "est le type de document de"@fr ;
    rdfs:comment """Connects a Documentary Form Type to a Record or Record Part that
         it categorizes."""@en ;
    rdfs:domain :DocumentaryFormType ;
    rdfs:isDefinedBy <https://www.ica.org/standards/RiC/ontology> ;
    rdfs:range
        [
            a owl:Class ;
            owl:unionOf (
                :Record
                :RecordPart
            ) ;
        ] ;
    rdfs:subPropertyOf :isOrWasCategoryOf ;
    owl:inverseOf :hasDocumentaryFormType ;
    skos:changeNote
        [
            dc:date "2023-08-28" ;
            rdf:value "Added a new rdfs:label in French."@en ;
        ] ,
        [
            dc:date "2023-11-02" ;
            rdf:value "Added a new rdfs:label in Spanish."@en ;
        ] ,
        [
            dc:date "2021-01-22" ;
            rdf:value "changed the superproperty IRI."@en ;
        ] ;
.

:isDraftOf
    a owl:ObjectProperty ;
    rdfs:label
        "is draft of"@en ,
        "es borrador de"@es ,
        "est l’ébauche de"@fr ;
    rdfs:comment "Connects a draft to the final version of a Record."@en ;
    rdfs:domain
        [
            a owl:Class ;
            owl:unionOf (
                :Record
                :RecordPart
            ) ;
        ] ;
    rdfs:isDefinedBy <https://www.ica.org/standards/RiC/ontology> ;
    rdfs:range
        [
            a owl:Class ;
            owl:unionOf (
                :Record
                :RecordPart
            ) ;
        ] ;
    rdfs:subPropertyOf
        :hasGeneticLinkToRecordResource ,
        :precedesInTime ;
    owl:inverseOf :hasDraft ;
    skos:changeNote
        [
            dc:date "2023-11-12" ;
            rdf:value """Aligned with RiC-CM 1.0: updated the
               skos:scopeNote."""@en ;
        ] ,
        [
            dc:date "2023-08-28" ;
            rdf:value "Added a new rdfs:label in French."@en ;
        ] ,
        [
            dc:date "2023-11-02" ;
            rdf:value "Added a new rdfs:label in Spanish."@en ;
        ] ;
    skos:scopeNote """There may be zero to many intermediate records, ignored or
         unknown, between the two connected Records."""@en ;
    :RiCCMCorrespondingComponent """RiC-R011 ('is draft of'
         relation)"""@en ;
.

:isEquivalentTo
    a
        owl:ObjectProperty ,
        owl:SymmetricProperty ;
    rdfs:label
        "is equivalent to"@en ,
        "equivale a"@es ,
        "est l’équivalent de"@fr ;
    rdfs:comment "Connects two Things that are considered equivalent."@en ;
    rdfs:domain :Thing ;
    rdfs:isDefinedBy <https://www.ica.org/standards/RiC/ontology> ;
    rdfs:range :Thing ;
    rdfs:subPropertyOf :isRelatedTo ;
    skos:changeNote
        [
            dc:date "2023-11-02" ;
            rdf:value "Added a new rdfs:label in Spanish."@en ;
        ] ,
        [
            dc:date "2023-08-28" ;
            rdf:value "Added a new rdfs:label in French."@en ;
        ] ;
.

:isEventTypeOf
    a owl:ObjectProperty ;
    rdfs:label
        "is event type of"@en ,
        "es tipo de evento de"@es ,
        "est le type d’événement de"@fr ;
    rdfs:comment """Connects an Event Type to an Event that it
         categorizes."""@en ;
    rdfs:domain :EventType ;
    rdfs:isDefinedBy <https://www.ica.org/standards/RiC/ontology> ;
    rdfs:range :Event ;
    rdfs:subPropertyOf :isOrWasCategoryOf ;
    owl:inverseOf :hasEventType ;
    skos:changeNote
        [
            dc:date "2023-08-28" ;
            rdf:value "Added a new rdfs:label in French."@en ;
        ] ,
        [
            dc:date "2023-11-02" ;
            rdf:value "Added a new rdfs:label in Spanish."@en ;
        ] ,
        [
            dc:date "2021-01-22" ;
            rdf:value "changed the superproperty IRI."@en ;
        ] ,
        [
            dc:date "2024-03-15" ;
            rdf:value "Fixed typo in rdfs:comment"@en ;
        ] ;
.

:isEvidencedBy
    a owl:ObjectProperty ;
    rdfs:label
        "is evidenced by"@en ,
        "se evidencia en"@es ,
        "est attestée par"@fr ;
    rdfs:comment """Connects a Relation to a Record Resource that is used for proving
         is existence or describing it."""@en ;
    rdfs:domain :Relation ;
    rdfs:isDefinedBy <https://www.ica.org/standards/RiC/ontology> ;
    rdfs:range :RecordResource ;
    rdfs:subPropertyOf :relationConnects ;
    owl:inverseOf :evidences ;
    skos:changeNote
        [
            dc:date "2023-12-27" ;
            rdf:value """Renamed the object property (was 'has source') and reduced its
               domain to Relation (the domain was the union of Record Resource and Relation) and its
               range to Record Resource (the range was the union of Agent and Record Resource).
               Consequently updated the superproperty, the labels, and added a
               rico:RiCCMCorrespondingComponent. Same for the inverse object property."""@en ;
        ] ,
        [
            dc:date "2023-08-28" ;
            rdf:value "Added a new rdfs:label in French."@en ;
        ] ,
        [
            dc:date "2023-11-02" ;
            rdf:value "Added a new rdfs:label in Spanish."@en ;
        ] ;
    :RiCCMCorrespondingComponent """Object property implementation of RiC-RA05 (Source
         of Relation attribute)."""@en ;
.

:isExtentOf
    a owl:ObjectProperty ;
    rdfs:label
        "is extent of"@en ,
        "es extensión de"@es ,
        "est la mesure de"@fr ;
    rdfs:comment "Connects an Extent to a Thing"@en ;
    rdfs:domain :Extent ;
    rdfs:isDefinedBy <https://www.ica.org/standards/RiC/ontology> ;
    rdfs:range :Thing ;
    rdfs:subPropertyOf :isRelatedTo ;
    owl:inverseOf :hasExtent ;
    skos:changeNote
        [
            dc:date "2023-08-28" ;
            rdf:value """Added a new rdfs:label in French; added an xml:lang attribute
               to the rdfs:comment."""@en ;
        ] ,
        [
            dc:date "2023-08-28" ;
            rdf:value """Changed the range (was Instantiation or RecordResource) to
               Thing ; changed the definition accordingly"""@en ;
        ] ,
        [
            dc:date "2020-10-28" ;
            rdf:value """Object property created along with the Extent class and its
               subclasses, in order to provide methods for handling extent accurately."""@en ;
        ] ,
        [
            dc:date "2023-11-02" ;
            rdf:value "Added a new rdfs:label in Spanish."@en ;
        ] ,
        [
            dc:date "2023-11-08" ;
            rdf:value "Fixed the range."@en ;
        ] ;
.

:isExtentTypeOf
    a owl:ObjectProperty ;
    rdfs:label
        "is extent type of"@en ,
        "es tipo de extensión de"@es ,
        "est le type de mesure de"@fr ;
    rdfs:comment """Connects an Extent Type to an Extent that it
         categorizes."""@en ;
    rdfs:domain :ExtentType ;
    rdfs:isDefinedBy <https://www.ica.org/standards/RiC/ontology> ;
    rdfs:range :Extent ;
    rdfs:subPropertyOf :isOrWasCategoryOf ;
    owl:inverseOf :hasExtentType ;
    skos:changeNote
        [
            dc:date "2023-11-02" ;
            rdf:value "Added a new rdfs:label in Spanish."@en ;
        ] ,
        [
            dc:date "2020-11-01" ;
            rdf:value """Object property added along with the Extent Type
               class."""@en ;
        ] ,
        [
            dc:date "2020-11-21" ;
            rdf:value "Added a rdfs:comment."@en ;
        ] ,
        [
            dc:date "2023-08-28" ;
            rdf:value "Added a new rdfs:label in French."@en ;
        ] ;
.

:isFamilyTypeOf
    a owl:ObjectProperty ;
    rdfs:label
        "is family type of"@en ,
        "es tipo de familia de"@es ,
        "est le type de famille de"@fr ;
    rdfs:comment """Connects a Family Type to a Family that it
         categorizes."""@en ;
    rdfs:domain :FamilyType ;
    rdfs:isDefinedBy <https://www.ica.org/standards/RiC/ontology> ;
    rdfs:range :Family ;
    rdfs:subPropertyOf :isOrWasCategoryOf ;
    owl:inverseOf :hasFamilyType ;
    skos:changeNote
        [
            dc:date "2023-08-28" ;
            rdf:value "Added a new rdfs:label in French."@en ;
        ] ,
        [
            dc:date "2021-01-22" ;
            rdf:value "changed the superproperty IRI."@en ;
        ] ,
        [
            dc:date "2023-11-02" ;
            rdf:value "Added a new rdfs:label in Spanish."@en ;
        ] ,
        [
            dc:date "2024-03-15" ;
            rdf:value "Fixed typo in rdfs:comment"@en ;
        ] ;
.

:isFromUseDateOf
    a owl:ObjectProperty ;
    rdfs:label
        "is from use date of"@en ,
        "es fecha desde la que se usa de"@es ,
        "est la date à partir de laquelle est utilisé"@fr ;
    rdfs:comment """Connects a Date to an Appellation, when it is the date at which
         the Appellation was first used."""@en ;
    rdfs:domain :Date ;
    rdfs:isDefinedBy <https://www.ica.org/standards/RiC/ontology> ;
    rdfs:range :Appellation ;
    rdfs:subPropertyOf :isBeginningDateOf ;
    owl:inverseOf :wasUsedFromDate ;
    skos:changeNote
        [
            dc:date "2023-11-02" ;
            rdf:value "Added a new rdfs:label in Spanish."@en ;
        ] ,
        [
            dc:date "2023-10-19" ;
            rdf:value "Made this property subPropertyOf isBeginningDateOf."@en ;
        ] ,
        [
            dc:date "2023-08-28" ;
            rdf:value "Added a new rdfs:label in French."@en ;
        ] ;
.

:isIdentifierTypeOf
    a owl:ObjectProperty ;
    rdfs:label
        "is identifier type of"@en ,
        "es tipo de identificador de"@es ,
        "est le type d’identifiant de"@fr ;
    rdfs:comment """Connects an Identifier Type and an Identifier that it
         categorizes."""@en ;
    rdfs:domain :IdentifierType ;
    rdfs:isDefinedBy <https://www.ica.org/standards/RiC/ontology> ;
    rdfs:range :Identifier ;
    rdfs:subPropertyOf :isOrWasCategoryOf ;
    owl:inverseOf :hasIdentifierType ;
    skos:changeNote
        [
            dc:date "2021-01-22" ;
            rdf:value "changed the superproperty IRI."@en ;
        ] ,
        [
            dc:date "2020-10-19" ;
            rdf:value """Object property added along with IdentifierType class and
               hasIdentifierType object property. """@en ;
        ] ,
        [
            dc:date "2023-11-02" ;
            rdf:value "Added a new rdfs:label in Spanish."@en ;
        ] ,
        [
            dc:date "2023-08-28" ;
            rdf:value "Added a new rdfs:label in French."@en ;
        ] ;
.

:isLastUpdateDateOf
    a owl:ObjectProperty ;
    rdfs:label
        "is last update date of"@en ,
        "es fecha de última actualización de"@es ,
        "est la date de dernière mise à jour de"@fr ;
    rdfs:comment """Connects a Date and a Thing that was last modified at this
         Date."""@en ;
    rdfs:domain :Date ;
    rdfs:isDefinedBy <https://www.ica.org/standards/RiC/ontology> ;
    rdfs:range :Thing ;
    rdfs:subPropertyOf :isModificationDateOf ;
    owl:inverseOf :wasLastUpdatedAtDate ;
    skos:changeNote
        [
            dc:date "2023-11-02" ;
            rdf:value "Added a new rdfs:label in Spanish."@en ;
        ] ,
        [
            dc:date "2023-08-28" ;
            rdf:value "Added a new rdfs:label in French."@en ;
        ] ;
.

:isOrWasAffectedBy
    a owl:ObjectProperty ;
    rdfs:label
        "is or was affected by"@en ,
        "es o era afectado por"@es ,
        "est ou a été affecté par"@fr ;
    rdfs:comment "Inverse of 'affects or affected' object property."@en ;
    rdfs:domain :Thing ;
    rdfs:isDefinedBy <https://www.ica.org/standards/RiC/ontology> ;
    rdfs:range :Event ;
    rdfs:subPropertyOf :isOrWasParticipantIn ;
    owl:inverseOf :affectsOrAffected ;
    skos:changeNote
        [
            dc:date "2023-08-28" ;
            rdf:value "Added a new rdfs:label in French."@en ;
        ] ,
        [
            dc:date "2021-01-22" ;
            rdf:value """changed the IRI, label, inverse property IRI, text definition
               and corresponding CM component (changed made in order to make RiC-O compliant with
               RiC-CM 0.2; the name of this property in RiC-O 0.1 was "affectedBy")."""@en ;
        ] ,
        [
            dc:date "2023-11-02" ;
            rdf:value "Added a new rdfs:label in Spanish."@en ;
        ] ;
    :RiCCMCorrespondingComponent """RiC-R059i ('is or was affected by'
         relation)"""@en ;
.

:isOrWasAgentNameOf
    a owl:ObjectProperty ;
    rdfs:label
        "is or was agent name of"@en ,
        "es o era el nombre de agente de"@es ,
        "est ou a été le nom de"@fr ;
    rdfs:comment """Connects an Agent Name to an Agent it designates or
         designated."""@en ;
    rdfs:domain :AgentName ;
    rdfs:isDefinedBy <https://www.ica.org/standards/RiC/ontology> ;
    rdfs:range :Agent ;
    rdfs:subPropertyOf :isOrWasNameOf ;
    owl:inverseOf :hasOrHadAgentName ;
    skos:changeNote
        [
            dc:date "2023-11-02" ;
            rdf:value "Added a new rdfs:label in Spanish."@en ;
        ] ,
        [
            dc:date "2023-08-28" ;
            rdf:value "Added a new rdfs:label in French."@en ;
        ] ,
        [
            dc:date "2021-01-22" ;
            rdf:value """changed the IRI, label, inverse property IRI, textual
               definition (the name of this property in RiC-O 0.1 was "isAgentNameOf")."""@en ;
        ] ;
.

:isOrWasAnalogueInstantiationOf
    a owl:ObjectProperty ;
    rdfs:label
        "is or was analogue instantiation of"@en ,
        "es or era instanciación analogica de"@es ,
        "est ou a été une instanciation analogique de"@fr ;
    rdfs:comment """Inverse of 'has or had analogue instantiation' object
         property."""@en ;
    rdfs:domain :Instantiation ;
    rdfs:isDefinedBy <https://www.ica.org/standards/RiC/ontology> ;
    rdfs:range :RecordResource ;
    rdfs:subPropertyOf :isOrWasInstantiationOf ;
    owl:inverseOf :hasOrHadAnalogueInstantiation ;
    skos:changeNote
        [
            dc:date "2023-08-29" ;
            rdf:value "Added the property."@en ;
        ] ,
        [
            dc:date "2023-11-27" ;
            rdf:value "Added a new rdfs:label in Spanish."@en ;
        ] ,
        [
            dc:date "2023-12-30" ;
            rdf:value "Fixed a typo in the French label."@en ;
        ] ;
.

:isOrWasContentTypeOfAllMembersOf
    a owl:ObjectProperty ;
    rdfs:label
        "is or was content type of all members of"@en ,
        "es o era tipo de contenido de todos los miembros de"@es ,
        "est ou a été le type de contenu de tous les membres de"@fr ;
    rdfs:comment """Connects a Content Type and a Record Set whose all past or present
         Record or Record Part members have that Content Type."""@en ;
    rdfs:domain :ContentType ;
    rdfs:isDefinedBy <https://www.ica.org/standards/RiC/ontology> ;
    rdfs:range :RecordSet ;
    rdfs:subPropertyOf :isOrWasCategoryOfAllMembersOf ;
    owl:inverseOf :hasOrHadAllMembersWithContentType ;
    skos:changeNote
        [
            dc:date "2023-08-28" ;
            rdf:value "Added a new rdfs:label in French."@en ;
        ] ,
        [
            dc:date "2020-12-28" ;
            rdf:value """Object property added for handling the case where a Record Set
               is described as having all or some members that belong to some category (see RiC-CM
               0.2 attributes section, #4.4 on Record Set, Record and Record Part
               attributes)."""@en ;
        ] ,
        [
            dc:date "2023-11-02" ;
            rdf:value "Added a new rdfs:label in Spanish."@en ;
        ] ;
.

:isOrWasContentTypeOfSomeMembersOf
    a owl:ObjectProperty ;
    rdfs:label
        "is or was content type of some members of"@en ,
        "es o era tipo de contenido de algunos miembros de"@es ,
        "est ou a été le type de contenu de certains membres de"@fr ;
    rdfs:comment """Connects a Content Type and a Record Set whose some past or
         present Record or Record Part members have that Content Type."""@en ;
    rdfs:domain :ContentType ;
    rdfs:isDefinedBy <https://www.ica.org/standards/RiC/ontology> ;
    rdfs:range :RecordSet ;
    rdfs:subPropertyOf :isOrWasCategoryOfSomeMembersOf ;
    owl:inverseOf :hasOrHadSomeMembersWithContentType ;
    skos:changeNote
        [
            dc:date "2023-08-28" ;
            rdf:value "Added a new rdfs:label in French."@en ;
        ] ,
        [
            dc:date "2023-11-02" ;
            rdf:value "Added a new rdfs:label in Spanish."@en ;
        ] ,
        [
            dc:date "2020-12-28" ;
            rdf:value """Object property added for handling the case where a Record Set
               is described as having all or some members that belong to some category (see RiC-CM
               0.2 attributes section, #4.4 on Record Set, Record and Record Part
               attributes)."""@en ;
        ] ;
.

:isOrWasCoordinatesOf
    a owl:ObjectProperty ;
    rdfs:label
        "is or was coordinates of"@en ,
        "son o eran coordenadas de lugar de"@es ,
        "ont ou ont été les coordonnées de"@fr ;
    rdfs:comment """Connects an instance of Coordinates to a Physical Location it
         locates or located on earth, according to some reference system."""@en ;
    rdfs:domain :Coordinates ;
    rdfs:isDefinedBy <https://www.ica.org/standards/RiC/ontology> ;
    rdfs:range :PhysicalLocation ;
    rdfs:subPropertyOf :isRelatedTo ;
    owl:inverseOf :hasOrHadCoordinates ;
    skos:changeNote
        [
            dc:date "2023-08-28" ;
            rdf:value "Added a new rdfs:label in French."@en ;
        ] ,
        [
            dc:date "2021-01-22" ;
            rdf:value """changed the IRI, label, inverse property IRI, text definition
               (the name of this property in RiC-O 0.1 was "isCoordinatesOf")."""@en ;
        ] ,
        [
            dc:date "2023-11-02" ;
            rdf:value "Added a new rdfs:label in Spanish."@en ;
        ] ;
.

:isOrWasCorporateBodyTypeOf
    a owl:ObjectProperty ;
    rdfs:label
        "is or was corporate body type of"@en ,
        "es o era tipo de institución de"@es ,
        "est ou a été le type de collectivité de"@fr ;
    rdfs:comment """Connects a Corporate Body Type to a Corporate Body that it
         categorizes or categorized."""@en ;
    rdfs:domain :CorporateBodyType ;
    rdfs:isDefinedBy <https://www.ica.org/standards/RiC/ontology> ;
    rdfs:range :CorporateBody ;
    rdfs:subPropertyOf :isOrWasCategoryOf ;
    owl:inverseOf :hasOrHadCorporateBodyType ;
    skos:changeNote
        [
            dc:date "2023-08-28" ;
            rdf:value "Added a new rdfs:label in French."@en ;
        ] ,
        [
            dc:date "2021-01-22" ;
            rdf:value """changed the IRI, label, inverse property IRI, text definition
               (the name of this property in RiC-O 0.1 was "isCorporateBodyTypeOf")."""@en ;
        ] ,
        [
            dc:date "2023-11-02" ;
            rdf:value "Added a new rdfs:label in Spanish."@en ;
        ] ;
.

:isOrWasCreationDateOfAllMembersOf
    a owl:ObjectProperty ;
    rdfs:label
        "is or was creation date of all members of"@en ,
        "es o era fecha de creación de todos los miembros de"@es ,
        "est ou a été la date de création de tous les membres de"@fr ;
    rdfs:comment """Connects a Date to a Record Set all of whose present or past
         members were created at this Date."""@en ;
    rdfs:domain :Date ;
    rdfs:isDefinedBy <https://www.ica.org/standards/RiC/ontology> ;
    rdfs:range :RecordSet ;
    rdfs:subPropertyOf :isBeginningDateOf ;
    owl:inverseOf :hasOrHadAllMembersWithCreationDate ;
    skos:changeNote
        [
            dc:date "2023-10-13" ;
            rdf:value """renamed the property in order to take the past members of the
               record set into account. Adjusted the annotations accordingly."""@en ;
        ] ,
        [
            dc:date "2023-11-27" ;
            rdf:value "Added a new rdfs:label in Spanish."@en ;
        ] ,
        [
            dc:date "2023-09-22" ;
            rdf:value "Added in RiC-O 1.0."@en ;
        ] ,
        [
            dc:date "2023-10-12" ;
            rdf:value "Added the French label" ;
        ] ;
    :RiCCMCorrespondingComponent """RiC-R081 ('is or was creation date of all members
         of' relation)"""@en ;
.

:isOrWasCreationDateOfMostMembersOf
    a owl:ObjectProperty ;
    rdfs:label
        "is or was creation date of most members of"@en ,
        """es o era fecha de creación de la mayoría de los miembros
         de"""@es ,
        """est ou a été la date de création de la plupart des membres
         de"""@fr ;
    rdfs:comment """Connects a Date to a Record Set most of whose present or past
         members were created at this Date."""@en ;
    rdfs:domain :Date ;
    rdfs:isDefinedBy <https://www.ica.org/standards/RiC/ontology> ;
    rdfs:range :RecordSet ;
    rdfs:subPropertyOf :isOrWasCreationDateOfSomeMembersOf ;
    owl:inverseOf :hasOrHadMostMembersWithCreationDate ;
    skos:changeNote
        [
            dc:date "2023-10-10" ;
            rdf:value """Made this property a subproperty of
               isCreationDateOfSomeMembersOf."""@en ;
        ] ,
        [
            dc:date "2023-10-13" ;
            rdf:value """Renamed the property in order to take the past members of the
               record set into account. Adjusted the annotations accordingly."""@en ;
        ] ,
        [
            dc:date "2023-09-22" ;
            rdf:value "Added in RiC-O 1.0."@en ;
        ] ,
        [
            dc:date "2023-11-27" ;
            rdf:value "Added a new rdfs:label in Spanish."@en ;
        ] ,
        [
            dc:date "2023-10-12" ;
            rdf:value "Added the French label"@en ;
        ] ;
    skos:scopeNote """To be used for specifying a bulk date, i.e. the predominant date
         of the members of the record set."""@en ;
    :RiCCMCorrespondingComponent """RiC-R083 ('is or was creation date of most members
         of' relation)"""@en ;
.

:isOrWasDescribedBy
    a owl:ObjectProperty ;
    rdfs:label
        "is or was described by"@en ,
        "es o fue descrito por"@es ,
        "est ou a été décrit par"@fr ;
    rdfs:comment """Inverse of 'describes or described' object
         property."""@en ;
    rdfs:domain :Thing ;
    rdfs:isDefinedBy <https://www.ica.org/standards/RiC/ontology> ;
    rdfs:range :RecordResource ;
    rdfs:subPropertyOf :isOrWasSubjectOf ;
    owl:inverseOf :describesOrDescribed ;
    skos:changeNote
        [
            dc:date "2023-08-28" ;
            rdf:value "Added a new rdfs:label in French."@en ;
        ] ,
        [
            dc:date "2023-08-28" ;
            rdf:value "Added a new rdfs:label in French."@en ;
        ] ,
        [
            dc:date "2021-01-22" ;
            rdf:value """changed the IRI, label, inverse property IRI, text definition,
               corresponding CM component name (changed made in order to make RiC-O compliant with
               RiC-CM 0.2; the name of this property in RiC-O 0.1 was "describedBy")."""@en ;
        ] ,
        [
            dc:date "2023-11-02" ;
            rdf:value "Added a new rdfs:label in Spanish."@en ;
        ] ;
    :RiCCMCorrespondingComponent """RiC-R021i ('is or was described by'
         relation)"""@en ;
.

:isOrWasDigitalInstantiationOf
    a owl:ObjectProperty ;
    rdfs:label
        "is or was digital instantiation of"@en ,
        "es o era instanciación digital de"@es ,
        "est ou a été une instanciation numérique de"@fr ;
    rdfs:comment """Inverse of 'has or had digital instantiation' object
         property."""@en ;
    rdfs:domain :Instantiation ;
    rdfs:isDefinedBy <https://www.ica.org/standards/RiC/ontology> ;
    rdfs:range :RecordResource ;
    rdfs:subPropertyOf :isOrWasInstantiationOf ;
    owl:inverseOf :hasOrHadDigitalInstantiation ;
    skos:changeNote
        [
            dc:date "2023-11-27" ;
            rdf:value "Added a new rdfs:label in Spanish."@en ;
        ] ,
        [
            dc:date "2023-08-29" ;
            rdf:value "Added the property."@en ;
        ] ;
.

:isOrWasDocumentaryFormTypeOfAllMembersOf
    a owl:ObjectProperty ;
    rdfs:label
        "is or was documentary form type of all members of"@en ,
        "es o era tipo documental de todos los miembros de"@es ,
        "est ou a été le type de document de tous les membres de"@fr ;
    rdfs:comment """Connects a Documentary Form Type and a Record Set whose all past
         or present Record or Record Part members have that Documentary Form Type."""@en ;
    rdfs:domain :DocumentaryFormType ;
    rdfs:isDefinedBy <https://www.ica.org/standards/RiC/ontology> ;
    rdfs:range :RecordSet ;
    rdfs:subPropertyOf :isOrWasCategoryOfAllMembersOf ;
    owl:inverseOf :hasOrHadAllMembersWithDocumentaryFormType ;
    skos:changeNote
        [
            dc:date "2023-11-02" ;
            rdf:value "Added a new rdfs:label in Spanish."@en ;
        ] ,
        [
            dc:date "2020-12-28" ;
            rdf:value """Object property added for handling the case where a Record Set
               is described as having all or some members that belong to some category (see RiC-CM
               0.2 attributes section, #4.4 on Record Set, Record and Record Part
               attributes)."""@en ;
        ] ,
        [
            dc:date "2023-08-28" ;
            rdf:value "Added a new rdfs:label in French."@en ;
        ] ;
.

:isOrWasDocumentaryFormTypeOfSomeMembersOf
    a owl:ObjectProperty ;
    rdfs:label
        "is or was documentary form type of some members of"@en ,
        "es o era tipo documental de algunos miembros de"@es ,
        "est ou a été le type de document de certains membres de"@fr ;
    rdfs:comment """Connects a Documentary Form Type and a Record Set whose some past
         or present Record or Record Part members have that Documentary Form Type."""@en ;
    rdfs:domain :DocumentaryFormType ;
    rdfs:isDefinedBy <https://www.ica.org/standards/RiC/ontology> ;
    rdfs:range :RecordSet ;
    rdfs:subPropertyOf :isOrWasCategoryOfSomeMembersOf ;
    owl:inverseOf :hasOrHadSomeMembersWithDocumentaryFormType ;
    skos:changeNote
        [
            dc:date "2023-08-28" ;
            rdf:value "Added a new rdfs:label in French."@en ;
        ] ,
        [
            dc:date "2020-12-28" ;
            rdf:value """Object property added for handling the case where a Record Set
               is described as having all or some members that belong to some category (see RiC-CM
               0.2 attributes section, #4.4 on Record Set, Record and Record Part
               attributes)."""@en ;
        ] ,
        [
            dc:date "2023-11-02" ;
            rdf:value "Added a new rdfs:label in Spanish."@en ;
        ] ;
.

:isOrWasEmployerOf
    a owl:ObjectProperty ;
    rdfs:label
        "is or was employer of"@en ,
        "es o era empleador(a) de"@es ,
        "a ou a été l'employeur de"@fr ;
    rdfs:comment """Connects a Corporate Body or a Person to a Person who is or was
         their employee."""@en ;
    rdfs:domain
        [
            a owl:Class ;
            owl:unionOf (
                :CorporateBody
                :Person
            ) ;
        ] ;
    rdfs:isDefinedBy <https://www.ica.org/standards/RiC/ontology> ;
    rdfs:range :Person ;
    rdfs:subPropertyOf :isOrWasControllerOf ;
    owl:inverseOf :hasOrHadEmployer ;
    skos:changeNote
        [
            dc:date "2023-11-27" ;
            rdf:value "Added a new rdfs:label in Spanish."@en ;
        ] ,
        [
            dc:date "2023-10-19" ;
            rdf:value "Adder for RiC-O v1.0."@en ;
        ] ,
        [
            dc:date "2023-10-26" ;
            rdf:value """Changed the domain and range of the property. Added a
               rdfs:comment. Removed the 'has or had member' super-property."""@en ;
        ] ;
.

:isOrWasEnforcedBy
    a owl:ObjectProperty ;
    rdfs:label
        "is or was enforced by"@en ,
        "es o era una regla aplicada por"@es ,
        "est ou a été fait appliquer par"@fr ;
    rdfs:comment """Connects a Rule to an Agent that enforces or enforced the
         Rule."""@en ;
    rdfs:domain :Rule ;
    rdfs:isDefinedBy <https://www.ica.org/standards/RiC/ontology> ;
    rdfs:range :Agent ;
    rdfs:subPropertyOf :isRuleAssociatedWith ;
    owl:inverseOf :isOrWasResponsibleForEnforcing ;
    skos:changeNote
        [
            dc:date "2023-08-28" ;
            rdf:value "Added a new rdfs:label in French."@en ;
        ] ,
        [
            dc:date "2021-01-22" ;
            rdf:value """changed the IRI, label, inverse property IRI, text definition,
               corresponding CM component name (changed made in order to make RiC-O compliant with
               RiC-CM 0.2; the name of this property in RiC-O 0.1 was "enforcedBy")."""@en ;
        ] ,
        [
            dc:date "2023-11-02" ;
            rdf:value "Added a new rdfs:label in Spanish."@en ;
        ] ;
    :RiCCMCorrespondingComponent """RiC-R066 ('is or was enforced by'
         relation)"""@en ;
.

:isOrWasExpressedBy
    a owl:ObjectProperty ;
    rdfs:label
        "is or was expressed by"@en ,
        "es o era una regla expresada en"@es ,
        "est ou a été exprimé par"@fr ;
    rdfs:comment """Connects a Rule to a Record Resource that expresses or expressed
         the Rule."""@en ;
    rdfs:domain :Rule ;
    rdfs:isDefinedBy <https://www.ica.org/standards/RiC/ontology> ;
    rdfs:range :RecordResource ;
    rdfs:subPropertyOf :isRuleAssociatedWith ;
    owl:inverseOf :expressesOrExpressed ;
    skos:changeNote
        [
            dc:date "2023-08-28" ;
            rdf:value "Added a new rdfs:label in French."@en ;
        ] ,
        [
            dc:date "2023-11-02" ;
            rdf:value "Added a new rdfs:label in Spanish."@en ;
        ] ,
        [
            dc:date "2021-01-22" ;
            rdf:value """changed the IRI, label, inverse property IRI, text definition,
               corresponding CM component name (changed made in order to make RiC-O compliant with
               RiC-CM 0.2; the name of this property in RiC-O 0.1 was "expressedBy")."""@en ;
        ] ;
    :RiCCMCorrespondingComponent """RiC-R064 ('is or was expressed by'
         relation)"""@en ;
.

:isOrWasHolderOf
    a owl:ObjectProperty ;
    rdfs:label
        "is or was holder of"@en ,
        "es o era conservador de"@es ,
        "détient ou a détenu"@fr ;
    rdfs:comment """Connects an Agent to a Record Resource or Instantiation that the
         Agent holds or held."""@en ;
    rdfs:domain :Agent ;
    rdfs:isDefinedBy <https://www.ica.org/standards/RiC/ontology> ;
    rdfs:range
        [
            a owl:Class ;
            owl:unionOf (
                :Instantiation
                :RecordResource
            ) ;
        ] ;
    rdfs:subPropertyOf :isOrWasManagerOf ;
    owl:inverseOf :hasOrHadHolder ;
    owl:propertyChainAxiom (
        :thingIsSourceOfRelation
        :recordResourceHoldingRelation_role
        :relationHasTarget
    ) ;
    skos:changeNote
        [
            dc:date "2023-11-08" ;
            rdf:value """In order to get a system of rolified Relation classes: modified
               the property chain axiom so that it now involves the new
               recordResourceHoldingRelation_role object property."""@en ;
        ] ,
        [
            dc:date "2023-11-02" ;
            rdf:value "Added a new rdfs:label in Spanish."@en ;
        ] ,
        [
            dc:date "2023-08-28" ;
            rdf:value "Added a new rdfs:label in French."@en ;
        ] ,
        [
            dc:date "2021-01-22" ;
            rdf:value """changed the IRI, label, inverse property IRI, super = property
               IRI and text definition (changed made in order to make RiC-O compliant with RiC-CM
               0.2; the name of this property in RiC-O 0.1 was "isHolderOf")."""@en ;
        ] ;
    :RiCCMCorrespondingComponent """RiC-R039 ('is or was holder of'
         relation)"""@en ;
.

:isOrWasHolderOfIntellectualPropertyRightsOf
    a owl:ObjectProperty ;
    rdfs:label
        "is or was holder of intellectual property rights of"@en ,
        """es o era conservador de derechos de propiedad intelectual
         de"""@es ,
        """détient ou a détenu les droits de propriété intellectuelle
         sur"""@fr ;
    rdfs:comment """Connects an Agent to a Record Resource or Instantiation on which
         the Agent has or had some intellectual property rights."""@en ;
    rdfs:domain
        [
            a owl:Class ;
            owl:unionOf (
                :Group
                :Person
                :Position
            ) ;
        ] ;
    rdfs:isDefinedBy <https://www.ica.org/standards/RiC/ontology> ;
    rdfs:range
        [
            a owl:Class ;
            owl:unionOf (
                :Instantiation
                :RecordResource
            ) ;
        ] ;
    rdfs:subPropertyOf :hasOrHadAuthorityOver ;
    owl:inverseOf :hasOrHadIntellectualPropertyRightsHolder ;
    owl:propertyChainAxiom (
        :thingIsSourceOfRelation
        :intellectualPropertyRightsRelation_role
        :relationHasTarget
    ) ;
    skos:changeNote
        [
            dc:date "2023-11-02" ;
            rdf:value "Added a new rdfs:label in Spanish."@en ;
        ] ,
        [
            dc:date "2023-08-28" ;
            rdf:value "Added a new rdfs:label in French."@en ;
        ] ,
        [
            dc:date "2023-11-08" ;
            rdf:value """In order to get a system of rolified Relation classes: modified
               the property chain axiom so that it now involves the new
               intellectualPropertyRightsRelation_role object property."""@en ;
        ] ,
        [
            dc:date "2021-01-22" ;
            rdf:value """changed the IRI, label, inverse property IRI and textual
               definition (changed made in order to make RiC-O compliant with RiC-CM 0.2; the name
               of this property in RiC-O 0.1 was "hasIntellectualPropertyRightsOn")."""@en ;
        ] ;
    :RiCCMCorrespondingComponent """RiC-R040 ('is or was holder of intellectual
         property rights of' relation)"""@en ;
.

:isOrWasIdentifierOf
    a owl:ObjectProperty ;
    rdfs:label
        "is or was identifier of"@en ,
        "es o era identificador de"@es ,
        "est ou a été l’identifiant de"@fr ;
    rdfs:comment """Connects an Identifier to a Thing that it identified or
         identifies."""@en ;
    rdfs:domain :Identifier ;
    rdfs:isDefinedBy <https://www.ica.org/standards/RiC/ontology> ;
    rdfs:range :Thing ;
    rdfs:subPropertyOf :isOrWasAppellationOf ;
    owl:inverseOf :hasOrHadIdentifier ;
    skos:changeNote
        [
            dc:date "2023-11-02" ;
            rdf:value "Added a new rdfs:label in Spanish."@en ;
        ] ,
        [
            dc:date "2023-08-28" ;
            rdf:value "Added a new rdfs:label in French."@en ;
        ] ,
        [
            dc:date "2021-01-22" ;
            rdf:value """changed the IRI, label, inverse property IRI, text definition,
               super property IRI (the name of this property in RiC-O 0.1 was
               "identifies")."""@en ;
        ] ;
.

:isOrWasJurisdictionOf
    a owl:ObjectProperty ;
    rdfs:label
        "is or was jurisdiction of"@en ,
        "es o era jurisdicción de"@es ,
        "a ou a été le ressort de"@fr ;
    rdfs:comment """Connects a Place to an Agent that has or had jurisdiction over the
         Place."""@en ;
    rdfs:domain :Place ;
    rdfs:isDefinedBy <https://www.ica.org/standards/RiC/ontology> ;
    rdfs:range :Agent ;
    rdfs:subPropertyOf :isPlaceAssociatedWithAgent ;
    owl:inverseOf :hasOrHadJurisdiction ;
    skos:changeNote
        [
            dc:date "2023-08-28" ;
            rdf:value "Added a new rdfs:label in French."@en ;
        ] ,
        [
            dc:date "2021-01-22" ;
            rdf:value """changed the IRI, label, inverse property IRI, textual
               definition (changed made in order to make RiC-O compliant with RiC-CM 0.2; the name
               of this property in RiC-O 0.1 was "isJurisdictionOf")."""@en ;
        ] ,
        [
            dc:date "2021-01-22" ;
            rdf:value """changed the IRI, label, inverse property IRI, textual
               definition (changed made in order to make RiC-O compliant with RiC-CM 0.2; the name
               of this property in RiC-O 0.1 was "isJurisdictionOf")."""@en ;
        ] ,
        [
            dc:date "2023-11-02" ;
            rdf:value "Added a new rdfs:label in Spanish."@en ;
        ] ,
        [
            dc:date "2023-10-19" ;
            rdf:value """Made subproperty of new property isPlaceAssociatedWithAgent
               instead of its parent isPlaceAssociatedWith."""@en ;
        ] ;
    :RiCCMCorrespondingComponent """RiC-R076 ('is or was jurisdiction of'
         relation)"""@en ;
.

:isOrWasLanguageOf
    a owl:ObjectProperty ;
    rdfs:label
        "is or was language of"@en ,
        "es o era lengua de"@es ,
        "est ou a été la langue de"@fr ;
    rdfs:comment """Connects a Language to an Agent, Record or Record Part that uses
         or used it."""@en ;
    rdfs:domain :Language ;
    rdfs:isDefinedBy <https://www.ica.org/standards/RiC/ontology> ;
    rdfs:range
        [
            a owl:Class ;
            owl:unionOf (
                :Agent
                :Record
                :RecordPart
            ) ;
        ] ;
    rdfs:subPropertyOf :isRelatedTo ;
    owl:inverseOf :hasOrHadLanguage ;
    skos:changeNote
        [
            dc:date "2023-11-02" ;
            rdf:value "Added a new rdfs:label in Spanish."@en ;
        ] ,
        [
            dc:date "2021-01-22" ;
            rdf:value """changed the IRI, label, inverse property IRI, textual
               definition (the name of this property in RiC-O 0.1 was "isLanguageOf")."""@en ;
        ] ,
        [
            dc:date "2023-08-28" ;
            rdf:value "Added a new rdfs:label in French."@en ;
        ] ;
.

:isOrWasLanguageOfAllMembersOf
    a owl:ObjectProperty ;
    rdfs:label
        "is or was language of all members of"@en ,
        "es o era lengua de todos los miembros de"@es ,
        "est ou a été la langue de tous les membres de"@fr ;
    rdfs:comment """Connects a Language and a Record Set whose all present or past
         Record or Record Part members use that Language."""@en ;
    rdfs:domain :Language ;
    rdfs:isDefinedBy <https://www.ica.org/standards/RiC/ontology> ;
    rdfs:range :RecordSet ;
    rdfs:subPropertyOf :isRelatedTo ;
    owl:inverseOf :hasOrHadAllMembersWithLanguage ;
    skos:changeNote
        [
            dc:date "2020-12-28" ;
            rdf:value """Object property added for handling the case where a Record Set
               is described as having all or some members that belong to some category (see RiC-CM
               0.2 attributes section, #4.4 on Record Set, Record and Record Part
               attributes)."""@en ;
        ] ,
        [
            dc:date "2023-08-28" ;
            rdf:value "Added a new rdfs:label in French."@en ;
        ] ,
        [
            dc:date "2023-11-02" ;
            rdf:value "Added a new rdfs:label in Spanish."@en ;
        ] ;
.

:isOrWasLanguageOfSomeMembersOf
    a owl:ObjectProperty ;
    rdfs:label
        "is or was language of some members of"@en ,
        "es o era lengua de algunos miembros de"@es ,
        "est ou a été la langue de certains membres de"@fr ;
    rdfs:comment """Connects a Language and a Record Set whose some present or past
         Record or Record Part members use that Language."""@en ;
    rdfs:domain :Language ;
    rdfs:isDefinedBy <https://www.ica.org/standards/RiC/ontology> ;
    rdfs:range :RecordSet ;
    rdfs:subPropertyOf :isRelatedTo ;
    owl:inverseOf :hasOrHadSomeMembersWithLanguage ;
    skos:changeNote
        [
            dc:date "2023-08-28" ;
            rdf:value "Added a new rdfs:label in French."@en ;
        ] ,
        [
            dc:date "2023-11-02" ;
            rdf:value "Added a new rdfs:label in Spanish."@en ;
        ] ,
        [
            dc:date "2020-12-28" ;
            rdf:value """Object property added for handling the case where a Record Set
               is described as having all or some members that belong to some category (see RiC-CM
               0.2 attributes section, #4.4 on Record Set, Record and Record Part
               attributes)."""@en ;
        ] ;
.

:isOrWasLeaderOf
    a owl:ObjectProperty ;
    rdfs:label
        "is or was leader of"@en ,
        "es o era líder de"@es ,
        "est ou a été le dirigeant de"@fr ;
    rdfs:comment """Connects a Person to the Group that Person leads or led in the
         past."""@en ;
    rdfs:domain :Person ;
    rdfs:isDefinedBy <https://www.ica.org/standards/RiC/ontology> ;
    rdfs:range :Group ;
    rdfs:subPropertyOf :isOrWasControllerOf ;
    owl:inverseOf :hasOrHadLeader ;
    owl:propertyChainAxiom (
        :thingIsSourceOfRelation
        :leadershipRelation_role
        :relationHasTarget
    ) ;
    skos:changeNote
        [
            dc:date "2023-08-28" ;
            rdf:value "Added a new rdfs:label in French."@en ;
        ] ,
        [
            dc:date "2021-01-22" ;
            rdf:value """changed the IRI, label, inverse property IRI, super property
               IRI, textual definition (changed made in order to make RiC-O compliant with RiC-CM
               0.2; the name of this property in RiC-O 0.1 was "isLeaderOf")."""@en ;
        ] ,
        [
            dc:date "2023-11-08" ;
            rdf:value """In order to get a system of rolified Relation classes: modified
               the property chain axiom so that it now involves the new leadershipRelation_role
               object property."""@en ;
        ] ,
        [
            dc:date "2023-11-02" ;
            rdf:value "Added a new rdfs:label in Spanish."@en ;
        ] ;
    :RiCCMCorrespondingComponent """RiC-R042 ('is or was leader of'
         relation)"""@en ;
.

:isOrWasLegalStatusOf
    a owl:ObjectProperty ;
    rdfs:label
        "is or was legal status of"@en ,
        "es o era status jurídico de"@es ,
        "est ou a été le statut légal de"@fr ;
    rdfs:comment """Connects a Legal Status to an Agent or Record Resource that it
         categorizes."""@en ;
    rdfs:domain :LegalStatus ;
    rdfs:isDefinedBy <https://www.ica.org/standards/RiC/ontology> ;
    rdfs:range
        [
            a owl:Class ;
            owl:unionOf (
                :Agent
                :Record
                :RecordPart
            ) ;
        ] ;
    rdfs:subPropertyOf :isOrWasCategoryOf ;
    owl:inverseOf :hasOrHadLegalStatus ;
    skos:changeNote
        [
            dc:date "2021-01-22" ;
            rdf:value """changed the IRI, label, inverse property IRI, textual
               definition (the name of this property in RiC-O 0.1 was
               "isLegalStatusOf")."""@en ;
        ] ,
        [
            dc:date "2023-08-28" ;
            rdf:value "Added a new rdfs:label in French."@en ;
        ] ,
        [
            dc:date "2023-11-02" ;
            rdf:value "Added a new rdfs:label in Spanish."@en ;
        ] ;
    skos:scopeNote """Connects a Legal Status to an Agent, Record or Record Part that
         it categorized or categorizes."""@en ;
.

:isOrWasLegalStatusOfAllMembersOf
    a owl:ObjectProperty ;
    rdfs:label
        "is or was legal status of all members of"@en ,
        "es o era status jurídico de todos los miembros de"@es ,
        "est ou a été le statut légal de tous les membres de"@fr ;
    rdfs:comment """Connects a Legal Status and a Record Set whose all past or present
         Record or Record Part members have that Legal Status."""@en ;
    rdfs:domain :LegalStatus ;
    rdfs:isDefinedBy <https://www.ica.org/standards/RiC/ontology> ;
    rdfs:range :RecordSet ;
    rdfs:subPropertyOf :isOrWasCategoryOfAllMembersOf ;
    owl:inverseOf :hasOrHadAllMembersWithLegalStatus ;
    skos:changeNote
        [
            dc:date "2023-11-02" ;
            rdf:value "Added a new rdfs:label in Spanish."@en ;
        ] ,
        [
            dc:date "2020-12-28" ;
            rdf:value """Object property added for handling the case where a Record Set
               is described as having all or some members that belong to some category (see RiC-CM
               0.2 attributes section, #4.4 on Record Set, Record and Record Part
               attributes)."""@en ;
        ] ,
        [
            dc:date "2023-08-28" ;
            rdf:value "Added a new rdfs:label in French."@en ;
        ] ;
.

:isOrWasLegalStatusOfSomeMembersOf
    a owl:ObjectProperty ;
    rdfs:label
        "is or was legal status of some members of"@en ,
        "es o era status jurídico de algunos miembros de"@es ,
        "est ou a été le statut légal de certains membres de"@fr ;
    rdfs:comment """Connects a Legal Status and a Record Set whose some past or
         present Record or Record Part members have that Legal Status."""@en ;
    rdfs:domain :LegalStatus ;
    rdfs:isDefinedBy <https://www.ica.org/standards/RiC/ontology> ;
    rdfs:range :RecordSet ;
    rdfs:subPropertyOf :isOrWasCategoryOfSomeMembersOf ;
    owl:inverseOf :hasOrHadSomeMembersWithLegalStatus ;
    skos:changeNote
        [
            dc:date "2023-08-28" ;
            rdf:value "Added a new rdfs:label in French."@en ;
        ] ,
        [
            dc:date "2020-12-28" ;
            rdf:value """Object property added for handling the case where a Record Set
               is described as having all or some members that belong to some category (see RiC-CM
               0.2 attributes section, #4.4 on Record Set, Record and Record Part
               attributes)."""@en ;
        ] ,
        [
            dc:date "2023-11-02" ;
            rdf:value "Added a new rdfs:label in Spanish."@en ;
        ] ;
.

:isOrWasLocationOfAgent
    a owl:ObjectProperty ;
    rdfs:label
        "is or was location of agent"@en ,
        "es o era localización de agente"@es ,
        "est ou a été la localisation de l'agent"@fr ;
    rdfs:comment """Connects a Place to an Agent that is or was located in this
         Place."""@en ;
    rdfs:domain :Place ;
    rdfs:isDefinedBy <https://www.ica.org/standards/RiC/ontology> ;
    rdfs:range :Agent ;
    rdfs:subPropertyOf
        :isOrWasLocationOf ,
        :isPlaceAssociatedWithAgent ;
    owl:inverseOf :agentHasOrHadLocation ;
    skos:changeNote
        [
            dc:date "2023-10-20" ;
            rdf:value "Added for RiC-O 1.0."@en ;
        ] ,
        [
            dc:date "2023-11-27" ;
            rdf:value "Added a new rdfs:label in Spanish."@en ;
        ] ,
        [
            dc:date "2023-10-26" ;
            rdf:value "Renamed the property and added an rdfs:comment."@en ;
        ] ;
.

:isOrWasMainSubjectOf
    a owl:ObjectProperty ;
    rdfs:label
        "is or was main subject of"@en ,
        "es o era la materia principal de"@es ,
        "est ou a été le sujet principal de"@fr ;
    rdfs:comment """Inverse of 'has or had main subject' object
         property."""@en ;
    rdfs:domain :Thing ;
    rdfs:isDefinedBy <https://www.ica.org/standards/RiC/ontology> ;
    rdfs:range :RecordResource ;
    rdfs:subPropertyOf :isOrWasSubjectOf ;
    owl:inverseOf :hasOrHadMainSubject ;
    skos:changeNote
        [
            dc:date "2023-08-28" ;
            rdf:value "Added a new rdfs:label in French."@en ;
        ] ,
        [
            dc:date "2021-01-22" ;
            rdf:value """changed the IRI, label, inverse property IRI, super property
               IRI, textual definition (changed made in order to make RiC-O compliant with RiC-CM
               0.2; the name of this property in RiC-O 0.1 was "isMainSubjectOf")."""@en ;
        ] ,
        [
            dc:date "2023-11-02" ;
            rdf:value "Added a new rdfs:label in Spanish."@en ;
        ] ;
    :RiCCMCorrespondingComponent """RiC-R020i ('is or was main subject of'
         relation)"""@en ;
.

:isOrWasMandateTypeOf
    a owl:ObjectProperty ;
    rdfs:label
        "is or was mandate type of"@en ,
        "es o era tipo de norma de"@es ,
        "est ou a été le type de mandat de"@fr ;
    rdfs:comment """Connects a Mandate Type to a Mandate that it categorized or
         categorizes."""@en ;
    rdfs:domain :MandateType ;
    rdfs:isDefinedBy <https://www.ica.org/standards/RiC/ontology> ;
    rdfs:range :Mandate ;
    rdfs:subPropertyOf :isOrWasRuleTypeOf ;
    owl:inverseOf :hasOrHadMandateType ;
    skos:changeNote
        [
            dc:date "2023-11-13" ;
            rdf:value """Added the property, and its inverse one, following the creation
               of the MandateType class, that corresponds to the new Mandate Type attribute in
               RiC-CM 1.0."""@en ;
        ] ,
        [
            dc:date "2024-03-15" ;
            rdf:value "Make capitalisation of rdfs:comment consistent."@en ;
        ] ;
.

:isOrWasMemberOf
    a owl:ObjectProperty ;
    rdfs:label
        "is or was member of"@en ,
        "es o era miembro de"@es ,
        "est ou a été membre de"@fr ;
    rdfs:comment "Inverse of 'has or had member' object property."@en ;
    rdfs:domain :Person ;
    rdfs:isDefinedBy <https://www.ica.org/standards/RiC/ontology> ;
    rdfs:range :Group ;
    rdfs:subPropertyOf :isAgentAssociatedWithAgent ;
    owl:inverseOf :hasOrHadMember ;
    owl:propertyChainAxiom (
        :thingIsTargetOfRelation
        :membershipRelation_role
        :relationHasSource
    ) ;
    skos:changeNote
        [
            dc:date "2021-01-22" ;
            rdf:value """changed the IRI, label, inverse property IRI, textual
               definition (changed made in order to make RiC-O compliant with RiC-CM 0.2; the name
               of this property in RiC-O 0.1 was "isMemberOf")."""@en ;
        ] ,
        [
            dc:date "2023-08-28" ;
            rdf:value "Added a new rdfs:label in French."@en ;
        ] ,
        [
            dc:date "2023-11-08" ;
            rdf:value """In order to get a system of rolified Relation classes: modified
               the property chain axiom so that it now involves the new membershipRelation_role
               object property."""@en ;
        ] ,
        [
            dc:date "2023-11-02" ;
            rdf:value "Added a new rdfs:label in Spanish."@en ;
        ] ;
    :RiCCMCorrespondingComponent """RiC-R055i ('is or was member of'
         relation)"""@en ;
.

:isOrWasOccupationTypeOf
    a owl:ObjectProperty ;
    rdfs:label
        "is or was occupation type of"@en ,
        "es o era tipo de ocupación de"@es ,
        "est ou a été le type d’occupation de"@fr ;
    rdfs:comment """Connects an Occupation Type to a Person whose occupation is or was
         categorized by it."""@en ;
    rdfs:domain :OccupationType ;
    rdfs:isDefinedBy <https://www.ica.org/standards/RiC/ontology> ;
    rdfs:range :Person ;
    rdfs:subPropertyOf :isOrWasDemographicGroupOf ;
    owl:inverseOf :hasOrHadOccupationOfType ;
    skos:changeNote
        [
            dc:date "2023-11-02" ;
            rdf:value "Added a new rdfs:label in Spanish."@en ;
        ] ,
        [
            dc:date "2023-08-28" ;
            rdf:value "Added a new rdfs:label in French."@en ;
        ] ,
        [
            dc:date "2021-01-22" ;
            rdf:value """changed the IRI, label, inverse property IRI, textual
               definition, super property IRI (the name of this property in RiC-O 0.1 was
               "isOccupationTypeOf")."""@en ;
        ] ;
.

:isOrWasOccupiedBy
    a owl:ObjectProperty ;
    rdfs:label
        "is or was occupied by"@en ,
        "está o estaba ocupado por"@es ,
        "est ou a été occupé par"@fr ;
    rdfs:comment "Inverse of 'occupies or occupied' object property."@en ;
    rdfs:domain :Position ;
    rdfs:isDefinedBy <https://www.ica.org/standards/RiC/ontology> ;
    rdfs:range :Person ;
    rdfs:subPropertyOf :isAgentAssociatedWithAgent ;
    owl:inverseOf :occupiesOrOccupied ;
    owl:propertyChainAxiom (
        :thingIsTargetOfRelation
        :positionHoldingRelation_role
        :relationHasSource
    ) ;
    skos:changeNote
        [
            dc:date "2023-08-28" ;
            rdf:value "Added a new rdfs:label in French."@en ;
        ] ,
        [
            dc:date "2021-01-22" ;
            rdf:value """changed the IRI, label, inverse property IRI, text definition
               (changed made in order to make RiC-O compliant with RiC-CM 0.2; the name of this
               property in RiC-O 0.1 was "occupiedBy")."""@en ;
        ] ,
        [
            dc:date "2023-11-02" ;
            rdf:value "Added a new rdfs:label in Spanish."@en ;
        ] ,
        [
            dc:date "2023-11-08" ;
            rdf:value """In order to get a system of rolified Relation classes: modified
               the property chain axiom so that it now involves the new positionHoldingRelation_role
               object property."""@en ;
        ] ;
    :RiCCMCorrespondingComponent """RiC-R054i ('is or was occupied by'
         relation)"""@en ;
.

:isOrWasOwnerOf
    a owl:ObjectProperty ;
    rdfs:label
        "is or was owner of"@en ,
        "es o era poseedor(a) de"@es ,
        "est ou a été propriétaire de"@fr ;
    rdfs:comment """Connects a Group, Person or Position to a Thing that this Agent
         owns or owned."""@en ;
    rdfs:domain
        [
            a owl:Class ;
            owl:unionOf (
                :Group
                :Person
                :Position
            ) ;
        ] ;
    rdfs:isDefinedBy <https://www.ica.org/standards/RiC/ontology> ;
    rdfs:range :Thing ;
    rdfs:subPropertyOf :hasOrHadAuthorityOver ;
    owl:inverseOf :hasOrHadOwner ;
    owl:propertyChainAxiom (
        :thingIsSourceOfRelation
        :ownershipRelation_role
        :relationHasTarget
    ) ;
    skos:changeNote
        [
            dc:date "2023-11-02" ;
            rdf:value "Added a new rdfs:label in Spanish."@en ;
        ] ,
        [
            dc:date "2023-08-28" ;
            rdf:value "Added a new rdfs:label in French."@en ;
        ] ,
        [
            dc:date "2023-11-08" ;
            rdf:value """In order to get a system of rolified Relation classes: modified
               the property chain axiom so that it now involves the new ownershipRelation_role
               object property."""@en ;
        ] ,
        [
            dc:date "2021-01-22" ;
            rdf:value """changed the IRI, label, inverse property IRI, textual
               definition, super property IRI (changed made in order to make RiC-O compliant with
               RiC-CM 0.2; the name of this property in RiC-O 0.1 was "isOwnerOf")."""@en ;
        ] ;
    :RiCCMCorrespondingComponent """RiC-R037 ('is or was owner of'
         relation)"""@en ;
.

:isOrWasPerformedBy
    a owl:ObjectProperty ;
    rdfs:label
        "is or was performed by"@en ,
        "es o fue desarrollado por"@es ,
        "est ou a été réalisée par"@fr ;
    rdfs:comment """Connects an Activity to an Agent that performed or performs the
         Activity."""@en ;
    rdfs:domain :Activity ;
    rdfs:isDefinedBy <https://www.ica.org/standards/RiC/ontology> ;
    rdfs:range :Agent ;
    rdfs:subPropertyOf :hasOrHadParticipant ;
    owl:inverseOf :performsOrPerformed ;
    owl:propertyChainAxiom (
        :thingIsSourceOfRelation
        :performanceRelation_role
        :relationHasTarget
    ) ;
    skos:changeNote
        [
            dc:date "2021-01-22" ;
            rdf:value """changed the IRI, label, inverse property IRI, text definition,
               super property IRI (changed made in order to make RiC-O compliant with RiC-CM 0.2;
               the name of this property in RiC-O 0.1 was "performedBy")."""@en ;
        ] ,
        [
            dc:date "2023-11-02" ;
            rdf:value "Added a new rdfs:label in Spanish."@en ;
        ] ,
        [
            dc:date "2023-11-08" ;
            rdf:value """In order to get a system of rolified Relation classes: modified
               the property chain axiom so that it now involves the new performanceRelation_role
               object property."""@en ;
        ] ,
        [
            dc:date "2023-08-28" ;
            rdf:value "Added a new rdfs:label in French."@en ;
        ] ;
    :RiCCMCorrespondingComponent """RiC-R060 ('is or was performed by'
         relation)"""@en ;
.

:isOrWasPhysicalLocationOf
    a owl:ObjectProperty ;
    rdfs:label
        "is or was physical location of"@en ,
        "es o era localización física de"@es ,
        "a ou a été la localisation physique de"@fr ;
    rdfs:comment """Connects a Physical Location to a Place, when it is or was its
         location."""@en ;
    rdfs:domain :PhysicalLocation ;
    rdfs:isDefinedBy <https://www.ica.org/standards/RiC/ontology> ;
    rdfs:range :Place ;
    rdfs:subPropertyOf :isAssociatedWithPlace ;
    owl:inverseOf :hasOrHadPhysicalLocation ;
    skos:changeNote
        [
            dc:date "2023-11-02" ;
            rdf:value "Added a new rdfs:label in Spanish."@en ;
        ] ,
        [
            dc:date "2021-01-22" ;
            rdf:value """changed the IRI, label, inverse property IRI, textual
               definition (the name of this property in RiC-O 0.1 was
               "isPhysicalLocationOf")."""@en ;
        ] ,
        [
            dc:date "2021-02-01" ;
            rdf:value """Property made a subproperty of
               'isAssociatedWithPlace"."""@en ;
        ] ,
        [
            dc:date "2023-08-28" ;
            rdf:value "Added a new rdfs:label in French."@en ;
        ] ;
.

:isOrWasPlaceNameOf
    a owl:ObjectProperty ;
    rdfs:label
        "is or was place name of"@en ,
        "es o era nombre de lugar de"@es ,
        "a ou a été le nom de lieu de"@fr ;
    rdfs:comment """Connects a Place Name to a Place that was or is designated by
         it."""@en ;
    rdfs:domain :PlaceName ;
    rdfs:isDefinedBy <https://www.ica.org/standards/RiC/ontology> ;
    rdfs:range :Place ;
    rdfs:subPropertyOf :isOrWasNameOf ;
    owl:inverseOf :hasOrHadPlaceName ;
    skos:changeNote
        [
            dc:date "2023-11-02" ;
            rdf:value "Added a new rdfs:label in Spanish."@en ;
        ] ,
        [
            dc:date "2023-08-28" ;
            rdf:value "Added a new rdfs:label in French."@en ;
        ] ,
        [
            dc:date "2021-01-22" ;
            rdf:value """changed the IRI, label, inverse property IRI, text definition,
               super property IRI (the name of this property in RiC-O 0.1 was
               "isPlaceNameOf")."""@en ;
        ] ;
.

:isOrWasPlaceTypeOf
    a owl:ObjectProperty ;
    rdfs:label
        "is or was place type of"@en ,
        "es o era tipo de lugar de"@es ,
        "a ou a été le type de lieu de"@fr ;
    rdfs:comment """Connects a Place Type to a Place that is or was categorized by
         it."""@en ;
    rdfs:domain :PlaceType ;
    rdfs:isDefinedBy <https://www.ica.org/standards/RiC/ontology> ;
    rdfs:range :Place ;
    rdfs:subPropertyOf :isOrWasCategoryOf ;
    owl:inverseOf :hasOrHadPlaceType ;
    skos:changeNote
        [
            dc:date "2023-11-02" ;
            rdf:value "Added a new rdfs:label in Spanish."@en ;
        ] ,
        [
            dc:date "2023-08-28" ;
            rdf:value "Added a new rdfs:label in French."@en ;
        ] ,
        [
            dc:date "2021-01-22" ;
            rdf:value """changed the IRI, label, inverse property IRI, text definition,
               super property IRI (the name of this property in RiC-O 0.1 was
               "isPlaceTypeOf")."""@en ;
        ] ;
.

:isOrWasRecordStateOfAllMembersOf
    a owl:ObjectProperty ;
    rdfs:label
        "is or was record state of all members of"@en ,
        "es o era estado de documento de todos los miembros de"@es ,
        "a ou a été l’état de tous les membres de"@fr ;
    rdfs:comment """Connects a Record State and a Record Set whose all past or present
         Record or Record Part members have that Record State."""@en ;
    rdfs:domain :RecordState ;
    rdfs:isDefinedBy <https://www.ica.org/standards/RiC/ontology> ;
    rdfs:range :RecordSet ;
    rdfs:subPropertyOf :isOrWasCategoryOfAllMembersOf ;
    owl:inverseOf :hasOrHadAllMembersWithRecordState ;
    skos:changeNote
        [
            dc:date "2020-12-28" ;
            rdf:value """Object property added for handling the case where a Record Set
               is described as having all or some members that belong to some category (see RiC-CM
               0.2 attributes section, #4.4 on Record Set, Record and Record Part
               attributes)."""@en ;
        ] ,
        [
            dc:date "2023-11-02" ;
            rdf:value "Added a new rdfs:label in Spanish."@en ;
        ] ,
        [
            dc:date "2023-08-28" ;
            rdf:value "Added a new rdfs:label in French."@en ;
        ] ;
.

:isOrWasRecordStateOfSomeMembersOf
    a owl:ObjectProperty ;
    rdfs:label
        "is or was record state of some members of"@en ,
        "es o era estado de documento de algunos miembros de"@es ,
        "a ou a été l’état de certains membres de"@fr ;
    rdfs:comment """Connects a Record State and a Record Set whose some past or
         present Record or Record Part members have that Record State."""@en ;
    rdfs:domain :RecordState ;
    rdfs:isDefinedBy <https://www.ica.org/standards/RiC/ontology> ;
    rdfs:range :RecordSet ;
    rdfs:subPropertyOf :isOrWasCategoryOfSomeMembersOf ;
    owl:inverseOf :hasOrHadSomeMembersWithRecordState ;
    skos:changeNote
        [
            dc:date "2023-08-28" ;
            rdf:value "Added a new rdfs:label in French."@en ;
        ] ,
        [
            dc:date "2023-11-02" ;
            rdf:value "Added a new rdfs:label in Spanish."@en ;
        ] ,
        [
            dc:date "2020-12-28" ;
            rdf:value """Object property added for handling the case where a Record Set
               is described as having all or some members that belong to some category (see RiC-CM
               0.2 attributes section, #4.4 on Record Set, Record and Record Part
               attributes)."""@en ;
        ] ;
.

:isOrWasRegulatedBy
    a owl:ObjectProperty ;
    rdfs:label
        "is or was regulated by"@en ,
        "está o estaba regulado por"@es ,
        "est ou a été régulé par"@fr ;
    rdfs:comment """Inverse of the 'regulates or regulated' object
         property."""@en ;
    rdfs:domain :Thing ;
    rdfs:isDefinedBy <https://www.ica.org/standards/RiC/ontology> ;
    rdfs:range :Rule ;
    rdfs:subPropertyOf :isAssociatedWithRule ;
    owl:inverseOf :regulatesOrRegulated ;
    skos:changeNote
        [
            dc:date "2021-01-22" ;
            rdf:value """changed the IRI, label, inverse property IRI (changed made in
               order to make RiC-O compliant with RiC-CM 0.2; the name of this property in RiC-O 0.1
               was "regulatedBy")."""@en ;
        ] ,
        [
            dc:date "2023-11-02" ;
            rdf:value "Added a new rdfs:label in Spanish."@en ;
        ] ,
        [
            dc:date "2023-08-28" ;
            rdf:value "Added a new rdfs:label in French."@en ;
        ] ;
    :RiCCMCorrespondingComponent """RiC-R063i ('is or was regulated by'
         relation)"""@en ;
.

:isOrWasResponsibleForEnforcing
    a owl:ObjectProperty ;
    rdfs:label
        "is or was responsible for enforcing"@en ,
        "es o era responsable de aplicar"@es ,
        "a fait ou fait appliquer"@fr ;
    rdfs:comment "Inverse of 'is or was enforced by' object property."@en ;
    rdfs:domain :Agent ;
    rdfs:isDefinedBy <https://www.ica.org/standards/RiC/ontology> ;
    rdfs:range :Rule ;
    rdfs:subPropertyOf :isAssociatedWithRule ;
    owl:inverseOf :isOrWasEnforcedBy ;
    skos:changeNote
        [
            dc:date "2021-01-22" ;
            rdf:value """changed the IRI, label, inverse property IRI, text definition,
               corresponding CM component name (changed made in order to make RiC-O compliant with
               RiC-CM 0.2; the name of this property in RiC-O 0.1 was
               "isResponsibleForEnforcing")."""@en ;
        ] ,
        [
            dc:date "2023-08-28" ;
            rdf:value "Added a new rdfs:label in French."@en ;
        ] ,
        [
            dc:date "2023-11-02" ;
            rdf:value "Added a new rdfs:label in Spanish."@en ;
        ] ;
    :RiCCMCorrespondingComponent """RiC-R066i ('is or was responsible for enforcing'
         relation)"""@en ;
.

:isOrWasTitleOf
    a owl:ObjectProperty ;
    rdfs:label
        "is or was title of"@en ,
        "es o era título de"@es ,
        "est ou a été l’intitulé de"@fr ;
    rdfs:comment """Connects a Title to a Record Resource, Instantiation or Rule that
         it designated or designates."""@en ;
    rdfs:domain :Title ;
    rdfs:isDefinedBy <https://www.ica.org/standards/RiC/ontology> ;
    rdfs:range
        [
            a owl:Class ;
            owl:unionOf (
                :Instantiation
                :RecordResource
                :Rule
            ) ;
        ] ;
    rdfs:subPropertyOf :isOrWasNameOf ;
    owl:inverseOf :hasOrHadTitle ;
    skos:changeNote
        [
            dc:date "2021-01-22" ;
            rdf:value """changed the IRI, label, inverse property IRI, text definition,
               super property IRI (the name of this property in RiC-O 0.1 was
               "isTitleOf")."""@en ;
        ] ,
        [
            dc:date "2023-08-28" ;
            rdf:value "Added a new rdfs:label in French."@en ;
        ] ,
        [
            dc:date "2023-11-02" ;
            rdf:value "Added a new rdfs:label in Spanish."@en ;
        ] ;
.

:isOriginalOf
    a owl:ObjectProperty ;
    rdfs:label
        "is original of"@en ,
        "es original de"@es ,
        "est l’original de"@fr ;
    rdfs:comment """Connects the original version of a Record to a copy or a later
         version."""@en ;
    rdfs:domain
        [
            a owl:Class ;
            owl:unionOf (
                :Record
                :RecordPart
            ) ;
        ] ;
    rdfs:isDefinedBy <https://www.ica.org/standards/RiC/ontology> ;
    rdfs:range
        [
            a owl:Class ;
            owl:unionOf (
                :Record
                :RecordPart
            ) ;
        ] ;
    rdfs:subPropertyOf
        :hasGeneticLinkToRecordResource ,
        :precedesInTime ;
    owl:inverseOf :hasOriginal ;
    skos:changeNote
        [
            dc:date "2023-11-02" ;
            rdf:value "Added a new rdfs:label in Spanish."@en ;
        ] ,
        [
            dc:date "2023-08-28" ;
            rdf:value "Added a new rdfs:label in French."@en ;
        ] ;
    skos:scopeNote """There may be zero to many intermediate Records, ignored or
         unknown, between the two connected Records"""@en ;
    :RiCCMCorrespondingComponent """RiC-R010 (is original of
         relation)"""@en ;
.

:isProductionTechniqueTypeOf
    a owl:ObjectProperty ;
    rdfs:label
        "is production technique type of"@en ,
        "es tipo de técnica de producción de"@es ,
        "est le type de technique de production de"@fr ;
    rdfs:comment """Connects a Production Technique Type to an Instantiation whose
         production technique is categorized by it."""@en ;
    rdfs:domain :ProductionTechniqueType ;
    rdfs:isDefinedBy <https://www.ica.org/standards/RiC/ontology> ;
    rdfs:range :Instantiation ;
    rdfs:subPropertyOf :isOrWasCategoryOf ;
    owl:inverseOf :hasProductionTechniqueType ;
    skos:changeNote
        [
            dc:date "2021-01-22" ;
            rdf:value "changed the super property IRI."@en ;
        ] ,
        [
            dc:date "2023-08-28" ;
            rdf:value "Added a new rdfs:label in French."@en ;
        ] ,
        [
            dc:date "2023-11-02" ;
            rdf:value "Added a new rdfs:label in Spanish."@en ;
        ] ;
.

:isPublicationDateOf
    a owl:ObjectProperty ;
    rdfs:label
        "is publication date of"@en ,
        "es fecha de publicación de"@es ,
        "est la date de publication de"@fr ;
    rdfs:comment """Connects a Date to a Record Resource that was made public at this
         Date."""@en ;
    rdfs:domain :Date ;
    rdfs:isDefinedBy <https://www.ica.org/standards/RiC/ontology> ;
    rdfs:range :RecordResource ;
    rdfs:subPropertyOf :isBeginningDateOf ;
    owl:inverseOf :hasPublicationDate ;
    skos:changeNote
        [
            dc:date "2023-10-12" ;
            rdf:value "Added the French label"@en ;
        ] ,
        [
            dc:date "2023-09-22" ;
            rdf:value "Added in RiC-O 1.0."@en ;
        ] ,
        [
            dc:date "2023-11-27" ;
            rdf:value "Added a new rdfs:label in Spanish."@en ;
        ] ;
.

:isPublisherOf
    a owl:ObjectProperty ;
    rdfs:label
        "is publisher of"@en ,
        "es editor(a) de"@es ,
        "est l’éditeur de"@fr ;
    rdfs:comment """Connects an Agent to a Record Resource that it
         published."""@en ;
    rdfs:domain :Agent ;
    rdfs:isDefinedBy <https://www.ica.org/standards/RiC/ontology> ;
    rdfs:range :RecordResource ;
    rdfs:subPropertyOf :isRelatedTo ;
    owl:inverseOf :hasPublisher ;
    skos:changeNote
        [
            dc:date "2023-08-28" ;
            rdf:value "Added a new rdfs:label in French."@en ;
        ] ,
        [
            dc:date "2021-01-22" ;
            rdf:value """changed the IRI, label, inverse property IRI (the name of this
               property in RiC-O 0.1 was "publishes")."""@en ;
        ] ,
        [
            dc:date "2023-11-02" ;
            rdf:value "Added a new rdfs:label in Spanish."@en ;
        ] ;
.

:isReceiverOf
    a owl:ObjectProperty ;
    rdfs:label
        "is receiver of"@en ,
        "es receptor(a) de"@es ,
        "reçoit"@fr ;
    rdfs:comment "Inverse of 'received by' object property."@en ;
    rdfs:domain :Agent ;
    rdfs:isDefinedBy <https://www.ica.org/standards/RiC/ontology> ;
    rdfs:range
        [
            a owl:Class ;
            owl:unionOf (
                :Instantiation
                :RecordResource
            ) ;
        ] ;
    rdfs:subPropertyOf :isAccumulatorOf ;
    owl:inverseOf :hasReceiver ;
    skos:changeNote
        [
            dc:date "2023-11-02" ;
            rdf:value "Added a new rdfs:label in Spanish."@en ;
        ] ,
        [
            dc:date "2023-08-28" ;
            rdf:value "Added a new rdfs:label in French."@en ;
        ] ,
        [
            dc:date "2021-01-22" ;
            rdf:value """changed the IRI, label, inverse property IRI, super property
               IRI (changed made in order to make RiC-O compliant with RiC-CM 0.2; the name of this
               property in RiC-O 0.1 was "receives")."""@en ;
        ] ;
    :RiCCMCorrespondingComponent """RiC-R029i ('is receiver of'
         relation)"""@en ;
.

:isRecordSetTypeOf
    a owl:ObjectProperty ;
    rdfs:label
        "is record set type of"@en ,
        "es tipo de agrupación documental de"@es ,
        "est le type d’ensemble d’objets informationnels de"@fr ;
    rdfs:comment """Connects a Record Set Type to a Record Set that it
         categorizes."""@en ;
    rdfs:domain :RecordSetType ;
    rdfs:isDefinedBy <https://www.ica.org/standards/RiC/ontology> ;
    rdfs:range :RecordSet ;
    rdfs:subPropertyOf :isOrWasCategoryOf ;
    owl:inverseOf :hasRecordSetType ;
    skos:changeNote
        [
            dc:date "2023-11-02" ;
            rdf:value "Added a new rdfs:label in Spanish."@en ;
        ] ,
        [
            dc:date "2023-08-28" ;
            rdf:value "Added a new rdfs:label in French."@en ;
        ] ,
        [
            dc:date "2021-01-22" ;
            rdf:value "changed the super property IRI."@en ;
        ] ;
.

:isRecordStateOf
    a owl:ObjectProperty ;
    rdfs:label
        "is record state of"@en ,
        "es estado de documento de"@es ,
        "est l’état de"@fr ;
    rdfs:comment """Connects a Record State to a Record or Record Part whose state it
         categorizes."""@en ;
    rdfs:domain :RecordState ;
    rdfs:isDefinedBy <https://www.ica.org/standards/RiC/ontology> ;
    rdfs:range
        [
            a owl:Class ;
            owl:unionOf (
                :Record
                :RecordPart
            ) ;
        ] ;
    rdfs:subPropertyOf :isOrWasCategoryOf ;
    owl:inverseOf :hasRecordState ;
    skos:changeNote
        [
            dc:date "2023-08-28" ;
            rdf:value "Added a new rdfs:label in French."@en ;
        ] ,
        [
            dc:date "2023-11-02" ;
            rdf:value "Added a new rdfs:label in Spanish."@en ;
        ] ,
        [
            dc:date "2020-12-28" ;
            rdf:value """Changed the IRI, label, textual definition and range (Record
               Resource removed, replaced by Record or Record Part)."""@en ;
        ] ;
.

:isReplyTo
    a owl:ObjectProperty ;
    rdfs:label
        "is reply to"@en ,
        "es contestación de"@es ,
        "est une réponse à"@fr ;
    rdfs:comment "Inverse of 'has reply' object property."@en ;
    rdfs:domain :RecordResource ;
    rdfs:isDefinedBy <https://www.ica.org/standards/RiC/ontology> ;
    rdfs:range :RecordResource ;
    rdfs:subPropertyOf
        :followsInTime ,
        :isRecordResourceAssociatedWithRecordResource ;
    owl:inverseOf :hasReply ;
    skos:changeNote
        [
            dc:date "2021-01-22" ;
            rdf:value """changed the IRI, label, inverse property IRI, text definition
               (changed made in order to make RiC-O compliant with RiC-CM 0.2; the name of this
               property in RiC-O 0.1 was "repliesTo")."""@en ;
        ] ,
        [
            dc:date "2023-11-02" ;
            rdf:value "Added a new rdfs:label in Spanish."@en ;
        ] ,
        [
            dc:date "2023-08-28" ;
            rdf:value "Added a new rdfs:label in French."@en ;
        ] ;
    :RiCCMCorrespondingComponent """RiC-R013i ('is reply to'
         relation)"""@en ;
.

:isRepresentationTypeOf
    a owl:ObjectProperty ;
    rdfs:label
        "is representation type of"@en ,
        "es tipo de grabación de"@es ,
        "est le type de représentation de"@fr ;
    rdfs:comment """Connects a Representation Type to an Instantiation that it
         categorizes."""@en ;
    rdfs:domain :RepresentationType ;
    rdfs:isDefinedBy <https://www.ica.org/standards/RiC/ontology> ;
    rdfs:range :Instantiation ;
    rdfs:subPropertyOf :isOrWasCategoryOf ;
    owl:inverseOf :hasRepresentationType ;
    skos:changeNote
        [
            dc:date "2021-01-22" ;
            rdf:value "changed the super property IRI."@en ;
        ] ,
        [
            dc:date "2023-08-28" ;
            rdf:value "Added a new rdfs:label in French."@en ;
        ] ,
        [
            dc:date "2023-11-02" ;
            rdf:value "Added a new rdfs:label in Spanish."@en ;
        ] ;
.

:isResponsibleForIssuing
    a owl:ObjectProperty ;
    rdfs:label
        "is responsible for issuing"@en ,
        "es responsable de emisión de"@es ,
        "est chargé de rendre publique"@fr ;
    rdfs:comment "Inverse of 'issued by' object property."@en ;
    rdfs:domain :Agent ;
    rdfs:isDefinedBy <https://www.ica.org/standards/RiC/ontology> ;
    rdfs:range :Rule ;
    rdfs:subPropertyOf :isAssociatedWithRule ;
    owl:inverseOf :issuedBy ;
    skos:changeNote
        [
            dc:date "2023-08-28" ;
            rdf:value "Added a new rdfs:label in French."@en ;
        ] ,
        [
            dc:date "2023-11-02" ;
            rdf:value "Added a new rdfs:label in Spanish."@en ;
        ] ;
    :RiCCMCorrespondingComponent """RiC-R065i ('is responsible for issuing'
         relation)"""@en ;
.

:isSenderOf
    a owl:ObjectProperty ;
    rdfs:label
        "is sender of"@en ,
        "es remitente de"@es ,
        "est l’expéditeur de"@fr ;
    rdfs:comment "Inverse of 'has sender' object property."@en ;
    rdfs:domain :Agent ;
    rdfs:isDefinedBy <https://www.ica.org/standards/RiC/ontology> ;
    rdfs:range
        [
            a owl:Class ;
            owl:unionOf (
                :Instantiation
                :RecordResource
            ) ;
        ] ;
    rdfs:subPropertyOf :isOrganicProvenanceOf ;
    owl:inverseOf :hasSender ;
    skos:changeNote
        [
            dc:date "2023-08-28" ;
            rdf:value "Added a new rdfs:label in French."@en ;
        ] ,
        [
            dc:date "2023-11-02" ;
            rdf:value "Added a new rdfs:label in Spanish."@en ;
        ] ;
    :RiCCMCorrespondingComponent """RiC-R031i ('is sender of'
         relation)"""@en ;
.

:isToUseDateOf
    a owl:ObjectProperty ;
    rdfs:label
        "is to use date of"@en ,
        "es fecha hasta la que se usa"@es ,
        "est la date jusqu’à laquelle est utilisé"@fr ;
    rdfs:comment """Connects a Date to an Appellation, when it is the date till which
         the Appellation was used."""@en ;
    rdfs:domain :Date ;
    rdfs:isDefinedBy <https://www.ica.org/standards/RiC/ontology> ;
    rdfs:range :Appellation ;
    rdfs:subPropertyOf :isEndDateOf ;
    owl:inverseOf :wasUsedToDate ;
    skos:changeNote
        [
            dc:date "2023-10-19" ;
            rdf:value "Made this property a subPropertyOf isEndDateOf."@en ;
        ] ,
        [
            dc:date "2023-11-02" ;
            rdf:value "Added a new rdfs:label in Spanish."@en ;
        ] ,
        [
            dc:date "2023-08-28" ;
            rdf:value "Added a new rdfs:label in French."@en ;
        ] ;
.

:isUnitOfMeasurementOf
    a owl:ObjectProperty ;
    rdfs:label
        "is unit of measurement of"@en ,
        "es unidad de medida de"@es ,
        "est l’unité de mesure de"@fr ;
    rdfs:comment """Inverse of 'has unit of measurement' object
         property"""@en ;
    rdfs:domain :UnitOfMeasurement ;
    rdfs:isDefinedBy <https://www.ica.org/standards/RiC/ontology> ;
    rdfs:range :Extent ;
    rdfs:subPropertyOf :isRelatedTo ;
    owl:inverseOf :hasUnitOfMeasurement ;
    skos:changeNote
        [
            dc:date "2023-08-28" ;
            rdf:value """Added a new rdfs:label in French; added an xml:lang attribute
               to the rdfs:comment."""@en ;
        ] ,
        [
            dc:date "2023-11-02" ;
            rdf:value "Added a new rdfs:label in Spanish."@en ;
        ] ,
        [
            dc:date "2020-10-28" ;
            rdf:value """Object property created along with Extent and UnitOfMeasurement
               classes, in order to provide methods for handling extent accurately."""@en ;
        ] ;
.

:isWithin
    a owl:ObjectProperty ;
    rdfs:label
        "is within"@en ,
        "está dentro"@es ,
        "est contenu dans"@fr ;
    rdfs:comment "Connects a Date to a Date in which it is contained."@en ;
    rdfs:domain :Date ;
    rdfs:isDefinedBy <https://www.ica.org/standards/RiC/ontology> ;
    rdfs:range :Date ;
    rdfs:subPropertyOf
        :isAssociatedWithDate ,
        :isDateAssociatedWith ,
        :isOrWasPartOf ;
    owl:inverseOf :hasWithin ;
    skos:changeNote
        [
            dc:date "2023-11-27" ;
            rdf:value "Added a new rdfs:label in Spanish."@en ;
        ] ,
        [
            dc:date "2023-10-12" ;
            rdf:value "Added the property"@en ;
        ] ,
        [
            dc:date "2023-10-13" ;
            rdf:value """made this property a subproperty of both isDateAssociatedWith
               and isAssociatedWithdate, and of isOrWasPartOf."""@en ;
        ] ;
    :RiCCMCorrespondingComponent """RiC-R085 ('is within'
         relation)"""@en ;
.

:issuedBy
    a owl:ObjectProperty ;
    rdfs:label
        "issued by"@en ,
        "emitido por"@es ,
        "rendue publique par"@fr ;
    rdfs:comment """Connects a Rule to the Agent that issued or published the
         Rule."""@en ;
    rdfs:domain :Rule ;
    rdfs:isDefinedBy <https://www.ica.org/standards/RiC/ontology> ;
    rdfs:range :Agent ;
    rdfs:subPropertyOf :isRuleAssociatedWith ;
    owl:inverseOf :isResponsibleForIssuing ;
    skos:changeNote
        [
            dc:date "2023-11-02" ;
            rdf:value "Added a new rdfs:label in Spanish."@en ;
        ] ,
        [
            dc:date "2023-08-28" ;
            rdf:value "Added a new rdfs:label in French."@en ;
        ] ;
    :RiCCMCorrespondingComponent """RiC-R065 ('issued by'
         relation)"""@en ;
.

:knownBy
    a owl:ObjectProperty ;
    rdfs:label
        "known by"@en ,
        "conocido por"@es ,
        "est connue par"@fr ;
    rdfs:comment "Inverse of 'knows of' object property."@en ;
    rdfs:domain :Person ;
    rdfs:isDefinedBy <https://www.ica.org/standards/RiC/ontology> ;
    rdfs:range :Person ;
    rdfs:subPropertyOf :isAgentAssociatedWithAgent ;
    owl:inverseOf :knowsOf ;
    owl:propertyChainAxiom (
        :thingIsTargetOfRelation
        :knowingOfRelation_role
        :relationHasSource
    ) ;
    skos:changeNote
        [
            dc:date "2023-08-28" ;
            rdf:value "Added a new rdfs:label in French."@en ;
        ] ,
        [
            dc:date "2023-11-02" ;
            rdf:value "Added a new rdfs:label in Spanish."@en ;
        ] ,
        [
            dc:date "2023-11-08" ;
            rdf:value """In order to get a system of rolified Relation classes: modified
               the property chain axiom so that it now involves the new knowingOfRelation_role
               object property."""@en ;
        ] ;
    :RiCCMCorrespondingComponent """RiC-R050i ('known by'
         relation)"""@en ;
.

:knowsOf
    a owl:ObjectProperty ;
    rdfs:label
        "knows of"@en ,
        "conoce indirectamente a"@es ,
        "a connaissance de la personne"@fr ;
    rdfs:comment """Connects a Person to another Person they have some knowledge of
         through time or space."""@en ;
    rdfs:domain :Person ;
    rdfs:isDefinedBy <https://www.ica.org/standards/RiC/ontology> ;
    rdfs:range :Person ;
    rdfs:subPropertyOf :isAgentAssociatedWithAgent ;
    owl:inverseOf :knownBy ;
    owl:propertyChainAxiom (
        :thingIsSourceOfRelation
        :knowingOfRelation_role
        :relationHasTarget
    ) ;
    skos:changeNote
        [
            dc:date "2023-08-28" ;
            rdf:value "Added a new rdfs:label in French."@en ;
        ] ,
        [
            dc:date "2023-11-08" ;
            rdf:value """In order to get a system of rolified Relation classes: modified
               the property chain axiom so that it now involves the new knowingOfRelation_role
               object property."""@en ;
        ] ,
        [
            dc:date "2023-11-02" ;
            rdf:value "Added a new rdfs:label in Spanish."@en ;
        ] ;
    :RiCCMCorrespondingComponent """RiC-R050 ('knows of'
         relation)"""@en ;
.

:migratedFrom
    a owl:ObjectProperty ;
    rdfs:label
        "migrated from"@en ,
        "migrado desde"@es ,
        "a été produite par migration de"@fr ;
    rdfs:comment "Inverse of 'migrated into' object property."@en ;
    rdfs:domain :Instantiation ;
    rdfs:isDefinedBy <https://www.ica.org/standards/RiC/ontology> ;
    rdfs:range :Instantiation ;
    rdfs:subPropertyOf :isOrWasDerivedFromInstantiation ;
    owl:inverseOf :migratedInto ;
    owl:propertyChainAxiom (
        :thingIsTargetOfRelation
        :migrationRelation_role
        :relationHasSource
    ) ;
    skos:changeNote
        [
            dc:date "2023-08-29" ;
            rdf:value """Updated subpropertyOf; this in order to make the specification
               compliant with RiC-CM 1.0."""@en ;
        ] ,
        [
            dc:date "2023-11-08" ;
            rdf:value """In order to get a system of rolified Relation classes: modified
               the property chain axiom so that it now involves the new migrationRelation_role
               object property."""@en ;
        ] ,
        [
            dc:date "2023-11-02" ;
            rdf:value "Added a new rdfs:label in Spanish."@en ;
        ] ,
        [
            dc:date "2021-01-22" ;
            rdf:value """changed the IRI, label, inverse property IRI, text definition,
               corresponding CM component name (changed made in order to make RiC-O compliant with
               RiC-CM 0.2; the name of this property in RiC-O 0.1 was
               "createdByMigrationFromInstantiation")."""@en ;
        ] ,
        [
            dc:date "2023-08-28" ;
            rdf:value "Added a new rdfs:label in French."@en ;
        ] ;
    :RiCCMCorrespondingComponent """RiC-R015i ('migrated from'
         relation)"""@en ;
.

:migratedInto
    a owl:ObjectProperty ;
    rdfs:label
        "migrated into"@en ,
        "migrado a"@es ,
        "a été migrée vers"@fr ;
    rdfs:comment """Connects an Instantiation to a version it has been migrated
         into."""@en ;
    rdfs:domain :Instantiation ;
    rdfs:isDefinedBy <https://www.ica.org/standards/RiC/ontology> ;
    rdfs:range :Instantiation ;
    rdfs:subPropertyOf :hasOrHadDerivedInstantiation ;
    owl:inverseOf :migratedFrom ;
    owl:propertyChainAxiom (
        :thingIsSourceOfRelation
        :migrationRelation_role
        :relationHasTarget
    ) ;
    skos:changeNote
        [
            dc:date "2023-11-08" ;
            rdf:value """In order to get a system of rolified Relation classes: modified
               the property chain axiom so that it now involves the new migrationRelation_role
               object property."""@en ;
        ] ,
        [
            dc:date "2021-01-22" ;
            rdf:value """changed the IRI, label and inverse property IRI (changed made
               in order to make RiC-O compliant with RiC-CM 0.2; the name of this property in RiC-O
               0.1 was "isMigratedIntoInstantiation")."""@en ;
        ] ,
        [
            dc:date "2023-08-29" ;
            rdf:value """Updated subpropertyOf; this in order to make the specification
               compliant with RiC-CM 1.0."""@en ;
        ] ,
        [
            dc:date "2023-11-02" ;
            rdf:value "Added a new rdfs:label in Spanish."@en ;
        ] ,
        [
            dc:date "2023-08-28" ;
            rdf:value "Added a new rdfs:label in French."@en ;
        ] ,
        [
            dc:date "2023-11-12" ;
            rdf:value """Aligned with RiC-CM 1.0: updated the description
               (rdfs:comment)."""@en ;
        ] ;
    skos:scopeNote "Use for digital instantiations."@en ;
    :RiCCMCorrespondingComponent """RiC-R015 ('migrated into'
         relation)"""@en ;
.

:modificationDate
    a owl:DatatypeProperty ;
    rdfs:label
        "modification date"@en ,
        "fecha de modificación"@es ,
        "date de modification"@fr ;
    rdfs:comment "Date of the modification of an entity."@en ;
    rdfs:domain :Thing ;
    rdfs:isDefinedBy <https://www.ica.org/standards/RiC/ontology> ;
    rdfs:range rdfs:Literal ;
    rdfs:subPropertyOf :date ;
    skos:changeNote
        [
            dc:date "2023-11-02" ;
            rdf:value "Added a new rdfs:label in Spanish."@en ;
        ] ,
        [
            dc:date "2023-08-25" ;
            rdf:value "Added a new rdfs:label in French."@en ;
        ] ;
    skos:scopeNote """Provided for usability reasons. May be deprecated and removed
         later on. Use only if you don't use Date classes for handling dates."""@en ;
    :RiCCMCorrespondingComponent """Datatype property specialized implementation of
         RiC-E18 (Date entity)"""@en ;
.

:normalizedValue
    a owl:DatatypeProperty ;
    rdfs:label
        "normalized value"@en ,
        "valor normalizado"@es ,
        "valeur normalisée"@fr ;
    rdfs:comment """Value representation based on a standard, preferably
         machine-readable."""@en ;
    rdfs:domain
        [
            a owl:Class ;
            owl:unionOf (
                :Appellation
                :Date
            ) ;
        ] ;
    rdfs:isDefinedBy <https://www.ica.org/standards/RiC/ontology> ;
    rdfs:range rdfs:Literal ;
    rdfs:subPropertyOf :textualValue ;
    skos:changeNote
        [
            dc:date "2023-08-25" ;
            rdf:value "Added a new rdfs:label in French."@en ;
        ] ,
        [
            dc:date "2023-11-02" ;
            rdf:value "Added a new rdfs:label in Spanish."@en ;
        ] ;
.

:occupiesOrOccupied
    a owl:ObjectProperty ;
    rdfs:label
        "occupies or occupied"@en ,
        "ocupa u ocupaba"@es ,
        "occupe ou a occupé"@fr ;
    rdfs:comment """Connects a Person to a Position they occupy or
         occupied."""@en ;
    rdfs:domain :Person ;
    rdfs:isDefinedBy <https://www.ica.org/standards/RiC/ontology> ;
    rdfs:range :Position ;
    rdfs:subPropertyOf :isAgentAssociatedWithAgent ;
    owl:inverseOf :isOrWasOccupiedBy ;
    owl:propertyChainAxiom (
        :thingIsSourceOfRelation
        :positionHoldingRelation_role
        :relationHasTarget
    ) ;
    skos:changeNote
        [
            dc:date "2021-01-22" ;
            rdf:value """changed the IRI, label, inverse property IRI, text definition
               (changed made in order to make RiC-O compliant with RiC-CM 0.2; the name of this
               property in RiC-O 0.1 was "occupies")."""@en ;
        ] ,
        [
            dc:date "2023-08-28" ;
            rdf:value "Added a new rdfs:label in French."@en ;
        ] ,
        [
            dc:date "2023-11-08" ;
            rdf:value """In order to get a system of rolified Relation classes: modified
               the property chain axiom so that it now involves the new positionHoldingRelation_role
               object property."""@en ;
        ] ,
        [
            dc:date "2023-11-02" ;
            rdf:value "Added a new rdfs:label in Spanish."@en ;
        ] ;
    :RiCCMCorrespondingComponent """RiC-R054 ('occupies or occupied'
         relation)"""@en ;
.

:occurredAtDate
    a owl:ObjectProperty ;
    rdfs:label
        "occurred at date"@en ,
        "tiene como fecha de ocurrencia"@es ,
        "a pour date d'occurrence"@fr ;
    rdfs:comment """Inverse of 'is date of occurrence of' object
         property"""@en ;
    rdfs:domain :Event ;
    rdfs:isDefinedBy <https://www.ica.org/standards/RiC/ontology> ;
    rdfs:range :Date ;
    rdfs:subPropertyOf
        :isAssociatedWithDate ,
        :isEventAssociatedWith ;
    owl:inverseOf :isDateOfOccurrenceOf ;
    skos:changeNote
        [
            dc:date "2023-11-27" ;
            rdf:value "Added a new rdfs:label in Spanish."@en ;
        ] ,
        [
            dc:date "2023-10-17" ;
            rdf:value """Made this property a subproperty of
               isEventAssociatedWith"""@en ;
        ] ,
        [
            dc:date "2023-10-13" ;
            rdf:value """Renamed the property to correct a spelling mistake. Also
               corrected the annotations when necessary."""@en ;
        ] ;
    :RiCCMCorrespondingComponent """RiC-R084i ('occurred at date'
         relation)"""@en ;
.

:performsOrPerformed
    a owl:ObjectProperty ;
    rdfs:label
        "performs or performed"@en ,
        "desarrolla o desarrollaba"@es ,
        "exerce ou a exercé"@fr ;
    rdfs:comment """Inverse of 'is or was performed by' object
         property."""@en ;
    rdfs:domain :Agent ;
    rdfs:isDefinedBy <https://www.ica.org/standards/RiC/ontology> ;
    rdfs:range :Activity ;
    rdfs:subPropertyOf :isOrWasParticipantIn ;
    owl:inverseOf :isOrWasPerformedBy ;
    owl:propertyChainAxiom (
        :thingIsTargetOfRelation
        :performanceRelation_role
        :relationHasSource
    ) ;
    skos:changeNote
        [
            dc:date "2023-08-28" ;
            rdf:value "Added a new rdfs:label in French."@en ;
        ] ,
        [
            dc:date "2023-11-08" ;
            rdf:value """In order to get a system of rolified Relation classes: modified
               the property chain axiom so that it now involves the new performanceRelation_role
               object property."""@en ;
        ] ,
        [
            dc:date "2021-01-22" ;
            rdf:value """changed the IRI, label, inverse property IRI, text definition,
               super property IRI (changed made in order to make RiC-O compliant with RiC-CM 0.2;
               the name of this property in RiC-O 0.1 was "performs")."""@en ;
        ] ,
        [
            dc:date "2023-11-02" ;
            rdf:value "Added a new rdfs:label in Spanish."@en ;
        ] ;
    :RiCCMCorrespondingComponent """RiC-R060i ('performs or performed'
         relation)"""@en ;
.

:physicalCharacteristicsNote
    a owl:DatatypeProperty ;
    rdfs:label
        "physical characteristics note"@en ,
        "nota sobre las características físicas"@es ,
        "note sur les caractéristiques physiques"@fr ;
    rdfs:comment """Information about the physical features, completeness, or
         conservation status of an Instantiation. Includes information about the physical nature and
         condition such as conservation status or the deterioration of an Instantiation (for example
         its carrier) affecting the ability to recover information. """@en ;
    rdfs:domain :Instantiation ;
    rdfs:isDefinedBy <https://www.ica.org/standards/RiC/ontology> ;
    rdfs:range rdfs:Literal ;
    skos:changeNote
        [
            dc:date "2023-11-02" ;
            rdf:value "Added a new rdfs:label in Spanish."@en ;
        ] ,
        [
            dc:date "2023-08-25" ;
            rdf:value "Added a new rdfs:label in French."@en ;
        ] ,
        [
            dc:date "2023-11-11" ;
            rdf:value """Aligned with RiC-CM 1.0: updated the IRI, mapping to RiC-CM
               (rico:RiCCMCorrespondingComponent), labels, description (rdfs:comment),
               skos:scopeNote, examples (skos:example)."""@en ;
        ] ,
        [
            dc:date "2020-11-01" ;
            rdf:value """Text definition updated. Examples added. Objective: to make
               RiC-O compliant with RiC-CM v0.2."""@en ;
        ] ;
    skos:example
        """A web page (HTML, 15 images, 2 CSS, 1 JavaScript), with 1 CSS
         missing."""@en ,
        "British Library binding"@en ,
        "Digital file format: JPEG-2000"@en ,
        """For carrier: hard drives on which the author wrote physically
         (using a pen)."""@en ,
        """Letter physical characteristics: corner without text missing – the
         carrier is damaged, but no information of the content is missing"""@en ,
        "The charter is missing the seal."@en ,
        "Watermarked"@en ,
        "carrier heavily foxed"@en ,
        "some loss of text due to rodent damage"@en ;
    skos:scopeNote """Not to be confused with the intellectual completeness of a
         Record Resource and its sub-entities, which is covered by the Integrity attribute. May
         include digital file fixity. """@en ;
    :RiCCMCorrespondingComponent """Corresponds to RiC-A31 (Physical
         Characteristics Note attribute)"""@en ;
.

:positionIsContextOfLeadershipRelation
    a owl:ObjectProperty ;
    rdfs:label
        "position is context of leadership relation"@en ,
        "puesto es contexto de relación de liderazgo"@es ,
        "poste est le contexte de la relation de direction"@fr ;
    rdfs:comment """Connects a Position to a Leadership Relation (the leading Person
         occupies that Position)."""@en ;
    rdfs:domain :Position ;
    rdfs:isDefinedBy <https://www.ica.org/standards/RiC/ontology> ;
    rdfs:range :LeadershipRelation ;
    rdfs:subPropertyOf :thingIsContextOfRelation ;
    owl:inverseOf :leadershipWithPosition ;
    skos:changeNote
        [
            dc:date "2023-11-12" ;
            rdf:value "Updated the labels."@en ;
        ] ,
        [
            dc:date "2023-11-02" ;
            rdf:value "Added a new rdfs:label in Spanish."@en ;
        ] ;
.

:positionIsContextOfMembershipRelation
    a owl:ObjectProperty ;
    rdfs:label
        "position is context of membership relation"@en ,
        "puesto es contexto de relación de membresía"@es ,
        "poste est le contexte de la relation d'appartenance"@fr ;
    rdfs:comment """Connects a Position to a Membership Relation (the member Person
         occupies that Position)."""@en ;
    rdfs:domain :Position ;
    rdfs:isDefinedBy <https://www.ica.org/standards/RiC/ontology> ;
    rdfs:range :MembershipRelation ;
    rdfs:subPropertyOf :thingIsContextOfRelation ;
    owl:inverseOf :membershipWithPosition ;
    skos:changeNote
        [
            dc:date "2023-11-02" ;
            rdf:value "Added a new rdfs:label in Spanish."@en ;
        ] ,
        [
            dc:date "2023-11-12" ;
            rdf:value "Updated the labels."@en ;
        ] ;
.

:precededInSequence
    a owl:ObjectProperty ;
    rdfs:label
        "preceded in sequence"@en ,
        "precedía secuencialmente a"@es ,
        "a précédé dans la séquence"@fr ;
    rdfs:comment """Connects a Thing to a Thing that followed it in some non
         chronological sequence in the past."""@en ;
    rdfs:domain :Thing ;
    rdfs:isDefinedBy <https://www.ica.org/standards/RiC/ontology> ;
    rdfs:range :Thing ;
    rdfs:subPropertyOf :precedesOrPreceded ;
    owl:inverseOf :followedInSequence ;
    skos:changeNote
        [
            dc:date "2023-09-08" ;
            rdf:value """Object property added, along with its inverse property, in
               order to enable to express past sequential relations between things (the current
               sequential relations being also added, including a transitive one)."""@en ;
        ] ,
        [
            dc:date "2023-11-12" ;
            rdf:value "Updated the labels."@en ;
        ] ,
        [
            dc:date "2023-09-22" ;
            rdf:value """Renamed the property and modified its definition (rdfs:comment)
               in order to better distinguish it from precedesInTime."""@en ;
        ] ,
        [
            dc:date "2023-11-27" ;
            rdf:value "Added a new rdfs:label in Spanish."@en ;
        ] ;
.

:proxyFor
    a owl:ObjectProperty ;
    rdfs:label
        "proxy for"@en ,
        "es proxy para"@es ,
        "proxy pour"@fr ;
    rdfs:comment """Connects a Proxy to the Record Resource it stands for in the
         specific context of a Record Set."""@en ;
    rdfs:domain :Proxy ;
    rdfs:isDefinedBy <https://www.ica.org/standards/RiC/ontology> ;
    rdfs:range :RecordResource ;
    rdfs:subPropertyOf :isRelatedTo ;
    skos:changeNote
        [
            dc:date "2023-11-02" ;
            rdf:value "Added a new rdfs:label in Spanish."@en ;
        ] ,
        [
            dc:date "2023-08-28" ;
            rdf:value "Added a new rdfs:label in French."@en ;
        ] ;
.

:proxyIn
    a owl:ObjectProperty ;
    rdfs:label
        "proxy in"@en ,
        "es proxy en"@es ,
        "proxy dans"@fr ;
    rdfs:comment """Connects a Proxy to the Record Set in which it stands for
         (represents) another Record Resource."""@en ;
    rdfs:domain :Proxy ;
    rdfs:isDefinedBy <https://www.ica.org/standards/RiC/ontology> ;
    rdfs:range :RecordSet ;
    rdfs:subPropertyOf :isRelatedTo ;
    skos:changeNote
        [
            dc:date "2023-08-28" ;
            rdf:value "Added a new rdfs:label in French."@en ;
        ] ,
        [
            dc:date "2023-11-02" ;
            rdf:value "Added a new rdfs:label in Spanish."@en ;
        ] ;
.

:regulatesOrRegulated
    a owl:ObjectProperty ;
    rdfs:label
        "regulates or regulated"@en ,
        "regula o regulaba"@es ,
        "régule ou a régulé"@fr ;
    rdfs:comment """Connects a Rule to a Thing that it regulates or
         regulated."""@en ;
    rdfs:domain :Rule ;
    rdfs:isDefinedBy <https://www.ica.org/standards/RiC/ontology> ;
    rdfs:range :Thing ;
    rdfs:subPropertyOf :isRuleAssociatedWith ;
    owl:inverseOf :isOrWasRegulatedBy ;
    skos:changeNote
        [
            dc:date "2023-11-02" ;
            rdf:value "Added a new rdfs:label in Spanish."@en ;
        ] ,
        [
            dc:date "2021-01-22" ;
            rdf:value """changed the IRI, label, inverse property IRI (changed made in
               order to make RiC-O compliant with RiC-CM 0.2; the name of this property in RiC-O 0.1
               was "regulates")."""@en ;
        ] ,
        [
            dc:date "2023-08-28" ;
            rdf:value "Added a new rdfs:label in French."@en ;
        ] ;
    :RiCCMCorrespondingComponent """RiC-R063 ('regulates or regulated'
         relation)"""@en ;
.

:resultedFromTheMergerOf
    a owl:ObjectProperty ;
    rdfs:label
        "resulted from the merger of"@en ,
        "resultado de la fusión de"@es ,
        "résulte de la fusion de"@fr ;
    rdfs:comment "Inverse of 'was merged into' object property."@en ;
    rdfs:domain :CorporateBody ;
    rdfs:isDefinedBy <https://www.ica.org/standards/RiC/ontology> ;
    rdfs:range :CorporateBody ;
    rdfs:subPropertyOf :isSuccessorOf ;
    owl:inverseOf :wasMergedInto ;
    skos:changeNote
        [
            dc:date "2023-11-02" ;
            rdf:value "Added a new rdfs:label in Spanish."@en ;
        ] ,
        [
            dc:date "2024-03-15" ;
            rdf:value "Make capitalisation of rdfs:comment consistent."@en ;
        ] ,
        [
            dc:date "2023-06-21" ;
            rdf:value """Object property created in order to enable an accurate
               representation of mergers between corporate bodies."""@en ;
        ] ,
        [
            dc:date "2023-11-12" ;
            rdf:value "Updated the labels."@en ;
        ] ;
.

:resultedFromTheSplitOf
    a owl:ObjectProperty ;
    rdfs:label
        "resulted from the split of"@en ,
        "resultado de la separación de"@es ,
        "résulte de la séparation de"@fr ;
    rdfs:comment "Inverse of 'was split into' object property."@en ;
    rdfs:domain :CorporateBody ;
    rdfs:isDefinedBy <https://www.ica.org/standards/RiC/ontology> ;
    rdfs:range :CorporateBody ;
    rdfs:subPropertyOf :isSuccessorOf ;
    owl:inverseOf :wasSplitInto ;
    skos:changeNote
        [
            dc:date "2023-11-02" ;
            rdf:value "Added a new rdfs:label in Spanish."@en ;
        ] ,
        [
            dc:date "2023-11-12" ;
            rdf:value "Updated the labels."@en ;
        ] ,
        [
            dc:date "2023-06-21"@en ;
            rdf:value """Object property created in order to enable an accurate
               representation of the split of a corporate body into two or more new corporate
               bodies."""@en ;
        ] ;
.

:roleIsContextOfCreationRelation
    a owl:ObjectProperty ;
    rdfs:label
        "role is context of creation relation"@en ,
        "rol es contexto de relación de creación"@es ,
        "rôle est le contexte de la relation de création"@fr ;
    rdfs:comment """Connects a Role Type to a Creation Relation (this Role Type being
         the specific role played by the creating Person in the context of this
         Relation)."""@en ;
    rdfs:domain :RoleType ;
    rdfs:isDefinedBy <https://www.ica.org/standards/RiC/ontology> ;
    rdfs:range :CreationRelation ;
    rdfs:subPropertyOf :thingIsContextOfRelation ;
    owl:inverseOf :creationWithRole ;
    skos:changeNote
        [
            dc:date "2023-08-28" ;
            rdf:value "Added a new rdfs:label in French."@en ;
        ] ,
        [
            dc:date "2023-11-02" ;
            rdf:value "Added a new rdfs:label in Spanish."@en ;
        ] ;
.

:ruleFollowed
    a owl:DatatypeProperty ;
    rdfs:label
        "rule followed"@en ,
        "regla aplicada"@es ,
        "règle suivie"@fr ;
    rdfs:comment """The rule or conditions that govern the existence or lifecycle of a
         Thing."""@en ;
    rdfs:domain :Thing ;
    rdfs:isDefinedBy <https://www.ica.org/standards/RiC/ontology> ;
    rdfs:range rdfs:Literal ;
    skos:changeNote
        [
            dc:date "2023-08-25" ;
            rdf:value "Added a new rdfs:label in French."@en ;
        ] ,
        [
            dc:date "2023-11-02" ;
            rdf:value "Added a new rdfs:label in Spanish."@en ;
        ] ;
    skos:scopeNote """Provided for usability reasons. May be deprecated and removed
         later on. Use only if you don't use the Rule class for handling rules."""@en ;
.

:wasComponentOf
    a owl:ObjectProperty ;
    rdfs:label
        "was component of"@en ,
        "era componente de"@es ,
        "a été le composant de"@fr ;
    rdfs:comment """Connects an Instantiation to another Instantiation of which it was
         a component in the past."""@en ;
    rdfs:domain :Instantiation ;
    rdfs:isDefinedBy <https://www.ica.org/standards/RiC/ontology> ;
    rdfs:range :Instantiation ;
    rdfs:subPropertyOf
        :isOrWasComponentOf ,
        :wasPartOf ;
    owl:inverseOf :hadComponent ;
    skos:changeNote
        [
            dc:date "2023-11-12" ;
            rdf:value "Updated the description (rdfs:comment) and labels."@en ;
        ] ,
        [
            dc:date "2023-09-08" ;
            rdf:value """Object property added, along with its inverse property, in
               order to enable to express past partitive relations between instantiations (the
               current partitive relations being also added, including a transitive
               one)."""@en ;
        ] ,
        [
            dc:date "2023-11-27" ;
            rdf:value "Added a new rdfs:label in Spanish."@en ;
        ] ;
.

:wasConstituentOf
    a owl:ObjectProperty ;
    rdfs:label
        "was constituent of"@en ,
        "era elemento constitutivo de"@es ,
        "a été un constituant de"@fr ;
    rdfs:comment """Connects a Record or Record Part to another Record or Record Part
         of which it was a constituent in the past."""@en ;
    rdfs:domain
        [
            a owl:Class ;
            owl:unionOf (
                :Record
                :RecordPart
            ) ;
        ] ;
    rdfs:isDefinedBy <https://www.ica.org/standards/RiC/ontology> ;
    rdfs:range
        [
            a owl:Class ;
            owl:unionOf (
                :Record
                :RecordPart
            ) ;
        ] ;
    rdfs:subPropertyOf
        :isOrWasConstituentOf ,
        :wasPartOf ;
    owl:inverseOf :hadConstituent ;
    skos:changeNote
        [
            dc:date "2023-10-26" ;
            rdf:value "Added RecordPart to the range."@en ;
        ] ,
        [
            dc:date "2023-11-27" ;
            rdf:value "Added a new rdfs:label in Spanish."@en ;
        ] ,
        [
            dc:date "2023-09-08" ;
            rdf:value """Object property added, along with its inverse property, in
               order to enable to express past partitive relations between Record and Record or
               Record Part (the current partitive relations being also added, including a transitive
               one)."""@en ;
        ] ,
        [
            dc:date "2023-11-12" ;
            rdf:value "Updated the labels."@en ;
        ] ;
.

:wasContainedBy
    a owl:ObjectProperty ;
    rdfs:label
        "was contained by"@en ,
        "estaba contenido en"@es ,
        "a été contenu par"@fr ;
    rdfs:comment """Connects a Place to a Place within which it was
         contained."""@en ;
    rdfs:domain :Place ;
    rdfs:isDefinedBy <https://www.ica.org/standards/RiC/ontology> ;
    rdfs:range :Place ;
    rdfs:subPropertyOf
        :isOrWasContainedBy ,
        :wasPartOf ;
    owl:inverseOf :contained ;
    skos:changeNote
        [
            dc:date "2023-11-27" ;
            rdf:value "Added a new rdfs:label in Spanish."@en ;
        ] ,
        [
            dc:date "2023-09-08" ;
            rdf:value """Object property added, along with its inverse property, in
               order to enable to express past partitive relations between places (the current
               partitive relations being also added, including a transitive one)."""@en ;
        ] ,
        [
            dc:date "2023-11-12" ;
            rdf:value "Updated the description (rdfs:comment) and labels."@en ;
        ] ;
.

:wasIncludedIn
    a owl:ObjectProperty ;
    rdfs:label
        "was included in"@en ,
        "estaba incluido en"@es ,
        "a été inclus dans"@fr ;
    rdfs:comment """Connects a Record to a Record or Record Set in which it was
         included in the past."""@en ;
    rdfs:domain
        [
            a owl:Class ;
            owl:unionOf (
                :Record
                :RecordSet
            ) ;
        ] ;
    rdfs:isDefinedBy <https://www.ica.org/standards/RiC/ontology> ;
    rdfs:range :RecordSet ;
    rdfs:subPropertyOf
        :isOrWasIncludedIn ,
        :wasPartOf ;
    owl:inverseOf :included ;
    skos:changeNote
        [
            dc:date "2023-09-08" ;
            rdf:value """Object property added, along with its inverse property, in
               order to enable to express past partitive relations between Record Sets and their
               members (the current partitive relations being also added, including a transitive
               one)."""@en ;
        ] ,
        [
            dc:date "2023-11-27" ;
            rdf:value "Added a new rdfs:label in Spanish."@en ;
        ] ,
        [
            dc:date "2023-11-12" ;
            rdf:value "Updated the labels."@en ;
        ] ;
.

:wasLastUpdatedAtDate
    a owl:ObjectProperty ;
    rdfs:label
        "was last updated at date"@en ,
        "fue actualizado por última vez en fecha"@es ,
        "a pour date de dernière mise à jour"@fr ;
    rdfs:comment """Connects a Thing to the Date when it was last
         modified."""@en ;
    rdfs:domain :Thing ;
    rdfs:isDefinedBy <https://www.ica.org/standards/RiC/ontology> ;
    rdfs:range :Date ;
    rdfs:subPropertyOf :hasModificationDate ;
    owl:inverseOf :isLastUpdateDateOf ;
    skos:changeNote
        [
            dc:date "2023-08-28" ;
            rdf:value "Added a new rdfs:label in French."@en ;
        ] ,
        [
            dc:date "2023-11-02" ;
            rdf:value "Added a new rdfs:label in Spanish."@en ;
        ] ;
.

:wasMergedInto
    a owl:ObjectProperty ;
    rdfs:label
        "was merged into"@en ,
        "se fusionó en"@es ,
        "a été fusionné dans"@fr ;
    rdfs:comment """Connects a Corporate Body to another Corporate Body that is the
         result of a merger of the previous one with one to many other corporate
         bodies."""@en ;
    rdfs:domain :CorporateBody ;
    rdfs:isDefinedBy <https://www.ica.org/standards/RiC/ontology> ;
    rdfs:range :CorporateBody ;
    rdfs:subPropertyOf :hasSuccessor ;
    owl:inverseOf :resultedFromTheMergerOf ;
    skos:changeNote
        [
            dc:date "2023-06-21" ;
            rdf:value """Object property created in order to enable an accurate
               representation of mergers between corporate bodies."""@en ;
        ] ,
        [
            dc:date "2023-11-02" ;
            rdf:value "Added a new rdfs:label in Spanish."@en ;
        ] ,
        [
            dc:date "2023-11-12" ;
            rdf:value "Updated the labels."@en ;
        ] ;
.

:wasSplitInto
    a owl:ObjectProperty ;
    rdfs:label
        "was split into"@en ,
        "se separó en"@es ,
        "a été séparé en"@fr ;
    rdfs:comment """Connects a Corporate Body to one of the Corporate Bodies that
         results from the split of the previous one into two to many corporate
         bodies."""@en ;
    rdfs:domain :CorporateBody ;
    rdfs:isDefinedBy <https://www.ica.org/standards/RiC/ontology> ;
    rdfs:range :CorporateBody ;
    rdfs:subPropertyOf :hasSuccessor ;
    owl:inverseOf :resultedFromTheSplitOf ;
    skos:changeNote
        [
            dc:date "2023-11-02" ;
            rdf:value "Added a new rdfs:label in Spanish."@en ;
        ] ,
        [
            dc:date "2023-06-21" ;
            rdf:value """Object property created in order to enable an accurate
               representation of the split of a corporate body into two or more new corporate
               bodies."""@en ;
        ] ,
        [
            dc:date "2023-11-12" ;
            rdf:value "Updated the labels."@en ;
        ] ;
.

:wasSubdivisionOf
    a owl:ObjectProperty ;
    rdfs:label
        "was subdivision of"@en ,
        "era subdivisión de"@es ,
        "a été une subdivision de"@fr ;
    rdfs:comment """Connects a subdivision to the Group it was a part of in the
         past."""@en ;
    rdfs:domain :Group ;
    rdfs:isDefinedBy <https://www.ica.org/standards/RiC/ontology> ;
    rdfs:range :Group ;
    rdfs:subPropertyOf
        :isOrWasSubdivisionOf ,
        :wasPartOf ,
        :wasSubordinateTo ;
    owl:inverseOf :hadSubdivision ;
    skos:changeNote
        [
            dc:date "2023-09-08" ;
            rdf:value """Object property added, along with its inverse property, in
               order to enable to express past partitive relations between Groups (the current
               partitive relations being also added, including a transitive one)."""@en ;
        ] ,
        [
            dc:date "2023-11-27" ;
            rdf:value "Added a new rdfs:label in Spanish."@en ;
        ] ,
        [
            dc:date "2023-11-12" ;
            rdf:value "Updated the labels."@en ;
        ] ;
.

:wasSubeventOf
    a owl:ObjectProperty ;
    rdfs:label
        "was subevent of"@en ,
        "era parte de evento de"@es ,
        "a été un événement constitutif de l'événement"@fr ;
    rdfs:comment """Connects a past Event to the broader Event of which it was a
         part."""@en ;
    rdfs:domain :Event ;
    rdfs:isDefinedBy <https://www.ica.org/standards/RiC/ontology> ;
    rdfs:range :Event ;
    rdfs:subPropertyOf
        :isOrWasSubeventOf ,
        :wasPartOf ;
    owl:inverseOf :hadSubevent ;
    skos:changeNote
        [
            dc:date "2023-11-27" ;
            rdf:value "Added a new rdfs:label in Spanish."@en ;
        ] ,
        [
            dc:date "2023-09-08" ;
            rdf:value """Object property added, along with its inverse property, in
               order to enable to express partitive relations between past Events (the partitive
               relations between ongoing events being also added, including a transitive
               one)."""@en ;
        ] ,
        [
            dc:date "2023-11-12" ;
            rdf:value "Updated the labels."@en ;
        ] ;
.

:wasUsedFromDate
    a owl:ObjectProperty ;
    rdfs:label
        "was used from date"@en ,
        "fue usado desde"@es ,
        "a été utilisé à partir de la date"@fr ;
    rdfs:comment """Connects an Appellation to the Date from which it was
         used."""@en ;
    rdfs:domain :Appellation ;
    rdfs:isDefinedBy <https://www.ica.org/standards/RiC/ontology> ;
    rdfs:range :Date ;
    rdfs:subPropertyOf :hasBeginningDate ;
    owl:inverseOf :isFromUseDateOf ;
    skos:changeNote
        [
            dc:date "2023-11-02" ;
            rdf:value "Added a new rdfs:label in Spanish."@en ;
        ] ,
        [
            dc:date "2023-08-28" ;
            rdf:value "Added a new rdfs:label in French."@en ;
        ] ,
        [
            dc:date "2023-10-19" ;
            rdf:value "Made this property subPropertyOf hasBeginningDate."@en ;
        ] ;
.

:wasUsedToDate
    a owl:ObjectProperty ;
    rdfs:label
        "was used to date"@en ,
        "fue usado hasta"@es ,
        "a été utilisé jusqu’à la date"@fr ;
    rdfs:comment """Connects an Appellation to the Date till when it was
         used."""@en ;
    rdfs:domain :Appellation ;
    rdfs:isDefinedBy <https://www.ica.org/standards/RiC/ontology> ;
    rdfs:range :Date ;
    rdfs:subPropertyOf :hasEndDate ;
    owl:inverseOf :isToUseDateOf ;
    skos:changeNote
        [
            dc:date "2023-10-19" ;
            rdf:value "Made this property subPropertyOf hasEndDate."@en ;
        ] ,
        [
            dc:date "2023-11-02" ;
            rdf:value "Added a new rdfs:label in Spanish."@en ;
        ] ,
        [
            dc:date "2023-08-28" ;
            rdf:value "Added a new rdfs:label in French."@en ;
        ] ;
.

ric-dft:AuthorityRecord
    a
        owl:NamedIndividual ,
        skos:Concept ,
        :DocumentaryFormType ;
    rdfs:label
        "authority record"@en ,
        "registro de autoridad"@es ,
        "notice d’autorité"@fr ;
    skos:changeNote
        [
            dc:date "2023-08-28" ;
            rdf:value "Added a new rdfs:label in French."@en ;
        ] ,
        [
            dc:date "2023-11-25" ;
            rdf:value "Added a new rdfs:label in Spanish."@en ;
        ] ;
    skos:definition """This category can be used for records that describe an
         entity."""@en ;
    skos:inScheme <https://www.ica.org/standards/RiC/vocabularies/documentaryFormTypes> ;
    skos:topConceptOf <https://www.ica.org/standards/RiC/vocabularies/documentaryFormTypes> ;
.

ric-dft:FindingAid
    a
        owl:NamedIndividual ,
        skos:Concept ,
        :DocumentaryFormType ;
    rdfs:label
        "finding aid"@en ,
        "instrumento de descripción"@es ,
        "instrument de recherche"@fr ;
    skos:changeNote
        [
            dc:date "2023-08-28" ;
            rdf:value "Added a new rdfs:label in French."@en ;
        ] ,
        [
            dc:date "2023-11-25" ;
            rdf:value "Added a new rdfs:label in Spanish."@en ;
        ] ;
    skos:definition """This documentary form type can be used for records that
         aggregate and organizes metadata on some record(s) or record set(s)."""@en ;
    skos:inScheme <https://www.ica.org/standards/RiC/vocabularies/documentaryFormTypes> ;
    skos:topConceptOf <https://www.ica.org/standards/RiC/vocabularies/documentaryFormTypes> ;
.

ric-rst:Collection
    a
        owl:NamedIndividual ,
        skos:Concept ,
        :RecordSetType ;
    rdfs:label
        "collection"@en ,
        "colección"@es ,
        "collection"@fr ;
    skos:changeNote
        [
            dc:date "2023-11-25" ;
            rdf:value "Added a new rdfs:label in Spanish."@en ;
        ] ,
        [
            dc:date "2023-08-28" ;
            rdf:value "Added a new rdfs:label in French."@en ;
        ] ;
    skos:definition """An artificial assemblage of documents accumulated on the basis
         of some common characteristic without regard to the provenance of those documents. Not to
         be confused with an archival fonds. (From ICA ISAD(G))"""@en ;
    skos:inScheme <https://www.ica.org/standards/RiC/vocabularies/recordSetTypes> ;
    skos:topConceptOf <https://www.ica.org/standards/RiC/vocabularies/recordSetTypes> ;
.

ric-rst:File
    a
        owl:NamedIndividual ,
        skos:Concept ,
        :RecordSetType ;
    rdfs:label
        "file"@en ,
        "expediente"@es ,
        "dossier"@fr ;
    skos:changeNote
        [
            dc:date "2023-11-25" ;
            rdf:value "Added a new rdfs:label in Spanish."@en ;
        ] ,
        [
            dc:date "2023-08-28" ;
            rdf:value "Added a new rdfs:label in French."@en ;
        ] ;
    skos:definition """An organized unit of documents grouped together either for
         current use by the creator or in the process of archival arrangement, because they relate
         to the same subject, activity, or transaction. A file is usually the basic unit within a
         record series. (From ICA ISAD(G))"""@en ;
    skos:inScheme <https://www.ica.org/standards/RiC/vocabularies/recordSetTypes> ;
    skos:topConceptOf <https://www.ica.org/standards/RiC/vocabularies/recordSetTypes> ;
.

ric-rst:Fonds
    a
        owl:NamedIndividual ,
        skos:Concept ,
        :RecordSetType ;
    rdfs:label
        "fonds"@en ,
        "fondo"@es ,
        "fonds"@fr ;
    skos:changeNote
        [
            dc:date "2023-08-28" ;
            rdf:value "Added a new rdfs:label in French."@en ;
        ] ,
        [
            dc:date "2023-11-25" ;
            rdf:value "Added a new rdfs:label in Spanish."@en ;
        ] ;
    skos:definition """The whole of the records, regardless of form or medium,
         organically created and/or accumulated and used by a particular person, family, or
         corporate body in the course of that creator's activities and functions. (From ICA
         ISAD(G))"""@en ;
    skos:inScheme <https://www.ica.org/standards/RiC/vocabularies/recordSetTypes> ;
    skos:topConceptOf <https://www.ica.org/standards/RiC/vocabularies/recordSetTypes> ;
.

ric-rst:Series
    a
        owl:NamedIndividual ,
        skos:Concept ,
        :RecordSetType ;
    rdfs:label
        "series"@en ,
        "serie"@es ,
        "série organique"@fr ;
    skos:changeNote
        [
            dc:date "2023-11-25" ;
            rdf:value "Added a new rdfs:label in Spanish."@en ;
        ] ,
        [
            dc:date "2023-08-28" ;
            rdf:value "Added a new rdfs:label in French."@en ;
        ] ;
    skos:definition """Documents arranged in accordance with a filing system or
         maintained as a unit because they result from the same accumulation or filing process, or
         the same activity; have a particular form; or because of some other relationship arising
         out of their creation, receipt, or use. A series is also known as a records series. (From
         ICA ISAD(G))"""@en ;
    skos:inScheme <https://www.ica.org/standards/RiC/vocabularies/recordSetTypes> ;
    skos:topConceptOf <https://www.ica.org/standards/RiC/vocabularies/recordSetTypes> ;
.

skos:ConceptScheme
    a owl:Class ;
    rdfs:isDefinedBy <http://www.w3.org/2004/02/skos/core> ;
.

:AccumulationRelation
    a owl:Class ;
    rdfs:label
        "Accumulation Relation"@en ,
        "Relación de acumulación"@es ,
        "Relation d’accumulation"@fr ;
    rdfs:comment """Connects at least one Record Resource or Instantiation to at least
         one Agent, when the Record Resource or Instantiation is or was accumulated by the Agent, be
         it intentionally (collecting it) or not (receiving it in the course of its activities). The
         Record Resource(s) or Instantiation(s) is the source of the Relation, and the Agent(s) is
         the target."""@en ;
    rdfs:isDefinedBy <https://www.ica.org/standards/RiC/ontology> ;
    rdfs:subClassOf
        [
            a owl:Restriction ;
            owl:minQualifiedCardinality "1"^^xsd:nonNegativeInteger ;
            owl:onClass
                [
                    a owl:Class ;
                    owl:unionOf (
                        :Instantiation
                        :RecordResource
                    ) ;
                ] ;
            owl:onProperty :relationHasSource ;
        ] ,
        [
            a owl:Restriction ;
            owl:minQualifiedCardinality "1"^^xsd:nonNegativeInteger ;
            owl:onClass :Agent ;
            owl:onProperty :relationHasTarget ;
        ] ,
        :OrganicProvenanceRelation ;
    owl:equivalentClass
        [
            a owl:Restriction ;
            owl:hasSelf true ;
            owl:onProperty :accumulationRelation_role ;
        ] ;
    skos:changeNote
        [
            dc:date "2023-11-08" ;
            rdf:value """In order to get a system of rolified Relation classes: added an
               equivalentClass object property; replaced the specific object properties by the
               generic ones in the subClassOf declarations."""@en ;
        ] ,
        [
            dc:date "2023-08-25" ;
            rdf:value "Added a new rdfs:label in French."@en ;
        ] ,
        [
            dc:date "2023-11-02" ;
            rdf:value "Added a new rdfs:label in Spanish."@en ;
        ] ,
        [
            dc:date "2023-12-06" ;
            rdf:value """Improved the description of the Relation class (rdfs:comment)
               by clearly specifying how it is directed."""@en ;
        ] ,
        [
            dc:date "2023-11-12" ;
            rdf:value """Aligned with RiC-CM 1.0: updated the description
               (rdfs:comment)."""@en ;
        ] ;
    :RiCCMCorrespondingComponent """Class implementation of RiC-R028 and RiC-R028i
         relations"""@en ;
.

:ActivityDocumentationRelation
    a owl:Class ;
    rdfs:label
        "Activity Documentation Relation"@en ,
        "Relación de procedencia funcional"@es ,
        "Relation entre activités et ressources archivistiques"@fr ;
    rdfs:comment """Connects at least one Record Resource or Instantiation to at least
         one Activity, when the Record Resource or Instantiation results from the Activity. The
         Record Resource(s) or Instantiation(s) is the source of the Relation, and the
         Activity(-ies) is the target."""@en ;
    rdfs:isDefinedBy <https://www.ica.org/standards/RiC/ontology> ;
    rdfs:subClassOf
        [
            a owl:Restriction ;
            owl:minQualifiedCardinality "1"^^xsd:nonNegativeInteger ;
            owl:onClass
                [
                    a owl:Class ;
                    owl:unionOf (
                        :Instantiation
                        :RecordResource
                    ) ;
                ] ;
            owl:onProperty :relationHasSource ;
        ] ,
        [
            a owl:Restriction ;
            owl:minQualifiedCardinality "1"^^xsd:nonNegativeInteger ;
            owl:onClass :Activity ;
            owl:onProperty :relationHasTarget ;
        ] ,
        :EventRelation ,
        :OrganicOrFunctionalProvenanceRelation ;
    owl:equivalentClass
        [
            a owl:Restriction ;
            owl:hasSelf true ;
            owl:onProperty :activityDocumentationRelation_role ;
        ] ;
    skos:changeNote
        [
            dc:date "2023-11-12" ;
            rdf:value "Aligned with RiC-CM 1.0: updated the ."@en ;
        ] ,
        [
            dc:date "2023-11-02" ;
            rdf:value "Added a new rdfs:label in Spanish."@en ;
        ] ,
        [
            dc:date "2023-12-06" ;
            rdf:value """Improved the description of the Relation class (rdfs:comment)
               by clearly specifying how it is directed."""@en ;
        ] ,
        [
            dc:date "2023-11-08" ;
            rdf:value """In order to get a system of rolified Relation classes: added an
               equivalentClass object property; replaced the specific object properties by the
               generic ones in the subClassOf declarations."""@en ;
        ] ,
        [
            dc:date "2023-08-25" ;
            rdf:value "Added a new rdfs:label in French."@en ;
        ] ,
        [
            dc:date "2023-11-08" ;
            rdf:value "Made this relation a subclass of EventRelation."@en ;
        ] ;
    :RiCCMCorrespondingComponent """Class implementation of RiC-R033 and RiC-R033
         relations"""@en ;
.

:AgentName
    a owl:Class ;
    rdfs:label
        "Agent Name"@en ,
        "Nombre de Agente"@es ,
        "Nom d’agent"@fr ;
    rdfs:comment """A label, title or term designating an Agent in order to make it
         distinguishable from other similar entities."""@en ;
    rdfs:isDefinedBy <https://www.ica.org/standards/RiC/ontology> ;
    rdfs:subClassOf :Name ;
    skos:changeNote
        [
            dc:date "2023-08-25" ;
            rdf:value "Added a new rdfs:label in French."@en ;
        ] ,
        [
            dc:date "2023-11-02" ;
            rdf:value "Added a new rdfs:label in Spanish."@en ;
        ] ;
    :RiCCMCorrespondingComponent """Class implementation of a specialization of RiC-A28
         (Name attribute)"""@en ;
.

:AppellationRelation
    a owl:Class ;
    rdfs:label
        "Appellation Relation"@en ,
        "Relación de denominación"@es ,
        "Relation d’appellation"@fr ;
    rdfs:comment """Connects an Appellation and at least one Thing that the
         Appellation designates or designated. The Appellation is the source of the Relation and the
         Thing(s) is the target."""@en ;
    rdfs:isDefinedBy <https://www.ica.org/standards/RiC/ontology> ;
    rdfs:subClassOf
        [
            a owl:Restriction ;
            owl:minQualifiedCardinality "1"^^xsd:nonNegativeInteger ;
            owl:onClass :Thing ;
            owl:onProperty :relationHasTarget ;
        ] ,
        [
            a owl:Restriction ;
            owl:onClass :Appellation ;
            owl:onProperty :relationHasSource ;
            owl:qualifiedCardinality "1"^^xsd:nonNegativeInteger ;
        ] ,
        :Relation ;
    owl:equivalentClass
        [
            a owl:Restriction ;
            owl:hasSelf true ;
            owl:onProperty :appellationRelation_role ;
        ] ;
    skos:changeNote
        [
            dc:date "2023-11-08" ;
            rdf:value """In order to get a system of rolified Relation classes: added an
               equivalentClass object property; replaced the specific object properties by the
               generic ones in the subClassOf declarations."""@en ;
        ] ,
        [
            dc:date "2023-12-06" ;
            rdf:value """Improved the description of the Relation class (rdfs:comment)
               by clearly specifying how it is directed."""@en ;
        ] ,
        [
            dc:date "2023-08-25" ;
            rdf:value "Added a new rdfs:label in French."@en ;
        ] ,
        [
            dc:date "2023-11-02" ;
            rdf:value "Added a new rdfs:label in Spanish."@en ;
        ] ,
        [
            dc:date "2023-11-12" ;
            rdf:value """Aligned with RiC-CM 1.0: updated the description
               (rdfs:comment)."""@en ;
        ] ;
.

:AuthorshipRelation
    a owl:Class ;
    rdfs:label
        "Authorship Relation"@en ,
        "Relación de autoría"@es ,
        "Relation de responsabilité intellectuelle"@fr ;
    rdfs:comment """Connects at least one Record to at least one Person, Group or
         Position that is or was responsible for conceiving and formulating the information
         contained in the Record. The Record is the source of the Relation and the Person(s),
         Group(s) or Position(s) is the target. """@en ;
    rdfs:isDefinedBy <https://www.ica.org/standards/RiC/ontology> ;
    rdfs:subClassOf
        [
            a owl:Restriction ;
            owl:minQualifiedCardinality "1"^^xsd:nonNegativeInteger ;
            owl:onClass
                [
                    a owl:Class ;
                    owl:unionOf (
                        :Group
                        :Person
                        :Position
                    ) ;
                ] ;
            owl:onProperty :relationHasTarget ;
        ] ,
        [
            a owl:Restriction ;
            owl:minQualifiedCardinality "1"^^xsd:nonNegativeInteger ;
            owl:onClass :Record ;
            owl:onProperty :relationHasSource ;
        ] ,
        :CreationRelation ;
    owl:equivalentClass
        [
            a owl:Restriction ;
            owl:hasSelf true ;
            owl:onProperty :authorshipRelation_role ;
        ] ;
    skos:changeNote
        [
            dc:date "2023-12-06" ;
            rdf:value """Improved the description of the Relation class (rdfs:comment)
               by clearly specifying how it is directed."""@en ;
        ] ,
        [
            dc:date "2020-12-29" ;
            rdf:value """Created following the addition of RiC-R079 relation in RiC-CM
               0.2"""@en ;
        ] ,
        [
            dc:date "2023-11-12" ;
            rdf:value """Aligned with RiC-CM 1.0: updated the description
               (rdfs:comment), skos:scopeNote."""@en ;
        ] ,
        [
            dc:date "2023-08-25" ;
            rdf:value "Added a new rdfs:label in French."@en ;
        ] ,
        [
            dc:date "2023-11-02" ;
            rdf:value "Added a new rdfs:label in Spanish."@en ;
        ] ,
        [
            dc:date "2023-11-08" ;
            rdf:value """In order to get a system of rolified Relation classes: added an
               equivalentClass object property; replaced the specific object properties by the
               generic ones in the subClassOf declarations."""@en ;
        ] ;
    skos:scopeNote """To be used for a person, group or position that makes any
         contribution to the content of a record. Includes the person, group or position in whose
         name or by whose command the content may have been formulated and first instantiated (for
         example the person who signed the record). """@en ;
    :RiCCMCorrespondingComponent """Class implementation of RiC-R079 and RiC-R079i
         relations"""@en ;
.

:CarrierType
    a owl:Class ;
    rdfs:label
        "Carrier Type"@en ,
        "Tipo de soporte"@es ,
        "Type de support"@fr ;
    rdfs:comment """Categorization of physical material on which information is
         represented."""@en ;
    rdfs:isDefinedBy <https://www.ica.org/standards/RiC/ontology> ;
    rdfs:subClassOf :Type ;
    skos:changeNote
        [
            dc:date "2023-11-02" ;
            rdf:value "Added a new rdfs:label in Spanish."@en ;
        ] ,
        [
            dc:date "2023-08-25" ;
            rdf:value "Added a new rdfs:label in French."@en ;
        ] ,
        [
            dc:date "2023-11-12" ;
            rdf:value """Aligned with RiC-CM 1.0: updated the description
               (rdfs:comment), skos:scopeNote."""@en ;
        ] ,
        [
            dc:date "2023-04-19" ;
            rdf:value "Removed the 0.2 existing unnecessary restriction."@en ;
        ] ,
        [
            dc:date "2020-10-23" ;
            rdf:value """Scope note: updated (quite the same as RiC-CM definition).
               Objective: to make RiC-O compliant with RiC-CM v0.2."""@en ;
        ] ;
    skos:scopeNote """In order to manage an instantiation of a record resource, it is
         necessary to note the type of carrier on which the record resource is instantiated as its
         nature will determine the environmental storage conditions and the prerequisites for and
         possible ways of accessing and using the record resource."""@en ;
    :RiCCMCorrespondingComponent """Corresponds to RiC-A05 (Carrier Type
         attribute)"""@en ;
.

:ChildRelation
    a owl:Class ;
    rdfs:label
        "Child Relation"@en ,
        "Relación de filiación"@es ,
        "Relation de filiation"@fr ;
    rdfs:comment """Connects at least one Person to at least another Person, when the
         first has(ave) child(s) the second one(s). The Relation is oriented from the parent to the
         child: the parent is the source of the relation, and the child(ren) is the
         target."""@en ;
    rdfs:isDefinedBy <https://www.ica.org/standards/RiC/ontology> ;
    rdfs:subClassOf
        [
            a owl:Restriction ;
            owl:minQualifiedCardinality "1"^^xsd:nonNegativeInteger ;
            owl:onClass :Person ;
            owl:onProperty :relationHasSource ;
        ] ,
        [
            a owl:Restriction ;
            owl:minQualifiedCardinality "1"^^xsd:nonNegativeInteger ;
            owl:onClass :Person ;
            owl:onProperty :relationHasTarget ;
        ] ,
        :DescendanceRelation ;
    owl:equivalentClass
        [
            a owl:Restriction ;
            owl:hasSelf true ;
            owl:onProperty :childRelation_role ;
        ] ;
    skos:changeNote
        [
            dc:date "2023-11-02" ;
            rdf:value "Added a new rdfs:label in Spanish."@en ;
        ] ,
        [
            dc:date "2023-08-25" ;
            rdf:value "Added a new rdfs:label in French."@en ;
        ] ,
        [
            dc:date "2023-11-08" ;
            rdf:value """In order to get a system of rolified Relation classes: added an
               equivalentClass object property; replaced the specific object properties by the
               generic ones in the subClassOf declarations."""@en ;
        ] ,
        [
            dc:date "2023-12-06" ;
            rdf:value """Improved the description of the Relation class (rdfs:comment)
               by clearly specifying how it is directed."""@en ;
        ] ,
        [
            dc:date "2023-11-12" ;
            rdf:value """Aligned with RiC-CM 1.0: updated the description
               (rdfs:comment)."""@en ;
        ] ;
    :RiCCMCorrespondingComponent """Class implementation of RiC-R018 and RiC-R018i
         relations"""@en ;
.

:CorporateBodyType
    a owl:Class ;
    rdfs:label
        "Corporate Body Type"@en ,
        "Tipo de institución"@es ,
        "Type de collectivité"@fr ;
    rdfs:comment "Categorization of a Corporate Body."@en ;
    rdfs:isDefinedBy <https://www.ica.org/standards/RiC/ontology> ;
    rdfs:subClassOf :Type ;
    skos:changeNote
        [
            dc:date "2023-04-19" ;
            rdf:value "Removed the 0.2 existing unnecessary restriction."@en ;
        ] ,
        [
            dc:date "2023-11-02" ;
            rdf:value "Added a new rdfs:label in Spanish."@en ;
        ] ,
        [
            dc:date "2023-08-25" ;
            rdf:value "Added a new rdfs:label in French."@en ;
        ] ;
    :RiCCMCorrespondingComponent """Corresponds to RiC-A12 (Corporate Body Type
         attribute)"""@en ;
.

:CorrespondenceRelation
    a owl:Class ;
    rdfs:label
        "Correspondence Relation"@en ,
        "Relación entre personas por correspondencia"@es ,
        "Relation épistolaire"@fr ;
    rdfs:comment """Connects at least two Persons, when they correspond or
         corresponded to each other. This Relation is not oriented."""@en ;
    rdfs:isDefinedBy <https://www.ica.org/standards/RiC/ontology> ;
    rdfs:subClassOf
        [
            a owl:Restriction ;
            owl:minQualifiedCardinality "2"^^xsd:nonNegativeInteger ;
            owl:onClass :Person ;
            owl:onProperty :relationConnects ;
        ] ,
        :KnowingRelation ;
    owl:equivalentClass
        [
            a owl:Restriction ;
            owl:hasSelf true ;
            owl:onProperty :correspondenceRelation_role ;
        ] ;
    skos:changeNote
        [
            dc:date "2023-11-12" ;
            rdf:value """Aligned with RiC-CM 1.0: updated the description
               (rdfs:comment)."""@en ;
        ] ,
        [
            dc:date "2023-11-02" ;
            rdf:value "Added a new rdfs:label in Spanish."@en ;
        ] ,
        [
            dc:date "2023-11-08" ;
            rdf:value """In order to get a system of rolified Relation classes: added an
               equivalentClass object property; replaced the specific object properties by the
               generic ones in the subClassOf declarations."""@en ;
        ] ,
        [
            dc:date "2023-08-25" ;
            rdf:value "Added a new rdfs:label in French."@en ;
        ] ,
        [
            dc:date "2023-12-06" ;
            rdf:value """Improved the description of the Relation class (rdfs:comment)
               by clearly specifying how it is directed."""@en ;
        ] ;
    :RiCCMCorrespondingComponent """Class implementation of RiC-R052 and Ri052i
         relations"""@en ;
.

:DateType
    a owl:Class ;
    rdfs:label
        "Date Type"@en ,
        "Tipo de fecha"@es ,
        "Type de date"@fr ;
    rdfs:comment "Categorization of a Date."@en ;
    rdfs:isDefinedBy <https://www.ica.org/standards/RiC/ontology> ;
    rdfs:subClassOf :Type ;
    skos:changeNote
        [
            dc:date "2023-09-22"@en ;
            rdf:value "Added in RiC-O 1.0."@en ;
        ] ,
        [
            dc:date "2023-11-12" ;
            rdf:value """Aligned with RiC-CM 1.0: updated the description
               (rdfs:comment), skos:scopeNote. Added a label in Spanish."""@en ;
        ] ,
        [
            dc:date "2023-10-10" ;
            rdf:value """Added the rdfs:comment, a French rdfs:label, and adjusted the
               rico:RiCCMCorrespondingComponent annotation."""@en ;
        ] ;
    skos:scopeNote """May be used to categorize a Date as a single date, a date range
         or a date set or sub-categories of these broad types. This attribute should not be confused
         with the date relations defined to connect a Date entity and any other entity (such as
         RiC-R069 ‘is beginning date of’)."""@en ;
    :RiCCMCorrespondingComponent """Corresponds to RiC-A42 (Date Type attribute) (new
         in RiC-CM 1.0)."""@en ;
.

:EventType
    a owl:Class ;
    rdfs:label
        "Event Type"@en ,
        "Tipo de evento"@es ,
        "Type d’événement"@fr ;
    rdfs:comment "Categorization of an Event."@en ;
    rdfs:isDefinedBy <https://www.ica.org/standards/RiC/ontology> ;
    rdfs:subClassOf :Type ;
    skos:changeNote
        [
            dc:date "2023-08-25" ;
            rdf:value "Added a new rdfs:label in French."@en ;
        ] ,
        [
            dc:date "2023-11-02" ;
            rdf:value "Added a new rdfs:label in Spanish."@en ;
        ] ,
        [
            dc:date "2023-04-19" ;
            rdf:value "Removed the 0.2 existing unnecessary restriction."@en ;
        ] ,
        [
            dc:date "2023-11-12" ;
            rdf:value """Aligned with RiC-CM 1.0: updated the
               skos:scopeNote."""@en ;
        ] ,
        [
            dc:date "2020-10-23" ;
            rdf:value """Scope note: updated and made several paragraphs. Objective: to
               make RiC-O compliant with RiC-CM v0.2."""@en ;
        ] ;
    skos:scopeNote """Events of all kinds can be categorized. Curation event types
         include creation; acquisition; transfer; arrangement; description; digitization, etc.
         Biographical event types include birth, marriage, death, etc."""@en ;
    :RiCCMCorrespondingComponent """Corresponds to RiC-A18 (Event Type
         attribute)"""@en ;
.

:ExtentType
    a owl:Class ;
    rdfs:label
        "Extent Type"@en ,
        "Tipo de Extensión"@es ,
        "Type de mesure"@fr ;
    rdfs:comment """Categorization of the extent that is being
         measured."""@en ;
    rdfs:isDefinedBy <https://www.ica.org/standards/RiC/ontology> ;
    rdfs:subClassOf :Type ;
    skos:changeNote
        [
            dc:date "2023-08-25" ;
            rdf:value "Added a new rdfs:label in French."@en ;
        ] ,
        [
            dc:date "2023-08-28" ;
            rdf:value "Added an xml:lang attribute to the rdfs:comment."@en ;
        ] ,
        [
            dc:date "2023-11-02" ;
            rdf:value "Added a new rdfs:label in Spanish."@en ;
        ] ,
        [
            dc:date "2020-11-01" ;
            rdf:value """Added to specify the dimension that is being
               measured"""@en ;
        ] ;
.

:Family
    a owl:Class ;
    rdfs:label
        "Family"@en ,
        "Familia"@es ,
        "Famille"@fr ;
    rdfs:comment """Two or more persons related by birth, or through marriage,
         adoption, civil union, or other social conventions that bind them together as a socially
         recognized familial group."""@en ;
    rdfs:isDefinedBy <https://www.ica.org/standards/RiC/ontology> ;
    rdfs:subClassOf :Group ;
    skos:changeNote
        [
            dc:date "2020-10-23" ;
            rdf:value """Scope note: made separate paragraphs and some
               changes."""@en ;
        ] ,
        [
            dc:date "2023-08-25" ;
            rdf:value "Added a new rdfs:label in French."@en ;
        ] ,
        [
            dc:date "2023-11-02" ;
            rdf:value "Added a new rdfs:label in Spanish."@en ;
        ] ;
    skos:scopeNote """Family is a kind of Group. “Family” is used here as a general
         term that encompasses a wide variety of familial groups. Other types of familial groups
         include Dynasty, Clan, House, Tribe and others. Though family may be a recognized legal
         group in specific contexts, the term may also be used for groups that are socially
         recognized as families. A family may be a group of persons related either by consanguinity
         or affinity or cohabitation or other social conventions. In some context, a Family may be
         legally recognized as Corporate Body. For example, certain North American peoples (tribes)
         retain self-government rights and have jurisdiction over defined tribal
         lands."""@en ;
    :RiCCMCorrespondingComponent """Corresponds to RiC-E10 (Family
         entity)"""@en ;
.

:FamilyType
    a owl:Class ;
    rdfs:label
        "Family Type"@en ,
        "Tipo de familia"@es ,
        "Type de famille"@fr ;
    rdfs:comment "Categorization of a Family."@en ;
    rdfs:isDefinedBy <https://www.ica.org/standards/RiC/ontology> ;
    rdfs:subClassOf :Type ;
    skos:changeNote
        [
            dc:date "2023-04-19" ;
            rdf:value "Removed the 0.2 existing unnecessary restriction."@en ;
        ] ,
        [
            dc:date "2020-10-23" ;
            rdf:value "Comment: slighty changed."@en ;
        ] ,
        [
            dc:date "2023-11-02" ;
            rdf:value "Added a new rdfs:label in Spanish."@en ;
        ] ,
        [
            dc:date "2023-08-25" ;
            rdf:value "Added a new rdfs:label in French."@en ;
        ] ,
        [
            dc:date "2023-11-12" ;
            rdf:value """Aligned with RiC-CM 1.0: updated the
               skos:scopeNote."""@en ;
        ] ;
    skos:scopeNote """Encompasses a wide variety of familial groups related by
         consanguinity, affinity, cohabitation, or other social conventions."""@en ;
    :RiCCMCorrespondingComponent """Corresponds to RiC-A20 (Family Type
         attribute)"""@en ;
.

:FunctionalEquivalenceRelation
    a owl:Class ;
    rdfs:label
        "Functional Equivalence Relation"@en ,
        "Relación de equivalencia funcional"@es ,
        "Relation d’équivalence fonctionnelle"@fr ;
    rdfs:comment """Connects at least two Instantiations which may be considered as
         equivalent. This Relation is not oriented."""@en ;
    rdfs:isDefinedBy <https://www.ica.org/standards/RiC/ontology> ;
    rdfs:subClassOf
        [
            a owl:Restriction ;
            owl:minQualifiedCardinality "2"^^xsd:nonNegativeInteger ;
            owl:onClass :Instantiation ;
            owl:onProperty :relationConnects ;
        ] ,
        :InstantiationToInstantiationRelation ;
    owl:equivalentClass
        [
            a owl:Restriction ;
            owl:hasSelf true ;
            owl:onProperty :functionalEquivalenceRelation_role ;
        ] ;
    skos:changeNote
        [
            dc:date "2023-11-12" ;
            rdf:value """Aligned with RiC-CM 1.0: updated the
               skos:scopeNote."""@en ;
        ] ,
        [
            dc:date "2023-12-06" ;
            rdf:value """Improved the description of the Relation class (rdfs:comment)
               by clearly specifying how it is directed."""@en ;
        ] ,
        [
            dc:date "2023-08-25" ;
            rdf:value "Added a new rdfs:label in French."@en ;
        ] ,
        [
            dc:date "2023-11-08" ;
            rdf:value """In order to get a system of rolified Relation classes: added an
               equivalentClass object property; replaced the specific object properties by the
               generic ones in the subClassOf declarations."""@en ;
        ] ,
        [
            dc:date "2023-11-02" ;
            rdf:value "Added a new rdfs:label in Spanish."@en ;
        ] ;
    skos:scopeNote """Two instantiations, from some point of view, may be considered
         as equivalent. This equivalence is usually based upon the fact that the instantiations have
         at least the same intellectual content (they instantiate the same record
         resource)."""@en ;
    :RiCCMCorrespondingComponent """Class implementation of RiC-R035 and RiC-R035i
         relations"""@en ;
.

:GroupSubdivisionRelation
    a owl:Class ;
    rdfs:label
        "Group Subdivision Relation"@en ,
        "Relación de subdivisión entre grupos de agentes"@es ,
        "Relation de subdivision entre groupes d’agents"@fr ;
    rdfs:comment """Connects a Group and at least another Group, when the first one
         has or had the second one(s) among its subdivisions. The Relation is oriented from the
         Group to its subdivision(s): the parent Group is the source and the subdivision Group(s) is
         the target."""@en ;
    rdfs:isDefinedBy <https://www.ica.org/standards/RiC/ontology> ;
    rdfs:subClassOf
        [
            a owl:Restriction ;
            owl:minQualifiedCardinality "1"^^xsd:nonNegativeInteger ;
            owl:onClass :Group ;
            owl:onProperty :relationHasTarget ;
        ] ,
        [
            a owl:Restriction ;
            owl:onClass :Group ;
            owl:onProperty :relationHasSource ;
            owl:qualifiedCardinality "1"^^xsd:nonNegativeInteger ;
        ] ,
        :AgentHierarchicalRelation ,
        :WholePartRelation ;
    owl:equivalentClass
        [
            a owl:Restriction ;
            owl:hasSelf true ;
            owl:onProperty :groupSubdivisionRelation_role ;
        ] ;
    skos:changeNote
        [
            dc:date "2023-08-25" ;
            rdf:value "Added a new rdfs:label in French."@en ;
        ] ,
        [
            dc:date "2023-11-12" ;
            rdf:value """Aligned with RiC-CM 1.0: updated the description
               (rdfs:comment)."""@en ;
        ] ,
        [
            dc:date "2023-11-08" ;
            rdf:value """In order to get a system of rolified Relation classes: added an
               equivalentClass object property; replaced the specific object properties by the
               generic ones in the subClassOf declarations."""@en ;
        ] ,
        [
            dc:date "2023-12-06" ;
            rdf:value """Improved the description of the Relation class (rdfs:comment)
               by clearly specifying how it is directed."""@en ;
        ] ,
        [
            dc:date "2023-11-02" ;
            rdf:value "Added a new rdfs:label in Spanish."@en ;
        ] ;
    :RiCCMCorrespondingComponent """Class implementation of RiC-R005 and RiC-R005i
         relations"""@en ;
.

:IdentifierType
    a owl:Class ;
    rdfs:label
        "Identifier Type"@en ,
        "Tipo de identificador"@es ,
        "Type d’identifiant"@fr ;
    rdfs:comment "Categorization of an Identifier."@en ;
    rdfs:isDefinedBy <https://www.ica.org/standards/RiC/ontology> ;
    rdfs:subClassOf :Type ;
    skos:changeNote
        [
            dc:date "2023-11-02" ;
            rdf:value "Added a new rdfs:label in Spanish."@en ;
        ] ,
        [
            dc:date "2023-04-19" ;
            rdf:value "Removed the 0.2 existing unnecessary restriction."@en ;
        ] ,
        [
            dc:date "2020-10-19" ;
            rdf:value """Class added along with hasIdentifierType and isIdentifierTypeOf
               object properties."""@en ;
        ] ,
        [
            dc:date "2023-08-25" ;
            rdf:value "Added a new rdfs:label in French."@en ;
        ] ;
    skos:scopeNote """For example, 'old identifier' ; 'ISNI' (for a person or
         corporate body), etc."""@en ;
.

:IntellectualPropertyRightsRelation
    a owl:Class ;
    rdfs:label
        "Intellectual Property Rights Relation"@en ,
        "Relación de propiedad intelectual"@es ,
        "Relation de propriété intellectuelle"@fr ;
    rdfs:comment """Connects at least one Agent and one Record Resource or
         Instantiation on which the Agent has or had some intellectual property rights. The Agent(s)
         is the source of the Relation and the Record Resource(s) or Instantiation(s) is the
         target."""@en ;
    rdfs:isDefinedBy <https://www.ica.org/standards/RiC/ontology> ;
    rdfs:subClassOf
        [
            a owl:Restriction ;
            owl:minQualifiedCardinality "1"^^xsd:nonNegativeInteger ;
            owl:onClass
                [
                    a owl:Class ;
                    owl:unionOf (
                        :Instantiation
                        :RecordResource
                    ) ;
                ] ;
            owl:onProperty :relationHasTarget ;
        ] ,
        [
            a owl:Restriction ;
            owl:minQualifiedCardinality "1"^^xsd:nonNegativeInteger ;
            owl:onClass
                [
                    a owl:Class ;
                    owl:unionOf (
                        :Group
                        :Person
                        :Position
                    ) ;
                ] ;
            owl:onProperty :relationHasSource ;
        ] ,
        :AuthorityRelation ;
    owl:equivalentClass
        [
            a owl:Restriction ;
            owl:hasSelf true ;
            owl:onProperty :intellectualPropertyRightsRelation_role ;
        ] ;
    skos:changeNote
        [
            dc:date "2023-12-06" ;
            rdf:value """Improved the description of the Relation class (rdfs:comment)
               by clearly specifying how it is directed."""@en ;
        ] ,
        [
            dc:date "2023-11-08" ;
            rdf:value """In order to get a system of rolified Relation classes: added an
               equivalentClass object property; replaced the specific object properties by the
               generic ones in the subClassOf declarations."""@en ;
        ] ,
        [
            dc:date "2023-11-02" ;
            rdf:value "Added a new rdfs:label in Spanish."@en ;
        ] ,
        [
            dc:date "2023-08-25" ;
            rdf:value "Added a new rdfs:label in French."@en ;
        ] ,
        [
            dc:date "2023-11-12" ;
            rdf:value """Aligned with RiC-CM 1.0: updated the description
               (rdfs:comment)."""@en ;
        ] ;
    skos:scopeNote """Can be used, when the record resource is a work, for specifying
         the connection between the record resource and its author(s)."""@en ;
    :RiCCMCorrespondingComponent """Class implementation of RiC-R040 and RiC-R040i
         relations"""@en ;
.

:KnowingOfRelation
    a owl:Class ;
    rdfs:label
        "Knowing Of Relation"@en ,
        "Relación de conocimieto indirecto entre personas"@es ,
        "Relation de connaissance à propos d’une personne"@fr ;
    rdfs:comment """Connects at least one Person to at least another one, when the
         first one has some knowledge of the second one through time or space. The first Person is
         the source of the Relation, and the second one is the target."""@en ;
    rdfs:isDefinedBy <https://www.ica.org/standards/RiC/ontology> ;
    rdfs:subClassOf
        [
            a owl:Restriction ;
            owl:minQualifiedCardinality "1"^^xsd:nonNegativeInteger ;
            owl:onClass :Person ;
            owl:onProperty :relationHasSource ;
        ] ,
        [
            a owl:Restriction ;
            owl:minQualifiedCardinality "1"^^xsd:nonNegativeInteger ;
            owl:onClass :Person ;
            owl:onProperty :relationHasTarget ;
        ] ,
        :AgentToAgentRelation ;
    owl:equivalentClass
        [
            a owl:Restriction ;
            owl:hasSelf true ;
            owl:onProperty :knowingOfRelation_role ;
        ] ;
    skos:changeNote
        [
            dc:date "2023-11-02" ;
            rdf:value "Added a new rdfs:label in Spanish."@en ;
        ] ,
        [
            dc:date "2023-12-06" ;
            rdf:value """Improved the description of the Relation class (rdfs:comment)
               by clearly specifying how it is directed."""@en ;
        ] ,
        [
            dc:date "2023-08-25" ;
            rdf:value "Added a new rdfs:label in French."@en ;
        ] ,
        [
            dc:date "2023-11-08" ;
            rdf:value """In order to get a system of rolified Relation classes: added an
               equivalentClass object property; replaced the specific object properties by the
               generic ones in the subClassOf declarations."""@en ;
        ] ;
    :RiCCMCorrespondingComponent """Class implementation of RiC-R050 and RiC-R050i
         relations"""@en ;
.

:MandateType
    a owl:Class ;
    rdfs:label
        "Mandate Type"@en ,
        "Tipo de norma"@es ,
        "Type de mandat"@fr ;
    rdfs:comment "Categorization of a Mandate."@en ;
    rdfs:isDefinedBy <https://www.ica.org/standards/RiC/ontology> ;
    rdfs:subClassOf :RuleType ;
    skos:changeNote
        [
            dc:date "2023-11-12" ;
            rdf:value """Added in RiC-0 1.0 as it has been added to RiC-CM
               1.0."""@en ;
        ] ;
    skos:scopeNote """For example : charter, treaty, contract, letter of appointment,
         papal mandate, episcopal mandate, ciurt mandate, election mandate, popular mandate, federal
         mandate, etc."""@en ;
    :RiCCMCorrespondingComponent """Corresponds to RiC-A44 (Mandate Type
         attribute)."""@en ;
.

:Mechanism
    a owl:Class ;
    rdfs:label
        "Mechanism"@en ,
        "Mecanismo"@es ,
        "Système"@fr ;
    rdfs:comment """A process or system created by a Person or Group that performs an
         Activity."""@en ;
    rdfs:isDefinedBy <https://www.ica.org/standards/RiC/ontology> ;
    rdfs:subClassOf :Agent ;
    owl:disjointWith
        :Person ,
        :Position ;
    skos:changeNote
        [
            dc:date "2023-11-02" ;
            rdf:value "Added a new rdfs:label in Spanish."@en ;
        ] ,
        [
            dc:date "2023-08-25" ;
            rdf:value "Added a new rdfs:label in French."@en ;
        ] ,
        [
            dc:date "2023-11-12" ;
            rdf:value """Aligned with RiC-CM 1.0: updated the
               skos:scopeNote."""@en ;
        ] ,
        [
            dc:date "2020-10-23" ;
            rdf:value """scope note: made separate paragraphs. Disjoint with:
               enriched."""@en ;
        ] ;
    skos:scopeNote """Mechanism is a kind of Agent. A mechanism may have both
         mechanical and software components or may be exclusively software. A mechanism acts in the
         world producing physical or social effects and may generate or modify records. A mechanism
         performs activities based on rules determined by the agent that designed and created it. A
         mechanism has an essential, derivative relation with the designing and creating
         agent."""@en ;
    :RiCCMCorrespondingComponent """Corresponds to RiC-E13 (Mechanism
         entity)"""@en ;
.

:MigrationRelation
    a owl:Class ;
    rdfs:label
        "Migration Relation"@en ,
        "Relación de migración entre instanciaciones"@es ,
        "Relation de migration"@fr ;
    rdfs:comment """Connects an Instantiation and at least another Instantiation it
         has been migrated into. The Relation is oriented chronologically, from the first
         Instantiation in time (the migrated one) to the one which results from its migration: the
         first Instantiation in time is the source of the Relation, and the resulting Instantiation
         is the target."""@en ;
    rdfs:isDefinedBy <https://www.ica.org/standards/RiC/ontology> ;
    rdfs:subClassOf
        [
            a owl:Restriction ;
            owl:minQualifiedCardinality "1"^^xsd:nonNegativeInteger ;
            owl:onClass :Instantiation ;
            owl:onProperty :relationHasTarget ;
        ] ,
        [
            a owl:Restriction ;
            owl:onClass :Instantiation ;
            owl:onProperty :relationHasSource ;
            owl:qualifiedCardinality "1"^^xsd:nonNegativeInteger ;
        ] ,
        :DerivationRelation ;
    owl:equivalentClass
        [
            a owl:Restriction ;
            owl:hasSelf true ;
            owl:onProperty :migrationRelation_role ;
        ] ;
    skos:changeNote
        [
            dc:date "2023-12-06" ;
            rdf:value """Improved the description of the Relation class (rdfs:comment)
               by clearly specifying how it is directed."""@en ;
        ] ,
        [
            dc:date "2023-11-02" ;
            rdf:value "Added a new rdfs:label in Spanish."@en ;
        ] ,
        [
            dc:date "2023-11-08" ;
            rdf:value """In order to get a system of rolified Relation classes: added an
               equivalentClass object property; replaced the specific object properties by the
               generic ones in the subClassOf declarations."""@en ;
        ] ,
        [
            dc:date "2023-11-12" ;
            rdf:value """Aligned with RiC-CM 1.0: updated the description
               (rdfs:comment), skos:scopeNote."""@en ;
        ] ,
        [
            dc:date "2023-08-25" ;
            rdf:value "Added a new rdfs:label in French."@en ;
        ] ;
    skos:scopeNote "Use for digital instantiations."@en ;
    :RiCCMCorrespondingComponent """Class implementation of RiC-R015 and RiC-R015i
         relations"""@en ;
.

:OccupationType
    a owl:Class ;
    rdfs:label
        "Occupation Type"@en ,
        "Tipo de ocupación"@es ,
        "Type d’occupation"@fr ;
    rdfs:comment """Categorization of a profession, trade, or craft pursued by a
         Person in fulfilment of an Activity."""@en ;
    rdfs:isDefinedBy <https://www.ica.org/standards/RiC/ontology> ;
    rdfs:subClassOf
        :ActivityType ,
        :DemographicGroup ;
    skos:changeNote
        [
            dc:date "2023-11-12" ;
            rdf:value """Aligned with RiC-CM 1.0: updated the description
               (rdfs:comment), skos:scopeNote."""@en ;
        ] ,
        [
            dc:date "2023-11-02" ;
            rdf:value "Added a new rdfs:label in Spanish."@en ;
        ] ,
        [
            dc:date "2020-10-23" ;
            rdf:value "scope note: added."@en ;
        ] ,
        [
            dc:date "2023-04-19" ;
            rdf:value "Removed the 0.2 existing unnecessary restriction."@en ;
        ] ,
        [
            dc:date "2023-08-25" ;
            rdf:value "Added a new rdfs:label in French."@en ;
        ] ;
    skos:scopeNote """The pursuit of an occupation involves the performance of an
         Activity. Successful performance of the Activity is based on the ability to perform related
         competencies successfully. Such competencies may be acquired through education or
         experience, or a combination of both. The authority of the Person to pursue the occupation
         may be derived tacitly or explicitly from an external Agent, based on a demonstrated
         mastery of the competency. An occupation may be pursued independently by a Person or a
         Group, thereby contributing to the fulfilment of the function (activity) of the group.
         Should not be confused with Position where, for example, an agent with the occupation type
         "lawyer" holds the position of "legal counsel" in an agency. Related to but should not be
         confused with the domain or field of activity, such as an archivist who works in the domain
         of archival science."""@en ;
    :RiCCMCorrespondingComponent """Corresponds to RiC-A30 (Occupation Type
         attribute)"""@en ;
.

:OwnershipRelation
    a owl:Class ;
    rdfs:label
        "Ownership Relation"@en ,
        "Relación de posesión"@es ,
        "Relation de propriété"@fr ;
    rdfs:comment """Connects at least one Group, Person or Position and at least a
         Thing that these Agent(s) own(s) or owned. The Group(s), Person(s) or Position(s) is the
         source of the Relation, and the Agent(s) is the target."""@en ;
    rdfs:isDefinedBy <https://www.ica.org/standards/RiC/ontology> ;
    rdfs:subClassOf
        [
            a owl:Restriction ;
            owl:minQualifiedCardinality "1"^^xsd:nonNegativeInteger ;
            owl:onClass :Thing ;
            owl:onProperty :relationHasTarget ;
        ] ,
        [
            a owl:Restriction ;
            owl:minQualifiedCardinality "1"^^xsd:nonNegativeInteger ;
            owl:onClass
                [
                    a owl:Class ;
                    owl:unionOf (
                        :Group
                        :Person
                        :Position
                    ) ;
                ] ;
            owl:onProperty :relationHasSource ;
        ] ,
        :AuthorityRelation ;
    owl:equivalentClass
        [
            a owl:Restriction ;
            owl:hasSelf true ;
            owl:onProperty :ownershipRelation_role ;
        ] ;
    skos:changeNote
        [
            dc:date "2023-12-06" ;
            rdf:value """Improved the description of the Relation class (rdfs:comment)
               by clearly specifying how it is directed."""@en ;
        ] ,
        [
            dc:date "2023-08-25" ;
            rdf:value "Added a new rdfs:label in French."@en ;
        ] ,
        [
            dc:date "2023-11-08" ;
            rdf:value """In order to get a system of rolified Relation classes: added an
               equivalentClass object property; replaced the specific object properties by the
               generic ones in the subClassOf declarations."""@en ;
        ] ,
        [
            dc:date "2023-11-02" ;
            rdf:value "Added a new rdfs:label in Spanish."@en ;
        ] ,
        [
            dc:date "2023-11-12" ;
            rdf:value """Aligned with RiC-CM 1.0: updated the description
               (rdfs:comment), skos:scopeNote."""@en ;
        ] ;
    skos:scopeNote """Among other probably more rare use cases for archival
         description, can be used between agents (a person owns a corporate body, a corporate body
         owns a mechanism), or between agents and record resources."""@en ;
    :RiCCMCorrespondingComponent """Class implementation of RiC-R037 and RiC-R037i
         relations"""@en ;
.

:PerformanceRelation
    a owl:Class ;
    rdfs:label
        "Performance Relation"@en ,
        "Relación de desarrollo funcional"@es ,
        "Relation entre activités et agents"@fr ;
    rdfs:comment """Connects at least one Activity to at least one Agent that performs
         or performed the activity. The Activity(-ies) is the source of the Relation and the
         Agent(s) is the target."""@en ;
    rdfs:isDefinedBy <https://www.ica.org/standards/RiC/ontology> ;
    rdfs:subClassOf
        [
            a owl:Restriction ;
            owl:minQualifiedCardinality "1"^^xsd:nonNegativeInteger ;
            owl:onClass :Activity ;
            owl:onProperty :relationHasSource ;
        ] ,
        [
            a owl:Restriction ;
            owl:minQualifiedCardinality "1"^^xsd:nonNegativeInteger ;
            owl:onClass :Agent ;
            owl:onProperty :relationHasTarget ;
        ] ,
        :EventRelation ;
    owl:equivalentClass
        [
            a owl:Restriction ;
            owl:hasSelf true ;
            owl:onProperty :performanceRelation_role ;
        ] ;
    skos:changeNote
        [
            dc:date "2023-11-02" ;
            rdf:value "Added a new rdfs:label in Spanish."@en ;
        ] ,
        [
            dc:date "2023-08-25" ;
            rdf:value "Added a new rdfs:label in French."@en ;
        ] ,
        [
            dc:date "2023-12-06" ;
            rdf:value """Improved the description of the Relation class (rdfs:comment)
               by clearly specifying how it is directed."""@en ;
        ] ,
        [
            dc:date "2023-11-12" ;
            rdf:value """Aligned with RiC-CM 1.0: updated the description
               (rdfs:comment)."""@en ;
        ] ,
        [
            dc:date "2023-11-08" ;
            rdf:value """In order to get a system of rolified Relation classes: added an
               equivalentClass object property; replaced the specific object properties by the
               generic ones in the subClassOf declarations."""@en ;
        ] ;
    :RiCCMCorrespondingComponent """Class implementation of RiC-R060 and RiC-R060i
         relations"""@en ;
.

:PlaceName
    a owl:Class ;
    rdfs:label
        "Place Name"@en ,
        "Nombre de lugar"@es ,
        "Nom de lieu"@fr ;
    rdfs:comment """A label, title or term designating a Place in order to make it
         distinguishable from other similar entities."""@en ;
    rdfs:isDefinedBy <https://www.ica.org/standards/RiC/ontology> ;
    rdfs:subClassOf :Name ;
    skos:changeNote
        [
            dc:date "2023-08-25" ;
            rdf:value "Added a new rdfs:label in French."@en ;
        ] ,
        [
            dc:date "2023-11-02" ;
            rdf:value "Added a new rdfs:label in Spanish."@en ;
        ] ;
    :RiCCMCorrespondingComponent """Class implementation of a specialization of RiC-A28
         (Name attribute)"""@en ;
.

:PlaceRelation
    a owl:Class ;
    rdfs:label
        "Place Relation"@en ,
        "Relación con lugar"@es ,
        "Relation impliquant un lieu"@fr ;
    rdfs:comment """Connects a Place and at least one Thing when the first is
         associated with the existence and lifecycle of the second one. The Place is the source of
         the Relation and the Thing(s) is the target."""@en ;
    rdfs:isDefinedBy <https://www.ica.org/standards/RiC/ontology> ;
    rdfs:subClassOf
        [
            a owl:Restriction ;
            owl:onClass :Place ;
            owl:onProperty :relationHasSource ;
            owl:qualifiedCardinality "1"^^xsd:nonNegativeInteger ;
        ] ,
        [
            a owl:Restriction ;
            owl:minQualifiedCardinality "1"^^xsd:nonNegativeInteger ;
            owl:onClass :Thing ;
            owl:onProperty :relationHasTarget ;
        ] ,
        :Relation ;
    owl:equivalentClass
        [
            a owl:Restriction ;
            owl:hasSelf true ;
            owl:onProperty :placeRelation_role ;
        ] ;
    skos:changeNote
        [
            dc:date "2023-08-25" ;
            rdf:value "Added a new rdfs:label in French."@en ;
        ] ,
        [
            dc:date "2023-12-06" ;
            rdf:value """Improved the description of the Relation class (rdfs:comment)
               by clearly specifying how it is directed."""@en ;
        ] ,
        [
            dc:date "2023-11-02" ;
            rdf:value "Added a new rdfs:label in Spanish."@en ;
        ] ,
        [
            dc:date "2023-11-08" ;
            rdf:value """In order to get a system of rolified Relation classes: added an
               equivalentClass object property; replaced the specific object properties by the
               generic ones in the subClassOf declarations."""@en ;
        ] ;
    :RiCCMCorrespondingComponent """Class implementation of RiC-R074 and RiC-R074i
         relations"""@en ;
.

:PlaceType
    a owl:Class ;
    rdfs:label
        "Place Type"@en ,
        "Tipo de lugar"@es ,
        "Type de lieu"@fr ;
    rdfs:comment "Categorization of a Place."@en ;
    rdfs:isDefinedBy <https://www.ica.org/standards/RiC/ontology> ;
    rdfs:subClassOf :Type ;
    skos:changeNote
        [
            dc:date "2023-08-25" ;
            rdf:value "Added a new rdfs:label in French."@en ;
        ] ,
        [
            dc:date "2023-04-19" ;
            rdf:value "Removed the 0.2 existing unnecessary restriction."@en ;
        ] ,
        [
            dc:date "2023-11-02" ;
            rdf:value "Added a new rdfs:label in Spanish."@en ;
        ] ;
    skos:scopeNote """Broadly, a Place may be a member of three broad categories:
         jurisdiction, manmade structure, or a natural feature. Each of these three categories can
         subdivided into narrower categories."""@en ;
    :RiCCMCorrespondingComponent """Corresponds to RiC-A32 (Place Type
         attribute)"""@en ;
.

:PositionHoldingRelation
    a owl:Class ;
    rdfs:label
        "Position Holding Relation"@en ,
        "Relación de ocupación entre una persona y un puesto"@es ,
        "Relation entre une personne et un poste"@fr ;
    rdfs:comment """Connects at least one Person and at least one Position that the
         Person(s) occupies or occupied. The Person is the source of the Relation and the Position
         is the target."""@en ;
    rdfs:isDefinedBy <https://www.ica.org/standards/RiC/ontology> ;
    rdfs:subClassOf
        [
            a owl:Restriction ;
            owl:minQualifiedCardinality "1"^^xsd:nonNegativeInteger ;
            owl:onClass :Position ;
            owl:onProperty :relationHasTarget ;
        ] ,
        [
            a owl:Restriction ;
            owl:minQualifiedCardinality "1"^^xsd:nonNegativeInteger ;
            owl:onClass :Person ;
            owl:onProperty :relationHasSource ;
        ] ,
        :AgentToAgentRelation ;
    owl:equivalentClass
        [
            a owl:Restriction ;
            owl:hasSelf true ;
            owl:onProperty :positionHoldingRelation_role ;
        ] ;
    skos:changeNote
        [
            dc:date "2023-11-02" ;
            rdf:value "Added a new rdfs:label in Spanish."@en ;
        ] ,
        [
            dc:date "2023-11-12" ;
            rdf:value """Aligned with RiC-CM 1.0: updated the description
               (rdfs:comment)."""@en ;
        ] ,
        [
            dc:date "2023-08-25" ;
            rdf:value "Added a new rdfs:label in French."@en ;
        ] ,
        [
            dc:date "2023-12-06" ;
            rdf:value """Improved the description of the Relation class (rdfs:comment)
               by clearly specifying how it is directed."""@en ;
        ] ,
        [
            dc:date "2023-11-08" ;
            rdf:value """In order to get a system of rolified Relation classes: added an
               equivalentClass object property; replaced the specific object properties by the
               generic ones in the subClassOf declarations."""@en ;
        ] ;
    :RiCCMCorrespondingComponent """Class implementation of RiC-R054 and RiC-R054i
         relations"""@en ;
.

:PositionToGroupRelation
    a owl:Class ;
    rdfs:label
        "Position to Group Relation"@en ,
        "Relación de ocupación entre un grupo y un puesto"@es ,
        "Relation entre un poste et un groupe"@fr ;
    rdfs:comment """Connects at least one Position and a Group in which the
         position(s) exist(s) or existed, or that is (are) defined by that group's organizational
         structure. The Position(s) is the source of the Relation and the Group is the
         target."""@en ;
    rdfs:isDefinedBy <https://www.ica.org/standards/RiC/ontology> ;
    rdfs:subClassOf
        [
            a owl:Restriction ;
            owl:minQualifiedCardinality "1"^^xsd:nonNegativeInteger ;
            owl:onClass :Position ;
            owl:onProperty :relationHasSource ;
        ] ,
        [
            a owl:Restriction ;
            owl:onClass :Group ;
            owl:onProperty :relationHasTarget ;
            owl:qualifiedCardinality "1"^^xsd:nonNegativeInteger ;
        ] ,
        :AgentToAgentRelation ;
    owl:equivalentClass
        [
            a owl:Restriction ;
            owl:hasSelf true ;
            owl:onProperty :positionToGroupRelation_role ;
        ] ;
    skos:changeNote
        [
            dc:date "2023-11-02" ;
            rdf:value "Added a new rdfs:label in Spanish."@en ;
        ] ,
        [
            dc:date "2023-11-12" ;
            rdf:value """Aligned with RiC-CM 1.0: updated the description
               (rdfs:comment)."""@en ;
        ] ,
        [
            dc:date "2023-11-08" ;
            rdf:value """In order to get a system of rolified Relation classes: added an
               equivalentClass object property; replaced the specific object properties by the
               generic ones in the subClassOf declarations."""@en ;
        ] ,
        [
            dc:date "2023-08-25" ;
            rdf:value "Added a new rdfs:label in French."@en ;
        ] ,
        [
            dc:date "2023-12-06" ;
            rdf:value """Improved the description of the Relation class (rdfs:comment)
               by clearly specifying how it is directed."""@en ;
        ] ;
    :RiCCMCorrespondingComponent """Class implementation of RiC-R056 and RiC-R056i
         relations"""@en ;
.

:ProductionTechniqueType
    a owl:Class ;
    rdfs:label
        "Production Technique Type"@en ,
        "Tipo de técnica de producción"@es ,
        "Type de technique de production"@fr ;
    rdfs:comment """The method used in the representation of information on an
         instantiation."""@en ;
    rdfs:isDefinedBy <https://www.ica.org/standards/RiC/ontology> ;
    rdfs:subClassOf :Type ;
    skos:changeNote
        [
            dc:date "2020-10-23" ;
            rdf:value """Comment: updated. Objective: to make RiC-O compliant with
               RiC-CM v0.2."""@en ;
        ] ,
        [
            dc:date "2023-11-02" ;
            rdf:value "Added a new rdfs:label in Spanish."@en ;
        ] ,
        [
            dc:date "2023-08-25" ;
            rdf:value "Added a new rdfs:label in French."@en ;
        ] ,
        [
            dc:date "2023-04-19" ;
            rdf:value "Removed the 0.2 existing unnecessary restriction."@en ;
        ] ,
        [
            dc:date "2023-11-12" ;
            rdf:value """Aligned with RiC-CM 1.0: updated the description
               (rdfs:comment)."""@en ;
        ] ;
    :RiCCMCorrespondingComponent """Class implementation of RiC-A33 (Production
         Technique attribute)"""@en ;
.

:Proxy
    a owl:Class ;
    rdfs:label
        "Proxy"@en ,
        "Proxy"@es ,
        "Proxy"@fr ;
    rdfs:comment """A Proxy represents (stands for) a Record Resource as it exists in
         a specific Record Set."""@en ;
    rdfs:isDefinedBy <https://www.ica.org/standards/RiC/ontology> ;
    rdfs:subClassOf
        [
            a owl:Restriction ;
            owl:onClass :RecordResource ;
            owl:onProperty :proxyFor ;
            owl:qualifiedCardinality "1"^^xsd:nonNegativeInteger ;
        ] ,
        [
            a owl:Restriction ;
            owl:onClass :RecordSet ;
            owl:onProperty :proxyIn ;
            owl:qualifiedCardinality "1"^^xsd:nonNegativeInteger ;
        ] ,
        :Concept ;
    skos:changeNote
        [
            dc:date "2023-11-02" ;
            rdf:value "Added a new rdfs:label in Spanish."@en ;
        ] ,
        [
            dc:date "2023-08-25" ;
            rdf:value "Added a new rdfs:label in French."@en ;
        ] ;
    skos:scopeNote """Useful for handling in RDF the sequencing of records or records
         sets in the context of a Record set. A Record Resource has only one Proxy in the context of
         one specific Record Set. It may have many Proxies simultaneously or through
         time."""@en ;
    :closeTo "ORE Proxy (http://www.openarchives.org/ore/terms/Proxy)"@en ;
.

:RecordResourceGeneticRelation
    a owl:Class ;
    rdfs:label
        "Record Resource Genetic Relation"@en ,
        "Relación genética entre recursos documentales"@es ,
        "Relation génétique entre des ressources archivistiques"@fr ;
    rdfs:comment """Connects two or more record resources when there is a genetic link
         between them. Genetic in this sense is as defined by diplomatics, i.e., the process by
         which a record resource is developed. This Relation is a generic, not oriented
         one."""@en ;
    rdfs:isDefinedBy <https://www.ica.org/standards/RiC/ontology> ;
    rdfs:subClassOf
        [
            a owl:Restriction ;
            owl:minQualifiedCardinality "2"^^xsd:nonNegativeInteger ;
            owl:onClass :RecordResource ;
            owl:onProperty :relationConnects ;
        ] ,
        :RecordResourceToRecordResourceRelation ;
    owl:equivalentClass
        [
            a owl:Restriction ;
            owl:hasSelf true ;
            owl:onProperty :recordResourceGeneticRelation_role ;
        ] ;
    skos:changeNote
        [
            dc:date "2023-11-02" ;
            rdf:value "Added a new rdfs:label in Spanish."@en ;
        ] ,
        [
            dc:date "2023-11-12" ;
            rdf:value """Aligned with RiC-CM 1.0: updated the description
               (rdfs:comment)."""@en ;
        ] ,
        [
            dc:date "2023-08-25" ;
            rdf:value "Added a new rdfs:label in French."@en ;
        ] ,
        [
            dc:date "2023-11-08" ;
            rdf:value """In order to get a system of rolified Relation classes: added an
               equivalentClass object property; replaced the specific object properties by the
               generic ones in the subClassOf declarations."""@en ;
        ] ,
        [
            dc:date "2023-12-06" ;
            rdf:value """Improved the description of the Relation class (rdfs:comment)
               by clearly specifying how it is directed."""@en ;
        ] ;
    :RiCCMCorrespondingComponent """Class implementation of RiC-R023 and RiC-023i
         relations"""@en ;
.

:RecordResourceHoldingRelation
    a owl:Class ;
    rdfs:label
        "Record Resource Holding Relation"@en ,
        """Relación entre agentes y recursos documentales que
         conservan"""@es ,
        """Relation entre agents et ressources archivistiques ou instanciations
         conservées"""@fr ;
    rdfs:comment """Connects at least one Agent and one or more Record Resource or
         Instantiation that the Agent(s) hold(s) or held. The Agent(s) is the source of the Relation
         and the Record Resource(s) or Instantiation is the target."""@en ;
    rdfs:isDefinedBy <https://www.ica.org/standards/RiC/ontology> ;
    rdfs:subClassOf
        [
            a owl:Restriction ;
            owl:minQualifiedCardinality "1"^^xsd:nonNegativeInteger ;
            owl:onClass
                [
                    a owl:Class ;
                    owl:unionOf (
                        :Instantiation
                        :RecordResource
                    ) ;
                ] ;
            owl:onProperty :relationHasTarget ;
        ] ,
        [
            a owl:Restriction ;
            owl:minQualifiedCardinality "1"^^xsd:nonNegativeInteger ;
            owl:onClass :Agent ;
            owl:onProperty :relationHasSource ;
        ] ,
        :ManagementRelation ;
    owl:equivalentClass
        [
            a owl:Restriction ;
            owl:hasSelf true ;
            owl:onProperty :recordResourceHoldingRelation_role ;
        ] ;
    skos:changeNote
        [
            dc:date "2023-11-02" ;
            rdf:value "Added a new rdfs:label in Spanish."@en ;
        ] ,
        [
            dc:date "2023-11-08" ;
            rdf:value """In order to get a system of rolified Relation classes: added an
               equivalentClass object property; replaced the specific object properties by the
               generic ones in the subClassOf declarations."""@en ;
        ] ,
        [
            dc:date "2023-11-12" ;
            rdf:value """Aligned with RiC-CM 1.0: updated the description
               (rdfs:comment)."""@en ;
        ] ,
        [
            dc:date "2023-08-25" ;
            rdf:value "Added a new rdfs:label in French."@en ;
        ] ,
        [
            dc:date "2023-12-30" ;
            rdf:value "Fixed a typo in the French label."@en ;
        ] ,
        [
            dc:date "2023-12-06" ;
            rdf:value """Improved the description of the Relation class (rdfs:comment)
               by clearly specifying how it is directed."""@en ;
        ] ;
    :RiCCMCorrespondingComponent """Class implementation of RiC-R039 and RiC-039i
         relations"""@en ;
.

:RecordResourceToInstantiationRelation
    a owl:Class ;
    rdfs:label
        "Record Resource to Instantiation Relation"@en ,
        "Relación de recurso documental a instanciación"@es ,
        "Relation d’instanciation"@fr ;
    rdfs:comment """Connects a Record Resource to one or more Instantiations that
         instantiate it, and which either may exist or may have been lost or destroyed. The Record
         Resource is the source of the Relation and the Instantiation(s) is the
         target."""@en ;
    rdfs:isDefinedBy <https://www.ica.org/standards/RiC/ontology> ;
    rdfs:subClassOf
        [
            a owl:Restriction ;
            owl:minQualifiedCardinality "1"^^xsd:nonNegativeInteger ;
            owl:onClass :Instantiation ;
            owl:onProperty :relationHasTarget ;
        ] ,
        [
            a owl:Restriction ;
            owl:onClass :RecordResource ;
            owl:onProperty :relationHasSource ;
            owl:qualifiedCardinality "1"^^xsd:nonNegativeInteger ;
        ] ,
        :Relation ;
    owl:equivalentClass
        [
            a owl:Restriction ;
            owl:hasSelf true ;
            owl:onProperty :recordResourceToInstantiationRelation_role ;
        ] ;
    skos:changeNote
        [
            dc:date "2023-11-12" ;
            rdf:value """Aligned with RiC-CM 1.0: updated the description
               (rdfs:comment), skos:scopeNote."""@en ;
        ] ,
        [
            dc:date "2023-12-06" ;
            rdf:value """Improved the description of the Relation class (rdfs:comment)
               by clearly specifying how it is directed."""@en ;
        ] ,
        [
            dc:date "2023-11-02" ;
            rdf:value "Added a new rdfs:label in Spanish."@en ;
        ] ,
        [
            dc:date "2023-08-25" ;
            rdf:value "Added a new rdfs:label in French."@en ;
        ] ,
        [
            dc:date "2023-11-08" ;
            rdf:value """In order to get a system of rolified Relation classes: added an
               equivalentClass object property; replaced the specific object properties by the
               generic ones in the subClassOf declarations."""@en ;
        ] ;
    skos:scopeNote """In some situations, it may be useful or necessary to connect a
         record resource to an instantiation that no longer exists or has been lost, when some of
         its characteristics are known from a source, such as an old finding aid."""@en ;
    :RiCCMCorrespondingComponent """Class implementation of RiC-R025 and RiC-R025i
         relations"""@en ;
.

:RepresentationType
    a owl:Class ;
    rdfs:label
        "Representation Type"@en ,
        "Tipo de grabación"@es ,
        "Type de représentation"@fr ;
    rdfs:comment """Method of recording the content type of an
         Instantiation"""@en ;
    rdfs:isDefinedBy <https://www.ica.org/standards/RiC/ontology> ;
    rdfs:subClassOf :Type ;
    skos:changeNote
        [
            dc:date "2023-08-25" ;
            rdf:value "Added a new rdfs:label in French."@en ;
        ] ,
        [
            dc:date "2023-11-02" ;
            rdf:value "Added a new rdfs:label in Spanish."@en ;
        ] ,
        [
            dc:date "2023-11-12" ;
            rdf:value """Aligned with RiC-CM 1.0: updated the description
               (rdfs:comment), skos:scopeNote."""@en ;
        ] ,
        [
            dc:date "2023-04-19" ;
            rdf:value "Removed the 0.2 existing unnecessary restriction."@en ;
        ] ,
        [
            dc:date "2020-10-23" ;
            rdf:value """Comment and scope note: updated. Objective: to make RiC-O
               compliant with RiC-CM v0.2."""@en ;
        ] ;
    skos:scopeNote """Can be unmediated (which allows humans to receive the message
         communicated without an intermediation of a device) and mediated (which needs a device to
         decode the message). A lot of contemporary mediated types are digital. Each representation
         type may present specific features: bit rate for audio, resolution for digital images,
         encoding format for video etc. Depending on the type, specific attributes may be added to
         describe their characteristics."""@en ;
    :RiCCMCorrespondingComponent """Corresponds to RiC-A37 (Representation Type
         attribute)"""@en ;
.

:RoleType
    a owl:Class ;
    rdfs:label
        "Role Type"@en ,
        "Tipo de rol"@es ,
        "Type de rôle"@fr ;
    rdfs:comment """The role an Agent plays in some context (usually in some creation
         relation). Not to be confused with a Position (position of an agent in some group). For
         example, a Person who is the head of some Corporate Body may play the role of annotator (of
         a record) in a creation relation."""@en ;
    rdfs:isDefinedBy <https://www.ica.org/standards/RiC/ontology> ;
    rdfs:subClassOf :Type ;
    skos:changeNote
        [
            dc:date "2023-11-02" ;
            rdf:value "Added a new rdfs:label in Spanish."@en ;
        ] ,
        [
            dc:date "2023-08-25" ;
            rdf:value "Added a new rdfs:label in French."@en ;
        ] ;
.

:SiblingRelation
    a owl:Class ;
    rdfs:label
        "Sibling Relation"@en ,
        "Relación familiar entre hermanos"@es ,
        "Relation de fratrie"@fr ;
    rdfs:comment """Connects at least two Persons, when they are siblings. This
         Relation is not oriented."""@en ;
    rdfs:isDefinedBy <https://www.ica.org/standards/RiC/ontology> ;
    rdfs:subClassOf
        [
            a owl:Restriction ;
            owl:minQualifiedCardinality "2"^^xsd:nonNegativeInteger ;
            owl:onClass :Person ;
            owl:onProperty :relationConnects ;
        ] ,
        :FamilyRelation ;
    owl:equivalentClass
        [
            a owl:Restriction ;
            owl:hasSelf true ;
            owl:onProperty :siblingRelation_role ;
        ] ;
    skos:changeNote
        [
            dc:date "2023-08-25" ;
            rdf:value "Added a new rdfs:label in French."@en ;
        ] ,
        [
            dc:date "2023-11-08" ;
            rdf:value """In order to get a system of rolified Relation classes: added an
               equivalentClass object property; replaced the specific object properties by the
               generic ones in the subClassOf declarations."""@en ;
        ] ,
        [
            dc:date "2023-12-06" ;
            rdf:value """Improved the description of the Relation class (rdfs:comment)
               by clearly specifying how it is directed."""@en ;
        ] ,
        [
            dc:date "2023-11-02" ;
            rdf:value "Added a new rdfs:label in Spanish."@en ;
        ] ;
    :RiCCMCorrespondingComponent """Class implementation of RiC-R048 and RiC-R048i
         relations"""@en ;
.

:SpouseRelation
    a owl:Class ;
    rdfs:label
        "Spouse Relation"@en ,
        "Relación matrimonial entre personas"@es ,
        "Relation matrimoniale"@fr ;
    rdfs:comment """Connects at least two Persons, when they are spouses. This
         Relation is not oriented."""@en ;
    rdfs:isDefinedBy <https://www.ica.org/standards/RiC/ontology> ;
    rdfs:subClassOf
        [
            a owl:Restriction ;
            owl:minQualifiedCardinality "2"^^xsd:nonNegativeInteger ;
            owl:onClass :Person ;
            owl:onProperty :relationConnects ;
        ] ,
        :FamilyRelation ;
    owl:equivalentClass
        [
            a owl:Restriction ;
            owl:hasSelf true ;
            owl:onProperty :spouseRelation_role ;
        ] ;
    skos:changeNote
        [
            dc:date "2023-12-06" ;
            rdf:value """Improved the description of the Relation class (rdfs:comment)
               by clearly specifying how it is directed."""@en ;
        ] ,
        [
            dc:date "2023-08-25" ;
            rdf:value "Added a new rdfs:label in French."@en ;
        ] ,
        [
            dc:date "2023-11-08" ;
            rdf:value """In order to get a system of rolified Relation classes: added an
               equivalentClass object property; replaced the specific object properties by the
               generic ones in the subClassOf declarations."""@en ;
        ] ,
        [
            dc:date "2023-11-02" ;
            rdf:value "Added a new rdfs:label in Spanish."@en ;
        ] ;
    :RiCCMCorrespondingComponent """Class implementation of RiC-R049 and RiC-R049i
         relations"""@en ;
.

:TeachingRelation
    a owl:Class ;
    rdfs:label
        "Teaching Relation"@en ,
        "Relación académica entre profesor y alumno"@es ,
        "Relation entre enseignants et étudiants"@fr ;
    rdfs:comment """Connects at least one Person to at least another Person who is or
         was their student. The Relation is oriented from the teacher(s) to the student(s): the
         teacher Person(s) is the source of the Relation, and the student Person(s) is the
         target."""@en ;
    rdfs:isDefinedBy <https://www.ica.org/standards/RiC/ontology> ;
    rdfs:subClassOf
        [
            a owl:Restriction ;
            owl:minQualifiedCardinality "1"^^xsd:nonNegativeInteger ;
            owl:onClass :Person ;
            owl:onProperty :relationHasSource ;
        ] ,
        [
            a owl:Restriction ;
            owl:minQualifiedCardinality "1"^^xsd:nonNegativeInteger ;
            owl:onClass :Person ;
            owl:onProperty :relationHasTarget ;
        ] ,
        :KnowingRelation ;
    owl:equivalentClass
        [
            a owl:Restriction ;
            owl:hasSelf true ;
            owl:onProperty :teachingRelation_role ;
        ] ;
    skos:changeNote
        [
            dc:date "2023-12-06" ;
            rdf:value """Improved the description of the Relation class (rdfs:comment)
               by clearly specifying how it is directed."""@en ;
        ] ,
        [
            dc:date "2023-11-08" ;
            rdf:value """In order to get a system of rolified Relation classes: added an
               equivalentClass object property; replaced the specific object properties by the
               generic ones in the subClassOf declarations."""@en ;
        ] ,
        [
            dc:date "2023-11-12" ;
            rdf:value """Aligned with RiC-CM 1.0: updated the description
               (rdfs:comment)."""@en ;
        ] ,
        [
            dc:date "2023-08-25" ;
            rdf:value "Added a new rdfs:label in French."@en ;
        ] ,
        [
            dc:date "2023-11-02" ;
            rdf:value "Added a new rdfs:label in Spanish."@en ;
        ] ;
    :RiCCMCorrespondingComponent """Class implementation of RiC-R053 and RiC-R053i
         relations"""@en ;
.

:Title
    a owl:Class ;
    rdfs:label
        "Title"@en ,
        "Título"@es ,
        "Intitulé"@fr ;
    rdfs:comment "A name that is used for a Record Resource or a Rule"@en ;
    rdfs:isDefinedBy <https://www.ica.org/standards/RiC/ontology> ;
    rdfs:subClassOf :Name ;
    skos:changeNote
        [
            dc:date "2023-08-25" ;
            rdf:value "Added a new rdfs:label in French."@en ;
        ] ,
        [
            dc:date "2023-11-02" ;
            rdf:value "Added a new rdfs:label in Spanish."@en ;
        ] ;
    :RiCCMCorrespondingComponent """Class implementation of a specialization of RiC-A28
         (Name attribute)"""@en ;
.

:TypeRelation
    a owl:Class ;
    rdfs:label
        "Type Relation"@en ,
        "Tipo de relación"@es ,
        "Relation de catégorisation"@fr ;
    rdfs:comment """Connects a category (a Type) and at least one Thing that belongs
         to this category. The Type(s) is the source of the Relation, and the Thing(s) is the
         target."""@en ;
    rdfs:isDefinedBy <https://www.ica.org/standards/RiC/ontology> ;
    rdfs:subClassOf
        [
            a owl:Restriction ;
            owl:onClass :Type ;
            owl:onProperty :relationHasSource ;
            owl:qualifiedCardinality "1"^^xsd:nonNegativeInteger ;
        ] ,
        [
            a owl:Restriction ;
            owl:minQualifiedCardinality "1"^^xsd:nonNegativeInteger ;
            owl:onClass :Thing ;
            owl:onProperty :relationHasTarget ;
        ] ,
        :Relation ;
    owl:equivalentClass
        [
            a owl:Restriction ;
            owl:hasSelf true ;
            owl:onProperty :typeRelation_role ;
        ] ;
    skos:changeNote
        [
            dc:date "2023-12-06" ;
            rdf:value """Improved the description of the Relation class (rdfs:comment)
               by clearly specifying how it is directed."""@en ;
        ] ,
        [
            dc:date "2023-11-08" ;
            rdf:value """In order to get a system of rolified Relation classes: added an
               equivalentClass object property; replaced the specific object properties by the
               generic ones in the subClassOf declarations."""@en ;
        ] ,
        [
            dc:date "2023-11-02" ;
            rdf:value "Added a new rdfs:label in Spanish."@en ;
        ] ,
        [
            dc:date "2023-08-25" ;
            rdf:value "Added a new rdfs:label in French."@en ;
        ] ;
    skos:scopeNote """may be useful at least for some types (e.g. demographic
         group)"""@en ;
.

:UnitOfMeasurement
    a owl:Class ;
    rdfs:label
        "Unit Of Measurement"@en ,
        "Unidad de medida"@es ,
        "Unité de mesure"@fr ;
    rdfs:comment """A definite magnitude of a quantity, defined and adopted by
         convention or by law, that is used as a standard for measurement of the same kind of
         quantity. Can be spacial units (cm, m), weight (g, kg), time (s, h), storage (MB, TB) or
         more informal units used in the archival context like number of boxes, pages or
         words."""@en ;
    rdfs:isDefinedBy <https://www.ica.org/standards/RiC/ontology> ;
    rdfs:subClassOf :Concept ;
    skos:changeNote
        [
            dc:date "2023-08-28" ;
            rdf:value "Added an xml:lang attribute to the rdfs:comment."@en ;
        ] ,
        [
            dc:date "2023-08-25" ;
            rdf:value "Added a new rdfs:label in French."@en ;
        ] ,
        [
            dc:date "2020-10-28" ;
            rdf:value """Class added in order to be able to handle units of measurement
               as full entities."""@en ;
        ] ,
        [
            dc:date "2023-11-02" ;
            rdf:value "Added a new rdfs:label in Spanish."@en ;
        ] ;
.

:WorkRelation
    a owl:Class ;
    rdfs:label
        "Work Relation"@en ,
        "Relación profesional"@es ,
        "Relation de travail"@fr ;
    rdfs:comment """Connects at least two Agents that have or had some type of work
         relation in the course of their activities. This Relation is not oriented."""@en ;
    rdfs:isDefinedBy <https://www.ica.org/standards/RiC/ontology> ;
    rdfs:subClassOf
        [
            a owl:Restriction ;
            owl:minQualifiedCardinality "2"^^xsd:nonNegativeInteger ;
            owl:onClass :Agent ;
            owl:onProperty :relationConnects ;
        ] ,
        :AgentToAgentRelation ;
    owl:equivalentClass
        [
            a owl:Restriction ;
            owl:hasSelf true ;
            owl:onProperty :workRelation_role ;
        ] ;
    skos:changeNote
        [
            dc:date "2023-11-02" ;
            rdf:value "Added a new rdfs:label in Spanish."@en ;
        ] ,
        [
            dc:date "2023-11-12" ;
            rdf:value """Aligned with RiC-CM 1.0: updated the description
               (rdfs:comment)."""@en ;
        ] ,
        [
            dc:date "2023-11-08" ;
            rdf:value """In order to get a system of rolified Relation classes: added an
               equivalentClass object property; replaced the specific object properties by the
               generic ones in the subClassOf declarations."""@en ;
        ] ,
        [
            dc:date "2023-08-25" ;
            rdf:value "Added a new rdfs:label in French."@en ;
        ] ,
        [
            dc:date "2023-12-06" ;
            rdf:value """Improved the description of the Relation class (rdfs:comment)
               by clearly specifying how it is directed."""@en ;
        ] ;
    :RiCCMCorrespondingComponent """Class implementation of RiC-R046 and RiR046i
         relations"""@en ;
.

:asConcernsActivity
    a owl:ObjectProperty ;
    rdfs:label
        "as concerns activity"@en ,
        "en cuanto a actividad"@es ,
        "en ce qui concerne l’activité"@fr ;
    rdfs:comment """Connects an Agent Temporal Relation or Mandate Relation, to an
         Activity that is, either transferred from an Agent to another one, or assigned by a Mandate
         to an Agent."""@en ;
    rdfs:domain
        [
            a owl:Class ;
            owl:unionOf (
                :AgentTemporalRelation
                :MandateRelation
            ) ;
        ] ;
    rdfs:isDefinedBy <https://www.ica.org/standards/RiC/ontology> ;
    rdfs:range :Activity ;
    rdfs:subPropertyOf :relationHasContext ;
    owl:inverseOf :activityIsContextOfRelation ;
    skos:changeNote
        [
            dc:date "2023-11-02" ;
            rdf:value "Added a new rdfs:label in Spanish."@en ;
        ] ,
        [
            dc:date "2023-08-28" ;
            rdf:value "Added a new rdfs:label in French."@en ;
        ] ;
.

:containsTransitive
    a
        owl:ObjectProperty ,
        owl:TransitiveProperty ;
    rdfs:label
        "contains transitive"@en ,
        "contiene transitivo"@es ,
        "contient transitif"@fr ;
    rdfs:comment """Connects a Place to a Place that it contains, directly or indirectly. This is a
         transitive relation.""" ;
    rdfs:domain :Place ;
    rdfs:isDefinedBy <https://www.ica.org/standards/RiC/ontology> ;
    rdfs:range :Place ;
    rdfs:subPropertyOf
        :containsOrContained ,
        :hasPartTransitive ;
    owl:inverseOf :isContainedByTransitive ;
    skos:changeNote
        [
            dc:date "2023-11-27" ;
            rdf:value "Added a new rdfs:label in Spanish."@en ;
        ] ,
        [
            dc:date "2023-09-05" ;
            rdf:value """Object property added, along with its inverse property, in order to enable to
               express current partitive relations between places (the past partitive relation also
               being added).""" ;
        ] ,
        [
            dc:date "2023-11-12" ;
            rdf:value "Updated the description (rdfs:comment) and labels."@en ;
        ] ;
.

:correspondenceRelation_role
    a
        owl:ObjectProperty ,
        owl:ReflexiveProperty ;
    rdfs:label
        "has the role of the Correspondence Relation"@en ,
        """desempeña el papel de la Relación entre personas por
         correspondencia"""@es ,
        "a le rôle de la Relation épistolaire"@fr ;
    rdfs:comment """Connects a CorrespondenceRelation to itself. It is a reflexive
         property, that can stand for an instance of the class when necessary, e.g. when you explore
         a knowledge graph."""@en ;
    rdfs:domain :CorrespondenceRelation ;
    rdfs:isDefinedBy <https://www.ica.org/standards/RiC/ontology> ;
    rdfs:range :CorrespondenceRelation ;
    rdfs:subPropertyOf :knowingRelation_role ;
    skos:changeNote
        [
            dc:date "2023-11-08" ;
            rdf:value """In order to get a system of rolified Relation classes: created
               the object property, with domain and range the CorrespondenceRelation rolified class.
               Declared it as reflexive. Declared it(s) superproperty(ies)."""@en ;
        ] ;
    skos:scopeNote """This property "rolifies" the CorrespondenceRelation class. It
         should be used only when you have to manage instances of the CorrespondenceRelation class,
         to connect each instance to itself, in order to be able to infer, using OWL-RL and property
         paths, the two shortcuts corresponding to this n-ary class."""@en ;
.

:followsInSequenceTransitive
    a
        owl:ObjectProperty ,
        owl:TransitiveProperty ;
    rdfs:label
        "follows in sequence transitive"@en ,
        "sigue en la secuencia transitivo"@es ,
        "suit dans la séquence transitif"@fr ;
    rdfs:comment """Connects a Thing to a Thing that it directly or indirectly follows
         in some non chronological sequence."""@en ;
    rdfs:domain :Thing ;
    rdfs:isDefinedBy <https://www.ica.org/standards/RiC/ontology> ;
    rdfs:range :Thing ;
    rdfs:subPropertyOf :followsOrFollowed ;
    owl:inverseOf :precedesInSequenceTransitive ;
    skos:changeNote
        [
            dc:date "2023-09-08" ;
            rdf:value """Added transitive super-property and both present direct and
               past sequential relations as well as their respective inverse relations."""@en ;
        ] ,
        [
            dc:date "2023-11-27" ;
            rdf:value "Added a new rdfs:label in Spanish."@en ;
        ] ,
        [
            dc:date "2023-11-12" ;
            rdf:value "Updated the description (rdfs:comment) and labels."@en ;
        ] ,
        [
            dc:date "2023-09-22" ;
            rdf:value """Renamed the property and modified its definition (rdfs:comment)
               in order to better distinguish it from followsInTime."""@en ;
        ] ;
.

:functionalEquivalenceRelation_role
    a
        owl:ObjectProperty ,
        owl:ReflexiveProperty ;
    rdfs:label
        "has the role of the Functional Equivalence Relation"@en ,
        """desempeña el papel de la Relación de equivalencia
         funcional"""@es ,
        "a le rôle de la Relation d’équivalence fonctionnelle"@fr ;
    rdfs:comment """Connects a FunctionalEquivalenceRelation to itself. It is a
         reflexive property, that can stand for an instance of the class when necessary, e.g. when
         you explore a knowledge graph."""@en ;
    rdfs:domain :FunctionalEquivalenceRelation ;
    rdfs:isDefinedBy <https://www.ica.org/standards/RiC/ontology> ;
    rdfs:range :FunctionalEquivalenceRelation ;
    rdfs:subPropertyOf :instantiationToInstantiationRelation_role ;
    skos:changeNote
        [
            dc:date "2023-11-08" ;
            rdf:value """In order to get a system of rolified Relation classes: created
               the object property, with domain and range the FunctionalEquivalenceRelation rolified
               class. Declared it as reflexive. Declared it(s) superproperty(ies)."""@en ;
        ] ;
    skos:scopeNote """This property "rolifies" the FunctionalEquivalenceRelation
         class. It should be used only when you have to manage instances of the
         FunctionalEquivalenceRelation class, to connect each instance to itself, in order to be
         able to infer, using OWL-RL and property paths, the two shortcuts corresponding to this
         n-ary class."""@en ;
.

:hadSubordinate
    a owl:ObjectProperty ;
    rdfs:label
        "had subordinate"@en ,
        "tenía como subordinado o subordinada a"@es ,
        "a eu pour subalterne"@fr ;
    rdfs:comment """Connects an Agent to an Agent that was hierarchically inferior in
         the past."""@en ;
    rdfs:domain :Agent ;
    rdfs:isDefinedBy <https://www.ica.org/standards/RiC/ontology> ;
    rdfs:range :Agent ;
    rdfs:subPropertyOf :hasOrHadSubordinate ;
    owl:inverseOf :wasSubordinateTo ;
    skos:changeNote
        [
            dc:date "2023-09-08" ;
            rdf:value """Object property added, along with its inverse property, in
               order to enable to express past subordination relations between Agents (the current
               subordination relations being also added, including a transitive one)."""@en ;
        ] ,
        [
            dc:date "2023-11-27" ;
            rdf:value "Added a new rdfs:label in Spanish."@en ;
        ] ,
        [
            dc:date "2023-11-12" ;
            rdf:value "Updated the labels."@en ;
        ] ;
.

:hasAncestor
    a
        owl:ObjectProperty ,
        owl:TransitiveProperty ;
    rdfs:label
        "has ancestor"@en ,
        "tiene como ancestro a"@es ,
        "a pour ancêtre"@fr ;
    rdfs:comment """Inverse of 'has descendant' object property. This is a transitive
         relation."""@en ;
    rdfs:domain :Person ;
    rdfs:isDefinedBy <https://www.ica.org/standards/RiC/ontology> ;
    rdfs:range :Person ;
    rdfs:subPropertyOf
        :hasFamilyAssociationWith ,
        :isSuccessorOf ;
    owl:inverseOf :hasDescendant ;
    owl:propertyChainAxiom (
        :thingIsTargetOfRelation
        :descendanceRelation_role
        :relationHasSource
    ) ;
    skos:changeNote
        [
            dc:date "2023-11-08" ;
            rdf:value """In order to get a system of rolified Relation classes: modified
               the property chain axiom so that it now involves the new descendanceRelation_role
               object property."""@en ;
        ] ,
        [
            dc:date "2021-01-22" ;
            rdf:value "changed the superproperty IRIs."@en ;
        ] ,
        [
            dc:date "2023-11-02" ;
            rdf:value "Added a new rdfs:label in Spanish."@en ;
        ] ,
        [
            dc:date "2023-09-08" ;
            rdf:value "made property transitive"@en ;
        ] ,
        [
            dc:date "2023-08-28" ;
            rdf:value "Added a new rdfs:label in French."@en ;
        ] ;
    :RiCCMCorrespondingComponent """RiC-R017i (has ancestor
         relation)"""@en ;
.

:hasComponentTransitive
    a
        owl:ObjectProperty ,
        owl:TransitiveProperty ;
    rdfs:label
        "has component transitive"@en ,
        "tiene como componente transitivo"@es ,
        "a pour composant transitif"@fr ;
    rdfs:comment """Connects an Instantiation to another Instantiation that is,
         directly or indirectly, a component of that Instantiation. This is a transitive
         relation."""@en ;
    rdfs:domain :Instantiation ;
    rdfs:isDefinedBy <https://www.ica.org/standards/RiC/ontology> ;
    rdfs:range :Instantiation ;
    rdfs:subPropertyOf
        :hasOrHadComponent ,
        :hasPartTransitive ;
    owl:inverseOf :isComponentOfTransitive ;
    skos:changeNote
        [
            dc:date "2023-09-08" ;
            rdf:value """Object property added, along with its inverse property, in
               order to enable to express current partitive relations between instantiations (the
               past partitive relation also being added)."""@en ;
        ] ,
        [
            dc:date "2023-11-27" ;
            rdf:value "Added a new rdfs:label in Spanish."@en ;
        ] ,
        [
            dc:date "2023-11-12" ;
            rdf:value "Updated the description (rdfs:comment) and labels."@en ;
        ] ;
.

:hasConstituentTransitive
    a
        owl:ObjectProperty ,
        owl:TransitiveProperty ;
    rdfs:label
        "has constituent transitive"@en ,
        "tiene como elemento constitutivo transitivo"@es ,
        "a pour constituant transitif"@fr ;
    rdfs:comment """Connects a Record or Record Part to another Record or Record Part
         that is its constituent, directly or indirectly. This is a transitive
         relation."""@en ;
    rdfs:domain
        [
            a owl:Class ;
            owl:unionOf (
                :Record
                :RecordPart
            ) ;
        ] ;
    rdfs:isDefinedBy <https://www.ica.org/standards/RiC/ontology> ;
    rdfs:range
        [
            a owl:Class ;
            owl:unionOf (
                :Record
                :RecordPart
            ) ;
        ] ;
    rdfs:subPropertyOf
        :hasOrHadConstituent ,
        :hasPartTransitive ;
    owl:inverseOf :isConstituentOfTransitive ;
    skos:changeNote
        [
            dc:date "2023-11-12" ;
            rdf:value "Updated the description (rdfs:comment) and labels."@en ;
        ] ,
        [
            dc:date "2023-10-26" ;
            rdf:value "Added RecordPart to the domain."@en ;
        ] ,
        [
            dc:date "2023-11-27" ;
            rdf:value "Added a new rdfs:label in Spanish."@en ;
        ] ,
        [
            dc:date "2023-09-08" ;
            rdf:value """Object property added, along with its inverse property, in
               order to enable to express current partitive relations between records and other
               records or record parts (the past partitive relation also being added)."""@en ;
        ] ;
.

:hasCreator
    a owl:ObjectProperty ;
    rdfs:label
        "has creator"@en ,
        "tiene como creador a"@es ,
        "a pour créateur"@fr ;
    rdfs:comment """Connects a Record Resource or an Instantiation to an Agent that is
         either responsible for all or some of the content of the Record Resource or is a
         contributor to the genesis or production of an Instantiation."""@en ;
    rdfs:domain
        [
            a owl:Class ;
            owl:unionOf (
                :Instantiation
                :RecordResource
            ) ;
        ] ;
    rdfs:isDefinedBy <https://www.ica.org/standards/RiC/ontology> ;
    rdfs:range :Agent ;
    rdfs:subPropertyOf :hasOrganicProvenance ;
    owl:inverseOf :isCreatorOf ;
    owl:propertyChainAxiom (
        :thingIsSourceOfRelation
        :creationRelation_role
        :relationHasTarget
    ) ;
    skos:changeNote
        [
            dc:date "2021-01-22" ;
            rdf:value """changed the IRI and label (changed made in order to make RiC-O
               compliant with RiC-CM 0.2; the name of this property in RiC-O 0.1 was
               "createdBy")."""@en ;
        ] ,
        [
            dc:date "2023-11-02" ;
            rdf:value "Added a new rdfs:label in Spanish."@en ;
        ] ,
        [
            dc:date "2023-08-28" ;
            rdf:value "Added a new rdfs:label in French."@en ;
        ] ,
        [
            dc:date "2023-12-29" ;
            rdf:value """Added the property chain axiom, that had been
               forgotten."""@en ;
        ] ;
    skos:scopeNote """Covers the definition of author in diplomatics, and any
         contribution to the intellectual content of a Record Resource."""@en ;
    :RiCCMCorrespondingComponent """RiC-R027 ('has creator'
         relation)"""@en ;
.

:hasDescendant
    a
        owl:ObjectProperty ,
        owl:TransitiveProperty ;
    rdfs:label
        "has descendant"@en ,
        "tiene como descendiente a"@es ,
        "a pour descendant"@fr ;
    rdfs:comment """Connects a Person to one of their descendants. This is a
         transitive relation."""@en ;
    rdfs:domain :Person ;
    rdfs:isDefinedBy <https://www.ica.org/standards/RiC/ontology> ;
    rdfs:range :Person ;
    rdfs:subPropertyOf
        :hasFamilyAssociationWith ,
        :hasSuccessor ;
    owl:inverseOf :hasAncestor ;
    owl:propertyChainAxiom (
        :thingIsSourceOfRelation
        :descendanceRelation_role
        :relationHasTarget
    ) ;
    skos:changeNote
        [
            dc:date "2023-11-12" ;
            rdf:value """Aligned with RiC-CM 1.0: updated the
               skos:scopeNote."""@en ;
        ] ,
        [
            dc:date "2021-01-22" ;
            rdf:value "changed the superproperties IRIs."@en ;
        ] ,
        [
            dc:date "2023-08-28" ;
            rdf:value "Added a new rdfs:label in French."@en ;
        ] ,
        [
            dc:date "2023-09-08" ;
            rdf:value "made property transitive"@en ;
        ] ,
        [
            dc:date "2023-11-02" ;
            rdf:value "Added a new rdfs:label in Spanish."@en ;
        ] ,
        [
            dc:date "2023-11-08" ;
            rdf:value """In order to get a system of rolified Relation classes: modified
               the property chain axiom so that it now involves the new descendanceRelation_role
               object property."""@en ;
        ] ;
    skos:scopeNote """There may be zero to many intermediate persons, ignored or
         unknown, between the two connected persons."""@en ;
    :RiCCMCorrespondingComponent """RiC-R017 ('has descendant'
         relation)"""@en ;
.

:hasDirectSubordinate
    a owl:ObjectProperty ;
    rdfs:label
        "has direct subordinate"@en ,
        "tiene directamente como subordinado o subordinada a"@es ,
        "a directement pour subalterne"@fr ;
    rdfs:comment """Connects an Agent to an Agent that is its direct
         subordinate."""@en ;
    rdfs:domain :Agent ;
    rdfs:isDefinedBy <https://www.ica.org/standards/RiC/ontology> ;
    rdfs:range :Agent ;
    rdfs:subPropertyOf :hasSubordinateTransitive ;
    owl:inverseOf :isDirectSubordinateTo ;
    skos:changeNote
        [
            dc:date "2023-11-27" ;
            rdf:value "Added a new rdfs:label in Spanish."@en ;
        ] ,
        [
            dc:date "2023-11-12" ;
            rdf:value "Updated the labels."@en ;
        ] ,
        [
            dc:date "2023-09-08" ;
            rdf:value """Object property added, along with its inverse property, in
               order to enable to express current, direct, subordination relations between agents
               (the possibly indirect, transitive relation, superproperty of this one, being also
               added)."""@en ;
        ] ;
.

:hasModificationDate
    a owl:ObjectProperty ;
    rdfs:label
        "has modification date"@en ,
        "tiene como fecha de modificación"@es ,
        "a pour date de modification"@fr ;
    rdfs:comment """Inverse of 'is modification date of' object
         property."""@en ;
    rdfs:domain :Thing ;
    rdfs:isDefinedBy <https://www.ica.org/standards/RiC/ontology> ;
    rdfs:range :Date ;
    rdfs:subPropertyOf :isAssociatedWithDate ;
    owl:inverseOf :isModificationDateOf ;
    skos:changeNote
        [
            dc:date "2023-11-02" ;
            rdf:value "Added a new rdfs:label in Spanish."@en ;
        ] ,
        [
            dc:date "2023-08-28" ;
            rdf:value "Added a new rdfs:label in French."@en ;
        ] ;
    :RiCCMCorrespondingComponent """RiC-R073i ('has modification date'
         relation)"""@en ;
.

:hasOrHadDemographicGroup
    a owl:ObjectProperty ;
    rdfs:label
        "has or had demographic group"@en ,
        "tiene o tenía como categoría demográfica"@es ,
        "a ou a eu pour catégorie démographique"@fr ;
    rdfs:comment """Connects a Person or a Group to a Demographic Group to which it
         belongs or belonged."""@en ;
    rdfs:domain
        [
            a owl:Class ;
            owl:unionOf (
                :Group
                :Person
            ) ;
        ] ;
    rdfs:isDefinedBy <https://www.ica.org/standards/RiC/ontology> ;
    rdfs:range :DemographicGroup ;
    rdfs:subPropertyOf :hasOrHadCategory ;
    owl:inverseOf :isOrWasDemographicGroupOf ;
    skos:changeNote
        [
            dc:date "2023-08-28" ;
            rdf:value "Added a new rdfs:label in French."@en ;
        ] ,
        [
            dc:date "2021-01-22" ;
            rdf:value """changed the IRI, label, inverse property IRI, text definition,
               domain (the name of this property in RiC-O 0.1 was
               "belongsToDemographicGroup")."""@en ;
        ] ,
        [
            dc:date "2023-11-02" ;
            rdf:value "Added a new rdfs:label in Spanish."@en ;
        ] ;
.

:hasOrHadDerivedInstantiation
    a owl:ObjectProperty ;
    rdfs:label
        "has or had derived instantiation"@en ,
        "tiene o tenía como instanciación derivada"@es ,
        "a ou a eu pour instanciation dérivée"@fr ;
    rdfs:comment """Connects an instantiation to an instantiation that is derived from
         it, whether it exists or has been lost or destroyed."""@en ;
    rdfs:domain :Instantiation ;
    rdfs:isDefinedBy <https://www.ica.org/standards/RiC/ontology> ;
    rdfs:range :Instantiation ;
    rdfs:subPropertyOf
        :isInstantiationAssociatedWithInstantiation ,
        :precedesInTime ;
    owl:inverseOf :isOrWasDerivedFromInstantiation ;
    owl:propertyChainAxiom (
        :thingIsSourceOfRelation
        :derivationRelation_role
        :relationHasTarget
    ) ;
    skos:changeNote
        [
            dc:date "2023-08-28" ;
            rdf:value "Added a new rdfs:label in French."@en ;
        ] ,
        [
            dc:date "2023-08-29" ;
            rdf:value """Updated the IRI, inverse property, definition, labels and
               RiCMCorrespondingComponent, and added a skos:scopeNote; this in order to make the
               specification compliant with RiC-CM 1.0. The name of the property in RiC-O 0.2 was
               'has derived instantiation'."""@en ;
        ] ,
        [
            dc:date "2023-11-27" ;
            rdf:value "Added a new rdfs:label in Spanish."@en ;
        ] ,
        [
            dc:date "2023-11-08" ;
            rdf:value """In order to get a system of rolified Relation classes: modified
               the property chain axiom so that it now involves the new derivationRelation_role
               object property."""@en ;
        ] ;
    skos:scopeNote """In some situations, it may be useful or necessary to connect an
         instantiation to an instantiation that was derived from it but no longer exists or or has
         been lost."""@en ;
    :RiCCMCorrespondingComponent """RiC-R014 ('has or had derived instantiation'
         relation)"""@en ;
.

:hasOrHadLocation
    a owl:ObjectProperty ;
    rdfs:label
        "has or had location"@en ,
        "tiene o tenía como localización"@es ,
        "a ou a eu pour localisation"@fr ;
    rdfs:comment "Inverse of 'is or was location of' object property."@en ;
    rdfs:domain :Thing ;
    rdfs:isDefinedBy <https://www.ica.org/standards/RiC/ontology> ;
    rdfs:range :Place ;
    rdfs:subPropertyOf :isAssociatedWithPlace ;
    owl:inverseOf :isOrWasLocationOf ;
    skos:changeNote
        [
            dc:date "2021-01-22" ;
            rdf:value """changed the IRI, label, inverse property IRI and textual
               definition (changed made in order to make RiC-O compliant with RiC-CM 0.2; the name
               of this property in RiC-O 0.1 was "hasLocation")."""@en ;
        ] ,
        [
            dc:date "2023-08-28" ;
            rdf:value "Added a new rdfs:label in French."@en ;
        ] ,
        [
            dc:date "2023-11-02" ;
            rdf:value "Added a new rdfs:label in Spanish."@en ;
        ] ;
    :RiCCMCorrespondingComponent """RiC-R075i ('has or had location'
         relation)"""@en ;
.

:hasOrHadManager
    a owl:ObjectProperty ;
    rdfs:label
        "has or had manager"@en ,
        "tiene o tenía como gestor a"@es ,
        "a ou a eu pour gestionnaire"@fr ;
    rdfs:comment "Inverse of 'is or was manager of' object property."@en ;
    rdfs:domain
        [
            a owl:Class ;
            owl:unionOf (
                :Instantiation
                :RecordResource
            ) ;
        ] ;
    rdfs:isDefinedBy <https://www.ica.org/standards/RiC/ontology> ;
    rdfs:range :Agent ;
    rdfs:subPropertyOf :isOrWasUnderAuthorityOf ;
    owl:inverseOf :isOrWasManagerOf ;
    owl:propertyChainAxiom (
        :thingIsTargetOfRelation
        :managementRelation_role
        :relationHasSource
    ) ;
    skos:changeNote
        [
            dc:date "2023-11-02" ;
            rdf:value "Added a new rdfs:label in Spanish."@en ;
        ] ,
        [
            dc:date "2021-01-22" ;
            rdf:value """changed the IRI, label, inverse property IRI, text definition,
               super property IRI (changed made in order to make RiC-O compliant with RiC-CM 0.2;
               the name of this property in RiC-O 0.1 was "managedBy")."""@en ;
        ] ,
        [
            dc:date "2023-08-28" ;
            rdf:value "Added a new rdfs:label in French."@en ;
        ] ,
        [
            dc:date "2023-11-08" ;
            rdf:value """In order to get a system of rolified Relation classes: modified
               the property chain axiom so that it now involves the new managementRelation_role
               object property."""@en ;
        ] ;
    :RiCCMCorrespondingComponent """RiC-R038i ('is or was managed by'
         relation)"""@en ;
.

:hasOrHadRuleType
    a owl:ObjectProperty ;
    rdfs:label
        "has or had rule type"@en ,
        "tiene o tenía como tipo de regla"@es ,
        "a ou a eu pour type de règle"@fr ;
    rdfs:comment """Connects a Rule to a Rule Type that categorized or categorizes
         it."""@en ;
    rdfs:domain :Rule ;
    rdfs:isDefinedBy <https://www.ica.org/standards/RiC/ontology> ;
    rdfs:range :RuleType ;
    rdfs:subPropertyOf :hasOrHadCategory ;
    owl:inverseOf :isOrWasRuleTypeOf ;
    skos:changeNote
        [
            dc:date "2021-01-22" ;
            rdf:value """changed the IRI, label, inverse property IRI, text definition,
               super property IRI (the name of this property in RiC-O 0.1 was
               "hasRuleType")."""@en ;
        ] ,
        [
            dc:date "2023-11-02" ;
            rdf:value "Added a new rdfs:label in Spanish."@en ;
        ] ,
        [
            dc:date "2020-10-19" ;
            rdf:value """Object property added along with RuleType class and
               isRuleTypeOf object property. """@en ;
        ] ,
        [
            dc:date "2023-08-28" ;
            rdf:value "Added a new rdfs:label in French."@en ;
        ] ;
.

:hasOrHadSomeMembersWithCreationDate
    a owl:ObjectProperty ;
    rdfs:label
        "has or had some members with creation date"@en ,
        """tienen o tenían algunos de sus miembros como fecha de
         creación"""@es ,
        """inclut ou a inclus des membres ayant pour date de
         création"""@fr ;
    rdfs:comment """Inverse of 'is or was creation date of some members of' object
         property"""@en ;
    rdfs:domain :RecordSet ;
    rdfs:isDefinedBy <https://www.ica.org/standards/RiC/ontology> ;
    rdfs:range :Date ;
    rdfs:subPropertyOf :hasBeginningDate ;
    owl:inverseOf :isOrWasCreationDateOfSomeMembersOf ;
    skos:changeNote
        [
            dc:date "2023-09-22" ;
            rdf:value "Added in RiC-O 1.0."@en ;
        ] ,
        [
            dc:date "2023-10-13" ;
            rdf:value """Renamed the property in order to take the past members of the
               record set into account. Adjusted the annotations accordingly."""@en ;
        ] ,
        [
            dc:date "2023-11-27" ;
            rdf:value "Added a new rdfs:label in Spanish."@en ;
        ] ,
        [
            dc:date "2023-10-12" ;
            rdf:value "Added the French label"@en ;
        ] ;
    :RiCCMCorrespondingComponent """RiC-R082i ('has or had some members with creation
         date' relation)"""@en ;
.

:hasSubdivisionTransitive
    a
        owl:ObjectProperty ,
        owl:TransitiveProperty ;
    rdfs:label
        "has subdivision transitive"@en ,
        "tiene como subdivisión transitivo"@es ,
        "a pour subdivision transitif"@fr ;
    rdfs:comment """Connects a Group to another Group that is one of its direct or
         indirect subdivisions. This is a transitive relation."""@en ;
    rdfs:domain :Group ;
    rdfs:isDefinedBy <https://www.ica.org/standards/RiC/ontology> ;
    rdfs:range :Group ;
    rdfs:subPropertyOf
        :hasOrHadSubdivision ,
        :hasPartTransitive ,
        :hasSubordinateTransitive ;
    owl:inverseOf :isSubdivisionOfTransitive ;
    skos:changeNote
        [
            dc:date "2023-11-27" ;
            rdf:value "Added a new rdfs:label in Spanish."@en ;
        ] ,
        [
            dc:date "2023-11-25" ;
            rdf:value "Fixed the French label."@en ;
        ] ,
        [
            dc:date "2023-11-12" ;
            rdf:value "Updated the labels."@en ;
        ] ,
        [
            dc:date "2023-09-08" ;
            rdf:value """Object property added, along with its inverse property, in
               order to enable to express current partitive relations between groups (the past
               partitive relation also being added)."""@en ;
        ] ;
.

:hasSubeventTransitive
    a
        owl:ObjectProperty ,
        owl:TransitiveProperty ;
    rdfs:label
        "has subevent transitive"@en ,
        "como parte de evento transitivo"@es ,
        "est constitué de l’événement transitif"@fr ;
    rdfs:comment """Connects an ongoing Event to one of a series of Events that
         directly or indirectly constitute that broader, ongoing Event. This is a transitive
         relation."""@en ;
    rdfs:domain :Event ;
    rdfs:isDefinedBy <https://www.ica.org/standards/RiC/ontology> ;
    rdfs:range :Event ;
    rdfs:subPropertyOf
        :hasOrHadSubevent ,
        :hasPartTransitive ;
    owl:inverseOf :isSubeventOfTransitive ;
    skos:changeNote
        [
            dc:date "2023-11-12" ;
            rdf:value "Updated the labels."@en ;
        ] ,
        [
            dc:date "2023-11-27" ;
            rdf:value "Added a new rdfs:label in Spanish."@en ;
        ] ,
        [
            dc:date "2023-09-08" ;
            rdf:value """Object property added, along with its inverse property, in
               order to enable to express partitive relations between ongoing events (the past
               partitive relation also being added)."""@en ;
        ] ;
.

:includesTransitive
    a
        owl:ObjectProperty ,
        owl:TransitiveProperty ;
    rdfs:label
        "includes transitive"@en ,
        "incluye transitivo"@es ,
        "inclut transitif"@fr ;
    rdfs:comment """Connects a Record Set to a Record or Record Set which it includes
         directly or indirectly. This is a transitive relation."""@en ;
    rdfs:domain :RecordSet ;
    rdfs:isDefinedBy <https://www.ica.org/standards/RiC/ontology> ;
    rdfs:range
        [
            a owl:Class ;
            owl:unionOf (
                :Record
                :RecordSet
            ) ;
        ] ;
    rdfs:subPropertyOf
        :hasPartTransitive ,
        :includesOrIncluded ;
    owl:inverseOf :isIncludedInTransitive ;
    skos:changeNote
        [
            dc:date "2023-11-27" ;
            rdf:value "Added a new rdfs:label in Spanish."@en ;
        ] ,
        [
            dc:date "2023-09-08" ;
            rdf:value """Object property added, along with its inverse property, in
               order to enable to express current partitive relations between Record Sets and their
               members (the past partitive relation also being added)."""@en ;
        ] ,
        [
            dc:date "2023-11-13" ;
            rdf:value "Added two labels."@en ;
        ] ;
.

:isComponentOfTransitive
    a
        owl:ObjectProperty ,
        owl:TransitiveProperty ;
    rdfs:label
        "is component of transitive"@en ,
        "es componente de transitivo"@es ,
        "est un composant de transitif"@fr ;
    rdfs:comment """Connects an Instantiation to another Instantiation of which it is,
         directly or indirectly, a component. This is a transitive relation."""@en ;
    rdfs:domain :Instantiation ;
    rdfs:isDefinedBy <https://www.ica.org/standards/RiC/ontology> ;
    rdfs:range :Instantiation ;
    rdfs:subPropertyOf
        :isOrWasComponentOf ,
        :isPartOfTransitive ;
    owl:inverseOf :hasComponentTransitive ;
    skos:changeNote
        [
            dc:date "2023-09-08" ;
            rdf:value """Object property added, along with its inverse property, in
               order to enable to express current partitive relations between instantiations (the
               past partitive relation also being added)."""@en ;
        ] ,
        [
            dc:date "2023-11-12" ;
            rdf:value "Updated the labels."@en ;
        ] ,
        [
            dc:date "2023-11-27" ;
            rdf:value "Added a new rdfs:label in Spanish."@en ;
        ] ;
.

:isConstituentOfTransitive
    a
        owl:ObjectProperty ,
        owl:TransitiveProperty ;
    rdfs:label
        "is constituent of transitive"@en ,
        "es elemento constitutivo de transitivo"@es ,
        "est le constituant de transitif"@fr ;
    rdfs:comment """Connects a Record or Record Part to another Record or Record Part
         of which it is a constituent, directly or indirectly. This is a transitive
         relation."""@en ;
    rdfs:domain
        [
            a owl:Class ;
            owl:unionOf (
                :Record
                :RecordPart
            ) ;
        ] ;
    rdfs:isDefinedBy <https://www.ica.org/standards/RiC/ontology> ;
    rdfs:range
        [
            a owl:Class ;
            owl:unionOf (
                :Record
                :RecordPart
            ) ;
        ] ;
    rdfs:subPropertyOf
        :isOrWasConstituentOf ,
        :isPartOfTransitive ;
    owl:inverseOf :hasConstituentTransitive ;
    skos:changeNote
        [
            dc:date "2023-11-12" ;
            rdf:value "Updated the labels."@en ;
        ] ,
        [
            dc:date "2023-10-26" ;
            rdf:value "Added RecordPart to the range."@en ;
        ] ,
        [
            dc:date "2023-11-27" ;
            rdf:value "Added a new rdfs:label in Spanish."@en ;
        ] ,
        [
            dc:date "2023-09-08" ;
            rdf:value """Object property added, along with its inverse property, in
               order to enable to express current partitive relations between records and other
               records or record parts (the past partitive relation also being added)."""@en ;
        ] ;
.

:isContainedByTransitive
    a
        owl:ObjectProperty ,
        owl:TransitiveProperty ;
    rdfs:label
        "is contained by transitive"@en ,
        "está contenido en transitivo"@es ,
        "est contenu par transitif"@fr ;
    rdfs:comment """Connects a Place to a Place that is, directly or indirectly,
         contained by it. This is a transitive relation."""@en ;
    rdfs:domain :Place ;
    rdfs:isDefinedBy <https://www.ica.org/standards/RiC/ontology> ;
    rdfs:range :Place ;
    rdfs:subPropertyOf
        :isOrWasContainedBy ,
        :isPartOfTransitive ;
    owl:inverseOf :containsTransitive ;
    skos:changeNote
        [
            dc:date "2023-09-08" ;
            rdf:value """Object property added, along with its inverse property, in
               order to enable to express current partitive relations between places (the past
               partitive relation also being added)."""@en ;
        ] ,
        [
            dc:date "2023-11-12" ;
            rdf:value "Updated the labels."@en ;
        ] ,
        [
            dc:date "2023-11-27" ;
            rdf:value "Added a new rdfs:label in Spanish."@en ;
        ] ;
.

:isCreatorOf
    a owl:ObjectProperty ;
    rdfs:label
        "is creator of"@en ,
        "es creador(a) de"@es ,
        "est le créateur de"@fr ;
    rdfs:comment "Inverse of 'has creator' object property."@en ;
    rdfs:domain :Agent ;
    rdfs:isDefinedBy <https://www.ica.org/standards/RiC/ontology> ;
    rdfs:range
        [
            a owl:Class ;
            owl:unionOf (
                :Instantiation
                :RecordResource
            ) ;
        ] ;
    rdfs:subPropertyOf :isOrganicProvenanceOf ;
    owl:inverseOf :hasCreator ;
    owl:propertyChainAxiom (
        :thingIsTargetOfRelation
        :creationRelation_role
        :relationHasSource
    ) ;
    skos:changeNote
        [
            dc:date "2023-11-02" ;
            rdf:value "Added a new rdfs:label in Spanish."@en ;
        ] ,
        [
            dc:date "2021-01-22" ;
            rdf:value "change the inverse property IRI."@en ;
        ] ,
        [
            dc:date "2023-11-08" ;
            rdf:value """In order to get a system of rolified Relation classes: modified
               the property chain axiom so that it now involves the new creationRelation_role object
               property."""@en ;
        ] ,
        [
            dc:date "2023-08-28" ;
            rdf:value "Added a new rdfs:label in French."@en ;
        ] ;
    :RiCCMCorrespondingComponent """RiC-R027i ('is creator of
         'relation')"""@en ;
.

:isDirectSubordinateTo
    a owl:ObjectProperty ;
    rdfs:label
        "is direct subordinate to"@en ,
        "está directamente subordinado(a) a"@es ,
        "est directement subalterne de"@fr ;
    rdfs:comment """Connects an Agent to an Agent that is directly hierarchically
         superior."""@en ;
    rdfs:domain :Agent ;
    rdfs:isDefinedBy <https://www.ica.org/standards/RiC/ontology> ;
    rdfs:range :Agent ;
    rdfs:subPropertyOf :isSubordinateToTransitive ;
    owl:inverseOf :hasDirectSubordinate ;
    skos:changeNote
        [
            dc:date "2023-11-27" ;
            rdf:value "Added a new rdfs:label in Spanish."@en ;
        ] ,
        [
            dc:date "2023-11-12" ;
            rdf:value "Updated the labels."@en ;
        ] ,
        [
            dc:date "2023-09-08" ;
            rdf:value """Object property added, along with its inverse property, in
               order to enable to express current, direct, subordination relations between agents
               (the possibly indirect, transitive relation, superproperty of this one, being also
               added)."""@en ;
        ] ;
.

:isIncludedInTransitive
    a
        owl:ObjectProperty ,
        owl:TransitiveProperty ;
    rdfs:label
        "is included in transitive"@en ,
        "está incluido en transitivo"@es ,
        "est inclus dans transitif"@fr ;
    rdfs:comment """Connects a Record to a Record or Record Set in which it is
         directly or indirectly included. This is a transitive relation."""@en ;
    rdfs:domain
        [
            a owl:Class ;
            owl:unionOf (
                :Record
                :RecordSet
            ) ;
        ] ;
    rdfs:isDefinedBy <https://www.ica.org/standards/RiC/ontology> ;
    rdfs:range :RecordSet ;
    rdfs:subPropertyOf
        :isOrWasIncludedIn ,
        :isPartOfTransitive ;
    owl:inverseOf :includesTransitive ;
    skos:changeNote
        [
            dc:date "2023-11-13" ;
            rdf:value "Added a French label."@en ;
        ] ,
        [
            dc:date "2023-11-27" ;
            rdf:value "Added a new rdfs:label in Spanish."@en ;
        ] ,
        [
            dc:date "2023-09-08" ;
            rdf:value """Object property added, along with its inverse property, in
               order to enable to express current partitive relations between Record Sets and their
               members (the past partitive relation also being added)."""@en ;
        ] ;
.

:isModificationDateOf
    a owl:ObjectProperty ;
    rdfs:label
        "is modification date of"@en ,
        "es fecha de modificación de"@es ,
        "est une date de modification de"@fr ;
    rdfs:comment """Connects a Date to a Thing that was modified on that
         Date."""@en ;
    rdfs:domain :Date ;
    rdfs:isDefinedBy <https://www.ica.org/standards/RiC/ontology> ;
    rdfs:range :Thing ;
    rdfs:subPropertyOf :isDateAssociatedWith ;
    owl:inverseOf :hasModificationDate ;
    skos:changeNote
        [
            dc:date "2023-08-28" ;
            rdf:value "Added a new rdfs:label in French."@en ;
        ] ,
        [
            dc:date "2023-11-02" ;
            rdf:value "Added a new rdfs:label in Spanish."@en ;
        ] ;
    :RiCCMCorrespondingComponent """RiC-R073 ('is modification date of'
         relation)"""@en ;
.

:isOrWasCreationDateOfSomeMembersOf
    a owl:ObjectProperty ;
    rdfs:label
        "is or was creation date of some members of"@en ,
        "es o era fecha de creación de algunos miembros de"@es ,
        "est ou a été la date de création de certains membres de"@fr ;
    rdfs:comment """Connects a Date to a Record Set some of whose present or past
         members were created at this Date."""@en ;
    rdfs:domain :Date ;
    rdfs:isDefinedBy <https://www.ica.org/standards/RiC/ontology> ;
    rdfs:range :RecordSet ;
    rdfs:subPropertyOf :isBeginningDateOf ;
    owl:inverseOf :hasOrHadSomeMembersWithCreationDate ;
    skos:changeNote
        [
            dc:date "2023-09-22" ;
            rdf:value "Added in RiC-O 1.0."@en ;
        ] ,
        [
            dc:date "2023-11-27" ;
            rdf:value "Added a new rdfs:label in Spanish."@en ;
        ] ,
        [
            dc:date "2023-10-13" ;
            rdf:value """Renamed the property in order to take the past members of the
               record set into account. Adjusted the annotations accordingly."""@en ;
        ] ,
        [
            dc:date "2023-10-12" ;
            rdf:value "Added the French label and the rdfs:comment"@en ;
        ] ;
    :RiCCMCorrespondingComponent """RiC-R082 ('is or was creation date of some members
         of' relation)"""@en ;
.

:isOrWasDemographicGroupOf
    a owl:ObjectProperty ;
    rdfs:label
        "is or was demographic group of"@en ,
        "es o era grupo demográfico de"@es ,
        "est ou a été la catégorie démographique de"@fr ;
    rdfs:comment """Connects a Demographic Group to a Person or Group which belongs or
         belonged to it."""@en ;
    rdfs:domain :DemographicGroup ;
    rdfs:isDefinedBy <https://www.ica.org/standards/RiC/ontology> ;
    rdfs:range
        [
            a owl:Class ;
            owl:unionOf (
                :Group
                :Person
            ) ;
        ] ;
    rdfs:subPropertyOf :isOrWasCategoryOf ;
    owl:inverseOf :hasOrHadDemographicGroup ;
    skos:changeNote
        [
            dc:date "2023-11-02" ;
            rdf:value "Added a new rdfs:label in Spanish."@en ;
        ] ,
        [
            dc:date "2023-08-28" ;
            rdf:value "Added a new rdfs:label in French."@en ;
        ] ,
        [
            dc:date "2021-01-22" ;
            rdf:value """changed the IRI, label, inverse property IRI, text definition,
               range (the name of this property in RiC-O 0.1 was
               "isDemographicGroupOf")."""@en ;
        ] ;
.

:isOrWasDerivedFromInstantiation
    a owl:ObjectProperty ;
    rdfs:label
        "is or was derived from instantiation"@en ,
        "es o era un derivado de instanciación"@es ,
        "est ou a été une instanciation dérivée de"@fr ;
    rdfs:comment """Inverse of 'has or had derived instantiation' object
         property."""@en ;
    rdfs:domain :Instantiation ;
    rdfs:isDefinedBy <https://www.ica.org/standards/RiC/ontology> ;
    rdfs:range :Instantiation ;
    rdfs:subPropertyOf
        :followsInTime ,
        :isInstantiationAssociatedWithInstantiation ;
    owl:inverseOf :hasOrHadDerivedInstantiation ;
    owl:propertyChainAxiom (
        :thingIsTargetOfRelation
        :derivationRelation_role
        :relationHasSource
    ) ;
    skos:changeNote
        [
            dc:date "2023-11-07" ;
            rdf:value """Added the property chain axiom so that this property is
               formally defined as a shortcut (the inverse property already was)."""@en ;
        ] ,
        [
            dc:date "2023-11-27" ;
            rdf:value "Added a new rdfs:label in Spanish."@en ;
        ] ,
        [
            dc:date "2023-08-28" ;
            rdf:value "Added a new rdfs:label in French."@en ;
        ] ,
        [
            dc:date "2023-11-08" ;
            rdf:value """In order to get a system of rolified Relation classes: modified
               the property chain axiom so that it now involves the new derivationRelation_role
               object property."""@en ;
        ] ,
        [
            dc:date "2023-08-29" ;
            rdf:value """Updated the IRI, inverse property, definition, labels and
               RiCMCorrespondingComponent; this in order to make the specification compliant with
               RiC-CM 1.0. The name of the property in RiC-O 0.2 was 'is derived from
               instantiation'."""@en ;
        ] ;
    :RiCCMCorrespondingComponent """RiC-R014i ('is or was derived from instantiation'
         relation)"""@en ;
.

:isOrWasLocationOf
    a owl:ObjectProperty ;
    rdfs:label
        "is or was location of"@en ,
        "es o era localización de"@es ,
        "est ou a été la localisation de"@fr ;
    rdfs:comment """Connects a Place to a Thing that is or was located in the
         Place."""@en ;
    rdfs:domain :Place ;
    rdfs:isDefinedBy <https://www.ica.org/standards/RiC/ontology> ;
    rdfs:range :Thing ;
    rdfs:subPropertyOf :isPlaceAssociatedWith ;
    owl:inverseOf :hasOrHadLocation ;
    skos:changeNote
        [
            dc:date "2021-01-22" ;
            rdf:value """changed the IRI, label, inverse property IRI, textual
               definition (changed made in order to make RiC-O compliant with RiC-CM 0.2; the name
               of this property in RiC-O 0.1 was "isLocationOf")."""@en ;
        ] ,
        [
            dc:date "2023-08-28" ;
            rdf:value "Added a new rdfs:label in French."@en ;
        ] ,
        [
            dc:date "2023-11-02" ;
            rdf:value "Added a new rdfs:label in Spanish."@en ;
        ] ;
    :RiCCMCorrespondingComponent """RiC-R075 ('is or was location of'
         relation)"""@en ;
.

:isOrWasManagerOf
    a owl:ObjectProperty ;
    rdfs:label
        "is or was manager of"@en ,
        "es o era gestor de"@es ,
        "est ou a été le gestionnaire de"@fr ;
    rdfs:comment """Connects an Agent to a Record Resource or Instantiation that the
         Agent managed or manages."""@en ;
    rdfs:domain :Agent ;
    rdfs:isDefinedBy <https://www.ica.org/standards/RiC/ontology> ;
    rdfs:range
        [
            a owl:Class ;
            owl:unionOf (
                :Instantiation
                :RecordResource
            ) ;
        ] ;
    rdfs:subPropertyOf :hasOrHadAuthorityOver ;
    owl:inverseOf :hasOrHadManager ;
    owl:propertyChainAxiom (
        :thingIsSourceOfRelation
        :managementRelation_role
        :relationHasTarget
    ) ;
    skos:changeNote
        [
            dc:date "2021-01-22" ;
            rdf:value """changed the IRI, label, inverse property IRI, super property
               IRI, textual definition (changed made in order to make RiC-O compliant with RiC-CM
               0.2; the name of this property in RiC-O 0.1 was "isManagerOf")."""@en ;
        ] ,
        [
            dc:date "2023-11-08" ;
            rdf:value """In order to get a system of rolified Relation classes: modified
               the property chain axiom so that it now involves the new managementRelation_role
               object property."""@en ;
        ] ,
        [
            dc:date "2023-08-28" ;
            rdf:value "Added a new rdfs:label in French."@en ;
        ] ,
        [
            dc:date "2023-11-02" ;
            rdf:value "Added a new rdfs:label in Spanish."@en ;
        ] ;
    :RiCCMCorrespondingComponent """RiC-R038 ('is or was manager of'
         relation)"""@en ;
.

:isOrWasRuleTypeOf
    a owl:ObjectProperty ;
    rdfs:label
        "is or was rule type of"@en ,
        "es o era tipo de regla de"@es ,
        "est ou a été le type de règle de"@fr ;
    rdfs:comment """Connects a Rule Type to a Rule that it categorized or
         categorizes."""@en ;
    rdfs:domain :RuleType ;
    rdfs:isDefinedBy <https://www.ica.org/standards/RiC/ontology> ;
    rdfs:range :Rule ;
    rdfs:subPropertyOf :isOrWasCategoryOf ;
    owl:inverseOf :hasOrHadRuleType ;
    skos:changeNote
        [
            dc:date "2023-11-02" ;
            rdf:value "Added a new rdfs:label in Spanish."@en ;
        ] ,
        [
            dc:date "2024-03-15" ;
            rdf:value "Make capitalisation of rdfs:comment consistent."@en ;
        ] ,
        [
            dc:date "2023-08-28" ;
            rdf:value "Added a new rdfs:label in French."@en ;
        ] ,
        [
            dc:date "2020-10-19" ;
            rdf:value """Object property added along with RuleType class and hasRuleType
               object property. """@en ;
        ] ,
        [
            dc:date "2021-01-22" ;
            rdf:value """changed the IRI, label, inverse property IRI, text definition,
               super property URI (the name of this property in RiC-O 0.1 was
               "isRuleTypeOf")."""@en ;
        ] ;
.

:isSubdivisionOfTransitive
    a
        owl:ObjectProperty ,
        owl:TransitiveProperty ;
    rdfs:label
        "is subdivision of transitive"@en ,
        "es subdivisión de transitivo"@es ,
        "est une subdivision de transitif"@fr ;
    rdfs:comment """Connects a Group to the Group it is a direct or indirect
         subdivision of. This is a transitive relation."""@en ;
    rdfs:domain :Group ;
    rdfs:isDefinedBy <https://www.ica.org/standards/RiC/ontology> ;
    rdfs:range :Group ;
    rdfs:subPropertyOf
        :isOrWasSubdivisionOf ,
        :isPartOfTransitive ,
        :isSubordinateToTransitive ;
    owl:inverseOf :hasSubdivisionTransitive ;
    skos:changeNote
        [
            dc:date "2023-11-12" ;
            rdf:value "Updated the labels."@en ;
        ] ,
        [
            dc:date "2023-11-27" ;
            rdf:value "Added a new rdfs:label in Spanish."@en ;
        ] ,
        [
            dc:date "2023-09-08"@en ;
            rdf:value """Object property added, along with its inverse property, in
               order to enable to express current partitive relations between groups (the past
               partitive relation also being added)."""@en ;
        ] ;
.

:isSubeventOfTransitive
    a
        owl:ObjectProperty ,
        owl:TransitiveProperty ;
    rdfs:label
        "is subevent of transitive"@en ,
        "es elemento constitutivo de transitivo"@es ,
        "est un événement constituant de transitif"@fr ;
    rdfs:comment """Connects an ongoing Event to an Event of which it is a direct or
         indirect part. This is a transitive relation."""@en ;
    rdfs:domain :Event ;
    rdfs:isDefinedBy <https://www.ica.org/standards/RiC/ontology> ;
    rdfs:range :Event ;
    rdfs:subPropertyOf
        :isOrWasSubeventOf ,
        :isPartOfTransitive ;
    owl:inverseOf :hasSubeventTransitive ;
    skos:changeNote
        [
            dc:date "2023-11-27" ;
            rdf:value "Added a new rdfs:label in Spanish."@en ;
        ] ,
        [
            dc:date "2023-11-12" ;
            rdf:value "Updated the labels."@en ;
        ] ,
        [
            dc:date "2023-09-08" ;
            rdf:value """Object property added, along with its inverse property, in
               order to enable to express partitive relations between ongoing events (the past
               partitive relation also being added)."""@en ;
        ] ;
.

:leadershipWithPosition
    a owl:ObjectProperty ;
    rdfs:label
        "leadership with position"@en ,
        "liderazgo en puesto"@es ,
        "relation de direction dans le cadre du poste"@fr ;
    rdfs:comment """Connects a Leadership Relation to the Position occupied by the
         leading Person."""@en ;
    rdfs:domain :LeadershipRelation ;
    rdfs:isDefinedBy <https://www.ica.org/standards/RiC/ontology> ;
    rdfs:range :Position ;
    rdfs:subPropertyOf :relationHasContext ;
    owl:inverseOf :positionIsContextOfLeadershipRelation ;
    skos:changeNote
        [
            dc:date "2023-08-28" ;
            rdf:value "Added a new rdfs:label in French."@en ;
        ] ,
        [
            dc:date "2023-11-02" ;
            rdf:value "Added a new rdfs:label in Spanish."@en ;
        ] ;
.

:membershipWithPosition
    a owl:ObjectProperty ;
    rdfs:label
        "membership with position"@en ,
        "membresía en puesto"@es ,
        "relation d’appartenance dans le cadre du poste"@fr ;
    rdfs:comment """Connects a Membership Relation to the Position occupied by the
         member Person(s)."""@en ;
    rdfs:domain :MembershipRelation ;
    rdfs:isDefinedBy <https://www.ica.org/standards/RiC/ontology> ;
    rdfs:range :Position ;
    rdfs:subPropertyOf :relationHasContext ;
    owl:inverseOf :positionIsContextOfMembershipRelation ;
    skos:changeNote
        [
            dc:date "2023-11-02" ;
            rdf:value "Added a new rdfs:label in Spanish."@en ;
        ] ,
        [
            dc:date "2023-08-28" ;
            rdf:value "Added a new rdfs:label in French."@en ;
        ] ;
.

:name
    a owl:DatatypeProperty ;
    rdfs:label
        "name"@en ,
        "nombre"@es ,
        "nom"@fr ;
    rdfs:comment """A label, title or term designating an entity in order to make it
         distinguishable from other similar entities."""@en ;
    rdfs:domain :Thing ;
    rdfs:isDefinedBy <https://www.ica.org/standards/RiC/ontology> ;
    rdfs:range rdfs:Literal ;
    skos:changeNote
        [
            dc:date "2023-11-11" ;
            rdf:value """Aligned with RiC-CM 1.0: updated the description
               (rdfs:comment), skos:scopeNote, examples (skos:example)."""@en ;
        ] ,
        [
            dc:date "2020-11-01" ;
            rdf:value """Text definition updated. Examples added. Objective: to make
               RiC-O compliant with RiC-CM v0.2."""@en ;
        ] ,
        [
            dc:date "2023-08-25" ;
            rdf:value "Added a new rdfs:label in French."@en ;
        ] ,
        [
            dc:date "2023-11-02" ;
            rdf:value "Added a new rdfs:label in Spanish."@en ;
        ] ;
    skos:example
        "D-Day (about a Date or Event)"@en ,
        """Digital copy of the Pomarius archival inventory from 1575 (about
         an Instantiation)"""@en ,
        """Fundraising, University of Glasgow (about an
         Activity)"""@en ,
        "Halloween 2016 (about a Date)"@en ,
        "Nelson Mandela (about a Person)"@en ,
        """Papers of the Earls of Liverpool (about a Record
         Set)"""@en ,
        "Paris (about a Place)"@en ,
        "Prime Minister (about a Position)"@en ,
        "Providing hearing services (about an Activity)"@en ,
        "Sketch Map of the Qatar Peninsula (about a Record)"@en ,
        """The Letter of Neacsu from Campulung to the Mayor of Brasov (about
         a Record)"""@en ;
    skos:scopeNote """Use only if you don't use Name class for handling names.
         Provides brief information about the content or other individual characteristics of the
         entity being described, necessary to distinguish it from other perhaps similar
         entities."""@en ;
    :RiCCMCorrespondingComponent """Corrresponds to RiC-A28 (Name
         attribute)"""@en ;
.

:precedesInSequenceTransitive
    a
        owl:ObjectProperty ,
        owl:TransitiveProperty ;
    rdfs:label
        "precedes in sequence transitive"@en ,
        "precede secuencialmente a transitivo"@es ,
        "précède dans la séquence transitif"@fr ;
    rdfs:comment """Connects a Thing to a Thing that follows it directly or indirectly
         in some non chronological sequence. This is a transitive relation."""@en ;
    rdfs:domain :Thing ;
    rdfs:isDefinedBy <https://www.ica.org/standards/RiC/ontology> ;
    rdfs:range :Thing ;
    rdfs:subPropertyOf :precedesOrPreceded ;
    owl:inverseOf :followsInSequenceTransitive ;
    skos:changeNote
        [
            dc:date "2023-09-08"@en ;
            rdf:value """Object property added, along with its inverse property, in
               order to enable to express current, direct or indirect, sequential relations between
               things (the past sequential relation also being added)."""@en ;
        ] ,
        [
            dc:date "2023-09-22" ;
            rdf:value """Renamed the property and modified its definition (rdfs:comment)
               in order to better distinguish it from precedesInTime."""@en ;
        ] ,
        [
            dc:date "2023-11-27" ;
            rdf:value "Added a new rdfs:label in Spanish."@en ;
        ] ,
        [
            dc:date "2023-11-12" ;
            rdf:value "Updated the labels."@en ;
        ] ;
.

:recordResourceGeneticRelation_role
    a
        owl:ObjectProperty ,
        owl:ReflexiveProperty ;
    rdfs:label
        "has the role of the Record Resource Genetic Relation"@en ,
        """desempeña el papel de la Relación genética entre recursos
         documentales"""@es ,
        """a le rôle de la Relation génétique entre des ressources
         archivistiques"""@fr ;
    rdfs:comment """Connects a RecordResourceGeneticRelation to itself. It is a
         reflexive property, that can stand for an instance of the class when necessary, e.g. when
         you explore a knowledge graph."""@en ;
    rdfs:domain :RecordResourceGeneticRelation ;
    rdfs:isDefinedBy <https://www.ica.org/standards/RiC/ontology> ;
    rdfs:range :RecordResourceGeneticRelation ;
    rdfs:subPropertyOf :recordResourceToRecordResourceRelation_role ;
    skos:changeNote
        [
            dc:date "2023-11-08" ;
            rdf:value """In order to get a system of rolified Relation classes: created
               the object property, with domain and range the RecordResourceGeneticRelation rolified
               class. Declared it as reflexive. Declared it(s) superproperty(ies)."""@en ;
        ] ;
    skos:scopeNote """This property "rolifies" the RecordResourceGeneticRelation
         class. It should be used only when you have to manage instances of the
         RecordResourceGeneticRelation class, to connect each instance to itself, in order to be
         able to infer, using OWL-RL and property paths, the two shortcuts corresponding to this
         n-ary class."""@en ;
.

:referenceSystem
    a owl:DatatypeProperty ;
    rdfs:label
        "reference system"@en ,
        "sistema de referencia"@es ,
        "système de référence"@fr ;
    rdfs:comment """Framework or standard used to represent an
         information."""@en ;
    rdfs:domain :Thing ;
    rdfs:isDefinedBy <https://www.ica.org/standards/RiC/ontology> ;
    rdfs:range rdfs:Literal ;
    skos:changeNote
        [
            dc:date "2023-11-02" ;
            rdf:value "Added a new rdfs:label in Spanish."@en ;
        ] ,
        [
            dc:date "2023-08-25" ;
            rdf:value "Added a new rdfs:label in French."@en ;
        ] ;
.

:resultsOrResultedFrom
    a owl:ObjectProperty ;
    rdfs:label
        "results or resulted from"@en ,
        "resulta o resultaba"@es ,
        "résulte ou a résulté de"@fr ;
    rdfs:comment """Inverse of 'results or resulted in' object
         property."""@en ;
    rdfs:domain :Thing ;
    rdfs:isDefinedBy <https://www.ica.org/standards/RiC/ontology> ;
    rdfs:range :Event ;
    rdfs:subPropertyOf :isAssociatedWithEvent ;
    owl:inverseOf :resultsOrResultedIn ;
    skos:changeNote
        [
            dc:date "2021-01-22" ;
            rdf:value """changed the IRI, label, inverse property IRI, text definition
               (changed made in order to make RiC-O compliant with RiC-CM 0.2; the name of this
               property in RiC-O 0.1 was "resultsFrom")."""@en ;
        ] ,
        [
            dc:date "2023-08-28" ;
            rdf:value "Added a new rdfs:label in French."@en ;
        ] ,
        [
            dc:date "2023-11-02" ;
            rdf:value "Added a new rdfs:label in Spanish."@en ;
        ] ;
    :RiCCMCorrespondingComponent """RiC-R061i ('results or resulted from'
         relation)"""@en ;
.

:resultsOrResultedIn
    a owl:ObjectProperty ;
    rdfs:label
        "results or resulted in"@en ,
        "tiene o tenía como resultado a"@es ,
        "a ou a eu pour résultat"@fr ;
    rdfs:comment """Connects an Event to a Thing that results or resulted from the
         Event."""@en ;
    rdfs:domain :Event ;
    rdfs:isDefinedBy <https://www.ica.org/standards/RiC/ontology> ;
    rdfs:range :Thing ;
    rdfs:subPropertyOf :isEventAssociatedWith ;
    owl:inverseOf :resultsOrResultedFrom ;
    skos:changeNote
        [
            dc:date "2023-08-28" ;
            rdf:value "Added a new rdfs:label in French."@en ;
        ] ,
        [
            dc:date "2023-11-02" ;
            rdf:value "Added a new rdfs:label in Spanish."@en ;
        ] ,
        [
            dc:date "2021-01-22" ;
            rdf:value """changed the IRI, label, inverse property IRI, text definition
               (changed made in order to make RiC-O compliant with RiC-CM 0.2; the name of this
               property in RiC-O 0.1 was "resultsIn")."""@en ;
        ] ;
    :RiCCMCorrespondingComponent """RiC-R061 ('results or resulted in'
         relation)"""@en ;
.

:siblingRelation_role
    a
        owl:ObjectProperty ,
        owl:ReflexiveProperty ;
    rdfs:label
        "has the role of the Sibling Relation"@en ,
        """desempeña el papel de la Relación familiar entre
         hermanos"""@es ,
        "a le rôle de la Relation de fratrie"@fr ;
    rdfs:comment """Connects a SiblingRelation to itself. It is a reflexive property,
         that can stand for an instance of the class when necessary, e.g. when you explore a
         knowledge graph."""@en ;
    rdfs:domain :SiblingRelation ;
    rdfs:isDefinedBy <https://www.ica.org/standards/RiC/ontology> ;
    rdfs:range :SiblingRelation ;
    rdfs:subPropertyOf :familyRelation_role ;
    skos:changeNote
        [
            dc:date "2023-11-08" ;
            rdf:value """In order to get a system of rolified Relation classes: created
               the object property, with domain and range the SiblingRelation rolified class.
               Declared it as reflexive. Declared it(s) superproperty(ies)."""@en ;
        ] ;
    skos:scopeNote """This property "rolifies" the SiblingRelation class. It should be
         used only when you have to manage instances of the SiblingRelation class, to connect each
         instance to itself, in order to be able to infer, using OWL-RL and property paths, the two
         shortcuts corresponding to this n-ary class."""@en ;
.

:spouseRelation_role
    a
        owl:ObjectProperty ,
        owl:ReflexiveProperty ;
    rdfs:label
        "has the role of the Spouse Relation"@en ,
        """desempeña el papel de la Relación matrimonial entre
         personas"""@es ,
        "a le rôle de la Relation matrimoniale"@fr ;
    rdfs:comment """Connects a SpouseRelation to itself. It is a reflexive property,
         that can stand for an instance of the class when necessary, e.g. when you explore a
         knowledge graph."""@en ;
    rdfs:domain :SpouseRelation ;
    rdfs:isDefinedBy <https://www.ica.org/standards/RiC/ontology> ;
    rdfs:range :SpouseRelation ;
    rdfs:subPropertyOf :familyRelation_role ;
    skos:changeNote
        [
            dc:date "2023-11-08" ;
            rdf:value """In order to get a system of rolified Relation classes: created
               the object property, with domain and range the SpouseRelation rolified class.
               Declared it as reflexive. Declared it(s) superproperty(ies)."""@en ;
        ] ;
    skos:scopeNote """This property "rolifies" the SpouseRelation class. It should be
         used only when you have to manage instances of the SpouseRelation class, to connect each
         instance to itself, in order to be able to infer, using OWL-RL and property paths, the two
         shortcuts corresponding to this n-ary class."""@en ;
.

:structure
    a owl:DatatypeProperty ;
    rdfs:label
        "structure"@en ,
        "estructura"@es ,
        "structure"@fr ;
    rdfs:comment """Information about the intellectual arrangement and composition of
         a Record Resource or the physical arrangement and composition of an Instantiation. For
         Record and Record Part, it encompasses information about the intellectual composition of
         the record, the presence of record parts and their functions. For Record Set, it
         encompasses information about the methodology or criteria used for arranging the Record Set
         members or Record members within the containing Record Set. For Instantiation, it may
         comprise information about the composition of the physical elements of the
         instantiation"""@en ;
    rdfs:domain
        [
            a owl:Class ;
            owl:unionOf (
                :Instantiation
                :RecordResource
            ) ;
        ] ;
    rdfs:isDefinedBy <https://www.ica.org/standards/RiC/ontology> ;
    rdfs:range rdfs:Literal ;
    skos:changeNote
        [
            dc:date "2023-08-25" ;
            rdf:value "Added a new rdfs:label in French."@en ;
        ] ,
        [
            dc:date "2023-11-02" ;
            rdf:value "Added a new rdfs:label in Spanish."@en ;
        ] ,
        [
            dc:date "2020-11-01" ;
            rdf:value """Text definition updated. Objective: to make RiC-O compliant
               with RiC-CM v0.2."""@en ;
        ] ,
        [
            dc:date "2023-11-11" ;
            rdf:value """Aligned with RiC-CM 1.0: updated the skos:scopeNote, examples
               (skos:example)."""@en ;
        ] ;
    skos:example
        """Inside each file, the records are arranged chronologically (about
         a record set)"""@en ,
        """The database has three related tables: names, addresses, and
         passport numbers (about a record)"""@en ,
        """The record has two appendices, comprising a full account of the
         income from car taxes and real estate taxes"""@en ,
        """The series have the files arranged according to the alphabetical
         order of the places concerned"""@en ;
    skos:scopeNote """Use only if you cannot use the subproperties (particularly if
         the same free text is being used in your current metadata for describing the record
         resource and the instantiation structure). For a Record Set, may be used to summarize the
         structure of the Record Set itself, or additionally to summarize the structure of some or
         all members of the Record Set. Should not be confused with the classification datatype
         property, which provides information about the category which the Record Set belongs to
         within a classification scheme. """@en ;
    :RiCCMCorrespondingComponent """Corresponds to RiC-A40 (Structure
         attribute)"""@en ;
.

:wasSubordinateTo
    a owl:ObjectProperty ;
    rdfs:label
        "was subordinate to"@en ,
        "estaba subordinado(a) a"@es ,
        "a été subalterne de"@fr ;
    rdfs:comment """Connects an Agent to an Agent that was hierarchically superior in
         the past."""@en ;
    rdfs:domain :Agent ;
    rdfs:isDefinedBy <https://www.ica.org/standards/RiC/ontology> ;
    rdfs:range :Agent ;
    rdfs:subPropertyOf :isOrWasSubordinateTo ;
    owl:inverseOf :hadSubordinate ;
    skos:changeNote
        [
            dc:date "2023-11-12" ;
            rdf:value "Updated the labels."@en ;
        ] ,
        [
            dc:date "2023-11-27" ;
            rdf:value "Added a new rdfs:label in Spanish."@en ;
        ] ,
        [
            dc:date "2023-09-08"@en ;
            rdf:value """Object property added, along with its inverse property, in
               order to enable to express past subordination relations between Agents (the current
               subordination relations being also added, including a transitive one)."""@en ;
        ] ;
.

:workRelation_role
    a
        owl:ObjectProperty ,
        owl:ReflexiveProperty ;
    rdfs:label
        "has the role of the Work Relation"@en ,
        "desempeña el papel de la Relación profesional"@es ,
        "a le rôle de la Relation de travail"@fr ;
    rdfs:comment """Connects a WorkRelation to itself. It is a reflexive property,
         that can stand for an instance of the class when necessary, e.g. when you explore a
         knowledge graph."""@en ;
    rdfs:domain :WorkRelation ;
    rdfs:isDefinedBy <https://www.ica.org/standards/RiC/ontology> ;
    rdfs:range :WorkRelation ;
    rdfs:subPropertyOf :agentToAgentRelation_role ;
    skos:changeNote
        [
            dc:date "2023-11-08" ;
            rdf:value """In order to get a system of rolified Relation classes: created
               the object property, with domain and range the WorkRelation rolified class. Declared
               it as reflexive. Declared it(s) superproperty(ies)."""@en ;
        ] ;
    skos:scopeNote """This property "rolifies" the WorkRelation class. It should be
         used only when you have to manage instances of the WorkRelation class, to connect each
         instance to itself, in order to be able to infer, using OWL-RL and property paths, the two
         shortcuts corresponding to this n-ary class."""@en ;
.

:ActivityType
    a owl:Class ;
    rdfs:label
        "Activity Type"@en ,
        "Tipo de actividad"@es ,
        "Type d’activité"@fr ;
    rdfs:comment "Categorization of an Activity."@en ;
    rdfs:isDefinedBy <https://www.ica.org/standards/RiC/ontology> ;
    rdfs:subClassOf :Type ;
    skos:changeNote
        [
            dc:date "2023-04-19" ;
            rdf:value "Removed the 0.2 existing unnecessary restriction."@en ;
        ] ,
        [
            dc:date "2023-08-25" ;
            rdf:value "Added a new rdfs:label in French."@en ;
        ] ,
        [
            dc:date "2020-10-23" ;
            rdf:value """Scope note: updated (different from RiC-CM scope note).
               Objective: to make RiC-O compliant with RiC-CM v0.2."""@en ;
        ] ,
        [
            dc:date "2023-11-02" ;
            rdf:value "Added a new rdfs:label in Spanish."@en ;
        ] ;
    skos:scopeNote """Can be extended with any number of subclasses, e.g.
         “function/action” and “activity domain”. This allows for a faceted approach that enables an
         Activity to be categorized using a combination of components, general or more specific. For
         example, “monitoring” can be used in combination with “election polls” or “water
         resources”."""@en ;
    :RiCCMCorrespondingComponent """Corresponds to RiC-A02 (Activity Type
         attribute)"""@en ;
.

:AgentControlRelation
    a owl:Class ;
    rdfs:label
        "Agent Control Relation"@en ,
        "Relación de control entre agentes"@es ,
        "Relation de contrôle entre agents"@fr ;
    rdfs:comment """Connects at least one Agent, to at least another Agent, when the
         first one(s) control(s) or controlled in a way the activities of the second one(s). The
         Relation is oriented from the controlling agent to the controlled one: the controlling
         Agent(s) is the source of the Relation, and the controlled Agent(s) is the
         target."""@en ;
    rdfs:isDefinedBy <https://www.ica.org/standards/RiC/ontology> ;
    rdfs:subClassOf
        [
            a owl:Restriction ;
            owl:minQualifiedCardinality "1"^^xsd:nonNegativeInteger ;
            owl:onClass :Agent ;
            owl:onProperty :relationHasSource ;
        ] ,
        [
            a owl:Restriction ;
            owl:minQualifiedCardinality "1"^^xsd:nonNegativeInteger ;
            owl:onClass :Agent ;
            owl:onProperty :relationHasTarget ;
        ] ,
        :AgentHierarchicalRelation ,
        :AuthorityRelation ;
    owl:equivalentClass
        [
            a owl:Restriction ;
            owl:hasSelf true ;
            owl:onProperty :agentControlRelation_role ;
        ] ;
    skos:changeNote
        [
            dc:date "2023-12-06" ;
            rdf:value """Improved the description of the Relation class (rdfs:comment)
               by clearly specifying how it is directed."""@en ;
        ] ,
        [
            dc:date "2023-11-08" ;
            rdf:value """In order to get a system of rolified Relation classes: added an
               equivalentClass object property; replaced the specific object properties by the
               generic ones in the subClassOf declarations."""@en ;
        ] ,
        [
            dc:date "2023-11-12" ;
            rdf:value """Aligned with RiC-CM 1.0: updated the description
               (rdfs:comment)."""@en ;
        ] ,
        [
            dc:date "2023-11-02" ;
            rdf:value "Added a new rdfs:label in Spanish."@en ;
        ] ,
        [
            dc:date "2023-08-25" ;
            rdf:value "Added a new rdfs:label in French."@en ;
        ] ;
    :RiCCMCorrespondingComponent """Class implementation of RiC-R041 and RiC-R041i
         relations"""@en ;
.

:DemographicGroup
    a owl:Class ;
    rdfs:label
        "Demographic Group"@en ,
        "Categoría demográfica"@es ,
        "Catégorie démographique"@fr ;
    rdfs:comment """Categorization of a Person or Group based on shared
         characteristics."""@en ;
    rdfs:isDefinedBy <https://www.ica.org/standards/RiC/ontology> ;
    rdfs:subClassOf :Type ;
    skos:changeNote
        [
            dc:date "2021-02-08"@en ;
            rdf:value "Removed the Restriction."@en ;
        ] ,
        [
            dc:date "2020-10-23" ;
            rdf:value """Comment: updated. Scope note: updated and made several
               paragraphs. Objective: to make RiC-O compliant with RiC-CM v0.2."""@en ;
        ] ,
        [
            dc:date "2023-11-12" ;
            rdf:value """Aligned with RiC-CM 1.0: updated the description
               (rdfs:comment), skos:scopeNote."""@en ;
        ] ,
        [
            dc:date "2023-08-25" ;
            rdf:value "Added a new rdfs:label in French."@en ;
        ] ,
        [
            dc:date "2023-11-02" ;
            rdf:value "Added a new rdfs:label in Spanish."@en ;
        ] ;
    skos:scopeNote """Can be extended with any number of specific subclasses. Among
         possible specific demographic groups are gender, (biological) sex, education, identity,
         place, ancestry, ethnic/cultural identification, and religion."""@en ;
    :RiCCMCorrespondingComponent """Corresponds to RiC-A15 (Demographic Group
         attribute)"""@en ;
.

:DerivationRelation
    a owl:Class ;
    rdfs:label
        "Derivation Relation"@en ,
        "Relación de derivación"@es ,
        "Relation de dérivation"@fr ;
    rdfs:comment """Connects an Instantiation to at least one Instantiation that is
         derived from it, whether it exists or has been lost or destroyed. The Relation is oriented
         chronologically, from the first Instantiation in time to the derived Instantiation: the
         first Instantiation is the source of the Relation, and the derived Instantiation(s) is the
         target."""@en ;
    rdfs:isDefinedBy <https://www.ica.org/standards/RiC/ontology> ;
    rdfs:subClassOf
        [
            a owl:Restriction ;
            owl:minQualifiedCardinality "1"^^xsd:nonNegativeInteger ;
            owl:onClass :Instantiation ;
            owl:onProperty :relationHasTarget ;
        ] ,
        [
            a owl:Restriction ;
            owl:onClass :Instantiation ;
            owl:onProperty :relationHasSource ;
            owl:qualifiedCardinality "1"^^xsd:nonNegativeInteger ;
        ] ,
        :InstantiationToInstantiationRelation ,
        :TemporalRelation ;
    owl:equivalentClass
        [
            a owl:Restriction ;
            owl:hasSelf true ;
            owl:onProperty :derivationRelation_role ;
        ] ;
    skos:changeNote
        [
            dc:date "2023-11-08" ;
            rdf:value """In order to get a system of rolified Relation classes: added an
               equivalentClass object property; replaced the specific object properties by the
               generic ones in the subClassOf declarations."""@en ;
        ] ,
        [
            dc:date "2023-08-25" ;
            rdf:value "Added a new rdfs:label in French."@en ;
        ] ,
        [
            dc:date "2023-12-06" ;
            rdf:value """Improved the description of the Relation class (rdfs:comment)
               by clearly specifying how it is directed."""@en ;
        ] ,
        [
            dc:date "2023-11-02" ;
            rdf:value "Added a new rdfs:label in Spanish."@en ;
        ] ,
        [
            dc:date "2023-11-12" ;
            rdf:value """Aligned with RiC-CM 1.0: updated the description
               (rdfs:comment), skos:scopeNote."""@en ;
        ] ;
    skos:scopeNote """In some situations, it may be useful or necessary to connect an
         instantiation to an instantiation that was derived from it but no longer exists or has been
         lost."""@en ;
    :RiCCMCorrespondingComponent """Class implementation of RiC-R014 and RiR014i
         relations"""@en ;
.

:DescendanceRelation
    a owl:Class ;
    rdfs:label
        "Descendance Relation"@en ,
        "Relación de descendencia"@es ,
        "Relation de descendance"@fr ;
    rdfs:comment """Connects at least one Person to at least another Person, when the
         first has/have descendant the second one(s). The Relation is oriented from the ascendant to
         the descendant: the ascendant Person(s) is the source of the Relation, and the descendant
         Person(s) is the target."""@en ;
    rdfs:isDefinedBy <https://www.ica.org/standards/RiC/ontology> ;
    rdfs:subClassOf
        [
            a owl:Restriction ;
            owl:minQualifiedCardinality "1"^^xsd:nonNegativeInteger ;
            owl:onClass :Person ;
            owl:onProperty :relationHasTarget ;
        ] ,
        [
            a owl:Restriction ;
            owl:minQualifiedCardinality "1"^^xsd:nonNegativeInteger ;
            owl:onClass :Person ;
            owl:onProperty :relationHasSource ;
        ] ,
        :AgentTemporalRelation ,
        :FamilyRelation ;
    owl:equivalentClass
        [
            a owl:Restriction ;
            owl:hasSelf true ;
            owl:onProperty :descendanceRelation_role ;
        ] ;
    skos:changeNote
        [
            dc:date "2023-08-25" ;
            rdf:value "Added a new rdfs:label in French."@en ;
        ] ,
        [
            dc:date "2023-11-02" ;
            rdf:value "Added a new rdfs:label in Spanish."@en ;
        ] ,
        [
            dc:date "2023-11-08" ;
            rdf:value """In order to get a system of rolified Relation classes: added an
               equivalentClass object property; replaced the specific object properties by the
               generic ones in the subClassOf declarations."""@en ;
        ] ,
        [
            dc:date "2023-12-06" ;
            rdf:value """Improved the description of the Relation class (rdfs:comment)
               by clearly specifying how it is directed."""@en ;
        ] ;
    :RiCCMCorrespondingComponent """Class implementation of RiC-R017 and RiC-R017i
         relations"""@en ;
.

:ManagementRelation
    a owl:Class ;
    rdfs:label
        "Management Relation"@en ,
        "Relación de gestión"@es ,
        "Relation de gestion"@fr ;
    rdfs:comment """Connects at least one Agent and at least one Record Resource or
         Instantiation that the Agent manages or managed. The Agent(s) is the source of the
         Relation, and the Record Resource(s) or Instantiation(s) is the target."""@en ;
    rdfs:isDefinedBy <https://www.ica.org/standards/RiC/ontology> ;
    rdfs:subClassOf
        [
            a owl:Restriction ;
            owl:minQualifiedCardinality "1"^^xsd:nonNegativeInteger ;
            owl:onClass :Agent ;
            owl:onProperty :relationHasSource ;
        ] ,
        [
            a owl:Restriction ;
            owl:minQualifiedCardinality "1"^^xsd:nonNegativeInteger ;
            owl:onClass
                [
                    a owl:Class ;
                    owl:unionOf (
                        :Instantiation
                        :RecordResource
                    ) ;
                ] ;
            owl:onProperty :relationHasTarget ;
        ] ,
        :AuthorityRelation ;
    owl:equivalentClass
        [
            a owl:Restriction ;
            owl:hasSelf true ;
            owl:onProperty :managementRelation_role ;
        ] ;
    skos:changeNote
        [
            dc:date "2023-11-02" ;
            rdf:value "Added a new rdfs:label in Spanish."@en ;
        ] ,
        [
            dc:date "2023-11-08" ;
            rdf:value """In order to get a system of rolified Relation classes: added an
               equivalentClass object property; replaced the specific object properties by the
               generic ones in the subClassOf declarations."""@en ;
        ] ,
        [
            dc:date "2023-08-25" ;
            rdf:value "Added a new rdfs:label in French."@en ;
        ] ,
        [
            dc:date "2023-12-06" ;
            rdf:value """Improved the description of the Relation class (rdfs:comment)
               by clearly specifying how it is directed."""@en ;
        ] ,
        [
            dc:date "2023-11-12" ;
            rdf:value """Aligned with RiC-CM 1.0: updated the description
               (rdfs:comment)."""@en ;
        ] ;
    :RiCCMCorrespondingComponent """Class implementation of RiC-R038 and RiC-R038i
         relations"""@en ;
.

:RecordResourceToRecordResourceRelation
    a owl:Class ;
    rdfs:label
        "Record Resource to Record Resource Relation"@en ,
        "Relación entre recursos documentales"@es ,
        "Relation entre ressources archivistiques"@fr ;
    rdfs:comment """Connects at least two Record Resources. This Relation is a
         generic, not oriented one."""@en ;
    rdfs:isDefinedBy <https://www.ica.org/standards/RiC/ontology> ;
    rdfs:subClassOf
        [
            a owl:Restriction ;
            owl:minQualifiedCardinality "2"^^xsd:nonNegativeInteger ;
            owl:onClass :RecordResource ;
            owl:onProperty :relationConnects ;
        ] ,
        :Relation ;
    owl:equivalentClass
        [
            a owl:Restriction ;
            owl:hasSelf true ;
            owl:onProperty :recordResourceToRecordResourceRelation_role ;
        ] ;
    skos:changeNote
        [
            dc:date "2023-11-08" ;
            rdf:value """In order to get a system of rolified Relation classes: added an
               equivalentClass object property; replaced the specific object properties by the
               generic ones in the subClassOf declarations."""@en ;
        ] ,
        [
            dc:date "2023-11-12" ;
            rdf:value """Aligned with RiC-CM 1.0: updated the
               skos:scopeNote."""@en ;
        ] ,
        [
            dc:date "2023-12-06" ;
            rdf:value """Improved the description of the Relation class (rdfs:comment)
               by clearly specifying how it is directed."""@en ;
        ] ,
        [
            dc:date "2023-08-25" ;
            rdf:value "Added a new rdfs:label in French."@en ;
        ] ,
        [
            dc:date "2023-11-02" ;
            rdf:value "Added a new rdfs:label in Spanish."@en ;
        ] ;
    skos:scopeNote """Use to connect two record resources only if it is not possible
         to use a narrower, more specific relation, for example
         RecordResourceGeneticRelation."""@en ;
    :RiCCMCorrespondingComponent """Class implementation of RiC-R022 and RiC-022i
         relations"""@en ;
.

:RuleRelation
    a owl:Class ;
    rdfs:label
        "Rule Relation"@en ,
        "Relación con regla"@es ,
        "Relation impliquant une règle"@fr ;
    rdfs:comment """Connects at least one Rule to at least one Thing when it is
         associated with existence and lifecycle of the Thing. The Rule(s) is the source of the
         Relation, and the Thing(s) is the target."""@en ;
    rdfs:isDefinedBy <https://www.ica.org/standards/RiC/ontology> ;
    rdfs:subClassOf
        [
            a owl:Restriction ;
            owl:minQualifiedCardinality "1"^^xsd:nonNegativeInteger ;
            owl:onClass :Thing ;
            owl:onProperty :relationHasTarget ;
        ] ,
        [
            a owl:Restriction ;
            owl:minQualifiedCardinality "1"^^xsd:nonNegativeInteger ;
            owl:onClass :Rule ;
            owl:onProperty :relationHasSource ;
        ] ,
        :Relation ;
    owl:equivalentClass
        [
            a owl:Restriction ;
            owl:hasSelf true ;
            owl:onProperty :ruleRelation_role ;
        ] ;
    skos:changeNote
        [
            dc:date "2023-11-02" ;
            rdf:value "Added a new rdfs:label in Spanish."@en ;
        ] ,
        [
            dc:date "2023-08-25" ;
            rdf:value "Added a new rdfs:label in French."@en ;
        ] ,
        [
            dc:date "2023-11-08" ;
            rdf:value """In order to get a system of rolified Relation classes: added an
               equivalentClass object property; replaced the specific object properties by the
               generic ones in the subClassOf declarations."""@en ;
        ] ,
        [
            dc:date "2023-12-06" ;
            rdf:value """Improved the description of the Relation class (rdfs:comment)
               by clearly specifying how it is directed."""@en ;
        ] ;
    :RiCCMCorrespondingComponent """Class implementation of RiC-R062 and RiC-R062i
         relations"""@en ;
.

:RuleType
    a owl:Class ;
    rdfs:label
        "Rule Type"@en ,
        "Tipo de regla"@es ,
        "Type de règle"@fr ;
    rdfs:comment "Categorization of a Rule."@en ;
    rdfs:isDefinedBy <https://www.ica.org/standards/RiC/ontology> ;
    rdfs:subClassOf :Type ;
    skos:changeNote
        [
            dc:date "2023-11-12" ;
            rdf:value """Aligned with RiC-CM 1.0: added a
               rico:RiCCMCorrespondingComponent."""@en ;
        ] ,
        [
            dc:date "2020-10-19" ;
            rdf:value """Class added along with hasRuleType and isRuleTypeOf object
               properties."""@en ;
        ] ,
        [
            dc:date "2023-11-02" ;
            rdf:value "Added a new rdfs:label in Spanish."@en ;
        ] ,
        [
            dc:date "2023-08-25" ;
            rdf:value "Added a new rdfs:label in French."@en ;
        ] ,
        [
            dc:date "2023-04-19" ;
            rdf:value "Removed the 0.2 existing unnecessary restriction."@en ;
        ] ;
    skos:scopeNote """For example, for rules that can be applied to record resources :
         access rule, use rule, etc."""@en ;
    :RiCCMCorrespondingComponent """Corresponds to RiC-A45 (Rule Type
         attribute)."""@en ;
.

:SequentialRelation
    a owl:Class ;
    rdfs:label
        "Sequential Relation"@en ,
        "Relación secuencial"@es ,
        "Relation séquentielle"@fr ;
    rdfs:comment """Connects at least one Thing to at least one other Thing that
         follows or followed it in some sequence. The Relation is oriented from the first Thing(s)
         in the sequence to the following one(s): the first Thing(s) is the source, and the
         following Thing(s) is the target."""@en ;
    rdfs:isDefinedBy <https://www.ica.org/standards/RiC/ontology> ;
    rdfs:subClassOf
        [
            a owl:Restriction ;
            owl:minQualifiedCardinality "1"^^xsd:nonNegativeInteger ;
            owl:onClass :Thing ;
            owl:onProperty :relationHasSource ;
        ] ,
        [
            a owl:Restriction ;
            owl:minQualifiedCardinality "1"^^xsd:nonNegativeInteger ;
            owl:onClass :Thing ;
            owl:onProperty :relationHasTarget ;
        ] ,
        :Relation ;
    owl:equivalentClass
        [
            a owl:Restriction ;
            owl:hasSelf true ;
            owl:onProperty :sequentialRelation_role ;
        ] ;
    skos:changeNote
        [
            dc:date "2023-08-25" ;
            rdf:value "Added a new rdfs:label in French."@en ;
        ] ,
        [
            dc:date "2023-11-12" ;
            rdf:value """Aligned with RiC-CM 1.0: updated the description
               (rdfs:comment), skos:scopeNote."""@en ;
        ] ,
        [
            dc:date "2023-11-02" ;
            rdf:value "Added a new rdfs:label in Spanish."@en ;
        ] ,
        [
            dc:date "2023-11-08" ;
            rdf:value """In order to get a system of rolified Relation classes: added an
               equivalentClass object property; replaced the specific object properties by the
               generic ones in the subClassOf declarations."""@en ;
        ] ,
        [
            dc:date "2023-12-06" ;
            rdf:value """Improved the description of the Relation class (rdfs:comment)
               by clearly specifying how it is directed."""@en ;
        ] ;
    skos:scopeNote """The relation does not specify the criteria used for ordering the
         sequence. There may be zero to many intermediate entities, ignored or unknown, in the
         sequence between the two connected things. Can be used, for example, for specifying that a
         record "has next" another record within a record set."""@en ;
    :RiCCMCorrespondingComponent """Class implementation of RiC-R008 and RiC-R008i
         relations"""@en ;
.

:WholePartRelation
    a owl:Class ;
    rdfs:label
        "Whole Part Relation"@en ,
        "Relación entre todo y parte"@es ,
        "Relation partitive"@fr ;
    rdfs:comment """Connects a Thing to at least one other Thing that is or was a
         portion or division of the whole Thing. The Relation is oriented from the Thing to its
         part(s): the Thing is the source of the Relation, and the part Thing(s) is the
         target."""@en ;
    rdfs:isDefinedBy <https://www.ica.org/standards/RiC/ontology> ;
    rdfs:subClassOf
        [
            a owl:Restriction ;
            owl:onClass :Thing ;
            owl:onProperty :relationHasSource ;
            owl:qualifiedCardinality "1"^^xsd:nonNegativeInteger ;
        ] ,
        [
            a owl:Restriction ;
            owl:minQualifiedCardinality "1"^^xsd:nonNegativeInteger ;
            owl:onClass :Thing ;
            owl:onProperty :relationHasTarget ;
        ] ,
        :Relation ;
    owl:equivalentClass
        [
            a owl:Restriction ;
            owl:hasSelf true ;
            owl:onProperty :wholePartRelation_role ;
        ] ;
    skos:changeNote
        [
            dc:date "2023-11-02" ;
            rdf:value "Added a new rdfs:label in Spanish."@en ;
        ] ,
        [
            dc:date "2023-08-25" ;
            rdf:value "Added a new rdfs:label in French."@en ;
        ] ,
        [
            dc:date "2023-11-12" ;
            rdf:value """Aligned with RiC-CM 1.0: updated the description
               (rdfs:comment)."""@en ;
        ] ,
        [
            dc:date "2023-12-06" ;
            rdf:value """Improved the description of the Relation class (rdfs:comment)
               by clearly specifying how it is directed."""@en ;
        ] ,
        [
            dc:date "2023-11-08" ;
            rdf:value """In order to get a system of rolified Relation classes: added an
               equivalentClass object property; replaced the specific object properties by the
               generic ones in the subClassOf declarations."""@en ;
        ] ;
    :RiCCMCorrespondingComponent """Class implementation of RiC-R002 and RiC-R002i
         relations"""@en ;
.

:accumulationRelation_role
    a
        owl:ObjectProperty ,
        owl:ReflexiveProperty ;
    rdfs:label
        "has the role of the Accumulation Relation"@en ,
        "desempeña el papel de la Relación de Acumulación"@es ,
        "a le rôle de la Relation d’accumulation"@fr ;
    rdfs:comment """Connects a AccumulationRelation to itself. It is a reflexive
         property, that can stand for an instance of the class when necessary, e.g. when you explore
         a knowledge graph."""@en ;
    rdfs:domain :AccumulationRelation ;
    rdfs:isDefinedBy <https://www.ica.org/standards/RiC/ontology> ;
    rdfs:range :AccumulationRelation ;
    rdfs:subPropertyOf :organicProvenanceRelation_role ;
    skos:changeNote
        [
            dc:date "2023-11-08" ;
            rdf:value """In order to get a system of rolified Relation classes: created
               the object property, with domain and range the AccumulationRelation rolified class.
               Declared it as reflexive. Declared it(s) superproperty(ies)."""@en ;
        ] ;
    skos:scopeNote """This property "rolifies" the AccumulationRelation class. It
         should be used only when you have to manage instances of the AccumulationRelation class, to
         connect each instance to itself, in order to be able to infer, using OWL-RL and property
         paths, the two shortcuts corresponding to this n-ary class."""@en ;
.

:activityDocumentationRelation_role
    a
        owl:ObjectProperty ,
        owl:ReflexiveProperty ;
    rdfs:label
        "has the role of the Activity Documentation Relation"@en ,
        """desempeña el papel de la Relación de procedencia
         funcional"""@es ,
        """a le rôle de la Relation entre activités et ressources
         archivistiques"""@fr ;
    rdfs:comment """Connects a ActivityDocumentationRelation to itself. It is a
         reflexive property, that can stand for an instance of the class when necessary, e.g. when
         you explore a knowledge graph."""@en ;
    rdfs:domain :ActivityDocumentationRelation ;
    rdfs:isDefinedBy <https://www.ica.org/standards/RiC/ontology> ;
    rdfs:range :ActivityDocumentationRelation ;
    rdfs:subPropertyOf
        :eventRelation_role ,
        :organicOrFunctionalProvenanceRelation_role ;
    skos:changeNote
        [
            dc:date "2023-11-08" ;
            rdf:value """In order to get a system of rolified Relation classes: created
               the object property, with domain and range the ActivityDocumentationRelation rolified
               class. Declared it as reflexive. Declared it(s) superproperty(ies)."""@en ;
        ] ;
    skos:scopeNote """This property "rolifies" the ActivityDocumentationRelation
         class. It should be used only when you have to manage instances of the
         ActivityDocumentationRelation class, to connect each instance to itself, in order to be
         able to infer, using OWL-RL and property paths, the two shortcuts corresponding to this
         n-ary class."""@en ;
.

:appellationRelation_role
    a
        owl:ObjectProperty ,
        owl:ReflexiveProperty ;
    rdfs:label
        "has the role of the Appellation Relation"@en ,
        "desempeña el papel de la Relación de denominación"@es ,
        "a le rôle de la Relation d’appellation"@fr ;
    rdfs:comment """Connects a AppellationRelation to itself. It is a reflexive
         property, that can stand for an instance of the class when necessary, e.g. when you explore
         a knowledge graph."""@en ;
    rdfs:domain :AppellationRelation ;
    rdfs:isDefinedBy <https://www.ica.org/standards/RiC/ontology> ;
    rdfs:range :AppellationRelation ;
    rdfs:subPropertyOf :relation_role ;
    skos:changeNote
        [
            dc:date "2023-11-08" ;
            rdf:value """In order to get a system of rolified Relation classes: created
               the object property, with domain and range the AppellationRelation rolified class.
               Declared it as reflexive. Declared it(s) superproperty(ies)."""@en ;
        ] ;
    skos:scopeNote """This property "rolifies" the AppellationRelation class. It
         should be used only when you have to manage instances of the AppellationRelation class, to
         connect each instance to itself, in order to be able to infer, using OWL-RL and property
         paths, the two shortcuts corresponding to this n-ary class."""@en ;
.

:authorshipRelation_role
    a
        owl:ObjectProperty ,
        owl:ReflexiveProperty ;
    rdfs:label
        "has the role of the Authorship Relation"@en ,
        "desempeña el papel de la Relación de autoría"@es ,
        """a le rôle de la Relation de responsabilité
         intellectuelle"""@fr ;
    rdfs:comment """Connects a AuthorshipRelation to itself. It is a reflexive
         property, that can stand for an instance of the class when necessary, e.g. when you explore
         a knowledge graph."""@en ;
    rdfs:domain :AuthorshipRelation ;
    rdfs:isDefinedBy <https://www.ica.org/standards/RiC/ontology> ;
    rdfs:range :AuthorshipRelation ;
    rdfs:subPropertyOf :creationRelation_role ;
    skos:changeNote
        [
            dc:date "2023-11-08" ;
            rdf:value """In order to get a system of rolified Relation classes: created
               the object property, with domain and range the AuthorshipRelation rolified class.
               Declared it as reflexive. Declared it(s) superproperty(ies)."""@en ;
        ] ;
    skos:scopeNote """This property "rolifies" the AuthorshipRelation class. It should
         be used only when you have to manage instances of the AuthorshipRelation class, to connect
         each instance to itself, in order to be able to infer, using OWL-RL and property paths, the
         two shortcuts corresponding to this n-ary class."""@en ;
.

:beginningDate
    a owl:DatatypeProperty ;
    rdfs:label
        "beginning date"@en ,
        "fecha de inicio"@es ,
        "date de début"@fr ;
    rdfs:comment "Date at which something began."@en ;
    rdfs:domain :Thing ;
    rdfs:isDefinedBy <https://www.ica.org/standards/RiC/ontology> ;
    rdfs:range rdfs:Literal ;
    rdfs:subPropertyOf :date ;
    skos:changeNote
        [
            dc:date "2023-08-25" ;
            rdf:value "Added a new rdfs:label in French."@en ;
        ] ,
        [
            dc:date "2023-11-02" ;
            rdf:value "Added a new rdfs:label in Spanish."@en ;
        ] ;
    skos:scopeNote """Provided for usability reasons. May be deprecated and removed
         later on. Use only if you don't use Date classes for handling dates."""@en ;
    :RiCCMCorrespondingComponent """Datatype property specialized implementation of
         RiC-E18 (Date entity)"""@en ;
.

:childRelation_role
    a
        owl:ObjectProperty ,
        owl:ReflexiveProperty ;
    rdfs:label
        "has the role of the Child Relation"@en ,
        "desempeña el papel de la Relación de filiación"@es ,
        "a le rôle de la Relation de filiation"@fr ;
    rdfs:comment """Connects a ChildRelation to itself. It is a reflexive property,
         that can stand for an instance of the class when necessary, e.g. when you explore a
         knowledge graph."""@en ;
    rdfs:domain :ChildRelation ;
    rdfs:isDefinedBy <https://www.ica.org/standards/RiC/ontology> ;
    rdfs:range :ChildRelation ;
    rdfs:subPropertyOf :descendanceRelation_role ;
    skos:changeNote
        [
            dc:date "2023-11-08" ;
            rdf:value """In order to get a system of rolified Relation classes: created
               the object property, with domain and range the ChildRelation rolified class. Declared
               it as reflexive. Declared it(s) superproperty(ies)."""@en ;
        ] ;
    skos:scopeNote """This property "rolifies" the ChildRelation class. It should be
         used only when you have to manage instances of the ChildRelation class, to connect each
         instance to itself, in order to be able to infer, using OWL-RL and property paths, the two
         shortcuts corresponding to this n-ary class."""@en ;
.

:containsOrContained
    a owl:ObjectProperty ;
    rdfs:label
        "contains or contained"@en ,
        "contiene o contenía"@es ,
        "contient ou a contenu"@fr ;
    rdfs:comment """Connects a Place to a region that is or was within
         it."""@en ;
    rdfs:domain :Place ;
    rdfs:isDefinedBy <https://www.ica.org/standards/RiC/ontology> ;
    rdfs:range :Place ;
    rdfs:subPropertyOf
        :hasOrHadPart ,
        :isAssociatedWithPlace ,
        :isPlaceAssociatedWith ;
    owl:inverseOf :isOrWasContainedBy ;
    skos:changeNote
        [
            dc:date "2023-08-28" ;
            rdf:value "Added a new rdfs:label in French."@en ;
        ] ,
        [
            dc:date "2023-11-02" ;
            rdf:value "Added a new rdfs:label in Spanish."@en ;
        ] ,
        [
            dc:date "2021-01-22" ;
            rdf:value """changed the IRI, label, inverse property IRI, text definition,
               corresponding CM component name ; added a scope note (changed made in order to make
               RiC-O compliant with RiC-CM 0.2; the name of this property in RiC-O 0.1 was
               "contains")."""@en ;
        ] ;
    skos:scopeNote """Use for connecting two geographical or administrative
         regions."""@en ;
    :RiCCMCorrespondingComponent """RiC-R007 ('contains or contained'
         relation)"""@en ;
.

:endDate
    a owl:DatatypeProperty ;
    rdfs:label
        "end date"@en ,
        "fecha final"@es ,
        "date de fin"@fr ;
    rdfs:comment "Date at which something ended."@en ;
    rdfs:domain :Thing ;
    rdfs:isDefinedBy <https://www.ica.org/standards/RiC/ontology> ;
    rdfs:range rdfs:Literal ;
    rdfs:subPropertyOf :date ;
    skos:changeNote
        [
            dc:date "2023-08-25" ;
            rdf:value "Added a new rdfs:label in French."@en ;
        ] ,
        [
            dc:date "2023-11-02" ;
            rdf:value "Added a new rdfs:label in Spanish."@en ;
        ] ;
    skos:scopeNote """Provided for usability reasons. May be deprecated and removed
         later on. Use only if you don't use Date classes for handling dates."""@en ;
    :RiCCMCorrespondingComponent """Datatype property specialized implementation of
         RiC-E18 (Date entity)"""@en ;
.

:groupSubdivisionRelation_role
    a
        owl:ObjectProperty ,
        owl:ReflexiveProperty ;
    rdfs:label
        "has the role of the Group Subdivision Relation"@en ,
        """desempeña el papel de la Relación de subdivisión entre grupos de
         agentes"""@es ,
        """a le rôle de la Relation de subdivision entre groupes
         d’agents"""@fr ;
    rdfs:comment """Connects a GroupSubdivisionRelation to itself. It is a reflexive
         property, that can stand for an instance of the class when necessary, e.g. when you explore
         a knowledge graph."""@en ;
    rdfs:domain :GroupSubdivisionRelation ;
    rdfs:isDefinedBy <https://www.ica.org/standards/RiC/ontology> ;
    rdfs:range :GroupSubdivisionRelation ;
    rdfs:subPropertyOf
        :agentHierarchicalRelation_role ,
        :wholePartRelation_role ;
    skos:changeNote
        [
            dc:date "2023-11-08" ;
            rdf:value """In order to get a system of rolified Relation classes: created
               the object property, with domain and range the GroupSubdivisionRelation rolified
               class. Declared it as reflexive. Declared it(s) superproperty(ies)."""@en ;
        ] ;
    skos:scopeNote """This property "rolifies" the GroupSubdivisionRelation class. It
         should be used only when you have to manage instances of the GroupSubdivisionRelation
         class, to connect each instance to itself, in order to be able to infer, using OWL-RL and
         property paths, the two shortcuts corresponding to this n-ary class."""@en ;
.

:hasAccumulator
    a owl:ObjectProperty ;
    rdfs:label
        "has accumulator"@en ,
        "tiene como acumulador a"@es ,
        "est accumulé par"@fr ;
    rdfs:comment """Connects a Record Resource or an Instantiation to the Agent that
         accumulates it, be it intentionally (collecting) or not (receiving in the course of its
         activities)."""@en ;
    rdfs:domain
        [
            a owl:Class ;
            owl:unionOf (
                :Instantiation
                :RecordResource
            ) ;
        ] ;
    rdfs:isDefinedBy <https://www.ica.org/standards/RiC/ontology> ;
    rdfs:range :Agent ;
    rdfs:subPropertyOf :hasOrganicProvenance ;
    owl:inverseOf :isAccumulatorOf ;
    owl:propertyChainAxiom (
        :thingIsSourceOfRelation
        :accumulationRelation_role
        :relationHasTarget
    ) ;
    skos:changeNote
        [
            dc:date "2023-11-08" ;
            rdf:value """In order to get a system of rolified Relation classes: modified
               the property chain axiom so that it now involves the new accumulationRelation_role
               object property."""@en ;
        ] ,
        [
            dc:date "2023-08-28" ;
            rdf:value "Added a new rdfs:label in French."@en ;
        ] ,
        [
            dc:date "2023-11-02" ;
            rdf:value "Added a new rdfs:label in Spanish."@en ;
        ] ,
        [
            dc:date "2021-01-22" ;
            rdf:value """changed the IRI, label, inverse property IRI, text definition
               and corresponding CM component (changed made in order to make RiC-O compliant with
               RiC-CM 0.2; the name of this property in RiC-O 0.1 was "accumulatedBy")."""@en ;
        ] ;
    :RiCCMCorrespondingComponent """RiC-R028 ('has accumulator'
         relation)"""@en ;
.

:hasOrHadAppellation
    a owl:ObjectProperty ;
    rdfs:label
        "has or had appellation"@en ,
        "tiene o tenía como denominación"@es ,
        "a ou a eu pour appellation"@fr ;
    rdfs:comment """Connects a Thing to an Appellation that is or was used for
         designating it."""@en ;
    rdfs:domain :Thing ;
    rdfs:isDefinedBy <https://www.ica.org/standards/RiC/ontology> ;
    rdfs:range :Appellation ;
    rdfs:subPropertyOf :isRelatedTo ;
    owl:inverseOf :isOrWasAppellationOf ;
    owl:propertyChainAxiom (
        :thingIsTargetOfRelation
        :appellationRelation_role
        :relationHasSource
    ) ;
    skos:changeNote
        [
            dc:date "2023-11-08" ;
            rdf:value """In order to get a system of rolified Relation classes: modified
               the property chain axiom so that it now involves the new appellationRelation_role
               object property."""@en ;
        ] ,
        [
            dc:date "2023-08-28" ;
            rdf:value "Added a new rdfs:label in French."@en ;
        ] ,
        [
            dc:date "2021-01-22" ;
            rdf:value """changed the IRI, label, inverse property IRI, textual
               definition (the name of this property in RiC-O 0.1 was "hasAppellation")."""@en ;
        ] ,
        [
            dc:date "2023-11-02" ;
            rdf:value "Added a new rdfs:label in Spanish."@en ;
        ] ;
.

:hasOrHadComponent
    a owl:ObjectProperty ;
    rdfs:label
        "has or had component"@en ,
        "tiene o tenía como componente"@es ,
        "a ou a eu pour composant"@fr ;
    rdfs:comment """Connects an Instantiation to one of its present or past component
         instantiations."""@en ;
    rdfs:domain :Instantiation ;
    rdfs:isDefinedBy <https://www.ica.org/standards/RiC/ontology> ;
    rdfs:range :Instantiation ;
    rdfs:subPropertyOf
        :hasOrHadPart ,
        :isInstantiationAssociatedWithInstantiation ;
    owl:inverseOf :isOrWasComponentOf ;
    skos:changeNote
        [
            dc:date "2023-08-28" ;
            rdf:value "Added a new rdfs:label in French."@en ;
        ] ,
        [
            dc:date "2021-01-22" ;
            rdf:value """changed the IRI, label, inverse property IRI, textual
               definition (changed made in order to make RiC-O compliant with RiC-CM 0.2; the name
               of this property in RiC-O 0.1 was "hasComponent")."""@en ;
        ] ,
        [
            dc:date "2023-11-02" ;
            rdf:value "Added a new rdfs:label in Spanish."@en ;
        ] ;
    :RiCCMCorrespondingComponent """RiC-R004 ('has or had component'
         relation)"""@en ;
.

:hasOrHadConstituent
    a owl:ObjectProperty ;
    rdfs:label
        "has or had constituent"@en ,
        "tiene o tenía como elemento constitutivo"@es ,
        "a ou a eu pour constituant"@fr ;
    rdfs:comment """Connects a Record or Record Part to a Record or Record part that
         is or was a constituent of that Record or Record Part."""@en ;
    rdfs:domain
        [
            a owl:Class ;
            owl:unionOf (
                :Record
                :RecordPart
            ) ;
        ] ;
    rdfs:isDefinedBy <https://www.ica.org/standards/RiC/ontology> ;
    rdfs:range
        [
            a owl:Class ;
            owl:unionOf (
                :Record
                :RecordPart
            ) ;
        ] ;
    rdfs:subPropertyOf
        :hasOrHadPart ,
        :isRecordResourceAssociatedWithRecordResource ;
    owl:inverseOf :isOrWasConstituentOf ;
    skos:changeNote
        [
            dc:date "2021-01-22" ;
            rdf:value """changed the IRI, label, inverse property IRI, textual
               definition (changed made in order to make RiC-O compliant with RiC-CM 0.2; the name
               of this property in RiC-O 0.1 was "hasConstituent")."""@en ;
        ] ,
        [
            dc:date "2023-10-19" ;
            rdf:value "Added Record Part to the domain."@en ;
        ] ,
        [
            dc:date "2023-11-12" ;
            rdf:value """Aligned with RiC-CM 1.0: updated the description
               (rdfs:comment)."""@en ;
        ] ,
        [
            dc:date "2023-11-02" ;
            rdf:value "Added a new rdfs:label in Spanish."@en ;
        ] ,
        [
            dc:date "2023-08-28" ;
            rdf:value "Added a new rdfs:label in French."@en ;
        ] ;
    :RiCCMCorrespondingComponent """RiC-R003 ('has or had constituent'
         relation)"""@en ;
.

:hasOrHadController
    a owl:ObjectProperty ;
    rdfs:label
        "has or had controller"@en ,
        "tiene o tenía como controlador"@es ,
        "a ou a été contrôlé par"@fr ;
    rdfs:comment """Inverse of 'is or was controller of' object
         property."""@en ;
    rdfs:domain :Agent ;
    rdfs:isDefinedBy <https://www.ica.org/standards/RiC/ontology> ;
    rdfs:range :Agent ;
    rdfs:subPropertyOf
        :isOrWasSubordinateTo ,
        :isOrWasUnderAuthorityOf ;
    owl:inverseOf :isOrWasControllerOf ;
    owl:propertyChainAxiom (
        :thingIsTargetOfRelation
        :agentControlRelation_role
        :relationHasSource
    ) ;
    skos:changeNote
        [
            dc:date "2023-11-02" ;
            rdf:value "Added a new rdfs:label in Spanish."@en ;
        ] ,
        [
            dc:date "2023-08-28" ;
            rdf:value "Added a new rdfs:label in French."@en ;
        ] ,
        [
            dc:date "2021-01-22" ;
            rdf:value """changed the IRI, label, inverse property IRI, text definition,
               corresponding CM component name (changed made in order to make RiC-O compliant with
               RiC-CM 0.2; the name of this property in RiC-O 0.1 was "controlledBy")."""@en ;
        ] ,
        [
            dc:date "2023-11-08" ;
            rdf:value """In order to get a system of rolified Relation classes: modified
               the property chain axiom so that it now involves the new agentControlRelation_role
               object property."""@en ;
        ] ;
    :RiCCMCorrespondingComponent """RiC-R041i ('has or had controller'
         relation)"""@en ;
.

:hasOrHadInstantiation
    a owl:ObjectProperty ;
    rdfs:label
        "has or had instantiation"@en ,
        "tiene o tenía como instanciación"@es ,
        "a ou a eu pour instanciation"@fr ;
    rdfs:comment """Connects a Record Resource to an Instantiation, which either may
         exist or may have been lost or destroyed."""@en ;
    rdfs:domain :RecordResource ;
    rdfs:isDefinedBy <https://www.ica.org/standards/RiC/ontology> ;
    rdfs:range :Instantiation ;
    rdfs:subPropertyOf :isRelatedTo ;
    owl:inverseOf :isOrWasInstantiationOf ;
    owl:propertyChainAxiom (
        :thingIsSourceOfRelation
        :recordResourceToInstantiationRelation_role
        :relationHasTarget
    ) ;
    skos:changeNote
        [
            dc:date "2023-11-08" ;
            rdf:value """In order to get a system of rolified Relation classes: modified
               the property chain axiom so that it now involves the new
               recordResourceToInstantiationRelation_role object property."""@en ;
        ] ,
        [
            dc:date "2023-11-27" ;
            rdf:value "Added a new rdfs:label in Spanish."@en ;
        ] ,
        [
            dc:date "2023-11-12" ;
            rdf:value """Aligned with RiC-CM 1.0: updated the description
               (rdfs:comment)."""@en ;
        ] ,
        [
            dc:date "2023-08-28" ;
            rdf:value "Added a new rdfs:label in French."@en ;
        ] ,
        [
            dc:date "2023-08-29" ;
            rdf:value """Updated the IRI, inverse property, definition, labels and
               RiCMCorrespondingComponent, and added a skos:scopeNote; this in order to make the
               specification compliant with RiC-CM 1.0. The name of the property in RiC-O 0.2 was
               'has instantiation'."""@en ;
        ] ,
        [
            dc:date "2021-01-22" ;
            rdf:value "changed the inverse property IRI."@en ;
        ] ;
    skos:scopeNote """In some situations, it may be useful or necessary to connect a
         record resource to an instantiation that no longer exists or or has been lost, when some of
         its characteristics are known from some source, like an old finding aid."""@en ;
    :RiCCMCorrespondingComponent """RiC-R025 ('has or had instantiation'
         relation)"""@en ;
.

:hasOrHadParticipant
    a owl:ObjectProperty ;
    rdfs:label
        "has or had participant"@en ,
        "tiene o tenía como participante"@es ,
        "a ou a eu pour participant"@fr ;
    rdfs:comment """Connects an Event to a Thing that is or was actively or passively
         involved in it."""@en ;
    rdfs:domain :Event ;
    rdfs:isDefinedBy <https://www.ica.org/standards/RiC/ontology> ;
    rdfs:range :Thing ;
    rdfs:subPropertyOf :isEventAssociatedWith ;
    owl:inverseOf :isOrWasParticipantIn ;
    skos:changeNote
        [
            dc:date "2023-08-28" ;
            rdf:value "Added a new rdfs:label in French."@en ;
        ] ,
        [
            dc:date "2023-11-02" ;
            rdf:value "Added a new rdfs:label in Spanish."@en ;
        ] ,
        [
            dc:date "2021-01-22" ;
            rdf:value """changed the IRI, label, inverse property IRI, textual
               definition (changed made in order to make RiC-O compliant with RiC-CM 0.2; the name
               of this property in RiC-O 0.1 was "involves")."""@en ;
        ] ;
    :RiCCMCorrespondingComponent """RiC-R058 ('has or had participant'
         relation)"""@en ;
.

:hasOrHadSubdivision
    a owl:ObjectProperty ;
    rdfs:label
        "has or had subdivision"@en ,
        "tiene o tenía como subdivisión"@es ,
        "a ou a eu pour subdivision"@fr ;
    rdfs:comment """Connects a Group to one of its present or past
         subdivisions."""@en ;
    rdfs:domain :Group ;
    rdfs:isDefinedBy <https://www.ica.org/standards/RiC/ontology> ;
    rdfs:range :Group ;
    rdfs:subPropertyOf
        :hasOrHadPart ,
        :hasOrHadSubordinate ;
    owl:inverseOf :isOrWasSubdivisionOf ;
    owl:propertyChainAxiom (
        :thingIsSourceOfRelation
        :groupSubdivisionRelation_role
        :relationHasTarget
    ) ;
    skos:changeNote
        [
            dc:date "2021-01-22" ;
            rdf:value """changed the IRI, label, inverse property IRI, text definition,
               super property IRIs (changed made in order to make RiC-O compliant with RiC-CM 0.2;
               the name of this property in RiC-O 0.1 was "hasSubdivision")."""@en ;
        ] ,
        [
            dc:date "2023-11-02" ;
            rdf:value "Added a new rdfs:label in Spanish."@en ;
        ] ,
        [
            dc:date "2023-08-28" ;
            rdf:value "Added a new rdfs:label in French."@en ;
        ] ,
        [
            dc:date "2023-11-08" ;
            rdf:value """In order to get a system of rolified Relation classes: modified
               the property chain axiom so that it now involves the new
               groupSubdivisionRelation_role object property."""@en ;
        ] ;
    :RiCCMCorrespondingComponent """RiC-R005 ('has or had subdivision'
         relation)"""@en ;
.

:hasOrHadSubevent
    a owl:ObjectProperty ;
    rdfs:label
        "has or had subevent"@en ,
        "tiene o tenía como parte de evento"@es ,
        "est ou a été constitué de l’événement"@fr ;
    rdfs:comment """Connects an Event to one of a series of Events that constitute the
         original, broader, past or ongoing Event."""@en ;
    rdfs:domain :Event ;
    rdfs:isDefinedBy <https://www.ica.org/standards/RiC/ontology> ;
    rdfs:range :Event ;
    rdfs:subPropertyOf
        :hasOrHadPart ,
        :isAssociatedWithEvent ,
        :isEventAssociatedWith ;
    owl:inverseOf :isOrWasSubeventOf ;
    skos:changeNote
        [
            dc:date "2021-01-22" ;
            rdf:value """changed the IRI, label, inverse property IRI, text definition,
               super property IRI (changed made in order to make RiC-O compliant with RiC-CM 0.2;
               the name of this property in RiC-O 0.1 was "hasSubEvent")."""@en ;
        ] ,
        [
            dc:date "2023-11-02" ;
            rdf:value "Added a new rdfs:label in Spanish."@en ;
        ] ,
        [
            dc:date "2023-08-28" ;
            rdf:value "Added a new rdfs:label in French."@en ;
        ] ;
    skos:scopeNote """Since an Activity is a kind of Event, this Relation can also be
         used for Activity."""@en ;
    :RiCCMCorrespondingComponent """RiC-R006 ('has or had subevent'
         relation)"""@en ;
.

:hasOrHadSubject
    a owl:ObjectProperty ;
    rdfs:label
        "has or had subject"@en ,
        "tiene o tenía como materia"@es ,
        "a ou a eu pour sujet"@fr ;
    rdfs:comment """Connects a Record Resource to a Thing that is or was its
         subject."""@en ;
    rdfs:domain :RecordResource ;
    rdfs:isDefinedBy <https://www.ica.org/standards/RiC/ontology> ;
    rdfs:range :Thing ;
    rdfs:subPropertyOf :isRelatedTo ;
    owl:inverseOf :isOrWasSubjectOf ;
    skos:changeNote
        [
            dc:date "2021-01-22" ;
            rdf:value """changed the IRI, label, inverse property IRI, text definition
               (changed made in order to make RiC-O compliant with RiC-CM 0.2; the name of this
               property in RiC-O 0.1 was "hasSubject")."""@en ;
        ] ,
        [
            dc:date "2023-11-12" ;
            rdf:value """Aligned with RiC-CM 1.0: updated the
               skos:scopeNote."""@en ;
        ] ,
        [
            dc:date "2023-08-28" ;
            rdf:value "Added a new rdfs:label in French."@en ;
        ] ,
        [
            dc:date "2023-11-02" ;
            rdf:value "Added a new rdfs:label in Spanish."@en ;
        ] ;
    skos:scopeNote """The subject of a Record Set may be affected if the Record Set
         loses some of the Records."""@en ;
    :RiCCMCorrespondingComponent """RiC-R019 ('has or had subject'
         relation)"""@en ;
.

:hasOrganicOrFunctionalProvenance
    a owl:ObjectProperty ;
    rdfs:label
        "has organic or functional provenance"@en ,
        "tiene como procedencia orgánica o funcional"@es ,
        "a pour provenance organique ou fonctionnelle"@fr ;
    rdfs:comment """Connects a Record Resource or an Instantiation to an Agent that
         creates or accumulates it, receives it, or sends it, or to an Activity that generates
         it."""@en ;
    rdfs:domain
        [
            a owl:Class ;
            owl:unionOf (
                :Instantiation
                :RecordResource
            ) ;
        ] ;
    rdfs:isDefinedBy <https://www.ica.org/standards/RiC/ontology> ;
    rdfs:range
        [
            a owl:Class ;
            owl:unionOf (
                :Activity
                :Agent
            ) ;
        ] ;
    rdfs:subPropertyOf :isRelatedTo ;
    owl:inverseOf :isOrganicOrFunctionalProvenanceOf ;
    owl:propertyChainAxiom (
        :thingIsSourceOfRelation
        :organicOrFunctionalProvenanceRelation_role
        :relationHasTarget
    ) ;
    skos:changeNote
        [
            dc:date "2023-11-07" ;
            rdf:value """Property added as a superproperty of hasProvenance and
               documents, along with its inverse property. Shortcut also added."""@en ;
        ] ,
        [
            dc:date "2023-11-08" ;
            rdf:value """In order to get a system of rolified Relation classes: modified
               the property chain axiom so that it now involves the new
               organicOrFunctionalProvenanceRelation_role object property."""@en ;
        ] ;
.

:hasSubordinateTransitive
    a
        owl:ObjectProperty ,
        owl:TransitiveProperty ;
    rdfs:label
        "has subordinate transitive"@en ,
        "tiene como subordinado o subordinada a transitivo"@es ,
        "a pour subalterne transitif"@fr ;
    rdfs:comment """Connects an Agent to an Agent that is directly or indirectly
         hierarchically inferior. This is a transitive relation."""@en ;
    rdfs:domain :Agent ;
    rdfs:isDefinedBy <https://www.ica.org/standards/RiC/ontology> ;
    rdfs:range :Agent ;
    rdfs:subPropertyOf :hasOrHadSubordinate ;
    owl:inverseOf :isSubordinateToTransitive ;
    skos:changeNote
        [
            dc:date "2023-11-12" ;
            rdf:value "Updated the labels."@en ;
        ] ,
        [
            dc:date "2023-09-08" ;
            rdf:value """Object property added, along with its inverse property, in
               order to enable to express current subordination relations between agents (the past
               subordination relation also being added)."""@en ;
        ] ,
        [
            dc:date "2023-11-27" ;
            rdf:value "Added a new rdfs:label in Spanish."@en ;
        ] ;
.

:includesOrIncluded
    a owl:ObjectProperty ;
    rdfs:label
        "includes or included"@en ,
        "incluye o incluía"@es ,
        "inclut ou a inclus"@fr ;
    rdfs:comment """Connects a Record Set to a Record or Record Set it aggregates, or
         aggregated in the past."""@en ;
    rdfs:domain :RecordSet ;
    rdfs:isDefinedBy <https://www.ica.org/standards/RiC/ontology> ;
    rdfs:range
        [
            a owl:Class ;
            owl:unionOf (
                :Record
                :RecordSet
            ) ;
        ] ;
    rdfs:subPropertyOf
        :hasOrHadPart ,
        :isRecordResourceAssociatedWithRecordResource ;
    owl:inverseOf :isOrWasIncludedIn ;
    skos:changeNote
        [
            dc:date "2023-06-05" ;
            rdf:value """Made this object property a subproperty of
               hasOrHadPart."""@en ;
        ] ,
        [
            dc:date "2023-08-28" ;
            rdf:value "Added a new rdfs:label in French."@en ;
        ] ,
        [
            dc:date "2021-01-22" ;
            rdf:value """changed the IRI, label, inverse property IRI, text definition
               (changed made in order to make RiC-O compliant with RiC-CM 0.2; the name of this
               property in RiC-O 0.1 was "includes")."""@en ;
        ] ,
        [
            dc:date "2023-11-02" ;
            rdf:value "Added a new rdfs:label in Spanish."@en ;
        ] ;
    skos:scopeNote """A Record or Record Set can be aggregated in one or many Record
         Sets simultaneously or through time."""@en ;
    :RiCCMCorrespondingComponent """RiC-R024 ('includes or included'
         relation)"""@en ;
.

:intellectualPropertyRightsRelation_role
    a
        owl:ObjectProperty ,
        owl:ReflexiveProperty ;
    rdfs:label
        """has the role of the Intellectual Property Rights
         Relation"""@en ,
        """desempeña el papel de la Relación de propiedad
         intelectual"""@es ,
        "a le rôle de la Relation de propriété intellectuelle"@fr ;
    rdfs:comment """Connects a IntellectualPropertyRightsRelation to itself. It is a
         reflexive property, that can stand for an instance of the class when necessary, e.g. when
         you explore a knowledge graph."""@en ;
    rdfs:domain :IntellectualPropertyRightsRelation ;
    rdfs:isDefinedBy <https://www.ica.org/standards/RiC/ontology> ;
    rdfs:range :IntellectualPropertyRightsRelation ;
    rdfs:subPropertyOf :authorityRelation_role ;
    skos:changeNote
        [
            dc:date "2023-11-08" ;
            rdf:value """In order to get a system of rolified Relation classes: created
               the object property, with domain and range the IntellectualPropertyRightsRelation
               rolified class. Declared it as reflexive. Declared it(s)
               superproperty(ies)."""@en ;
        ] ;
    skos:scopeNote """This property "rolifies" the IntellectualPropertyRightsRelation
         class. It should be used only when you have to manage instances of the
         IntellectualPropertyRightsRelation class, to connect each instance to itself, in order to
         be able to infer, using OWL-RL and property paths, the two shortcuts corresponding to this
         n-ary class."""@en ;
.

:isAccumulatorOf
    a owl:ObjectProperty ;
    rdfs:label
        "is accumulator of"@en ,
        "es acumulador(a) de"@es ,
        "accumule"@fr ;
    rdfs:comment "Inverse of 'has accumulator' object property."@en ;
    rdfs:domain :Agent ;
    rdfs:isDefinedBy <https://www.ica.org/standards/RiC/ontology> ;
    rdfs:range
        [
            a owl:Class ;
            owl:unionOf (
                :Instantiation
                :RecordResource
            ) ;
        ] ;
    rdfs:subPropertyOf :isOrganicProvenanceOf ;
    owl:inverseOf :hasAccumulator ;
    owl:propertyChainAxiom (
        :thingIsTargetOfRelation
        :accumulationRelation_role
        :relationHasSource
    ) ;
    skos:changeNote
        [
            dc:date "2021-01-22" ;
            rdf:value """changed the IRI, label, inverse property IRI, text definition
               and corresponding CM component (changed made in order to make RiC-O compliant with
               RiC-CM 0.2; the name of this property in RiC-O 0.1 was "accumulates")."""@en ;
        ] ,
        [
            dc:date "2023-11-08" ;
            rdf:value """In order to get a system of rolified Relation classes: modified
               the property chain axiom so that it now involves the new accumulationRelation_role
               object property."""@en ;
        ] ,
        [
            dc:date "2023-11-02" ;
            rdf:value "Added a new rdfs:label in Spanish."@en ;
        ] ,
        [
            dc:date "2023-08-28" ;
            rdf:value "Added a new rdfs:label in French."@en ;
        ] ;
    :RiCCMCorrespondingComponent """RiC-R028i ('is accumulator of'
         relation)"""@en ;
.

:isOrWasAppellationOf
    a owl:ObjectProperty ;
    rdfs:label
        "is or was appellation of"@en ,
        "es o era la denominación de"@es ,
        "est ou a été l’appellation de"@fr ;
    rdfs:comment """Connects an Appellation to a Thing that it designates or
         designated."""@en ;
    rdfs:domain :Appellation ;
    rdfs:isDefinedBy <https://www.ica.org/standards/RiC/ontology> ;
    rdfs:range :Thing ;
    rdfs:subPropertyOf :isRelatedTo ;
    owl:inverseOf :hasOrHadAppellation ;
    owl:propertyChainAxiom (
        :thingIsSourceOfRelation
        :appellationRelation_role
        :relationHasTarget
    ) ;
    skos:changeNote
        [
            dc:date "2023-11-08" ;
            rdf:value """In order to get a system of rolified Relation classes: modified
               the property chain axiom so that it now involves the new appellationRelation_role
               object property."""@en ;
        ] ,
        [
            dc:date "2023-08-28" ;
            rdf:value "Added a new rdfs:label in French."@en ;
        ] ,
        [
            dc:date "2021-01-22" ;
            rdf:value """changed the IRI, label, inverse property IRI, text definition
               (the name of this property in RiC-O 0.1 was "isAppellationOf")."""@en ;
        ] ,
        [
            dc:date "2023-11-07" ;
            rdf:value """Added the property chain axiom so that this property is
               formally defined as a shortcut (the inverse property already was)."""@en ;
        ] ,
        [
            dc:date "2023-11-02" ;
            rdf:value "Added a new rdfs:label in Spanish."@en ;
        ] ;
.

:isOrWasComponentOf
    a owl:ObjectProperty ;
    rdfs:label
        "is or was component of"@en ,
        "es o era componente de"@es ,
        "est ou a été un composant de"@fr ;
    rdfs:comment "Inverse of 'has or had component' object property."@en ;
    rdfs:domain :Instantiation ;
    rdfs:isDefinedBy <https://www.ica.org/standards/RiC/ontology> ;
    rdfs:range :Instantiation ;
    rdfs:subPropertyOf
        :isInstantiationAssociatedWithInstantiation ,
        :isOrWasPartOf ;
    owl:inverseOf :hasOrHadComponent ;
    skos:changeNote
        [
            dc:date "2023-11-02" ;
            rdf:value "Added a new rdfs:label in Spanish."@en ;
        ] ,
        [
            dc:date "2023-08-28" ;
            rdf:value "Added a new rdfs:label in French."@en ;
        ] ,
        [
            dc:date "2021-01-22" ;
            rdf:value """changed the IRI, label, inverse property IRI, text definition
               (changed made in order to make RiC-O compliant with RiC-CM 0.2; the name of this
               property in RiC-O 0.1 was "isComponentOf")."""@en ;
        ] ;
    :RiCCMCorrespondingComponent """RiC-R004i ('is or was component of'
         relation)"""@en ;
.

:isOrWasConstituentOf
    a owl:ObjectProperty ;
    rdfs:label
        "is or was constituent of"@en ,
        "es o era elemento constitutivo de"@es ,
        "est ou a été un constituant de"@fr ;
    rdfs:comment """Inverse of 'has or had constituent' object
         property."""@en ;
    rdfs:domain
        [
            a owl:Class ;
            owl:unionOf (
                :Record
                :RecordPart
            ) ;
        ] ;
    rdfs:isDefinedBy <https://www.ica.org/standards/RiC/ontology> ;
    rdfs:range
        [
            a owl:Class ;
            owl:unionOf (
                :Record
                :RecordPart
            ) ;
        ] ;
    rdfs:subPropertyOf
        :isOrWasPartOf ,
        :isRecordResourceAssociatedWithRecordResource ;
    owl:inverseOf :hasOrHadConstituent ;
    skos:changeNote
        [
            dc:date "2023-10-26" ;
            rdf:value "Added RecordPart to the range."@en ;
        ] ,
        [
            dc:date "2023-11-02" ;
            rdf:value "Added a new rdfs:label in Spanish."@en ;
        ] ,
        [
            dc:date "2023-08-28" ;
            rdf:value "Added a new rdfs:label in French."@en ;
        ] ,
        [
            dc:date "2021-01-22" ;
            rdf:value """changed the IRI, label, inverse property IRI, text definition
               (changed made in order to make RiC-O compliant with RiC-CM 0.2; the name of this
               property in RiC-O 0.1 was "isConstituentOf")."""@en ;
        ] ;
    :RiCCMCorrespondingComponent """RiC-R003i ('is or was constituent of'
         relation)"""@en ;
.

:isOrWasContainedBy
    a owl:ObjectProperty ;
    rdfs:label
        "is or was contained by"@en ,
        "está o estaba contenido en"@es ,
        "est ou a été contenu par"@fr ;
    rdfs:comment "Inverse of 'contains or contained' object property."@en ;
    rdfs:domain :Place ;
    rdfs:isDefinedBy <https://www.ica.org/standards/RiC/ontology> ;
    rdfs:range :Place ;
    rdfs:subPropertyOf
        :isAssociatedWithPlace ,
        :isOrWasPartOf ,
        :isPlaceAssociatedWith ;
    owl:inverseOf :containsOrContained ;
    skos:changeNote
        [
            dc:date "2023-11-02" ;
            rdf:value "Added a new rdfs:label in Spanish."@en ;
        ] ,
        [
            dc:date "2021-01-22" ;
            rdf:value """changed the IRI, label, inverse property IRI, text definition,
               corresponding CM component name (changed made in order to make RiC-O compliant with
               RiC-CM 0.2; the name of this property in RiC-O 0.1 was "containedBy")."""@en ;
        ] ,
        [
            dc:date "2023-08-28" ;
            rdf:value "Added a new rdfs:label in French."@en ;
        ] ;
    :RiCCMCorrespondingComponent """RiC-R007i ('is or was contained by'
         relation)"""@en ;
.

:isOrWasControllerOf
    a owl:ObjectProperty ;
    rdfs:label
        "is or was controller of"@en ,
        "es o era controlador de"@es ,
        "a contrôlé ou contrôle"@fr ;
    rdfs:comment """Connects an Agent to another Agent it controls or
         controlled."""@en ;
    rdfs:domain :Agent ;
    rdfs:isDefinedBy <https://www.ica.org/standards/RiC/ontology> ;
    rdfs:range :Agent ;
    rdfs:subPropertyOf
        :hasOrHadAuthorityOver ,
        :hasOrHadSubordinate ;
    owl:inverseOf :hasOrHadController ;
    owl:propertyChainAxiom (
        :thingIsSourceOfRelation
        :agentControlRelation_role
        :relationHasTarget
    ) ;
    skos:changeNote
        [
            dc:date "2021-01-22" ;
            rdf:value """changed the IRI, label, inverse property IRI, text definition,
               corresponding CM component name (changed made in order to make RiC-O compliant with
               RiC-CM 0.2; the name of this property in RiC-O 0.1 was "controls")."""@en ;
        ] ,
        [
            dc:date "2023-08-28" ;
            rdf:value "Added a new rdfs:label in French."@en ;
        ] ,
        [
            dc:date "2023-11-12" ;
            rdf:value """Aligned with RiC-CM 1.0: updated the description
               (rdfs:comment)."""@en ;
        ] ,
        [
            dc:date "2023-11-08" ;
            rdf:value """In order to get a system of rolified Relation classes: modified
               the property chain axiom so that it now involves the new agentControlRelation_role
               object property."""@en ;
        ] ,
        [
            dc:date "2023-11-02" ;
            rdf:value "Added a new rdfs:label in Spanish."@en ;
        ] ;
    :RiCCMCorrespondingComponent """RiC-R041 ('is or was controller of'
         relation)"""@en ;
.

:isOrWasIncludedIn
    a owl:ObjectProperty ;
    rdfs:label
        "is or was included in"@en ,
        "está o estaba incluido en"@es ,
        "est ou a été inclus dans"@fr ;
    rdfs:comment "Inverse of 'includes or included' object property."@en ;
    rdfs:domain
        [
            a owl:Class ;
            owl:unionOf (
                :Record
                :RecordSet
            ) ;
        ] ;
    rdfs:isDefinedBy <https://www.ica.org/standards/RiC/ontology> ;
    rdfs:range :RecordSet ;
    rdfs:subPropertyOf
        :isOrWasPartOf ,
        :isRecordResourceAssociatedWithRecordResource ;
    owl:inverseOf :includesOrIncluded ;
    skos:changeNote
        [
            dc:date "2021-01-22" ;
            rdf:value """changed the IRI, label, inverse property IRI, text definition
               (changed made in order to make RiC-O compliant with RiC-CM 0.2; the name of this
               property in RiC-O 0.1 was "includedIn")."""@en ;
        ] ,
        [
            dc:date "2023-08-28" ;
            rdf:value "Added a new rdfs:label in French."@en ;
        ] ,
        [
            dc:date "2023-06-05" ;
            rdf:value """Made this object property a subproperty of
               isOrWasPartOf."""@en ;
        ] ,
        [
            dc:date "2023-11-02" ;
            rdf:value "Added a new rdfs:label in Spanish."@en ;
        ] ;
    :RiCCMCorrespondingComponent """RiC-R024i ('is or was included in'
         relation)"""@en ;
.

:isOrWasInstantiationOf
    a owl:ObjectProperty ;
    rdfs:label
        "is or was instantiation of"@en ,
        "es o era instanciación de"@es ,
        "est ou a été une instanciation de"@fr ;
    rdfs:comment """Inverse of 'has or had instantiation' object
         property."""@en ;
    rdfs:domain :Instantiation ;
    rdfs:isDefinedBy <https://www.ica.org/standards/RiC/ontology> ;
    rdfs:range :RecordResource ;
    rdfs:subPropertyOf :isRelatedTo ;
    owl:inverseOf :hasOrHadInstantiation ;
    owl:propertyChainAxiom (
        :thingIsTargetOfRelation
        :recordResourceToInstantiationRelation_role
        :relationHasSource
    ) ;
    skos:changeNote
        [
            dc:date "2023-11-27" ;
            rdf:value "Added a new rdfs:label in Spanish."@en ;
        ] ,
        [
            dc:date "2023-11-08" ;
            rdf:value """In order to get a system of rolified Relation classes: modified
               the property chain axiom so that it now involves the new
               recordResourceToInstantiationRelation_role object property."""@en ;
        ] ,
        [
            dc:date "2023-08-29" ;
            rdf:value """Updated the IRI, inverse property, definition, labels and
               RiCMCorrespondingComponent; this in order to make the specification compliant with
               RiC-CM 1.0. The name of the property in RiC-O 0.2 was 'is instantiation
               of'."""@en ;
        ] ,
        [
            dc:date "2023-08-28" ;
            rdf:value "Added a new rdfs:label in French."@en ;
        ] ,
        [
            dc:date "2021-01-22" ;
            rdf:value """changed the IRI and label (changed made in order to make RiC-O
               compliant with RiC-CM 0.2; the name of this property in RiC-O 0.1 was
               "instantiates")."""@en ;
        ] ;
    :RiCCMCorrespondingComponent """RiC-R025i ('is or was instantiation of'
         relation)"""@en ;
.

:isOrWasParticipantIn
    a owl:ObjectProperty ;
    rdfs:label
        "is or was participant in"@en ,
        "es o era participante de"@es ,
        "participe ou a participé à"@fr ;
    rdfs:comment """Inverse of 'has or had participant' object
         property."""@en ;
    rdfs:domain :Thing ;
    rdfs:isDefinedBy <https://www.ica.org/standards/RiC/ontology> ;
    rdfs:range :Event ;
    rdfs:subPropertyOf :isAssociatedWithEvent ;
    owl:inverseOf :hasOrHadParticipant ;
    skos:changeNote
        [
            dc:date "2023-11-02" ;
            rdf:value "Added a new rdfs:label in Spanish."@en ;
        ] ,
        [
            dc:date "2023-08-28" ;
            rdf:value "Added a new rdfs:label in French."@en ;
        ] ,
        [
            dc:date "2021-01-22" ;
            rdf:value """changed the IRI, label, inverse property IRI, textual
               definition (changed made in order to make RiC-O compliant with RiC-CM 0.2; the name
               of this property in RiC-O 0.1 was "involvedIn")."""@en ;
        ] ;
    :RiCCMCorrespondingComponent """RiC-R058i ('is or was participant in'
         relation)"""@en ;
.

:isOrWasSubdivisionOf
    a owl:ObjectProperty ;
    rdfs:label
        "is or was subdivision of"@en ,
        "es o era subdivisión de"@es ,
        "est ou a été une subdivision de"@fr ;
    rdfs:comment """Inverse of 'has or had subdivision' object
         property."""@en ;
    rdfs:domain :Group ;
    rdfs:isDefinedBy <https://www.ica.org/standards/RiC/ontology> ;
    rdfs:range :Group ;
    rdfs:subPropertyOf
        :isOrWasPartOf ,
        :isOrWasSubordinateTo ;
    owl:inverseOf :hasOrHadSubdivision ;
    owl:propertyChainAxiom (
        :thingIsTargetOfRelation
        :groupSubdivisionRelation_role
        :relationHasSource
    ) ;
    skos:changeNote
        [
            dc:date "2023-11-08" ;
            rdf:value """In order to get a system of rolified Relation classes: modified
               the property chain axiom so that it now involves the new
               groupSubdivisionRelation_role object property."""@en ;
        ] ,
        [
            dc:date "2023-11-02" ;
            rdf:value "Added a new rdfs:label in Spanish."@en ;
        ] ,
        [
            dc:date "2021-01-22" ;
            rdf:value """changed the IRI, label, inverse property IRI, text definition,
               super property IRIs (changed made in order to make RiC-O compliant with RiC-CM 0.2;
               the name of this property in RiC-O 0.1 was "isSubdivisionOf")."""@en ;
        ] ,
        [
            dc:date "2023-08-28" ;
            rdf:value "Added a new rdfs:label in French."@en ;
        ] ;
    :RiCCMCorrespondingComponent """RiC-R005i ('is or was subdivision'
         relation)"""@en ;
.

:isOrWasSubeventOf
    a owl:ObjectProperty ;
    rdfs:label
        "is or was subevent of"@en ,
        "es o era parte de evento de"@es ,
        "est ou a été un événement constituant de"@fr ;
    rdfs:comment "Inverse of 'has or had subevent' object property."@en ;
    rdfs:domain :Event ;
    rdfs:isDefinedBy <https://www.ica.org/standards/RiC/ontology> ;
    rdfs:range :Event ;
    rdfs:subPropertyOf
        :isAssociatedWithEvent ,
        :isEventAssociatedWith ,
        :isOrWasPartOf ;
    owl:inverseOf :hasOrHadSubevent ;
    skos:changeNote
        [
            dc:date "2021-01-22" ;
            rdf:value """changed the IRI, label, inverse property IRI, text definition,
               super property URI (changed made in order to make RiC-O compliant with RiC-CM 0.2;
               the name of this property in RiC-O 0.1 was "isSubEventOf")."""@en ;
        ] ,
        [
            dc:date "2023-08-28" ;
            rdf:value "Added a new rdfs:label in French."@en ;
        ] ,
        [
            dc:date "2023-11-02" ;
            rdf:value "Added a new rdfs:label in Spanish."@en ;
        ] ;
    :RiCCMCorrespondingComponent """RiC-R006i ('is or was subevent of'
         relation)"""@en ;
.

:isOrWasSubjectOf
    a owl:ObjectProperty ;
    rdfs:label
        "is or was subject of"@en ,
        "es o era materia de"@es ,
        "est ou a été le sujet de"@fr ;
    rdfs:comment "Inverse of 'has or had subject' object property."@en ;
    rdfs:domain :Thing ;
    rdfs:isDefinedBy <https://www.ica.org/standards/RiC/ontology> ;
    rdfs:range :RecordResource ;
    rdfs:subPropertyOf :isRelatedTo ;
    owl:inverseOf :hasOrHadSubject ;
    skos:changeNote
        [
            dc:date "2023-11-02" ;
            rdf:value "Added a new rdfs:label in Spanish."@en ;
        ] ,
        [
            dc:date "2021-01-22" ;
            rdf:value """changed the IRI, label, inverse property IRI, text definition
               (changed made in order to make RiC-O compliant with RiC-CM 0.2; the name of this
               property in RiC-O 0.1 was "isSubjectOf")."""@en ;
        ] ,
        [
            dc:date "2023-08-28" ;
            rdf:value "Added a new rdfs:label in French."@en ;
        ] ;
    :RiCCMCorrespondingComponent """RIc-R019i ('is or was subject of'
         relation)"""@en ;
.

:isOrganicOrFunctionalProvenanceOf
    a owl:ObjectProperty ;
    rdfs:label
        "is organic or functional provenance of"@en ,
        "es procedencia orgánica o funcional de"@es ,
        "est la provenance organique ou fonctionnelle de"@fr ;
    rdfs:comment """Inverse of 'has organic or functional provenance' object
         property."""@en ;
    rdfs:domain
        [
            a owl:Class ;
            owl:unionOf (
                :Activity
                :Agent
            ) ;
        ] ;
    rdfs:isDefinedBy <https://www.ica.org/standards/RiC/ontology> ;
    rdfs:range
        [
            a owl:Class ;
            owl:unionOf (
                :Instantiation
                :RecordResource
            ) ;
        ] ;
    rdfs:subPropertyOf :isRelatedTo ;
    owl:inverseOf :hasOrganicOrFunctionalProvenance ;
    owl:propertyChainAxiom (
        :thingIsTargetOfRelation
        :organicOrFunctionalProvenanceRelation_role
        :relationHasSource
    ) ;
    skos:changeNote
        [
            dc:date "2023-11-08" ;
            rdf:value """In order to get a system of rolified Relation classes: modified
               the property chain axiom so that it now involves the new
               organicOrFunctionalProvenanceRelation_role object property."""@en ;
        ] ,
        [
            dc:date "2023-11-07" ;
            rdf:value """Property added as a superproperty of isProvenance and
               documentedBy, along with its inverse property. Shortcut also added."""@en ;
        ] ;
.

:isSubordinateToTransitive
    a
        owl:ObjectProperty ,
        owl:TransitiveProperty ;
    rdfs:label
        "is subordinate to transitive"@en ,
        "está subordinado(a) a transitivo"@es ,
        "est subalterne de transitif"@fr ;
    rdfs:comment """Connects an Agent to an Agent that is directly or indirectly
         hierarchically superior. This is a transitive relation."""@en ;
    rdfs:domain :Agent ;
    rdfs:isDefinedBy <https://www.ica.org/standards/RiC/ontology> ;
    rdfs:range :Agent ;
    rdfs:subPropertyOf :isOrWasSubordinateTo ;
    owl:inverseOf :hasSubordinateTransitive ;
    skos:changeNote
        [
            dc:date "2023-11-27" ;
            rdf:value "Added a new rdfs:label in Spanish."@en ;
        ] ,
        [
            dc:date "2023-11-12" ;
            rdf:value "Updated the labels."@en ;
        ] ,
        [
            dc:date "2023-09-08" ;
            rdf:value """Object property added, along with its inverse property, in
               order to enable to express current subordination relations between agents (the past
               subordination relation also being added)."""@en ;
        ] ;
.

:knowingOfRelation_role
    a
        owl:ObjectProperty ,
        owl:ReflexiveProperty ;
    rdfs:label
        "has the role of the Knowing Of Relation"@en ,
        """desempeña el papel de la Relación de conocimieto indirecto entre
         personas"""@es ,
        """a le rôle de la Relation de connaissance à propos d’une
         personne"""@fr ;
    rdfs:comment """Connects a KnowingOfRelation to itself. It is a reflexive
         property, that can stand for an instance of the class when necessary, e.g. when you explore
         a knowledge graph."""@en ;
    rdfs:domain :KnowingOfRelation ;
    rdfs:isDefinedBy <https://www.ica.org/standards/RiC/ontology> ;
    rdfs:range :KnowingOfRelation ;
    rdfs:subPropertyOf :agentToAgentRelation_role ;
    skos:changeNote
        [
            dc:date "2023-11-08" ;
            rdf:value """In order to get a system of rolified Relation classes: created
               the object property, with domain and range the KnowingOfRelation rolified class.
               Declared it as reflexive. Declared it(s) superproperty(ies)."""@en ;
        ] ;
    skos:scopeNote """This property "rolifies" the KnowingOfRelation class. It should
         be used only when you have to manage instances of the KnowingOfRelation class, to connect
         each instance to itself, in order to be able to infer, using OWL-RL and property paths, the
         two shortcuts corresponding to this n-ary class."""@en ;
.

:knows
    a
        owl:ObjectProperty ,
        owl:SymmetricProperty ;
    rdfs:label
        "knows"@en ,
        "conoce a"@es ,
        "connaît"@fr ;
    rdfs:comment """Connects two Persons that directly know each other during their
         existence. This relation is symmetric."""@en ;
    rdfs:domain :Person ;
    rdfs:isDefinedBy <https://www.ica.org/standards/RiC/ontology> ;
    rdfs:range :Person ;
    rdfs:subPropertyOf :isAgentAssociatedWithAgent ;
    owl:propertyChainAxiom (
        :thingIsConnectedToRelation
        :knowingRelation_role
        :relationConnects
    ) ;
    skos:changeNote
        [
            dc:date "2023-11-08" ;
            rdf:value """In order to get a system of rolified Relation classes: modified
               the property chain axiom so that it now involves the new knowingRelation_role object
               property."""@en ;
        ] ,
        [
            dc:date "2023-11-12" ;
            rdf:value """Aligned with RiC-CM 1.0: updated the description
               (rdfs:comment), skos:scopeNote."""@en ;
        ] ,
        [
            dc:date "2023-11-02" ;
            rdf:value "Added a new rdfs:label in Spanish."@en ;
        ] ,
        [
            dc:date "2023-08-28" ;
            rdf:value "Added a new rdfs:label in French."@en ;
        ] ;
    skos:scopeNote """The relation implies that the two Persons met or at least
         corresponded with each other."""@en ;
    :RiCCMCorrespondingComponent """RiC-R051 ('knows'
         relation)"""@en ;
.

:leadershipRelation_role
    a
        owl:ObjectProperty ,
        owl:ReflexiveProperty ;
    rdfs:label
        "has the role of the Leadership Relation"@en ,
        "desempeña el papel de la Relación de liderazgo"@es ,
        "a le rôle de la Relation de direction"@fr ;
    rdfs:comment """Connects a LeadershipRelation to itself. It is a reflexive
         property, that can stand for an instance of the class when necessary, e.g. when you explore
         a knowledge graph."""@en ;
    rdfs:domain :LeadershipRelation ;
    rdfs:isDefinedBy <https://www.ica.org/standards/RiC/ontology> ;
    rdfs:range :LeadershipRelation ;
    rdfs:subPropertyOf :agentControlRelation_role ;
    skos:changeNote
        [
            dc:date "2023-11-08" ;
            rdf:value """In order to get a system of rolified Relation classes: created
               the object property, with domain and range the LeadershipRelation rolified class.
               Declared it as reflexive. Declared it(s) superproperty(ies)."""@en ;
        ] ;
    skos:scopeNote """This property "rolifies" the LeadershipRelation class. It should
         be used only when you have to manage instances of the LeadershipRelation class, to connect
         each instance to itself, in order to be able to infer, using OWL-RL and property paths, the
         two shortcuts corresponding to this n-ary class."""@en ;
.

:mandateRelation_role
    a
        owl:ObjectProperty ,
        owl:ReflexiveProperty ;
    rdfs:label
        "has the role of the Mandate Relation"@en ,
        "desempeña el papel de la Relación normativa"@es ,
        "a le rôle de la Relation impliquant un mandat"@fr ;
    rdfs:comment """Connects a MandateRelation to itself. It is a reflexive property,
         that can stand for an instance of the class when necessary, e.g. when you explore a
         knowledge graph."""@en ;
    rdfs:domain :MandateRelation ;
    rdfs:isDefinedBy <https://www.ica.org/standards/RiC/ontology> ;
    rdfs:range :MandateRelation ;
    rdfs:subPropertyOf :ruleRelation_role ;
    skos:changeNote
        [
            dc:date "2023-11-08" ;
            rdf:value """In order to get a system of rolified Relation classes: created
               the object property, with domain and range the MandateRelation rolified class.
               Declared it as reflexive. Declared it(s) superproperty(ies)."""@en ;
        ] ;
    skos:scopeNote """This property "rolifies" the MandateRelation class. It should be
         used only when you have to manage instances of the MandateRelation class, to connect each
         instance to itself, in order to be able to infer, using OWL-RL and property paths, the two
         shortcuts corresponding to this n-ary class."""@en ;
.

:membershipRelation_role
    a
        owl:ObjectProperty ,
        owl:ReflexiveProperty ;
    rdfs:label
        "has the role of the Membership Relation"@en ,
        "desempeña el papel de la Relación de membresía"@es ,
        "a le rôle de la Relation d’appartenance"@fr ;
    rdfs:comment """Connects a MembershipRelation to itself. It is a reflexive
         property, that can stand for an instance of the class when necessary, e.g. when you explore
         a knowledge graph."""@en ;
    rdfs:domain :MembershipRelation ;
    rdfs:isDefinedBy <https://www.ica.org/standards/RiC/ontology> ;
    rdfs:range :MembershipRelation ;
    rdfs:subPropertyOf :agentToAgentRelation_role ;
    skos:changeNote
        [
            dc:date "2023-11-08" ;
            rdf:value """In order to get a system of rolified Relation classes: created
               the object property, with domain and range the MembershipRelation rolified class.
               Declared it as reflexive. Declared it(s) superproperty(ies)."""@en ;
        ] ;
    skos:scopeNote """This property "rolifies" the MembershipRelation class. It should
         be used only when you have to manage instances of the MembershipRelation class, to connect
         each instance to itself, in order to be able to infer, using OWL-RL and property paths, the
         two shortcuts corresponding to this n-ary class."""@en ;
.

:migrationRelation_role
    a
        owl:ObjectProperty ,
        owl:ReflexiveProperty ;
    rdfs:label
        "has the role of the Migration Relation"@en ,
        """desempeña el papel de la Relación de migración entre
         instanciaciones"""@es ,
        "a le rôle de la Relation de migration"@fr ;
    rdfs:comment """Connects a MigrationRelation to itself. It is a reflexive
         property, that can stand for an instance of the class when necessary, e.g. when you explore
         a knowledge graph."""@en ;
    rdfs:domain :MigrationRelation ;
    rdfs:isDefinedBy <https://www.ica.org/standards/RiC/ontology> ;
    rdfs:range :MigrationRelation ;
    rdfs:subPropertyOf :derivationRelation_role ;
    skos:changeNote
        [
            dc:date "2023-11-08" ;
            rdf:value """In order to get a system of rolified Relation classes: created
               the object property, with domain and range the MigrationRelation rolified class.
               Declared it as reflexive. Declared it(s) superproperty(ies)."""@en ;
        ] ;
    skos:scopeNote """This property "rolifies" the MigrationRelation class. It should
         be used only when you have to manage instances of the MigrationRelation class, to connect
         each instance to itself, in order to be able to infer, using OWL-RL and property paths, the
         two shortcuts corresponding to this n-ary class."""@en ;
.

:ownershipRelation_role
    a
        owl:ObjectProperty ,
        owl:ReflexiveProperty ;
    rdfs:label
        "has the role of the Ownership Relation"@en ,
        "desempeña el papel de la Relación de posesión"@es ,
        "a le rôle de la Relation de propriété"@fr ;
    rdfs:comment """Connects a OwnershipRelation to itself. It is a reflexive
         property, that can stand for an instance of the class when necessary, e.g. when you explore
         a knowledge graph."""@en ;
    rdfs:domain :OwnershipRelation ;
    rdfs:isDefinedBy <https://www.ica.org/standards/RiC/ontology> ;
    rdfs:range :OwnershipRelation ;
    rdfs:subPropertyOf :authorityRelation_role ;
    skos:changeNote
        [
            dc:date "2023-11-08" ;
            rdf:value """In order to get a system of rolified Relation classes: created
               the object property, with domain and range the OwnershipRelation rolified class.
               Declared it as reflexive. Declared it(s) superproperty(ies)."""@en ;
        ] ;
    skos:scopeNote """This property "rolifies" the OwnershipRelation class. It should
         be used only when you have to manage instances of the OwnershipRelation class, to connect
         each instance to itself, in order to be able to infer, using OWL-RL and property paths, the
         two shortcuts corresponding to this n-ary class."""@en ;
.

:performanceRelation_role
    a
        owl:ObjectProperty ,
        owl:ReflexiveProperty ;
    rdfs:label
        "has the role of the Performance Relation"@en ,
        """desempeña el papel de la Relación de desarrollo
         funcional"""@es ,
        "a le rôle de la Relation entre activités et agents"@fr ;
    rdfs:comment """Connects a PerformanceRelation to itself. It is a reflexive
         property, that can stand for an instance of the class when necessary, e.g. when you explore
         a knowledge graph."""@en ;
    rdfs:domain :PerformanceRelation ;
    rdfs:isDefinedBy <https://www.ica.org/standards/RiC/ontology> ;
    rdfs:range :PerformanceRelation ;
    rdfs:subPropertyOf :eventRelation_role ;
    skos:changeNote
        [
            dc:date "2023-11-08" ;
            rdf:value """In order to get a system of rolified Relation classes: created
               the object property, with domain and range the PerformanceRelation rolified class.
               Declared it as reflexive. Declared it(s) superproperty(ies)."""@en ;
        ] ;
    skos:scopeNote """This property "rolifies" the PerformanceRelation class. It
         should be used only when you have to manage instances of the PerformanceRelation class, to
         connect each instance to itself, in order to be able to infer, using OWL-RL and property
         paths, the two shortcuts corresponding to this n-ary class."""@en ;
.

:physicalOrLogicalExtent
    a owl:DatatypeProperty ;
    rdfs:label
        "physical or logical extent"@en ,
        "soporte físico o lógico"@es ,
        "importance physique ou logique"@fr ;
    rdfs:comment """Countable characteristics of the content of an entity expressed as
         a quantity."""@en ;
    rdfs:domain
        [
            a owl:Class ;
            owl:unionOf (
                :Instantiation
                :RecordResource
            ) ;
        ] ;
    rdfs:isDefinedBy <https://www.ica.org/standards/RiC/ontology> ;
    rdfs:range rdfs:Literal ;
    skos:changeNote
        [
            dc:date "2023-11-02" ;
            rdf:value "Added a new rdfs:label in Spanish."@en ;
        ] ,
        [
            dc:date "2023-08-25" ;
            rdf:value "Added a new rdfs:label in French."@en ;
        ] ;
    skos:scopeNote """Provided for usability reasons. Use only if you cannot use the
         subproperties (particularly if the same free text is being used in your current metadata
         for describing the record resource, carrier and instantiation extent)."""@en ;
.

:placeRelation_role
    a
        owl:ObjectProperty ,
        owl:ReflexiveProperty ;
    rdfs:label
        "has the role of the Place Relation"@en ,
        "desempeña el papel de la Relación con lugar"@es ,
        "a le rôle de la Relation impliquant un lieu"@fr ;
    rdfs:comment """Connects a PlaceRelation to itself. It is a reflexive property,
         that can stand for an instance of the class when necessary, e.g. when you explore a
         knowledge graph."""@en ;
    rdfs:domain :PlaceRelation ;
    rdfs:isDefinedBy <https://www.ica.org/standards/RiC/ontology> ;
    rdfs:range :PlaceRelation ;
    rdfs:subPropertyOf :relation_role ;
    skos:changeNote
        [
            dc:date "2023-11-08" ;
            rdf:value """In order to get a system of rolified Relation classes: created
               the object property, with domain and range the PlaceRelation rolified class. Declared
               it as reflexive. Declared it(s) superproperty(ies)."""@en ;
        ] ;
    skos:scopeNote """This property "rolifies" the PlaceRelation class. It should be
         used only when you have to manage instances of the PlaceRelation class, to connect each
         instance to itself, in order to be able to infer, using OWL-RL and property paths, the two
         shortcuts corresponding to this n-ary class."""@en ;
.

:positionHoldingRelation_role
    a
        owl:ObjectProperty ,
        owl:ReflexiveProperty ;
    rdfs:label
        "has the role of the Position Holding Relation"@en ,
        """desempeña el papel de la Relación de ocupación entre una persona y
         un puesto"""@es ,
        "a le rôle de la Relation entre une personne et un poste"@fr ;
    rdfs:comment """Connects a PositionHoldingRelation to itself. It is a reflexive
         property, that can stand for an instance of the class when necessary, e.g. when you explore
         a knowledge graph."""@en ;
    rdfs:domain :PositionHoldingRelation ;
    rdfs:isDefinedBy <https://www.ica.org/standards/RiC/ontology> ;
    rdfs:range :PositionHoldingRelation ;
    rdfs:subPropertyOf :agentToAgentRelation_role ;
    skos:changeNote
        [
            dc:date "2023-11-08" ;
            rdf:value """In order to get a system of rolified Relation classes: created
               the object property, with domain and range the PositionHoldingRelation rolified
               class. Declared it as reflexive. Declared it(s) superproperty(ies)."""@en ;
        ] ;
    skos:scopeNote """This property "rolifies" the PositionHoldingRelation class. It
         should be used only when you have to manage instances of the PositionHoldingRelation class,
         to connect each instance to itself, in order to be able to infer, using OWL-RL and property
         paths, the two shortcuts corresponding to this n-ary class."""@en ;
.

:positionToGroupRelation_role
    a
        owl:ObjectProperty ,
        owl:ReflexiveProperty ;
    rdfs:label
        "has the role of the Position to Group Relation"@en ,
        """desempeña el papel de la Relación de ocupación entre un grupo y un
         puesto"""@es ,
        "a le rôle de la Relation entre un poste et un groupe"@fr ;
    rdfs:comment """Connects a PositionToGroupRelation to itself. It is a reflexive
         property, that can stand for an instance of the class when necessary, e.g. when you explore
         a knowledge graph."""@en ;
    rdfs:domain :PositionToGroupRelation ;
    rdfs:isDefinedBy <https://www.ica.org/standards/RiC/ontology> ;
    rdfs:range :PositionToGroupRelation ;
    rdfs:subPropertyOf :agentToAgentRelation_role ;
    skos:changeNote
        [
            dc:date "2023-11-08" ;
            rdf:value """In order to get a system of rolified Relation classes: created
               the object property, with domain and range the PositionToGroupRelation rolified
               class. Declared it as reflexive. Declared it(s) superproperty(ies)."""@en ;
        ] ;
    skos:scopeNote """This property "rolifies" the PositionToGroupRelation class. It
         should be used only when you have to manage instances of the PositionToGroupRelation class,
         to connect each instance to itself, in order to be able to infer, using OWL-RL and property
         paths, the two shortcuts corresponding to this n-ary class."""@en ;
.

:recordResourceHoldingRelation_role
    a
        owl:ObjectProperty ,
        owl:ReflexiveProperty ;
    rdfs:label
        "has the role of the Record Resource Holding Relation"@en ,
        """desempeña el papel de la Relación entre agentes y recursos
         documentales que conservan"""@es ,
        """a le rôle de la Relation entre agents et ressources archivistiques
         ou instanciations conservées"""@fr ;
    rdfs:comment """Connects a RecordResourceHoldingRelation to itself. It is a
         reflexive property, that can stand for an instance of the class when necessary, e.g. when
         you explore a knowledge graph."""@en ;
    rdfs:domain :RecordResourceHoldingRelation ;
    rdfs:isDefinedBy <https://www.ica.org/standards/RiC/ontology> ;
    rdfs:range :RecordResourceHoldingRelation ;
    rdfs:subPropertyOf :managementRelation_role ;
    skos:changeNote
        [
            dc:date "2023-12-30" ;
            rdf:value "Fixed a typo in the French label."@en ;
        ] ,
        [
            dc:date "2023-11-08" ;
            rdf:value """In order to get a system of rolified Relation classes: created
               the object property, with domain and range the RecordResourceHoldingRelation rolified
               class. Declared it as reflexive. Declared it(s) superproperty(ies)."""@en ;
        ] ;
    skos:scopeNote """This property "rolifies" the RecordResourceHoldingRelation
         class. It should be used only when you have to manage instances of the
         RecordResourceHoldingRelation class, to connect each instance to itself, in order to be
         able to infer, using OWL-RL and property paths, the two shortcuts corresponding to this
         n-ary class."""@en ;
.

:recordResourceToInstantiationRelation_role
    a
        owl:ObjectProperty ,
        owl:ReflexiveProperty ;
    rdfs:label
        """has the role of the Record Resource to Instantiation
         Relation"""@en ,
        """desempeña el papel de la Relación de recurso documental a
         instanciación"""@es ,
        "a le rôle de la Relation d’instanciation"@fr ;
    rdfs:comment """Connects a RecordResourceToInstantiationRelation to itself. It is
         a reflexive property, that can stand for an instance of the class when necessary, e.g. when
         you explore a knowledge graph."""@en ;
    rdfs:domain :RecordResourceToInstantiationRelation ;
    rdfs:isDefinedBy <https://www.ica.org/standards/RiC/ontology> ;
    rdfs:range :RecordResourceToInstantiationRelation ;
    rdfs:subPropertyOf :relation_role ;
    skos:changeNote
        [
            dc:date "2023-11-08" ;
            rdf:value """In order to get a system of rolified Relation classes: created
               the object property, with domain and range the RecordResourceToInstantiationRelation
               rolified class. Declared it as reflexive. Declared it(s)
               superproperty(ies)."""@en ;
        ] ;
    skos:scopeNote """This property "rolifies" the
         RecordResourceToInstantiationRelation class. It should be used only when you have to manage
         instances of the RecordResourceToInstantiationRelation class, to connect each instance to
         itself, in order to be able to infer, using OWL-RL and property paths, the two shortcuts
         corresponding to this n-ary class."""@en ;
.

:recordResourceToRecordResourceRelation_role
    a
        owl:ObjectProperty ,
        owl:ReflexiveProperty ;
    rdfs:label
        """has the role of the Record Resource to Record Resource
         Relation"""@en ,
        """desempeña el papel de la Relación entre recursos
         documentales"""@es ,
        """a le rôle de la Relation entre ressources
         archivistiques"""@fr ;
    rdfs:comment """Connects a RecordResourceToRecordResourceRelation to itself. It is
         a reflexive property, that can stand for an instance of the class when necessary, e.g. when
         you explore a knowledge graph."""@en ;
    rdfs:domain :RecordResourceToRecordResourceRelation ;
    rdfs:isDefinedBy <https://www.ica.org/standards/RiC/ontology> ;
    rdfs:range :RecordResourceToRecordResourceRelation ;
    rdfs:subPropertyOf :relation_role ;
    skos:changeNote
        [
            dc:date "2023-11-08" ;
            rdf:value """In order to get a system of rolified Relation classes: created
               the object property, with domain and range the RecordResourceToRecordResourceRelation
               rolified class. Declared it as reflexive. Declared it(s)
               superproperty(ies)."""@en ;
        ] ;
    skos:scopeNote """This property "rolifies" the
         RecordResourceToRecordResourceRelation class. It should be used only when you have to
         manage instances of the RecordResourceToRecordResourceRelation class, to connect each
         instance to itself, in order to be able to infer, using OWL-RL and property paths, the two
         shortcuts corresponding to this n-ary class."""@en ;
.

:teachingRelation_role
    a
        owl:ObjectProperty ,
        owl:ReflexiveProperty ;
    rdfs:label
        "has the role of the Teaching Relation"@en ,
        """desempeña el papel de la Relación académica entre profesor y
         alumno"""@es ,
        "a le rôle de la Relation entre enseignants et étudiants"@fr ;
    rdfs:comment """Connects a TeachingRelation to itself. It is a reflexive property,
         that can stand for an instance of the class when necessary, e.g. when you explore a
         knowledge graph."""@en ;
    rdfs:domain :TeachingRelation ;
    rdfs:isDefinedBy <https://www.ica.org/standards/RiC/ontology> ;
    rdfs:range :TeachingRelation ;
    rdfs:subPropertyOf :knowingRelation_role ;
    skos:changeNote
        [
            dc:date "2023-11-08" ;
            rdf:value """In order to get a system of rolified Relation classes: created
               the object property, with domain and range the TeachingRelation rolified class.
               Declared it as reflexive. Declared it(s) superproperty(ies)."""@en ;
        ] ;
    skos:scopeNote """This property "rolifies" the TeachingRelation class. It should
         be used only when you have to manage instances of the TeachingRelation class, to connect
         each instance to itself, in order to be able to infer, using OWL-RL and property paths, the
         two shortcuts corresponding to this n-ary class."""@en ;
.

:textualValue
    a owl:DatatypeProperty ;
    rdfs:label
        "textual value"@en ,
        "valor textual"@es ,
        "valeur textuelle"@fr ;
    rdfs:comment "A textual expression of an Appellation or Date."@en ;
    rdfs:domain
        [
            a owl:Class ;
            owl:unionOf (
                :Appellation
                :Date
                :Extent
            ) ;
        ] ;
    rdfs:isDefinedBy <https://www.ica.org/standards/RiC/ontology> ;
    rdfs:range rdfs:Literal ;
    skos:changeNote
        [
            dc:date "2023-11-02" ;
            rdf:value "Added a new rdfs:label in Spanish."@en ;
        ] ,
        [
            dc:date "2023-08-25" ;
            rdf:value "Added a new rdfs:label in French."@en ;
        ] ;
.

:typeRelation_role
    a
        owl:ObjectProperty ,
        owl:ReflexiveProperty ;
    rdfs:label
        "has the role of the Type Relation"@en ,
        "desempeña el papel de la Tipo de relación"@es ,
        "a le rôle de la Relation de catégorisation"@fr ;
    rdfs:comment """Connects a TypeRelation to itself. It is a reflexive property,
         that can stand for an instance of the class when necessary, e.g. when you explore a
         knowledge graph."""@en ;
    rdfs:domain :TypeRelation ;
    rdfs:isDefinedBy <https://www.ica.org/standards/RiC/ontology> ;
    rdfs:range :TypeRelation ;
    rdfs:subPropertyOf :relation_role ;
    skos:changeNote
        [
            dc:date "2023-11-08" ;
            rdf:value """In order to get a system of rolified Relation classes: created
               the object property, with domain and range the TypeRelation rolified class. Declared
               it as reflexive. Declared it(s) superproperty(ies)."""@en ;
        ] ;
    skos:scopeNote """This property "rolifies" the TypeRelation class. It should be
         used only when you have to manage instances of the TypeRelation class, to connect each
         instance to itself, in order to be able to infer, using OWL-RL and property paths, the two
         shortcuts corresponding to this n-ary class."""@en ;
.

:AgentHierarchicalRelation
    a owl:Class ;
    rdfs:label
        "Agent Hierarchical Relation"@en ,
        "Relación jerárquica entre agentes"@es ,
        "Relation hiérarchique entre agents"@fr ;
    rdfs:comment """Connects at least one Agent to at least another Agent, when the
         first one is or was hierarchically superior to the second one. The Relation is oriented
         towards the 'bottom' of the hierarchical tree: the superior Agent(s) is the source of the
         Relation, and the inferior Agent(s) is the target."""@en ;
    rdfs:isDefinedBy <https://www.ica.org/standards/RiC/ontology> ;
    rdfs:subClassOf
        [
            a owl:Restriction ;
            owl:minQualifiedCardinality "1"^^xsd:nonNegativeInteger ;
            owl:onClass :Agent ;
            owl:onProperty :relationHasSource ;
        ] ,
        [
            a owl:Restriction ;
            owl:minQualifiedCardinality "1"^^xsd:nonNegativeInteger ;
            owl:onClass :Agent ;
            owl:onProperty :relationHasTarget ;
        ] ,
        :AgentToAgentRelation ;
    owl:equivalentClass
        [
            a owl:Restriction ;
            owl:hasSelf true ;
            owl:onProperty :agentHierarchicalRelation_role ;
        ] ;
    skos:changeNote
        [
            dc:date "2023-11-08" ;
            rdf:value """In order to get a system of rolified Relation classes: added an
               equivalentClass object property; replaced the specific object properties by the
               generic ones in the subClassOf declarations."""@en ;
        ] ,
        [
            dc:date "2023-08-25" ;
            rdf:value "Added a new rdfs:label in French."@en ;
        ] ,
        [
            dc:date "2023-11-12" ;
            rdf:value """Aligned with RiC-CM 1.0: updated the description
               (rdfs:comment), skos:scopeNote."""@en ;
        ] ,
        [
            dc:date "2023-11-02" ;
            rdf:value "Added a new rdfs:label in Spanish."@en ;
        ] ,
        [
            dc:date "2023-12-06" ;
            rdf:value """Improved the description of the Relation class (rdfs:comment)
               by clearly specifying how it is directed."""@en ;
        ] ;
    skos:scopeNote """The hierarchical relation can be an authority relation, or a
         whole/part relation between two agents."""@en ;
    :RiCCMCorrespondingComponent """Class implementation of RiC-R045 and RiC-R045i
         relations"""@en ;
.

:EventRelation
    a owl:Class ;
    rdfs:label
        "Event Relation"@en ,
        "Relación con un evento"@es ,
        "Relation impliquant un événement"@fr ;
    rdfs:comment """Connects at least one Event to at least one Thing, when the first
         is associated with the existence and lifecycle of the second one. The Event(s) is the
         source of the Relation, and the Thing(s) is the target."""@en ;
    rdfs:isDefinedBy <https://www.ica.org/standards/RiC/ontology> ;
    rdfs:subClassOf
        [
            a owl:Restriction ;
            owl:minQualifiedCardinality "1"^^xsd:nonNegativeInteger ;
            owl:onClass :Event ;
            owl:onProperty :relationHasSource ;
        ] ,
        [
            a owl:Restriction ;
            owl:minQualifiedCardinality "1"^^xsd:nonNegativeInteger ;
            owl:onClass :Thing ;
            owl:onProperty :relationHasTarget ;
        ] ,
        :Relation ;
    owl:equivalentClass
        [
            a owl:Restriction ;
            owl:hasSelf true ;
            owl:onProperty :eventRelation_role ;
        ] ;
    skos:changeNote
        [
            dc:date "2023-11-08" ;
            rdf:value """In order to get a system of rolified Relation classes: added an
               equivalentClass object property; replaced the specific object properties by the
               generic ones in the subClassOf declarations."""@en ;
        ] ,
        [
            dc:date "2023-11-12" ;
            rdf:value """Aligned with RiC-CM 1.0: updated the
               skos:scopeNote."""@en ;
        ] ,
        [
            dc:date "2023-08-25" ;
            rdf:value "Added a new rdfs:label in French."@en ;
        ] ,
        [
            dc:date "2023-11-02" ;
            rdf:value "Added a new rdfs:label in Spanish."@en ;
        ] ,
        [
            dc:date "2023-12-06" ;
            rdf:value """Improved the description of the Relation class (rdfs:comment)
               by clearly specifying how it is directed."""@en ;
        ] ;
    skos:scopeNote """Use to connect an event and an entity only if it is not possible
         to specify a narrower event relation, for example a PerformanceRelation."""@en ;
    :RiCCMCorrespondingComponent """Class implementation of RiC-R057 and RiC-R057i
         relations"""@en ;
.

:Identifier
    a owl:Class ;
    rdfs:label
        "Identifier"@en ,
        "Identificador"@es ,
        "Identifiant"@fr ;
    rdfs:comment """A word, number, letter, symbol, or any combination of these used
         to uniquely identify or reference an individual instance of an entity within a specific
         information domain."""@en ;
    rdfs:isDefinedBy <https://www.ica.org/standards/RiC/ontology> ;
    rdfs:subClassOf :Appellation ;
    skos:changeNote
        [
            dc:date "2023-08-25" ;
            rdf:value "Added a new rdfs:label in French."@en ;
        ] ,
        [
            dc:date "2023-04-19" ;
            rdf:value "Removed the 0.2 existing unnecessary restriction."@en ;
        ] ,
        [
            dc:date "2023-11-12" ;
            rdf:value """Aligned with RiC-CM 1.0: updated the
               skos:scopeNote."""@en ;
        ] ,
        [
            dc:date "2023-11-02" ;
            rdf:value "Added a new rdfs:label in Spanish."@en ;
        ] ;
    skos:scopeNote """Can include Global Persistent Identifiers (globally unique and
         persistently resolvable identifier for the entity) and/or Local Identifiers. Both the
         domain within which the identifier is unique, and the rules used in forming the identifier
         value should be provided with the identifier value."""@en ;
    :RiCCMCorrespondingComponent """Class implementation of RiC-A22 (Identifier
         attribute) (see also the identifier datatype property)"""@en ;
.

:InstantiationToInstantiationRelation
    a owl:Class ;
    rdfs:label
        "Instantiation to Instantiation Relation"@en ,
        "Relación entre instanciaciones"@es ,
        "Relation entre instanciations"@fr ;
    rdfs:comment """Connects at least two instantiations. This Relation is a generic,
         not oriented one."""@en ;
    rdfs:isDefinedBy <https://www.ica.org/standards/RiC/ontology> ;
    rdfs:subClassOf
        [
            a owl:Restriction ;
            owl:minQualifiedCardinality "2"^^xsd:nonNegativeInteger ;
            owl:onClass :Instantiation ;
            owl:onProperty :relationConnects ;
        ] ,
        :Relation ;
    owl:equivalentClass
        [
            a owl:Restriction ;
            owl:hasSelf true ;
            owl:onProperty :instantiationToInstantiationRelation_role ;
        ] ;
    skos:changeNote
        [
            dc:date "2023-08-25" ;
            rdf:value "Added a new rdfs:label in French."@en ;
        ] ,
        [
            dc:date "2023-11-02" ;
            rdf:value "Added a new rdfs:label in Spanish."@en ;
        ] ,
        [
            dc:date "2023-11-08" ;
            rdf:value """In order to get a system of rolified Relation classes: added an
               equivalentClass object property; replaced the specific object properties by the
               generic ones in the subClassOf declarations."""@en ;
        ] ,
        [
            dc:date "2023-12-06" ;
            rdf:value """Improved the description of the Relation class (rdfs:comment)
               by clearly specifying how it is directed."""@en ;
        ] ;
.

:KnowingRelation
    a owl:Class ;
    rdfs:label
        "Knowing Relation"@en ,
        "Relación de conocimiento directo entre personas"@es ,
        "Relation de connaissance entre personnes"@fr ;
    rdfs:comment """Connects at least two Persons who directly know each other during
         their existence. This Relation is not oriented."""@en ;
    rdfs:isDefinedBy <https://www.ica.org/standards/RiC/ontology> ;
    rdfs:subClassOf
        [
            a owl:Restriction ;
            owl:minQualifiedCardinality "2"^^xsd:nonNegativeInteger ;
            owl:onClass :Person ;
            owl:onProperty :relationConnects ;
        ] ,
        :AgentToAgentRelation ;
    owl:equivalentClass
        [
            a owl:Restriction ;
            owl:hasSelf true ;
            owl:onProperty :knowingRelation_role ;
        ] ;
    skos:changeNote
        [
            dc:date "2023-11-12" ;
            rdf:value """Aligned with RiC-CM 1.0: updated the description
               (rdfs:comment), skos:scopeNote."""@en ;
        ] ,
        [
            dc:date "2023-12-06" ;
            rdf:value """Improved the description of the Relation class (rdfs:comment)
               by clearly specifying how it is directed."""@en ;
        ] ,
        [
            dc:date "2023-11-02" ;
            rdf:value "Added a new rdfs:label in Spanish."@en ;
        ] ,
        [
            dc:date "2023-11-08" ;
            rdf:value """In order to get a system of rolified Relation classes: added an
               equivalentClass object property; replaced the specific object properties by the
               generic ones in the subClassOf declarations."""@en ;
        ] ,
        [
            dc:date "2023-08-25" ;
            rdf:value "Added a new rdfs:label in French."@en ;
        ] ;
    skos:scopeNote """The relation implies that the two persons met or at least
         corresponded with each other."""@en ;
    :RiCCMCorrespondingComponent """Class implementation of RiC-R051 and RiC—R051i
         relations"""@en ;
.

:LeadershipRelation
    a owl:Class ;
    rdfs:label
        "Leadership Relation"@en ,
        "Relación de liderazgo"@es ,
        "Relation de direction"@fr ;
    rdfs:comment """Connects at least one Person and at least one Group, when the
         first one(s) lead(s) or led the second one(s). The Relation is oriented from the leading
         Person to the Group: the leading Person(s) is the source of the Relation, and the Group(s)
         is the target."""@en ;
    rdfs:isDefinedBy <https://www.ica.org/standards/RiC/ontology> ;
    rdfs:subClassOf
        [
            a owl:Restriction ;
            owl:minQualifiedCardinality "1"^^xsd:nonNegativeInteger ;
            owl:onClass :Person ;
            owl:onProperty :relationHasSource ;
        ] ,
        [
            a owl:Restriction ;
            owl:maxQualifiedCardinality "1"^^xsd:nonNegativeInteger ;
            owl:onClass :Position ;
            owl:onProperty :leadershipWithPosition ;
        ] ,
        [
            a owl:Restriction ;
            owl:minQualifiedCardinality "1"^^xsd:nonNegativeInteger ;
            owl:onClass :Group ;
            owl:onProperty :relationHasTarget ;
        ] ,
        :AgentControlRelation ;
    owl:equivalentClass
        [
            a owl:Restriction ;
            owl:hasSelf true ;
            owl:onProperty :leadershipRelation_role ;
        ] ;
    skos:changeNote
        [
            dc:date "2023-11-08" ;
            rdf:value """In order to get a system of rolified Relation classes: added an
               equivalentClass object property; replaced the specific object properties by the
               generic ones in the subClassOf declarations."""@en ;
        ] ,
        [
            dc:date "2023-11-12" ;
            rdf:value """Aligned with RiC-CM 1.0: updated the description
               (rdfs:comment)."""@en ;
        ] ,
        [
            dc:date "2023-11-02" ;
            rdf:value "Added a new rdfs:label in Spanish."@en ;
        ] ,
        [
            dc:date "2023-08-25" ;
            rdf:value "Added a new rdfs:label in French."@en ;
        ] ,
        [
            dc:date "2023-12-06" ;
            rdf:value """Improved the description of the Relation class (rdfs:comment)
               by clearly specifying how it is directed."""@en ;
        ] ;
    :RiCCMCorrespondingComponent """Class implementation of RiC-R042 and RiC-R042i
         relations"""@en ;
.

:MembershipRelation
    a owl:Class ;
    rdfs:label
        "Membership Relation"@en ,
        "Relación de membresía"@es ,
        "Relation d’appartenance"@fr ;
    rdfs:comment """Connects a Group and at least one Person, when the first one has
         or had the second one(s) among its members. The Relation is oriented from the Group to its
         members: the Group(s) is the source of the Relation, and the Person(s) is the
         target."""@en ;
    rdfs:isDefinedBy <https://www.ica.org/standards/RiC/ontology> ;
    rdfs:subClassOf
        [
            a owl:Restriction ;
            owl:minQualifiedCardinality "1"^^xsd:nonNegativeInteger ;
            owl:onClass :Person ;
            owl:onProperty :relationHasTarget ;
        ] ,
        [
            a owl:Restriction ;
            owl:onClass :Group ;
            owl:onProperty :relationHasSource ;
            owl:qualifiedCardinality "1"^^xsd:nonNegativeInteger ;
        ] ,
        [
            a owl:Restriction ;
            owl:maxQualifiedCardinality "1"^^xsd:nonNegativeInteger ;
            owl:onClass :Position ;
            owl:onProperty :membershipWithPosition ;
        ] ,
        :AgentToAgentRelation ;
    owl:equivalentClass
        [
            a owl:Restriction ;
            owl:hasSelf true ;
            owl:onProperty :membershipRelation_role ;
        ] ;
    skos:changeNote
        [
            dc:date "2023-11-02" ;
            rdf:value "Added a new rdfs:label in Spanish."@en ;
        ] ,
        [
            dc:date "2023-08-25" ;
            rdf:value "Added a new rdfs:label in French."@en ;
        ] ,
        [
            dc:date "2023-12-06" ;
            rdf:value """Improved the description of the Relation class (rdfs:comment)
               by clearly specifying how it is directed."""@en ;
        ] ,
        [
            dc:date "2023-11-12" ;
            rdf:value """Aligned with RiC-CM 1.0: updated the description
               (rdfs:comment)."""@en ;
        ] ,
        [
            dc:date "2023-11-08" ;
            rdf:value """In order to get a system of rolified Relation classes: added an
               equivalentClass object property; replaced the specific object properties by the
               generic ones in the subClassOf declarations."""@en ;
        ] ;
    :RiCCMCorrespondingComponent """Class implementation of RiC-R055 and RiC-R055i
         relations"""@en ;
.

:OrganicOrFunctionalProvenanceRelation
    a owl:Class ;
    rdfs:label
        "Organic or functional provenance Relation"@en ,
        "Relación de procedencia orgánica or funcional"@es ,
        "Relation de provenance organique ou fonctionnelle"@fr ;
    rdfs:comment """Connects at least one Record Resource or Instantiation to at least
         one Agent or Activity, when the Agent or Activity is the provenance of the Record Resource
         or Instantiation (i.e. when the Agent created, accumulated or maintained the Record
         Resource or Instantiation, or when the Activity resulted into them). The Record Resource(s)
         or Instantiation(s) is the source of the Relation, and the Agent(s) or Activity(-ies) is
         the target."""@en ;
    rdfs:isDefinedBy <https://www.ica.org/standards/RiC/ontology> ;
    rdfs:subClassOf
        [
            a owl:Restriction ;
            owl:minQualifiedCardinality "1"^^xsd:nonNegativeInteger ;
            owl:onClass
                [
                    a owl:Class ;
                    owl:unionOf (
                        :Instantiation
                        :RecordResource
                    ) ;
                ] ;
            owl:onProperty :relationHasSource ;
        ] ,
        [
            a owl:Restriction ;
            owl:minQualifiedCardinality "1"^^xsd:nonNegativeInteger ;
            owl:onClass
                [
                    a owl:Class ;
                    owl:unionOf (
                        :Activity
                        :Agent
                    ) ;
                ] ;
            owl:onProperty :relationHasTarget ;
        ] ,
        :Relation ;
    owl:equivalentClass
        [
            a owl:Restriction ;
            owl:hasSelf true ;
            owl:onProperty :organicOrFunctionalProvenanceRelation_role ;
        ] ;
    skos:changeNote
        [
            dc:date "2023-11-07" ;
            rdf:value """Renamed the relation (its name was
               ProvenanceRelation)."""@en ;
        ] ,
        [
            dc:date "2023-08-25" ;
            rdf:value "Added a new rdfs:label in French."@en ;
        ] ,
        [
            dc:date "2023-12-06" ;
            rdf:value """Improved the description of the Relation class (rdfs:comment)
               by clearly specifying how it is directed."""@en ;
        ] ,
        [
            dc:date "2023-11-08" ;
            rdf:value """In order to get a system of rolified Relation classes: added an
               equivalentClass object property; replaced the specific object properties by the
               generic ones in the subClassOf declarations."""@en ;
        ] ,
        [
            dc:date "2023-11-02" ;
            rdf:value "Added a new rdfs:label in Spanish."@en ;
        ] ;
    skos:scopeNote """This relation stands for organic and for functional
         provenance."""@en ;
.

:OrganicProvenanceRelation
    a owl:Class ;
    rdfs:label
        "Organic Provenance Relation"@en ,
        "Relación de procedencia orgánica"@es ,
        "Relation de provenance organique"@fr ;
    rdfs:comment """Connects at least one Record Resource or an Instantiation to at
         least one Agent that creates or accumulates the Record Resource, receives it, or sends it.
         The Record Resource(s) or Instantiation(s) is the source of the Relation, and the Agent(s)
         is the target."""@en ;
    rdfs:isDefinedBy <https://www.ica.org/standards/RiC/ontology> ;
    rdfs:subClassOf
        [
            a owl:Restriction ;
            owl:minQualifiedCardinality "1"^^xsd:nonNegativeInteger ;
            owl:onClass :Agent ;
            owl:onProperty :relationHasTarget ;
        ] ,
        [
            a owl:Restriction ;
            owl:minQualifiedCardinality "1"^^xsd:nonNegativeInteger ;
            owl:onClass
                [
                    a owl:Class ;
                    owl:unionOf (
                        :Instantiation
                        :RecordResource
                    ) ;
                ] ;
            owl:onProperty :relationHasSource ;
        ] ,
        :OrganicOrFunctionalProvenanceRelation ;
    owl:equivalentClass
        [
            a owl:Restriction ;
            owl:hasSelf true ;
            owl:onProperty :organicProvenanceRelation_role ;
        ] ;
    skos:changeNote
        [
            dc:date "2023-11-12" ;
            rdf:value """Aligned with RiC-CM 1.0: updated the description
               (rdfs:comment), skos:scopeNote."""@en ;
        ] ,
        [
            dc:date "2023-08-25" ;
            rdf:value "Added a new rdfs:label in French."@en ;
        ] ,
        [
            dc:date "2023-11-07" ;
            rdf:value """Renamed the relation in order to make it clearer (its name was
               AgentOriginationRelation)."""@en ;
        ] ,
        [
            dc:date "2023-11-08" ;
            rdf:value """In order to get a system of rolified Relation classes: added an
               equivalentClass object property; replaced the specific object properties by the
               generic ones in the subClassOf declarations."""@en ;
        ] ,
        [
            dc:date "2023-12-06" ;
            rdf:value """Improved the description of the Relation class (rdfs:comment)
               by clearly specifying how it is directed."""@en ;
        ] ,
        [
            dc:date "2023-11-02" ;
            rdf:value "Added a new rdfs:label in Spanish."@en ;
        ] ;
    skos:scopeNote """This is the most general organic provenance relation. Use it to
         connect a record resource or instantiation with an agent only if it is not possible to use
         a narrower, more specific relation, for example Creation Relation."""@en ;
    :RiCCMCorrespondingComponent """Class implementation of RiC-R026 and RiC-R026i
         relations"""@en ;
.

:PhysicalLocation
    a owl:Class ;
    rdfs:label
        "Physical Location"@en ,
        "Localización física de lugar"@es ,
        "Localisation physique"@fr ;
    rdfs:comment """A delimitation of the physical territory of a
         Place."""@en ;
    rdfs:isDefinedBy <https://www.ica.org/standards/RiC/ontology> ;
    rdfs:subClassOf :Thing ;
    skos:changeNote
        [
            dc:date "2023-11-02" ;
            rdf:value "Added a new rdfs:label in Spanish."@en ;
        ] ,
        [
            dc:date "2023-04-19" ;
            rdf:value """Removed the two 0.2 existing unnecessary
               restrictions."""@en ;
        ] ,
        [
            dc:date "2023-11-12" ;
            rdf:value """Aligned with RiC-CM 1.0: updated the
               skos:scopeNote."""@en ;
        ] ,
        [
            dc:date "2023-08-25" ;
            rdf:value "Added a new rdfs:label in French."@en ;
        ] ;
    skos:scopeNote """Used to describe basic human-readable text such as an address, a
         cadastral reference, or less precise information found in a record. Use the coordinates
         datatype property, or the Coordinates class to capture the geographical coordinates of the
         Place. Use spatial relations (particularly 'has or had location') to capture a relation
         between two places."""@en ;
    :RiCCMCorrespondingComponent """Class implementation of RiC-A27 (Location
         attribute)"""@en ;
.

:TemporalRelation
    a owl:Class ;
    rdfs:label
        "Temporal Relation"@en ,
        "Relación temporal"@es ,
        "Relation temporelle"@fr ;
    rdfs:comment """Connects at least one Thing to at least one other Thing that
         follows it in chronological order. The Relation is oriented chronologically: the preceding
         Thing(s) is the source of the Relation, the following Thing(s) is the
         target."""@en ;
    rdfs:isDefinedBy <https://www.ica.org/standards/RiC/ontology> ;
    rdfs:subClassOf
        [
            a owl:Restriction ;
            owl:minQualifiedCardinality "1"^^xsd:nonNegativeInteger ;
            owl:onClass :Thing ;
            owl:onProperty :relationHasTarget ;
        ] ,
        [
            a owl:Restriction ;
            owl:minQualifiedCardinality "1"^^xsd:nonNegativeInteger ;
            owl:onClass :Thing ;
            owl:onProperty :relationHasSource ;
        ] ,
        :SequentialRelation ;
    owl:equivalentClass
        [
            a owl:Restriction ;
            owl:hasSelf true ;
            owl:onProperty :temporalRelation_role ;
        ] ;
    skos:changeNote
        [
            dc:date "2023-11-08" ;
            rdf:value """In order to get a system of rolified Relation classes: added an
               equivalentClass object property; replaced the specific object properties by the
               generic ones in the subClassOf declarations."""@en ;
        ] ,
        [
            dc:date "2023-12-06" ;
            rdf:value """Improved the description of the Relation class (rdfs:comment)
               by clearly specifying how it is directed."""@en ;
        ] ,
        [
            dc:date "2023-11-02" ;
            rdf:value "Added a new rdfs:label in Spanish."@en ;
        ] ,
        [
            dc:date "2023-08-25" ;
            rdf:value "Added a new rdfs:label in French."@en ;
        ] ,
        [
            dc:date "2023-11-12" ;
            rdf:value """Aligned with RiC-CM 1.0: updated the
               skos:scopeNote."""@en ;
        ] ;
    skos:scopeNote """There may be zero to many intermediate entities, ignored or
         unknown, in the chronological sequence between the connected entities."""@en ;
    :RiCCMCorrespondingComponent """Class implementation of RiC-R009 and RiC-R009i
         relations"""@en ;
.

:agentControlRelation_role
    a
        owl:ObjectProperty ,
        owl:ReflexiveProperty ;
    rdfs:label
        "has the role of the Agent Control Relation"@en ,
        """desempeña el papel de la Relación de control entre
         agentes"""@es ,
        "a le rôle de la Relation de contrôle entre agents"@fr ;
    rdfs:comment """Connects a AgentControlRelation to itself. It is a reflexive
         property, that can stand for an instance of the class when necessary, e.g. when you explore
         a knowledge graph."""@en ;
    rdfs:domain :AgentControlRelation ;
    rdfs:isDefinedBy <https://www.ica.org/standards/RiC/ontology> ;
    rdfs:range :AgentControlRelation ;
    rdfs:subPropertyOf
        :agentHierarchicalRelation_role ,
        :authorityRelation_role ;
    skos:changeNote
        [
            dc:date "2023-11-08" ;
            rdf:value """In order to get a system of rolified Relation classes: created
               the object property, with domain and range the AgentControlRelation rolified class.
               Declared it as reflexive. Declared it(s) superproperty(ies)."""@en ;
        ] ;
    skos:scopeNote """This property "rolifies" the AgentControlRelation class. It
         should be used only when you have to manage instances of the AgentControlRelation class, to
         connect each instance to itself, in order to be able to infer, using OWL-RL and property
         paths, the two shortcuts corresponding to this n-ary class."""@en ;
.

:agentTemporalRelation_role
    a
        owl:ObjectProperty ,
        owl:ReflexiveProperty ;
    rdfs:label
        "has the role of the Agent Temporal Relation"@en ,
        """desempeña el papel de la Relación temporal entre
         agentes"""@es ,
        "a le rôle de la Relation temporelle entre agents"@fr ;
    rdfs:comment """Connects a AgentTemporalRelation to itself. It is a reflexive
         property, that can stand for an instance of the class when necessary, e.g. when you explore
         a knowledge graph."""@en ;
    rdfs:domain :AgentTemporalRelation ;
    rdfs:isDefinedBy <https://www.ica.org/standards/RiC/ontology> ;
    rdfs:range :AgentTemporalRelation ;
    rdfs:subPropertyOf
        :agentToAgentRelation_role ,
        :temporalRelation_role ;
    skos:changeNote
        [
            dc:date "2023-11-08" ;
            rdf:value """In order to get a system of rolified Relation classes: created
               the object property, with domain and range the AgentTemporalRelation rolified class.
               Declared it as reflexive. Declared it(s) superproperty(ies)."""@en ;
        ] ;
    skos:scopeNote """This property "rolifies" the AgentTemporalRelation class. It
         should be used only when you have to manage instances of the AgentTemporalRelation class,
         to connect each instance to itself, in order to be able to infer, using OWL-RL and property
         paths, the two shortcuts corresponding to this n-ary class."""@en ;
.

:creationRelation_role
    a
        owl:ObjectProperty ,
        owl:ReflexiveProperty ;
    rdfs:label
        "has the role of the Creation Relation"@en ,
        "desempeña el papel de la Relación de creación"@es ,
        "a le rôle de la Relation de création"@fr ;
    rdfs:comment """Connects a CreationRelation to itself. It is a reflexive property,
         that can stand for an instance of the class when necessary, e.g. when you explore a
         knowledge graph."""@en ;
    rdfs:domain :CreationRelation ;
    rdfs:isDefinedBy <https://www.ica.org/standards/RiC/ontology> ;
    rdfs:range :CreationRelation ;
    rdfs:subPropertyOf :organicProvenanceRelation_role ;
    skos:changeNote
        [
            dc:date "2023-11-08" ;
            rdf:value """In order to get a system of rolified Relation classes: created
               the object property, with domain and range the CreationRelation rolified class.
               Declared it as reflexive. Declared it(s) superproperty(ies)."""@en ;
        ] ;
    skos:scopeNote """This property "rolifies" the CreationRelation class. It should
         be used only when you have to manage instances of the CreationRelation class, to connect
         each instance to itself, in order to be able to infer, using OWL-RL and property paths, the
         two shortcuts corresponding to this n-ary class."""@en ;
.

:date
    a owl:DatatypeProperty ;
    rdfs:label
        "date"@en ,
        "fecha"@es ,
        "date"@fr ;
    rdfs:comment """Chronological information associated with an entity that
         contributes to its identification and contextualization."""@en ;
    rdfs:domain :Thing ;
    rdfs:isDefinedBy <https://www.ica.org/standards/RiC/ontology> ;
    rdfs:range rdfs:Literal ;
    skos:changeNote
        [
            dc:date "2023-11-02" ;
            rdf:value "Added a new rdfs:label in Spanish."@en ;
        ] ,
        [
            dc:date "2023-08-25" ;
            rdf:value "Added a new rdfs:label in French."@en ;
        ] ;
    skos:scopeNote """Provided for usability reasons, like its subproperties. May be
         deprecated and removed later on. Use only if you don't use Date classes for handling
         dates."""@en ;
    :RiCCMCorrespondingComponent """Datatype property implementation of RiC-E18 (Date
         entity)"""@en ;
.

:derivationRelation_role
    a
        owl:ObjectProperty ,
        owl:ReflexiveProperty ;
    rdfs:label
        "has the role of the Derivation Relation"@en ,
        "desempeña el papel de la Relación de derivación"@es ,
        "a le rôle de la Relation de dérivation"@fr ;
    rdfs:comment """Connects a DerivationRelation to itself. It is a reflexive
         property, that can stand for an instance of the class when necessary, e.g. when you explore
         a knowledge graph."""@en ;
    rdfs:domain :DerivationRelation ;
    rdfs:isDefinedBy <https://www.ica.org/standards/RiC/ontology> ;
    rdfs:range :DerivationRelation ;
    rdfs:subPropertyOf
        :instantiationToInstantiationRelation_role ,
        :temporalRelation_role ;
    skos:changeNote
        [
            dc:date "2023-11-08" ;
            rdf:value """In order to get a system of rolified Relation classes: created
               the object property, with domain and range the DerivationRelation rolified class.
               Declared it as reflexive. Declared it(s) superproperty(ies)."""@en ;
        ] ;
    skos:scopeNote """This property "rolifies" the DerivationRelation class. It should
         be used only when you have to manage instances of the DerivationRelation class, to connect
         each instance to itself, in order to be able to infer, using OWL-RL and property paths, the
         two shortcuts corresponding to this n-ary class."""@en ;
.

:descendanceRelation_role
    a
        owl:ObjectProperty ,
        owl:ReflexiveProperty ;
    rdfs:label
        "has the role of the Descendance Relation"@en ,
        "desempeña el papel de la Relación de descendencia"@es ,
        "a le rôle de la Relation de descendance"@fr ;
    rdfs:comment """Connects a DescendanceRelation to itself. It is a reflexive
         property, that can stand for an instance of the class when necessary, e.g. when you explore
         a knowledge graph."""@en ;
    rdfs:domain :DescendanceRelation ;
    rdfs:isDefinedBy <https://www.ica.org/standards/RiC/ontology> ;
    rdfs:range :DescendanceRelation ;
    rdfs:subPropertyOf
        :agentTemporalRelation_role ,
        :familyRelation_role ;
    skos:changeNote
        [
            dc:date "2023-11-08" ;
            rdf:value """In order to get a system of rolified Relation classes: created
               the object property, with domain and range the DescendanceRelation rolified class.
               Declared it as reflexive. Declared it(s) superproperty(ies)."""@en ;
        ] ;
    skos:scopeNote """This property "rolifies" the DescendanceRelation class. It
         should be used only when you have to manage instances of the DescendanceRelation class, to
         connect each instance to itself, in order to be able to infer, using OWL-RL and property
         paths, the two shortcuts corresponding to this n-ary class."""@en ;
.

:followsOrFollowed
    a owl:ObjectProperty ;
    rdfs:label
        "follows or followed"@en ,
        "sigue o seguía a"@es ,
        "suit ou a suivi"@fr ;
    rdfs:comment "Inverse of 'precedesOrPreceded' object property."@en ;
    rdfs:domain :Thing ;
    rdfs:isDefinedBy <https://www.ica.org/standards/RiC/ontology> ;
    rdfs:range :Thing ;
    rdfs:subPropertyOf :isRelatedTo ;
    owl:inverseOf :precedesOrPreceded ;
    owl:propertyChainAxiom (
        :thingIsTargetOfRelation
        :sequentialRelation_role
        :relationHasSource
    ) ;
    skos:changeNote
        [
            dc:date "2021-01-22" ;
            rdf:value """changed the IRI, label, inverse property IRI, text definition,
               corresponding CM component name (changed made in order to make RiC-O compliant with
               RiC-CM 0.2; the name of this property in RiC-O 0.1 was "follows")."""@en ;
        ] ,
        [
            dc:date "2023-11-08" ;
            rdf:value """In order to get a system of rolified Relation classes: modified
               the property chain axiom so that it now involves the new sequentialRelation_role
               object property."""@en ;
        ] ,
        [
            dc:date "2023-08-28" ;
            rdf:value "Added a new rdfs:label in French."@en ;
        ] ,
        [
            dc:date "2023-11-02" ;
            rdf:value "Added a new rdfs:label in Spanish."@en ;
        ] ;
    :RiCCMCorrespondingComponent """RiC-R008i ('follows or followed'
         relation)"""@en ;
.

:hasEndDate
    a owl:ObjectProperty ;
    rdfs:label
        "has end date"@en ,
        "tiene como fecha final"@es ,
        "a pour date de fin"@fr ;
    rdfs:comment "Inverse of 'is end date of' object property."@en ;
    rdfs:domain :Thing ;
    rdfs:isDefinedBy <https://www.ica.org/standards/RiC/ontology> ;
    rdfs:range :Date ;
    rdfs:subPropertyOf :isAssociatedWithDate ;
    owl:inverseOf :isEndDateOf ;
    skos:changeNote
        [
            dc:date "2023-11-02" ;
            rdf:value "Added a new rdfs:label in Spanish."@en ;
        ] ,
        [
            dc:date "2023-08-28" ;
            rdf:value "Added a new rdfs:label in French."@en ;
        ] ;
    :RiCCMCorrespondingComponent """RiC-R071i ('has end date'
         relation)"""@en ;
.

:hasFamilyAssociationWith
    a
        owl:ObjectProperty ,
        owl:SymmetricProperty ;
    rdfs:label
        "has family association with"@en ,
        "tiene asociación familiar con"@es ,
        "a une relation familiale avec"@fr ;
    rdfs:comment """Connects two Persons that have some type of family link, i.e.
         belong to the same family. This relation is symmetric."""@en ;
    rdfs:domain :Person ;
    rdfs:isDefinedBy <https://www.ica.org/standards/RiC/ontology> ;
    rdfs:range :Person ;
    rdfs:subPropertyOf :isAgentAssociatedWithAgent ;
    owl:propertyChainAxiom (
        :thingIsConnectedToRelation
        :familyRelation_role
        :relationConnects
    ) ;
    skos:changeNote
        [
            dc:date "2023-08-28" ;
            rdf:value "Added a new rdfs:label in French."@en ;
        ] ,
        [
            dc:date "2023-11-08" ;
            rdf:value """In order to get a system of rolified Relation classes: modified
               the property chain axiom so that it now involves the new familyRelation_role object
               property."""@en ;
        ] ,
        [
            dc:date "2023-11-02" ;
            rdf:value "Added a new rdfs:label in Spanish."@en ;
        ] ,
        [
            dc:date "2021-01-22" ;
            rdf:value """changed the IRI, label, textual definition (changed made in
               order to make RiC-O compliant with RiC-CM 0.2; the name of this property in RiC-O 0.1
               was "hasFamilyLinkWith")."""@en ;
        ] ,
        [
            dc:date "2023-11-12" ;
            rdf:value """Aligned with RiC-CM 1.0: updated the
               skos:scopeNote."""@en ;
        ] ;
    skos:scopeNote """Use hasOrHadMember for connecting a Family and a
         Person."""@en ;
    :RiCCMCorrespondingComponent """RiC-R047 ('has family association with'
         relation)"""@en ;
.

:hasOrHadName
    a owl:ObjectProperty ;
    rdfs:label
        "has or had name"@en ,
        "tiene o tenía como nombre"@es ,
        "a ou a eu pour nom"@fr ;
    rdfs:comment """Connects a Thing to one of its past or present
         Names."""@en ;
    rdfs:domain :Thing ;
    rdfs:isDefinedBy <https://www.ica.org/standards/RiC/ontology> ;
    rdfs:range :Name ;
    rdfs:subPropertyOf :hasOrHadAppellation ;
    owl:inverseOf :isOrWasNameOf ;
    skos:changeNote
        [
            dc:date "2021-01-22" ;
            rdf:value """changed the IRI, label, inverse property IRI, textual
               definition, super property IRI (the name of this property in RiC-O 0.1 was
               "hasName")."""@en ;
        ] ,
        [
            dc:date "2023-08-28" ;
            rdf:value "Added a new rdfs:label in French."@en ;
        ] ,
        [
            dc:date "2023-11-02" ;
            rdf:value "Added a new rdfs:label in Spanish."@en ;
        ] ;
.

:hasSuccessor
    a owl:ObjectProperty ;
    rdfs:label
        "has successor"@en ,
        "tiene como sucesor(a) a"@es ,
        "a pour successeur"@fr ;
    rdfs:comment """Connects an Agent to another Agent that succeeds it
         chronologically."""@en ;
    rdfs:domain :Agent ;
    rdfs:isDefinedBy <https://www.ica.org/standards/RiC/ontology> ;
    rdfs:range :Agent ;
    rdfs:subPropertyOf
        :isAgentAssociatedWithAgent ,
        :precedesInTime ;
    owl:inverseOf :isSuccessorOf ;
    owl:propertyChainAxiom (
        :thingIsSourceOfRelation
        :agentTemporalRelation_role
        :relationHasTarget
    ) ;
    skos:changeNote
        [
            dc:date "2021-01-22" ;
            rdf:value """changed the IRI and label (changed made in order to make RiC-O
               compliant with RiC-CM 0.2; the name of this property in RiC-O 0.1 was
               "isAntecedentOf")."""@en ;
        ] ,
        [
            dc:date "2023-11-08" ;
            rdf:value """In order to get a system of rolified Relation classes: modified
               the property chain axiom so that it now involves the new agentTemporalRelation_role
               object property."""@en ;
        ] ,
        [
            dc:date "2023-11-02" ;
            rdf:value "Added a new rdfs:label in Spanish."@en ;
        ] ,
        [
            dc:date "2023-08-28" ;
            rdf:value "Added a new rdfs:label in French."@en ;
        ] ;
    skos:scopeNote """There may be zero to many intermediate Agents, ignored or
         unknown, between the two connected Agents. Can be used when there is a transfer of function
         from the first Agent to the second Agent."""@en ;
    :RiCCMCorrespondingComponent """RIC-R016 ('has successor'
         relation)"""@en ;
.

:instantiationToInstantiationRelation_role
    a
        owl:ObjectProperty ,
        owl:ReflexiveProperty ;
    rdfs:label
        """has the role of the Instantiation to Instantiation
         Relation"""@en ,
        "desempeña el papel de la Relación entre instanciaciones"@es ,
        "a le rôle de la Relation entre instanciations"@fr ;
    rdfs:comment """Connects a InstantiationToInstantiationRelation to itself. It is a
         reflexive property, that can stand for an instance of the class when necessary, e.g. when
         you explore a knowledge graph."""@en ;
    rdfs:domain :InstantiationToInstantiationRelation ;
    rdfs:isDefinedBy <https://www.ica.org/standards/RiC/ontology> ;
    rdfs:range :InstantiationToInstantiationRelation ;
    rdfs:subPropertyOf :relation_role ;
    skos:changeNote
        [
            dc:date "2023-11-08" ;
            rdf:value """In order to get a system of rolified Relation classes: created
               the object property, with domain and range the InstantiationToInstantiationRelation
               rolified class. Declared it as reflexive. Declared it(s)
               superproperty(ies)."""@en ;
        ] ;
    skos:scopeNote """This property "rolifies" the
         InstantiationToInstantiationRelation class. It should be used only when you have to manage
         instances of the InstantiationToInstantiationRelation class, to connect each instance to
         itself, in order to be able to infer, using OWL-RL and property paths, the two shortcuts
         corresponding to this n-ary class."""@en ;
.

:isEndDateOf
    a owl:ObjectProperty ;
    rdfs:label
        "is end date of"@en ,
        "es fecha final de"@es ,
        "est la date de fin de"@fr ;
    rdfs:comment """Connects a Date to a Thing whose existence ended on that
         Date."""@en ;
    rdfs:domain :Date ;
    rdfs:isDefinedBy <https://www.ica.org/standards/RiC/ontology> ;
    rdfs:range :Thing ;
    rdfs:subPropertyOf :isDateAssociatedWith ;
    owl:inverseOf :hasEndDate ;
    skos:changeNote
        [
            dc:date "2023-11-02" ;
            rdf:value "Added a new rdfs:label in Spanish."@en ;
        ] ,
        [
            dc:date "2023-08-28" ;
            rdf:value "Added a new rdfs:label in French."@en ;
        ] ;
    :RiCCMCorrespondingComponent """RiC-R071 ('is end date of'
         relation)"""@en ;
.

:isOrWasNameOf
    a owl:ObjectProperty ;
    rdfs:label
        "is or was name of"@en ,
        "es o era nombre de"@es ,
        "est ou a été le nom de"@fr ;
    rdfs:comment """Connects a Name to a Thing that it designated or
         designates."""@en ;
    rdfs:domain :Name ;
    rdfs:isDefinedBy <https://www.ica.org/standards/RiC/ontology> ;
    rdfs:range :Thing ;
    rdfs:subPropertyOf :isOrWasAppellationOf ;
    owl:inverseOf :hasOrHadName ;
    skos:changeNote
        [
            dc:date "2021-01-22" ;
            rdf:value """changed the IRI, label, inverse property IRI, textual
               definition, super property IRI (the name of this property in RiC-O 0.1 was
               "isNameOf")."""@en ;
        ] ,
        [
            dc:date "2023-08-28" ;
            rdf:value "Added a new rdfs:label in French."@en ;
        ] ,
        [
            dc:date "2023-11-02" ;
            rdf:value "Added a new rdfs:label in Spanish."@en ;
        ] ;
.

:isSuccessorOf
    a owl:ObjectProperty ;
    rdfs:label
        "is successor of"@en ,
        "es sucesor(a) de"@es ,
        "est le successeur de"@fr ;
    rdfs:comment "Inverse of 'has successor' object property."@en ;
    rdfs:domain :Agent ;
    rdfs:isDefinedBy <https://www.ica.org/standards/RiC/ontology> ;
    rdfs:range :Agent ;
    rdfs:subPropertyOf
        :followsInTime ,
        :isAgentAssociatedWithAgent ;
    owl:inverseOf :hasSuccessor ;
    owl:propertyChainAxiom (
        :thingIsTargetOfRelation
        :agentTemporalRelation_role
        :relationHasSource
    ) ;
    skos:changeNote
        [
            dc:date "2021-01-22" ;
            rdf:value """changed the inverse property IRI and the text
               definition."""@en ;
        ] ,
        [
            dc:date "2023-11-02" ;
            rdf:value "Added a new rdfs:label in Spanish."@en ;
        ] ,
        [
            dc:date "2023-11-08" ;
            rdf:value """In order to get a system of rolified Relation classes: modified
               the property chain axiom so that it now involves the new agentTemporalRelation_role
               object property."""@en ;
        ] ,
        [
            dc:date "2023-08-28" ;
            rdf:value "Added a new rdfs:label in French."@en ;
        ] ;
    :RiCCMCorrespondingComponent """RiC-R016i ('is successor of'
         relation)"""@en ;
.

:knowingRelation_role
    a
        owl:ObjectProperty ,
        owl:ReflexiveProperty ;
    rdfs:label
        "has the role of the Knowing Relation"@en ,
        """desempeña el papel de la Relación de conocimiento directo entre
         personas"""@es ,
        """a le rôle de la Relation de connaissance entre
         personnes"""@fr ;
    rdfs:comment """Connects a KnowingRelation to itself. It is a reflexive property,
         that can stand for an instance of the class when necessary, e.g. when you explore a
         knowledge graph."""@en ;
    rdfs:domain :KnowingRelation ;
    rdfs:isDefinedBy <https://www.ica.org/standards/RiC/ontology> ;
    rdfs:range :KnowingRelation ;
    rdfs:subPropertyOf :agentToAgentRelation_role ;
    skos:changeNote
        [
            dc:date "2023-11-08" ;
            rdf:value """In order to get a system of rolified Relation classes: created
               the object property, with domain and range the KnowingRelation rolified class.
               Declared it as reflexive. Declared it(s) superproperty(ies)."""@en ;
        ] ;
    skos:scopeNote """This property "rolifies" the KnowingRelation class. It should be
         used only when you have to manage instances of the KnowingRelation class, to connect each
         instance to itself, in order to be able to infer, using OWL-RL and property paths, the two
         shortcuts corresponding to this n-ary class."""@en ;
.

:managementRelation_role
    a
        owl:ObjectProperty ,
        owl:ReflexiveProperty ;
    rdfs:label
        "has the role of the Management Relation"@en ,
        "desempeña el papel de la Relación de gestión"@es ,
        "a le rôle de la Relation de gestion"@fr ;
    rdfs:comment """Connects a ManagementRelation to itself. It is a reflexive
         property, that can stand for an instance of the class when necessary, e.g. when you explore
         a knowledge graph."""@en ;
    rdfs:domain :ManagementRelation ;
    rdfs:isDefinedBy <https://www.ica.org/standards/RiC/ontology> ;
    rdfs:range :ManagementRelation ;
    rdfs:subPropertyOf :authorityRelation_role ;
    skos:changeNote
        [
            dc:date "2023-11-08" ;
            rdf:value """In order to get a system of rolified Relation classes: created
               the object property, with domain and range the ManagementRelation rolified class.
               Declared it as reflexive. Declared it(s) superproperty(ies)."""@en ;
        ] ;
    skos:scopeNote """This property "rolifies" the ManagementRelation class. It should
         be used only when you have to manage instances of the ManagementRelation class, to connect
         each instance to itself, in order to be able to infer, using OWL-RL and property paths, the
         two shortcuts corresponding to this n-ary class."""@en ;
.

:precedesOrPreceded
    a owl:ObjectProperty ;
    rdfs:label
        "precedes or preceded"@en ,
        "precede o precedía secuencialmente a"@es ,
        "précède ou a précédé"@fr ;
    rdfs:comment """Connects a Thing to a Thing that follows or followed it in some
         sequence."""@en ;
    rdfs:domain :Thing ;
    rdfs:isDefinedBy <https://www.ica.org/standards/RiC/ontology> ;
    rdfs:range :Thing ;
    rdfs:subPropertyOf :isRelatedTo ;
    owl:inverseOf :followsOrFollowed ;
    owl:propertyChainAxiom (
        :thingIsSourceOfRelation
        :sequentialRelation_role
        :relationHasTarget
    ) ;
    skos:changeNote
        [
            dc:date "2023-08-28" ;
            rdf:value "Added a new rdfs:label in French."@en ;
        ] ,
        [
            dc:date "2021-01-22" ;
            rdf:value """changed the IRI, label, inverse property IRI, text definition,
               corresponding CM component name (changed made in order to make RiC-O compliant with
               RiC-CM 0.2; the name of this property in RiC-O 0.1 was "precedes")."""@en ;
        ] ,
        [
            dc:date "2023-11-08" ;
            rdf:value """In order to get a system of rolified Relation classes: modified
               the property chain axiom so that it now involves the new sequentialRelation_role
               object property."""@en ;
        ] ,
        [
            dc:date "2023-11-02" ;
            rdf:value "Added a new rdfs:label in Spanish."@en ;
        ] ;
    skos:scopeNote """The relation does not specify by itself what criteria are used
         for ordering the sequence. There may actually be zero to many intermediate Entities,
         ignored or unkown, in the sequence between the two connected Things. Can be used, for
         example, for specifying that some Record 'precedes' (has next) some Record within a Record
         Set."""@en ;
    :RiCCMCorrespondingComponent """RiC-R008 ('precedes or preceded'
         relation)"""@en ;
.

:ruleRelation_role
    a
        owl:ObjectProperty ,
        owl:ReflexiveProperty ;
    rdfs:label
        "has the role of the Rule Relation"@en ,
        "desempeña el papel de la Relación con regla"@es ,
        "a le rôle de la Relation impliquant une règle"@fr ;
    rdfs:comment """Connects a RuleRelation to itself. It is a reflexive property,
         that can stand for an instance of the class when necessary, e.g. when you explore a
         knowledge graph."""@en ;
    rdfs:domain :RuleRelation ;
    rdfs:isDefinedBy <https://www.ica.org/standards/RiC/ontology> ;
    rdfs:range :RuleRelation ;
    rdfs:subPropertyOf :relation_role ;
    skos:changeNote
        [
            dc:date "2023-11-08" ;
            rdf:value """In order to get a system of rolified Relation classes: created
               the object property, with domain and range the RuleRelation rolified class. Declared
               it as reflexive. Declared it(s) superproperty(ies)."""@en ;
        ] ;
    skos:scopeNote """This property "rolifies" the RuleRelation class. It should be
         used only when you have to manage instances of the RuleRelation class, to connect each
         instance to itself, in order to be able to infer, using OWL-RL and property paths, the two
         shortcuts corresponding to this n-ary class."""@en ;
.

:sequentialRelation_role
    a
        owl:ObjectProperty ,
        owl:ReflexiveProperty ;
    rdfs:label
        "has the role of the Sequential Relation"@en ,
        "desempeña el papel de la Relación secuencial"@es ,
        "a le rôle de la Relation séquentielle"@fr ;
    rdfs:comment """Connects a SequentialRelation to itself. It is a reflexive
         property, that can stand for an instance of the class when necessary, e.g. when you explore
         a knowledge graph."""@en ;
    rdfs:domain :SequentialRelation ;
    rdfs:isDefinedBy <https://www.ica.org/standards/RiC/ontology> ;
    rdfs:range :SequentialRelation ;
    rdfs:subPropertyOf :relation_role ;
    skos:changeNote
        [
            dc:date "2023-11-08" ;
            rdf:value """In order to get a system of rolified Relation classes: created
               the object property, with domain and range the SequentialRelation rolified class.
               Declared it as reflexive. Declared it(s) superproperty(ies)."""@en ;
        ] ;
    skos:scopeNote """This property "rolifies" the SequentialRelation class. It should
         be used only when you have to manage instances of the SequentialRelation class, to connect
         each instance to itself, in order to be able to infer, using OWL-RL and property paths, the
         two shortcuts corresponding to this n-ary class."""@en ;
.

:wholePartRelation_role
    a
        owl:ObjectProperty ,
        owl:ReflexiveProperty ;
    rdfs:label
        "has the role of the Whole Part Relation"@en ,
        "desempeña el papel de la Relación entre todo y parte"@es ,
        "a le rôle de la Relation partitive"@fr ;
    rdfs:comment """Connects a WholePartRelation to itself. It is a reflexive
         property, that can stand for an instance of the class when necessary, e.g. when you explore
         a knowledge graph."""@en ;
    rdfs:domain :WholePartRelation ;
    rdfs:isDefinedBy <https://www.ica.org/standards/RiC/ontology> ;
    rdfs:range :WholePartRelation ;
    rdfs:subPropertyOf :relation_role ;
    skos:changeNote
        [
            dc:date "2023-11-08" ;
            rdf:value """In order to get a system of rolified Relation classes: created
               the object property, with domain and range the WholePartRelation rolified class.
               Declared it as reflexive. Declared it(s) superproperty(ies)."""@en ;
        ] ;
    skos:scopeNote """This property "rolifies" the WholePartRelation class. It should
         be used only when you have to manage instances of the WholePartRelation class, to connect
         each instance to itself, in order to be able to infer, using OWL-RL and property paths, the
         two shortcuts corresponding to this n-ary class."""@en ;
.

<https://www.ica.org/standards/RiC/vocabularies/documentaryFormTypes>
    a
        owl:NamedIndividual ,
        skos:ConceptScheme ;
    rdfs:label
        "Documentary Form Types"@en ,
        "Tipos documentales"@es ,
        "Types de documents"@fr ;
    dc:creator """International Coucil on Archives Expert Group on Archival
         Description (ICA EGAD)"""@en ;
    dc:language
        "en" ,
        "es" ,
        "fr" ;
    dc:title """International Council on Archives Records in Contexts Vocabulary for
         Documentary Form Types"""@en ;
    skos:changeNote
        [
            dc:date "2023-12-13" ;
            rdf:value """Completed the metadata of the vocabulary: added dc:language, a
               history note and a scope note."""@en ;
        ] ,
        [
            dc:date "2023-08-28" ;
            rdf:value "Added a new rdfs:label in French."@en ;
        ] ,
        [
            dc:date "2023-11-25" ;
            rdf:value "Added a new rdfs:label in Spanish."@en ;
        ] ;
    skos:definition """A vocabulary that provides URIs for describing documentary form
         types of RiC Records and Record Parts."""@en ;
    skos:hasTopConcept
        ric-dft:AuthorityRecord ,
        ric-dft:FindingAid ;
    skos:historyNote """This vocabulary was created within the Records in Contexts
         Ontology. When the ICA/EGAD developed RiC-O 1.0, it was decided that two versions of RiC-O
         would be released. The first one, consisting of a unique large OWL file, would remain the
         reference one. RiC-0 1.0 would also be provided as a set of files, in order to address
         specific needs, e.g. using only the core of the ontology, or using only the individuals it
         defined and defining new individuals. So from December 2023, you can find the vocabulary on
         Documentary Form Types, either in the unique large OWL RiC-O file, or as a separate file. """@en ;
    skos:scopeNote """For now this vocabulary only defines two top concepts; it should
         hopefully be completed later. The concepts defined in this vocabulary can be used in
         combination with RiC-O classes and properties, whenever necessary and appropriate, to
         assign a documentary form type to a Record or a Record Part, using the
         rico:hasDocumentaryFormType object property, or its inverse one. They also can be used to
         specify that a rico:RecordSet included or includes members whose some
         (rico:hasOrHadSomeMembersWithDocumentaryFormType) or all
         (rico:hasOrHadAllMembersWithDocumentaryFormType) have some Documentary Form Type. Each
         concept is both defined as a skos:Concept and a rico:DocumentaryFormType, so that it is
         possible to extend the classic definition of such concepts using RiC-O properties. For
         example, you can use rico:history, rico:date, or rico:isAssociatedWithPlace,
         rico:precedesInTime, if you consider a documentary form type as being a historical entity,
         known and used in some known space or time region."""@en ;
.

skos:note
    a owl:AnnotationProperty ;
    rdfs:isDefinedBy <http://www.w3.org/2004/02/skos/core> ;
.

:AgentTemporalRelation
    a owl:Class ;
    rdfs:label
        "Agent Temporal Relation"@en ,
        "Relación temporal entre agentes"@es ,
        "Relation temporelle entre agents"@fr ;
    rdfs:comment """Connects at least one Agent to at least another Agent that
         succeeds it chronologically for, for instance, fullfilling some functions or performing
         some activities. The Relation is oriented chronologically, from the predecessor to the
         successor: the predecessor Agent(s) is the source of the Relation, and the successor
         Agent(s) is the target."""@en ;
    rdfs:isDefinedBy <https://www.ica.org/standards/RiC/ontology> ;
    rdfs:subClassOf
        [
            a owl:Restriction ;
            owl:minQualifiedCardinality "1"^^xsd:nonNegativeInteger ;
            owl:onClass :Agent ;
            owl:onProperty :relationHasTarget ;
        ] ,
        [
            a owl:Restriction ;
            owl:minQualifiedCardinality "1"^^xsd:nonNegativeInteger ;
            owl:onClass :Agent ;
            owl:onProperty :relationHasSource ;
        ] ,
        :AgentToAgentRelation ,
        :TemporalRelation ;
    owl:equivalentClass
        [
            a owl:Restriction ;
            owl:hasSelf true ;
            owl:onProperty :agentTemporalRelation_role ;
        ] ;
    skos:changeNote
        [
            dc:date "2023-12-06" ;
            rdf:value """Improved the description of the Relation class (rdfs:comment)
               by clearly specifying how it is directed."""@en ;
        ] ,
        [
            dc:date "2023-08-25" ;
            rdf:value "Added a new rdfs:label in French."@en ;
        ] ,
        [
            dc:date "2023-11-02" ;
            rdf:value "Added a new rdfs:label in Spanish."@en ;
        ] ,
        [
            dc:date "2023-11-12" ;
            rdf:value """Aligned with RiC-CM 1.0: updated the
               skos:scopeNote."""@en ;
        ] ,
        [
            dc:date "2023-11-08" ;
            rdf:value """In order to get a system of rolified Relation classes: added an
               equivalentClass object property; replaced the specific object properties by the
               generic ones in the subClassOf declarations."""@en ;
        ] ,
        [
            dc:date "2023-04-19" ;
            rdf:value "Removed the 0.2 existing unnecessary restriction."@en ;
        ] ;
    skos:scopeNote """There may be zero to many intermediate agents, ignored or
         unknown, between the two connected agents. Can be used when there is a transfer of function
         from the first agent to the second agent."""@en ;
    :RiCCMCorrespondingComponent """Class implementation of RiC-R016 and RiC-016i
         relations"""@en ;
.

:Concept
    a owl:Class ;
    rdfs:label
        "Concept"@en ,
        "Concepto"@es ,
        "Concept"@fr ;
    rdfs:comment """An idea, unit of thought, abstract cultural object or
         category"""@en ;
    rdfs:isDefinedBy <https://www.ica.org/standards/RiC/ontology> ;
    rdfs:subClassOf :Thing ;
    skos:changeNote
        [
            dc:date "2023-11-02" ;
            rdf:value "Added a new rdfs:label in Spanish."@en ;
        ] ,
        [
            dc:date "2023-08-25" ;
            rdf:value "Added a new rdfs:label in French."@en ;
        ] ;
.

:CreationRelation
    a owl:Class ;
    rdfs:label
        "Creation Relation"@en ,
        "Relación de creación"@es ,
        "Relation de création"@fr ;
    rdfs:comment """Connects at least one Record Resource or Instantiation to at least
         one Agent, when the Agent is either responsible for all or some of the content of the
         Record Resource, or is a contributor to the genesis or production of the Instantiation. The
         Record Resource or Instantiation is the source of the Relation, and the Agent(s) is the
         target. """@en ;
    rdfs:isDefinedBy <https://www.ica.org/standards/RiC/ontology> ;
    rdfs:subClassOf
        [
            a owl:Restriction ;
            owl:minQualifiedCardinality "1"^^xsd:nonNegativeInteger ;
            owl:onClass
                [
                    a owl:Class ;
                    owl:unionOf (
                        :Instantiation
                        :RecordResource
                    ) ;
                ] ;
            owl:onProperty :relationHasSource ;
        ] ,
        [
            a owl:Restriction ;
            owl:minQualifiedCardinality "1"^^xsd:nonNegativeInteger ;
            owl:onClass :Agent ;
            owl:onProperty :relationHasTarget ;
        ] ,
        :OrganicProvenanceRelation ;
    owl:equivalentClass
        [
            a owl:Restriction ;
            owl:hasSelf true ;
            owl:onProperty :creationRelation_role ;
        ] ;
    skos:changeNote
        [
            dc:date "2023-11-12" ;
            rdf:value """Aligned with RiC-CM 1.0: updated the
               skos:scopeNote."""@en ;
        ] ,
        [
            dc:date "2023-12-06" ;
            rdf:value """Improved the description of the Relation class (rdfs:comment)
               by clearly specifying how it is directed."""@en ;
        ] ,
        [
            dc:date "2023-04-19" ;
            rdf:value "Removed a 0.2 existing unnecessary restriction."@en ;
        ] ,
        [
            dc:date "2023-11-02" ;
            rdf:value "Added a new rdfs:label in Spanish."@en ;
        ] ,
        [
            dc:date "2023-08-25" ;
            rdf:value "Added a new rdfs:label in French."@en ;
        ] ,
        [
            dc:date "2023-11-08" ;
            rdf:value """In order to get a system of rolified Relation classes: added an
               equivalentClass object property; replaced the specific object properties by the
               generic ones in the subClassOf declarations."""@en ;
        ] ;
    skos:scopeNote """Covers the definition of "author" in diplomatics, and any agent
         that makes a contribution to the intellectual content of a record resource. Can also be
         used for any agent that was involved in the genesis (e.g. with the role of witness,
         representative of the author etc.) or in the production (e.g. with the role of scribe,
         secretary, notary, printer etc.) of the record resource or instantiation."""@en ;
    :RiCCMCorrespondingComponent """Class implementation of RiC-R027 and RiC-R027i
         relations"""@en ;
.

:FamilyRelation
    a owl:Class ;
    rdfs:label
        "Family Relation"@en ,
        "Relación familiar"@es ,
        "Relation familiale"@fr ;
    rdfs:comment """Connects at least two Persons, when they have some family link,
         i.e. belong to the same family. This Relation is a generic, not oriented
         one."""@en ;
    rdfs:isDefinedBy <https://www.ica.org/standards/RiC/ontology> ;
    rdfs:subClassOf
        [
            a owl:Restriction ;
            owl:minQualifiedCardinality "2"^^xsd:nonNegativeInteger ;
            owl:onClass :Person ;
            owl:onProperty :relationConnects ;
        ] ,
        :AgentToAgentRelation ;
    owl:equivalentClass
        [
            a owl:Restriction ;
            owl:hasSelf true ;
            owl:onProperty :familyRelation_role ;
        ] ;
    skos:changeNote
        [
            dc:date "2023-11-02" ;
            rdf:value "Added a new rdfs:label in Spanish."@en ;
        ] ,
        [
            dc:date "2023-11-08" ;
            rdf:value """In order to get a system of rolified Relation classes: added an
               equivalentClass object property; replaced the specific object properties by the
               generic ones in the subClassOf declarations."""@en ;
        ] ,
        [
            dc:date "2023-08-25" ;
            rdf:value "Added a new rdfs:label in French."@en ;
        ] ,
        [
            dc:date "2023-11-12" ;
            rdf:value """Aligned with RiC-CM 1.0: updated the
               skos:scopeNote."""@en ;
        ] ,
        [
            dc:date "2023-12-06" ;
            rdf:value """Improved the description of the Relation class (rdfs:comment)
               by clearly specifying how it is directed."""@en ;
        ] ;
    skos:scopeNote """Use the MembershipRelation class for connecting a family and a
         person."""@en ;
    :RiCCMCorrespondingComponent """Class implementation of RiC-R047 and RiC-R047i
         relations"""@en ;
.

:Mandate
    a owl:Class ;
    rdfs:label
        "Mandate"@en ,
        "Norma"@es ,
        "Mandat"@fr ;
    rdfs:comment """Delegation of responsibility or authority by an Agent to another
         Agent to perform an Activity."""@en ;
    rdfs:isDefinedBy <https://www.ica.org/standards/RiC/ontology> ;
    rdfs:subClassOf :Rule ;
    skos:changeNote
        [
            dc:date "2023-04-21" ;
            rdf:value "Removed the 0.2 existing unnecessary restriction."@en ;
        ] ,
        [
            dc:date "2023-11-02" ;
            rdf:value "Added a new rdfs:label in Spanish."@en ;
        ] ,
        [
            dc:date "2023-08-25" ;
            rdf:value "Added a new rdfs:label in French."@en ;
        ] ,
        [
            dc:date "2020-10-23" ;
            rdf:value """Scope note: made separate paragraphs and updated. Objective: to
               make RiC-O compliant with RiC-CM v0.2."""@en ;
        ] ,
        [
            dc:date "2023-11-12" ;
            rdf:value """Aligned with RiC-CM 1.0: updated the description
               (rdfs:comment), skos:scopeNote."""@en ;
        ] ;
    skos:scopeNote """Mandate is a kind of Rule. A mandate confers the responsibility
         or authority of an agent to perform a specified activity. In addition to assigning an
         activity and delegating responsibility or authority to perform the activity to an agent, a
         mandate commonly limits the place (jurisdiction) and date (time period) within which an
         agent may perform the activity (where and when). Mandates exist in a specific social and
         cultural context, and within that context are subject to change over time. While a mandate
         may be tacit, in whole or part, it may be explicitly expressed in a variety of documentary
         sources (for example, constitutions, legislation, (legal) acts, statutes, legal codes,
         ordinances, charges, charters, or mission statements). The evidence for identifying a
         mandate may be found in its entirety in one documentary source (for example, a law or
         regulation), or may be found in two or more sources. A mandate should not be confused with
         the one or more documentary sources that serve as evidence of its identity. A documentary
         source is a record."""@en ;
    :RiCCMCorrespondingComponent """Corresponds to RiC-E17 (Mandate
         entity)"""@en ;
.

:Name
    a owl:Class ;
    rdfs:label
        "Name"@en ,
        "Nombre"@es ,
        "Nom"@fr ;
    rdfs:comment """A label, title or term designating an entity in order to make it
         distinguishable from other similar entities."""@en ;
    rdfs:isDefinedBy <https://www.ica.org/standards/RiC/ontology> ;
    rdfs:subClassOf :Appellation ;
    skos:changeNote
        [
            dc:date "2023-11-12" ;
            rdf:value """Aligned with RiC-CM 1.0: updated the description
               (rdfs:comment), skos:scopeNote."""@en ;
        ] ,
        [
            dc:date "2023-11-02" ;
            rdf:value "Added a new rdfs:label in Spanish."@en ;
        ] ,
        [
            dc:date "2023-08-25" ;
            rdf:value "Added a new rdfs:label in French."@en ;
        ] ;
    skos:scopeNote """Provides brief information about the content or other individual
         characteristics of the entity being described, necessary to distinguish it from other
         perhaps similar entities."""@en ;
    :RiCCMCorrespondingComponent """Class implementation of RiC-A28 (Name attribute)
         (see also the name datatype property)"""@en ;
.

:agentHierarchicalRelation_role
    a
        owl:ObjectProperty ,
        owl:ReflexiveProperty ;
    rdfs:label
        "has the role of the Agent Hierarchical Relation"@en ,
        """desempeña el papel de la Relación jerárquica entre
         agentes"""@es ,
        "a le rôle de la Relation hiérarchique entre agents"@fr ;
    rdfs:comment """Connects a AgentHierarchicalRelation to itself. It is a reflexive
         property, that can stand for an instance of the class when necessary, e.g. when you explore
         a knowledge graph."""@en ;
    rdfs:domain :AgentHierarchicalRelation ;
    rdfs:isDefinedBy <https://www.ica.org/standards/RiC/ontology> ;
    rdfs:range :AgentHierarchicalRelation ;
    rdfs:subPropertyOf :agentToAgentRelation_role ;
    skos:changeNote
        [
            dc:date "2023-11-08" ;
            rdf:value """In order to get a system of rolified Relation classes: created
               the object property, with domain and range the AgentHierarchicalRelation rolified
               class. Declared it as reflexive. Declared it(s) superproperty(ies)."""@en ;
        ] ;
    skos:scopeNote """This property "rolifies" the AgentHierarchicalRelation class. It
         should be used only when you have to manage instances of the AgentHierarchicalRelation
         class, to connect each instance to itself, in order to be able to infer, using OWL-RL and
         property paths, the two shortcuts corresponding to this n-ary class."""@en ;
.

:eventRelation_role
    a
        owl:ObjectProperty ,
        owl:ReflexiveProperty ;
    rdfs:label
        "has the role of the Event Relation"@en ,
        "desempeña el papel de la Relación con un evento"@es ,
        "a le rôle de la Relation impliquant un événement"@fr ;
    rdfs:comment """Connects a EventRelation to itself. It is a reflexive property,
         that can stand for an instance of the class when necessary, e.g. when you explore a
         knowledge graph."""@en ;
    rdfs:domain :EventRelation ;
    rdfs:isDefinedBy <https://www.ica.org/standards/RiC/ontology> ;
    rdfs:range :EventRelation ;
    rdfs:subPropertyOf :relation_role ;
    skos:changeNote
        [
            dc:date "2023-11-08" ;
            rdf:value """In order to get a system of rolified Relation classes: created
               the object property, with domain and range the EventRelation rolified class. Declared
               it as reflexive. Declared it(s) superproperty(ies)."""@en ;
        ] ;
    skos:scopeNote """This property "rolifies" the EventRelation class. It should be
         used only when you have to manage instances of the EventRelation class, to connect each
         instance to itself, in order to be able to infer, using OWL-RL and property paths, the two
         shortcuts corresponding to this n-ary class."""@en ;
.

:familyRelation_role
    a
        owl:ObjectProperty ,
        owl:ReflexiveProperty ;
    rdfs:label
        "has the role of the Family Relation"@en ,
        "desempeña el papel de la Relación familiar"@es ,
        "a le rôle de la Relation familiale"@fr ;
    rdfs:comment """Connects a FamilyRelation to itself. It is a reflexive property,
         that can stand for an instance of the class when necessary, e.g. when you explore a
         knowledge graph."""@en ;
    rdfs:domain :FamilyRelation ;
    rdfs:isDefinedBy <https://www.ica.org/standards/RiC/ontology> ;
    rdfs:range :FamilyRelation ;
    rdfs:subPropertyOf :agentToAgentRelation_role ;
    skos:changeNote
        [
            dc:date "2023-11-08" ;
            rdf:value """In order to get a system of rolified Relation classes: created
               the object property, with domain and range the FamilyRelation rolified class.
               Declared it as reflexive. Declared it(s) superproperty(ies)."""@en ;
        ] ;
    skos:scopeNote """This property "rolifies" the FamilyRelation class. It should be
         used only when you have to manage instances of the FamilyRelation class, to connect each
         instance to itself, in order to be able to infer, using OWL-RL and property paths, the two
         shortcuts corresponding to this n-ary class."""@en ;
.

:hasOrHadAllMembersWithCategory
    a owl:ObjectProperty ;
    rdfs:label
        "has or had all members with category"@en ,
        "tienen o tenían todos sus miembros como categoría"@es ,
        """inclut ou a inclus des membres ayant tous pour
         catégorie"""@fr ;
    rdfs:comment """Connects a Record Set and a Category (Type) to which all the
         Records or Record Parts that are or were included in the Record Set belong."""@en ;
    rdfs:domain :RecordSet ;
    rdfs:isDefinedBy <https://www.ica.org/standards/RiC/ontology> ;
    rdfs:range :Type ;
    rdfs:subPropertyOf :isRelatedTo ;
    owl:inverseOf :isOrWasCategoryOfAllMembersOf ;
    skos:changeNote
        [
            dc:date "2020-12-28" ;
            rdf:value """Object property added for handling the case where a Record Set
               is described as having all or some members that belong to some category (see RiC-CM
               0.2 attributes section, #4.4 on Record Set, Record and Record Part
               attributes)."""@en ;
        ] ,
        [
            dc:date "2023-08-28" ;
            rdf:value "Added a new rdfs:label in French."@en ;
        ] ,
        [
            dc:date "2023-11-02" ;
            rdf:value "Added a new rdfs:label in Spanish."@en ;
        ] ;
.

:hasOrHadAuthorityOver
    a owl:ObjectProperty ;
    rdfs:label
        "has or had authority over"@en ,
        "tiene o tenía control sobre"@es ,
        "a ou a eu autorité sur"@fr ;
    rdfs:comment """Connects an Agent to a Thing over which the Agent has or had some
         kind of authority."""@en ;
    rdfs:domain :Agent ;
    rdfs:isDefinedBy <https://www.ica.org/standards/RiC/ontology> ;
    rdfs:range :Thing ;
    rdfs:subPropertyOf :isRelatedTo ;
    owl:inverseOf :isOrWasUnderAuthorityOf ;
    owl:propertyChainAxiom (
        :thingIsSourceOfRelation
        :authorityRelation_role
        :relationHasTarget
    ) ;
    skos:changeNote
        [
            dc:date "2023-08-28" ;
            rdf:value "Added a new rdfs:label in French."@en ;
        ] ,
        [
            dc:date "2021-01-22" ;
            rdf:value """changed the IRI, label, inverse property IRI, textual
               definition (changed made in order to make RiC-O compliant with RiC-CM 0.2; the name
               of this property in RiC-O 0.1 was "hasAuthorityOver")."""@en ;
        ] ,
        [
            dc:date "2023-11-02" ;
            rdf:value "Added a new rdfs:label in Spanish."@en ;
        ] ,
        [
            dc:date "2023-11-12" ;
            rdf:value """Aligned with RiC-CM 1.0: updated the description
               (rdfs:comment), skos:scopeNote."""@en ;
        ] ,
        [
            dc:date "2023-11-08" ;
            rdf:value """In order to get a system of rolified Relation classes: modified
               the property chain axiom so that it now involves the new authorityRelation_role
               object property."""@en ;
        ] ;
    skos:scopeNote """Use only if it is not possible to specify a narrower authority
         relation, for example is or was owner of."""@en ;
    :RiCCMCorrespondingComponent """RiC-R036 ('has or had authority over'
         relation)"""@en ;
.

:hasOrHadSomeMembersWithCategory
    a owl:ObjectProperty ;
    rdfs:label
        "has or had some members with category"@en ,
        "tienen o tenían algunos de sus miembros como categoría"@es ,
        "inclut ou a inclus des membres ayant pour type"@fr ;
    rdfs:comment """Connects a Record Set and a Category (Type) to which some of the
         Records or Record Parts that are or were included in the Record Set belong."""@en ;
    rdfs:domain :RecordSet ;
    rdfs:isDefinedBy <https://www.ica.org/standards/RiC/ontology> ;
    rdfs:range :Type ;
    rdfs:subPropertyOf :isRelatedTo ;
    owl:inverseOf :isOrWasCategoryOfSomeMembersOf ;
    skos:changeNote
        [
            dc:date "2020-12-28" ;
            rdf:value """Object property added for handling the case where a Record Set
               is described as having all or some members that belong to some category (see RiC-CM
               0.2 attributes section, #4.4 on Record Set, Record and Record Part
               attributes)."""@en ;
        ] ,
        [
            dc:date "2023-11-02" ;
            rdf:value "Added a new rdfs:label in Spanish."@en ;
        ] ,
        [
            dc:date "2023-08-28" ;
            rdf:value "Added a new rdfs:label in French."@en ;
        ] ;
.

:hasOrHadSubordinate
    a owl:ObjectProperty ;
    rdfs:label
        "has or had subordinate"@en ,
        "tiene o tenía como subordinado o subordinada a"@es ,
        "a ou a eu pour subalterne"@fr ;
    rdfs:comment """Connects an Agent to an Agent that is hierarchically
         inferior."""@en ;
    rdfs:domain :Agent ;
    rdfs:isDefinedBy <https://www.ica.org/standards/RiC/ontology> ;
    rdfs:range :Agent ;
    rdfs:subPropertyOf :isAgentAssociatedWithAgent ;
    owl:inverseOf :isOrWasSubordinateTo ;
    owl:propertyChainAxiom (
        :thingIsSourceOfRelation
        :agentHierarchicalRelation_role
        :relationHasTarget
    ) ;
    skos:changeNote
        [
            dc:date "2023-11-02" ;
            rdf:value "Added a new rdfs:label in Spanish."@en ;
        ] ,
        [
            dc:date "2023-11-08" ;
            rdf:value """In order to get a system of rolified Relation classes: modified
               the property chain axiom so that it now involves the new
               agentHierarchicalRelation_role object property."""@en ;
        ] ,
        [
            dc:date "2023-11-12" ;
            rdf:value """Aligned with RiC-CM 1.0: updated the
               skos:scopeNote."""@en ;
        ] ,
        [
            dc:date "2021-01-22" ;
            rdf:value """changed the IRI, label, inverse property IRI (changed made in
               order to make RiC-O compliant with RiC-CM 0.2; the name of this property in RiC-O 0.1
               was "isHierarchicallySuperiorTo")."""@en ;
        ] ,
        [
            dc:date "2023-08-28" ;
            rdf:value "Added a new rdfs:label in French."@en ;
        ] ;
    skos:scopeNote """The hierarchical relation can be an authority relation, or a
         whole/part relation between two Agents."""@en ;
    :RiCCMCorrespondingComponent """RiC-R045 ('has or had subordinate '
         relation)"""@en ;
.

:hasOrganicProvenance
    a owl:ObjectProperty ;
    rdfs:label
        "has organic provenance"@en ,
        "tiene como procedencia orgánica"@es ,
        "a pour provenance organique"@fr ;
    rdfs:comment """Connects a Record Resource or an Instantiation to an Agent that
         creates or accumulates the Record Resource, receives it, or sends it."""@en ;
    rdfs:domain
        [
            a owl:Class ;
            owl:unionOf (
                :Instantiation
                :RecordResource
            ) ;
        ] ;
    rdfs:isDefinedBy <https://www.ica.org/standards/RiC/ontology> ;
    rdfs:range :Agent ;
    rdfs:subPropertyOf :hasOrganicOrFunctionalProvenance ;
    owl:inverseOf :isOrganicProvenanceOf ;
    owl:propertyChainAxiom (
        :thingIsSourceOfRelation
        :organicProvenanceRelation_role
        :relationHasTarget
    ) ;
    skos:changeNote
        [
            dc:date "2023-11-07" ;
            rdf:value """Made this property a subproperty of the new
               hasOrganicOrFunctionalProvenance property. Renamed it to make things clearer.
               Adjusted its labels."""@en ;
        ] ,
        [
            dc:date "2023-11-08" ;
            rdf:value """In order to get a system of rolified Relation classes: modified
               the property chain axiom so that it now involves the new
               organicProvenanceRelation_role object property."""@en ;
        ] ,
        [
            dc:date "2023-11-12" ;
            rdf:value """Aligned with RiC-CM 1.0: updated the
               skos:scopeNote."""@en ;
        ] ,
        [
            dc:date "2023-11-02" ;
            rdf:value "Added a new rdfs:label in Spanish."@en ;
        ] ,
        [
            dc:date "2023-08-28" ;
            rdf:value "Added a new rdfs:label in French."@en ;
        ] ;
    skos:scopeNote """This is the most general organic provenance relation. Use it to
         connect a Record Resource or Instantiation with an Agent only if it is not possible to use
         a narrower, more specific relation, for example has creator."""@en ;
    :RiCCMCorrespondingComponent """RiC-R026 ('has provenance'
         relation)"""@en ;
.

:isAgentAssociatedWithPlace
    a owl:ObjectProperty ;
    rdfs:label
        "is agent associated with place"@en ,
        "agente está asociado con lugar"@es ,
        "est un agent associé au lieu"@fr ;
    rdfs:comment """Inverse of 'is place associated with agent' object
         property."""@en ;
    rdfs:domain :Agent ;
    rdfs:isDefinedBy <https://www.ica.org/standards/RiC/ontology> ;
    rdfs:range :Place ;
    rdfs:subPropertyOf :isAssociatedWithPlace ;
    owl:inverseOf :isPlaceAssociatedWithAgent ;
    skos:changeNote
        [
            dc:date "2023-11-27" ;
            rdf:value "Added a new rdfs:label in Spanish."@en ;
        ] ,
        [
            dc:date "2023-10-26" ;
            rdf:value "Added a rdfs:comment."@en ;
        ] ,
        [
            dc:date "2023-10-19" ;
            rdf:value "Added for RiC-O v1.0."@en ;
        ] ;
.

:isInstantiationAssociatedWithInstantiation
    a
        owl:ObjectProperty ,
        owl:SymmetricProperty ;
    rdfs:label
        "is instantiation associated with instantiation"@en ,
        "se asocia con la instanciación"@es ,
        "est associée à l’instanciation"@fr ;
    rdfs:comment """Connects two Instantiations. This relation is
         symmetric."""@en ;
    rdfs:domain :Instantiation ;
    rdfs:isDefinedBy <https://www.ica.org/standards/RiC/ontology> ;
    rdfs:range :Instantiation ;
    rdfs:subPropertyOf :isRelatedTo ;
    owl:propertyChainAxiom (
        :thingIsConnectedToRelation
        :instantiationToInstantiationRelation_role
        :relationConnects
    ) ;
    skos:changeNote
        [
            dc:date "2023-11-12" ;
            rdf:value """Aligned with RiC-CM 1.0: updated the description
               (rdfs:comment), skos:scopeNote."""@en ;
        ] ,
        [
            dc:date "2023-11-08" ;
            rdf:value """In order to get a system of rolified Relation classes: modified
               the property chain axiom so that it now involves the new
               instantiationToInstantiationRelation_role object property."""@en ;
        ] ,
        [
            dc:date "2023-11-02" ;
            rdf:value "Added a new rdfs:label in Spanish."@en ;
        ] ,
        [
            dc:date "2023-08-28" ;
            rdf:value "Added a new rdfs:label in French."@en ;
        ] ;
    skos:scopeNote """Use only if it is not possible to specify a narrower
         Instantiation to Instantiation relation, for example is functionally equivalent
         to."""@en ;
    :RiCCMCorrespondingComponent """RiC-R034 ('is instantiation associated with
         instantiation' relation)"""@en ;
.

:isOrWasCategoryOfAllMembersOf
    a owl:ObjectProperty ;
    rdfs:label
        "is or was category of all members of"@en ,
        "es o era la categoría de todos los miembros de"@es ,
        "est ou a été la catégorie de tous les membres de"@fr ;
    rdfs:comment """Connects a Category (Type) and a Record Set whose all present or
         past Record or Record Part members belong to that Category."""@en ;
    rdfs:domain :Type ;
    rdfs:isDefinedBy <https://www.ica.org/standards/RiC/ontology> ;
    rdfs:range :RecordSet ;
    rdfs:subPropertyOf :isRelatedTo ;
    owl:inverseOf :hasOrHadAllMembersWithCategory ;
    skos:changeNote
        [
            dc:date "2023-08-28" ;
            rdf:value "Added a new rdfs:label in French."@en ;
        ] ,
        [
            dc:date "2023-11-02" ;
            rdf:value "Added a new rdfs:label in Spanish."@en ;
        ] ,
        [
            dc:date "2020-12-28" ;
            rdf:value """Object property added for handling the case where a Record Set
               is described as having all or some members that belong to some category (see RiC-CM
               0.2 attributes section, #4.4 on Record Set, Record and Record Part
               attributes)."""@en ;
        ] ;
.

:isOrWasCategoryOfSomeMembersOf
    a owl:ObjectProperty ;
    rdfs:label
        "is or was category of some members of"@en ,
        "es o era la categoría de algunos miembros de"@es ,
        "est ou a été la catégorie de certains membres de"@fr ;
    rdfs:comment """Connects a Category (Type) and a Record Set whose some present or
         past Record or Record Part members belong to that Category."""@en ;
    rdfs:domain :Type ;
    rdfs:isDefinedBy <https://www.ica.org/standards/RiC/ontology> ;
    rdfs:range :RecordSet ;
    rdfs:subPropertyOf :isRelatedTo ;
    owl:inverseOf :hasOrHadSomeMembersWithCategory ;
    skos:changeNote
        [
            dc:date "2023-11-02" ;
            rdf:value "Added a new rdfs:label in Spanish."@en ;
        ] ,
        [
            dc:date "2023-08-28" ;
            rdf:value "Added a new rdfs:label in French."@en ;
        ] ,
        [
            dc:date "2020-12-28" ;
            rdf:value """Object property added for handling the case where a Record Set
               is described as having all or some members that belong to some category (see RiC-CM
               0.2 attributes section, #4.4 on Record Set, Record and Record Part
               attributes)."""@en ;
        ] ;
.

:isOrWasSubordinateTo
    a owl:ObjectProperty ;
    rdfs:label
        "is or was subordinate to"@en ,
        "está o estaba subordinado(a) a"@es ,
        "est ou a été le subalterne de"@fr ;
    rdfs:comment """Inverse of 'has or had subordinate' object
         property."""@en ;
    rdfs:domain :Agent ;
    rdfs:isDefinedBy <https://www.ica.org/standards/RiC/ontology> ;
    rdfs:range :Agent ;
    rdfs:subPropertyOf :isAgentAssociatedWithAgent ;
    owl:inverseOf :hasOrHadSubordinate ;
    owl:propertyChainAxiom (
        :thingIsTargetOfRelation
        :agentHierarchicalRelation_role
        :relationHasSource
    ) ;
    skos:changeNote
        [
            dc:date "2023-11-02" ;
            rdf:value "Added a new rdfs:label in Spanish."@en ;
        ] ,
        [
            dc:date "2023-08-28" ;
            rdf:value "Added a new rdfs:label in French."@en ;
        ] ,
        [
            dc:date "2021-01-22" ;
            rdf:value """changed the IRI, label, inverse property IRI (changed made in
               order to make RiC-O compliant with RiC-CM 0.2; the name of this property in RiC-O 0.1
               was "isHierarchicallyInferiorTo")."""@en ;
        ] ,
        [
            dc:date "2023-11-08" ;
            rdf:value """In order to get a system of rolified Relation classes: modified
               the property chain axiom so that it now involves the new
               agentHierarchicalRelation_role object property."""@en ;
        ] ;
    :RiCCMCorrespondingComponent """RiC-R045i ('is or was subordinate to'
         relation)"""@en ;
.

:isOrWasUnderAuthorityOf
    a owl:ObjectProperty ;
    rdfs:label
        "is or was under authority of"@en ,
        "está o estaba bajo control de"@es ,
        "est ou a été sous l’autorité de"@fr ;
    rdfs:comment """Inverse of 'has or had authority over' object
         property."""@en ;
    rdfs:domain :Thing ;
    rdfs:isDefinedBy <https://www.ica.org/standards/RiC/ontology> ;
    rdfs:range :Agent ;
    rdfs:subPropertyOf :isRelatedTo ;
    owl:inverseOf :hasOrHadAuthorityOver ;
    owl:propertyChainAxiom (
        :thingIsTargetOfRelation
        :authorityRelation_role
        :relationHasSource
    ) ;
    skos:changeNote
        [
            dc:date "2023-11-02" ;
            rdf:value "Added a new rdfs:label in Spanish."@en ;
        ] ,
        [
            dc:date "2023-08-28" ;
            rdf:value "Added a new rdfs:label in French."@en ;
        ] ,
        [
            dc:date "2023-11-08" ;
            rdf:value """In order to get a system of rolified Relation classes: modified
               the property chain axiom so that it now involves the new authorityRelation_role
               object property."""@en ;
        ] ,
        [
            dc:date "2021-01-22" ;
            rdf:value """changed the IRI, label, inverse property IRI, text definition
               (changed made in order to make RiC-O compliant with RiC-CM 0.2; the name of this
               property in RiC-O 0.1 was "isUnderAuthorityOf")."""@en ;
        ] ;
    :RiCCMCorrespondingComponent """RiC-R036i ('is or was under authority of'
         relation)"""@en ;
.

:isOrganicProvenanceOf
    a owl:ObjectProperty ;
    rdfs:label
        "is organic provenance of"@en ,
        "es procedencia orgánica de"@es ,
        "est la provenance organique de"@fr ;
    rdfs:comment """Inverse of 'has organic provenance' object
         property."""@en ;
    rdfs:domain :Agent ;
    rdfs:isDefinedBy <https://www.ica.org/standards/RiC/ontology> ;
    rdfs:range
        [
            a owl:Class ;
            owl:unionOf (
                :Instantiation
                :RecordResource
            ) ;
        ] ;
    rdfs:subPropertyOf :isOrganicOrFunctionalProvenanceOf ;
    owl:inverseOf :hasOrganicProvenance ;
    owl:propertyChainAxiom (
        :thingIsTargetOfRelation
        :organicProvenanceRelation_role
        :relationHasSource
    ) ;
    skos:changeNote
        [
            dc:date "2023-11-02" ;
            rdf:value "Added a new rdfs:label in Spanish."@en ;
        ] ,
        [
            dc:date "2024-03-15" ;
            rdf:value "Make capitalisation of rdfs:comment consistent."@en ;
        ] ,
        [
            dc:date "2023-08-28" ;
            rdf:value "Added a new rdfs:label in French."@en ;
        ] ,
        [
            dc:date "2023-11-07" ;
            rdf:value """Made this property a subproperty of the new
               isOrganicOrFunctionalProvenanceOf property. Renamed it to make things clearer.
               Adjusted its labels."""@en ;
        ] ,
        [
            dc:date "2023-11-08" ;
            rdf:value """In order to get a system of rolified Relation classes: modified
               the property chain axiom so that it now involves the new
               organicProvenanceRelation_role object property."""@en ;
        ] ;
    :RiCCMCorrespondingComponent """RiC-R026i ('is provenance of'
         relation)"""@en ;
.

:isPlaceAssociatedWithAgent
    a owl:ObjectProperty ;
    rdfs:label
        "is place associated with agent"@en ,
        "es lugar asociado con agente"@es ,
        "est un lieu associé à l'agent"@fr ;
    rdfs:comment """Connects a Place to an Agent which is related to that
         Place."""@en ;
    rdfs:domain :Place ;
    rdfs:isDefinedBy <https://www.ica.org/standards/RiC/ontology> ;
    rdfs:range :Agent ;
    rdfs:subPropertyOf :isPlaceAssociatedWith ;
    owl:inverseOf :isAgentAssociatedWithPlace ;
    skos:changeNote
        [
            dc:date "2023-11-27" ;
            rdf:value "Added a new rdfs:label in Spanish."@en ;
        ] ,
        [
            dc:date "2023-10-19" ;
            rdf:value "Added for RiC-O v1.0."@en ;
        ] ,
        [
            dc:date "2023-10-26" ;
            rdf:value """fixed the domain and range, added a rdfs:comment and English
               and French labels."""@en ;
        ] ;
.

:organicOrFunctionalProvenanceRelation_role
    a
        owl:ObjectProperty ,
        owl:ReflexiveProperty ;
    rdfs:label
        """has the role of the Organic or functional provenance
         Relation"""@en ,
        """desempeña el papel de la Relación de procedencia orgánica or
         funcional"""@es ,
        """a le rôle de la Relation de provenance organique ou
         fonctionnelle"""@fr ;
    rdfs:comment """Connects a OrganicOrFunctionalProvenanceRelation to itself. It is
         a reflexive property, that can stand for an instance of the class when necessary, e.g. when
         you explore a knowledge graph."""@en ;
    rdfs:domain :OrganicOrFunctionalProvenanceRelation ;
    rdfs:isDefinedBy <https://www.ica.org/standards/RiC/ontology> ;
    rdfs:range :OrganicOrFunctionalProvenanceRelation ;
    rdfs:subPropertyOf :relation_role ;
    skos:changeNote
        [
            dc:date "2023-11-08" ;
            rdf:value """In order to get a system of rolified Relation classes: created
               the object property, with domain and range the OrganicOrFunctionalProvenanceRelation
               rolified class. Declared it as reflexive. Declared it(s)
               superproperty(ies)."""@en ;
        ] ;
    skos:scopeNote """This property "rolifies" the
         OrganicOrFunctionalProvenanceRelation class. It should be used only when you have to manage
         instances of the OrganicOrFunctionalProvenanceRelation class, to connect each instance to
         itself, in order to be able to infer, using OWL-RL and property paths, the two shortcuts
         corresponding to this n-ary class."""@en ;
.

:organicProvenanceRelation_role
    a
        owl:ObjectProperty ,
        owl:ReflexiveProperty ;
    rdfs:label
        "has the role of the Organic Provenance Relation"@en ,
        """desempeña el papel de la Relación de procedencia
         orgánica"""@es ,
        "a le rôle de la Relation de provenance organique"@fr ;
    rdfs:comment """Connects a OrganicProvenanceRelation to itself. It is a reflexive
         property, that can stand for an instance of the class when necessary, e.g. when you explore
         a knowledge graph."""@en ;
    rdfs:domain :OrganicProvenanceRelation ;
    rdfs:isDefinedBy <https://www.ica.org/standards/RiC/ontology> ;
    rdfs:range :OrganicProvenanceRelation ;
    rdfs:subPropertyOf :organicOrFunctionalProvenanceRelation_role ;
    skos:changeNote
        [
            dc:date "2023-11-08" ;
            rdf:value """In order to get a system of rolified Relation classes: created
               the object property, with domain and range the OrganicProvenanceRelation rolified
               class. Declared it as reflexive. Declared it(s) superproperty(ies)."""@en ;
        ] ;
    skos:scopeNote """This property "rolifies" the OrganicProvenanceRelation class. It
         should be used only when you have to manage instances of the OrganicProvenanceRelation
         class, to connect each instance to itself, in order to be able to infer, using OWL-RL and
         property paths, the two shortcuts corresponding to this n-ary class."""@en ;
.

:temporalRelation_role
    a
        owl:ObjectProperty ,
        owl:ReflexiveProperty ;
    rdfs:label
        "has the role of the Temporal Relation"@en ,
        "desempeña el papel de la Relación temporal"@es ,
        "a le rôle de la Relation temporelle"@fr ;
    rdfs:comment """Connects a TemporalRelation to itself. It is a reflexive property,
         that can stand for an instance of the class when necessary, e.g. when you explore a
         knowledge graph."""@en ;
    rdfs:domain :TemporalRelation ;
    rdfs:isDefinedBy <https://www.ica.org/standards/RiC/ontology> ;
    rdfs:range :TemporalRelation ;
    rdfs:subPropertyOf :sequentialRelation_role ;
    skos:changeNote
        [
            dc:date "2023-11-08" ;
            rdf:value """In order to get a system of rolified Relation classes: created
               the object property, with domain and range the TemporalRelation rolified class.
               Declared it as reflexive. Declared it(s) superproperty(ies)."""@en ;
        ] ;
    skos:scopeNote """This property "rolifies" the TemporalRelation class. It should
         be used only when you have to manage instances of the TemporalRelation class, to connect
         each instance to itself, in order to be able to infer, using OWL-RL and property paths, the
         two shortcuts corresponding to this n-ary class."""@en ;
.

skos:Concept
    a owl:Class ;
    rdfs:isDefinedBy <http://www.w3.org/2004/02/skos/core> ;
.

:AuthorityRelation
    a owl:Class ;
    rdfs:label
        "Authority Relation"@en ,
        "Relación de control por parte de agentes"@es ,
        "Relation d’autorité"@fr ;
    rdfs:comment """Connects at least one Agent and at least one Thing over which the
         Agent has or had some authority. The Agent(s) is the source of the relation, and the
         Thing(s) is the target."""@en ;
    rdfs:isDefinedBy <https://www.ica.org/standards/RiC/ontology> ;
    rdfs:subClassOf
        [
            a owl:Restriction ;
            owl:minQualifiedCardinality "1"^^xsd:nonNegativeInteger ;
            owl:onClass :Agent ;
            owl:onProperty :relationHasSource ;
        ] ,
        [
            a owl:Restriction ;
            owl:minQualifiedCardinality "1"^^xsd:nonNegativeInteger ;
            owl:onClass :Thing ;
            owl:onProperty :relationHasTarget ;
        ] ,
        :Relation ;
    owl:equivalentClass
        [
            a owl:Restriction ;
            owl:hasSelf true ;
            owl:onProperty :authorityRelation_role ;
        ] ;
    skos:changeNote
        [
            dc:date "2023-11-12" ;
            rdf:value """Aligned with RiC-CM 1.0: updated the description
               (rdfs:comment), skos:scopeNote."""@en ;
        ] ,
        [
            dc:date "2023-12-06" ;
            rdf:value """Improved the description of the Relation class (rdfs:comment)
               by clearly specifying how it is directed."""@en ;
        ] ,
        [
            dc:date "2023-11-02" ;
            rdf:value "Added a new rdfs:label in Spanish."@en ;
        ] ,
        [
            dc:date "2023-11-08" ;
            rdf:value """In order to get a system of rolified Relation classes: added an
               equivalentClass object property; replaced the specific object properties by the
               generic ones in the subClassOf declarations."""@en ;
        ] ,
        [
            dc:date "2023-08-25" ;
            rdf:value "Added a new rdfs:label in French."@en ;
        ] ;
    skos:scopeNote """Use only if it is not possible to specify a narrower authority
         relation, for example OwnershipRelation."""@en ;
    :RiCCMCorrespondingComponent """Class implementation of RiC-R036 and RiC-R036i
         relations"""@en ;
.

:ContentType
    a owl:Class ;
    rdfs:label
        "Content Type"@en ,
        "Tipo de contenido"@es ,
        "Type de contenu"@fr ;
    rdfs:comment """The fundamental form of communication in which a Record or Record
         Part is expressed."""@en ;
    rdfs:isDefinedBy <https://www.ica.org/standards/RiC/ontology> ;
    rdfs:subClassOf :Type ;
    skos:changeNote
        [
            dc:date "2023-11-12" ;
            rdf:value """Aligned with RiC-CM 1.0: updated the description
               (rdfs:comment), skos:scopeNote."""@en ;
        ] ,
        [
            dc:date "2023-04-19" ;
            rdf:value "Removed the 0.2 existing unnecessary restriction."@en ;
        ] ,
        [
            dc:date "2020-10-23" ;
            rdf:value """Scope note: added (quite the same as RiC-CM
               definition)."""@en ;
        ] ,
        [
            dc:date "2023-11-02" ;
            rdf:value "Added a new rdfs:label in Spanish."@en ;
        ] ,
        [
            dc:date "2023-08-25" ;
            rdf:value "Added a new rdfs:label in French."@en ;
        ] ;
    skos:scopeNote """Content Type should not be confused with Representation Type or
         Carrier Type that would concern a related Instantiation since the form of communication can
         be independent of the representation or carrier, for example a map (content type
         "cartographic image") may be represented as a sketch (representation type "visual")
         recorded as a physical document (carrier type "paper"). It also should not be confused with
         the Documentary Form Type of a Record, or Record Part, which describes a specific document
         form (for example a deed of sale)."""@en ;
    :RiCCMCorrespondingComponent """Corresponds to RiC-A10 (Content Type
         attribute)"""@en ;
.

:Language
    a owl:Class ;
    rdfs:label
        "Language"@en ,
        "Lengua"@es ,
        "Langue"@fr ;
    rdfs:comment """A spoken or written human language represented in a Record
         Resource or used by an Agent."""@en ;
    rdfs:isDefinedBy <https://www.ica.org/standards/RiC/ontology> ;
    rdfs:subClassOf :Concept ;
    skos:changeNote
        [
            dc:date "2023-08-25" ;
            rdf:value "Added a new rdfs:label in French."@en ;
        ] ,
        [
            dc:date "2020-10-23" ;
            rdf:value "Scope note from RiC-CM : deleted."@en ;
        ] ,
        [
            dc:date "2020-12-28" ;
            rdf:value """Changed the definition (skos:comment annotation); so that it
               conforms to the RiC-CM one."""@en ;
        ] ,
        [
            dc:date "2023-11-12" ;
            rdf:value """Aligned with RiC-CM 1.0: updated the description
               (rdfs:comment)."""@en ;
        ] ,
        [
            dc:date "2023-11-02" ;
            rdf:value "Added a new rdfs:label in Spanish."@en ;
        ] ;
    :RiCCMCorrespondingComponent """Corresponds to RiC-A25 (Language
         attribute)"""@en ;
.

:LegalStatus
    a owl:Class ;
    rdfs:label
        "Legal Status"@en ,
        "Status jurídico"@es ,
        "Statut légal"@fr ;
    rdfs:comment "A status defined by law."@en ;
    rdfs:isDefinedBy <https://www.ica.org/standards/RiC/ontology> ;
    rdfs:subClassOf :Type ;
    skos:changeNote
        [
            dc:date "2023-08-25" ;
            rdf:value "Added a new rdfs:label in French."@en ;
        ] ,
        [
            dc:date "2023-11-02" ;
            rdf:value "Added a new rdfs:label in Spanish."@en ;
        ] ;
    :RiCCMCorrespondingComponent """Corresponds to RiC-A26 (Legal Status
         attribute)"""@en ;
.

:MandateRelation
    a owl:Class ;
    rdfs:label
        "Mandate Relation"@en ,
        "Relación normativa"@es ,
        "Relation impliquant un mandat"@fr ;
    rdfs:comment """Connects at least one Mandate and at least one Agent, when the
         first gives or gave the second one the authority or competencies to act. May also involve
         one to many Activities that the Mandate(s) assign(s) or assigned to the Agent(s). The
         Mandate(s) is the source of the Relation and the Agent(s) is the target."""@en ;
    rdfs:isDefinedBy <https://www.ica.org/standards/RiC/ontology> ;
    rdfs:subClassOf
        [
            a owl:Restriction ;
            owl:minQualifiedCardinality "1"^^xsd:nonNegativeInteger ;
            owl:onClass :Activity ;
            owl:onProperty :asConcernsActivity ;
        ] ,
        [
            a owl:Restriction ;
            owl:minQualifiedCardinality "1"^^xsd:nonNegativeInteger ;
            owl:onClass :Agent ;
            owl:onProperty :relationHasTarget ;
        ] ,
        [
            a owl:Restriction ;
            owl:minQualifiedCardinality "1"^^xsd:nonNegativeInteger ;
            owl:onClass :Mandate ;
            owl:onProperty :relationHasSource ;
        ] ,
        :RuleRelation ;
    owl:equivalentClass
        [
            a owl:Restriction ;
            owl:hasSelf true ;
            owl:onProperty :mandateRelation_role ;
        ] ;
    skos:changeNote
        [
            dc:date "2023-12-06" ;
            rdf:value """Improved the description of the Relation class (rdfs:comment)
               by clearly specifying how it is directed."""@en ;
        ] ,
        [
            dc:date "2023-04-19" ;
            rdf:value "Removed a 0.2 existing unnecessary restriction."@en ;
        ] ,
        [
            dc:date "2023-08-25" ;
            rdf:value "Added a new rdfs:label in French."@en ;
        ] ,
        [
            dc:date "2023-11-02" ;
            rdf:value "Added a new rdfs:label in Spanish."@en ;
        ] ,
        [
            dc:date "2023-11-08" ;
            rdf:value """In order to get a system of rolified Relation classes: added an
               equivalentClass object property; replaced the specific object properties by the
               generic ones in the subClassOf declarations."""@en ;
        ] ,
        [
            dc:date "2023-11-12" ;
            rdf:value """Aligned with RiC-CM 1.0: updated the description
               (rdfs:comment)."""@en ;
        ] ;
    :RiCCMCorrespondingComponent """Class implementation of RiC-R067 and RiC-R067i
         relations"""@en ;
.

:RecordSetType
    a owl:Class ;
    rdfs:label
        "Record Set Type"@en ,
        "Tipo de agrupación documental"@es ,
        "Type d’ensemble d’objets informationnels"@fr ;
    rdfs:comment "A broad categorization of the type of Record Set."@en ;
    rdfs:isDefinedBy <https://www.ica.org/standards/RiC/ontology> ;
    rdfs:subClassOf :Type ;
    skos:changeNote
        [
            dc:date "2023-11-02" ;
            rdf:value "Added a new rdfs:label in Spanish."@en ;
        ] ,
        [
            dc:date "2020-10-23" ;
            rdf:value """scope note: updated. Objective: to make RiC-O compliant with
               RiC-CM v0.2."""@en ;
        ] ,
        [
            dc:date "2023-08-25" ;
            rdf:value "Added a new rdfs:label in French."@en ;
        ] ,
        [
            dc:date "2023-04-19" ;
            rdf:value "Removed the 0.2 existing unnecessary restriction."@en ;
        ] ,
        [
            dc:date "2023-11-12" ;
            rdf:value """Aligned with RiC-CM 1.0: updated the
               skos:scopeNote."""@en ;
        ] ;
    skos:scopeNote """Four instances of Record Set Type are included for now in RiC-O;
         they also are instances of skos:Concept and, as such, part of a SKOS vocabulary. Record Set
         Type may also be used (or extended) to categorize types of Record Set that have not
         traditionally been considered archival, e.g. search result list."""@en ;
    :RiCCMCorrespondingComponent """Corresponds to RiC-A36 (Record Set Type
         attribute)"""@en ;
.

:RecordState
    a owl:Class ;
    rdfs:label
        "Record State"@en ,
        "Estado de documento"@es ,
        "État d’un objet informationnel"@fr ;
    rdfs:comment """Description of the production or reproduction status of a Record
         or Record Part."""@en ;
    rdfs:isDefinedBy <https://www.ica.org/standards/RiC/ontology> ;
    rdfs:subClassOf :Type ;
    skos:changeNote
        [
            dc:date "2020-12-28" ;
            rdf:value """IRI and label changed (RecordResourceState to RecordState), as
               well as textual definition."""@en ;
        ] ,
        [
            dc:date "2020-10-23" ;
            rdf:value """scope note: updated. Objective: to make RiC-O compliant with
               RiC-CM v0.2."""@en ;
        ] ,
        [
            dc:date "2023-11-12" ;
            rdf:value """Aligned with RiC-CM 1.0: updated the description
               (rdfs:comment), skos:scopeNote."""@en ;
        ] ,
        [
            dc:date "2023-11-02" ;
            rdf:value "Added a new rdfs:label in Spanish."@en ;
        ] ,
        [
            dc:date "2023-08-25" ;
            rdf:value "Added a new rdfs:label in French."@en ;
        ] ;
    skos:scopeNote """Can refer both to a record's stage of creation (for example
         "draft") and its form of transmission when the record was received (for example
         "copy")."""@en ;
    :RiCCMCorrespondingComponent """Corresponds to RiC-A39 (State
         attribute)"""@en ;
.

:hasBeginningDate
    a owl:ObjectProperty ;
    rdfs:label
        "has beginning date"@en ,
        "tiene como fecha de inicio"@es ,
        "a pour date de début"@fr ;
    rdfs:comment "Inverse of 'is beginning date of' object property"@en ;
    rdfs:domain :Thing ;
    rdfs:isDefinedBy <https://www.ica.org/standards/RiC/ontology> ;
    rdfs:range :Date ;
    rdfs:subPropertyOf :isAssociatedWithDate ;
    owl:inverseOf :isBeginningDateOf ;
    skos:changeNote
        [
            dc:date "2023-08-28" ;
            rdf:value "Added a new rdfs:label in French."@en ;
        ] ,
        [
            dc:date "2023-11-02" ;
            rdf:value "Added a new rdfs:label in Spanish."@en ;
        ] ;
    :RiCCMCorrespondingComponent """RiC-R069i ('has beginning date'
         relation)"""@en ;
.

:hasGeneticLinkToRecordResource
    a
        owl:ObjectProperty ,
        owl:SymmetricProperty ;
    rdfs:label
        "has genetic link to record resource"@en ,
        "tiene vínculo de origen con recurso documental"@es ,
        """a une relation génétique avec la ressource
         archivistique"""@fr ;
    rdfs:comment """Connects two Record Resources when there is a genetic link between
         them. Genetic in this sense is as defined by diplomatics, i.e. the process by which a
         Record Resource is developed. This relation is symmetric."""@en ;
    rdfs:domain :RecordResource ;
    rdfs:isDefinedBy <https://www.ica.org/standards/RiC/ontology> ;
    rdfs:range :RecordResource ;
    rdfs:subPropertyOf :isRecordResourceAssociatedWithRecordResource ;
    owl:propertyChainAxiom (
        :thingIsConnectedToRelation
        :recordResourceGeneticRelation_role
        :relationConnects
    ) ;
    skos:changeNote
        [
            dc:date "2023-11-02" ;
            rdf:value "Added a new rdfs:label in Spanish."@en ;
        ] ,
        [
            dc:date "2023-08-28" ;
            rdf:value "Added a new rdfs:label in French."@en ;
        ] ,
        [
            dc:date "2023-11-12" ;
            rdf:value """Aligned with RiC-CM 1.0: updated the
               skos:scopeNote."""@en ;
        ] ,
        [
            dc:date "2023-11-08" ;
            rdf:value """In order to get a system of rolified Relation classes: modified
               the property chain axiom so that it now involves the new
               recordResourceGeneticRelation_role object property."""@en ;
        ] ,
        [
            dc:date "2023-11-07" ;
            rdf:value """Added the property chain axiom so that this property is
               formally defined as a shortcut."""@en ;
        ] ;
    skos:scopeNote """Use to connect two Record Resources only if it is not possible
         to use a narrower, more specific, asymmetric Record Resource to Record Resource relation,
         for example is original of."""@en ;
    :RiCCMCorrespondingComponent """RiC-R023 ('has genetic link to record resource'
         relation)"""@en ;
.

:isAssociatedWithEvent
    a owl:ObjectProperty ;
    rdfs:label
        "is associated with event"@en ,
        "está asociado con evento"@es ,
        "est associé à l’événement"@fr ;
    rdfs:comment """Inverse of 'is event associated with' object
         property."""@en ;
    rdfs:domain :Thing ;
    rdfs:isDefinedBy <https://www.ica.org/standards/RiC/ontology> ;
    rdfs:range :Event ;
    rdfs:subPropertyOf :isRelatedTo ;
    owl:inverseOf :isEventAssociatedWith ;
    owl:propertyChainAxiom (
        :thingIsTargetOfRelation
        :eventRelation_role
        :relationHasSource
    ) ;
    skos:changeNote
        [
            dc:date "2023-08-28" ;
            rdf:value "Added a new rdfs:label in French."@en ;
        ] ,
        [
            dc:date "2023-11-02" ;
            rdf:value "Added a new rdfs:label in Spanish."@en ;
        ] ,
        [
            dc:date "2023-11-08" ;
            rdf:value """In order to get a system of rolified Relation classes: modified
               the property chain axiom so that it now involves the new eventRelation_role object
               property."""@en ;
        ] ;
    :RiCCMCorrespondingComponent """RiC-R057i ('is associated with event'
         relation)"""@en ;
.

:isAssociatedWithRule
    a owl:ObjectProperty ;
    rdfs:label
        "is associated with rule"@en ,
        "está asociado con regla"@es ,
        "est associé à la règle"@fr ;
    rdfs:comment """Inverse of 'is rule associated with' object
         property."""@en ;
    rdfs:domain :Thing ;
    rdfs:isDefinedBy <https://www.ica.org/standards/RiC/ontology> ;
    rdfs:range :Rule ;
    rdfs:subPropertyOf :isRelatedTo ;
    owl:inverseOf :isRuleAssociatedWith ;
    owl:propertyChainAxiom (
        :thingIsTargetOfRelation
        :ruleRelation_role
        :relationHasSource
    ) ;
    skos:changeNote
        [
            dc:date "2023-08-28" ;
            rdf:value "Added a new rdfs:label in French."@en ;
        ] ,
        [
            dc:date "2023-11-02" ;
            rdf:value "Added a new rdfs:label in Spanish."@en ;
        ] ,
        [
            dc:date "2023-11-08" ;
            rdf:value """In order to get a system of rolified Relation classes: modified
               the property chain axiom so that it now involves the new ruleRelation_role object
               property."""@en ;
        ] ;
    :RiCCMCorrespondingComponent """RiC-R062i ('is associated with rule'
         relation)"""@en ;
.

:isEventAssociatedWith
    a owl:ObjectProperty ;
    rdfs:label
        "is event associated with"@en ,
        "es evento asociado con"@es ,
        "est un événement associé a"@fr ;
    rdfs:comment """Connects an Event to a Thing that is associated with the existence
         and lifecycle of the Event."""@en ;
    rdfs:domain :Event ;
    rdfs:isDefinedBy <https://www.ica.org/standards/RiC/ontology> ;
    rdfs:range :Thing ;
    rdfs:subPropertyOf :isRelatedTo ;
    owl:inverseOf :isAssociatedWithEvent ;
    owl:propertyChainAxiom (
        :thingIsSourceOfRelation
        :eventRelation_role
        :relationHasTarget
    ) ;
    skos:changeNote
        [
            dc:date "2023-11-02" ;
            rdf:value "Added a new rdfs:label in Spanish."@en ;
        ] ,
        [
            dc:date "2023-08-28" ;
            rdf:value "Added a new rdfs:label in French."@en ;
        ] ,
        [
            dc:date "2023-11-08" ;
            rdf:value """In order to get a system of rolified Relation classes: modified
               the property chain axiom so that it now involves the new eventRelation_role object
               property."""@en ;
        ] ,
        [
            dc:date "2023-11-12" ;
            rdf:value """Aligned with RiC-CM 1.0: updated the
               skos:scopeNote."""@en ;
        ] ;
    skos:scopeNote """Use to connect an Event and an entity only if it is not possible
         to specify a narrower Event relation, for example has or had participant."""@en ;
    :RiCCMCorrespondingComponent """RiC-R057 ('is event associated with'
         relation)"""@en ;
.

:isRuleAssociatedWith
    a owl:ObjectProperty ;
    rdfs:label
        "is rule associated with"@en ,
        "es regla asociada con"@es ,
        "est une règle associée à"@fr ;
    rdfs:comment """Connects a Rule to a Thing that is associated with the
         Rule."""@en ;
    rdfs:domain :Rule ;
    rdfs:isDefinedBy <https://www.ica.org/standards/RiC/ontology> ;
    rdfs:range :Thing ;
    rdfs:subPropertyOf :isRelatedTo ;
    owl:inverseOf :isAssociatedWithRule ;
    owl:propertyChainAxiom (
        :thingIsSourceOfRelation
        :ruleRelation_role
        :relationHasTarget
    ) ;
    skos:changeNote
        [
            dc:date "2023-11-12" ;
            rdf:value """Aligned with RiC-CM 1.0: updated the description
               (rdfs:comment), skos:scopeNote."""@en ;
        ] ,
        [
            dc:date "2023-11-08" ;
            rdf:value """In order to get a system of rolified Relation classes: modified
               the property chain axiom so that it now involves the new ruleRelation_role object
               property."""@en ;
        ] ,
        [
            dc:date "2023-08-28" ;
            rdf:value "Added a new rdfs:label in French."@en ;
        ] ,
        [
            dc:date "2023-11-02" ;
            rdf:value "Added a new rdfs:label in Spanish."@en ;
        ] ;
    skos:scopeNote """Use only if it is not possible to specify a narrower Rule
         relation, for example, regulates or regulated."""@en ;
    :RiCCMCorrespondingComponent """RiC-R062 ('is rule associated with'
         relation)"""@en ;
.

:measure
    a owl:DatatypeProperty ;
    rdfs:label
        "measure"@en ,
        "medida"@es ,
        "mesure"@fr ;
    rdfs:comment """The extent, quantity, amount, or degree of an entity, as
         determined by measurement or calculation."""@en ;
    rdfs:domain :Thing ;
    rdfs:isDefinedBy <https://www.ica.org/standards/RiC/ontology> ;
    rdfs:range rdfs:Literal ;
    skos:changeNote
        [
            dc:date "2023-08-25" ;
            rdf:value "Added a new rdfs:label in French."@en ;
        ] ,
        [
            dc:date "2023-11-02" ;
            rdf:value "Added a new rdfs:label in Spanish."@en ;
        ] ;
.

:relationHasContext
    a owl:ObjectProperty ;
    rdfs:label
        "relation has context"@en ,
        "relación tiene como contexto"@es ,
        "relation a pour contexte"@fr ;
    rdfs:comment """Connects an n-ary Relation to a Thing that is a secondary,
         contextual entity during the existence of the Relation."""@en ;
    rdfs:domain :Relation ;
    rdfs:isDefinedBy <https://www.ica.org/standards/RiC/ontology> ;
    rdfs:range :Thing ;
    rdfs:subPropertyOf :relationConnects ;
    owl:inverseOf :thingIsContextOfRelation ;
    skos:changeNote
        [
            dc:date "2023-11-02" ;
            rdf:value "Added a new rdfs:label in Spanish."@en ;
        ] ,
        [
            dc:date "2023-08-28" ;
            rdf:value "Added a new rdfs:label in French."@en ;
        ] ;
    skos:scopeNote """The secondary entity may be, for instance, a Position or a Role
         Type."""@en ;
.

:thingIsContextOfRelation
    a owl:ObjectProperty ;
    rdfs:label
        "thing is context of relation"@en ,
        "cosa es contexto de relación"@es ,
        "chose est le contexte de la relation"@fr ;
    rdfs:comment """Connects a Thing (that is a secondary, contextual entity during
         the existence of the Relation) to a n-ary Relation."""@en ;
    rdfs:domain :Thing ;
    rdfs:isDefinedBy <https://www.ica.org/standards/RiC/ontology> ;
    rdfs:range :Relation ;
    rdfs:subPropertyOf :thingIsConnectedToRelation ;
    owl:inverseOf :relationHasContext ;
    skos:changeNote
        [
            dc:date "2023-11-12" ;
            rdf:value "Updated the labels."@en ;
        ] ,
        [
            dc:date "2023-11-02" ;
            rdf:value "Added a new rdfs:label in Spanish."@en ;
        ] ;
.

:Coordinates
    a owl:Class ;
    rdfs:label
        "Coordinates"@en ,
        "Coordenadas de lugar"@es ,
        "Coordonnées géographiques"@fr ;
    rdfs:comment """Longitudinal and latitudinal information about a
         Place."""@en ;
    rdfs:isDefinedBy <https://www.ica.org/standards/RiC/ontology> ;
    rdfs:subClassOf :Thing ;
    skos:changeNote
        [
            dc:date "2023-08-25" ;
            rdf:value "Added a new rdfs:label in French."@en ;
        ] ,
        [
            dc:date "2023-11-12" ;
            rdf:value """Aligned with RiC-CM 1.0: updated the description
               (rdfs:comment)."""@en ;
        ] ,
        [
            dc:date "2021-02-08"@en ;
            rdf:value """Removed the cardinality Restrictions when the range is a
               datatype property"""@en ;
        ] ,
        [
            dc:date "2023-11-02" ;
            rdf:value "Added a new rdfs:label in Spanish."@en ;
        ] ,
        [
            dc:date "2023-04-19" ;
            rdf:value "Removed the 0.2 existing unnecessary restriction."@en ;
        ] ;
    :RiCCMCorrespondingComponent """Class implementation of RiC-A11 (Coordinates
         attribute)"""@en ;
.

:authorityRelation_role
    a
        owl:ObjectProperty ,
        owl:ReflexiveProperty ;
    rdfs:label
        "has the role of the Authority Relation"@en ,
        """desempeña el papel de la Relación de control por parte de
         agentes"""@es ,
        "a le rôle de la Relation d’autorité"@fr ;
    rdfs:comment """Connects a AuthorityRelation to itself. It is a reflexive
         property, that can stand for an instance of the class when necessary, e.g. when you explore
         a knowledge graph."""@en ;
    rdfs:domain :AuthorityRelation ;
    rdfs:isDefinedBy <https://www.ica.org/standards/RiC/ontology> ;
    rdfs:range :AuthorityRelation ;
    rdfs:subPropertyOf :relation_role ;
    skos:changeNote
        [
            dc:date "2023-11-08" ;
            rdf:value """In order to get a system of rolified Relation classes: created
               the object property, with domain and range the AuthorityRelation rolified class.
               Declared it as reflexive. Declared it(s) superproperty(ies)."""@en ;
        ] ;
    skos:scopeNote """This property "rolifies" the AuthorityRelation class. It should
         be used only when you have to manage instances of the AuthorityRelation class, to connect
         each instance to itself, in order to be able to infer, using OWL-RL and property paths, the
         two shortcuts corresponding to this n-ary class."""@en ;
.

:followsInTime
    a
        owl:ObjectProperty ,
        owl:TransitiveProperty ;
    rdfs:label
        "follows in time"@en ,
        "sigue en el tiempo a"@es ,
        "suit dans le temps"@fr ;
    rdfs:comment """Inverse of 'precedes in time' object property. This is a
         transitive relation."""@en ;
    rdfs:domain :Thing ;
    rdfs:isDefinedBy <https://www.ica.org/standards/RiC/ontology> ;
    rdfs:range :Thing ;
    rdfs:subPropertyOf :followsOrFollowed ;
    owl:inverseOf :precedesInTime ;
    owl:propertyChainAxiom (
        :thingIsTargetOfRelation
        :temporalRelation_role
        :relationHasSource
    ) ;
    skos:changeNote
        [
            dc:date "2023-09-22" ;
            rdf:value "Property made transitive."@en ;
        ] ,
        [
            dc:date "2023-11-08" ;
            rdf:value """In order to get a system of rolified Relation classes: modified
               the property chain axiom so that it now involves the new temporalRelation_role object
               property."""@en ;
        ] ,
        [
            dc:date "2023-11-02" ;
            rdf:value "Added a new rdfs:label in Spanish."@en ;
        ] ,
        [
            dc:date "2021-01-22" ;
            rdf:value "changed the superproperty IRI."@en ;
        ] ,
        [
            dc:date "2023-08-28" ;
            rdf:value "Added a new rdfs:label in French."@en ;
        ] ;
    :RiCCMCorrespondingComponent """RiC-R009i ('follows in time'
         relation)"""@en ;
.

:hadPart
    a owl:ObjectProperty ;
    rdfs:label
        "had part"@en ,
        "tenía como parte"@es ,
        "a eu pour partie"@fr ;
    rdfs:comment """Connects a Thing to a Thing that was a constitutive or component
         part of that Thing in the past."""@en ;
    rdfs:domain :Thing ;
    rdfs:isDefinedBy <https://www.ica.org/standards/RiC/ontology> ;
    rdfs:range :Thing ;
    rdfs:subPropertyOf :hasOrHadPart ;
    owl:inverseOf :wasPartOf ;
    skos:changeNote
        [
            dc:date "2023-11-12" ;
            rdf:value "Updated the labels."@en ;
        ] ,
        [
            dc:date "2023-07-12" ;
            rdf:value """Object property added, along with its inverse property, in
               order to enable to express past partitive relations between things (the current
               partitive relations being also added, including a transitive one)."""@en ;
        ] ,
        [
            dc:date "2023-11-27" ;
            rdf:value "Added a new rdfs:label in Spanish."@en ;
        ] ;
.

:hasDirectPart
    a owl:ObjectProperty ;
    rdfs:label
        "has direct part"@en ,
        "tiene directamente como parte"@es ,
        "a directement pour partie"@fr ;
    rdfs:comment """Connects a Thing to a Thing that is a direct constitutive or
         component part of that Thing."""@en ;
    rdfs:domain :Thing ;
    rdfs:isDefinedBy <https://www.ica.org/standards/RiC/ontology> ;
    rdfs:range :Thing ;
    rdfs:subPropertyOf :hasPartTransitive ;
    owl:inverseOf :isDirectPartOf ;
    skos:changeNote
        [
            dc:date "2023-11-27" ;
            rdf:value "Added a new rdfs:label in Spanish."@en ;
        ] ,
        [
            dc:date "2023-07-12" ;
            rdf:value """Object property added, along with its inverse property, in
               order to enable to express current, direct, partitive relations between things (the
               possibly indirect, transitive relation, superproperty of this one, being also
               added)."""@en ;
        ] ,
        [
            dc:date "2023-11-12" ;
            rdf:value "Updated the labels."@en ;
        ] ;
    skos:scopeNote """To be used only when the current partitive relation is direct,
         without any intermediate node between the related things."""@en ;
.

:isBeginningDateOf
    a owl:ObjectProperty ;
    rdfs:label
        "is beginning date of"@en ,
        "es fecha de inicio de"@es ,
        "est la date de début de"@fr ;
    rdfs:comment """Connects a Date to a Thing that came into existence on that
         Date."""@en ;
    rdfs:domain :Date ;
    rdfs:isDefinedBy <https://www.ica.org/standards/RiC/ontology> ;
    rdfs:range :Thing ;
    rdfs:subPropertyOf :isDateAssociatedWith ;
    owl:inverseOf :hasBeginningDate ;
    skos:changeNote
        [
            dc:date "2023-11-02" ;
            rdf:value "Added a new rdfs:label in Spanish."@en ;
        ] ,
        [
            dc:date "2023-08-28" ;
            rdf:value "Added a new rdfs:label in French."@en ;
        ] ;
    :RiCCMCorrespondingComponent """RiC-R069 ('is beginning date of'
         relation)"""@en ;
.

:isDirectPartOf
    a owl:ObjectProperty ;
    rdfs:label
        "is direct part of"@en ,
        "es parte directa de"@es ,
        "fait directement partie de"@fr ;
    rdfs:comment """Connects a Thing to a Thing of which it is direct constitutive or
         component part."""@en ;
    rdfs:domain :Thing ;
    rdfs:isDefinedBy <https://www.ica.org/standards/RiC/ontology> ;
    rdfs:range :Thing ;
    rdfs:subPropertyOf :isPartOfTransitive ;
    owl:inverseOf :hasDirectPart ;
    skos:changeNote
        [
            dc:date "2023-11-12" ;
            rdf:value "Updated the labels."@en ;
        ] ,
        [
            dc:date "2023-11-27" ;
            rdf:value "Added a new rdfs:label in Spanish."@en ;
        ] ,
        [
            dc:date "2023-07-12" ;
            rdf:value """Object property added, along with its inverse property, in
               order to enable to express current, direct, partitive relations between things (the
               possibly indirect, transitive relation, superproperty of this one, being also
               added)."""@en ;
        ] ;
    skos:scopeNote """To be used only when the current partitive relation is direct,
         without any intermediate node between the related things."""@en ;
.

:isRecordResourceAssociatedWithRecordResource
    a
        owl:ObjectProperty ,
        owl:SymmetricProperty ;
    rdfs:label
        "is record resource associated with record resource"@en ,
        "es recurso documental asociado con"@es ,
        """est une ressource archivistique associée avec la ressource
         archivistique"""@fr ;
    rdfs:comment """Connects two Record Resources. This relation is
         symmetric."""@en ;
    rdfs:domain :RecordResource ;
    rdfs:isDefinedBy <https://www.ica.org/standards/RiC/ontology> ;
    rdfs:range :RecordResource ;
    rdfs:subPropertyOf :isRelatedTo ;
    owl:propertyChainAxiom (
        :thingIsConnectedToRelation
        :recordResourceToRecordResourceRelation_role
        :relationConnects
    ) ;
    skos:changeNote
        [
            dc:date "2023-11-08" ;
            rdf:value """In order to get a system of rolified Relation classes: modified
               the property chain axiom so that it now involves the new
               recordResourceToRecordResourceRelation_role object property."""@en ;
        ] ,
        [
            dc:date "2023-11-12" ;
            rdf:value """Aligned with RiC-CM 1.0: updated the description
               (rdfs:comment), skos:scopeNote."""@en ;
        ] ,
        [
            dc:date "2023-08-28" ;
            rdf:value "Added a new rdfs:label in French."@en ;
        ] ,
        [
            dc:date "2023-11-25" ;
            rdf:value "Fixed the French label."@en ;
        ] ,
        [
            dc:date "2023-11-02" ;
            rdf:value "Added a new rdfs:label in Spanish."@en ;
        ] ;
    skos:scopeNote """Use to connect two Record Resources only if it is not possible
         to use a narrower, more specific relation, for example has genetic link
         to."""@en ;
    :RiCCMCorrespondingComponent """RiC-R022 ('is record resource associated with
         record resource' relation)"""@en ;
.

:precedesInTime
    a
        owl:ObjectProperty ,
        owl:TransitiveProperty ;
    rdfs:label
        "precedes in time"@en ,
        "precede en el tiempo a"@es ,
        "précède dans le temps"@fr ;
    rdfs:comment """Connects a Thing to a Thing that follows it in chronological
         order. This is a transitive relation."""@en ;
    rdfs:domain :Thing ;
    rdfs:isDefinedBy <https://www.ica.org/standards/RiC/ontology> ;
    rdfs:range :Thing ;
    rdfs:subPropertyOf :precedesOrPreceded ;
    owl:inverseOf :followsInTime ;
    owl:propertyChainAxiom (
        :thingIsSourceOfRelation
        :temporalRelation_role
        :relationHasTarget
    ) ;
    skos:changeNote
        [
            dc:date "2023-08-28" ;
            rdf:value "Added a new rdfs:label in French."@en ;
        ] ,
        [
            dc:date "2021-01-22" ;
            rdf:value "changed the superproperty IRI"@en ;
        ] ,
        [
            dc:date "2023-11-08" ;
            rdf:value """In order to get a system of rolified Relation classes: modified
               the property chain axiom so that it now involves the new temporalRelation_role object
               property."""@en ;
        ] ,
        [
            dc:date "2023-11-02" ;
            rdf:value "Added a new rdfs:label in Spanish."@en ;
        ] ,
        [
            dc:date "2023-09-21" ;
            rdf:value "Property made transitive."@en ;
        ] ;
    skos:scopeNote """There may actually be zero to many intermediate Entities,
         ignored or unknown, in the chronological sequence between the two connected
         Entities."""@en ;
    :RiCCMCorrespondingComponent """RiC-R009 ('precedes in time'
         relation)"""@en ;
.

:wasPartOf
    a owl:ObjectProperty ;
    rdfs:label
        "was part of"@en ,
        "era parte de"@es ,
        "a fait partie de"@fr ;
    rdfs:comment """Connects a Thing to a Thing of which it was a constitutive or
         component part in the past."""@en ;
    rdfs:domain :Thing ;
    rdfs:isDefinedBy <https://www.ica.org/standards/RiC/ontology> ;
    rdfs:range :Thing ;
    rdfs:subPropertyOf :isOrWasPartOf ;
    owl:inverseOf :hadPart ;
    skos:changeNote
        [
            dc:date "2023-11-12" ;
            rdf:value "Updated the labels."@en ;
        ] ,
        [
            dc:date "2023-11-27" ;
            rdf:value "Added a new rdfs:label in Spanish."@en ;
        ] ,
        [
            dc:date "2023-07-12" ;
            rdf:value """Object property added, along with its inverse property, in
               order to enable to express past partitive relations between things (the current
               partitive relations being also added, including a transitive one)."""@en ;
        ] ;
.

:DocumentaryFormType
    a owl:Class ;
    rdfs:label
        "Documentary Form Type"@en ,
        "Tipo documental"@es ,
        "Type de document"@fr ;
    rdfs:comment """Categorization of a Record or Record Part with respect to its
         extrinsic and intrinsic elements that together communicate its content, administrative and
         documentary context, and authority."""@en ;
    rdfs:isDefinedBy <https://www.ica.org/standards/RiC/ontology> ;
    rdfs:subClassOf :Type ;
    skos:changeNote
        [
            dc:date "2020-10-23" ;
            rdf:value """Comment: updated. Scope note: made several paragraphs.
               Objective: to make RiC-O compliant with RiC-CM v0.2."""@en ;
        ] ,
        [
            dc:date "2023-04-19" ;
            rdf:value "Removed the 0.2 existing unnecessary restriction."@en ;
        ] ,
        [
            dc:date "2023-08-25" ;
            rdf:value "Added a new rdfs:label in French."@en ;
        ] ,
        [
            dc:date "2023-11-12" ;
            rdf:value """Aligned with RiC-CM 1.0: updated the description
               (rdfs:comment)."""@en ;
        ] ,
        [
            dc:date "2023-11-02" ;
            rdf:value "Added a new rdfs:label in Spanish."@en ;
        ] ;
    skos:scopeNote """Documentary Form Type plays an important role in determining the
         type of information a Record may comprise, its status of perfection, and its authenticity
         and reliability. Documentary form types exist in a specific social and cultural context,
         and within that context, are subject to change over time."""@en ;
    :RiCCMCorrespondingComponent """Corresponds to RiC-A17 (Documentary Form Type
         attribute)"""@en ;
.

:hasPartTransitive
    a
        owl:ObjectProperty ,
        owl:TransitiveProperty ;
    rdfs:label
        "has part transitive"@en ,
        "tiene como parte transitivo"@es ,
        "a pour partie transitif"@fr ;
    rdfs:comment """Connects a Thing to a Thing that is, directly or indirectly, a
         constitutive or component part of that Thing. This is a transitive relation."""@en ;
    rdfs:domain :Thing ;
    rdfs:isDefinedBy <https://www.ica.org/standards/RiC/ontology> ;
    rdfs:range :Thing ;
    rdfs:subPropertyOf :hasOrHadPart ;
    owl:inverseOf :isPartOfTransitive ;
    skos:changeNote
        [
            dc:date "2023-11-27" ;
            rdf:value "Added a new rdfs:label in Spanish."@en ;
        ] ,
        [
            dc:date "2023-07-12" ;
            rdf:value """Object property added, along with its inverse property, in
               order to enable to express current partitive relations between things (the past
               partitive relation also being added)."""@en ;
        ] ,
        [
            dc:date "2023-11-12" ;
            rdf:value "Updated the labels."@en ;
        ] ;
    skos:scopeNote """To be used, either to infer, then query or browse, relations
         from existing direct 'hasDirectPart' relations between things, or to record a current
         partitive relation when you do not know if there are intermediate nodes between the related
         things."""@en ;
.

:isAssociatedWithPlace
    a owl:ObjectProperty ;
    rdfs:label
        "is associated with place"@en ,
        "está asociado con lugar"@es ,
        "est associé au lieu"@fr ;
    rdfs:comment """Inverse of 'is place associated with' object
         property."""@en ;
    rdfs:domain :Thing ;
    rdfs:isDefinedBy <https://www.ica.org/standards/RiC/ontology> ;
    rdfs:range :Place ;
    rdfs:subPropertyOf :isRelatedTo ;
    owl:inverseOf :isPlaceAssociatedWith ;
    owl:propertyChainAxiom (
        :thingIsTargetOfRelation
        :placeRelation_role
        :relationHasSource
    ) ;
    skos:changeNote
        [
            dc:date "2023-08-28" ;
            rdf:value "Added a new rdfs:label in French."@en ;
        ] ,
        [
            dc:date "2023-11-08" ;
            rdf:value """In order to get a system of rolified Relation classes: modified
               the property chain axiom so that it now involves the new placeRelation_role object
               property."""@en ;
        ] ,
        [
            dc:date "2023-11-02" ;
            rdf:value "Added a new rdfs:label in Spanish."@en ;
        ] ;
    :RiCCMCorrespondingComponent """RiC-R074i ('is associated with place'
         relation)"""@en ;
.

:isDateAssociatedWith
    a owl:ObjectProperty ;
    rdfs:label
        "is date associated with"@en ,
        "es fecha asociada con"@es ,
        "est une date associée a"@fr ;
    rdfs:comment """Connects a Date to a Thing with whose existence and lifecycle the
         Date is associated."""@en ;
    rdfs:domain :Date ;
    rdfs:isDefinedBy <https://www.ica.org/standards/RiC/ontology> ;
    rdfs:range :Thing ;
    rdfs:subPropertyOf :isRelatedTo ;
    owl:inverseOf :isAssociatedWithDate ;
    skos:changeNote
        [
            dc:date "2023-08-28" ;
            rdf:value "Added a new rdfs:label in French."@en ;
        ] ,
        [
            dc:date "2023-11-12" ;
            rdf:value """Aligned with RiC-CM 1.0: updated the description
               (rdfs:comment), skos:scopeNote."""@en ;
        ] ,
        [
            dc:date "2023-11-02" ;
            rdf:value "Added a new rdfs:label in Spanish."@en ;
        ] ;
    skos:scopeNote """Use to connect a date and an entity only if it is not possible
         to specify a narrower date relation, for example, is beginning date of."""@en ;
    :RiCCMCorrespondingComponent """RiC-R068 ('is date associated with'
         relation)"""@en ;
.

:isPartOfTransitive
    a
        owl:ObjectProperty ,
        owl:TransitiveProperty ;
    rdfs:label
        "is part of transitive"@en ,
        "es parte de transitivo"@es ,
        "est une partie de transitif"@fr ;
    rdfs:comment """Connects a Thing to a Thing of which it is a a constitutive or
         component part, directly or indirectly. This is a transitive relation."""@en ;
    rdfs:domain :Thing ;
    rdfs:isDefinedBy <https://www.ica.org/standards/RiC/ontology> ;
    rdfs:range :Thing ;
    rdfs:subPropertyOf :isOrWasPartOf ;
    owl:inverseOf :hasPartTransitive ;
    skos:changeNote
        [
            dc:date "2023-11-27" ;
            rdf:value "Added a new rdfs:label in Spanish."@en ;
        ] ,
        [
            dc:date "2023-11-13" ;
            rdf:value "Added a French label."@en ;
        ] ,
        [
            dc:date "2023-07-12" ;
            rdf:value """Object property added, along with its inverse property, in
               order to enable to express current partitive relations between things (the past
               partitive relation also being added)."""@en ;
        ] ;
    skos:scopeNote """To be used, either to infer, then query or browse, relations
         from existing direct 'isDirectPartOf' relations between things, or to record a current
         partitive relation when you do not know if there are intermediate nodes between the related
         things."""@en ;
.

:isPlaceAssociatedWith
    a owl:ObjectProperty ;
    rdfs:label
        "is place associated with"@en ,
        "es lugar asociado con"@es ,
        "est un lieu associé à"@fr ;
    rdfs:comment """Connects a Place to a Thing with whose existence and lifecycle the
         Place is associated."""@en ;
    rdfs:domain :Place ;
    rdfs:isDefinedBy <https://www.ica.org/standards/RiC/ontology> ;
    rdfs:range :Thing ;
    rdfs:subPropertyOf :isRelatedTo ;
    owl:inverseOf :isAssociatedWithPlace ;
    owl:propertyChainAxiom (
        :thingIsSourceOfRelation
        :placeRelation_role
        :relationHasTarget
    ) ;
    skos:changeNote
        [
            dc:date "2023-11-02" ;
            rdf:value "Added a new rdfs:label in Spanish."@en ;
        ] ,
        [
            dc:date "2023-08-28" ;
            rdf:value "Added a new rdfs:label in French."@en ;
        ] ,
        [
            dc:date "2023-11-12" ;
            rdf:value """Aligned with RiC-CM 1.0: updated the description
               (rdfs:comment), skos:scopeNote."""@en ;
        ] ,
        [
            dc:date "2023-11-08" ;
            rdf:value """In order to get a system of rolified Relation classes: modified
               the property chain axiom so that it now involves the new placeRelation_role object
               property."""@en ;
        ] ;
    skos:scopeNote """Use to connect a Place to an entity only if it is not possible
         to specify a narrower spatial relation, for example, is or was location
         of."""@en ;
    :RiCCMCorrespondingComponent """RiC-R074 ('is place associated with'
         relation)"""@en ;
.

<https://www.ica.org/standards/RiC/vocabularies/recordSetTypes>
    a
        owl:NamedIndividual ,
        skos:ConceptScheme ;
    rdfs:label
        "Record Set Types"@en ,
        "Tipos de agrupación documental"@es ,
        "Types d’ensembles d’objets informationnels"@fr ;
    dc:creator """International Coucil on Archives Expert Group on Archival
         Description (ICA EGAD)"""@en ;
    dc:language
        "en" ,
        "es" ,
        "fr" ;
    dc:title """International Council on Archives Records in Contexts Vocabulary for
         Record Set Types"""@en ;
    skos:changeNote
        [
            dc:date "2023-12-13" ;
            rdf:value """Completed the metadata of the vocabulary: added dc:language, a
               history note and a scope note."""@en ;
        ] ,
        [
            dc:date "2023-11-25" ;
            rdf:value "Added a new rdfs:label in Spanish."@en ;
        ] ,
        [
            dc:date "2023-08-28" ;
            rdf:value "Added a new rdfs:label in French."@en ;
        ] ;
    skos:definition """A vocabulary that provides URIs for describing types of RiC
         Record Sets."""@en ;
    skos:hasTopConcept
        ric-rst:Collection ,
        ric-rst:File ,
        ric-rst:Fonds ,
        ric-rst:Series ;
    skos:historyNote """This vocabulary was created within the Records in Contexts
         Ontology. When the ICA/EGAD developed RiC-O 1.0, it was decided that two versions of RiC-O
         would be released. The first one, consisting of a unique large OWL file, would remain the
         reference one. RiC-0 1.0 would also be provided as a set of files, in order to address
         specific needs, e.g. using only the core of the ontology, or using only the individuals it
         defined and defining new individuals. So from December 2023, you can find the vocabulary on
         Record Set Types, either in the unique large OWL RiC-O file, or as a separate file. """@en ;
    skos:scopeNote """For now this vocabulary only defines four top concepts; it
         should hopefully be completed later. The concepts defined in this vocabulary can be used in
         combination with RiC-O classes and properties, whenever necessary and appropriate, to
         assign a record set type to a Record Set, using the rico:hasRecordSetType object property,
         or its inverse one. Each concept is both defined as a skos:Concept and a
         rico:RecordSetType, so that it is possible to extend the classic definition of such
         concepts using RiC-O properties. For example, you can use rico:history, rico:date, or
         rico:isAssociatedWithPlace, rico:precedesInTime, if you consider a record set type as being
         a historical entity, known and used in some known space or time region."""@en ;
.

:isAssociatedWithDate
    a owl:ObjectProperty ;
    rdfs:label
        "is associated with date"@en ,
        "está asociado con fecha"@es ,
        "est associé à la date"@fr ;
    rdfs:comment """Inverse of 'is date associated with' object
         property."""@en ;
    rdfs:domain :Thing ;
    rdfs:isDefinedBy <https://www.ica.org/standards/RiC/ontology> ;
    rdfs:range :Date ;
    rdfs:subPropertyOf :isRelatedTo ;
    owl:inverseOf :isDateAssociatedWith ;
    skos:changeNote
        [
            dc:date "2023-11-02" ;
            rdf:value "Added a new rdfs:label in Spanish."@en ;
        ] ,
        [
            dc:date "2023-08-28" ;
            rdf:value "Added a new rdfs:label in French."@en ;
        ] ;
    :RiCCMCorrespondingComponent """RiC-R068i ('is associated with date'
         relation)"""@en ;
.

:hasOrHadPart
    a owl:ObjectProperty ;
    rdfs:label
        "has or had part"@en ,
        "tiene o tenía como parte"@es ,
        "a ou a eu pour partie"@fr ;
    rdfs:comment """Connects a Thing to a constitutive or component part of that
         Thing."""@en ;
    rdfs:domain :Thing ;
    rdfs:isDefinedBy <https://www.ica.org/standards/RiC/ontology> ;
    rdfs:range :Thing ;
    rdfs:subPropertyOf :isRelatedTo ;
    owl:inverseOf :isOrWasPartOf ;
    owl:propertyChainAxiom (
        :thingIsSourceOfRelation
        :wholePartRelation_role
        :relationHasTarget
    ) ;
    skos:changeNote
        [
            dc:date "2023-08-28" ;
            rdf:value "Added a new rdfs:label in French."@en ;
        ] ,
        [
            dc:date "2023-11-08" ;
            rdf:value """In order to get a system of rolified Relation classes: modified
               the property chain axiom so that it now involves the new wholePartRelation_role
               object property."""@en ;
        ] ,
        [
            dc:date "2021-01-22" ;
            rdf:value """changed the IRI, label, inverse property IRI, textual
               definition (changed made in order to make RiC-O compliant with RiC-CM 0.2; the name
               of this property in RiC-O 0.1 was "hasPart")."""@en ;
        ] ,
        [
            dc:date "2023-11-12" ;
            rdf:value """Aligned with RiC-CM 1.0: updated the
               skos:scopeNote."""@en ;
        ] ,
        [
            dc:date "2023-11-02" ;
            rdf:value "Added a new rdfs:label in Spanish."@en ;
        ] ;
    skos:scopeNote """Use to connect a Thing to another Thing that is or was a part of
         the whole Thing only if it is not possible to use a narrower, more specific whole/part
         relation, for example has or had constituent. The end of existence of a whole/part relation
         may affect the integrity or nature of the domain entity."""@en ;
    :RiCCMCorrespondingComponent """RiC-R002 ('has or had part'
         relation)"""@en ;
.

:isOrWasPartOf
    a owl:ObjectProperty ;
    rdfs:label
        "is or was part of"@en ,
        "es o era parte de"@es ,
        "est ou a été une partie de"@fr ;
    rdfs:comment "Inverse of 'has or had part' relation."@en ;
    rdfs:domain :Thing ;
    rdfs:isDefinedBy <https://www.ica.org/standards/RiC/ontology> ;
    rdfs:range :Thing ;
    rdfs:subPropertyOf :isRelatedTo ;
    owl:inverseOf :hasOrHadPart ;
    owl:propertyChainAxiom (
        :thingIsTargetOfRelation
        :wholePartRelation_role
        :relationHasSource
    ) ;
    skos:changeNote
        [
            dc:date "2023-08-28" ;
            rdf:value "Added a new rdfs:label in French."@en ;
        ] ,
        [
            dc:date "2021-01-22" ;
            rdf:value """changed the IRI, label, inverse property IRI, textual
               definition (changed made in order to make RiC-O compliant with RiC-CM 0.2; the name
               of this property in RiC-O 0.1 was "isPartOf")."""@en ;
        ] ,
        [
            dc:date "2023-11-08" ;
            rdf:value """In order to get a system of rolified Relation classes: modified
               the property chain axiom so that it now involves the new wholePartRelation_role
               object property."""@en ;
        ] ,
        [
            dc:date "2023-11-02" ;
            rdf:value "Added a new rdfs:label in Spanish."@en ;
        ] ;
    :RiCCMCorrespondingComponent """RiC-R002i ('is or was part of'
         relation)"""@en ;
.

:AgentToAgentRelation
    a owl:Class ;
    rdfs:label
        "Agent Relation"@en ,
        "Relación entre agentes"@es ,
        "Relation entre agents"@fr ;
    rdfs:comment """Connects at least two Agents. This Relation is a generic, not
         oriented one."""@en ;
    rdfs:isDefinedBy <https://www.ica.org/standards/RiC/ontology> ;
    rdfs:subClassOf
        [
            a owl:Restriction ;
            owl:minQualifiedCardinality "2"^^xsd:nonNegativeInteger ;
            owl:onClass :Agent ;
            owl:onProperty :relationConnects ;
        ] ,
        :Relation ;
    owl:equivalentClass
        [
            a owl:Restriction ;
            owl:hasSelf true ;
            owl:onProperty :agentToAgentRelation_role ;
        ] ;
    skos:changeNote
        [
            dc:date "2023-08-25" ;
            rdf:value "Added a new rdfs:label in French."@en ;
        ] ,
        [
            dc:date "2023-11-08" ;
            rdf:value """In order to get a system of rolified Relation classes: added an
               equivalentClass object property; replaced the specific object properties by the
               generic ones in the subClassOf declarations."""@en ;
        ] ,
        [
            dc:date "2023-11-02" ;
            rdf:value "Added a new rdfs:label in Spanish."@en ;
        ] ,
        [
            dc:date "2023-12-06" ;
            rdf:value """Improved the description of the Relation class (rdfs:comment)
               by clearly specifying how it is directed."""@en ;
        ] ,
        [
            dc:date "2023-11-12" ;
            rdf:value """Aligned with RiC-CM 1.0: updated the
               skos:scopeNote."""@en ;
        ] ;
    skos:scopeNote """Use only if it is not possible to specify a narrower agent to
         agent relation, for example a WorkRelation."""@en ;
    :RiCCMCorrespondingComponent """Class implementation of RiC-R044 and RiC-044i
         relations"""@en ;
.

:agentToAgentRelation_role
    a
        owl:ObjectProperty ,
        owl:ReflexiveProperty ;
    rdfs:label
        "has the role of the Agent Relation"@en ,
        "desempeña el papel de la Relación entre agentes"@es ,
        "a le rôle de la Relation entre agents"@fr ;
    rdfs:comment """Connects a AgentToAgentRelation to itself. It is a reflexive
         property, that can stand for an instance of the class when necessary, e.g. when you explore
         a knowledge graph."""@en ;
    rdfs:domain :AgentToAgentRelation ;
    rdfs:isDefinedBy <https://www.ica.org/standards/RiC/ontology> ;
    rdfs:range :AgentToAgentRelation ;
    rdfs:subPropertyOf :relation_role ;
    skos:changeNote
        [
            dc:date "2023-11-08" ;
            rdf:value """In order to get a system of rolified Relation classes: created
               the object property, with domain and range the AgentToAgentRelation rolified class.
               Declared it as reflexive. Declared it(s) superproperty(ies)."""@en ;
        ] ;
    skos:scopeNote """This property "rolifies" the AgentToAgentRelation class. It
         should be used only when you have to manage instances of the AgentToAgentRelation class, to
         connect each instance to itself, in order to be able to infer, using OWL-RL and property
         paths, the two shortcuts corresponding to this n-ary class."""@en ;
.

:CorporateBody
    a owl:Class ;
    rdfs:label
        "Corporate Body"@en ,
        "Institución"@es ,
        "Collectivité"@fr ;
    rdfs:comment """An organized group of persons that act together as an Agent, and
         that has a recognized legal or social status."""@en ;
    rdfs:isDefinedBy <https://www.ica.org/standards/RiC/ontology> ;
    rdfs:subClassOf :Group ;
    skos:changeNote
        [
            dc:date "2023-08-25" ;
            rdf:value "Added a new rdfs:label in French."@en ;
        ] ,
        [
            dc:date "2023-08-25" ;
            rdf:value "Added a new rdfs:label in French."@en ;
        ] ,
        [
            dc:date "2020-10-23" ;
            rdf:value """scope note: updated. Objective: to make RiC-O compliant with
               RiC-CM v0.2."""@en ;
        ] ,
        [
            dc:date "2023-11-12" ;
            rdf:value """Aligned with RiC-CM 1.0: updated the description
               (rdfs:comment), skos:scopeNote."""@en ;
        ] ,
        [
            dc:date "2023-11-02" ;
            rdf:value "Added a new rdfs:label in Spanish."@en ;
        ] ;
    skos:scopeNote """Corporate body is a kind of Group (RiC-E09). By exception,
         within some legal contexts, a sole trader or sole proprietor may be recognized as a
         corporate body, even when the economic enterprise does not have additional members.
         Corporate bodies often have a mandate giving them the authority to act within their area(s)
         of competence. They will also usually act within a particular jurisdiction being governed
         by legal and other rule-based frameworks. A corporate body though may be constituted in a
         more informal manner and exist as an entity by virtue of its recognition as such by its
         members."""@en ;
    :RiCCMCorrespondingComponent """Corresponds to RiC-E11 (Corporate Body
         entity)"""@en ;
.

:Extent
    a owl:Class ;
    rdfs:label
        "Extent"@en ,
        "Extensión"@es ,
        "Mesure"@fr ;
    rdfs:comment """Countable characteristics of the content of an entity expressed as
         a quantity."""@en ;
    rdfs:isDefinedBy <https://www.ica.org/standards/RiC/ontology> ;
    rdfs:subClassOf :Thing ;
    skos:changeNote
        [
            dc:date "2020-10-28" ;
            rdf:value """Class added together with three subclasses and hasExtent and
               isExtentOf Object properties"""@en ;
        ] ,
        [
            dc:date "2023-11-02" ;
            rdf:value "Added a new rdfs:label in Spanish."@en ;
        ] ,
        [
            dc:date "2023-08-25" ;
            rdf:value "Added a new rdfs:label in French."@en ;
        ] ;
    skos:scopeNote "Physical or logical extent of a resource"@en ;
.

:Appellation
    a owl:Class ;
    rdfs:label
        "Appellation"@en ,
        "Denominación"@es ,
        "Appellation"@fr ;
    rdfs:comment """A concept of any kind that is used for designating an Entity and
         referring to it."""@en ;
    rdfs:isDefinedBy <https://www.ica.org/standards/RiC/ontology> ;
    rdfs:subClassOf :Concept ;
    skos:changeNote
        [
            dc:date "2023-11-02" ;
            rdf:value "Added a new rdfs:label in Spanish."@en ;
        ] ,
        [
            dc:date "2023-08-25" ;
            rdf:value "Added a new rdfs:label in French."@en ;
        ] ;
.

:Activity
    a owl:Class ;
    rdfs:label
        "Activity"@en ,
        "Actividad"@es ,
        "Activité"@fr ;
    rdfs:comment "The doing of something for some human purpose."@en ;
    rdfs:isDefinedBy <https://www.ica.org/standards/RiC/ontology> ;
    rdfs:subClassOf :Event ;
    skos:changeNote
        [
            dc:date "2023-04-19" ;
            rdf:value "Removed the 0.2 existing unnecessary restriction."@en ;
        ] ,
        [
            dc:date "2020-10-23" ;
            rdf:value """Scope note: made separate paragraphs and updated. Objective: to
               make RiC-O compliant with RiC-CM v0.2."""@en ;
        ] ,
        [
            dc:date "2023-11-02" ;
            rdf:value "Added a new rdfs:label in Spanish."@en ;
        ] ,
        [
            dc:date "2023-08-25" ;
            rdf:value "Added a new rdfs:label in French."@en ;
        ] ;
    skos:scopeNote """Activity is a kind of Event. Activity is specifically used to
         designate purposeful human activity. Activity may be understood from two perspectives.
         First it can be understood as leading to an end. The end is the purpose of the Activity, or
         why the Activity is performed. Second, it can be understood in terms of the processes that
         lead to achieving the end, how the end is realized through coordinated actions. Purpose and
         process are complementary understandings of Activity. Together the two perspectives address
         why the Activity is performed, the expected ends or outcomes; and how the Activity fulfills
         the purpose. While activity has an intended end, it also has unintended consequences and
         results, or side-effects. By and large, these may not be the focus of the description, but
         they are, unquestionably, context. |In a corporate or government context an Activity may
         also be called a 'function'. An Activity exists in a specific social and cultural context,
         and within that context is subject to change over time. An Activity may be composed of
         other Activities."""@en ;
    :RiCCMCorrespondingComponent """Corresponds to RiC-E15 (Activity
         entity)"""@en ;
.

:isAgentAssociatedWithAgent
    a
        owl:ObjectProperty ,
        owl:SymmetricProperty ;
    rdfs:label
        "is agent associated with agent"@en ,
        "agente está asociado con agente"@es ,
        "est un agent associé à l’agent"@fr ;
    rdfs:comment """Connects two Agents. This object property is
         symmetric."""@en ;
    rdfs:domain :Agent ;
    rdfs:isDefinedBy <https://www.ica.org/standards/RiC/ontology> ;
    rdfs:range :Agent ;
    rdfs:subPropertyOf :isRelatedTo ;
    owl:propertyChainAxiom (
        :thingIsConnectedToRelation
        :agentToAgentRelation_role
        :relationConnects
    ) ;
    skos:changeNote
        [
            dc:date "2023-11-08" ;
            rdf:value """In order to get a system of rolified Relation classes: modified
               the property chain axiom so that it now involves the new agentToAgentRelation_role
               object property."""@en ;
        ] ,
        [
            dc:date "2023-08-28" ;
            rdf:value "Added a new rdfs:label in French."@en ;
        ] ,
        [
            dc:date "2023-11-25" ;
            rdf:value "Fixed the French label."@en ;
        ] ,
        [
            dc:date "2023-11-12" ;
            rdf:value """Aligned with RiC-CM 1.0: updated the
               skos:scopeNote."""@en ;
        ] ,
        [
            dc:date "2023-11-02" ;
            rdf:value "Added a new rdfs:label in Spanish."@en ;
        ] ;
    skos:scopeNote """Use only if it is not possible to specify a narrower Agent to
         Agent relation, for example has or had work relation with."""@en ;
    :RiCCMCorrespondingComponent """RiC-R044 ('is agent associated with agent'
         relation)"""@en ;
.

:relation_role
    a
        owl:ObjectProperty ,
        owl:ReflexiveProperty ;
    rdfs:label
        "has the role of the Relation"@en ,
        "desempeña el papel de la Relación"@es ,
        "a le rôle de la Relation"@fr ;
    rdfs:comment """Connects a Relation to itself. It is a reflexive property, that
         can stand for an instance of the class when necessary, e.g. when you explore a knowledge
         graph."""@en ;
    rdfs:domain :Relation ;
    rdfs:isDefinedBy <https://www.ica.org/standards/RiC/ontology> ;
    rdfs:range :Relation ;
    skos:changeNote
        [
            dc:date "2023-11-08" ;
            rdf:value """In order to get a system of rolified Relation classes: created
               the object property, with domain and range the Relation rolified class. Declared it
               as reflexive."""@en ;
        ] ;
    skos:scopeNote """This property "rolifies" the generic Relation class. It should
         be used only when you have to manage instances of this Relation class, to connect each
         instance to itself, in order to be able to infer, using OWL-RL and property paths, the two
         shortcuts corresponding to this n-ary class."""@en ;
.

:thingIsConnectedToRelation
    a owl:ObjectProperty ;
    rdfs:label
        "thing is connected to relation"@en ,
        "cosa está conectada con relación"@es ,
        "chose est connectée à la relation"@fr ;
    rdfs:comment "Connects a Thing to a n-ary Relation."@en ;
    rdfs:domain :Thing ;
    rdfs:isDefinedBy <https://www.ica.org/standards/RiC/ontology> ;
    rdfs:range :Relation ;
    rdfs:subPropertyOf :isRelatedTo ;
    owl:inverseOf :relationConnects ;
    skos:changeNote
        [
            dc:date "2023-11-12" ;
            rdf:value "Updated the labels."@en ;
        ] ,
        [
            dc:date "2023-11-02" ;
            rdf:value "Added a new rdfs:label in Spanish."@en ;
        ] ,
        [
            dc:date "2023-12-30" ;
            rdf:value "Fixed a typo in the French label."@en ;
        ] ;
.

:Rule
    a owl:Class ;
    rdfs:label
        "Rule"@en ,
        "Regla"@es ,
        "Règle"@fr ;
    rdfs:comment """Conditions that govern the existence, responsibility, or authority
         of an Agent; or the performance of an Activity by an Agent; or that contribute to the
         distinct characteristics of things created or managed by an Agent."""@en ;
    rdfs:isDefinedBy <https://www.ica.org/standards/RiC/ontology> ;
    rdfs:subClassOf :Thing ;
    skos:changeNote
        [
            dc:date "2023-08-25" ;
            rdf:value "Added a new rdfs:label in French."@en ;
        ] ,
        [
            dc:date "2021-02-11" ;
            rdf:value """Updated the definition (rdfs:comment) and scope note, as they
               were recently changed in RiC-CM 0.2 full draft."""@en ;
        ] ,
        [
            dc:date "2020-10-23" ;
            rdf:value """Scope note: made separate paragraphs and updated. Objective: to
               make RiC-O compliant with RiC-CM v0.2."""@en ;
        ] ,
        [
            dc:date "2023-11-12" ;
            rdf:value """Aligned with RiC-CM 1.0: updated the description
               (rdfs:comment), skos:scopeNote."""@en ;
        ] ,
        [
            dc:date "2023-04-19" ;
            rdf:value "Removed the 0.2 existing unnecessary restriction."@en ;
        ] ,
        [
            dc:date "2023-11-02" ;
            rdf:value "Added a new rdfs:label in Spanish."@en ;
        ] ;
    skos:scopeNote """Rule is a kind of Thing. Rule can be related directly to agent,
         activity, or anything created or managed by agents, such as a record resource or
         instantiation. A rule may be unwritten or written or otherwise documented. Unwritten rules
         may include though are not limited to the following: social mores, customs, or community
         expectations. Written rules may include though are not limited to the following:
         constitutions, legislation, acts (legal), statutes, legal codes, ordinances, charters,
         mission statements, regulations, policies, procedures, instructions, codes of conduct or
         ethics, professional standards, work assignments, or work plans. The source or sources of
         some rules governing the existence or activity of an agent may be external (for example,
         expressed in elections, social mores, customs, community expectations, laws, regulations,
         standards, and best practice codes), while others may be expressed within the immediate
         context of an agent (for example, policies, or written or verbal instructions). The
         evidence for identifying rules may be found in their entirety in one documentary source
         (for example, a law or regulation) or may be found in two or more sources. Rule should not
         be confused with the one or more documentary sources that serve as evidence of its
         identity. A documentary source is a record."""@en ;
    :RiCCMCorrespondingComponent """Corresponds to RiC-E16 (Rule
         entity)"""@en ;
.

:hasOrHadCategory
    a owl:ObjectProperty ;
    rdfs:label
        "has or had category"@en ,
        "tiene o tenía como categoría"@es ,
        "a ou a eu pour catégorie"@fr ;
    rdfs:comment """Connects a Thing to a Type that categorizes or categorized
         it."""@en ;
    rdfs:domain :Thing ;
    rdfs:isDefinedBy <https://www.ica.org/standards/RiC/ontology> ;
    rdfs:range :Type ;
    rdfs:subPropertyOf :isRelatedTo ;
    owl:inverseOf :isOrWasCategoryOf ;
    owl:propertyChainAxiom (
        :thingIsTargetOfRelation
        :typeRelation_role
        :relationHasSource
    ) ;
    skos:changeNote
        [
            dc:date "2023-11-02" ;
            rdf:value "Added a new rdfs:label in Spanish."@en ;
        ] ,
        [
            dc:date "2023-11-08" ;
            rdf:value """In order to get a system of rolified Relation classes: modified
               the property chain axiom so that it now involves the new typeRelation_role object
               property."""@en ;
        ] ,
        [
            dc:date "2023-08-28" ;
            rdf:value "Added a new rdfs:label in French."@en ;
        ] ,
        [
            dc:date "2021-01-22" ;
            rdf:value """changed the IRI, label, inverse property IRI, text definition
               (the name of this property in RiC-O 0.1 was "belongsToCategory")."""@en ;
        ] ;
.

:isOrWasCategoryOf
    a owl:ObjectProperty ;
    rdfs:label
        "is or was category of"@en ,
        "es o era la categoría de"@es ,
        "est ou a été la catégorie de"@fr ;
    rdfs:comment """Connects a Type (a category) to a Thing that it categorizes or
         categorized."""@en ;
    rdfs:domain :Type ;
    rdfs:isDefinedBy <https://www.ica.org/standards/RiC/ontology> ;
    rdfs:range :Thing ;
    rdfs:subPropertyOf :isRelatedTo ;
    owl:inverseOf :hasOrHadCategory ;
    owl:propertyChainAxiom (
        :thingIsSourceOfRelation
        :typeRelation_role
        :relationHasTarget
    ) ;
    skos:changeNote
        [
            dc:date "2023-11-02" ;
            rdf:value "Added a new rdfs:label in Spanish."@en ;
        ] ,
        [
            dc:date "2023-11-08" ;
            rdf:value """In order to get a system of rolified Relation classes: modified
               the property chain axiom so that it now involves the new typeRelation_role object
               property."""@en ;
        ] ,
        [
            dc:date "2021-01-22" ;
            rdf:value """changed the IRI, label, inverse property IRI, text definition
               (the name of this property in RiC-O 0.1 was "isCategoryOf")."""@en ;
        ] ,
        [
            dc:date "2023-08-28" ;
            rdf:value "Added a new rdfs:label in French."@en ;
        ] ;
.

:Position
    a owl:Class ;
    rdfs:label
        "Position"@en ,
        "Puesto"@es ,
        "Poste occupé"@fr ;
    rdfs:comment "The functional role of a Person within a Group."@en ;
    rdfs:isDefinedBy <https://www.ica.org/standards/RiC/ontology> ;
    rdfs:subClassOf :Agent ;
    skos:changeNote
        [
            dc:date "2023-11-02" ;
            rdf:value "Added a new rdfs:label in Spanish."@en ;
        ] ,
        [
            dc:date "2020-10-23" ;
            rdf:value """Scope note: made separate paragraphs and updated. Disjoint
               with: enriched. Objective: to make RiC-O compliant with RiC-CM v0.2."""@en ;
        ] ,
        [
            dc:date "2023-08-25" ;
            rdf:value "Added a new rdfs:label in French."@en ;
        ] ;
    skos:scopeNote """Position is a kind of Agent. Position is the intersection of a
         Person and a Group. Position exists independently of the Person that holds the Position
         within a Group. More than one Person may hold a Position. Position is commonly defined in a
         Mandate, often called a position description or job description. The Mandate may specify
         the work to be performed (Activity) as well as the competencies for performing the
         Activity. A Position is often given a Name. A Position may be tied to a project or to a set
         of tasks and thus have a defined duration. A Position may change over time, as the Group
         that establishes it changes over time. Position is not to be confused with Occupation or
         Activity. Within the records created by a Corporate Body, a Position may be used to
         identify the record sets resulting from activities performed by one or more persons holding
         the Position over time, without necessarily identifying or describing the Person or
         persons, or identifying which records were created by each Person."""@en ;
    :RiCCMCorrespondingComponent """Corresponds to RiC-E12 (Position
         entity)"""@en ;
.

:Type
    a owl:Class ;
    rdfs:label
        "Type"@en ,
        "Tipo"@es ,
        "Type"@fr ;
    rdfs:comment """A superclass for any category of some thing. A type characterizes
         an entity."""@en ;
    rdfs:isDefinedBy <https://www.ica.org/standards/RiC/ontology> ;
    rdfs:subClassOf :Concept ;
    skos:changeNote
        [
            dc:date "2023-11-02" ;
            rdf:value "Added a new rdfs:label in Spanish."@en ;
        ] ,
        [
            dc:date "2023-08-25" ;
            rdf:value "Added a new rdfs:label in French."@en ;
        ] ;
.

:Relation
    a owl:Class ;
    rdfs:label
        "Relation"@en ,
        "Relación"@es ,
        "Relation"@fr ;
    rdfs:comment """The top level relation class. It connects at least two Things. An
         instance of a Relation may have some datatype and object properties: a general description
         (datatype property) like any Thing; a certainty (for 'certain', 'quite probable',
         'uncertain','unknown'); a date (use either the date datatype property or the Date class and
         isAssociatedWithDate object property); a state (relationState); a location (use the Place
         class and isAssociatedWithPlace object property); a source of information that can be used
         as an evidence for it (use either source datatype property or hasSource object property).
         This Relation is the most generic one; it is not oriented."""@en ;
    rdfs:isDefinedBy <https://www.ica.org/standards/RiC/ontology> ;
    rdfs:subClassOf :Thing ;
    owl:equivalentClass
        [
            a owl:Restriction ;
            owl:hasSelf true ;
            owl:onProperty :relation_role ;
        ] ;
    skos:changeNote
        [
            dc:date "2023-12-06" ;
            rdf:value """Improved the description of the Relation class (rdfs:comment)
               by clearly specifying how it is directed."""@en ;
        ] ,
        [
            dc:date "2023-08-25" ;
            rdf:value "Added a new rdfs:label in French."@en ;
        ] ,
        [
            dc:date "2021-02-08" ;
            rdf:value """Removed the restrictions; completed the definition and scope
               note."""@en ;
        ] ,
        [
            dc:date "2023-11-08" ;
            rdf:value "added the equivalence to relation_role."@en ;
        ] ,
        [
            dc:date "2023-11-12" ;
            rdf:value """Aligned with RiC-CM 1.0: updated the description
               (rdfs:comment)."""@en ;
        ] ,
        [
            dc:date "2023-11-02" ;
            rdf:value "Added a new rdfs:label in Spanish."@en ;
        ] ;
    skos:scopeNote """Use when direct, binary object properties are not enough, e.g.
         when you need to record a date, a location or any other descriptive element for a relation
         (till RDF-Star becomes a W3C recommendation and provides a lighter method for doing so); or
         when the relation invloves more than two entities (n-ary relation). It is recommended to
         use the subclasses of the Relation class."""@en ;
.

:relationConnects
    a owl:ObjectProperty ;
    rdfs:label
        "relation connects"@en ,
        "relación conecta"@es ,
        "relation connecte"@fr ;
    rdfs:comment """Connects an n-ary Relation to any of the Things
         involved."""@en ;
    rdfs:domain :Relation ;
    rdfs:isDefinedBy <https://www.ica.org/standards/RiC/ontology> ;
    rdfs:range :Thing ;
    rdfs:subPropertyOf :isRelatedTo ;
    owl:inverseOf :thingIsConnectedToRelation ;
    skos:changeNote
        [
            dc:date "2023-11-02" ;
            rdf:value "Added a new rdfs:label in Spanish."@en ;
        ] ,
        [
            dc:date "2023-08-28" ;
            rdf:value "Added a new rdfs:label in French."@en ;
        ] ;
.

:Event
    a owl:Class ;
    rdfs:label
        "Event"@en ,
        "Evento"@es ,
        "Événement"@fr ;
    rdfs:comment "Something that happens or occurs in time and space."@en ;
    rdfs:isDefinedBy <https://www.ica.org/standards/RiC/ontology> ;
    rdfs:subClassOf :Thing ;
    skos:changeNote
        [
            dc:date "2023-11-02" ;
            rdf:value "Added a new rdfs:label in Spanish."@en ;
        ] ,
        [
            dc:date "2023-04-19" ;
            rdf:value "Removed the 0.2 existing unnecessary restriction."@en ;
        ] ,
        [
            dc:date "2023-08-25" ;
            rdf:value "Added a new rdfs:label in French."@en ;
        ] ,
        [
            dc:date "2023-11-12" ;
            rdf:value """Aligned with RiC-CM 1.0: updated the description
               (rdfs:comment), skos:scopeNote."""@en ;
        ] ,
        [
            dc:date "2020-10-23" ;
            rdf:value """Scope note: made separate paragraphs and some
               changes."""@en ;
        ] ;
    skos:scopeNote """An event may be caused by nature, an agent, or a combination of
         nature and agent. Events have temporal and spatial boundaries. An event may actively
         involve some agent(s) and affect any entity. An event may be discrete, happening at a
         specific moment in time, or may occur over an extended period of time. Events may have
         events as parts, and events may precede or follow one another. Multiple agents may
         participate in the same event, and in different roles."""@en ;
    :RiCCMCorrespondingComponent """Corresponds to RiC-E14 (Event
         entity)"""@en ;
    :closeTo "LODE Event class (http://linkedevents.org/ontology/#Event)"@en ;
.

:RecordPart
    a owl:Class ;
    rdfs:label
        "Record Part"@en ,
        "Componente documental"@es ,
        "Partie d’objet informationnel"@fr ;
    rdfs:comment """Component of a Record with independent information content that
         contributes to the intellectual completeness of the Record."""@en ;
    rdfs:isDefinedBy <https://www.ica.org/standards/RiC/ontology> ;
    rdfs:subClassOf :RecordResource ;
    skos:changeNote
        [
            dc:date "2023-11-02" ;
            rdf:value "Added a new rdfs:label in Spanish."@en ;
        ] ,
        [
            dc:date "2020-10-23" ;
            rdf:value """comment: updated. Scope note: made several paragraphs.
               Objective: to make RiC-O compliant with RiC-CM v0.2."""@en ;
        ] ,
        [
            dc:date "2021-02-08" ;
            rdf:value "Removed the Restriction."@en ;
        ] ,
        [
            dc:date "2023-08-25" ;
            rdf:value "Added a new rdfs:label in French."@en ;
        ] ,
        [
            dc:date "2023-11-12" ;
            rdf:value """Aligned with RiC-CM 1.0: updated the description
               (rdfs:comment)."""@en ;
        ] ;
    skos:scopeNote """Record Part is a kind of Record Resource. A Record Part may
         itself have Record Parts."""@en ;
    :RiCCMCorrespondingComponent """Corresponds to RiC-E05 (Record Part
         entity)"""@en ;
.

:thingIsSourceOfRelation
    a owl:ObjectProperty ;
    rdfs:label
        "thing is source of relation"@en ,
        "cosa es fuente de relación"@es ,
        "chose est la source de la relation"@fr ;
    rdfs:comment """Connects a Thing (that is the source of a Relation) to a
         Relation."""@en ;
    rdfs:domain :Thing ;
    rdfs:isDefinedBy <https://www.ica.org/standards/RiC/ontology> ;
    rdfs:range :Relation ;
    rdfs:subPropertyOf :thingIsConnectedToRelation ;
    owl:inverseOf :relationHasSource ;
    skos:changeNote
        [
            dc:date "2023-11-12" ;
            rdf:value "Updated the labels."@en ;
        ] ,
        [
            dc:date "2023-11-27" ;
            rdf:value "Added a new rdfs:label in Spanish."@en ;
        ] ;
.

:thingIsTargetOfRelation
    a owl:ObjectProperty ;
    rdfs:label
        "thing is target of relation"@en ,
        "cosa es objetivo de relación"@es ,
        "chose est la cible de la relation"@fr ;
    rdfs:comment """Connects a Thing (that is the target of a Relation) to a n-ary
         Relation."""@en ;
    rdfs:domain :Thing ;
    rdfs:isDefinedBy <https://www.ica.org/standards/RiC/ontology> ;
    rdfs:range :Relation ;
    rdfs:subPropertyOf :thingIsConnectedToRelation ;
    owl:inverseOf :relationHasTarget ;
    skos:changeNote
        [
            dc:date "2023-11-27" ;
            rdf:value "Added a new rdfs:label in Spanish."@en ;
        ] ,
        [
            dc:date "2023-11-12" ;
            rdf:value "Updated the description (rdfs:comment) and labels."@en ;
        ] ;
.

:Group
    a owl:Class ;
    rdfs:label
        "Group"@en ,
        "Grupo de agentes"@es ,
        "Groupe d’agents"@fr ;
    rdfs:comment "Two or more Agents that act together as an Agent."@en ;
    rdfs:isDefinedBy <https://www.ica.org/standards/RiC/ontology> ;
    rdfs:subClassOf :Agent ;
    owl:disjointWith
        :Mechanism ,
        :Person ,
        :Position ;
    skos:changeNote
        [
            dc:date "2023-11-02" ;
            rdf:value "Added a new rdfs:label in Spanish."@en ;
        ] ,
        [
            dc:date "2020-10-23" ;
            rdf:value """Scope note: made separate paragraphs plus very few changes.
               Disjoint with: enriched."""@en ;
        ] ,
        [
            dc:date "2023-08-25" ;
            rdf:value "Added a new rdfs:label in French."@en ;
        ] ;
    skos:scopeNote """Group is a kind of Agent. A Group has a socially recognized
         identity. Each member of the Group plays a particular role or roles (that is has a
         particular Position) in the coordinated activity of the Group. Corporate bodies and
         families are kinds of groups, though other kinds of groups are possible. For example, the
         “electorate” -- all of the voters in a given election. Complex, large groups may be
         subdivided into other groups."""@en ;
    :RiCCMCorrespondingComponent """Corresponds to RiC-E09 (Group
         Entity)"""@en ;
.

:Place
    a owl:Class ;
    rdfs:label
        "Place"@en ,
        "Lugar"@es ,
        "Lieu"@fr ;
    rdfs:comment "Bounded, named geographic area or region."@en ;
    rdfs:isDefinedBy <https://www.ica.org/standards/RiC/ontology> ;
    rdfs:subClassOf :Thing ;
    skos:changeNote
        [
            dc:date "2020-10-23" ;
            rdf:value """Comment: updated. Scope note: updated and made several
               paragraphs. Objective: to make RiC-O compliant with RiC-CM v0.2."""@en ;
        ] ,
        [
            dc:date "2023-08-25" ;
            rdf:value "Added a new rdfs:label in French."@en ;
        ] ,
        [
            dc:date "2023-11-12" ;
            rdf:value """Aligned with RiC-CM 1.0: updated the
               skos:scopeNote."""@en ;
        ] ,
        [
            dc:date "2023-04-19" ;
            rdf:value "Removed the 0.2 existing unnecessary restriction."@en ;
        ] ,
        [
            dc:date "2023-11-02" ;
            rdf:value "Added a new rdfs:label in Spanish."@en ;
        ] ;
    skos:scopeNote """A jurisdiction is the bounded geographic area within which an
         Agent has the authority to perform specified activities constrained by rules.
         Jurisdictions, man-made structures, and natural features are historical entities. A Place
         thus may have a beginning date and ending date and changing boundaries that result from
         human or natural events. A Place may be systematically referenced to a location on the
         earth (geographic coordinates)."""@en ;
    :RiCCMCorrespondingComponent """Corresponds to RiC-E22 (Place
         entity)"""@en ;
.

:Date
    a owl:Class ;
    rdfs:label
        "Date"@en ,
        "Fecha"@es ,
        "Date"@fr ;
    rdfs:comment """Chronological information associated with an entity that
         contributes to its identification and contextualization."""@en ;
    rdfs:isDefinedBy <https://www.ica.org/standards/RiC/ontology> ;
    rdfs:subClassOf :Thing ;
    skos:changeNote
        [
            dc:date "2023-11-02" ;
            rdf:value "Added a new rdfs:label in Spanish."@en ;
        ] ,
        [
            dc:date "2023-08-25" ;
            rdf:value "Added a new rdfs:label in French."@en ;
        ] ,
        [
            dc:date "2020-10-23" ;
            rdf:value "Scope note: made separate paragraphs."@en ;
        ] ,
        [
            dc:date "2023-11-12" ;
            rdf:value """Aligned with RiC-CM 1.0: updated the
               skos:scopeNote."""@en ;
        ] ;
    skos:scopeNote """A Date may be represented in natural language, based on a
         digital standard, or both. Digital standard dates will typically be based on ISO 8601, or
         Extended Date-Time Format (EDTF)"""@en ;
    :RiCCMCorrespondingComponent """Corresponds to RiC-E18 (Date
         entity)"""@en ;
.

:Record
    a owl:Class ;
    rdfs:label
        "Record"@en ,
        "Documento"@es ,
        "Objet informationnel"@fr ;
    rdfs:comment """Discrete information content formed and inscribed, at least once,
         by any method on any carrier in any persistent, recoverable form by an Agent in the course
         of life or work activity."""@en ;
    rdfs:isDefinedBy <https://www.ica.org/standards/RiC/ontology> ;
    rdfs:subClassOf :RecordResource ;
    skos:changeNote
        [
            dc:date "2023-11-02" ;
            rdf:value "Added a new rdfs:label in Spanish."@en ;
        ] ,
        [
            dc:date "2023-08-25" ;
            rdf:value "Added a new rdfs:label in French."@en ;
        ] ,
        [
            dc:date "2020-10-23" ;
            rdf:value """Scope note: updated and made several paragraphs. Objective: to
               make RiC-O compliant with RiC-CM v0.2."""@en ;
        ] ,
        [
            dc:date "2021-02-08" ;
            rdf:value "Removed the Restriction."@en ;
        ] ,
        [
            dc:date "2023-11-12" ;
            rdf:value """Aligned with RiC-CM 1.0: updated the description
               (rdfs:comment), skos:scopeNote."""@en ;
        ] ;
    skos:scopeNote """Record is a kind of Record Resource. A Record may itself contain
         one or more Records, or may consist of one or more Record Parts. A Record must have or have
         had at least one Instantiation. A Record may have more than one Instantiation. An
         Instantiation derived from another Instantiation of a Record may be considered the
         instantiation of the same Record or an instantiation of a new Record, depending on the
         context. A Record may serve a variety of purposes, though it always documents or is
         evidence of Activity."""@en ;
    :RiCCMCorrespondingComponent """Corresponds to RiC-E04 (Record
         entity)"""@en ;
.

:isRelatedTo
    a
        owl:ObjectProperty ,
        owl:SymmetricProperty ;
    rdfs:label
        "is related to"@en ,
        "está relacionado con"@es ,
        "est relié à"@fr ;
    rdfs:comment """The most generic relation, is related to, connects any Thing to
         any other Thing. This relation is symmetric."""@en ;
    rdfs:domain :Thing ;
    rdfs:isDefinedBy <https://www.ica.org/standards/RiC/ontology> ;
    rdfs:range :Thing ;
    owl:propertyChainAxiom (
        :thingIsConnectedToRelation
        :relation_role
        :relationConnects
    ) ;
    skos:changeNote
        [
            dc:date "2023-08-28" ;
            rdf:value "Added a new rdfs:label in French."@en ;
        ] ,
        [
            dc:date "2023-11-02" ;
            rdf:value "Added a new rdfs:label in Spanish."@en ;
        ] ,
        [
            dc:date "2023-11-12" ;
            rdf:value """Aligned with RiC-CM 1.0: updated the description
               (rdfs:comment)."""@en ;
        ] ,
        [
            dc:date "2023-11-08" ;
            rdf:value """Added the chain property axiom in order to make this property a
               shortcut."""@en ;
        ] ;
    :RiCCMCorrespondingComponent """RiC-R001 ('is related to'
         relation)"""@en ;
.

:RecordSet
    a owl:Class ;
    rdfs:label
        "Record Set"@en ,
        "Agrupación documental"@es ,
        "Ensemble d’objets informationnels"@fr ;
    rdfs:comment """One or more records that are grouped together by an Agent based on
         the records sharing one or more attributes or relations."""@en ;
    rdfs:isDefinedBy <https://www.ica.org/standards/RiC/ontology> ;
    rdfs:subClassOf :RecordResource ;
    skos:changeNote
        [
            dc:date "2023-08-25" ;
            rdf:value "Added a new rdfs:label in French."@en ;
        ] ,
        [
            dc:date "2023-11-02" ;
            rdf:value "Added a new rdfs:label in Spanish."@en ;
        ] ,
        [
            dc:date "2023-04-19" ;
            rdf:value "Removed the 0.2 existing unnecessary restriction."@en ;
        ] ,
        [
            dc:date "2023-11-12" ;
            rdf:value """Aligned with RiC-CM 1.0: updated the description
               (rdfs:comment), skos:scopeNote."""@en ;
        ] ,
        [
            dc:date "2020-10-23" ;
            rdf:value """comment: updated. Scope note: updated and made several
               paragraphs. Objective: to make RiC-O compliant with RiC-CM v0.2."""@en ;
        ] ;
    skos:scopeNote """Record set is a kind of Record Resource. The member records in a
         Record Set may physically reside together, though physical proximity is not essential. In a
         particular context, an Agent (for example, administrator, records manager, archivist,
         end-user, etc.) may select the member records of a Record Set based on any shared attribute
         or attributes, or any shared relation or relations. The grouping of the records serves a
         purpose or purposes specific to the context of the Agent. For example, all member records
         of a Record Set have been accumulated by the same Agent; have the same Documentary Form
         Type; or are related to and document the same Activity. A Record Set may represent the act
         of classifying the records in accordance with a formal classification scheme that may be
         based on activity, subject, organizational structure, or other criteria; an act of archival
         arrangement (for example, based on common provenance); or some other selection and grouping
         that fulfils a particular purpose or purposes (for example, a classification that reflects
         or supports the purposes of a researcher). By exception, some records are brought together
         based on their not belonging in the context of selection to other designated groups: a
         'Miscellaneous' series, for example. A Record Sset accumulated by an Agent in the course of
         life or work activity should be described in a manner that preserves context and evidential
         value. Record Sets may also contain other Record Sets. A Record Set or Record may
         simultaneously be a member of more than one Record Set, and over the course of its
         existence, a Record Set or Record may be a member of an indeterminate number of Record Sets
         in an indeterminate number of contexts. Record Sets and Records contained within a Record
         Set may be ordered into a sequence based on a common property or relation, or common
         properties or relations (for example, alphabetical by agent or related place);
         chronological order by creation date; or some other criterion (for example, an imposed
         order by relevance)."""@en ;
    :RiCCMCorrespondingComponent """Corresponds to RiC-E03 (Record Set
         entity)"""@en ;
.

:relationHasSource
    a owl:ObjectProperty ;
    rdfs:label
        "relation has source"@en ,
        "relación tiene como fuente"@es ,
        "relation a pour source"@fr ;
    rdfs:comment """Connects an n-ary Relation to a Thing that is its
         source."""@en ;
    rdfs:domain :Relation ;
    rdfs:isDefinedBy <https://www.ica.org/standards/RiC/ontology> ;
    rdfs:range :Thing ;
    rdfs:subPropertyOf :relationConnects ;
    owl:inverseOf :thingIsSourceOfRelation ;
    skos:changeNote
        [
            dc:date "2023-11-02" ;
            rdf:value "Added a new rdfs:label in Spanish."@en ;
        ] ,
        [
            dc:date "2023-08-28" ;
            rdf:value "Added a new rdfs:label in French."@en ;
        ] ;
.

:relationHasTarget
    a owl:ObjectProperty ;
    rdfs:label
        "relation has target"@en ,
        "relación tiene como objetivo"@es ,
        "relation a pour cible"@fr ;
    rdfs:comment """Connects an n-ary Relation to a Thing that is its
         target."""@en ;
    rdfs:domain :Relation ;
    rdfs:isDefinedBy <https://www.ica.org/standards/RiC/ontology> ;
    rdfs:range :Thing ;
    rdfs:subPropertyOf :relationConnects ;
    owl:inverseOf :thingIsTargetOfRelation ;
    skos:changeNote
        [
            dc:date "2023-11-02" ;
            rdf:value "Added a new rdfs:label in Spanish."@en ;
        ] ,
        [
            dc:date "2023-08-28" ;
            rdf:value "Added a new rdfs:label in French."@en ;
        ] ;
.

:Person
    a owl:Class ;
    rdfs:label
        "Person"@en ,
        "Persona"@es ,
        "Personne"@fr ;
    rdfs:comment "An individual human being."@en ;
    rdfs:isDefinedBy <https://www.ica.org/standards/RiC/ontology> ;
    rdfs:subClassOf :Agent ;
    owl:disjointWith :Position ;
    skos:changeNote
        [
            dc:date "2021-02-08" ;
            rdf:value "Removed one Restriction."@en ;
        ] ,
        [
            dc:date "2023-11-12" ;
            rdf:value """Aligned with RiC-CM 1.0: updated the description
               (rdfs:comment), skos:scopeNote."""@en ;
        ] ,
        [
            dc:date "2023-04-19" ;
            rdf:value "Removed the 0.2 existing unnecessary restriction."@en ;
        ] ,
        [
            dc:date "2023-08-25" ;
            rdf:value "Added a new rdfs:label in French."@en ;
        ] ,
        [
            dc:date "2020-10-23" ;
            rdf:value """Scope note: made separate paragraphs and updated. Disjoint
               with: enriched. Objective: to make RiC-O compliant with RiC-CM v0.2."""@en ;
        ] ,
        [
            dc:date "2020-10-23" ;
            rdf:value """Scope note: made separate paragraphs and updated. Disjoint
               with: enriched. Objective: to make RiC-O compliant with RiC-CM v0.2."""@en ;
        ] ,
        [
            dc:date "2023-11-02" ;
            rdf:value "Added a new rdfs:label in Spanish."@en ;
        ] ;
    skos:scopeNote """Person is a kind of Agent. Most commonly, a human being
         (biological person) has a single socially constructed identity or persona. Less common
         though not rare, one or more personae in addition to the original persona which emerges at
         or near birth may be associated with the human being over the course of that human being’s
         lifetime. Such "alternative personae" are most often created by the original person for
         specific purposes. The original persona may, in everyday discourse, be regarded as “the
         real person”. Under some circumstances, an alternative persona might eclipse or replace the
         original person (Mark Twain eclipsing Samuel Clemens; John Wayne eclipsing Marion Mitchell
         Morrison), that is, the alternative identity becomes the predominant identity. Less common
         is when two or more persons collaborate to create a shared persona. A persona shared by two
         or more persons constitutes a kind of group. Within the archival context, the description
         of a person commonly will focus on the original associated persona, with alternative
         personae noted. Exceptionally, an alternative persona may displace the original persona as
         the focus of the description. Under some circumstances, for example, when record resources
         are associated with two or more different personae of one person, describing the different
         personae as separate though related persons may be desirable. Alternatively, a person may
         change their identity over the course of their lifetime."""@en ;
    :RiCCMCorrespondingComponent """Corresponds to RiC-E08 (Person
         entity)"""@en ;
.

:RecordResource
    a owl:Class ;
    rdfs:label
        "Record Resource"@en ,
        "Recurso documental"@es ,
        "Ressource archivistique"@fr ;
    rdfs:comment """Information produced or acquired and retained by an Agent in the
         course of life or work activity."""@en ;
    rdfs:isDefinedBy <https://www.ica.org/standards/RiC/ontology> ;
    rdfs:subClassOf :Thing ;
    skos:changeNote
        [
            dc:date "2023-04-19" ;
            rdf:value "Removed the 0.2 existing unnecessary restriction."@en ;
        ] ,
        [
            dc:date "2023-11-02" ;
            rdf:value "Added a new rdfs:label in Spanish."@en ;
        ] ,
        [
            dc:date "2020-10-23" ;
            rdf:value """Scope note: made separate paragraphs plus very few
               changes."""@en ;
        ] ,
        [
            dc:date "2023-11-12" ;
            rdf:value """Aligned with RiC-CM 1.0: updated the description
               (rdfs:comment), skos:scopeNote."""@en ;
        ] ,
        [
            dc:date "2023-08-25" ;
            rdf:value "Added a new rdfs:label in French."@en ;
        ] ,
        [
            dc:date "2021-02-08" ;
            rdf:value "Removed one Restriction."@en ;
        ] ;
    skos:scopeNote """Record resource is a kind of Thing. Producing a record resource
         may imply either its initial creation or a reuse of previous existing information by
         combination, rearrangement, selecting, reformatting, etc. Record set, record, and record
         part are kinds of record resource. A record resource is evidence of the activity of an
         agent. More than one agent may be involved in the creation of a record resource. The role
         of the agent in creating the record resource may take different forms, for example,
         authoring of an individual record, accumulating a record set, or arranging a record set.
         Though a record, record set, and record part, under most circumstances, may be easily
         distinguished from one another, identifying the boundary of each may frequently present
         particular challenges. Documentary forms provide the rules governing the structure of many
         types of records, providing criteria for identifying a record's boundary, and identifying
         its essential parts. Many records, though, do not have well-established documentary forms,
         particularly in the case of digital records, where it may be difficult to determine whether
         individual elements represented in separate bitstreams are record parts, records, or record
         sets. For example, is photographic information represented independently in a bitstream
         embedded in a text document a record or a record part? Or is the same photographic
         information attached to an email that maintains its independent representation, a record or
         a record part? Information grouped for some purpose, for example, ZIP or TAR "file
         compression" for saving storage space, presents a further challenge. One file comprises
         multiple bitstreams subjected to techniques that remove bits that can be losslessly
         recovered when decompressed. Under what circumstances is such a compressed bitstream a
         record or a record set? Determining when an information object is a record, record set, or
         record part is based on perspective and judgement exercised in a particular context. In one
         context, the agent describing an information object may designate it a record, while
         another agent in a different context may designate it a record part. Both designations are
         supported by RiC-CM, and the significance of the difference for users of the records is
         ameliorated by the fact that all of the attributes and relations employed in describing
         record and record part are shared, as are many of the attributes and relations employed in
         describing a record set."""@en ;
    :RiCCMCorrespondingComponent """Corresponds to RiC-E02 (Record Resource
         entity)"""@en ;
.

:Instantiation
    a owl:Class ;
    rdfs:label
        "Instantiation"@en ,
        "Instanciación"@es ,
        "Instanciation"@fr ;
    rdfs:comment """The inscription of information made by an Agent on a physical
         carrier in any persistent, recoverable form as a means of communicating information through
         time and space."""@en ;
    rdfs:isDefinedBy <https://www.ica.org/standards/RiC/ontology> ;
    rdfs:subClassOf :Thing ;
    skos:changeNote
        [
            dc:date "2023-11-02" ;
            rdf:value "Added a new rdfs:label in Spanish."@en ;
        ] ,
        [
            dc:date "2020-10-23" ;
            rdf:value """Comment: updated. Scope note: updated and made several
               paragraphs. Objective: to make RiC-O compliant with RiC-CM v0.2."""@en ;
        ] ,
        [
            dc:date "2023-04-19" ;
            rdf:value "Removed the 0.2 existing unnecessary restrictions."@en ;
        ] ,
        [
            dc:date "2023-08-25" ;
            rdf:value "Added a new rdfs:label in French."@en ;
        ] ;
    skos:scopeNote """A Record or Record Part must have been instantiated at least
         once, though this instantiation may no longer exist at the moment of description. An
         instantiation might also exist at the moment of description, but be destroyed at a later
         moment in time, when, for example, a derived instantiation might become the only remaining
         instantiation. A Record Set may have an instantiation, which is to say that it is not a
         necessary condition. An Instantiation may be derived from another Instantiation. A Record
         Resource may have many Instantiations simultaneously (for instance, a record printed and
         saved in the same time as DOCX and PDF/A would have 3 concurrent instantiations) or through
         time (for example, copy of a record). Depending on the context, a new instantiation may be
         seen as a new or as the same record resource. During in the process of re-instantiation
         something is lost and something is preserved, but it is up to the context and the Agent
         that produces or uses that Instantiation to assess whether the two instantiations are
         functionally equivalent or not. For instance, a postcard representing a town map from 1874
         (Instantiation 1) is digitized and kept as a JPEG file (Instantiation 2). The digital copy
         may be considered as instantiating the "same" Record by an Agent considering the
         information transmitted by the Record (e.g., the urban landscape displayed), but as a"
         different" Record by an antiquarian more focused on the materiality of the carrier.
         Successive instantiations may change the perceivable boundaries of a Record Resource. For
         instance, a case file comprising many records may be digitized and saved as one single PDF
         file, which, from management perspective, may be treated as one Record. Similarly, a large
         Record Set (a fonds or a series) may be maintained as one database. On the other hand, one
         record (main document and its annexes) may be digitized in separate files and each one may
         be managed as a discrete “physical” item. Instantiations may require mediation to
         communicate the information in the Record Resource. While a traditional Record on paper can
         simply be read by an Agent in order to understand the information, a vinyl recording, a
         video cassette or a digital file needs a device (mediator) to codify or decodify the
         information conveyed. This mediator may imply simple physical components (a turntable
         needle, for example), or a complex gallery of software and hardware elements.
         Instantiations are more than the mere informational content of Record Resource and may be
         the focus of preservation and physical management of records. The use of particular
         document types for records, such as a medieval charter, may have implications for the
         authenticity of the records. Hence, the way a Record Resource is instantiated contributes
         to the contextualizing of the content.record resource is instantiated contributes to the
         contextualizing the content. Distinguishing the message conveyed (Record Resource) and its
         physical representations (Instantiation) allows for the efficient management of their
         descriptions, and preserve information about a Record Resource even when no physical
         representation of it exists or is known to exist anymore. The relations between distinct
         instantiations can then be expressed wherever they coexist, and they can be related to the
         Record Resource they instantiate."""@en ;
    :RiCCMCorrespondingComponent """Corresponds to RiC-E06 (Instantiation
         entity)"""@en ;
    :closeTo "PREMIS Representation"@en ;
.

:Agent
    a owl:Class ;
    rdfs:label
        "Agent"@en ,
        "Agente"@es ,
        "Agent"@fr ;
    rdfs:comment """A Person, or Group, or an entity created by a Person or Group
         (Mechanism), or a Position, that acts in the world."""@en ;
    rdfs:isDefinedBy <https://www.ica.org/standards/RiC/ontology> ;
    rdfs:subClassOf :Thing ;
    skos:changeNote
        [
            dc:date "2023-08-25" ;
            rdf:value "Added a new rdfs:label in French."@en ;
        ] ,
        [
            dc:date "2021-02-08" ;
            rdf:value "removed the Restrictions"@en ;
        ] ,
        [
            dc:date "2020-10-23" ;
            rdf:value """Comment: updated. Scope note: updated and made several
               paragraphs. Objective: to make RiC-O compliant with RiC-CM v0.2."""@en ;
        ] ,
        [
            dc:date "2023-11-02" ;
            rdf:value "Added a new rdfs:label in Spanish."@en ;
        ] ;
    skos:scopeNote """An Agent may have one or more identities; an identity is a
         constellation of properties or relations that together “identify” the Agent. A Person or
         Group commonly has one identity, though each also may have one or more alternative
         identities. Such alternative identities may be shared by more than one Person or Group.
         Alternative identities include but are not limited to pseudonyms, heteronyms, DBA (Doing
         Business As), and trade identities. An alternative identity should not be confused with a
         Position in a Group, for example, presidents, prime ministers, governors, popes, royalty,
         or bishops. Nor should an alternative identity be confused with a variant name or
         identifier of the same identity. Agent also includes entities created by a Person or Group
         that act on behalf of the creating Agent in an autonomous or semi-autonomous manner.
         Examples of a Mechanism include software agents, robots, and space and underwater probes
         that generate data (records) in the course of Activity assigned to and in conformance with
         the instructions given to them by the creating Person or Group."""@en ;
    :RiCCMCorrespondingComponent """Corresponds to RiC-E07 (Agent
         entity)"""@en ;
.

:Thing
    a owl:Class ;
    rdfs:label
        "Thing"@en ,
        "Cosa"@es ,
        "Chose"@fr ;
    rdfs:comment """Any idea, material thing, or event within the realm of human
         experience."""@en ;
    rdfs:isDefinedBy <https://www.ica.org/standards/RiC/ontology> ;
    skos:changeNote
        [
            dc:date "2023-11-02" ;
            rdf:value "Added a new rdfs:label in Spanish."@en ;
        ] ,
        [
            dc:date "2023-08-25" ;
            rdf:value "Added a new rdfs:label in French."@en ;
        ] ,
        [
            dc:date "2020-10-23" ;
            rdf:value "made separate paragraphs in the scope note."@en ;
        ] ;
    skos:scopeNote """Includes all RiC entities as well as any concept, material
         thing, or event that may be the subject of a Record Resource or associated with an
         Activity. Examples of entities not explicitly addressed in RiC includes but is not limited
         to the following: abstract concepts; cultural movements, named periods and events; named
         things, objects and works; legendary, mythical or fictitious figures, characters or
         beings."""@en ;
    :RiCCMCorrespondingComponent """Corresponds to RiC-E01 (Thing
         entity)"""@en ;
.

<https://www.ica.org/standards/RiC/ontology>
    a
        voaf:Vocabulary ,
        owl:NamedIndividual ,
        owl:Ontology ;
    rdfs:label """International Council on Archives Records in Contexts Ontology (ICA
         RiC-O) version 1.0.1"""@en ;
    cc:license <https://creativecommons.org/licenses/by/4.0/> ;
    dc:contributor
        """Regine I. Heberlein (University of Princeton, USA), member of EGAD and EGAD
         RiC-O team from 2023""" ,
        """Aaron Rubinstein (University of Massachusetts Amherst, USA),
         member of EGAD and EGAD RiC-O team from 2012 to 2022"""@en ,
        """Daniel Pitti (University of Virginia, USA), chair of EGAD from
         2012"""@en ,
        """Florence Clavaud (Archives nationales de France), member of EGAD
         and lead of EGAD RiC-O team from 2012"""@en ,
        """Ivo Zandhuis (Consultant Digital Cultural Heritage, The
         Netherlands), member of EGAD and EGAD RiC-O team from 2023"""@en ,
        """Jan Krause-Bilvin (docuteam, Switzerland),
         member of EGAD and EGAD RiC-O team from 2023"""@en ,
        """Miia Herrala (National Archives of Finland), member of EGAD and
         EGAD RiC-O team from 2016 to 2022"""@en ,
        """Richard David Williamson (National Archives of Norway), member
         of EGAD and of EGAD RiC-O team from 2024"""@en ,
        "Tobias Wildi (docuteam, Switzerland), member of EGAD and EGAD RiC-O team from 2019"@en ;
    dc:creator """International Council on Archives Expert Group on Archival
         Description (ICA EGAD)"""@en ;
    dc:publisher "International Council on Archives"@en ;
    dc:rights "Copyright 2019-, International Council on Archives (ICA)"@en ;
    dcterms:abstract """
         <html:div xmlns:html="http://www.w3.org/1999/xhtml" xml:lang="en">
            <html:p>RiC-O (Records in Contexts-Ontology) is an OWL ontology for describing archival
               record resources. As the third part of Records in Contexts standard, it is a formal
               representation of Records in Contexts Conceptual Model (RiC-CM).</html:p>
            <html:p>The current version is <html:strong>v1.0.1</html:strong>; <html:strong>it is
                  compliant with RiC-CM 1.0</html:strong>, which was published by EGAD on November
               30, 2023. Version 1.0.1 follows the release of RiC-O 1.0, dated December 2023, which
               was the first stable and complete version of this ontology, and thus a major
               milestone. Apart from slightly modifying a few details in the introduction, adding the name and ORCID of Richard Williamson as a contributor, and fixing
               a few typos in the documentation of RiC-O 1.0, version 1.0.1 only brings one change:
               it fixes the IRI of 'hasOrHadSomeMemberswithDocumentaryFormType' object property
               (changed to <html:a href="#rico:hasOrHadSomeMembersWithDocumentaryFormType">rico:hasOrHadSomeMembersWithDocumentaryFormType</html:a>).</html:p>
            <html:p>RiC-O provides a generic vocabulary and formal rules for creating RDF datasets
               to describe any kind of archival record resource, whether natively or by transforming
               existing metadata (or generating them from existing archival metadata). It supports
               publishing RDF datasets as Linked Data, querying them using SPARQL, and making
               inferences.</html:p>
         </html:div>
      """^^rdf:XMLLiteral ;
    dcterms:contributor
        <https://orcid.org/0000-0001-6743-9622> ,
        <https://orcid.org/0000-0001-9375-2102> ,
        <https://orcid.org/0000-0001-9938-6502> ,
        <https://orcid.org/0000-0002-0803-8025> ,
        <https://orcid.org/0000-0002-5681-4850> ,
        <https://orcid.org/0000-0003-0165-8341> ,
        <https://orcid.org/0009-0004-3219-2534> ;
    dcterms:description """
         <html:div xmlns:html="http://www.w3.org/1999/xhtml" xml:lang="en" id="introduction">
            <html:h3>Introduction</html:h3>
            <html:p>RiC-O (Records in Contexts-Ontology) is an OWL ontology for describing archival
               record resources. As the third part of Records in Contexts standard, it is a formal
               representation of Records in Contexts Conceptual Model (RiC-CM). This version, which
               is v1.0.1, is the latest official release. It is compliant with RiC-CM v1.0.</html:p>
            <html:p>The following diagram shows the main RiC-CM 1.0 entities and a few relations
               between them: <html:img src="https://github.com/ICA-EGAD/RiC-O/blob/7bc6d5d59ecc85a4b901cc79d649ae50209fd69e/diagrams/diagrams_v1-0/RiC-CM-overview/diagram_RiC-CM-overview-RiC-v1-0.jpg?raw=true" alt="A partial overview of RiC-CM 1.0 main entities" class="diagram"/>
            </html:p>
            <html:div id="design-principles">
               <html:h4>RiC-O design principles</html:h4>
               <html:p>The following design principles were followed when developing RiC-O.</html:p>
               <html:p>
                  <html:strong>1. RiC-O is a domain and reference ontology</html:strong>.</html:p>
               <html:p>RiC-O provides <html:strong>a generic vocabulary and formal rules for
                     creating RDF datasets (or generating them from existing archival metadata) that
                     describe in a consistent way any kind of archival record
                  resource</html:strong>. It supports publishing RDF datasets as Linked Data,
                  querying them using SPARQL, and making inferences using the logic of the
                  ontology.</html:p>
               <html:p>While some projects have built some specific ontologies for describing
                  archives, in 2013 no generic domain ontology existed for the specific needs of the
                  archival community. This is why EGAD decided to develop RiC-O as a part of RiC
                  standard.</html:p>
               <html:p>Apart from this first, main target, <html:strong>RiC-O, as a technical
                     implementation of RiC-CM that also extends and refines it and that includes
                     formal logic, can guide or inspire, in many ways, the development of any tool
                     or system that manages (i.e. stores, enables to edit or processes) and
                     publishes descriptive archival metadata.</html:strong>. Of course, other
                  technical implementations of RiC-CM may be developed later on. Also, the current
                  technical implementations of the former ICA standards, e.g. EAD and EAC-CPF XML
                  schemas, should be made closer to RiC-CM in the future; on this topic, see <html:a href="https://www2.archivists.org/groups/technical-subcommittee-on-encoded-archival-standards-ts-eas">the news and announcements of the Technical Subcommittee on Encoded Archival
                     Standards (TS-EAS) of the Society of American Archivists</html:a>.</html:p>
               <html:p>As RiC-O is a generic, domain ontology, <html:strong>it does not address by
                     itself every specific need or expectation</html:strong> that may occur in every
                  archival institution or project. It is rather <html:strong>a high level
                     framework</html:strong> and an institution or project implementing RiC-O can
                  apply only such a subset of properties as meets their needs, or extend the
                  specification according to their particular requirements, or do both.</html:p>
               <html:p>As a domain ontology, RiC-O, at this stage, does not borrow from other
                  existing ontologies (such as the cultural heritage models – IFLA-LRM and
                  CIDOC-CRM, PREMIS, or PROV-O). It should therefore be easier, for an archival
                  institution or archival project, to understand, implement and maintain RiC-O
                  within its system.</html:p>
               <html:p>Alignment with those and other models, where possible, will be undertaken in
                  a future revision cycle to support the interconnected nature of resource
                  description across the domains. This is of course essential for interconnecting
                  RDF datasets conforming to RiC-O with other datasets, or for using parts of RiC-O
                  in other contexts than the archival or records management realm.</html:p>
               <html:p>
                  <html:strong>2. RiC-O is immediately usable.</html:strong>
               </html:p>
               <html:p><html:strong>This is a key feature</html:strong>. <html:strong>Metadata
                     conforming to superseded ICA standards can be transformed to RiC-O
                     successfully</html:strong>. Converting existing archival metadata created or
                  generated in current information systems and compliant with ICA standards to
                  RDF/RiC-O is possible without losing data or structure.</html:p>
               <html:p>During the ongoing development process of RiC-O, intensive conversion
                  testing, either by hand or using scripts, was conducted on XML/EAD finding aids
                  and XML/EAC-CPF authority records to ensure that RiC-O is usable with existing
                  descriptive metadata. An <html:a href="https://github.com/ArchivesNationalesFR/rico-converter">open source
                     conversion software</html:a> was also developed and made available in April
                  2020.</html:p>
               <html:p>While some existing metadata sets may have a very fine level of granularity
                  and accuracy, already using, for example, controlled vocabularies, or describing
                  curation events separately, often these metadata don’t have the very precise
                  structure that RiC-CM recommends. Even then, such a conversion process remains
                  possible. In order to allow this, RiC-O sometimes provides several methods for
                  representing information (as described below). From this point of view, RiC-O v1.0
                  may be considered a transitional ontology, in which some components may be
                  deprecated later on.</html:p>
               <html:p>The usability of a model also depends on its documentation. RiC-O is
                  documented extensively. The documentation will be reviewed and updated on a
                  continuing basis.</html:p>
               <html:p>
                  <html:strong>3. RiC-O provides a flexible framework</html:strong>.</html:p>
               <html:p>
                  <html:strong>This is a very important principle too</html:strong>. It is related
                  with the usability principle quoted above. Moreover, <html:strong>archival
                     description is flexible by essence</html:strong>. It is quite commonly noted
                  that today the level of granularity of information varies from one finding aid to
                  another (or from one authority record to another), or even within the same finding
                  aid. Some series or agents are described summarily because little is known about
                  them and there is little time for extensive research, while other series, even
                  records, or agents are described in detail; some relations (e.g. that relating to
                  provenance) may be described without any detail while others may be thoroughly
                  documented, as ISAAR(CPF) and EAC-CPF allow it.</html:p>
               <html:p>Being generally flexible, for an OWL ontology, depends first on the
                  polyhierarchical systems of classes and properties it provides. A superproperty or
                  superclass, more general or generic than its subproperties or subclasses, must
                  exist and be available for handling information, while at the same time more
                  accurate subcomponents must be there for handling more accurate description. Also,
                  RiC-O provides methods for describing relations as full entities, as well as
                  direct and short paths between entities.</html:p>
               <html:p>
                  <html:strong>4. RiC-O opens new potential for archival description.</html:strong>
               </html:p>
               <html:p><html:strong>Linked Data tools and interfaces enable end users to go through
                     RDF/RiC-O graphs, query them using SPARQL, and make inferences. This means a
                     completely new way of consulting archival metadata and their multiple
                     contexts.</html:strong> An end user should be able to ask of any given data
                  set, for example, “What are (according to your dataset) the corporate bodies that
                  succeeded a given entity from its end of existence to now (as concerns this given
                  activity)?”, or “what instantiations of this photograph exist?”, or “what are the
                  existing copies of this original charter?”, and get a list of these entities. This
                  means that institutions or projects that invest in the implementation of RiC-O
                  will be able to query their data in ways not possible with the previous ICA
                  standards, and will get new insight into the content and context of their archives
                  that wasn’t visible with the existing ICA-standards. What is more, repositories
                  using RiC-O may infer new assertions from the RDF datasets and link them to other
                  resources outside their institution, thereby amplifying the query and inferencing
                  possibilities manifold.</html:p>
               <html:p>
                  <html:strong>5. RiC-O is extensible.</html:strong>
               </html:p>
               <html:p>Institutions with descriptive needs beyond what RiC-O provides out-of-the-box
                  have the option of extending the ontology by adding new subclasses or
                  subproperties as needed. Also, the concepts defined in existing SKOS vocabularies
                  (e.g. a list of documentary form types) can also be connected to RiC-O based
                  graphs (using the *Type classes, and properties which are in the domain or range
                  of these classes).</html:p>
               <html:p>RiC-O has also the potential to be usable in other contexts than purely
                  archival ones. It can be used to “hook” archival description to descriptive
                  metadata in other domains (e.g. bibliographic or museum metadata). As said above,
                  alignment with other models will be undertaken by EGAD in a future revision cycle,
                  facilitating such connections.</html:p>
            </html:div>
            <html:div id="understanding-RiCO">
               <html:h4>Understanding RiC-O: a quick overview of some features</html:h4>
               <html:div id="fromRiCCM-to-RiCO">
                  <html:h5>From RiC-CM to RiC-O</html:h5>
                  <html:div id="From_RiC-CM_components_to_RiC-O_classes">
                     <html:h6>1. From RiC-CM components to RiC-O classes</html:h6>
                     <html:p><html:strong>Each RiC-CM entity has a corresponding class in
                           RiC-O</html:strong>. These classes are organized according to the same
                        hierarchy as in RiC-CM. Some projects may need very few of them (e.g. Agent,
                        Record Resource and Activity only), while others may need more (e.g.
                        Corporate Body and Person; Record; Place; Organic Provenance
                        Relation).</html:p>
                     <html:p><html:strong>Many classes only exist in RiC-O and not in
                           RiC-CM</html:strong>. These additional classes address special
                        needs:</html:p>
                     <html:ul>
                        <html:li><html:strong>some correspond to RiC-CM attributes</html:strong>,
                           when it may be considered necessary to handle them as full entities. This
                           is the case for <html:a href="#rico:Type">Type</html:a> and its
                           subclasses, that correspond to RiC-CM attributes that contain controlled
                           values, and that can help to articulate RiC-O with external RDF resources
                           like SKOS vocabularies; and also for <html:a href="#rico:Language">Language</html:a>, <html:a href="#rico:Name">Name</html:a> and
                              <html:a href="#rico:Identifier">Identifier</html:a>, that can be
                           considered as full entities and as key linking nodes in a RDF graph. All
                           these classes have been grouped under a <html:a href="#rico:Concept">Concept</html:a> class. </html:li>
                        <html:li><html:strong>some classes have been added in order to provide a
                              more accurate definition and model for some entities</html:strong>.
                              <html:a href="#rico:Place">Place</html:a> thus comes along with a
                              <html:a href="#rico:PhysicalLocation">Physical Location
                           class</html:a>, and with a <html:a href="#rico:Coordinates">Coordinates
                              class</html:a>. A Place is considered both a geographical and
                           historical entity. As a historical entity, among other features, it has a
                           history, and may be preceded or succeeded by other Places. A Place also
                           may have zero to many Physical Location through time (for instance, its
                           boundaries, if it is an administrative area or a country, may change).
                           Each Physical Location may be connected to zero to many Coordinates. This
                           model is quite close to the Linked Places Format (<html:a href="https://github.com/LinkedPasts/linked-places">https://github.com/LinkedPasts/linked-places</html:a>). Another
                           example of such an addition is the <html:a href="#rico:Proxy">Proxy
                              class</html:a>, that represents (stands for) a Record Resource as it
                           exists in a specific Record Set.</html:li>
                        <html:li><html:strong>finally, a system of n-ary classes helps to implement
                              the Relations section of RiC-CM</html:strong>. While these relations
                           also are represented as simple, binary object properties (e.g. <html:a href="#rico:hasOrganicProvenance">hasOrganicProvenance</html:a> that
                           corresponds to RiC-R026 relation), you may need to assign different
                           attributes to a relation, e.g. a date, certainty or description, as it is
                           already possible, and quite often done, in a XML/EAC-CPF file. One of the
                           standard available methods for representing such a documented relation in
                           RDF for now is to use a class. The RDF-star specification, which is being
                           developed by the W3C RDF-DEV Community Group, provides a far simpler
                           method (allowing to consider a triple as the subject or object of another
                           triple; see <html:a href="https://w3c.github.io/rdf-star/">https://w3c.github.io/rdf-star/</html:a>) and is already being used
                           by some tools; however it is not yet a complete W3C standard. Thus, for
                           example, in RiC-O a <html:a href="#rico:OrganicProvenanceRelation">OrganicProvenanceRelation class</html:a> exists. This class may
                           connect one to many Agents to one to many created or accumulated Record
                           Resources or Instantiations, and has some specific object properties
                           (certainty, date, description, source). Back to the <html:a href="#rico:hasOrganicProvenance">hasOrganicProvenance</html:a> object
                           property, let us add that it is formally defined in RiC-O, using OWL 2
                           property chain axiom (see <html:a href="https://www.w3.org/TR/owl2-new-features/#F8:_Property_Chain_Inclusion">https://www.w3.org/TR/owl2-new-features/#F8:_Property_Chain_Inclusion</html:a>),
                           as a ‘shortcut’ for the longer path
                           ‘thingIsSourceOfRelation/organicProvenanceRelation_role/relationHasTarget’,
                           where the intermediate node is an instance of OrganicProvenanceRelation:<html:br/>
                           
                           
                           <html:img src="https://github.com/ICA-EGAD/RiC-O/blob/prepare_1.0.1_version/ontology/current-version/HTML_view/rico_hasOrganicProvenance.png?raw=true" class="code" alt="rico:hasOrganicProvenance object property as a shortcut"/>
                           
                           
                           <html:br/>A triplestore, with the appropriate configuration, may thus
                           infer the direct ‘hasOrganicProvenance’ assertion from this long
                           path.</html:li>
                     </html:ul>
                  </html:div>
                  <html:div id="about_RiC-O_datatype-properties">
                     <html:h6>2. About RiC-O datatype properties (relations whose object is a
                        litteral)</html:h6>
                     <html:p><html:strong>Most of the datatype properties in RiC-O correspond to
                           RiC-CM attributes that contain free, plain text</html:strong>. See for
                        example <html:a href="#rico:generalDescription">rico:generalDescription</html:a>, <html:a href="#rico:history">rico:history</html:a> and <html:a href="#scopeAndContent">rico:scopeAndContent</html:a>.</html:p>
                     <html:p>In many simple usecases it’s sufficent to just use the <html:a href="#rico:identifier">rico:identifier</html:a> or <html:a href="#rico:name">rico:name</html:a> datatype properties. However, in
                        addition to these datatype properties, the Name and Identifier RiC-CM
                        attributes also have corresponding classes (subclasses of <html:a href="#rico:Appellation">rico:Appellation</html:a>). A resource may have
                        several Identifiers (e.g. archival reference code, system number, digital
                        object identifier) or Names and each comes with different attributes; in
                        this case instances of classes are needed.</html:p>
                     <html:p>The Location RiC-CM attribute also has a <html:a href="#rico:PhysicalLocation">rico:PhysicalLocation</html:a>
                        corresponding class (for users who want to use Place, Physical Location and
                        Coordinates for handling places).</html:p>
                     <html:p>As already said too, every RiC-CM attribute that has ‘controlled value’
                        or ‘rule-based’ as a schema value, has a class as corresponding component in
                        RiC-O. <html:strong>However, for these CM attributes that correspond to a
                           RiC-O class, as it is necessary to provide an immediately usable
                           ontology, two supplementary datatype properties exist that allow not to
                           use the classes, at least for a while, if you want to implement RiC-O and
                           create RiC-O/RDF datasets from existing archival metadata without being
                           able to handle URIs for the information you have</html:strong>.</html:p>
                     <html:p>For example, you may not be able to handle and maintain URIs for some
                        controlled values you use in EAD finding aids for carrier types: maybe your
                        information system does not use a vocabulary for this, and you cannot for a
                        while consider these carrier types as full entities. Nevertheless you want
                        to produce RiC-O datasets where every piece of information is kept, and you
                        want to avoid blank nodes. If RiC-O would only provide the Carrier Type
                        class, it would be an issue for you.</html:p>
                     <html:p>So RiC-O provides a <html:a href="#rico:type">rico:type</html:a>
                        datatype property, with range rdfs:literal, which allows you to move
                        forward. For RiC-CM Coordinates attribute, you also have the <html:a href="#rico:geographicalCoordinates">rico:geographicalCoordinates</html:a> datatype property.</html:p>
                     <html:p>These datatype properties have a skos:scopeNote which says (for
                        example) &quot;Provided for usability reasons. May be made deprecated or removed
                        later on. Use only if you don’t use Physical Location and Coordinates
                        classes with Place.&quot;</html:p>
                     <html:p><html:strong>The same key design principle (RiC-O must be immediately
                           usable) led us to define some datatype properties that would enable users
                           to use RiC-O in simple usecases where they do not want to consider dates
                           and rules as full entities</html:strong>. Thus, there of course is Date
                        and Rule classes in RiC-O (since there are Date and Rule entities in
                        RiC-CM). And <html:strong>you also have a <html:a href="#rico:date">rico:date</html:a> datatype property, which has several
                           subproperties; plus a <html:a href="#rico:ruleFollowed">rico:ruleFollowed</html:a> datatype property</html:strong>. The same
                        analysis led us to keep the <html:a href="#rico:history">rico:history</html:a> datatype property in RiC-O (same as RiC-CM history
                        attribute), while RiC-CM and RiC-O also provide the <html:a href="#rico:Event">Event</html:a> class, and using a series of Events may
                        of course be a better method, easier to query, link and display, than simply
                        using a history prose discourse. The two methods may be used in parallel
                        within the same dataset by an institution that, for example, would decide to
                        emphasize only the accession, appraisal and description events among the
                        whole history of Record Resources.</html:p>
                     <html:p>These datatype properties have the same kind of skos:scopeNote as
                        above.</html:p>
                     <html:p>Finally, <html:strong>we have introduced a few datatype properties that
                           do not correspond to any RiC-CM attribute</html:strong>.</html:p>
                     <html:p>Some are superproperties, and thus group datatype properties: <html:a href="#rico:physicalOrLogicalExtent">rico:physicalOrLogicalExtent</html:a>, with rico:carrierExtent,
                        rico:instantiationExtent and rico:recordResourceExtent as subproperties;
                           <html:a href="#rico:textualValue">rico:textualValue</html:a>, with
                        rico:expressedDate, rico:normalizedValue and rico:quantity as subproperties;
                           <html:a href="#rico:measure">rico:measure</html:a>; <html:a href="#rico:referenceSystem">rico:referenceSystem</html:a>.</html:p>
                     <html:p>Some are simply more specific properties: <html:a href="#rico:accrualsStatus">rico:accrualsStatus</html:a>; <html:a href="#rico:recordResourceStructure">rico:recordResourceStructure</html:a> and <html:a href="#rico:instantiationStructure">rico:instantiationStructure</html:a>,
                        subproperties of rico:structure; <html:a href="#rico:title">rico:title</html:a> (subproperty of rico:name); rico:altitude,
                        rico:height, rico:latitude, rico:length, rico:longitude, rico:width
                        (subproperties of <html:a href="#rico:measure">rico:measure</html:a>),
                        rico:geodesicSystem and rico:altimetricSystem (subproperties of <html:a href="#rico:referenceSystem">rico:referenceSystem</html:a>).</html:p>
                  </html:div>
                  <html:div id="about_RiC-O_object-properties">
                     <html:h6>3. About RiC-O object properties (relations between two
                        entities)</html:h6>
                     <html:p>In order to connect all the classes created, <html:strong>a significant
                           number of object properties have been defined, in addition to the 85
                           relations defined in RiC-CM 1.0.</html:strong></html:p>
                     <html:p>While the 'flat' list of object properties is a long one,
                           <html:strong>the object properties are grouped
                           hierarchically</html:strong>, so that one can use the upper to
                        intermediate level ones for simplicity sake, or choose the most accurate and
                        expressive ones, or extend the system adding a subproperty easily. It is
                        expected that, in most use cases, a subset of these properties only will be
                        needed.</html:p>
                     <html:p>Below we just give a few details on certain specific sets of
                        properties.</html:p>
                     <html:p>While in RiC-CM it was not possible to achieve such a level of
                        precision with simple attributes, <html:strong>RiC-O includes object
                           properties to assert that a <html:a href="#rico:RecordSet">rico:RecordSet</html:a> has or had members (either all of them, or
                           some of them) that share some characteristics</html:strong>, i.e.
                        Language, ContentType, DocumentaryFormType, LegalStatus, or RecordState. See
                        for example <html:a href="#rico:hasOrHadAllMembersWithCategory">rico:hasOrHadAllMembersWithCategory</html:a>, and its
                        subproperties.</html:p>
                     <html:p><html:strong>Some of the object properties are formally defined as
                           shortcuts</html:strong>: they can be inferred if you create triples that
                        include instances of the Relation classes. See the example explained above
                        in the <html:a href="#RiC-O_classes">section dedicated to
                        classes</html:a>.</html:p>
                     <html:p><html:strong>Many properties, new in RiC-O 1.0, are transitive or
                           reflexive</html:strong>, as explained in the <html:a href="#history-note">history note</html:a> above.</html:p>
                  </html:div>
                  <html:div id="named-individuals">
                     <html:h6>4. Named Individuals</html:h6>
                     <html:p>RiC-O adds six individuals to address current and frequent
                        needs:</html:p>
                     <html:ul>
                        <html:li><html:a href="#FindingAid">FindingAid</html:a> and <html:a href="#AuthorityRecord">AuthorityRecord</html:a>, which are instances
                           of both RiC-O Documentary Form Type and SKOS Concept. They can be used
                           for categorizing Records, finding aids and authority records being
                           considered as Records. For example, a Record with Documentary Form Type
                           ‘Finding Aid’ may be connected to one to many Record Resources using the
                           'rico:describes’ object property. </html:li>
                        <html:li><html:a href="#Fonds">Fonds</html:a>, <html:a href="#Series">Series</html:a>, <html:a href="#File">File</html:a>, and <html:a href="#Collection">Collection</html:a> are instances of both Record
                           Set Type class and skos:Concept. Their definition is taken from the
                           ISAD(G) glossary. They can be used for categorizing Record
                           Sets.</html:li>
                     </html:ul>
                     <html:p>We expect other categories to be defined by the archival community as
                        RiC-O matures, forming rich, hopefully multilingual, SKOS vocabularies that
                        support rich description (for example, allowing an instance of the <html:a href="#rico:DocumentaryFormType">Documentary Form Type class</html:a> to
                        have a history and temporal relations to other documentary form
                        types).</html:p>
                  </html:div>
               </html:div>
               <html:div id="RiCO-documentation">
                  <html:h5>RiC-O documentation and annotation properties</html:h5>
                  <html:p>Each class or property has an English, a French and a Spanish label
                     (rdfs:label), and a description (rdfs:comment). Some also have a skos:scopeNote
                     or a skos:example.</html:p>
                  <html:p>When a RiC-O class or property corresponds to a RiC-CM component in any
                     way, its description and scope note are either the same as or derived from
                     their RiC-CM definition and scope note.</html:p>
                  <html:p>RiC-O provides two annotation properties (subproperties of rdfs:comment)
                     for handling:</html:p>
                  <html:ul>
                     <html:li>information about the corresponding RiC-CM component when applicable
                           (<html:a href="#rico:RiCCMCorrespondingComponent">rico:RiCCMCorrespondingComponent</html:a>). Various phrasings are used
                        in this property depending on the rule applied for defining the RiC-CM
                        component.</html:li>
                     <html:li>information about possible mappings with other models or ontologies
                           (<html:a href="#rico:closeTo">rico:closeTo</html:a>, rarely used in this
                        1.0.1 version)).</html:li>
                  </html:ul>
                  <html:p>Any change in the definition of a class or property made since December
                     2019 is documented using a skos:changeNote.</html:p>
               </html:div>
            </html:div>
            <html:div id="next-steps">
               <html:h4>Next steps</html:h4>
               <html:p>The following is a non exhaustive list of known issues, topics or tasks on
                  which EGAD has begun to work and will continue to work in the next
                  months.</html:p>
               <html:ul>
                  <html:li>articulate the Event and Activity classes, and the Relation system of
                     classes</html:li>
                  <html:li>add suggestions of mappings (in rico:closeTo) and OWL equivalences
                     between some classes or properties and components in other models (among which
                     - this is not an exhaustive list- PREMIS, Schema.org, PROV-O, IFLA-LRM and RDA,
                     CIDOC-CRM), or document how these models can be used together. </html:li>
               </html:ul>
            </html:div>
         </html:div>
      """^^rdf:XMLLiteral ;
    dcterms:publisher <http://www.wikidata.org/entity/Q1421986> ;
    dcterms:title """International Council on Archives Records in Contexts Ontology
         (ICA RiC-O) version 1.0.1"""@en ;
    vann:preferredNamespacePrefix "rico" ;
    vann:preferredNamespaceUri "https://www.ica.org/standards/RiC/ontology#" ;
    owl:incompatibleWith <https://raw.githubusercontent.com/ICA-EGAD/RiC-O/master/ontology/previous-versions/RiC-O_v0-2_release/RiC-O_v0-2.rdf> ;
    owl:priorVersion
        <https://raw.githubusercontent.com/ICA-EGAD/RiC-O/master/ontology/previous-versions/RiC-O_v0-2_release/RiC-O_v0-2.rdf> ,
        <https://raw.githubusercontent.com/ICA-EGAD/RiC-O/master/ontology/previous-versions/RiC-O_v1-0-beta_release/RiC-O_1-0-beta.rdf> ,
        <https://raw.githubusercontent.com/ICA-EGAD/RiC-O/master/ontology/previous-versions/RiC-O_v1-0_release/RiC-O_1-0.rdf> ;
    owl:versionInfo "Version 1.0.1 - 2024-05-13."@en ;
    skos:historyNote """
         <html:div xmlns:html="http://www.w3.org/1999/xhtml" xml:lang="en">
            <html:div id="history-note">
               <html:h3>History note</html:h3>
               <html:p>A first beta version of RiC-O was developed in 2017 and used by the National
                  Archives of France for building a proof of concept (<html:a href="https://piaaf.demo.logilab.fr">https://piaaf.demo.logilab.fr</html:a>).</html:p>
               <html:p>EGAD continued to develop the ontology, and this process entered a very
                  active period in 2019, while RiC-CM v0.2 was being designed and edited. From
                  December 2018 to November 2019, about 65 persons that responded to a call for
                  reviewers, received successive beta versions of RiC-O and sent a few first
                  comments. While EGAD RiC-O team could not answer to each of these comments, each
                  was taken into account. RiC-O v0.1 was released on December 2019, at the same time
                  as RiC-CM v0.2 preview.</html:p>
               <html:p>The Git repository that is used for handling RiC-O was made public in March
                  2020 (see <html:a href="https://github.com/ICA-EGAD/RiC-O">https://github.com/ICA-EGAD/RiC-O</html:a>).</html:p>
               <html:p>In 2020, RiC-CM v0.2 preview was significantly updated: the textual
                  definitions of many entities were changed, as well as the specifications of many
                  attributes; and the IRIs of lot of relations were changed, in order to take into
                  account past situations and to adopt some simple naming rules. As a consequence,
                  RiC-O had to be updated in order to remain compliant with RiC-CM. These changes
                  could not be made before the end of 2020, when RiC-CM could be considered stable.
                  EGAD also decided to make other changes in RiC-O, among which the most important
                  are mentioned in bold in the following list.</html:p>
               <html:p>RiC-O 0.2 results from these updates and changes. It was released in February
                  2021, and is fully compliant with RiC-CM 0.2, which was released in July
                  2021.</html:p>
               <html:p>
                  <html:strong>At the end of 2022</html:strong>, while the EGAD group, as part of
                  the development of version 1.0 of RiC-CM, was working on analyzing and taking into
                  account the very numerous comments relating to RiC-CM 0.2 received, <html:strong>a
                     new active phase of development started for RiC-O. A team of no longer three,
                     but six people prepared this version.</html:strong> It was then absolutely not
                  a question of breaking with the principles and methods already used; the work was
                  a continuation of what had already been done. It was a matter of
                     <html:strong>improving what had already been done, by simplifying wherever
                     possible the specifications, by adding some properties and taking into account
                     the needs that a growing community of users was expressing</html:strong>. On
                  the other hand, it was obviously a question of <html:strong>making RiC-O 1.0
                     compliant with RiC-CM 1.0</html:strong>.</html:p>
               <html:p>As the result of this work, RiC-O 1.0.1 defines:</html:p>
               <html:ul>
                  <html:li>
                     <html:strong>105 classes</html:strong>, one less than in v0.2. As in RiC-CM
                     1.0, the modeling of dates has been modified, this led to the removal of the
                     three subclasses of <html:a href="#rico:Date">rico:Date</html:a>. It was
                     necessary to add a <html:a href="#rico:MandateType">rico:MandateType</html:a>
                     class, corresponding to the new RiC-A44 Mandate Type attribute of RiC-CM 1.0. A
                     generic <html:a href="#rico:OrganicOrFunctionalProvenanceRelation">rico:OrganicOrFunctionalProvenanceRelation</html:a> class was also
                     added.</html:li>
                  <html:li>
                     <html:strong>61 datatype properties</html:strong>, one less than in v0.2.
                     Several properties were renamed, to make the ontology compliant with RiC-CM 1.0
                     (so rico:descriptiveNote has become <html:a href="#rico:generalDescription">rico:generalDescription</html:a>, whose definition is a little different).
                     A <html:a href="#rico:length">rico:length</html:a> property was added;
                     rico:calendar and rico:dateStandard were removed. The hierarchy of <html:a href="#rico:date">rico:date</html:a> subproperties was revised. Some
                     properties were made subproperties of others (like <html:a href="#rico:scopeAndContent">rico:scopeAndContent</html:a>, now a
                     subproperty of <html:a href="#rico:generalDescription">rico:generalDescription</html:a>).</html:li>
                  <html:li>
                     <html:strong>400 object properties</html:strong>, compared to 423 in RiC-O 0.2.
                     This simple count poorly accounts for <html:strong>the significant
                        modifications that were made to the object properties of RiC-O
                        0.2</html:strong>. <html:br/>On the one hand, <html:strong>a certain number
                        of properties were added to make RiC-O compliant with RiC-CM
                        1.0</html:strong>: addition of properties whose domain or range are <html:a href="#rico:Date">rico:Date</html:a> or <html:a href="#rico:Event">rico:Event</html:a>; addition of <html:a href="#rico:hasOrHadMandateType">rico:hasOrHadMandateType</html:a> and <html:a href="#rico:isOrWasMandateTypeOf">rico:isOrWasMandateTypeOf</html:a>,
                     properties related to the new <html:a href="#rico:MandateType">rico:MandateType</html:a> class. On the other hand, <html:strong>to meet
                        the needs expressed by RiC-O users, other properties were
                        added</html:strong>: <html:a href="#rico:isAgentAssociatedWithPlace">rico:isAgentAssociatedWithPlace</html:a>, <html:a href="#rico:isOrWasEmployerOf">rico:isOrWasEmployerOf</html:a>, <html:a href="#rico:wasMergedInto">rico:wasMergedInto</html:a>, <html:a href="#rico:wasSplitInto">rico:wasSplitInto</html:a>, <html:a href="#rico:hasDeathPlace">rico:hasDeathPlace</html:a>, <html:a href="#rico:hasBirthPlace">rico:hasBirthPlace</html:a>, <html:a href="#rico:hasOrHadAnalogueInstantiation">rico:hasOrHadAnalogueInstantiation</html:a>, <html:a href="#rico:hasOrHadDigitalInstantiation">rico:hasOrHadDigitalInstantiation</html:a>, and their inverse properties.
                     <html:br/>Furthermore, <html:strong>a significant number of properties were
                        added to allow the expression of indirect relationships</html:strong>. Thus,
                     it is now possible, for instance, to specify that a <html:a href="#rico:Record">rico:Record</html:a> is included indirectly in a <html:a href="#rico:RecordSet">rico:RecordSet</html:a> such as a fonds, using
                        <html:a href="#rico:isIncludedInTransitive">rico:isIncludedInTransitive</html:a>, or to infer this relation, which is
                     the super property of the new <html:a href="#rico:isDirectlyIncludedIn">rico:isDirectlyIncludedIn</html:a> property. <html:strong>The addition of
                        such transitive properties concerned partitive (sub-properties of <html:a href="#rico:hasOrHadPart">rico:hasOrHadPart</html:a>), sequential
                        (sub-properties of <html:a href="#rico:precedesOrPreceded">rico:precedesOrPreceded</html:a>) and authority (sub-properties of
                           <html:a href="#rico:hasOrHadSubordinate">rico:hasOrHadSubordinate</html:a>) relations</html:strong>, and the
                     inverse properties. It was accompanied by the creation of properties specifying
                     past relations. <html:br/> Finally, <html:strong>in order to simplify their
                        maintenance, the n-ary Relation classes were rolified</html:strong>. 48 new
                     reflexive object properties were created to do this, such as for example
                        <html:a href="#rico:leadershipRelation_role">rico:leadershipRelation_role</html:a>; the definition of n-ary Relation
                     classes (such as <html:a href="#rico:LeadershipRelation">rico:LeadershipRelation</html:a>) was revised to introduce an equivalence
                     with these properties when they have the same source and the same target, and
                     the chain property axioms of the corresponding binary properties (such as
                        <html:a href="#rico:hasOrHadLeader">rico:hasOrHadLeader</html:a>) were
                     revised. 166 object properties, which existed in RiC-O 0.2 and were specific to
                     each of the n-ary relations, could then be deleted. A full accounting of the
                     rolification of n-ary relations may be found at <html:a href="https://github.com/ICA-EGAD/RiC-O/issues/67">https://github.com/ICA-EGAD/RiC-O/issues/67</html:a>).</html:li>
               </html:ul>
               <html:p>RiC-O 1.0.1 therefore presents itself as an ontology that is
                     <html:strong>more compact than RiC-O 0.2, while being richer, technically
                     opening up new possibilities (with transitive relations) and preserving the
                     semantics defined previously</html:strong>.</html:p>
               <html:p>Besides, an effort has been made regarding the documentation of the ontology.
                  In particular, <html:strong>the labels of each class and property (rdfs:label
                     annotations) are now available in French and Spanish as well as in
                     English</html:strong>. We would like to thank our French-speaking and
                  Spanish-speaking colleagues, members or not of the ICA/EGAD group, who contributed
                  to this translation work.</html:p>
               <html:p>Various bugs have been fixed and the OWL file has been systematically reread
                  many times.</html:p>
               <html:p>A running list of changes since v0.1 may be found in <html:a href="#appendix-I">Appendix I</html:a>. <html:strong>Note that from October
                     2020 any change on a component is described and dated in the specification of
                     this component, using skos:changeNote</html:strong>.</html:p>
            </html:div>
            <html:div id="appendix-I">
               <html:h3>Appendix I: list of the changes made since the release of RiC-O
                  v0.1</html:h3>
               <html:p>The following is a list of the changes made to RiC-O since the release of
                  RiC-O v0.1 in December 2019. The most important changes are mentioned in bold.
                     <html:strong>Note that from October 2020 any change on a component is described
                     and dated in the specification of this component, using
                     skos:changeNote</html:strong>.</html:p>
               <html:ul>
                  <html:li>Fixed a bug in the documentation of rico:PerformanceRelation and its
                     object properties.</html:li>
                  <html:li>Renamed the file and updated the ontology metadata.</html:li>
                  <html:li>OccupationType made a subclass of ActivityType.</html:li>
                  <html:li>Changed the domain and range of rico:hasOriginal and rico:hasDraft (it is
                     now Record or Record Part); same for their inverse properties.</html:li>
                  <html:li>Fixed a bug in the definition of rico:provenanceRelationHasTarget
                     (removed the owl:propertyChainAxiom).</html:li>
                  <html:li>Changed the name of rico:leadBy object property (grammatical mistake) to
                     rico:ledBy. </html:li>
                  <html:li>2020, October 19: Added a vann:preferredNamespaceUri and
                     vann:preferredNamespacePrefix property to the ontology metadata</html:li>
                  <html:li>2020, October 19 : created RuleType and IdentifierType classes, along
                     with the associated object properties.</html:li>
                  <html:li>2020, October 23: <html:strong>updated the text definition and/or scope
                        note of 33 classes, that correspond to RiC-CM entities or attributes, in
                        order to make them compliant with RiC-CM v0.2</html:strong>. Added a few
                     owl:disjointWith properties.</html:li>
                  <html:li>2020, November 1: <html:strong>updated the text definition and/or scope
                        note of, and/or added examples for, 27 datatype properties, that correspond
                        to RiC-CM attributes, in order to make them compliant with RiC-CM
                        v0.2</html:strong>.</html:li>
                  <html:li>2020, November 20: <html:strong>created new classes and properties for
                        handling an accurate description of instantation and record resource
                        extent</html:strong>: Extent, Carrier Extent, Instantiation Extent, Record
                     Resource Extent, Unit of measurement, Extent Type classes; unit of measurement
                     and quantity datatype properties; has Extent, is Extent Of, has Extent Type, is
                     Extent Type Of, has Unit Of Measurement, is Unit of Measurement Of, object
                     properties.</html:li>
                  <html:li>2020, December 28: changed the IRIs and definition of RecordResourceState
                     class and of the associated object properties; <html:strong>changed the domain
                        or ranges and textual definitions of properties associated with Language,
                        LegalStatus, ContentType, DocumentaryFormType; added new object properties
                        for handling the description of some or all members of Record
                        Set</html:strong>. Added the corresponding change notes.</html:li>
                  <html:li>2020, December 29: deleted the isSuperiorTo and isInferiorTo object
                     properties, as well as the AgentSubordinationRelation and its object properties
                     (as the RiC-R043 relation has been removed from RiC-CM 0.2). Added the
                     hasAuthor/isAuthorOf object properties, plus an AuthorshipRelation class and
                     its specific object properties (as the RiC-R079 relation has been added to
                     RiC-CM 0.2). Added the corresponding change notes.</html:li>
                  <html:li>2021, January 22: <html:strong>changed the IRI, label, and/or
                        superproperties or inverse property IRI, and/or textual definition, and/or
                        domain or range, of 152 object properties. Among them, changed the IRI of
                        119 object properties; 85 correspond to RiC-CM relations whose name has been
                        changed in RiC-CM 0.2</html:strong>. Added the corresponding change
                     notes.</html:li>
                  <html:li>2021, January 27: added an rdfs:isDefinedBy to the specification of each
                     RiC-O class and property and made the last changes to the ontology metadata
                     (mainly in the history note).</html:li>
                  <html:li>2021, February 1: last small changes in the ontology metadata (mainly in
                     the abstract).</html:li>
                  <html:li>2021, February 1: 'hasOrHadPhysicalLocation' made a subproperty of
                     'isPlaceAssociatedWith'; 'isOrWasPhysicalLocationOf' made a subproperty of
                     'isAssociatedWithPlace'.</html:li>
                  <html:li>2021, February 1: reordered everything with Protégé without changing the
                     content</html:li>
                  <html:li>2021, February 4: checked and fixed the language of the
                     examples.</html:li>
                  <html:li>2021, February 8: removed a few Restriction classes
                     (rdfs:subClassOf/owl:Restriction) in the definition of classes; completed the
                     textual definition and scope note of the Relation class.</html:li>
                  <html:li>2021, February 9: added a link to RiC-CM 0.2 diagram overview in the
                     introduction; fixed some typos.</html:li>
                  <html:li>2021, February 11: added an @xml:lang='en' on a few labels; updated the
                     definition (rdfs:comment) and scope note of the Rule class, as they were
                     recently changed in RiC-CM 0.2 full draft.</html:li>
                  <html:li>2023, April 17: renamed the file (moving to RiC-O 1.0) and started to
                     update the ontology metadata.</html:li>
                  <html:li>2023, April 19: <html:strong>removed the unnecessary restrictions
                        specified for a significant number of classes</html:strong>, among which
                     most of the subclasses of Type, plus Activity, AgentTemporalRelation,
                     Coordinates, CreationRelation, Event, Identifier, Instantiation,
                     MandateRelation, Person, PhysicalLocation, Place, RecordResource, RecordSet,
                     Rule.</html:li>
                  <html:li>2023, April 21: removed an unnecessary restriction that remained on
                     Mandate class.</html:li>
                  <html:li>2023, end of May-June 5: fixed some typos in the introduction and
                     definition of entities, including the use of &quot;data property&quot; term instead of
                     the correct &quot;datatype property&quot; one.</html:li>
                  <html:li>2023, June 5: <html:strong>made includesOrIncluded object property a
                        subproperty of hasOrHadPart in addition to
                        isRecordResourceAssociatedToRecordResource</html:strong>.</html:li>
                  <html:li>2023, June 21: <html:strong>added two object properties, sub-properties
                        of hasSuccessor: wasMergedInto and wasSplitInto</html:strong>, with
                     Corporate Body as domain and range, and their inverse ones.</html:li>
                  <html:li>2023, July 25: adjusted definition of hasOrHadLanguage</html:li>
                  <html:li>2023, August 25: added French labels to the descriptions of classes and
                     of datatype properties</html:li>
                  <html:li>2023, August 28: added French labels to the descriptions of 250 object
                     properties; added an xml:lang attribute with value 'en' on rdfs:comment when it
                     was missing. Also added French labels to the two RiC-O annotation properties
                     and to the few named individuals already defined.</html:li>
                  <html:li>2023, August 28: changed the domain of hasExtent (from Instantiation or
                     RecordResource to Thing), same for the range of isExtentOf; added a length
                     datatype property under measure.</html:li>
                  <html:li>2023, August 29: <html:strong>updated hasInstantiation and
                        hasDerivedInstantiation</html:strong>, and the inverse properties (changed
                     their IRIs, labels, definitions, inverse properties, according to RiC-CM 1.0).
                     As a consequence, also updated the superproperties of migratedInto and
                     migratedFrom. <html:strong>Created four new object properties:
                        hasOrHadDigitalInstantiation, hasOrHadAnalogueInstantiation, and the inverse
                        ones</html:strong>.</html:li>
                  <html:li>2023, August 29: fixed some typos in the English labels of a few object
                     properties and added the past tense to the English label of
                     hasOrHadCoordinates.</html:li>
                  <html:li>2023, September 13: added 54 new object properties under 'hasorhadpart',
                     in order to extend the following nine existing properties:
                     'containsOrContained', 'hasOrHadComponent', 'hasOrHadConstituent',
                     'includesOrIncluded', 'hasOrHadSubdivision', 'hasOrHadSubevent'. Also did the
                     same for 'followsInTime', 'followsOrFollowed', 'isOrWasSubordinateto'. For each
                     listed property, one was added to express past partitive relations, and 2 other
                     ones for present partitive relations, the first one being transitive and the
                     superproperty of the second one. Added the inverse properties as well. Made
                     'hasDescendant' and 'hasAncestor' transitive.</html:li>
                  <html:li>2023, September 20: <html:strong>began to review and adjust the object
                        properties added on September 13, starting with the properties under
                        hasOrHadPart, and under the inverse isOrWasPartOf property. Among the
                        changes made: adjusted the change notes, added a few 'this is a transitive
                        relation' when missing in the rdfs:comment, and fixed the hierarchy of the
                        properties. Also, every past relation (e.g. contained) also made a
                        subproperty of hadPart. Every current transitive relation (e.g.
                        containsTransitive) made a subproperty of hasPartTransitive. Every current
                        direct relation (e.g. directlyContains) made a subproperty of
                        hasDirectPart</html:strong>. Fixed a syntaxic bug on the ontology history
                     note.</html:li>
                  <html:li>2023, September 22: finished to check and fix the object properties added
                     on September 13, working on hasOrHadSubordinate/isOrWasSubordinateTo
                     subproperties and on precedesOrPreceded/followsOrFollowed
                     subproperties.</html:li>
                  <html:li>2023, September 22: <html:strong>removed DateSingle, DateRange, DateSet
                        and added datatype and properties for dates</html:strong>.</html:li>
                  <html:li>2023, October 10: began to complete the updates made for date and its
                     properties. work done for Date Type, hasDateType, is dateTypeOf, expressedDate,
                     normalizedDateValue and dateQualifier. Also made isCreationDateOfMostMembersOf
                     a subproperty of isCreationDateOfSomeMembersOf; same for the inverse object
                     properties.</html:li>
                  <html:li>2023, October 12: <html:strong>finished to complete the updates made for
                        date and its properties</html:strong>. updated isCreationDateOf,
                     isCreationDateOfSomeMembersOf, isCreationDateOfMostMembersOf,
                     isCreationDateOfAllMembersOf, isPublicationDateOf and the inverse properties.
                     Also, renamed isDeletionDateOf into isDestructionDateOf, and applied the same
                     change to hasDeletiondate. Created isOccurrenceOf, isWithin, intersects ant the
                     inverse properties.</html:li>
                  <html:li>2023, October 13: adjusted a few details on date object properties
                     (renamed some of them to correct the spelling or take past members of record
                     sets into account; added a few subPropertyOf; adjusted the annotations
                     accordingly). Fixed a syntax problem on the history note of the
                     ontology.</html:li>
                  <html:li>2023, October 14: reintroduced the certainty datatype property with
                     domain Event and Relation. Adjusted a few details in the annotations of the
                     date properties.</html:li>
                  <html:li>2023, October 16: fixed several bugs while resolving conflicts before
                     merging, including bad IRIs.</html:li>
                  <html:li>2023, October 17: made occurredAtDate and isDateOfOccurenceof
                     subproperties of isEventAssociatedWith and isAssociatedWithEvent</html:li>
                  <html:li>2023, October 19: made rico:wasUsedFromDate and rico:wasUsedToDate (and
                     its inverses) sub-properties of rico:hasBeginningDate and rico:hasEndDate (and
                     its inverses) respectively</html:li>
                  <html:li>2023, October 19: added RecordPart to domain of hasOrHadConstituent and
                     to the range of the inverse property as well.</html:li>
                  <html:li>2023, October 20: <html:strong>created the following new properties
                        isAgentAssociatedWithPlace, hasDeathPlace, hasBirthPlace,
                        agentHasOrHadLocation, hasOrHadEmployer and their inverse
                        properties</html:strong> as well.</html:li>
                  <html:li>2023, October 26: added Record Part to the domain of hadOrhadConstituent
                     subproperties, and RecordPart to the range of the inverse ones. Changed the
                     definitions of these properties accordingly. Fixed a bug in the history note of
                     the ontology. Regenerated the inverse properties.</html:li>
                  <html:li>2023, October 26: changed the domain and range of 'is or was employer
                     of', removed 'has or had member' super-property of the propertyn added an
                     rdfs:comment to it. Same for the inverse property.</html:li>
                  <html:li>2023, October 26: added rdfs:comments, fixed one IRI, French labels, some
                     domains and range, to the recently added isPlaceAssociatedWithAgent,
                     isBirthPlaceOf, isDeathPlaceOf, isOrWasLocationOfAgent, and their inverse
                     properties. Fixed a bug in the history note of the ontology. Regenerated the
                     inverse properties.</html:li>
                  <html:li>2023, November 2: <html:strong>added Spanish labels to 59 datatype
                        properties, 103 classes and 277 object properties</html:strong>.</html:li>
                  <html:li>2023, November 7: added property chain axioms that were missing, in order
                     to define the following properties as shortcuts: isChildOf, hasOrHadPosition,
                     isOrWasAppellationOf, isOrWasDerivedFromInstantiation, hasOrHadWorkRelationWith
                     and hasGeneticLinkToRecordResource.</html:li>
                  <html:li>2023, November 7: added a hasOrganicOrFunctionalProvenance property,
                     superproperty of documents and of hasOrganicProvenance (new name of
                     hasProvenance); added the shortcut. Same for the inverse property. Added a
                     OrganicAndFunctionalProvenanceRelation, superclass of OrganicProvenanceRelation
                     (new name of AgentOriginationRelation) and ActivityDocumentationRelation;
                     created the needed object properties. Adjusted the names of the properties of
                     OrganicProvenanceRelation.</html:li>
                  <html:li>2023, November 8: <html:strong>rolifying the Relation classes, step
                        1</html:strong>: created 48 reflexive object properties that rolify the
                     classes; modified the specifications of the Relation classes; modified the
                     chain property axioms of the corresponding shortcuts. Fixed the range of
                     isExtentOf.</html:li>
                  <html:li>2023, November 8, later: <html:strong>rolifying the Relation classes,
                        step 2</html:strong>: deleted 166 object properties that had become
                     unnecessary.</html:li>
                  <html:li>2023, November 12: <html:strong>updated the datatype properties in order
                        to make them compliant with RiC-CM 1.0 attributes</html:strong>. Changed the
                     IRIS of accrual (to accruals), accrualStatus (to accrualsStatus),
                     descriptiveNote (to generalDescription), integrity (to integrityNote),
                     physicalCharacteristics (to physicalCharacteristicsNote),
                     qualityOfRepresentation (to qualityOfRepresentationNote). Made scopeAndContent
                     a subproperty of generalDescription, and expressedDate a subproperty of name.
                     Updated or added a few domains and many rdfs:comment, skos:scopeNote,
                     skos:example. Also made usedFromDate a subproperty of beginningDate, and
                     usedToDate a subproperty of endDate.</html:li>
                  <html:li>2023, November 12: <html:strong>updated the classes in order to make them
                        compliant with RiC-CM 1.0 entities and attributes</html:strong>. Updated or
                     added many rdfs:comment and skos:scopeNote, taking into account, as concerns
                     the Relation classes, the fact that they are n-ary. Created a new MandateType
                     class, corresponding to RiC-A44 attribute in RiC-CM 1.0. Also added a
                     rdfs:isDefinedBy to skos:Concept, skos:ConceptScheme and
                     voaf:Vocabulary.</html:li>
                  <html:li>2023, November 12 and 13: <html:strong>updated 35 object properties in
                        order to make them compliant with RiC-CM 1.0 relations. Added labels or
                        modified rdfs:comment of 65 other object properties. Added
                        hasOrHadMandateType and isOrWasMandateType of.</html:strong>
                  </html:li>
                  <html:li>2023, November 13: added or modified a few French or Spanish
                     labels.</html:li>
                  <html:li>2023, November 13: updated the ontology metadata.</html:li>
                  <html:li>2023, November 14: fixed some typos in the ontology metadata.</html:li>
                  <html:li>2023, November 24: started to work on v1.0, after releasing v 1.0-beta:
                     renamed the file and updated a few metadata.</html:li>
                  <html:li>2023, November 25: fixed three French labels; added Spanish labels to the
                     annotation properties and named individuals.</html:li>
                  <html:li>2023, November 27: added Spanish labels to the 93 object properties which
                     were missing one.</html:li>
                  <html:li>2023, December 6: <html:strong>improved the description (rdfs:comment) of
                        the 48 n-ary Relation classes by clearly specifying how they are
                        directed</html:strong>.</html:li>
                  <html:li>2023, December 13: Completed the metadata of the vocabulary: added
                     dc:language, a history note and a scope note.</html:li>
                  <html:li>2023, December 21: <html:strong>revised and updated the ontology metadata
                        and introduction, and the HTML view.</html:strong>.</html:li>
                  <html:li>2023, December 27: in order to make the ontology clearer and more
                     consistent, renamed the certainty and source datatype properties to
                     relationCertainty and relationSource and reduced their domain to Relation.
                     Renamed the 'hasSource' object property to 'isEvidencedBy' and reduced its
                     domain to Relation and range to RecordResource; same for the inverse property,
                     'isSourceOf', renamed to 'evidences'. Updated the specifications of these
                     properties accordingly.</html:li>
                  <html:li>2023, December 27: added rdfs:isDefinedBy to all the properties not
                     defined in RiC-O itself.</html:li>
                  <html:li>2023, December 28: made a few changes in the ontology introduction
                     (dcterms:description) and metadata.</html:li>
                  <html:li>2023, December 29: Added the property chain axiom on
                     'hasCreator'.</html:li>
                  <html:li>2023, December 30: Fixed a typo in five French labels.</html:li>
                  <html:li>2024, February 21: Fixed a typo in the rdfs:comment of rico:RoleType
                     class.</html:li>
                  <html:li>2024, April 10: <html:strong>Fixed the IRI of
                        'hasOrHadSomeMemberswithDocumentaryFormType' object property (changed to
                        'hasOrHadSomeMembersWithDocumentaryFormType')</html:strong> and corrected
                     several typos.</html:li>
                  <html:li>2024, April 12: Replaced the code illustrating the shortcut by an image,
                     change the headers of the subsections in 'From RiC-CM to RiC-O'; added a few
                     details to an sentence in the section on Ric-O properties; adjusted the
                     metadata, mainly moved to v1.0.1.</html:li>
                  <html:li>2024, May 2: Added Richard David Williamson to the list of contributors and set the date of v1.0.1 to May 2, 2024.</html:li>
                  <html:li>2024, May 13: Added Richard Williamson's ORCID number, changed the affiliation of T. Wildi and J. Krause-Bilvin, and set the date of v1.0.1 to May 13, 2024.</html:li>
               </html:ul>
            </html:div>
         </html:div>
      """^^rdf:XMLLiteral ;
.
