PREFIX : <https://linked.data.gov.au/def/cn/>
PREFIX geo: <http://www.opengis.net/ont/geosparql#>
PREFIX model: <https://linked.data.gov.au/def/cn>
PREFIX rdf: <http://www.w3.org/1999/02/22-rdf-syntax-ns#>
PREFIX rdfs: <http://www.w3.org/2000/01/rdf-schema#>
PREFIX owl: <http://www.w3.org/2002/07/owl#>
PREFIX sdo: <https://schema.org/>
PREFIX skos: <http://www.w3.org/2004/02/skos/core#>
PREFIX xsd: <http://www.w3.org/2001/XMLSchema#>

<https://linked.data.gov.au/def/cn>
    a owl:Ontology ;
    owl:versionIRI :0.0.1 ;
    owl:versionInfo "0.0.1" ;
    sdo:codeRepository "https://github.com/AGLDWG/compound-naming-model/"^^xsd:anyURI ;
    sdo:copyrightHolder <https://orcid.org/0000-0002-8742-7730> ;
    sdo:copyrightNotice "(c) Nicholas J. Car, 2023" ;
    sdo:creator <https://orcid.org/0000-0002-8742-7730> ;
    sdo:dateCreated "2023-04-26"^^xsd:date ;
    sdo:dateIssued "2023-04-26"^^xsd:date ;
    sdo:dateModified "2022-04-26"^^xsd:date ;
    sdo:description "This model allows for the representation of compound names that can be assigned to be assigned to features"@en ;
    sdo:license
        "https://creativecommons.org/licenses/by/4.0/"^^xsd:anyURI ,
        <https://rdflicense.linkeddata.es/rdflicense/cc-by4.0> ;
    sdo:name "Compound Naming Model"@en ;
    sdo:publisher <https://www.linked.data.gov.au/org/agldwg> ;
    skos:historyNote """This ontology was made for the Queensland Department of Resources, Spatial Information unit in 2023 to assist with future Address, Place Names, Roads & Cadastre systems design however it is intended to provide background modelling for all ANZ jurisdictions' foundational spatial data.

This model has been made with the FSDF Supermodel in mind (https://linked.data.gov.au/def/fsdf-supermodel) so that is compatible with that, and the Locaiton Index (Loc-I) projects' modelling and goals."""@en ;
.

<https://linked.data.gov.au/org/agldwg>
    a sdo:Organization ;
    sdo:name "Australian Government Linked Data Working Group" ;
    sdo:url "https://www.linked.data.gov.au"^^xsd:anyURI ;
.

<https://orcid.org/0000-0002-8742-7730>
    a sdo:Person ;
    sdo:email "nick@kurrawong.ai"^^xsd:anyURI ;
    sdo:memberOf <https://www.linked.data.gov.au/org/agldwg> ;
    sdo:name "Nicholas J. Car"@en ;
.

:CompoundName
    a owl:Class ;
    rdfs:isDefinedBy model: ;
    skos:definition "A Compound Name is a literal value, or objects that can be interpreted as literal values, that describe or name a Feature"@en ;
    skos:example """# An example Compound Name that is an Address,
# constructed in the manner of Australian street addresses
# and typically rendered for letter sending as:
#
# 72 Yundah Street
# Shorncliffe, QLD, 4017
# Australia
#
PREFIX : <https://linked.data.gov.au/def/cn/>
PREFIX ex: <http://example.com/>
PREFIX rdf: <http://www.w3.org/1999/02/22-rdf-syntax-ns#>
PREFIX rdfs: <http://www.w3.org/2000/01/rdf-schema#>
PREFIX sdo: <https://schema.org/>

ex:72-yundah
    a :CompoundName ;
    rdfs:member [
        sdo:additionalType ex:streetNumber ;
        rdf:value 72 ;
    ] ,
    [
        sdo:additionalType ex:streetName ;
        rdf:value "Yundah" ;
    ] ,
    [
        sdo:additionalType ex:streetType ;
        rdf:value ex:Street ;
    ] ,
    [
        sdo:additionalType ex:locality ;
        rdf:value ex:Shorncliffe ;
    ] ,
    [
        sdo:additionalType ex:state ;
        rdf:value ex:Queensland ;
    ] ,
    [
        sdo:additionalType ex:postCode ;
        rdf:value 4017 ;
    ] ,
    [
        a :CompoundName ;
        sdo:additionalType ex:country ;
        rdf:value ex:aus ;
        sdo:name "Australia" ;
    ] ;
.

# An example Compound Name that is a Geographical Name,
# for an island off the coast of Brisbane, Australia
# that may be rendered as either Moreton Island or perhaps
# Moreton Is.
#
ex:moreton
    a :CompoundName ;
    rdfs:member [
        sdo:additionalType ex:geographicalName ;
        rdf:value "Moreton" ;
    ] ,
    [
        a :CompoundName ;
        sdo:additionalType ex:geographicalName ;
        rdf:value ex:Island ;
        sdo:name "Island" ;
    ] ;
."""@en ;
    skos:prefLabel "Compound Name"@en ;
.

rdfs:Resource
    a owl:Class ;
    rdfs:isDefinedBy rdfs: ;
    skos:definition "The class resource, everything"@en ;
    skos:example """See the non-literal values for rdf:value in the CompoundName example""" ;
    skos:prefLabel "Resource"@en ;
    skos:scopeNote "This class is used to represent both the things to which CompoundNames can be assigned and also the range value of the property rdf:value. It is not expected to be used directly but instead specialised types of Resource are expected"@en ;
.

rdfs:Literal
    a owl:Class ;
    rdfs:isDefinedBy rdfs: ;
    skos:definition "The class of literal values, eg. textual strings and integer"@en ;
    skos:example """See the literals values of '72' and 'Yundah' in the CompoundName example""" ;
    skos:prefLabel "Literal"@en ;
    skos:scopeNote "This class is used to represent the range value of the property :asLiteral. It is not expected to be used directly but instead specialised types of Literal are expected"@en ;
.

skos:Concept
    a owl:Class ;
    rdfs:isDefinedBy skos: ;
    skos:definition "An idea or notion; a unit of thought"@en ;
    skos:example """# See the example for CompoundName and add the following
#
PREFIX ex: <http://example.com/>
PREFIX skos: <http://www.w3.org/2004/02/skos/core#>

ex:Island
    a skos:Concept ;
    skos:inScheme ex:someConceptScheme ;
    skos:prefLabel "Island" ;
    skos:altLabel "Is." ;
.""" ;
    skos:prefLabel "Concept"@en ;
    skos:scopeNote "This class is the type of the expected values for the property sdo:additionalType when used within this model. Concepts are typically controlled terms within ConceptSchemes. Literal representations of Concepts should easily be obtainable"@en ;
.

:isNameFor
    a owl:ObjectProperty ;
    rdfs:isDefinedBy model: ;
    owl:inverseOf sdo:name ;
    skos:example """# Moreton Island is the Compound Name
# for a spatial object off the coast of Brisbane, Australia
#
PREFIX : <https://linked.data.gov.au/def/cn/>
PREFIX ex: <http://example.com/>
PREFIX geo: <http://www.opengis.net/ont/geosparql#>

ex:moreton
    a :CompoundName ;
    :isNameFor ex:feature-x ;
.

ex:feature-x
    a geo:Feature ;
    sdo:name ex:moreton ;
."""@en ;
    skos:prefLabel "is name for"@en ;
.

sdo:name
    a owl:DatatypeProperty ;
    rdfs:isDefinedBy sdo: ;
    skos:definition "The name of the item"@en ;
    skos:example """See example for isNameFor"""@en ;
    skos:prefLabel "name"@en ;
    skos:usageNote "In this model, name is used to indicate both a literal form of a resource`s name or a CompoundName object"
.

sdo:hasPart
    a owl:ObjectProperty ;
    rdfs:isDefinedBy sdo: ;
    skos:definition "Indicates a Resource that is part of this item"@en ;
    skos:example """See the example for CompoundName"""@en ;
    skos:prefLabel "member"@en ;
    skos:scopeNote "Use this property to indicate the individual parts of a Compound Name"@en ;
.

rdf:value
    a owl:ObjectProperty ;
    rdfs:isDefinedBy rdf: ;
    rdfs:range rdfs:Resource ;
    skos:definition "Idiomatic property used for structured values"@en ;
    skos:example """See the example for CompoundLiteral"""@en ;
    skos:prefLabel "value"@en ;
    skos:scopeNote "Use this property to indicate the value of a CompoundName, whether it's a literal or a complex object"@en ;
.

sdo:additionalType
    a owl:ObjectProperty ;
    rdfs:domain rdfs:Resource ;
    rdfs:isDefinedBy sdo: ;
    rdfs:range rdfs:Resource ;
    skos:definition "An additional type for the item, typically used for adding more specific types from external vocabularies"@en ;
    skos:example """See the example for CompoundLiteral"""@en ;
    skos:prefLabel "additional type"@en ;
    skos:scopeNote "Use this property to indicate the specialised type of a part of a CompoundName"@en ;
.
