PREFIX : <https://linked.data.gov.au/def/lifecycle/>
PREFIX model: <https://linked.data.gov.au/def/lifecycle>
PREFIX owl: <http://www.w3.org/2002/07/owl#>
PREFIX rdfs: <http://www.w3.org/2000/01/rdf-schema#>
PREFIX sdo: <https://schema.org/>
PREFIX skos: <http://www.w3.org/2004/02/skos/core#>
PREFIX time: <http://www.w3.org/2006/time#>
PREFIX xsd: <http://www.w3.org/2001/XMLSchema#>

model:
    a owl:Ontology ;
    owl:versionIRI :0.0.1 ;
    owl:versionInfo "0.0.1" ;
    sdo:codeRepository "https://github.com/AGLDWG/lifecycle-model/"^^xsd:anyURI ;
    sdo:copyrightHolder <https://orcid.org/0000-0002-8742-7730> ;
    sdo:copyrightNotice "(c) Nicholas J. Car, 2023" ;
    sdo:creator <https://orcid.org/0000-0002-8742-7730> ;
    sdo:dateCreated "2023-05-30"^^xsd:date ;
    sdo:dateIssued "2023-05-30"^^xsd:date ;
    sdo:dateModified "2023-11-04"^^xsd:date ;
    sdo:description "This model allows for the representation of lifecycle stages for any Resource. The specific stages are expected to be taken from vocabularies relevant to the Resource."@en ;
    sdo:license
        <https://rdflicense.linkeddata.es/rdflicense/cc-by4.0> ,
        "https://creativecommons.org/licenses/by/4.0/"^^xsd:anyURI ;
    sdo:name "Lifecycle Model"@en ;
    sdo:publisher <https://linked.data.gov.au/org/agldwg> ;
    skos:historyNote "This model was made for the Queensland Department of Resources, Spatial Information unit in 2023 to assist with the lifecylcing of components within multiple ontologies."@en ;
.

<https://linked.data.gov.au/org/agldwg>
    a sdo:Organization ;
    sdo:name "Australian Government Linked Data Working Group" ;
    sdo:url "https://www.linked.data.gov.au"^^xsd:anyURI ;
.

<https://orcid.org/0000-0002-8742-7730>
    a sdo:Person ;
    sdo:email "nick@kurrawong.ai"^^xsd:anyURI ;
    sdo:memberOf <https://linked.data.gov.au/org/agldwg> ;
    sdo:name "Nicholas J. Car"@en ;
.

:LifecycleStage
    a owl:Class ;
    rdfs:isDefinedBy model: ;
    skos:definition "A distinct part of a resource's lifecycle"@en ;
    skos:example """
# showing lifecycle stages for a Geographical Name
ex:name-1
  a gn:GeographicalName ;
  :hasLifeCycleStage [
    # this Stage has ceased
    time:hasTime [
      time:hasBeginning [ time:inXSDDate "1982-02-10"^^xsd:date ] ;
      time:hasEnd [ time:inXSDDate "1982-05-11"^^xsd:date ] ;
    ] ;
    sdo:additionalType <http://example.com/stage/proposed> ;
  ] ,
  [
    # this Stage is still in effect - no hasEnd given
    time:hasTime [
      time:hasBeginning [ time:inXSDDate "1982-05-11"^^xsd:date ] ;
    ] ;
    sdo:additionalType <http://example.com/stage/gazetted> ;
  ] ,
."""@en ;
    skos:prefLabel "Lifecycle Stage"@en ;
.

sdo:additionalType
    a owl:ObjectProperty ;
    rdfs:domain rdfs:Resource ;
    rdfs:isDefinedBy sdo: ;
    rdfs:range rdfs:Resource ;
    skos:definition "An additional type for the item, typically used for adding more specific types from external vocabularies"@en ;
    skos:example """See the example for :LifecycleStage"""@en ;
    skos:prefLabel "additional type"@en ;
    skos:scopeNote "Use this property to indicate the specialised type of a Lifeycle Stage which is likely selected from a controlled vocabulary"@en ;
.


time:hasTime
    a owl:ObjectProperty ;
    rdfs:isDefinedBy <http://www.w3.org/2006/time> ;
    rdfs:range time:TemporalEntity ;
    skos:definition "Supports the association of a temporal entity (instant or interval) to any thing."@en ;
    skos:example "See example for LifecycleStage"@en ;
    skos:prefLabel "has time"@en ;
    skos:scopeNote "This property is defined by the Time Ontology in OWL and is a general purpose property for indicating that something has a temporality. It should be used in this model to indicate the timespan of a Lifecycle Stage" ;
.

:hasLifecycleStage
    a owl:ObjectProperty ;
    rdfs:domain rdfs:Resource ;
    rdfs:isDefinedBy model: ;
    rdfs:range :LifecycleStage ;
    skos:definition "Indicates a Lifecycle Stage of a Resource"@en ;
    skos:example "See example for LifecycleStage"@en ;
    skos:prefLabel "has Lifecycle Stage"@en ;
.
